@prefix : <https://w3id.org/energy-domain/edo#> .
@prefix dcterms: <http://purl.org/dc/terms/> .
@prefix owl: <http://www.w3.org/2002/07/owl#> .
@prefix rdf: <http://www.w3.org/1999/02/22-rdf-syntax-ns#> .
@prefix rdfs: <http://www.w3.org/2000/01/rdf-schema#> .
@prefix skos: <http://www.w3.org/2004/02/skos/core#> .
@prefix xsd: <http://www.w3.org/2001/XMLSchema#> .

dcterms:accessRights a owl:AnnotationProperty .

dcterms:description a owl:AnnotationProperty .

dcterms:identifier a owl:AnnotationProperty .

dcterms:title a owl:AnnotationProperty .

rdfs:subClassOf a owl:AnnotationProperty .

owl:maxCardinality a owl:AnnotationProperty .

owl:minCardinality a owl:AnnotationProperty .

skos:altLabel a owl:AnnotationProperty .

skos:definition a owl:AnnotationProperty .

skos:prefLabel a owl:AnnotationProperty .

<https://w3id.org/energy-domain/edo> a owl:Ontology ;
    rdfs:label "Energy Domain Ontology" ;
    dcterms:description "An ontology designed to represent the energy domain with semantic richness, supporting interoperability across engineering systems and standards (e.g., IFC, CFIHOS, ISO15926)." ;
    dcterms:title "EDO - Energy Domain Ontology" ;
    owl:versionIRI <https://w3id.org/energy-domain/edo/v0.0.1> ;
    owl:versionInfo "v0.0.1" .

:AnchoringCollar a owl:Class ;
    dcterms:identifier "AnchoringCollar" ;
    rdfs:subClassOf :SplitCollar ;
    skos:altLabel "Anchor Clamp"@en,
        "Anchoring Device"@en,
        "Fixation Collar"@en,
        "Securing Collar"@en ;
    skos:definition "A mechanical device used to stabilize and secure flexible pipes, risers, or umbilical systems to fixed structures in subsea applications. By clamping onto the outer layers of the pipe, it prevents unwanted movement during installation and operation, helping to maintain alignment and integrity under tension or compression."@en,
        "Um dispositivo mecânico usado para estabilizar e fixar dutos flexíveis ou risers a estruturas fixas em aplicações submarinas, além de dar suporte aos sistemas umbilicais. Ao se prender às camadas externas do tubo, evita movimentos indesejados durante a instalação e operação, ajudando a manter o alinhamento e a integridade sob tensão ou compressão."@pt-br ;
    skos:prefLabel "Anchoring Collar"@en,
        "Colar de Ancoragem"@pt-br ;
    :hasAttribute :AnodeCollarsAxialSpacing,
        :AnodeCollarsQuantity,
        :ClampInternalDiameter,
        :ExternalDiameter,
        :GalvanicMaterial,
        :IndividualAnodeMass,
        :MetallicStrandLength,
        :MetallicStrandSpareQuantity,
        :SafeWorkingLoad ;
    :ifc_equivalentClass "IfcPipeFitting" ;
    :ifc_objectType "AnchoringCollar" ;
    :ifc_predefinedType "USERDEFINED" .

:AnodeCollarSet a owl:Class ;
    dcterms:identifier "AnodeCollarSet" ;
    rdfs:subClassOf :SplitCollar ;
    skos:altLabel "Anode Bracket"@en,
        "Anode Clamp"@en,
        "Cathodic Protection Collar"@en ;
    skos:definition "Sacrificial anode collar set used for corrosion protection in subsea environments. It is designed to attach around pipes or risers and undergo controlled corrosion, thus protecting the metallic structures from rust and degradation. Typically made from zinc or aluminum, it ensures the longevity of subsea equipment by sacrificing itself to prevent corrosion on critical infrastructure."@en,
        "Colar de anodo sacrifical usado para proteção contra corrosão em ambientes submarinos. É projetado para ser acoplado ao redor de tubos ou risers e sofrer corrosão controlada, protegendo assim as estruturas metálicas contra ferrugem e degradação. Geralmente fabricado de zinco ou alumínio, garante a longevidade dos equipamentos submarinos ao se sacrificar para evitar a corrosão em infraestruturas críticas."@pt-br ;
    skos:prefLabel "Anode Collar Set"@en,
        "Conjunto de Colares de Anodo"@pt-br ;
    :ifc_equivalentClass "IfcPipeFitting" ;
    :ifc_objectType "AnodeCollarSet" ;
    :ifc_predefinedType "USERDEFINED" .

:AnodeSled a owl:Class ;
    dcterms:identifier "AnodeSled" ;
    rdfs:subClassOf :Structure .

:AntiCollapseSheath a owl:Class ;
    dcterms:identifier "AntiCollapseSheath" ;
    rdfs:subClassOf :SolidLayer ;
    skos:definition "Reinforcement layer in subsea flexible pipes used in oil and gas exploration, designed to prevent the collapse of the pipe under high external pressure conditions, such as those encountered in deepwater environments. Its primary role is to provide structural support against external forces that could compress or deform the pipe, particularly during situations where the internal pressure is reduced or absent, like when the pipe is emptied. Typically made from high-strength metallic or polymeric materials, the Anti Collapse Sheath ensures the integrity of the flexible pipe under extreme conditions."@en,
        "Camada de reforço em dutos flexíveis submarinos usados na exploração de petróleo e gás, projetada para evitar o colapso do duto sob altas pressões externas, como as encontradas em ambientes de águas profundas. Sua função principal é fornecer suporte estrutural contra forças externas que poderiam comprimir ou deformar o duto, especialmente durante situações em que a pressão interna é reduzida ou ausente, como quando o duto está vazio. Normalmente feita de materiais metálicos ou poliméricos de alta resistência, a Capa Anti-Colapso garante a integridade do duto flexível em condições extremas."@pt-br ;
    skos:prefLabel "Anti Collapse Sheath"@en,
        "Capa Anti-Colapso"@pt-br ;
    :ifc_equivalentClass "IfcPipeSegment" ;
    :ifc_objectType "AntiCollapseSheath" ;
    :ifc_predefinedType "USERDEFINED" .

:AntiWearSheath a owl:Class ;
    dcterms:identifier "AntiWearSheath" ;
    rdfs:subClassOf :SolidLayer ;
    skos:definition "Reinforcement layer in subsea flexible pipes used in oil and gas exploration, designed to protect the pipe from external wear and abrasion caused by contact with the seabed, equipment, or other subsea elements. Its primary role is to provide a durable protective barrier that shields the underlying layers from mechanical damage, extending the lifespan of the flexible pipe. Typically made from wear-resistant polymeric materials, the Anti Wear Sheath ensures the pipe's integrity by reducing the risk of surface damage under harsh operating conditions."@en,
        "Camada de reforço em dutos flexíveis usados na exploração de petróleo e gás, projetada para proteger o duto do desgaste externo e da abrasão causados pelo contato com o fundo marinho, equipamentos ou outros elementos submarinos. Seu papel principal é fornecer uma barreira protetora durável que protege as camadas subjacentes contra danos mecânicos, aumentando a vida útil do tubo flexível. Geralmente feita de materiais poliméricos resistentes ao desgaste, a Capa Anti-Atrito garante a integridade do duto ao reduzir o risco de danos na superfície em condições operacionais adversas."@pt-br ;
    skos:prefLabel "Anti Wear Sheath"@en,
        "Capa Anti-Atrito"@pt-br ;
    :hasAttribute :TapesQuantity ;
    :ifc_equivalentClass "IfcPipeSegment" ;
    :ifc_objectType "AntiWearSheath" ;
    :ifc_predefinedType "USERDEFINED" .

:ArchitecturalEngineering a owl:Class ;
    rdfs:label "Architectural Engineering"@en,
        "Engenharia Arquitetônica"@pt-br ;
    rdfs:subClassOf :TechnicalDiscipline ;
    skos:definition "Engineering discipline focused on building design, construction and systems integration."@en,
        "Disciplina de engenharia focada no projeto de edifícios, construção e integração de sistemas."@pt-br .

:ArmorPot a owl:Class ;
    dcterms:identifier "ArmorPot" ;
    rdfs:subClassOf :LineTermination ;
    :ifc_equivalentClass "IfcPipeFitting" ;
    :ifc_objectType "ArmorPot" ;
    :ifc_predefinedType "USERDEFINED" .

:AutomationControlEngineering a owl:Class ;
    rdfs:label "Automation & Control Engineering"@en,
        "Engenharia de Automação e Controle"@pt-br ;
    rdfs:subClassOf :TechnicalDiscipline ;
    skos:definition "Engineering discipline focused on automated control systems and process automation."@en,
        "Disciplina de engenharia focada em sistemas de controle automatizado e automação de processos."@pt-br .

:BOP a owl:Class ;
    dcterms:identifier "BOP" ;
    rdfs:subClassOf :PressureEquipment .

:BasicDesign a owl:Class ;
    rdfs:label "Basic Design"@en,
        "Projeto Básico"@pt-br ;
    rdfs:subClassOf :LifecyclePhase ;
    skos:definition "Phase where general engineering specifications, layouts, and main equipment lists are developed."@en,
        "Fase onde são desenvolvidas especificações gerais de engenharia, layouts e listas de equipamentos principais."@pt-br .

:BatchLevelAttribute a owl:Class ;
    rdfs:label "Batch Attribute"@en,
        "Atributo de Lote"@pt-br ;
    rdfs:comment "Attribute common to a batch of equipment instances."@en ;
    rdfs:subClassOf :AttributeScope ;
    skos:definition "Attribute common to a batch of equipment instances"@en,
        "Atributo comum a um lote de instâncias de equipamento"@pt-br .

:BendRestrictor a owl:Class ;
    dcterms:identifier "BendRestrictor" ;
    rdfs:subClassOf :LineAncillary ;
    skos:altLabel "Bend Limiter"@en,
        "Bending Restrictor"@en,
        "Curvature Limiter"@en ;
    skos:definition "Device used in subsea flexible pipes to limit the bending radius and prevent over-bending that could damage the pipe. Typically installed near critical areas such as connectors or end fittings, where excessive bending could compromise the structural integrity of the pipe. The Bend Restrictor consists of multiple interlocking segments that allow flexibility up to a certain radius, beyond which the segments lock to prevent further bending, protecting the pipe from deformation or failure in harsh subsea environments."@en,
        "Dispositivo usado em dutos flexíveis para limitar o raio de curvatura e evitar curvaturas excessivas que poderiam danificar o duto. Normalmente instalado perto de áreas críticas, como conectores ou acessórios finais, onde curvaturas excessivas poderiam comprometer a integridade estrutural do duto. O Restritor de Curvatura consiste em múltiplos segmentos interligados que permitem flexibilidade até um certo raio, além do qual os segmentos se bloqueiam para impedir mais curvaturas, protegendo o duto contra deformações ou falhas em ambientes submarinos adversos."@pt-br ;
    skos:prefLabel "Bend Restrictor"@en,
        "Restritor de Curvatura"@pt-br ;
    :hasAttribute :BendMomentVsShearForceTable,
        :BendMomentVsShearForceTable_BendingMoment,
        :BendMomentVsShearForceTable_Condition,
        :BendMomentVsShearForceTable_ShearForce ;
    :ifc_equivalentClass "IfcPipeFitting" ;
    :ifc_objectType "BendRestrictor" .

:Biomass a owl:Class ;
    rdfs:label "Biomass Energy"@en,
        "Energia de Biomassa"@pt-br ;
    rdfs:subClassOf :Renewable ;
    skos:definition "Energy produced from organic materials such as wood, agricultural residues, or waste."@en,
        "Energia produzida a partir de materiais orgânicos como madeira, resíduos agrícolas ou lixo."@pt-br .

:BlockValve a owl:Class ;
    dcterms:identifier "BlockValve" ;
    rdfs:subClassOf :ActuatedValve .

:BuoyancyModule a owl:Class ;
    dcterms:identifier "BuoyancyModule" ;
    rdfs:subClassOf :LineAncillary ;
    skos:altLabel "Buoyancy Element"@en,
        "Buoyancy Unit"@en,
        "Floatation Module"@en,
        "Subsea Buoyancy Module"@en ;
    skos:definition "Device used in subsea systems to provide controlled buoyancy to flexible pipes, risers, or umbilicals, reducing the load on the structure and managing the configuration of the line in the water column. The Buoyancy Module is typically composed of syntactic foam or other materials with low density, designed to withstand high external pressures while maintaining its buoyant properties over time. It plays a key role in optimizing the performance and positioning of subsea lines, ensuring they maintain the required shape and depth in dynamic ocean conditions."@en,
        "Dispositivo utilizado em sistemas submarinos para fornecer flutuabilidade controlada a dutos flexíveis, risers ou umbilicais, reduzindo a carga na estrutura e gerenciando a configuração da linha na coluna d'água. O Módulo de Flutuação é tipicamente composto por espuma sintática ou outros materiais de baixa densidade, projetados para suportar altas pressões externas enquanto mantêm suas propriedades de flutuabilidade ao longo do tempo. Ele desempenha um papel fundamental na otimização do desempenho e do posicionamento das linhas subsea, garantindo que mantenham a forma e a profundidade necessárias em condições oceânicas dinâmicas."@pt-br ;
    skos:prefLabel "Buoyancy Module"@en,
        "Módulo de Flutuação"@pt-br ;
    :hasAttribute :LongTermFloatDensity,
        :LongTermFloatVolume,
        :NominalFloatDensity,
        :NominalFloatVolume,
        :PipeMountPosition,
        :ShortTermFloatDensity,
        :ShortTermFloatVolume ;
    :ifc_equivalentClass "IfcPipeFitting" ;
    :ifc_objectType "BuoyancyModule" ;
    :ifc_predefinedType "USERDEFINED" .

:CalculatedValue a owl:Class ;
    rdfs:label "Calculated"@en,
        "Calculado"@pt-br ;
    rdfs:comment "Derived from other values."@en ;
    rdfs:subClassOf :ValueOrigin ;
    skos:definition "Derived from other values"@en,
        "Derivado de outros valores"@pt-br .

:CasingHanger a owl:Class ;
    dcterms:identifier "CasingHanger" ;
    rdfs:subClassOf :PressureComponent .

:ChainSegment a owl:Class ;
    dcterms:identifier "ChainSegment" ;
    rdfs:subClassOf :LinearObject .

:ChemicalInjectionUnit a owl:Class ;
    dcterms:identifier "ChemicalInjectionUnit" ;
    rdfs:subClassOf :TopsideEquipment .

:ChokeModule a owl:Class ;
    dcterms:identifier "ChokeModule" ;
    rdfs:subClassOf :FlowControlModule .

:ChokeValve a owl:Class ;
    dcterms:identifier "ChokeValve" ;
    rdfs:subClassOf :ActuatedValve .

:Commissioning a owl:Class ;
    rdfs:label "Commissioning"@en,
        "Comissionamento"@pt-br ;
    rdfs:subClassOf :LifecyclePhase ;
    skos:definition "Final testing and handover of the system into operational status."@en,
        "Testes finais e entrega do sistema para status operacional."@pt-br .

:CommissioningActivity a owl:Class ;
    dcterms:identifier "CommissioningActivity" ;
    rdfs:subClassOf :CommissioningObject ;
    skos:prefLabel "Commissioning Activity"@en,
        "Atividade de Comissionamento"@pt-br ;
    :hasAttribute :Planned_Start_Timestamp ;
    :ifc_equivalentClass "IfcTask" ;
    :ifc_objectType "Activity" ;
    :ifc_predefinedType "USERDEFINED" .

:CommissioningContract a owl:Class ;
    dcterms:identifier "CommissioningContract" ;
    rdfs:subClassOf :CommissioningObject ;
    skos:prefLabel "Commissioning Contract"@en,
        "Contrato de Comissionamento"@pt-br ;
    :ifc_equivalentClass "IfcGroup" ;
    :ifc_objectType "Contract" ;
    :ifc_predefinedType "USERDEFINED" .

:CommissioningDigitalProcessStep a owl:Class ;
    dcterms:identifier "CommissioningDigitalProcessStep" ;
    rdfs:subClassOf :CommissioningObject ;
    skos:prefLabel "Commissioning Digital Process Step"@en,
        "Passo do Processo Digital"@pt-br ;
    :ifc_equivalentClass "IfcTask" ;
    :ifc_objectType "CommissioningDigitalProcessStep" ;
    :ifc_predefinedType "USERDEFINED" .

:CommissioningEvidence a owl:Class ;
    dcterms:identifier "CommissioningEvidence" ;
    rdfs:subClassOf :CommissioningObject ;
    skos:prefLabel "Commissioning Evidence"@en,
        "Evidência de Comissionamento"@pt-br ;
    :ifc_equivalentClass "IfcDocumentInformation" ;
    :ifc_objectType "CommissioningEvidence" ;
    :ifc_predefinedType "USERDEFINED" .

:CommissioningIssue a owl:Class ;
    dcterms:identifier "CommissioningIssue" ;
    rdfs:subClassOf :CommissioningObject ;
    skos:prefLabel "Commissioning Issue"@en,
        "Pendência de Comissionamento"@pt-br ;
    :ifc_equivalentClass "IfcClassification" ;
    :ifc_objectType "Pendency_Classification" ;
    :ifc_predefinedType "USERDEFINED" .

:CommissioningItemCheck a owl:Class ;
    dcterms:identifier "CommissioningItemCheck" ;
    rdfs:subClassOf :CommissioningObject ;
    skos:prefLabel "Commissioning Item Check"@en,
        "Verificação de Item Comissionável"@pt-br ;
    :ifc_equivalentClass "IfcClassificationReference" ;
    :ifc_objectType "FVI" ;
    :ifc_predefinedType "USERDEFINED" .

:CommissioningLoopCheck a owl:Class ;
    dcterms:identifier "CommissioningLoopCheck" ;
    rdfs:subClassOf :CommissioningObject ;
    skos:prefLabel "Commissioning Loop Check"@en,
        "Verificação de Malha"@pt-br ;
    :ifc_equivalentClass "IfcClassificationReference" ;
    :ifc_objectType "FVM" ;
    :ifc_predefinedType "USERDEFINED" .

:CommissioningPerson a owl:Class ;
    dcterms:identifier "CommissioningPerson" ;
    rdfs:subClassOf :CommissioningObject ;
    skos:prefLabel "Commissioning Person"@en,
        "Pessoa"@pt-br ;
    :ifc_equivalentClass "IfcPerson" ;
    :ifc_objectType "CommissioningPerson" ;
    :ifc_predefinedType "USERDEFINED" .

:CommissioningPreservationOrder a owl:Class ;
    dcterms:identifier "CommissioningPreservationOrder" ;
    rdfs:subClassOf :CommissioningObject ;
    skos:prefLabel "Commissioning Preservation Order"@en,
        "Ordem de Preservação"@pt-br ;
    :ifc_equivalentClass "IfcClassificationReference" ;
    :ifc_objectType "OP" ;
    :ifc_predefinedType "USERDEFINED" .

:CommissioningProgram a owl:Class ;
    dcterms:identifier "CommissioningProgram" ;
    rdfs:subClassOf :CommissioningObject ;
    skos:prefLabel "Commissioning Program"@en,
        "Programa de Comissionamento"@pt-br ;
    :ifc_equivalentClass "IfcGroup" ;
    :ifc_objectType "Program" ;
    :ifc_predefinedType "USERDEFINED" .

:CommissioningProject a owl:Class ;
    dcterms:identifier "CommissioningProject" ;
    rdfs:subClassOf :CommissioningObject ;
    skos:prefLabel "Commissioning Project"@en,
        "Projeto de Comissionamento"@pt-br ;
    :ifc_equivalentClass "IfcProject" ;
    :ifc_objectType "Project" ;
    :ifc_predefinedType "USERDEFINED" .

:CommissioningResponsibleActor a owl:Class ;
    dcterms:identifier "CommissioningResponsibleActor" ;
    rdfs:subClassOf :CommissioningObject ;
    skos:prefLabel "Commissioning Responsible Actor"@en,
        "Ator Responsável"@pt-br ;
    :ifc_equivalentClass "IfcActor" ;
    :ifc_objectType "CommissioningResponsibleActor" ;
    :ifc_predefinedType "USERDEFINED" .

:CommissioningResponsibleGroup a owl:Class ;
    dcterms:identifier "CommissioningResponsibleGroup" ;
    rdfs:subClassOf :CommissioningObject ;
    skos:prefLabel "Commissioning Responsible Group"@en,
        "Grupo Responsável"@pt-br ;
    :ifc_equivalentClass "IfcGroup" ;
    :ifc_objectType "CommissioningResponsibleGroup" ;
    :ifc_predefinedType "USERDEFINED" .

:CommissioningTask a owl:Class ;
    dcterms:identifier "CommissioningTask" ;
    rdfs:subClassOf :CommissioningObject ;
    skos:prefLabel "Commissioning Task"@en,
        "Tarefa de Comissionamento"@pt-br ;
    :hasAttribute :Content,
        :Creator,
        :CreatorId,
        :Timestamp ;
    :ifc_equivalentClass "IfcTask" ;
    :ifc_objectType "Task" ;
    :ifc_predefinedType "USERDEFINED" .

:CompositeMaterial a owl:Class ;
    dcterms:identifier "CompositeMaterial" ;
    rdfs:subClassOf :FlexibleStructureLayerMaterial ;
    skos:definition "Material made from two or more distinct components, typically reinforcing fibers and a matrix, used in the construction of layers in flexible pipes for subsea applications. The Composite Material offers a combination of high strength, corrosion resistance, and flexibility, making it suitable for withstanding the harsh conditions of deepwater environments. Its use in flexible pipe layers enhances the pipe's structural integrity, resistance to external pressure, and durability under cyclical loading, while also reducing weight compared to traditional metallic materials."@en,
        "Material composto por dois ou mais componentes distintos, geralmente fibras de reforço e uma matriz, usado na construção de camadas em dutos flexíveis para aplicações subsea. O Material Compósito oferece uma combinação de alta resistência, resistência à corrosão e flexibilidade, tornando-o adequado para suportar as condições severas de ambientes de águas profundas. Seu uso nas camadas do duto flexível melhora a integridade estrutural do duto, resistência à pressão externa e durabilidade sob carregamento cíclico, ao mesmo tempo em que reduz o peso em comparação com materiais metálicos tradicionais."@pt-br ;
    skos:prefLabel "Composite Material"@en,
        "Material Compósito"@pt-br ;
    :hasAttribute :CompositeLayerMaterialType,
        :RuptDefAlongFibers,
        :RuptDefPerpendFibers,
        :UltTensStrAlongFibers,
        :UltTensStrPerpendFibers ;
    :ifc_equivalentClass "IfcMaterial" ;
    :ifc_objectType "CompositeMaterial" .

:ConceptualDesign a owl:Class ;
    rdfs:label "Conceptual Design"@en,
        "Projeto Conceitual"@pt-br ;
    rdfs:subClassOf :LifecyclePhase ;
    skos:definition "Initial design phase focused on feasibility, scope definition, and technology selection."@en,
        "Fase inicial de projeto focada em viabilidade, definição de escopo e seleção de tecnologia."@pt-br .

:CrossoverModule a owl:Class ;
    dcterms:identifier "CrossoverModule" ;
    rdfs:subClassOf :FlowControlModule .

:DeadweightCollar a owl:Class ;
    dcterms:identifier "DeadweightCollar" ;
    rdfs:subClassOf :SplitCollar ;
    skos:altLabel "Ballast Collar"@en,
        "Dead Weight Clamp"@en,
        "Sinking Collar"@en,
        "Weight Collar"@en ;
    skos:definition "Component used in subsea systems to provide additional weight to flexible pipes, risers, or umbilicals, ensuring proper stability and positioning on the seabed. The Deadweight Collar is designed to counteract buoyant forces, preventing unwanted movement of the pipe due to ocean currents or other environmental factors. Typically made from dense materials, it plays a crucial role in maintaining the alignment and stability of lines in dynamic environments, ensuring that the system remains securely anchored."@en,
        "Componente utilizado em sistemas submersos para fornecer peso adicional a dutos flexíveis, risers ou umbilicais, garantindo a estabilidade e o posicionamento adequados no fundo marinho. O Colar de Peso Morto é projetado para contrabalançar as forças de flutuabilidade, prevenindo o movimento indesejado do duto devido a correntes oceânicas ou outros fatores ambientais. Geralmente feito de materiais densos, ele desempenha um papel crucial na manutenção do alinhamento e da estabilidade das linhas submersas em ambientes dinâmicos, garantindo que o sistema permaneça firmemente ancorado."@pt-br ;
    skos:prefLabel "Deadweight Collar"@en,
        "Colar de Peso Morto"@pt-br ;
    :ifc_equivalentClass "IfcPipeFitting" ;
    :ifc_objectType "DeadweightCollar" ;
    :ifc_predefinedType "USERDEFINED" .

:DeclaredValue a owl:Class ;
    rdfs:label "Declared"@en,
        "Declarado"@pt-br ;
    rdfs:comment "Manually specified value."@en ;
    rdfs:subClassOf :ValueOrigin ;
    skos:definition "Manually specified value"@en,
        "Valor especificado manualmente"@pt-br .

:Decommissioning a owl:Class ;
    rdfs:label "Decommissioning"@en,
        "Descomissionamento"@pt-br ;
    rdfs:subClassOf :LifecyclePhase ;
    skos:definition "Permanent removal of the asset from service, including dismantling and disposal."@en,
        "Remoção permanente do ativo do serviço, incluindo desmontagem e descarte."@pt-br .

:DeploymentAccessory a owl:Class ;
    dcterms:identifier "DeploymentAccessory" ;
    rdfs:subClassOf :Accessory .

:DetailedDesign a owl:Class ;
    rdfs:label "Detailed Design"@en,
        "Projeto Detalhado"@pt-br ;
    rdfs:subClassOf :LifecyclePhase ;
    skos:definition "Comprehensive engineering phase producing detailed drawings, material specifications, and construction plans."@en,
        "Fase abrangente de engenharia que produz desenhos detalhados, especificações de materiais e planos de construção."@pt-br .

:DimensionalAttribute a owl:Class ;
    rdfs:label "Dimensional Attribute"@en,
        "Atributo Dimensional"@pt-br ;
    rdfs:comment "Represents measurements such as length, diameter, volume."@en ;
    rdfs:subClassOf :AttributeDomainCategory ;
    skos:definition "Represents measurements such as length, diameter, volume"@en,
        "Representa medições como comprimento, diâmetro, volume"@pt-br .

:DimensionsDrawing a owl:Class ;
    dcterms:identifier "DimensionsDrawing" ;
    rdfs:subClassOf :ReferenceDrawing ;
    skos:definition "Technical drawing providing detailed measurements, geometric specifications, and angular data of components. The Dimensions Drawing includes critical information such as length, diameter, thickness, and angles, ensuring the precise fabrication, assembly, and installation of the parts. This drawing is essential for meeting design requirements and ensuring that all components fit accurately within the overall system, supporting efficient manufacturing and quality control."@en,
        "Desenho técnico que fornece medições detalhadas, especificações geométricas e dados angulares dos componentes utilizados. O Desenho de Cotas inclui informações críticas como comprimento, diâmetro, espessura e ângulos, garantindo a fabricação, montagem e instalação precisas das peças. Esse desenho é essencial para atender aos requisitos de projeto e garantir que todos os componentes se encaixem corretamente no sistema como um todo, apoiando a fabricação eficiente e o controle de qualidade."@pt-br ;
    skos:prefLabel "Dimensions Drawing"@en,
        "Desenho de Cotas"@pt-br ;
    :ifc_equivalentClass "IfcDocumentInformation" ;
    :ifc_objectType "DimensionsDrawing" .

:DistributionConnectionPoint a owl:Class ;
    dcterms:identifier "DistributionConnectionPoint" ;
    rdfs:subClassOf :LogicalConnection ;
    skos:definition "Location in a model that indicates the specific point where fluid distribution components are connected. The Distribution Connection Point provides precise information for the assembly and installation of these components, ensuring proper alignment and functionality within the system. This point is critical for defining the interface between fluid distribution elements in subsea or other fluid-handling systems."@en,
        "Localização em um modelo que indica o ponto específico onde os componentes de distribuição de fluido são conectados. O Ponto de Conexão de Distribuição fornece informações precisas para a montagem e instalação desses componentes, garantindo o alinhamento adequado e a funcionalidade dentro do sistema. Este ponto é crucial para definir a interface entre os elementos de distribuição de fluido em sistemas submarinos ou outros sistemas de manuseio de fluido."@pt-br ;
    skos:prefLabel "Distribution Connection Point"@en,
        "Ponto de Conexão de Distribuição"@pt-br ;
    :ifc_equivalentClass "IfcDistributionPort" ;
    :ifc_objectType "DistributionConnectionPoint" ;
    :ifc_predefinedType "USERDEFINED" .

:DistributionModule a owl:Class ;
    dcterms:identifier "DistributionModule" ;
    rdfs:subClassOf :AuxiliaryModule .

:DomainAuxiliarProperty a owl:ObjectProperty .

:DomainRelationship a owl:AnnotationProperty ;
    rdfs:subPropertyOf :DomainAnnotation .

:Downstream a owl:Class ;
    rdfs:label "Downstream"@en,
        "Downstream"@pt-br ;
    rdfs:subClassOf :OilAndGas ;
    skos:definition "Oil & Gas sector covering refining, processing, distribution, and retail of petroleum products."@en,
        "Setor de Petróleo & Gás que abrange refino, processamento, distribuição e varejo de produtos petrolíferos."@pt-br .

:DragAnchor a owl:Class ;
    dcterms:identifier "DragAnchor" ;
    rdfs:subClassOf :Anchor .

:DynamicUmbilicalSpan a owl:Class ;
    dcterms:identifier "DynamicUmbilicalSpan" ;
    rdfs:subClassOf :UmbilicalSpan .

:ElectricalCable a owl:Class ;
    dcterms:identifier "ElectricalCable" ;
    rdfs:subClassOf :FunctionLine ;
    :ifc_equivalentClass "IfcCableSegment" ;
    :ifc_objectType "ElectricalCable" ;
    :ifc_predefinedType "USERDEFINED" .

:ElectricalEngineering a owl:Class ;
    rdfs:label "Electrical Engineering"@en,
        "Engenharia Elétrica"@pt-br ;
    rdfs:subClassOf :TechnicalDiscipline ;
    skos:definition "Engineering discipline focused on electrical systems, power distribution and generation."@en,
        "Disciplina de engenharia focada em sistemas elétricos, distribuição e geração de energia."@pt-br .

:ElectricalJumper a owl:Class ;
    dcterms:identifier "ElectricalJumper" ;
    rdfs:subClassOf :Jumper .

:ElectricalPowerJumper a owl:Class ;
    dcterms:identifier "ElectricalPowerJumper" ;
    rdfs:subClassOf :Jumper .

:EndFitting a owl:Class ;
    dcterms:identifier "EndFitting" ;
    rdfs:subClassOf :PipeTermination ;
    skos:altLabel "Connector Fitting"@en,
        "End Termination"@en,
        "Termination Assembly"@en,
        "Termination Fitting"@en ;
    skos:definition "Component used in subsea flexible pipes to provide a secure transition between the flexible pipe and rigid structures, such as subsea equipment or topside facilities, as well as to connect two sections of flexible pipe. The End Fitting ensures the structural integrity and sealing of the pipe, allowing for the connection of the flexible line to other equipment or sections while withstanding internal pressures and environmental forces. It is a critical interface that accommodates the pipe's mechanical, hydraulic, and thermal loads, ensuring long-term reliable performance in harsh subsea conditions."@en,
        "Componente utilizado em dutos flexíveis para fornecer uma transição segura entre o duto flexível e estruturas rígidas, como equipamentos submersos ou instalações no topo, bem como para conectar duas seções de duto flexível. O Terminador garante a integridade estrutural e o vedamento do duto, permitindo a conexão da linha flexível a outros equipamentos ou seções, resistindo a pressões internas e forças ambientais. É uma interface crítica que acomoda as cargas mecânicas, hidráulicas e térmicas do duto, garantindo desempenho confiável a longo prazo em condições submarinas adversas."@pt-br ;
    skos:prefLabel "End fitting"@en,
        "Conector de Extremidade"@pt-br ;
    :hasAttribute :BoreDiameter,
        :FlangeFaceType,
        :FlangeType,
        :HasFaceORing,
        :HasModaSensor,
        :HasN2InjectionPort,
        :RingGasketInnerDIameter,
        :RingGasketOuterDiameter,
        :RingGasketPressureRating,
        :RingGasketSpecification,
        :RingGasketStandard,
        :RingGasketType ;
    :ifc_equivalentClass "IfcPipeFitting" ;
    :ifc_objectType "EndFitting" ;
    :ifc_predefinedType "USERDEFINED" .

:EnergyStorage a owl:Class ;
    rdfs:label "Energy Storage"@en,
        "Armazenamento de Energia"@pt-br ;
    rdfs:subClassOf :Domain ;
    skos:definition "Technologies for storing energy, such as batteries, pumped hydro, or compressed air."@en,
        "Tecnologias para armazenamento de energia, como baterias, hidroelétricas reversíveis ou ar comprimido."@pt-br .

:FEED a owl:Class ;
    rdfs:label "FEED (Front-End Engineering Design)"@en,
        "FEED (Projeto Básico de Engenharia)"@pt-br ;
    rdfs:subClassOf :LifecyclePhase ;
    skos:definition "Intermediate phase between conceptual and detailed design, refining technical and cost details."@en,
        "Fase intermediária entre o projeto conceitual e detalhado, refinando detalhes técnicos e de custo."@pt-br .

:FSHRLowerAssembly a owl:Class ;
    dcterms:identifier "FSHRLowerAssembly" ;
    rdfs:subClassOf :FlowControlEquipment .

:FSHRUpperAssembly a owl:Class ;
    dcterms:identifier "FSHRUpperAssembly" ;
    rdfs:subClassOf :FlowControlEquipment .

:FabricTape a owl:Class ;
    dcterms:identifier "FabricTape" ;
    rdfs:subClassOf :TapeLayer ;
    skos:definition "Material used in subsea flexible pipe construction, typically applied as a wrapping layer to provide protection and containment for internal components. Fabric Tape is designed to secure and hold various layers of the pipe in place during manufacturing and operation, preventing displacement or damage to the underlying layers. It also adds a layer of abrasion resistance, contributing to the overall durability of the pipe in dynamic subsea environments. Made from high-strength, flexible materials, Fabric Tape plays a key role in maintaining the integrity of the flexible pipe structure."@en,
        "Material utilizado na construção de dutos flexíveis, geralmente aplicado como uma camada de envolvimento para fornecer proteção e contenção para os componentes internos. A Fita Construtiva é projetada para segurar e manter as várias camadas do duto no lugar durante a fabricação e operação, evitando o deslocamento ou danos às camadas subjacentes. Ela também adiciona uma camada de resistência à abrasão, contribuindo para a durabilidade geral do duto em ambientes dinâmicos. Feita de materiais flexíveis e de alta resistência, a Fita Construtiva desempenha um papel crucial na manutenção da integridade da estrutura do duto flexível."@pt-br ;
    skos:prefLabel "Fabric Tape"@en,
        "Fita Construtiva"@pt-br ;
    :ifc_equivalentClass "IfcPipeSegment" ;
    :ifc_objectType "FabricTape" ;
    :ifc_predefinedType "USERDEFINED" .

:Fabrication a owl:Class ;
    rdfs:label "Fabrication"@en,
        "Fabricação"@pt-br ;
    rdfs:subClassOf :LifecyclePhase ;
    skos:definition "Manufacturing and assembly of components, modules, or structures in workshops or yards."@en,
        "Fabricação e montagem de componentes, módulos ou estruturas em oficinas ou estaleiros."@pt-br .

:FiberOpticJumper a owl:Class ;
    dcterms:identifier "FiberOpticJumper" ;
    rdfs:subClassOf :LinearObject .

:FiberRopeSegment a owl:Class ;
    dcterms:identifier "FiberRopeSegment" ;
    rdfs:subClassOf :RopeSegment .

:Filler a owl:Class ;
    dcterms:identifier "Filler" ;
    rdfs:subClassOf :UmbilicalComponent .

:FinancialAttribute a owl:Class ;
    rdfs:label "Financial Attribute"@en,
        "Atributo Financeiro"@pt-br ;
    rdfs:comment "Represents costs, prices, depreciation."@en ;
    rdfs:subClassOf :AttributeDomainCategory ;
    skos:definition "Represents costs, prices, depreciation"@en,
        "Representa custos, preços, depreciação"@pt-br .

:FlexiblePipeSegment a owl:Class ;
    dcterms:identifier "FlexiblePipeSegment" ;
    rdfs:subClassOf :PipeSegment ;
    skos:altLabel "Flexible Line Section"@en,
        "Flexible Pipe Section"@en,
        "Flexible Pipe Segment"@en,
        "Subsea Pipe Segment"@en ;
    skos:definition "A segment of a flexible pipe that forms part of the overall pipeline system. The Flexible Pipe Segment is designed to transport fluids or gases over varying distances and conditions on the seafloor. Each section is engineered to handle specific environmental and operational requirements, contributing to the flexibility, durability, and performance of the subsea pipeline system."@en,
        "Um segmento de duto flexível que faz parte do sistema de pipeline geral. O Tramo Flexível é projetado para transportar fluidos ou gases por distâncias e condições variadas no fundo do mar. Cada seção é projetada para atender a requisitos ambientais e operacionais específicos, contribuindo para a flexibilidade, durabilidade e desempenho do sistema de dutos submarinos."@pt-br ;
    skos:prefLabel "Flexible Pipe Segment"@en,
        "Tramo de Duto Flexível"@pt-br ;
    :hasAttribute :AssemblyShouldObeyModelPolarity,
        :EarlyLeakMaxPressTable_Press,
        :EarlyLeakMaxPressTable_PressIntValStrat,
        :EarlyLeakMaxPressTable_PressValRef,
        :EarlyLeakMaxPressTable_PressValRefMult,
        :EarlyLeakMaxPressTable_TensLimit,
        :EarlyLeakMaxPressTable_TensLimitValRef,
        :EarlyLeakNomPressTable_Press,
        :EarlyLeakNomPressTable_PressIntValStrat,
        :EarlyLeakNomPressTable_PressValRef,
        :EarlyLeakNomPressTable_PressValRefMult,
        :EarlyLeakNomPressTable_TensLimit,
        :EarlyLeakNomPressTable_TensLimitValRef,
        :FatMaxPress,
        :FatMaxPressValRef,
        :FatMaxPressValRefMult,
        :FatNomPress,
        :FatNomPressValRef,
        :FatNomPressValRefMult,
        :IdInUnifilarDiagram,
        :ManufacturingDate,
        :ManufacturingNonConformities,
        :MaxLengthTolerance,
        :NominalLength,
        :OffLeakPLevMaxPress,
        :OffLeakPLevMaxPressValRef,
        :OffLeakPLevMaxPressValRefMult,
        :OffLeakPLevNomPress,
        :OffLeakPLevNomPressValRef,
        :OffLeakPLevNomPressValRefMult,
        :PipeSectionApplication,
        :SpecialRequirements,
        :StrIntOffPLevMaxPress,
        :StrIntOffPLevMaxPressValRef,
        :StrIntOffPLevMaxPressValRefMult,
        :StrIntOffPLevNomPress,
        :StrIntOffPLevNomPressValRef,
        :StrIntOffPLevNomPressValRefMult,
        :StrIntOnNoTensMaxPress,
        :StrIntOnNoTensMaxPressValRef,
        :StrIntOnNoTensMaxPressValRefMult,
        :StrIntOnNoTensNomPress,
        :StrIntOnNoTensNomPressValRef,
        :StrIntOnNoTensNomPressValRefMult ;
    :ifc_equivalentClass "IfcPipeSegment" ;
    :ifc_objectType "FlexiblePipeSegment" ;
    :ifc_predefinedType "USERDEFINED" .

:FlexiblePipeStructure a owl:Class ;
    dcterms:identifier "FlexiblePipeStructure" ;
    rdfs:subClassOf :DomainElement ;
    skos:altLabel "Flexible Structure"@en,
        "Subsea Flexible Configuration"@en,
        "Subsea Flexible Design"@en ;
    skos:definition "The Flexible Pipe Structure is the layered configuration of a flexible pipe, designed to provide flexibility and strength in subsea environments. It consists of multiple layers, each serving a specific function, such as pressure containment, protection, or reinforcement. This structure is engineered to handle the demands of deepwater conditions, including high pressure and dynamic movements, ensuring the pipe's integrity and performance."@en,
        "A estrutura do duto flexível é a configuração em camadas de um duto flexível, projetada para fornecer flexibilidade e resistência em ambientes subsea. Ela consiste em múltiplas camadas, cada uma servindo a uma função específica, como contenção de pressão, proteção ou reforço. Essa estrutura é projetada para atender às exigências das condições de águas profundas, incluindo alta pressão e movimentos dinâmicos, garantindo a integridade e o desempenho do duto."@pt-br ;
    skos:prefLabel "Flexible Pipe Structure"@en,
        "Estrutura de Duto Flexível"@pt-br ;
    :hasAttribute :AbsoluteInsidePressure,
        :AbsoluteOutsidePressure,
        :AxialStiffnessUnderCompressionAtSeaLevel,
        :AxialStiffnessUnderTensionAtSeaLevel,
        :BendingMomentTable_BendingMoment,
        :BendingMomentTable_Curvature,
        :CalculatedAbsoluteBurstPressure,
        :CriticalCurvatureOfSlipping,
        :DamagingPullInStraightLine,
        :DimensioningCriteria,
        :ErosionalVelocity,
        :FlexibleStructureServicesList,
        :FrictionCoefBetweenPipeAndTensioner,
        :FrictionCoefficientTighteningTable_CoefficientOfFriction,
        :FrictionCoefficientTighteningTable_TighteningPerTrack,
        :HydrostaticCollapseAbsPressDry,
        :InsideTemperature,
        :IntermediateValuesStrategy,
        :InternalDiameter,
        :LayingMinimumRadiusTable_AbsoluteExternalPressure,
        :LayingMinimumRadiusTable_AbsoluteInternalPressure,
        :LayingMinimumRadiusTable_Compression,
        :LayingMinimumRadiusTable_MinimumAllowableBendingRadius,
        :LayingMinimumRadiusTable_SectionSupportedByRigidSupport,
        :LayingMinimumRadiusTable_TensileArmourAnnulusCondition,
        :LimpTorsionalStiffnessAtSeaLevel,
        :LinearMass,
        :MaxDesignPressure,
        :MaximumAllowableTensileForStraightLine,
        :MaximumAllowableTensionTable_MaximumAllowableTensile,
        :MaximumAllowableTensionTable_PulleyRadius,
        :MaximumAllowableTensionTable_PulleyVAngle,
        :MaximumAllowableTighteningTable_AxialLoad,
        :MaximumAllowableTighteningTable_TighteningPerTrack,
        :MaximumAmbientTemperature,
        :MinimumBendingRadiusForStorage,
        :OuterDiameter,
        :OutsideTemperature,
        :PostSlippingBendingStiffness,
        :PreSlippingBendingStiffness,
        :SpoolingTension,
        :StiffTorsionalStiffnessAtSeaLevel,
        :StructureApplicationsList,
        :StructureCode,
        :TensileArmourAnnulusCondition,
        :TensileArmourFreeAnnulusVolume,
        :TensionerPadsMaterial,
        :TensionerPadsOpeningAngle,
        :TensionerPadsShape,
        :TensionerTracksQuantity,
        :TestConditions,
        :ThermalExchangeCoefficientFlooded,
        :UtilizationFactor ;
    :ifc_equivalentClass "IfcPipeSegmentType" ;
    :ifc_objectType "FlexiblePipeStructure" ;
    :ifc_predefinedType "USERDEFINED" .

:FloatingProductionUnit a owl:Class ;
    dcterms:identifier "FloatingProductionUnit" ;
    rdfs:subClassOf :Location ;
    skos:altLabel "FLNG"@en,
        "FPSO"@en,
        "FPU"@en,
        "Floating Platform"@en,
        "Floating Production Facility"@en ;
    skos:definition "Offshore platform used in oil and gas exploration and production, designed to extract, process, and store hydrocarbons. The Floating Production Unit (FPU) is anchored or moored to the seabed and can operate in deep waters, often connected to subsea wells via flexible pipes and umbilicals. It accommodates processing equipment for separating oil, gas, and water, as well as facilities for temporary storage or transfer of processed hydrocarbons to tankers or pipelines. FPUs are essential for the efficient and safe production of oil and gas in challenging offshore environments."@en,
        "Plataforma offshore usada na exploração e produção de petróleo e gás, projetada para extrair, processar e armazenar hidrocarbonetos. A Unidade de Produção Flutuante (FPU) é ancorada ou amarrada ao leito marinho e pode operar em águas profundas, frequentemente conectada a poços submarinos por meio de dutos flexíveis e umbilicais. Ela acomoda equipamentos de processamento para separação de petróleo, gás e água, bem como instalações para armazenamento temporário ou transferência de hidrocarbonetos processados para navios-tanque ou dutos. As FPUs são essenciais para a produção eficiente e segura de petróleo e gás em ambientes offshore desafiadores."@pt-br ;
    skos:prefLabel "Floating Production Unit"@en,
        "Unidade de Produção Flutuante (UEP)"@pt-br ;
    :ifc_equivalentClass "IfcBuilding" ;
    :ifc_objectType "FloatingProductionUnit" ;
    :ifc_predefinedType "USERDEFINED" .

:FlowBase a owl:Class ;
    dcterms:identifier "FlowBase" ;
    rdfs:subClassOf :FlowControlEquipment .

:FlowConnector a owl:Class ;
    dcterms:identifier "FlowConnector" ;
    rdfs:subClassOf :PressureComponent .

:FlowLineMandrel a owl:Class ;
    dcterms:identifier "FlowLineMandrel" ;
    rdfs:subClassOf :TieInEquipment .

:FlowbaseRunningTool a owl:Class ;
    dcterms:identifier "FlowbaseRunningTool" ;
    rdfs:subClassOf :RunningTool .

:FlowlineSpan a owl:Class ;
    dcterms:identifier "FlowlineSpan" ;
    rdfs:subClassOf :PipelineSpan .

:FunctionalAttribute a owl:Class ;
    rdfs:label "Functional Attribute"@en,
        "Atributo Funcional"@pt-br ;
    rdfs:comment "Describes how the equipment functions or performs its intended purpose."@en ;
    rdfs:subClassOf :AttributeDomainCategory ;
    skos:definition "Represents operational characteristics and capabilities of the equipment"@en,
        "Representa características operacionais e capacidades do equipamento"@pt-br .

:Geothermal a owl:Class ;
    rdfs:label "Geothermal Energy"@en,
        "Energia Geotérmica"@pt-br ;
    rdfs:subClassOf :Renewable ;
    skos:definition "Energy derived from heat stored beneath the Earth's surface."@en,
        "Energia derivada do calor armazenado abaixo da superfície da Terra."@pt-br .

:GroovePoint a owl:Class ;
    dcterms:identifier "GroovePoint" ;
    rdfs:subClassOf :ModelLocationPoint ;
    skos:definition "The Groove Point is a designated point on the center line of the End Fitting, used to indicate the exact position of a groove. The groove itself is a recessed area designed specifically to lock the End Fitting during onboard installation, ensuring that it remains securely in place during the process. The Groove Support Point provides a reference for locating the groove, facilitating the precise alignment and positioning required for a smooth installation."@en,
        "Ponto na linha de centro do End Fitting para indicar a posição do Groove"@pt-br ;
    skos:prefLabel "Groove Point"@en,
        "Ponto de Groove"@pt-br ;
    :hasAttribute :GrooveDiameter,
        :GrooveHeight,
        :GrooveMinimumSupportArea,
        :GrooveSupportSurfaceDiameter,
        :GrooveSupportSurfaceFilletRadius,
        :GrvCntrPntDstnceFrmTermFlange,
        :SafeWorkingLoad,
        :TechnicalNotes ;
    :ifc_equivalentClass "IfcDistributionPort" ;
    :ifc_objectType "GroovePoint" ;
    :ifc_predefinedType "USERDEFINED" .

:GroutBag a owl:Class ;
    dcterms:identifier "GroutBag" ;
    rdfs:subClassOf :PipeSupport .

:GuideBase a owl:Class ;
    dcterms:identifier "GuideBase" ;
    rdfs:subClassOf :Structure .

:HCM a owl:Class ;
    dcterms:identifier "HCM" ;
    rdfs:subClassOf :ConnectionModule .

:HCRHose a owl:Class ;
    dcterms:identifier "HCRHose" ;
    rdfs:subClassOf :Tubing ;
    skos:definition "High Collapse Resistant Hose"@en ;
    skos:prefLabel "HCR Hose"@en ;
    :ifc_equivalentClass "IfcPipeSegment" ;
    :ifc_objectType "HCRHose" ;
    :ifc_predefinedType "USERDEFINED" .

:HPHousing a owl:Class ;
    dcterms:identifier "HPHousing" ;
    rdfs:subClassOf :PressureComponent .

:HVACEngineering a owl:Class ;
    rdfs:label "HVAC Engineering"@en,
        "Engenharia de HVAC"@pt-br ;
    rdfs:subClassOf :TechnicalDiscipline ;
    skos:definition "Engineering discipline focused on heating, ventilation and air conditioning systems."@en,
        "Disciplina de engenharia focada em sistemas de aquecimento, ventilação e ar condicionado."@pt-br .

:HandlingCollar a owl:Class ;
    dcterms:identifier "HandlingCollar" ;
    rdfs:subClassOf :SplitCollar ;
    skos:altLabel "Handling Clamp"@en,
        "Installation Collar"@en,
        "Lifting Collar"@en,
        "Support Collar"@en ;
    skos:definition "Device used in subsea operations to facilitate the safe handling, lifting, and maneuvering of flexible pipes or heavy components during installation or retrieval. Typically attached around the pipe or component, it provides secure lifting points for cranes or other lifting equipment. Designed to distribute the load evenly, it prevents damage to the pipe or equipment while ensuring efficient and controlled movements in subsea environments."@en ;
    skos:prefLabel "Handling Collar"@en,
        "Colar de Manuseio"@pt-br ;
    :ifc_equivalentClass "IfcPipeFitting" ;
    :ifc_objectType "HandlingCollar" ;
    :ifc_predefinedType "USERDEFINED" .

:HangOffCollar a owl:Class ;
    dcterms:identifier "HangOffCollar" ;
    rdfs:subClassOf :LineAncillary ;
    skos:altLabel "Hang-Off Clamp"@en,
        "Hang-Off Device"@en,
        "Support Collar"@en,
        "Termination Collar"@en ;
    skos:definition "Device used to secure and support flexible pipes or risers during installation, particularly when they are suspended from a platform or vessel. It provides a stable attachment point, distributing the load and preventing excessive movement or strain on the pipe. The Hang Off Collar is crucial for maintaining the integrity of the pipe while it is held in place before final connection or during temporary suspension in subsea operations."@en ;
    skos:prefLabel "Hang Off Collar"@en,
        "Sistema de Suspensão"@pt-br ;
    :hasAttribute :CollarInternalDiameter,
        :FlangeType,
        :MaxDynamicLoad,
        :SafeWorkingLoad,
        :UpperItubeDiameter ;
    :ifc_equivalentClass "IfcPipeFitting" ;
    :ifc_objectType "HangOffCollar" ;
    :ifc_predefinedType "USERDEFINED" .

:HighStrengthTape a owl:Class ;
    dcterms:identifier "HighStrengthTape" ;
    rdfs:subClassOf :TapeLayer ;
    skos:definition "Material used in subsea flexible pipes, typically applied as a reinforcing layer to provide additional strength and resistance to external forces. High Strength Tape is designed to improve the tensile properties of the flexible pipe, enhancing its ability to withstand high internal pressures, tension, and dynamic loads in harsh subsea environments. It is typically made from advanced fibers or composite materials, ensuring durability and long-term performance in demanding conditions."@en ;
    skos:prefLabel "High Strength Tape"@en,
        "Fita de Alta Resistência"@pt-br ;
    :ifc_equivalentClass "IfcPipeSegment" ;
    :ifc_objectType "HighStrengthTape" ;
    :ifc_predefinedType "USERDEFINED" .

:HistoricalAttribute a owl:Class ;
    rdfs:label "Historical Attribute"@en,
        "Atributo Histórico"@pt-br ;
    rdfs:comment "Represents records of past events, inspections, or modifications."@en ;
    rdfs:subClassOf :AttributeDomainCategory ;
    skos:definition "Represents records of past events, inspections, or modifications"@en,
        "Representa registros de eventos passados, inspeções ou modificações"@pt-br .

:HoldingBandage a owl:Class ;
    dcterms:identifier "HoldingBandage" ;
    rdfs:subClassOf :TapeLayer ;
    skos:definition "Reinforcement layer used in subsea flexible pipes to secure and hold internal components in place during manufacturing and operation. The Holding Bandage helps maintain the alignment and stability of the various layers of the pipe, preventing displacement or movement under dynamic conditions. Typically made from high-strength, flexible materials, it contributes to the overall durability and structural integrity of the pipe, ensuring reliable performance in harsh subsea environments."@en ;
    skos:prefLabel "Holding Bandage"@en,
        "Bandagem de Reforço"@pt-br ;
    :hasAttribute :ModulusOfElasticity,
        :StressAtDesignPressure,
        :TapesQuantity ;
    :ifc_equivalentClass "IfcPipeSegment" ;
    :ifc_objectType "HoldingBandage" ;
    :ifc_predefinedType "USERDEFINED" .

:Hook a owl:Class ;
    dcterms:identifier "Hook" ;
    rdfs:subClassOf :MooringAccessory .

:Hub a owl:Class ;
    dcterms:identifier "Hub" ;
    rdfs:subClassOf :PressureComponent .

:HubBlockCap a owl:Class ;
    dcterms:identifier "HubBlockCap" ;
    rdfs:subClassOf :FlowControlModule .

:HubProtectionCap a owl:Class ;
    dcterms:identifier "HubProtectionCap" ;
    rdfs:subClassOf :Accessory .

:HydraulicJumper a owl:Class ;
    dcterms:identifier "HydraulicJumper" ;
    rdfs:subClassOf :Jumper .

:HydraulicPowerUnit a owl:Class ;
    dcterms:identifier "HydraulicPowerUnit" ;
    rdfs:subClassOf :TopsideEquipment .

:HydrogenEnergy a owl:Class ;
    rdfs:label "Hydrogen Energy"@en,
        "Energia de Hidrogênio"@pt-br ;
    rdfs:subClassOf :Domain ;
    skos:definition "Production, storage, and utilization of hydrogen as an energy carrier."@en,
        "Produção, armazenamento e utilização de hidrogênio como vetor energético."@pt-br .

:Hydropower a owl:Class ;
    rdfs:label "Hydropower"@en,
        "Energia Hidrelétrica"@pt-br ;
    rdfs:subClassOf :Renewable ;
    skos:definition "Energy generated from moving water, including dams and tidal power."@en,
        "Energia gerada a partir da água em movimento, incluindo barragens e energia das marés."@pt-br .

:IMUX a owl:Class ;
    dcterms:identifier "IMUX" ;
    rdfs:subClassOf :ElectronicDevice .

:ITube a owl:Class ;
    dcterms:identifier "ITube" ;
    rdfs:subClassOf :RiserSupport .

:IdentificationAttribute a owl:Class ;
    rdfs:label "Identification Attribute"@en,
        "Atributo de Identificação"@pt-br ;
    rdfs:comment "Represents identifiers, codes, names."@en ;
    rdfs:subClassOf :AttributeDomainCategory ;
    skos:definition "Represents identifiers, codes, names"@en,
        "Representa identificadores, códigos, nomes"@pt-br .

:ImportedValue a owl:Class ;
    rdfs:label "Imported"@en,
        "Importado"@pt-br ;
    rdfs:comment "Imported from another system."@en ;
    rdfs:subClassOf :ValueOrigin ;
    skos:definition "Imported from another system"@en,
        "Importado de outro sistema"@pt-br .

:InlineT a owl:Class ;
    dcterms:identifier "InlineT" ;
    rdfs:subClassOf :FlowControlEquipment .

:InlineValve a owl:Class ;
    dcterms:identifier "InlineValve" ;
    rdfs:subClassOf :FlowControlEquipment .

:InlineY a owl:Class ;
    dcterms:identifier "InlineY" ;
    rdfs:subClassOf :FlowControlEquipment .

:InnerTube a owl:Class ;
    dcterms:identifier "InnerTube" ;
    rdfs:subClassOf :SolidLayer ;
    skos:definition "The Inner Tube is the innermost layer of a subsea flexible pipe, responsible for containing and transporting the fluid, such as oil or gas. It is designed to withstand internal pressures and prevent fluid leakage while offering resistance to the corrosive and abrasive nature of the transported substances. The Inner Tube is typically made from high-performance polymeric materials that ensure durability, flexibility, and chemical resistance, making it a critical component in maintaining the integrity of the flexible pipe in subsea operations."@en ;
    skos:prefLabel "Inner Tube"@en,
        "Tubo Interno"@pt-br ;
    :ifc_equivalentClass "IfcPipeSegment" ;
    :ifc_objectType "InnerTube" ;
    :ifc_predefinedType "USERDEFINED" .

:Installation a owl:Class ;
    rdfs:label "Installation"@en,
        "Instalação"@pt-br ;
    rdfs:subClassOf :LifecyclePhase ;
    skos:definition "Placement and integration of equipment, piping, and structures at the site."@en,
        "Posicionamento e integração de equipamentos, tubulações e estruturas no local."@pt-br .

:InstrumentationEngineering a owl:Class ;
    rdfs:label "Instrumentation Engineering"@en,
        "Engenharia de Instrumentação"@pt-br ;
    rdfs:subClassOf :TechnicalDiscipline ;
    skos:definition "Engineering discipline focused on measurement and control instrumentation systems."@en,
        "Disciplina de engenharia focada em sistemas de instrumentação de medição e controle."@pt-br .

:InsulationTape a owl:Class ;
    dcterms:identifier "InsulationTape" ;
    rdfs:subClassOf :TapeLayer ;
    skos:definition "Material used in subsea flexible pipes to provide thermal insulation, ensuring that the temperature of the transported fluids remains stable during flow. Insulation Tape is applied in layers around the pipe to minimize heat loss or gain, which is critical for maintaining the fluid's properties, such as viscosity, in deepwater environments. It is typically made from materials with low thermal conductivity, such as polymers or composites, and is essential for enhancing the efficiency and performance of subsea pipelines in harsh temperature conditions."@en ;
    skos:prefLabel "Insulation Tape"@en,
        "Fita de Isolamento"@pt-br ;
    :ifc_equivalentClass "IfcPipeSegment" ;
    :ifc_objectType "InsulationTape" ;
    :ifc_predefinedType "USERDEFINED" .

:IntegratedPipe a owl:Class ;
    dcterms:identifier "IntegratedPipe" ;
    rdfs:subClassOf :Tubing ;
    :ifc_equivalentClass "IfcPipeSegment" ;
    :ifc_objectType "IntegratedPipe" ;
    :ifc_predefinedType "USERDEFINED" .

:InterlockedCarcass a owl:Class ;
    dcterms:identifier "InterlockedCarcass" ;
    rdfs:subClassOf :CarcassLayer ;
    skos:definition "The Interlocked Carcass is a metallic layer used in certain subsea flexible pipes to provide internal pressure resistance and prevent collapse. It is designed with interlocking metal strips that offer high strength while maintaining flexibility. This layer enhances the structural integrity of the flexible pipe, protecting it from external pressures and harsh subsea conditions. The Interlocked Carcass allows the pipe to bend without losing its shape or collapsing under deepwater pressure."@en ;
    skos:prefLabel "Interlocked Carcass"@en,
        "Carcaça"@pt-br ;
    :ifc_equivalentClass "IfcPipeSegment" ;
    :ifc_objectType "InterlockedCarcass" ;
    :ifc_predefinedType "USERDEFINED" .

:IntermediateBendStiffener a owl:Class ;
    dcterms:identifier "IntermediateBendStiffener" ;
    rdfs:subClassOf :BendStiffener ;
    skos:altLabel "Curvature Stiffener"@en,
        "Intermediate Bending Stiffener"@en,
        "Stiffener"@en ;
    skos:definition "A device used in subsea flexible pipes to provide localized stiffness at specific points along the length of the pipe, preventing excessive bending and reducing stress concentration. The Intermediate Bend Stiffener is typically installed between critical areas to ensure that the pipe maintains a controlled bending radius, protecting it from over-flexing or fatigue. Made from durable materials, it helps prolong the service life of the flexible pipe by distributing loads more evenly and reducing the risk of damage in dynamic subsea environments."@en,
        "Dispositivo usado em tubos flexíveis submarinos para fornecer rigidez localizada em pontos específicos ao longo do comprimento do tubo, evitando dobras excessivas e reduzindo a concentração de tensões. O Enrijecedor de Curvatura Intermediário é tipicamente instalado entre áreas críticas para garantir que o tubo mantenha um raio de curvatura controlado, protegendo-o contra flexões excessivas ou fadiga. Feito de materiais duráveis, ajuda a prolongar a vida útil do tubo flexível, distribuindo as cargas de forma mais uniforme e reduzindo o risco de danos em ambientes submarinos dinâmicos."@pt-br ;
    skos:prefLabel "Intermediate Bend Stiffener"@en,
        "Enrijecedor de Curvatura Intermediário"@pt-br ;
    :ifc_equivalentClass "IfcPipeFitting" ;
    :ifc_objectType "IntermediateBendStiffener" .

:IntermediateSheath a owl:Class ;
    dcterms:identifier "IntermediateSheath" ;
    rdfs:subClassOf :SolidLayer ;
    skos:definition "A protective layer within a subsea flexible pipe, positioned between other structural layers to provide additional protection and separation. The Intermediate Sheath serves to isolate different layers, preventing abrasion, wear, or interaction that could compromise the integrity of the pipe. Typically made from polymeric materials, this sheath also contributes to the overall durability and flexibility of the pipe, ensuring it can withstand the dynamic conditions of subsea environments while maintaining the performance of the internal and external layers."@en ;
    skos:prefLabel "Intermediate Sheath"@en,
        "Barreira Intermediária de Vedação"@pt-br ;
    :ifc_equivalentClass "IfcPipeSegment" ;
    :ifc_objectType "IntermediateSheath" ;
    :ifc_predefinedType "USERDEFINED" .

:InternalPressureSheath a owl:Class ;
    dcterms:identifier "InternalPressureSheath" ;
    rdfs:subClassOf :SolidLayer ;
    skos:definition "A layer within a subsea flexible pipe designed to contain the internal fluid and withstand the internal pressure exerted by the transported medium, such as oil, gas, or water. The Internal Pressure Sheath plays a crucial role in preventing fluid leakage and maintaining pressure integrity within the pipe. Typically made from high-performance polymeric materials, it ensures the safe transport of fluids under high-pressure conditions, contributing to the pipe's overall structural stability and long-term reliability in harsh subsea environments."@en ;
    skos:prefLabel "Internal Pressure Sheath"@en,
        "Barreira Interna de Pressão"@pt-br ;
    :ifc_equivalentClass "IfcPipeSegment" ;
    :ifc_objectType "InternalPressureSheath" ;
    :ifc_predefinedType "USERDEFINED" .

:LPHousing a owl:Class ;
    dcterms:identifier "LPHousing" ;
    rdfs:subClassOf :PressureComponent .

:LogicCap a owl:Class ;
    dcterms:identifier "LogicCap" ;
    rdfs:subClassOf :AuxiliaryModule .

:LowResistanceTape a owl:Class ;
    dcterms:identifier "LowResistanceTape" ;
    rdfs:subClassOf :TapeLayer ;
    skos:definition "A layer used in subsea flexible pipes to reduce friction between different components or layers, enhancing the overall flexibility and durability of the pipe. The Low Resistance Tape minimizes wear and abrasion caused by the movement of adjacent layers during operation, particularly in dynamic subsea conditions. Made from materials with low friction properties, it helps extend the lifespan of the pipe by reducing internal stresses and preventing damage to critical layers, ensuring smooth and efficient operation under harsh underwater conditions."@en ;
    skos:prefLabel "Low Resistance Tape"@en,
        "Fita de Baixa Resistência"@pt-br ;
    :ifc_equivalentClass "IfcPipeSegment" ;
    :ifc_objectType "LowResistanceTape" ;
    :ifc_predefinedType "USERDEFINED" .

:Maintenance a owl:Class ;
    rdfs:label "Maintenance"@en,
        "Manutenção"@pt-br ;
    rdfs:subClassOf :LifecyclePhase ;
    skos:definition "Planned or corrective interventions to preserve asset functionality and safety."@en,
        "Intervenções planejadas ou corretivas para preservar a funcionalidade e segurança do ativo."@pt-br .

:MasterControlStation a owl:Class ;
    dcterms:identifier "MasterControlStation" ;
    rdfs:subClassOf :TopsideEquipment .

:Mattress a owl:Class ;
    dcterms:identifier "Mattress" ;
    rdfs:subClassOf :PipeSupport .

:MeasuredValue a owl:Class ;
    rdfs:label "Measured"@en,
        "Medido"@pt-br ;
    rdfs:comment "Obtained by direct measurement."@en ;
    rdfs:subClassOf :ValueOrigin ;
    skos:definition "Obtained by direct measurement"@en,
        "Obtido por medição direta"@pt-br .

:MetallicMaterial a owl:Class ;
    dcterms:identifier "MetallicMaterial" ;
    rdfs:subClassOf :FlexibleStructureLayerMaterial ;
    skos:definition "Material used in the fabrication of metallic layers in subsea flexible pipes, chosen for its strength, durability, and resistance to harsh environmental conditions. The Metallic Material provides structural reinforcement, enhances pressure resistance, and supports the pipe's overall integrity. Commonly used materials include stainless steel, carbon steel, or other corrosion-resistant alloys, which are selected based on their ability to withstand the operational demands of deepwater environments, such as high pressure, tension, and dynamic loading."@en ;
    skos:prefLabel "Metallic Material"@en,
        "Material Metálico"@pt-br ;
    :hasAttribute :FractureToughness,
        :MetallicLayerMaterialType,
        :UltimateTensileStress ;
    :ifc_equivalentClass "IfcMaterial" ;
    :ifc_objectType "MetallicMaterial" .

:MetallicStrandSet a owl:Class ;
    dcterms:identifier "MetallicStrandSet" ;
    rdfs:subClassOf :PhysicalConnection ;
    skos:definition "Galvanic connection cables set providing reliable electrical link between anodes and metal infrastructure for effective corrosion mitigation."@en ;
    skos:prefLabel "Metallic Strand Set"@en,
        "Conjunto de Cordoalhas de Continuidade"@pt-br ;
    :hasAttribute :StrandsTable_SpareQuantity,
        :StrandsTable_StrandsLength,
        :StrandsTable_StrandsQuantity ;
    :ifc_equivalentClass "IfcCableSegment" ;
    :ifc_objectType "MetallicStrandSet" ;
    :ifc_predefinedType "USERDEFINED" .

:MetallicTubing a owl:Class ;
    dcterms:identifier "MetallicTubing" ;
    rdfs:subClassOf :Tubing ;
    :ifc_equivalentClass "IfcPipeSegment" ;
    :ifc_objectType "MetallicTubing" ;
    :ifc_predefinedType "USERDEFINED" .

:MetricBoltSet a owl:Class ;
    dcterms:identifier "MetricBoltSet" ;
    rdfs:subClassOf :BoltSet ;
    skos:definition "A set of bolts and accompanying hardware sized using the metric measurement system, commonly used in subsea applications for international compatibility and standardization."@en ;
    skos:prefLabel "Metric Bolt Set"@en,
        "Conjunto de Parafusos Métrico"@pt-br ;
    :hasAttribute :NominalDiameter,
        :PitchToleranceClass,
        :ThreadPitch,
        :ThreadStandard ;
    :ifc_equivalentClass "IfcMechanicalFastener" ;
    :ifc_objectType "MetricBoltSet" ;
    :ifc_predefinedType "USERDEFINED" .

:MetricStudSet a owl:Class ;
    dcterms:identifier "MetricStudSet" ;
    rdfs:subClassOf :StudSet ;
    skos:altLabel "Metric Stud"@en,
        "Metric Threaded Rod"@en ;
    skos:definition "Metric studs are crucial fastening components for subsea oil and gas components, designed specifically to secure equipment parts. Each set includes bolts, nuts, and washers in metric sizing, made from high-strength, corrosion-resistant materials to withstand the demanding subsea environment. These components offer dependable fastening, ensuring structural integrity and leak prevention in end fittings. Metric stud sets are engineered to endure high pressure and extreme temperatures, making them essential for the safety and durability of subsea interconnections."@en ;
    skos:prefLabel "Metric Stud Set"@en,
        "Conjunto de Estojos Métrico"@pt-br ;
    :hasAttribute :PitchToleranceClass,
        :ThreadPitch,
        :ThreadStandard ;
    :ifc_equivalentClass "IfcMechanicalFastener" ;
    :ifc_objectType "MetricStudSet" ;
    :ifc_predefinedType "USERDEFINED" .

:Midstream a owl:Class ;
    rdfs:label "Midstream"@en,
        "Midstream"@pt-br ;
    rdfs:subClassOf :OilAndGas ;
    skos:definition "Oil & Gas sector covering transportation, storage, and wholesale marketing of crude or refined petroleum products."@en,
        "Setor de Petróleo & Gás que abrange transporte, armazenamento e comercialização atacadista de produtos petrolíferos brutos ou refinados."@pt-br .

:NuclearFuelCycle a owl:Class ;
    rdfs:label "Nuclear Fuel Cycle"@en,
        "Ciclo do Combustível Nuclear"@pt-br ;
    rdfs:subClassOf :Nuclear ;
    skos:definition "Processes involved in mining, processing, enrichment, and disposal of nuclear fuel."@en,
        "Processos envolvidos na mineração, processamento, enriquecimento e descarte de combustível nuclear."@pt-br .

:NuclearPowerGeneration a owl:Class ;
    rdfs:label "Nuclear Power Generation"@en,
        "Geração de Energia Nuclear"@pt-br ;
    rdfs:subClassOf :Nuclear ;
    skos:definition "Operation and maintenance of nuclear power plants for electricity production."@en,
        "Operação e manutenção de usinas nucleares para produção de eletricidade."@pt-br .

:Offshore a owl:Class ;
    rdfs:label "Offshore"@en,
        "Offshore"@pt-br ;
    rdfs:subClassOf :LocationType ;
    skos:definition "Industrial activities conducted at sea, typically for oil & gas or wind energy production."@en,
        "Atividades industriais realizadas no mar, tipicamente para produção de petróleo & gás ou energia eólica."@pt-br .

:Onshore a owl:Class ;
    rdfs:label "Onshore"@en,
        "Onshore"@pt-br ;
    rdfs:subClassOf :LocationType ;
    skos:definition "Industrial activities conducted on land."@en,
        "Atividades industriais realizadas em terra."@pt-br .

:OpenReceptacle a owl:Class ;
    dcterms:identifier "OpenReceptacle" ;
    rdfs:subClassOf :RiserSupport .

:Operation a owl:Class ;
    rdfs:label "Operation"@en,
        "Operação"@pt-br ;
    rdfs:subClassOf :LifecyclePhase ;
    skos:definition "Normal use of the asset for its intended purpose, including monitoring and control."@en,
        "Uso normal do ativo para seu propósito pretendido, incluindo monitoramento e controle."@pt-br .

:OpticalFiberCable a owl:Class ;
    dcterms:identifier "OpticalFiberCable" ;
    rdfs:subClassOf :FunctionLine ;
    :ifc_equivalentClass "IfcCableSegment" ;
    :ifc_objectType "OpticalFiberCable" ;
    :ifc_predefinedType "USERDEFINED" .

:OverrideTool a owl:Class ;
    dcterms:identifier "OverrideTool" ;
    rdfs:subClassOf :ROVTool .

:PLEM a owl:Class ;
    dcterms:identifier "PLEM" ;
    rdfs:subClassOf :Manifold .

:PLET a owl:Class ;
    dcterms:identifier "PLET" ;
    rdfs:subClassOf :FlowControlEquipment .

:PackageEquipmentEngineering a owl:Class ;
    rdfs:label "Package Equipment Engineering"@en,
        "Engenharia de Equipamentos Modulares"@pt-br ;
    rdfs:subClassOf :EquipmentEngineering ;
    skos:definition "Engineering of skid-mounted or modular equipment systems."@en,
        "Engenharia de sistemas de equipamentos modulares ou montados em skids."@pt-br .

:PerformanceAttribute a owl:Class ;
    rdfs:label "Performance Attribute"@en,
        "Atributo de Desempenho"@pt-br ;
    rdfs:comment "Represents performance or capacity values such as pressure rating or power."@en ;
    rdfs:subClassOf :AttributeDomainCategory ;
    skos:definition "Represents performance or capacity values such as pressure rating or power"@en,
        "Representa valores de desempenho ou capacidade como pressão nominal ou potência"@pt-br .

:PhysicalPropertyAttribute a owl:Class ;
    rdfs:label "Physical Property Attribute"@en,
        "Atributo de Propriedade Física"@pt-br ;
    rdfs:comment "Represents intrinsic physical properties such as mass, density, material."@en ;
    rdfs:subClassOf :AttributeDomainCategory ;
    skos:definition "Represents intrinsic physical properties such as mass, density, material"@en,
        "Representa propriedades físicas intrínsecas como massa, densidade, material"@pt-br .

:PipeMechanicalSupport a owl:Class ;
    dcterms:identifier "PipeMechanicalSupport" ;
    rdfs:subClassOf :PipeSupport .

:PipePullingHead a owl:Class ;
    dcterms:identifier "PipePullingHead" ;
    rdfs:subClassOf :PullingHead ;
    skos:altLabel "Cable Head"@en,
        "Installation Head"@en,
        "Pull Head"@en,
        "Pulling Grip"@en,
        "Pulling Tool"@en ;
    skos:definition "A component used in subsea flexible pipe installations to provide a secure attachment point for pulling the pipe into position during installation or retrieval operations. The Pulling Head is fitted to the end of the flexible pipe, allowing connection to pulling equipment such as winches or cranes. It is designed to withstand high loads, ensuring that the pipe can be pulled safely without causing damage. The Pulling Head is essential for handling, testing, and securing the pipe in place during subsea installation."@en ;
    skos:prefLabel "Pipe Pulling Head"@en,
        "Cabeça de Tração do Duto"@pt-br ;
    :hasAttribute :FlangeType,
        :PullingHeadType,
        :RingGasketInnerDIameter,
        :RingGasketMaterial,
        :RingGasketOuterDiameter,
        :RingGasketPressureRating,
        :RingGasketSpecification,
        :RingGasketStandard,
        :RingGasketType,
        :SafeWorkingLoad ;
    :ifc_equivalentClass "IfcPipeFitting" ;
    :ifc_objectType "PipePullingHead" ;
    :ifc_predefinedType "USERDEFINED" .

:PipingSpool a owl:Class ;
    dcterms:identifier "PipingSpool" ;
    rdfs:subClassOf :PressureComponent .

:PlasticHose a owl:Class ;
    dcterms:identifier "PlasticHose" ;
    rdfs:subClassOf :Tubing ;
    skos:prefLabel "Plastic Hose"@en ;
    :ifc_equivalentClass "IfcPipeSegment" ;
    :ifc_objectType "PlasticHose" ;
    :ifc_predefinedType "USERDEFINED" .

:PolymericMaterial a owl:Class ;
    dcterms:identifier "PolymericMaterial" ;
    rdfs:subClassOf :FlexibleStructureLayerMaterial ;
    skos:definition "Material made from polymers, used to fabricate flexible layers in subsea flexible pipes. Polymeric Material is selected for its properties such as flexibility, chemical resistance, and durability, making it suitable for withstanding the harsh conditions of subsea environments. These materials are commonly used in layers that provide insulation, protection, or pressure containment, ensuring the overall performance and integrity of the flexible pipe under dynamic loads and extreme underwater conditions."@en ;
    skos:prefLabel "Polymeric Material"@en,
        "Material Polimérico"@pt-br ;
    :hasAttribute :DiffusionTable,
        :DiffusionTable_DiffusionCoefficient,
        :DiffusionTable_MoleculeIdentifier,
        :DiffusionTable_PolymerState,
        :DiffusionTable_Temperature,
        :EModVsTempTable_ElasticityModulus,
        :MaxPermissibleDeformationDynamic,
        :MaxPermissibleDeformationStatic,
        :MinimumTemperature,
        :PermeabilityTable,
        :PermeabilityTable_MoleculeIdentifier,
        :PermeabilityTable_PermeabilityCoefficient,
        :PermeabilityTable_PolymerState,
        :PermeabilityTable_Temperature,
        :PolymericLayerMaterialType,
        :SolubilityTable,
        :SolubilityTable_MoleculeIdentifier,
        :SolubilityTable_PolymerState,
        :SolubilityTable_SolubilityCoefficient,
        :SolubilityTable_Temperature ;
    :ifc_equivalentClass "IfcMaterial" ;
    :ifc_objectType "PolymericMaterial" .

:PreCommissioning a owl:Class ;
    rdfs:label "Pre-Commissioning"@en,
        "Pré-Comissionamento"@pt-br ;
    rdfs:subClassOf :LifecyclePhase ;
    skos:definition "Verification and functional testing before introducing operational fluids or energy."@en,
        "Verificação e testes funcionais antes da introdução de fluidos ou energia operacionais."@pt-br .

:PressureArmour a owl:Class ;
    dcterms:identifier "PressureArmour" ;
    rdfs:subClassOf :CarcassLayer ;
    skos:definition "A high-strength, metallic layer used in subsea flexible pipes to provide resistance against both internal and external pressure. The Pressure Armour prevents the pipe from expanding under high internal pressures and protects against collapse due to external pressure. Typically made from helically wound steel or other strong materials, it supports the pipe's structural integrity and ensures reliable operation in harsh subsea environments."@en ;
    skos:prefLabel "Pressure Armour"@en,
        "Armadura de Pressão"@pt-br ;
    :ifc_equivalentClass "IfcPipeSegment" ;
    :ifc_objectType "PressureArmour" ;
    :ifc_predefinedType "USERDEFINED" .

:PressureSensor a owl:Class ;
    dcterms:identifier "PressureSensor" ;
    rdfs:subClassOf :Sensor .

:ProcessEngineering a owl:Class ;
    rdfs:label "Process Engineering"@en,
        "Engenharia de Processos"@pt-br ;
    rdfs:subClassOf :TechnicalDiscipline ;
    skos:definition "Engineering discipline focused on the design and optimization of industrial processes."@en,
        "Disciplina de engenharia focada no projeto e otimização de processos industriais."@pt-br .

:ProcessPipingEngineering a owl:Class ;
    rdfs:label "Process Piping Engineering"@en,
        "Engenharia de Tubulação de Processo"@pt-br ;
    rdfs:subClassOf :TechnicalDiscipline ;
    skos:definition "Engineering discipline focused on the design of piping systems for process fluids."@en,
        "Disciplina de engenharia focada no projeto de sistemas de tubulação para fluidos de processo."@pt-br .

:Procurement a owl:Class ;
    rdfs:label "Procurement"@en,
        "Aquisição"@pt-br ;
    rdfs:subClassOf :LifecyclePhase ;
    skos:definition "Acquisition of materials, equipment, and services required for project execution."@en,
        "Aquisição de materiais, equipamentos e serviços necessários para execução do projeto."@pt-br .

:Project a owl:Class ;
    dcterms:identifier "Project" ;
    rdfs:subClassOf :DomainElement ;
    skos:definition "A broad concept that encompasses the design, development, and planning of various components or systems."@en ;
    skos:prefLabel "Project"@en,
        "Projeto"@pt-br ;
    :ifc_equivalentClass "IfcProject" .

:ProtectiveSheath a owl:Class ;
    dcterms:identifier "ProtectiveSheath" ;
    rdfs:subClassOf :SolidLayer ;
    skos:definition "A layer in subsea flexible pipes designed to shield internal components from external environmental factors such as abrasion, mechanical damage, or chemical exposure. The Protective Sheath serves as the outermost barrier, providing defense against harsh subsea conditions while preserving the integrity of the underlying layers. Typically made from durable polymeric materials, it plays a critical role in extending the lifespan of the flexible pipe by protecting it from physical and chemical wear."@en ;
    skos:prefLabel "Protective Sheath"@en,
        "Capa de Proteção"@pt-br ;
    :ifc_equivalentClass "IfcPipeSegment" ;
    :ifc_objectType "ProtectiveSheath" ;
    :ifc_predefinedType "USERDEFINED" .

:PullInCollar a owl:Class ;
    dcterms:identifier "PullInCollar" ;
    rdfs:subClassOf :SplitCollar ;
    skos:altLabel "Installation Collar"@en,
        "Pull-In Clamp"@en,
        "Pulling Collar"@en,
        "Tension Collar"@en ;
    skos:definition "A device used in subsea operations to assist in the installation of flexible pipes or risers by providing a secure attachment point for pulling the pipe into position. The Pull In Collar is typically installed around the pipe and serves as a handling point for pulling equipment during installation. It ensures a controlled and secure method of pulling the pipe into place, preventing damage to the pipe while facilitating smooth and efficient installation in subsea environments."@en ;
    skos:prefLabel "Pull In Collar"@en,
        "Colar de Pull In"@pt-br ;
    :hasAttribute :WireRopeQuantity,
        :WireRopeSlingDiameter,
        :WireRopeSlingLength ;
    :ifc_equivalentClass "IfcPipeFitting" ;
    :ifc_objectType "PullInCollar" ;
    :ifc_predefinedType "USERDEFINED" .

:Pump a owl:Class ;
    dcterms:identifier "Pump" ;
    rdfs:subClassOf :RotatingMachine .

:PumpingModule a owl:Class ;
    dcterms:identifier "PumpingModule" ;
    rdfs:subClassOf :ProcessingModule .

:QuickDisconnectionTool a owl:Class ;
    dcterms:identifier "QuickDisconnectionTool" ;
    rdfs:subClassOf :RunningTool .

:Recycling a owl:Class ;
    rdfs:label "Recycling"@en,
        "Reciclagem"@pt-br ;
    rdfs:subClassOf :LifecyclePhase ;
    skos:definition "Processing and reusing materials recovered during decommissioning."@en,
        "Processamento e reutilização de materiais recuperados durante o descomissionamento."@pt-br .

:ReliefValve a owl:Class ;
    dcterms:identifier "ReliefValve" ;
    rdfs:subClassOf :CheckValve .

:RigidJumper a owl:Class ;
    dcterms:identifier "RigidJumper" ;
    rdfs:subClassOf :TieInEquipment .

:RingGasket a owl:Class ;
    dcterms:identifier "RingGasket" ;
    rdfs:subClassOf :PhysicalConnection ;
    skos:altLabel " Seal Ring"@en,
        "Gasket"@en,
        "O-Ring"@en,
        "Packing Ring"@en,
        "Seal Gasket"@en,
        "Sealing Ring"@en ;
    skos:definition "The seal ring is a crucial component used in subsea oil and gas interconnection end fittings to ensure a secure and leak-proof connection between pipes or equipment. Typically made from high-performance materials such as elastomers or metals, the seal ring is designed to withstand extreme pressure, temperature, and environmental conditions found in subsea operations. It is installed within the end fitting to create a reliable seal that prevents fluid leakage and maintains the integrity of the interconnection. The seal ring’s precise design and material selection are essential for ensuring long-term durability and performance in harsh subsea environments."@en ;
    skos:prefLabel "Ring Gasket"@en,
        "Junta de Conexão"@pt-br ;
    :hasAttribute :RingGasketInnerDIameter,
        :RingGasketMaterial,
        :RingGasketOuterDiameter,
        :RingGasketPressureRating,
        :RingGasketSpecification,
        :RingGasketStandard,
        :RingGasketType ;
    :ifc_equivalentClass "IfcMechanicalFastener" ;
    :ifc_objectType "RingGasket" ;
    :ifc_predefinedType "USERDEFINED" .

:RiserBalcony a owl:Class ;
    dcterms:identifier "RiserBalcony" ;
    rdfs:subClassOf :Location ;
    skos:definition "Installation location for supports and accessories on the riser balcony of the production unit."@en ;
    skos:prefLabel "Riser Balcony"@en,
        "Plataforma do Riser"@pt-br .

:RiserSpan a owl:Class ;
    dcterms:identifier "RiserSpan" ;
    rdfs:subClassOf :PipelineSpan .

:RiserSupportBuoy a owl:Class ;
    dcterms:identifier "RiserSupportBuoy" ;
    rdfs:subClassOf :BuoyancyTank .

:RoboticActuator a owl:Class ;
    dcterms:identifier "RoboticActuator" ;
    rdfs:subClassOf :AuxiliaryModule .

:RotatingEquipmentEngineering a owl:Class ;
    rdfs:label "Rotating Equipment Engineering"@en,
        "Engenharia de Equipamentos Rotativos"@pt-br ;
    rdfs:subClassOf :EquipmentEngineering ;
    skos:definition "Engineering of mechanical equipment with rotating components such as pumps, compressors, and turbines."@en,
        "Engenharia de equipamentos mecânicos com componentes rotativos como bombas, compressores e turbinas."@pt-br .

:SCM a owl:Class ;
    dcterms:identifier "SCM" ;
    rdfs:subClassOf :AuxiliaryModule .

:SCMMB a owl:Class ;
    dcterms:identifier "SCMMB" ;
    rdfs:subClassOf :AuxiliaryModule .

:SCMRunningTool a owl:Class ;
    dcterms:identifier "SCMRunningTool" ;
    rdfs:subClassOf :RunningTool .

:SDU a owl:Class ;
    dcterms:identifier "SDU" ;
    rdfs:subClassOf :SubseaEquipment .

:SEM a owl:Class ;
    dcterms:identifier "SEM" ;
    rdfs:subClassOf :ElectronicDevice .

:SacrificialSheath a owl:Class ;
    dcterms:identifier "SacrificialSheath" ;
    rdfs:subClassOf :SolidLayer ;
    skos:definition "A protective layer in subsea flexible pipes designed to absorb damage from external environmental factors, such as abrasion or impact, over time. The Sacrificial Sheath is intended to wear out or degrade under harsh conditions, thereby preserving the integrity of the underlying layers and prolonging the overall lifespan of the pipe. Made from durable materials, this sheath acts as the first line of defense, allowing for the controlled degradation of the pipe's outer surface without affecting its core structural or functional performance."@en ;
    skos:prefLabel "Sacrificial Sheath"@en,
        "Camada de Sacrifício"@pt-br ;
    :ifc_equivalentClass "IfcPipeSegment" ;
    :ifc_objectType "SacrificialSheath" ;
    :ifc_predefinedType "USERDEFINED" .

:SafetyLossPreventionEngineering a owl:Class ;
    rdfs:label "Safety & Loss Prevention Engineering"@en,
        "Engenharia de Segurança e Prevenção de Perdas"@pt-br ;
    rdfs:subClassOf :TechnicalDiscipline ;
    skos:definition "Engineering discipline focused on risk assessment, safety systems and loss prevention."@en,
        "Disciplina de engenharia focada em avaliação de riscos, sistemas de segurança e prevenção de perdas."@pt-br .

:SandDetector a owl:Class ;
    dcterms:identifier "SandDetector" ;
    rdfs:subClassOf :Sensor .

:SeparatorVessel a owl:Class ;
    dcterms:identifier "SeparatorVessel" ;
    rdfs:subClassOf :Vessel .

:Shackle a owl:Class ;
    dcterms:identifier "Shackle" ;
    rdfs:subClassOf :MooringAccessory ;
    skos:altLabel "Anchor Shackle"@en,
        "Bow Shackle"@en,
        "Clevis"@en,
        "D-Shackle"@en,
        "U-Bolt"@en ;
    skos:definition "A device used to connect and secure components in subsea systems, particularly during lifting, handling, or mooring operations. The Shackle typically consists of a U-shaped metal piece with a removable pin or bolt, allowing it to link components such as chains, slings, or cables. It provides a strong and reliable connection point, ensuring that loads can be safely transferred or lifted without risk of detachment or failure. Shackles are essential for securing flexible lines and other equipment during installation and maintenance in subsea environments."@en ;
    skos:prefLabel "Shackle"@en,
        "Manilha"@pt-br ;
    :hasAttribute :ShackleInnerDiameter,
        :ShackleOpeningWidth,
        :ShackleOuterDiameter,
        :ShackleThickness,
        :WorkingLoadLimit ;
    :ifc_equivalentClass "IfcMechanicalFastener" ;
    :ifc_objectType "Shackle" ;
    :ifc_predefinedType "USERDEFINED" .

:ShearableRiserJoint a owl:Class ;
    dcterms:identifier "ShearableRiserJoint" ;
    rdfs:subClassOf :RunningTool .

:Socket a owl:Class ;
    dcterms:identifier "Socket" ;
    rdfs:subClassOf :MooringAccessory .

:Solar a owl:Class ;
    rdfs:label "Solar Energy"@en,
        "Energia Solar"@pt-br ;
    rdfs:subClassOf :Renewable ;
    skos:definition "Energy harnessed from sunlight, including photovoltaic and thermal systems."@en,
        "Energia obtida da luz solar, incluindo sistemas fotovoltaicos e térmicos."@pt-br .

:SpliceBox a owl:Class ;
    dcterms:identifier "SpliceBox" ;
    rdfs:subClassOf :ComponentDevice .

:StaticEquipmentEngineering a owl:Class ;
    rdfs:label "Static Equipment Engineering"@en,
        "Engenharia de Equipamentos Estáticos"@pt-br ;
    rdfs:subClassOf :EquipmentEngineering ;
    skos:definition "Engineering of non-moving industrial equipment such as pressure vessels, tanks, and heat exchangers."@en,
        "Engenharia de equipamentos industriais sem partes móveis como vasos de pressão, tanques e trocadores de calor."@pt-br .

:StaticUmbilicalSpan a owl:Class ;
    dcterms:identifier "StaticUmbilicalSpan" ;
    rdfs:subClassOf :UmbilicalSpan .

:StopperCollar a owl:Class ;
    dcterms:identifier "StopperCollar" ;
    rdfs:subClassOf :SplitCollar ;
    skos:altLabel "Locking Collar"@en,
        "Positioning Collar"@en,
        "Retention Collar"@en,
        "Stopper Clamp"@en ;
    skos:definition "A component used to prevent the movement or displacement of other parts in subsea systems. The Stopper Collar is installed around the pipe or component and acts as a physical barrier to stop or limit movement, ensuring components stay in their intended positions. It is crucial for maintaining alignment and stability during installation, operation, or maintenance, providing secure positioning and preventing unwanted shifts or displacements."@en ;
    skos:prefLabel "Stopper Collar"@en,
        "Colar Batente"@pt-br ;
    :ifc_equivalentClass "IfcPipeFitting" ;
    :ifc_objectType "StopperCollar" ;
    :ifc_predefinedType "USERDEFINED" .

:StorageBox a owl:Class ;
    dcterms:identifier "StorageBox" ;
    rdfs:subClassOf :StorageAccessory .

:StorageSkid a owl:Class ;
    dcterms:identifier "StorageSkid" ;
    rdfs:subClassOf :StorageAccessory .

:StorageSpool a owl:Class ;
    dcterms:identifier "StorageSpool" ;
    rdfs:subClassOf :StorageAccessory .

:StructuralEngineering a owl:Class ;
    rdfs:label "Structural Engineering"@en,
        "Engenharia Estrutural"@pt-br ;
    rdfs:subClassOf :CivilEngineering ;
    skos:definition "Engineering discipline focused on the structural integrity and design of buildings and infrastructure."@en,
        "Disciplina de engenharia focada na integridade estrutural e projeto de edifícios e infraestrutura."@pt-br .

:SubseaConnectionPoint a owl:Class ;
    dcterms:identifier "SubseaConnectionPoint" ;
    rdfs:subClassOf :LogicalConnection ;
    skos:definition "The Subsea Connection Point is the interface on subsea equipment where a flexible pipe connects. It serves as the critical link between the flexible pipe and subsea systems, enabling the transfer of fluids or gases. Designed to withstand high pressures and harsh underwater conditions, the Subsea External Point ensures a secure and reliable connection, facilitating efficient operation of various subsea systems."@en ;
    skos:prefLabel "Subsea Connection Point"@en,
        "Ponto de Conexão Submarino"@pt-br ;
    :ifc_equivalentClass "IfcPipeFitting" ;
    :ifc_objectType "SubseaConnectionPoint" ;
    :ifc_predefinedType "USERDEFINED" .

:SubseaFlexiblePipesBsddDictionary a owl:Class ;
    dcterms:identifier "SubseaFlexiblePipesBsddDictionary" ;
    rdfs:subClassOf :DomainElement ;
    skos:definition "Bsdd Dictionary of Subsea Flexible Pipelines."@en ;
    skos:prefLabel "Subsea Flexible Pipes Bsdd Dictionary"@en,
        "Dicionário Bsdd de Dutos Flexíveis Submarinos"@pt-br ;
    :ifc_equivalentClass "IfcClassification" ;
    :ifc_objectType "SubseaFlexiblePipesBsddDictionary" ;
    :ifc_predefinedType "USERDEFINED" .

:SubseaFlexiblePipesEngineering a owl:Class ;
    rdfs:label "Subsea Flexible Pipes Engineering"@en,
        "Engenharia de Tubos Flexíveis Submarinos"@pt-br ;
    rdfs:subClassOf :SubseaEngineering ;
    skos:definition "Engineering of flexible pipe systems used in subsea applications."@en,
        "Engenharia de sistemas de tubos flexíveis utilizados em aplicações submarinas."@pt-br .

:SubseaOilField a owl:Class ;
    dcterms:identifier "SubseaOilField" ;
    rdfs:subClassOf :SubseaLayout ;
    skos:altLabel "Subsea Hydrocarbon Field"@en,
        "Subsea Oil Reservoir"@en,
        "Subsea Oil Site"@en,
        "Subsea Petroleum Field"@en ;
    skos:definition "A subsea oil field refers to an underwater reservoir of hydrocarbons located beneath the seabed. It involves the extraction of oil and gas from deposits situated in deepwater or shallow marine environments. The subsea oil field includes a range of equipment and infrastructure, such as subsea wells, pipelines, and production systems, all designed to safely and efficiently extract and transport hydrocarbons to processing facilities on the surface or shore. The development and operation of subsea oil fields require specialized technology and expertise to manage the challenges of deepwater environments and ensure the successful production and handling of resources."@en ;
    skos:prefLabel "Subsea Oil Field"@en,
        "Campo de Petróleo Submarino"@pt-br ;
    :ifc_equivalentClass "IfcSite" ;
    :ifc_objectType "SubseaOilField" .

:SubseaPipeline a owl:Class ;
    dcterms:identifier "SubseaPipeline" ;
    rdfs:subClassOf :Interconnection ;
    skos:definition "A Subsea Pipeline is a conduit installed on the seafloor designed to transport oil, gas, or other fluids from underwater production facilities to processing or storage locations on the surface or shore. Engineered to withstand harsh underwater conditions, including high pressures, corrosive environments, and dynamic movements, the Subsea Pipeline is constructed with durable materials and advanced technologies to ensure reliable and efficient fluid transfer."@en ;
    skos:prefLabel "Subsea Pipeline"@en,
        "Linha Submarina"@pt-br ;
    :hasAttribute :BasicProjectRevision,
        :CO2VolumePercentage,
        :ExecutiveProjectRevision,
        :H2SVolumeConcentration,
        :InternalDiameter,
        :InternalIncidentalPressureTable,
        :InternalIncidentalPressureTable_PositionReference,
        :InternalIncidentalPressureTable_Pressure,
        :InternalIncidentalPressureTable_VPosWRTWaterline,
        :MaterialRequest,
        :MaterialRequestRev,
        :MaxDesignAbsIntPresTable,
        :MaxDesignAbsIntPresTable_PositionReference,
        :MaxDesignAbsIntPresTable_Pressure,
        :MaxDesignAbsIntPresTable_VPosWRTWaterline,
        :MaximumTemperature,
        :MaximumThermalExchangeCoefficient,
        :MinimumThermalExchangeCoefficient,
        :NominalLength,
        :ProjectAcronym,
        :ProjectCode,
        :RiserConfiguration,
        :Service,
        :SubProjectId,
        :UnifilarDiagram,
        :UnifilarDiagramRev ;
    :ifc_equivalentClass "IfcBuilding" ;
    :ifc_objectType "SubseaPipeline" ;
    :ifc_predefinedType "USERDEFINED" .

:SubseaRigidPipesEngineering a owl:Class ;
    rdfs:label "Subsea Rigid Pipes Engineering"@en,
        "Engenharia de Tubos Rígidos Submarinos"@pt-br ;
    rdfs:subClassOf :SubseaEngineering ;
    skos:definition "Engineering of rigid pipeline systems used in subsea applications."@en,
        "Engenharia de sistemas de tubulações rígidas utilizadas em aplicações submarinas."@pt-br .

:SubseaStructuresEngineering a owl:Class ;
    rdfs:label "Subsea Structures Engineering"@en,
        "Engenharia de Estruturas Submarinas"@pt-br ;
    rdfs:subClassOf :SubseaEngineering ;
    skos:definition "Engineering of subsea manifolds, christmas trees, and other structural components."@en,
        "Engenharia de manifolds submarinos, árvores de natal e outros componentes estruturais."@pt-br .

:SubseaUmbilicalsEngineering a owl:Class ;
    rdfs:label "Subsea Umbilicals Engineering"@en,
        "Engenharia de Umbilicais Submarinos"@pt-br ;
    rdfs:subClassOf :SubseaEngineering ;
    skos:definition "Engineering of subsea umbilical systems providing control, power and chemical injection."@en,
        "Engenharia de sistemas de umbilicais submarinos fornecendo controle, energia e injeção química."@pt-br .

:SubseaWell a owl:Class ;
    dcterms:identifier "SubseaWell" ;
    rdfs:subClassOf :EquipmentLocation ;
    skos:definition "A Subsea Well is a well located on the seafloor from which hydrocarbons such as oil and gas are extracted. Positioned underwater, it typically involves a wellhead assembly that includes valves, controls, and monitoring equipment to manage the extraction process. The Subsea Well is connected to surface facilities via pipelines and umbilicals, which facilitate the transport of extracted resources and the provision of necessary services like power and communication. Designed to operate under high pressure and harsh marine conditions, the subsea well is a critical component of offshore oil and gas production systems."@en ;
    skos:prefLabel "Subsea Well"@en,
        "Poço"@pt-br ;
    :ifc_equivalentClass "IfcBuilding" ;
    :ifc_objectType "SubseaWell" ;
    :ifc_predefinedType "USERDEFINED" .

:SuctionPile a owl:Class ;
    dcterms:identifier "SuctionPile" ;
    rdfs:subClassOf :Pile .

:TPT a owl:Class ;
    dcterms:identifier "TPT" ;
    rdfs:subClassOf :Sensor .

:TemperatureSensor a owl:Class ;
    dcterms:identifier "TemperatureSensor" ;
    rdfs:subClassOf :Sensor .

:TensileArmour a owl:Class ;
    dcterms:identifier "TensileArmour" ;
    rdfs:subClassOf :WireLayer ;
    skos:definition "Protective layer designed to withstand high tensile stresses and mechanical loads, Tensile Armour is composed of high-strength steel wires or reinforced materials arranged in a helical configuration around the riser. It provides essential resistance to tension and shields the inner layers from mechanical damage and wear, ensuring the riser's integrity and durability during installation and operation in extreme underwater conditions."@en ;
    skos:prefLabel "Tensile Armour"@en,
        "Armadura de Tração"@pt-br ;
    :hasAttribute :TensileWireLayAngle,
        :TensileWiresCount ;
    :ifc_equivalentClass "IfcPipeSegment" ;
    :ifc_objectType "TensileArmour" ;
    :ifc_predefinedType "USERDEFINED" .

:TestBase a owl:Class ;
    dcterms:identifier "TestBase" ;
    rdfs:subClassOf :TestEquipment .

:ThermalPower a owl:Class ;
    rdfs:label "Thermal Power"@en,
        "Energia Térmica"@pt-br ;
    rdfs:subClassOf :Domain ;
    skos:definition "Energy production from fossil fuels (coal, natural gas) through thermal conversion."@en,
        "Produção de energia a partir de combustíveis fósseis (carvão, gás natural) através de conversão térmica."@pt-br .

:TieIn a owl:Class ;
    dcterms:identifier "TieIn" ;
    rdfs:subClassOf :PressureComponent .

:TopBendStiffener a owl:Class ;
    dcterms:identifier "TopBendStiffener" ;
    rdfs:subClassOf :BendStiffener ;
    skos:altLabel "Curvature Stiffener"@en,
        "Stiffener"@en,
        "Top Bending Stiffener"@en ;
    skos:definition "Designed to support and stabilize the riser where it transitions from the seabed to the floating platform or vessel, the Top Bend Stiffener is composed of high-strength materials such as steel or composites. It helps prevent excessive bending, distributes mechanical loads, and enhances flexibility management, ensuring the riser's structural integrity and performance during installation and operation in dynamic offshore conditions."@en ;
    skos:prefLabel "Top Bend Stiffener"@en,
        "Enrijecedor de Curvatura de Topo"@pt-br ;
    :ifc_equivalentClass "IfcPipeFitting" ;
    :ifc_objectType "TopBendStiffener" .

:TopsideConnectionPoint a owl:Class ;
    dcterms:identifier "TopsideConnectionPoint" ;
    rdfs:subClassOf :LogicalConnection ;
    skos:definition "Designed to connect the riser to the floating platform or vessel, the Topside Connection Point is a crucial component that ensures a secure and reliable interface between the riser and the topside facilities. Composed of high-strength materials, this connector is engineered to handle the mechanical loads and dynamic conditions of offshore environments. It facilitates the transfer of fluids and provides structural stability, playing a key role in maintaining the overall integrity and functionality of the riser system."@en ;
    skos:prefLabel "Topside Connection Point"@en,
        "Ponto de Conexão de Topo"@pt-br ;
    :ifc_equivalentClass "IfcPipeFitting" ;
    :ifc_objectType "TopsideConnectionPoint" ;
    :ifc_predefinedType "USERDEFINED" .

:TorpedoPile a owl:Class ;
    dcterms:identifier "TorpedoPile" ;
    rdfs:subClassOf :Pile .

:Transportation a owl:Class ;
    rdfs:label "Transportation"@en,
        "Transporte"@pt-br ;
    rdfs:subClassOf :LifecyclePhase ;
    skos:definition "Logistics and transport of materials and equipment to the construction or installation site."@en,
        "Logística e transporte de materiais e equipamentos para o local de construção ou instalação."@pt-br .

:TreeCap a owl:Class ;
    dcterms:identifier "TreeCap" ;
    rdfs:subClassOf :FlowControlModule .

:TreeRunningTool a owl:Class ;
    dcterms:identifier "TreeRunningTool" ;
    rdfs:subClassOf :RunningTool .

:TrianglePlate a owl:Class ;
    dcterms:identifier "TrianglePlate" ;
    rdfs:subClassOf :MooringAccessory .

:TubingHanger a owl:Class ;
    dcterms:identifier "TubingHanger" ;
    rdfs:subClassOf :PressureComponent .

:TubingHangerRunningTool a owl:Class ;
    dcterms:identifier "TubingHangerRunningTool" ;
    rdfs:subClassOf :RunningTool .

:UNSBoltSet a owl:Class ;
    dcterms:identifier "UNSBoltSet" ;
    rdfs:subClassOf :BoltSet ;
    skos:definition "A set of bolts conforming to the Unified Numbering System (UNS) standard, ensuring material consistency and reliability in subsea applications."@en ;
    skos:prefLabel "UNS Bolt Set"@en,
        "Conjunto de Parafusos UNS"@pt-br ;
    :hasAttribute :NominalDiameter,
        :PitchToleranceClass,
        :ThreadStandard,
        :ThreadsPerInch ;
    :ifc_equivalentClass "IfcMechanicalFastener" ;
    :ifc_objectType "UNSBoltSet" ;
    :ifc_predefinedType "USERDEFINED" .

:UNSStudSet a owl:Class ;
    dcterms:identifier "UNSStudSet" ;
    rdfs:subClassOf :StudSet ;
    skos:definition "UNS stud sets are essential fastening components for subsea oil and gas components, tailored to securely join equipment parts. Each set comprises bolts, nuts, and washers, all in UNS sizing and crafted from high-strength, corrosion-resistant materials to endure the challenging subsea environment. These components provide robust fastening, ensuring structural integrity and leak prevention in end fittings. UNS stud sets are engineered to withstand high pressure and extreme temperatures, playing a vital role in the safety and longevity of subsea interconnections."@en ;
    skos:prefLabel "UNS Stud Set"@en,
        "Conjunto de Estojos UNS"@pt-br ;
    :hasAttribute :PitchToleranceClass,
        :ThreadStandard,
        :ThreadsPerInch ;
    :ifc_equivalentClass "IfcMechanicalFastener" ;
    :ifc_objectType "UNSStudSet" ;
    :ifc_predefinedType "USERDEFINED" .

:UTA a owl:Class ;
    dcterms:identifier "UTA" ;
    rdfs:subClassOf :SubseaEquipment .

:UTM a owl:Class ;
    dcterms:identifier "UTM" ;
    rdfs:subClassOf :LineTerminationModule .

:UmbilicalLocation a owl:Class ;
    dcterms:identifier "UmbilicalLocation" ;
    rdfs:subClassOf :Interconnection .

:UmbilicalSegment a owl:Class ;
    dcterms:identifier "UmbilicalSegment" ;
    rdfs:subClassOf :TransportLineSegment ;
    :ifc_equivalentClass "UmbilicalSegment" ;
    :ifc_objectType "IfcPipeSegment" ;
    :ifc_predefinedType "USERDEFINED" .

:Upstream a owl:Class ;
    rdfs:label "Upstream"@en,
        "Upstream"@pt-br ;
    rdfs:subClassOf :OilAndGas ;
    skos:definition "Oil & Gas sector covering exploration, drilling, and production of hydrocarbon resources."@en,
        "Setor de Petróleo & Gás que abrange exploração, perfuração e produção de recursos de hidrocarbonetos."@pt-br .

:UtilityPipingEngineering a owl:Class ;
    rdfs:label "Utility Piping Engineering"@en,
        "Engenharia de Tubulação de Utilidades"@pt-br ;
    rdfs:subClassOf :TechnicalDiscipline ;
    skos:definition "Engineering discipline focused on the design of piping systems for utility services."@en,
        "Disciplina de engenharia focada no projeto de sistemas de tubulação para serviços de utilidades."@pt-br .

:VCM a owl:Class ;
    dcterms:identifier "VCM" ;
    rdfs:subClassOf :ConnectionModule .

:WaterIntake a owl:Class ;
    dcterms:identifier "WaterIntake" ;
    rdfs:subClassOf :SubseaEquipment .

:WearBushing a owl:Class ;
    dcterms:identifier "WearBushing" ;
    rdfs:subClassOf :Accessory .

:WearBushingRunningTool a owl:Class ;
    dcterms:identifier "WearBushingRunningTool" ;
    rdfs:subClassOf :RunningTool .

:Wellhead a owl:Class ;
    dcterms:identifier "Wellhead" ;
    rdfs:subClassOf :Structure .

:WetChristmasTree a owl:Class ;
    dcterms:identifier "WetChristmasTree" ;
    rdfs:subClassOf :FlowControlEquipment ;
    :ifc_objectType "WetChristmasTree" ;
    :ifc_predefinedType "USERDEFINED" .

:Wind a owl:Class ;
    rdfs:label "Wind Energy"@en,
        "Energia Eólica"@pt-br ;
    rdfs:subClassOf :Renewable ;
    skos:definition "Energy generated from wind using turbines and related technologies."@en,
        "Energia gerada a partir do vento usando turbinas e tecnologias relacionadas."@pt-br .

:WireRopeSegment a owl:Class ;
    dcterms:identifier "WireRopeSegment" ;
    rdfs:subClassOf :RopeSegment .

:anyURIType a owl:Class ;
    rdfs:label "URI Value"@en ;
    rdfs:comment "Constraint for xsd:anyURI (URIs/IRIs)"@en ;
    rdfs:subClassOf :TypedValue ;
    owl:equivalentClass [ a owl:Restriction ;
            owl:allValuesFrom xsd:anyURI ;
            owl:onProperty rdf:value ] .

:appliesTo a owl:AnnotationProperty ;
    rdfs:label "Applies to"@en,
        "Se aplica a"@pt-br ;
    rdfs:subPropertyOf :DomainAuxiliarAnnotation ;
    skos:definition "Indicates that the subject applies to the object"@en,
        "Indica que o sujeito se aplica ao predicado"@pt-br .

:base64BinaryType a owl:Class ;
    rdfs:label "Base64 Binary"@en ;
    rdfs:comment "Constraint for xsd:base64Binary (binary data)"@en ;
    rdfs:subClassOf :TypedValue ;
    owl:equivalentClass [ a owl:Restriction ;
            owl:allValuesFrom xsd:base64Binary ;
            owl:onProperty rdf:value ] .

:createdAtLifecyclePhase a owl:AnnotationProperty ;
    rdfs:label "Created at lifecycle phase"@en,
        "Criado na fase do ciclo de vida"@pt-br ;
    rdfs:subPropertyOf :DomainEngineeringAnnotation ;
    skos:definition "In which lifecycle phase the information was created"@en,
        "Em que fase do ciclo de vida a informação foi criada"@pt-br .

:dateValue a owl:Class ;
    rdfs:label "Date Value"@en ;
    rdfs:comment "Constraint for xsd:date (calendar dates)"@en ;
    rdfs:subClassOf :TypedValue ;
    owl:equivalentClass [ a owl:Restriction ;
            owl:allValuesFrom xsd:date ;
            owl:onProperty rdf:value ] .

:decimalValue a owl:Class ;
    rdfs:label "Decimal Value"@en ;
    rdfs:comment "Constraint for xsd:decimal (arbitrary precision numbers)"@en ;
    rdfs:subClassOf :TypedValue ;
    owl:equivalentClass [ a owl:Restriction ;
            owl:allValuesFrom xsd:decimal ;
            owl:onProperty rdf:value ] .

:doubleValue a owl:Class ;
    rdfs:label "Double Value"@en ;
    rdfs:comment "Constraint for xsd:double (64-bit floating point)"@en ;
    rdfs:subClassOf :TypedValue ;
    owl:equivalentClass [ a owl:Restriction ;
            owl:allValuesFrom xsd:double ;
            owl:onProperty rdf:value ] .

:hasAttribute a owl:AnnotationProperty ;
    rdfs:label "Has attribute"@en,
        "Possui atributo"@pt-br ;
    rdfs:subPropertyOf :DomainAuxiliarAnnotation ;
    skos:definition "Indicates attribute(s) that the entity has"@en,
        "Indica atributo(s) que a entidade possui"@pt-br .

:hasAttributeCategory a owl:AnnotationProperty ;
    rdfs:label "has attribute category"@en,
        "tem categoria de atributo"@pt-br ;
    skos:definition "The technical category of the attribute (geometric, functional, etc.)"@en,
        "A categoria técnica do atributo (geométrica, funcional, etc.)"@pt-br .

:hasAttributeGroup a owl:AnnotationProperty ;
    rdfs:label "has attribute group"@en,
        "tem grupo de atributo"@pt-br ;
    skos:definition "Indicates that the attribute has a special grouping for organizational purposes"@en,
        "Indica que o atributo tem um agrupamento especial para fins de organização"@pt-br .

:hasAttributeScope a owl:AnnotationProperty ;
    rdfs:label "has attribute scope"@en,
        "tem escopo de atributo"@pt-br ;
    skos:definition "Classifies whether the attribute applies to equipment type, instance or batch"@en,
        "Classifica se o atributo se aplica ao tipo de equipamento, instância ou lote"@pt-br .

:hasDiscipline a owl:AnnotationProperty ;
    rdfs:label "Has Discipline"@en,
        "Pertence a uma disciplina técnica"@pt-br ;
    rdfs:subPropertyOf :DomainEngineeringAnnotation ;
    skos:definition "Belongs to a technical discipline"@en,
        "Associa a entidade a uma disciplina técnica"@pt-br .

:hasDomain a owl:AnnotationProperty ;
    rdfs:label "Has Domain"@en,
        "Pertence a um domínio"@pt-br ;
    rdfs:subPropertyOf :DomainEngineeringAnnotation ;
    skos:definition "Belongs to one or more domains"@en,
        "Associa a entidade a um ou mais domínios"@pt-br .

:hasLifecycleCreationPhase a owl:AnnotationProperty ;
    rdfs:label "has lifecycle creation phase"@en,
        "tem fase de criação no ciclo de vida"@pt-br ;
    skos:definition "The lifecycle phase when the attribute value is created"@en,
        "A fase do ciclo de vida quando o valor do atributo é criado"@pt-br .

:hasLifecycleUsagePhase a owl:AnnotationProperty ;
    rdfs:label "has lifecycle usage phase"@en,
        "tem fase de uso no ciclo de vida"@pt-br ;
    skos:definition "The lifecycle phase(s) when the attribute value is used"@en,
        "A(s) fase(s) do ciclo de vida quando o valor do atributo é utilizado"@pt-br .

:hasLocationType a owl:AnnotationProperty ;
    rdfs:label "Has Location Type"@en,
        "Pertence a um tipo de locação"@pt-br ;
    rdfs:subPropertyOf :DomainEngineeringAnnotation ;
    skos:definition "Belongs to one or more Location Types"@en,
        "Associa a entidade a um tipo de locação"@pt-br .

:hasSubDomain a owl:AnnotationProperty ;
    rdfs:label "Has SubDomain"@en,
        "Pertence a um subdomínio"@pt-br ;
    rdfs:subPropertyOf :DomainEngineeringAnnotation ;
    skos:definition "Belongs to one or more subdomains"@en,
        "Associa a entidade a um ou mais subdomínios"@pt-br .

:hasTypedValue a owl:AnnotationProperty ;
    rdfs:label "Has Typed Value"@en,
        "Possui tipo de valor"@pt-br ;
    rdfs:subPropertyOf :DomainAuxiliarAnnotation ;
    skos:definition "Indicates that the entity has a typed value, lik float, string, boolean, integer, etc."@en,
        "Indica que a entidade tem um valor como número real, inteiro, texto, booleano e etc."@pt-br .

:hasValueCardinality a owl:AnnotationProperty ;
    rdfs:label "Has Value Cardinality"@en,
        "Possui cardinalidade de valor"@pt-br ;
    rdfs:subPropertyOf :DomainAuxiliarAnnotation ;
    skos:definition "Indicates the quantity of values the entity support"@en,
        "Indica a quantidade de valores que a entidade possui"@pt-br .

:ifc_equivalentClass a owl:AnnotationProperty ;
    rdfs:label "IFC equivalent Class"@en,
        "Classe IFC equivalente"@pt-br ;
    rdfs:subPropertyOf :DomainEngineeringAnnotation ;
    skos:definition "IFC equivalent class"@en,
        "Classe IFC equivalente"@pt-br .

:ifc_objectType a owl:AnnotationProperty ;
    rdfs:label "IFC ObjectType"@en,
        "ObjectType IFC"@pt-br ;
    rdfs:subPropertyOf :DomainEngineeringAnnotation ;
    skos:definition "Object Type for IFC class customization"@en,
        "Object Type para a customização de classes IFC"@pt-br .

:ifc_predefinedType a owl:AnnotationProperty ;
    rdfs:label "IFC PredefinedType"@en,
        "PredefinedType IFC"@pt-br ;
    rdfs:subPropertyOf :DomainEngineeringAnnotation ;
    skos:definition "Predefined Type for IFC class customization"@en,
        "Predefined Type para a customização de classes IFC"@pt-br .

:longValue a owl:Class ;
    rdfs:label "Long Value"@en ;
    rdfs:comment "Constraint for xsd:long (64-bit integer)"@en ;
    rdfs:subClassOf :TypedValue ;
    owl:equivalentClass [ a owl:Restriction ;
            owl:allValuesFrom xsd:long ;
            owl:onProperty rdf:value ] .

:timeValue a owl:Class ;
    rdfs:label "Time Value"@en ;
    rdfs:comment "Constraint for xsd:time (time of day)"@en ;
    rdfs:subClassOf :TypedValue ;
    owl:equivalentClass [ a owl:Restriction ;
            owl:allValuesFrom xsd:time ;
            owl:onProperty rdf:value ] .

:validValues a owl:AnnotationProperty ;
    rdfs:label "Valid Values"@en,
        "Valores Válidos"@pt-br ;
    rdfs:subPropertyOf :DomainAuxiliarAnnotation ;
    skos:definition "List of Valid Values for the Attribute"@en,
        "Lista de valores válidos para o atributo"@pt-br .

xsd:date a rdfs:Datatype .

xsd:time a rdfs:Datatype .

:AbsoluteInsidePressure a owl:DatatypeProperty ;
    dcterms:accessRights "PUBLIC" ;
    dcterms:identifier "AbsoluteInsidePressure" ;
    rdfs:subClassOf :BendingStiffnessAttribute ;
    skos:definition "Represents the absolute internal pressure exerted within a component or system. This property is crucial for evaluating the structural integrity and performance, ensuring that the system can withstand the specified pressure without failure, particularly in subsea environments where pressure management is critical."@en ;
    skos:prefLabel "Absolute Inside Pressure"@en,
        "Pressão Absoluta Interna"@pt-br ;
    :hasAttributeScope :TypeLevelAttribute ;
    :hasTypedValue :floatValue ;
    :hasValueCardinality :singleValue .

:AbsoluteOutsidePressure a owl:DatatypeProperty ;
    dcterms:accessRights "PUBLIC" ;
    dcterms:identifier "AbsoluteOutsidePressure" ;
    rdfs:subClassOf :BendingStiffnessAttribute ;
    skos:definition "Represents the absolute external pressure exerted on a component or system. This property is essential for evaluating how the system withstands pressure from its surrounding environment, particularly in subsea applications where external pressure can be significantly higher and impact the structural integrity of the system."@en ;
    skos:prefLabel "Absolute Outside Pressure"@en,
        "Pressão Absoluta Externa"@pt-br ;
    :hasAttributeScope :TypeLevelAttribute ;
    :hasTypedValue :floatValue ;
    :hasValueCardinality :singleValue .

:AnodeCollarsAxialSpacing a owl:DatatypeProperty ;
    dcterms:accessRights "PUBLIC" ;
    dcterms:identifier "AnodeCollarsAxialSpacing" ;
    rdfs:subPropertyOf :DomainAttribute ;
    skos:definition "Axial distance between each individual collar."@en ;
    skos:prefLabel "Anode Collars Axial Spacing"@en,
        "Espaçamento Axial entre os Colares de Anodo"@pt-br ;
    :hasAttributeScope :TypeLevelAttribute ;
    :hasTypedValue :floatValue ;
    :hasValueCardinality :singleValue .

:AnodeCollarsQuantity a owl:DatatypeProperty ;
    dcterms:accessRights "PUBLIC" ;
    dcterms:identifier "AnodeCollarsQuantity" ;
    rdfs:subPropertyOf :DomainAttribute ;
    skos:definition "The total number of anode collars to provide cathodic protection against corrosion."@en ;
    skos:prefLabel "Anode Collars Quantity"@en,
        "Quantidade de Colares de Anodo"@pt-br ;
    :hasAttributeScope :TypeLevelAttribute ;
    :hasTypedValue :intValue ;
    :hasValueCardinality :singleValue .

:AssemblyShouldObeyModelPolarity a owl:DatatypeProperty ;
    dcterms:accessRights "PUBLIC" ;
    dcterms:identifier "AssemblyShouldObeyModelPolarity" ;
    rdfs:subPropertyOf :DomainAttribute ;
    skos:definition "If true, the pipe section must be assembled according to the polarity in the model. If false, it can be mounted in any polarity."@en ;
    skos:prefLabel "Assembly Should Obey Model Polarity"@en,
        "A Montagem Deve Obedecer à Polaridade do Modelo"@pt-br ;
    :hasAttributeScope :InstanceLevelAttribute ;
    :hasTypedValue :booleanValue ;
    :hasValueCardinality :singleValue .

:AxialStiffnessUnderCompressionAtSeaLevel a owl:DatatypeProperty ;
    dcterms:accessRights "PUBLIC" ;
    dcterms:identifier "AxialStiffnessUnderCompressionAtSeaLevel" ;
    rdfs:subPropertyOf :DomainAttribute ;
    skos:definition "Represents the resistance of a component or system to axial deformation under compression when measured at sea level. This property is essential for understanding how the structure behaves under compressive loads, ensuring that it can maintain stability and structural integrity."@en,
        "Rigidez axial (EA) duto comprimido, 20°C e pressão atmosferica (dentro e fora)"@pt-br ;
    skos:prefLabel "Axial Stiffness Under Compression At Sea Level"@en,
        "Rigidez Axial sob Compressão ao Nível do Mar"@pt-br ;
    :hasAttributeScope :TypeLevelAttribute ;
    :hasTypedValue :floatValue ;
    :hasValueCardinality :singleValue .

:AxialStiffnessUnderTensionAtSeaLevel a owl:DatatypeProperty ;
    dcterms:accessRights "PUBLIC" ;
    dcterms:identifier "AxialStiffnessUnderTensionAtSeaLevel" ;
    rdfs:subPropertyOf :DomainAttribute ;
    skos:definition "Represents the resistance of a component or system to axial deformation under tension when measured at sea level. This property is crucial for evaluating how the structure performs under tensile loads, ensuring it can withstand stretching forces while maintaining its integrity."@en,
        "Rigidez axial (EA) duto tracionado, 20°C e pressão atmosferica (dentro e fora)"@pt-br ;
    skos:prefLabel "Axial Stiffness Under Tension At Sea Level"@en,
        "Rigidez Axial sob Tração ao Nível do Mar"@pt-br ;
    :hasAttributeScope :TypeLevelAttribute ;
    :hasTypedValue :floatValue ;
    :hasValueCardinality :singleValue .

:BasicProjectRevision a owl:DatatypeProperty ;
    dcterms:accessRights "PUBLIC" ;
    dcterms:identifier "BasicProjectRevision" ;
    rdfs:subPropertyOf :DomainAttribute ;
    skos:definition "Numeric value incremented with each new submission of the project (e.g., 0000, 0001, 0002, etc.), recorded as text. This value tracks revisions and ensures clarity in version control throughout the project lifecycle, allowing stakeholders to reference the most current or previous versions as needed."@en,
        "Valor numérico incrementado a cada novo envio (0000, 0001, 0002 e etc.) como texto"@pt-br ;
    skos:prefLabel "Basic Project Revision"@en,
        "Revisão do Projeto Básico"@pt-br ;
    :hasAttributeScope :InstanceLevelAttribute ;
    :hasTypedValue :stringValue ;
    :hasValueCardinality :singleValue .

:BendMomentVsShearForceTable_BendingMoment a owl:DatatypeProperty ;
    dcterms:accessRights "PUBLIC" ;
    dcterms:identifier "BendMomentVsShearForceTable_BendingMoment" ;
    rdfs:subClassOf :BendMomentVsShearForceTableColumn ;
    skos:definition "Represents the moment generated by a force causing the component or system to bend around an axis. This property is critical for assessing the structure's ability to resist bending under operational loads, ensuring it maintains its shape and structural integrity."@en ;
    skos:prefLabel "Bending Moment"@en,
        "Momento de flexão"@pt-br ;
    :hasAttributeScope :TypeLevelAttribute ;
    :hasTypedValue :floatValue ;
    :hasValueCardinality :multiValue .

:BendMomentVsShearForceTable_Condition a owl:DatatypeProperty ;
    dcterms:accessRights "PUBLIC" ;
    dcterms:identifier "BendMomentVsShearForceTable_Condition" ;
    rdfs:subClassOf :BendMomentVsShearForceAttribute ;
    skos:definition "Curve data flexible pipe condition."@en ;
    skos:prefLabel "Condition"@en,
        "Condição do flexível para os dados da curva"@pt-br ;
    :hasAttributeScope :TypeLevelAttribute ;
    :hasTypedValue :stringValue ;
    :hasValueCardinality :singleValue .

:BendMomentVsShearForceTable_ShearForce a owl:DatatypeProperty ;
    dcterms:accessRights "PUBLIC" ;
    dcterms:identifier "BendMomentVsShearForceTable_ShearForce" ;
    rdfs:subClassOf :BendMomentVsShearForceTableColumn ;
    skos:definition "Represents the force applied parallel to the surface of a material or component, causing it to experience shear stress. This property is essential for evaluating the material's ability to resist sliding or deformation when subjected to external forces."@en,
        "Força de cisalhamento (Obrigatório incluir o valor para força = 0)"@pt-br ;
    skos:prefLabel "Shear Force"@en,
        "Força de Cisalhamento"@pt-br ;
    :hasAttributeScope :TypeLevelAttribute ;
    :hasTypedValue :floatValue ;
    :hasValueCardinality :multiValue .

:BendingMomentTable_BendingMoment a owl:DatatypeProperty ;
    dcterms:accessRights "PUBLIC" ;
    dcterms:identifier "BendingMomentTable_BendingMoment" ;
    rdfs:subClassOf :BendingStiffnessTableColumn ;
    skos:definition "Represents the moment generated by a force causing the component or system to bend around an axis. This property is critical for assessing the structure's ability to resist bending under operational loads, ensuring it maintains its shape and structural integrity."@en ;
    skos:prefLabel "Bending Moment"@en,
        "Momento de Flexão"@pt-br ;
    :hasAttributeScope :TypeLevelAttribute ;
    :hasTypedValue :floatValue ;
    :hasValueCardinality :multiValue .

:BendingMomentTable_Curvature a owl:DatatypeProperty ;
    dcterms:accessRights "PUBLIC" ;
    dcterms:identifier "BendingMomentTable_Curvature" ;
    rdfs:subClassOf :BendingStiffnessTableColumn ;
    skos:definition "Represents the degree to which a component or structure bends or curves along its length. This property is important for understanding the flexibility and bending behavior, ensuring that the structure can perform as required under operational conditions without exceeding its design limits."@en ;
    skos:prefLabel "Curvature"@en,
        "Curvatura"@pt-br ;
    :hasAttributeScope :TypeLevelAttribute ;
    :hasTypedValue :floatValue ;
    :hasValueCardinality :multiValue .

:BoreDiameter a owl:DatatypeProperty ;
    dcterms:accessRights "PUBLIC" ;
    dcterms:identifier "BoreDiameter" ;
    rdfs:subPropertyOf :DomainAttribute ;
    skos:definition "Internal diameter that defines the size of the passage through which fluids or gases can flow. This dimension is essential in industrial piping, as it determines flow capacity and impacts pressure and velocity within the system."@en ;
    skos:prefLabel "Bore Diameter"@en,
        "Diâmetro do Furo"@pt-br ;
    :hasAttributeScope :TypeLevelAttribute ;
    :hasTypedValue :floatValue ;
    :hasValueCardinality :singleValue .

:BuoyancyTank a owl:Class ;
    dcterms:identifier "BuoyancyTank" ;
    rdfs:subClassOf :SubseaEquipment .

:CO2VolumePercentage a owl:DatatypeProperty ;
    dcterms:accessRights "PUBLIC" ;
    dcterms:identifier "CO2VolumePercentage" ;
    rdfs:subPropertyOf :DomainAttribute ;
    skos:definition "Represents the percentage of carbon dioxide (CO2) in the total volume of the fluid or gas mixture within the pipeline. This value is essential for determining the material selection and design considerations for the flexible subsea pipeline, as CO2 can influence corrosion rates and impact the overall integrity and lifespan of the pipeline."@en ;
    skos:prefLabel "Carbon Dioxide (CO2) Volume Percentage"@en,
        "Porcentagem de Volume de Dióxido de Carbono (CO2)"@pt-br ;
    :hasAttributeScope :InstanceLevelAttribute ;
    :hasTypedValue :floatValue ;
    :hasValueCardinality :singleValue .

:CalculatedAbsoluteBurstPressure a owl:DatatypeProperty ;
    dcterms:accessRights "PUBLIC" ;
    dcterms:identifier "CalculatedAbsoluteBurstPressure" ;
    rdfs:subPropertyOf :DomainAttribute ;
    skos:definition "Represents the estimated absolute pressure at which a component or system is expected to fail or rupture. This property is crucial for determining the maximum safe operating pressure, ensuring that the component can withstand internal forces without bursting."@en ;
    skos:prefLabel "Calculated Absolute Burst Pressure"@en,
        "Pressão Absoluta de Ruptura Calculada"@pt-br ;
    :hasAttributeScope :TypeLevelAttribute ;
    :hasTypedValue :floatValue ;
    :hasValueCardinality :singleValue .

:CheckValve a owl:Class ;
    dcterms:identifier "CheckValve" ;
    rdfs:subClassOf :Valve .

:CivilEngineering a owl:Class ;
    rdfs:label "Civil Engineering"@en,
        "Engenharia Civil"@pt-br ;
    rdfs:subClassOf :TechnicalDiscipline ;
    skos:definition "Engineering discipline focused on the design and construction of infrastructure."@en,
        "Disciplina de engenharia focada no projeto e construção de infraestrutura."@pt-br .

:ClampInternalDiameter a owl:DatatypeProperty ;
    dcterms:accessRights "PUBLIC" ;
    dcterms:identifier "ClampInternalDiameter" ;
    rdfs:subPropertyOf :DomainAttribute ;
    skos:definition "Is the clamp internal diameter"@en ;
    skos:prefLabel "Clamp Internal Diameter"@en,
        "Diâmetro interno do clamp"@pt-br ;
    :hasAttributeScope :TypeLevelAttribute ;
    :hasTypedValue :floatValue ;
    :hasValueCardinality :singleValue .

:CollarInternalDiameter a owl:DatatypeProperty ;
    dcterms:accessRights "PUBLIC" ;
    dcterms:identifier "CollarInternalDiameter" ;
    rdfs:subPropertyOf :DomainAttribute ;
    skos:definition "Inner dimension of the collar, to ensure proper fitting and secure attachment."@en ;
    skos:prefLabel "Collar Internal Diameter"@en,
        "Diâmetro Interno do Colar"@pt-br ;
    :hasAttributeScope :TypeLevelAttribute ;
    :hasTypedValue :floatValue ;
    :hasValueCardinality :singleValue .

:CompositeLayerMaterialType a owl:DatatypeProperty ;
    dcterms:accessRights "PUBLIC" ;
    dcterms:identifier "CompositeLayerMaterialType" ;
    rdfs:subPropertyOf :DomainAttribute ;
    skos:definition "Type of material from which an object is made, allowing for precise documentation and categorisation."@en ;
    skos:prefLabel "Composite Layer Material Type"@en,
        "Tipo de Material da Camada de Compósito"@pt-br ;
    :hasAttributeScope :TypeLevelAttribute ;
    :hasTypedValue :stringValue ;
    :hasValueCardinality :singleValue .

:Content a owl:DatatypeProperty ;
    dcterms:accessRights "PUBLIC" ;
    dcterms:identifier "Content" ;
    rdfs:subClassOf :JustificationAttribute,
        :Registry_GUIDAttribute,
        :StatusAttribute ;
    skos:definition "Text field for capturing observations, notes, or details related to the work. It allows for unstructured information to be recorded."@en ;
    skos:prefLabel "Content"@en ;
    :hasAttributeScope :InstanceLevelAttribute ;
    :hasTypedValue :stringValue ;
    :hasValueCardinality :singleValue .

:Creator a owl:DatatypeProperty ;
    dcterms:accessRights "PUBLIC" ;
    dcterms:identifier "Creator" ;
    rdfs:subClassOf :JustificationAttribute,
        :Registry_GUIDAttribute,
        :StatusAttribute ;
    skos:prefLabel "Creator"@en ;
    :hasAttributeScope :InstanceLevelAttribute ;
    :hasTypedValue :stringValue ;
    :hasValueCardinality :singleValue .

:CreatorId a owl:DatatypeProperty ;
    dcterms:accessRights "PUBLIC" ;
    dcterms:identifier "CreatorId" ;
    rdfs:subClassOf :JustificationAttribute,
        :Registry_GUIDAttribute,
        :StatusAttribute ;
    skos:prefLabel "Creator Id"@en ;
    :hasAttributeScope :InstanceLevelAttribute ;
    :hasTypedValue :stringValue ;
    :hasValueCardinality :singleValue .

:CriticalCurvatureOfSlipping a owl:DatatypeProperty ;
    dcterms:accessRights "PUBLIC" ;
    dcterms:identifier "CriticalCurvatureOfSlipping" ;
    rdfs:subClassOf :BendingStiffnessAttribute ;
    skos:definition "Represents the minimum curvature at which slipping or movement between layers or components begins to occur. This property is essential for assessing the flexibility and mechanical behavior of the structure, ensuring that it can maintain stability and performance under bending without experiencing slippage."@en ;
    skos:prefLabel "Critical Curvature Of Slipping"@en,
        "Curvatura crítica de escorregamento"@pt-br ;
    :hasAttributeScope :TypeLevelAttribute ;
    :hasTypedValue :floatValue ;
    :hasValueCardinality :singleValue .

:DamagingPullInStraightLine a owl:DatatypeProperty ;
    dcterms:accessRights "PUBLIC" ;
    dcterms:identifier "DamagingPullInStraightLine" ;
    rdfs:subPropertyOf :DomainAttribute ;
    skos:definition "Represents the force applied during a straight-line pull-in operation that could cause damage to a component or system. This property is critical for determining safe operational limits during installation, ensuring that the component can withstand the pulling force without suffering structural damage."@en ;
    skos:prefLabel "Damaging Pull In Straight Line"@en,
        "Tração Crítica em Linha Reta"@pt-br ;
    :hasAttributeScope :TypeLevelAttribute ;
    :hasTypedValue :floatValue ;
    :hasValueCardinality :singleValue .

:DiffusionTable_DiffusionCoefficient a owl:DatatypeProperty ;
    dcterms:accessRights "PUBLIC" ;
    dcterms:identifier "DiffusionTable_DiffusionCoefficient" ;
    rdfs:subClassOf :DiffusionTableAttribute ;
    skos:definition "Represents the rate at which particles, molecules, or substances diffuse through a material. This property is important for evaluating how gases or liquids move within or through a material, helping to understand the behavior of the component, where diffusion can affect performance and integrity."@en ;
    skos:prefLabel "Diffusion Coefficient"@en,
        "Coeficiente de difusão"@pt-br ;
    :hasAttributeScope :TypeLevelAttribute ;
    :hasTypedValue :floatValue ;
    :hasValueCardinality :multiValue .

:DiffusionTable_MoleculeIdentifier a owl:DatatypeProperty ;
    dcterms:accessRights "PUBLIC" ;
    dcterms:identifier "DiffusionTable_MoleculeIdentifier" ;
    rdfs:subClassOf :DiffusionTableAttribute ;
    skos:definition "Specifies the type of molecule. This property identifies the particular molecule involved, which is crucial for understanding the material's interaction with or response to different chemical substances."@en,
        "Tipo de Molécula (co2, h2s, ch4, h2o,…)"@pt-br ;
    skos:prefLabel "Molecule Identifier"@en,
        "Identificador de Molécula"@pt-br ;
    :hasAttributeScope :TypeLevelAttribute ;
    :hasTypedValue :stringValue ;
    :hasValueCardinality :multiValue .

:DiffusionTable_PolymerState a owl:DatatypeProperty ;
    dcterms:accessRights "PUBLIC" ;
    dcterms:identifier "DiffusionTable_PolymerState" ;
    rdfs:subClassOf :DiffusionTableAttribute ;
    skos:definition "The state of the polymeric material is specified.. This property is crucial for understanding how the material behaves under different conditions and its suitability for various applications."@en,
        "estado do polímero (plastificado, não plastificado,…)"@pt-br ;
    skos:prefLabel "Polymer State"@en,
        "Estado do Polímero"@pt-br ;
    :hasAttributeScope :TypeLevelAttribute ;
    :hasTypedValue :stringValue ;
    :hasValueCardinality :multiValue .

:DiffusionTable_Temperature a owl:DatatypeProperty ;
    dcterms:accessRights "PUBLIC" ;
    dcterms:identifier "DiffusionTable_Temperature" ;
    rdfs:subClassOf :DiffusionTableAttribute ;
    skos:definition "Represents the thermal condition or measurement of heat for a component or system. This property is important for assessing how the component performs or operates under specific thermal conditions, ensuring it remains within safe and effective operating limits."@en ;
    skos:prefLabel "Temperature"@en,
        "Temperatura"@pt-br ;
    :hasAttributeScope :TypeLevelAttribute ;
    :hasTypedValue :floatValue ;
    :hasValueCardinality :multiValue .

:DimensioningCriteria a owl:DatatypeProperty ;
    dcterms:accessRights "PUBLIC" ;
    dcterms:identifier "DimensioningCriteria" ;
    rdfs:subClassOf :LayingMinimumRadiusTableAttribute ;
    skos:definition "Specifies the criteria used to determine the dimensions, providing guidelines and standards for accurate sizing and ensuring that the structure meets required performance and safety specifications."@en,
        "Critério de dimensionamento de raio mínimo de lançamento. Lista pré definida:Linear interpolation (curvature)Most restrictive value between the neighbouring values"@pt-br ;
    skos:prefLabel "Dimensioning Criteria"@en,
        "Critério de Dimensionamento"@pt-br ;
    :hasAttributeScope :TypeLevelAttribute ;
    :hasTypedValue :stringValue ;
    :hasValueCardinality :singleValue .

:DisplacedVolume a owl:DatatypeProperty ;
    dcterms:accessRights "PUBLIC" ;
    dcterms:identifier "DisplacedVolume" ;
    rdfs:subPropertyOf :DomainAttribute ;
    skos:definition "Refers to the total volume of an object that is submerged or immersed in a fluid. This volume is used to calculate the buoyant force acting on the object and is crucial for understanding its buoyancy and stability in the fluid."@en ;
    skos:prefLabel "Displaced Volume"@en,
        "Volume Deslocado"@pt-br ;
    :hasAttributeScope :TypeLevelAttribute ;
    :hasTypedValue :floatValue ;
    :hasValueCardinality :singleValue .

:DrawingDimensionsTableAttribute a owl:Class ;
    rdfs:label "Drawing Dimensions Table" ;
    rdfs:subPropertyOf :DomainAttribute .

:DrawingDimensionsTable_DimensionDescription a owl:DatatypeProperty ;
    dcterms:accessRights "PUBLIC" ;
    dcterms:identifier "DrawingDimensionsTable_DimensionDescription" ;
    rdfs:subClassOf :DimensionsTableColumn ;
    skos:definition "Provides a detailed description of the dimension. This property explains what the dimension represents, including its relevance and how it relates to other features or components."@en,
        "Descrição (Exemplo: Cota do ponto A ao ponto B)"@pt-br ;
    skos:prefLabel "Dimension Description"@en,
        "Descrição da Dimensão"@pt-br ;
    :hasAttributeScope :TypeLevelAttribute ;
    :hasTypedValue :stringValue ;
    :hasValueCardinality :multiValue .

:DrawingDimensionsTable_DimensionName a owl:DatatypeProperty ;
    dcterms:accessRights "PUBLIC" ;
    dcterms:identifier "DrawingDimensionsTable_DimensionName" ;
    rdfs:subClassOf :DimensionsTableColumn ;
    skos:definition "Indicates the name or label assigned to the dimension. This property identifies the specific dimension, which helps in referencing and distinguishing it from other dimensions."@en ;
    skos:prefLabel "Dimension Name"@en,
        "Nome da dimensão"@pt-br ;
    :hasAttributeScope :TypeLevelAttribute ;
    :hasTypedValue :stringValue ;
    :hasValueCardinality :multiValue .

:DrawingDimensionsTable_DimensionUnit a owl:DatatypeProperty ;
    dcterms:accessRights "PUBLIC" ;
    dcterms:identifier "DrawingDimensionsTable_DimensionUnit" ;
    rdfs:subClassOf :DimensionsTableColumn ;
    skos:definition "Specifies the unit of measurement for the dimension value, expressed in SI units. For linear dimensions, this would be meters or millimeters, while for angles, it would be degrees. This property ensures that all measurements are clear, consistent, and standardized."@en,
        "A unidade pode qualquer uma do SI (Sistema Internacional de Unidades), por exemplo mm, °, etc."@pt-br ;
    skos:prefLabel "Dimension Unit"@en,
        "Unidade de Dimensão"@pt-br ;
    :hasAttributeScope :TypeLevelAttribute ;
    :hasTypedValue :stringValue ;
    :hasValueCardinality :multiValue .

:DrawingDimensionsTable_DimensionValue a owl:DatatypeProperty ;
    dcterms:accessRights "PUBLIC" ;
    dcterms:identifier "DrawingDimensionsTable_DimensionValue" ;
    rdfs:subClassOf :DimensionsTableColumn ;
    skos:definition "Specifies the actual measurement value of the dimension. This property provides the numerical value for the dimension, which is critical for understanding the size and placement of components or features."@en ;
    skos:prefLabel "Dimension Value"@en,
        "Valor da dimensão"@pt-br ;
    :hasAttributeScope :TypeLevelAttribute ;
    :hasTypedValue :floatValue ;
    :hasValueCardinality :multiValue .

:EModVsTempTable_ElasticityModulus a owl:DatatypeProperty ;
    dcterms:accessRights "PUBLIC" ;
    dcterms:identifier "EModVsTempTable_ElasticityModulus" ;
    rdfs:subPropertyOf :DomainAttribute ;
    skos:definition "Represents the modulus of elasticity values corresponding to specific temperatures. This property provides the stiffness or resistance to deformation of the material at each listed temperature, ensuring that the material's mechanical response is understood under varying thermal conditions."@en,
        "Módulo de elasticidade em função da temperatura (Específica para Materiais Poliméricos)"@pt-br ;
    skos:prefLabel "Elasticity Modulus Versus Temperature Table - Elasticity Modulus"@en,
        "Tabela do Módulo de Elasticidade em Função da Temperatura - Módulo de Elasticidade"@pt-br ;
    :hasAttributeScope :TypeLevelAttribute ;
    :hasTypedValue :floatValue ;
    :hasValueCardinality :multiValue .

:EarlyLeakMaxPressTable_Press a owl:DatatypeProperty ;
    dcterms:accessRights "PUBLIC" ;
    dcterms:identifier "EarlyLeakMaxPressTable_Press" ;
    rdfs:subClassOf :EarlyLeakMaxPressTableColumn ;
    skos:definition "The maximum pressure applied during the Early Leak Test, verifying resistance under extreme pressure conditions."@en,
        "Condições de teste dos tramos para Pressão - Máxima - Teste de vazamento hidrostático precoce"@pt-br ;
    skos:prefLabel "Early Leak Maximum Pressure Table - Pressure"@en,
        "Tabela de Pressão Máxima de Vazamento Precoce - Pressão"@pt-br ;
    :hasAttributeScope :InstanceLevelAttribute ;
    :hasTypedValue :floatValue ;
    :hasValueCardinality :multiValue .

:EarlyLeakMaxPressTable_PressIntValStrat a owl:DatatypeProperty ;
    dcterms:accessRights "PUBLIC" ;
    dcterms:identifier "EarlyLeakMaxPressTable_PressIntValStrat" ;
    rdfs:subClassOf :EarlyLeakMaxPressTableAttribute ;
    skos:definition "Strategy used to calculate intermediate values between maximum conditions during the Early Leak Test."@en,
        "Condições de teste dos tramos para Estratégia de valores intermediários - Máximo - Teste de vazamento hidrostático precoce"@pt-br ;
    skos:prefLabel "Early Leak Maximum Pressure Table - Pressure Intermediate Values Strategy"@en,
        "Tabela de Pressão Máxima de Vazamento Precoce - Estratégia de Valores Intermediários de Pressão"@pt-br ;
    :hasAttributeScope :InstanceLevelAttribute ;
    :hasTypedValue :stringValue ;
    :hasValueCardinality :singleValue .

:EarlyLeakMaxPressTable_PressValRef a owl:DatatypeProperty ;
    dcterms:accessRights "PUBLIC" ;
    dcterms:identifier "EarlyLeakMaxPressTable_PressValRef" ;
    rdfs:subClassOf :EarlyLeakMaxPressTableColumn ;
    skos:definition "Specifies the reference pressure used to determine the Early Leak Maximum Pressure value."@en,
        "Comentários Condições de teste dos tramos para - Máximo - Teste de vazamento hidrostático precoce"@pt-br ;
    skos:prefLabel "Early Leak Maximum Pressure Table - Pressure Value Reference"@en,
        "Tabela de Pressão Máxima de Vazamento Precoce - Referência de Valor de Pressão"@pt-br ;
    :hasAttributeScope :InstanceLevelAttribute ;
    :hasTypedValue :stringValue ;
    :hasValueCardinality :multiValue .

:EarlyLeakMaxPressTable_PressValRefMult a owl:DatatypeProperty ;
    dcterms:accessRights "PUBLIC" ;
    dcterms:identifier "EarlyLeakMaxPressTable_PressValRefMult" ;
    rdfs:subClassOf :EarlyLeakMaxPressTableColumn ;
    skos:definition "The multiplier applied to the reference pressure to determine the Early Leak Maximum Pressure value."@en,
        "Early Leak Maximum Pressure Table - Pressure Value Reference Multiplier"@pt-br ;
    skos:prefLabel "Early Leak Maximum Pressure Table - Pressure Value Reference Multiplier"@en,
        "Tabela de Pressão Máxima de Vazamento Precoce - Multiplicador de Referência de Valor de Pressão"@pt-br ;
    :hasAttributeScope :InstanceLevelAttribute ;
    :hasTypedValue :floatValue ;
    :hasValueCardinality :multiValue .

:EarlyLeakMaxPressTable_TensLimit a owl:DatatypeProperty ;
    dcterms:accessRights "PUBLIC" ;
    dcterms:identifier "EarlyLeakMaxPressTable_TensLimit" ;
    rdfs:subClassOf :EarlyLeakMaxPressTableColumn ;
    skos:definition "Tensile limit condition that must be respected to avoid damaging the tested product."@en,
        "Condições de teste dos tramos para Tensão - Máxima - Teste de vazamento hidrostático precoce"@pt-br ;
    skos:prefLabel "Early Leak Maximum Pressure Table - Tensile Limit"@en,
        "Tabela de Pressão Máxima de Vazamento Precoce - Limite de Tração"@pt-br ;
    :hasAttributeScope :InstanceLevelAttribute ;
    :hasTypedValue :floatValue ;
    :hasValueCardinality :multiValue .

:EarlyLeakMaxPressTable_TensLimitValRef a owl:DatatypeProperty ;
    dcterms:accessRights "PUBLIC" ;
    dcterms:identifier "EarlyLeakMaxPressTable_TensLimitValRef" ;
    rdfs:subClassOf :EarlyLeakMaxPressTableColumn ;
    skos:definition "Indicates the basis used to establish the tensile limit value during the Early Leak Maximum Pressure Test, ensuring the product's tensile strength is respected to avoid damage."@en ;
    skos:prefLabel "Early Leak Maximum Pressure Table - Tensile Limit Value Reference"@en,
        "Tabela de Pressão Máxima de Vazamento Precoce - Referência do Limite de Tração"@pt-br ;
    :hasAttributeScope :InstanceLevelAttribute ;
    :hasTypedValue :stringValue ;
    :hasValueCardinality :multiValue .

:EarlyLeakNomPressTable_Press a owl:DatatypeProperty ;
    dcterms:accessRights "PUBLIC" ;
    dcterms:identifier "EarlyLeakNomPressTable_Press" ;
    rdfs:subClassOf :EarlyLeakNomPressTableColumn ;
    skos:definition "The nominal pressure applied during the Early Leak Test, verifying standard operational conditions for leakage detection."@en,
        "Condições de teste dos tramos para Pressão - Nominal - Teste de vazamento hidrostático precoce"@pt-br ;
    skos:prefLabel "Early Leak Nominal Pressure Table - Pressure"@en,
        "Tabela de Pressão Nominal de Vazamento Precoce - Pressão"@pt-br ;
    :hasAttributeScope :InstanceLevelAttribute ;
    :hasTypedValue :floatValue ;
    :hasValueCardinality :multiValue .

:EarlyLeakNomPressTable_PressIntValStrat a owl:DatatypeProperty ;
    dcterms:accessRights "PUBLIC" ;
    dcterms:identifier "EarlyLeakNomPressTable_PressIntValStrat" ;
    rdfs:subClassOf :EarlyLeakNomPressTableAttribute ;
    skos:definition "Strategy used to calculate intermediate Pressure values between nominal conditions during the Early Leak Test."@en,
        "Condições de teste dos tramos para Estratégia de valores intermediários - Nominal - Teste de vazamento hidrostático precoce"@pt-br ;
    skos:prefLabel "Early Leak Nominal Pressure Table - Pressure Intermediate Values Strategy"@en,
        "Tabela de Pressão Nominal de Vazamento Precoce - Estratégia de Valores Intermediários de Pressão"@pt-br ;
    :hasAttributeScope :InstanceLevelAttribute ;
    :hasTypedValue :stringValue ;
    :hasValueCardinality :singleValue .

:EarlyLeakNomPressTable_PressValRef a owl:DatatypeProperty ;
    dcterms:accessRights "PUBLIC" ;
    dcterms:identifier "EarlyLeakNomPressTable_PressValRef" ;
    rdfs:subClassOf :EarlyLeakNomPressTableColumn ;
    skos:definition "Specifies the reference pressure used to determine the Early Leak Nominal Pressure value."@en,
        "Comentários Condições de teste dos tramos para - Nominal - Teste de vazamento hidrostático precoce"@pt-br ;
    skos:prefLabel "Early Leak Nominal Pressure Table - Pressure Value Reference"@en,
        "Tabela de Pressão Nominal de Vazamento Precoce - Referência de Valor de Pressão"@pt-br ;
    :hasAttributeScope :InstanceLevelAttribute ;
    :hasTypedValue :stringValue ;
    :hasValueCardinality :multiValue .

:EarlyLeakNomPressTable_PressValRefMult a owl:DatatypeProperty ;
    dcterms:accessRights "PUBLIC" ;
    dcterms:identifier "EarlyLeakNomPressTable_PressValRefMult" ;
    rdfs:subClassOf :EarlyLeakNomPressTableColumn ;
    skos:definition "The multiplier applied to the reference pressure to determine the Early Leak Nominal Pressure value."@en ;
    skos:prefLabel "Early Leak Nominal Pressure Table - Pressure Value Reference Multiplier"@en,
        "Tabela de Pressão Nominal de Vazamento Precoce - Multiplicador de Referência de Valor de Pressão"@pt-br ;
    :hasAttributeScope :InstanceLevelAttribute ;
    :hasTypedValue :floatValue ;
    :hasValueCardinality :multiValue .

:EarlyLeakNomPressTable_TensLimit a owl:DatatypeProperty ;
    dcterms:accessRights "PUBLIC" ;
    dcterms:identifier "EarlyLeakNomPressTable_TensLimit" ;
    rdfs:subClassOf :EarlyLeakNomPressTableColumn ;
    skos:definition "Tensile limit condition that must be respected to avoid damaging the tested product."@en,
        "Condições de teste dos tramos para Tensão - Nominal - Teste de vazamento hidrostático precoce"@pt-br ;
    skos:prefLabel "Early Leak Nominal Pressure Table - Tensile Limit"@en,
        "Tabela de Pressão Nominal de Vazamento Precoce - Limite de Tração"@pt-br ;
    :hasAttributeScope :InstanceLevelAttribute ;
    :hasTypedValue :floatValue ;
    :hasValueCardinality :multiValue .

:EarlyLeakNomPressTable_TensLimitValRef a owl:DatatypeProperty ;
    dcterms:accessRights "PUBLIC" ;
    dcterms:identifier "EarlyLeakNomPressTable_TensLimitValRef" ;
    rdfs:subClassOf :EarlyLeakNomPressTableColumn ;
    skos:definition "Indicates the basis used to establish the tensile limit value during the Early Leak Nominal Pressure Test, ensuring the product's tensile strength is respected to avoid damage."@en ;
    skos:prefLabel "Early Leak Nominal Pressure Table - Tensile Limit Value Reference"@en,
        "Tabela de Pressão Nominal de Vazamento Precoce - Referência do Limite de Tração"@pt-br ;
    :hasAttributeScope :InstanceLevelAttribute ;
    :hasTypedValue :stringValue ;
    :hasValueCardinality :multiValue .

:ElasticityModulusAt23Degrees a owl:DatatypeProperty ;
    dcterms:accessRights "PUBLIC" ;
    dcterms:identifier "ElasticityModulusAt23Degrees" ;
    rdfs:subPropertyOf :DomainAttribute ;
    skos:definition "Specifies the modulus of elasticity of the material at 23 degrees Celsius, indicating its stiffness or resistance to deformation under stress at this temperature. This property is crucial for determining how the flexible structure responds to mechanical loads, ensuring that it maintains structural integrity."@en,
        "Módulo de elasticidade a 23 graus Celsius (Específica para Materiais Metálicos e Poliméricos)"@pt-br ;
    skos:prefLabel "Elasticity Modulus At 23 Degrees"@en,
        "Módulo de Elasticidade a 23 Graus Celsius"@pt-br ;
    :hasAttributeScope :TypeLevelAttribute ;
    :hasTypedValue :floatValue ;
    :hasValueCardinality :singleValue .

:EquipmentLocation a owl:Class ;
    dcterms:identifier "EquipmentLocation" ;
    rdfs:subClassOf :PointLocation ;
    skos:definition "Base for installation sites for large underwater equipment."@en ;
    skos:prefLabel "Equipment Location"@en,
        "Localização de Equipamento"@pt-br .

:ErosionalVelocity a owl:DatatypeProperty ;
    dcterms:accessRights "PUBLIC" ;
    dcterms:identifier "ErosionalVelocity" ;
    rdfs:subPropertyOf :DomainAttribute ;
    skos:definition "Represents the maximum velocity of a fluid at which erosion of the material begins to occur. This property is crucial for determining the operational limits of the system, ensuring that the material can withstand fluid flow without suffering erosive damage."@en ;
    skos:prefLabel "Erosional Velocity"@en,
        "Velocidade erosional"@pt-br ;
    :hasAttributeScope :TypeLevelAttribute ;
    :hasTypedValue :stringValue ;
    :hasValueCardinality :singleValue .

:ExecutiveProjectRevision a owl:DatatypeProperty ;
    dcterms:accessRights "PUBLIC" ;
    dcterms:identifier "ExecutiveProjectRevision" ;
    rdfs:subPropertyOf :DomainAttribute ;
    skos:definition "Indicates the revision number of the executive project, represented as a numeric value that is incremented with each new submission (e.g., 0000, 0001, 0002), stored as text for consistency in formatting."@en,
        "Revisão do projeto executivo  Valor numérico incrementado a cada novo envio (0000, 0001, 0002 e etc.) como texto"@pt-br ;
    skos:prefLabel "Executive Project Revision"@en,
        "Revisão do Projeto Executivo"@pt-br ;
    :hasAttributeScope :InstanceLevelAttribute ;
    :hasTypedValue :stringValue ;
    :hasValueCardinality :singleValue .

:ExternalDiameter a owl:DatatypeProperty ;
    dcterms:accessRights "PUBLIC" ;
    dcterms:identifier "ExternalDiameter" ;
    rdfs:subPropertyOf :DomainAttribute ;
    skos:definition "Distance measured across the outermost points, passing through the center."@en ;
    skos:prefLabel "External Diameter"@en,
        "Diâmetro externo"@pt-br ;
    :hasAttributeScope :TypeLevelAttribute ;
    :hasTypedValue :floatValue ;
    :hasValueCardinality :singleValue .

:FatMaxPress a owl:DatatypeProperty ;
    dcterms:accessRights "PUBLIC" ;
    dcterms:identifier "FatMaxPress" ;
    rdfs:subClassOf :HydrostaticPressureTestsAttribute ;
    skos:definition "The maximum pressure applied during the Factory Acceptance Test (FAT) to ensure the equipment can withstand extreme conditions."@en,
        "Condições de teste dos tramos para Pressão - Máxima - FAT hidrostática"@pt-br ;
    skos:prefLabel "Factory Acceptance Test Maximum Pressure"@en,
        "Pressão Máxima para o Teste de Aceitação na Fábrica"@pt-br ;
    :hasAttributeScope :InstanceLevelAttribute ;
    :hasTypedValue :floatValue ;
    :hasValueCardinality :singleValue .

:FatMaxPressValRef a owl:DatatypeProperty ;
    dcterms:accessRights "PUBLIC" ;
    dcterms:identifier "FatMaxPressValRef" ;
    rdfs:subClassOf :HydrostaticPressureTestsAttribute ;
    skos:definition "Specifies the reference pressure used to determine the FAT maximum pressure value."@en,
        "Comentários Condições de teste dos tramos para - Máximo - FAT hidrostático"@pt-br ;
    skos:prefLabel "Factory Acceptance Test Maximum Pressure Value Reference"@en,
        "Referência de Valor de Pressão Máxima para o Teste de Aceitação na Fábrica"@pt-br ;
    :hasAttributeScope :InstanceLevelAttribute ;
    :hasTypedValue :stringValue ;
    :hasValueCardinality :singleValue .

:FatMaxPressValRefMult a owl:DatatypeProperty ;
    dcterms:accessRights "PUBLIC" ;
    dcterms:identifier "FatMaxPressValRefMult" ;
    rdfs:subClassOf :HydrostaticPressureTestsAttribute ;
    skos:definition "The multiplier applied to the reference pressure to determine the FAT maximum pressure value."@en ;
    skos:prefLabel "Factory Acceptance Test Maximum Pressure Value Reference Multiplier"@en,
        "Multiplicador de Referência de Valor de Pressão Máxima para Teste de Aceitação na Fábrica"@pt-br ;
    :hasAttributeScope :InstanceLevelAttribute ;
    :hasTypedValue :floatValue ;
    :hasValueCardinality :singleValue .

:FatNomPress a owl:DatatypeProperty ;
    dcterms:accessRights "PUBLIC" ;
    dcterms:identifier "FatNomPress" ;
    rdfs:subClassOf :HydrostaticPressureTestsAttribute ;
    skos:definition "The nominal pressure applied during the Factory Acceptance Test (FAT), simulating typical operating conditions to verify equipment performance."@en,
        "Condições de teste dos tramos para Pressão - Nominal - FAT hidrostático"@pt-br ;
    skos:prefLabel "Factory Acceptance Test Nominal Pressure"@en,
        "Pressão Nominal para o Teste de Aceitação na Fábrica"@pt-br ;
    :hasAttributeScope :InstanceLevelAttribute ;
    :hasTypedValue :floatValue ;
    :hasValueCardinality :singleValue .

:FatNomPressValRef a owl:DatatypeProperty ;
    dcterms:accessRights "PUBLIC" ;
    dcterms:identifier "FatNomPressValRef" ;
    rdfs:subClassOf :HydrostaticPressureTestsAttribute ;
    skos:definition "Specifies the reference pressure used to determine the FAT nominal pressure value."@en,
        "Comentários Condições de teste dos tramos para - Nominal - FAT hidrostático"@pt-br ;
    skos:prefLabel "Factory Acceptance Test Nominal Pressure Value Reference"@en,
        "Referência de Valor de Pressão Nominal para o Teste de Aceitação na Fábrica"@pt-br ;
    :hasAttributeScope :InstanceLevelAttribute ;
    :hasTypedValue :stringValue ;
    :hasValueCardinality :singleValue .

:FatNomPressValRefMult a owl:DatatypeProperty ;
    dcterms:accessRights "PUBLIC" ;
    dcterms:identifier "FatNomPressValRefMult" ;
    rdfs:subClassOf :HydrostaticPressureTestsAttribute ;
    skos:definition "The multiplier applied to the reference pressure to determine the FAT nominal pressure value."@en ;
    skos:prefLabel "Factory Acceptance Test Nominal Pressure Value Reference Multiplier"@en,
        "Multiplicador de Referência de Valor de Pressão Nominal para Teste de Aceitação na Fábrica"@pt-br ;
    :hasAttributeScope :InstanceLevelAttribute ;
    :hasTypedValue :floatValue ;
    :hasValueCardinality :singleValue .

:FlangeFaceType a owl:DatatypeProperty ;
    dcterms:accessRights "PUBLIC" ;
    dcterms:identifier "FlangeFaceType" ;
    rdfs:subClassOf :FlangeAttribute ;
    skos:definition "Specific design of the sealing surface used to ensure a secure, leak-tight connection. The face type plays a crucial role in maintaining the integrity of the seal under the extreme pressures and temperatures. It is engineered to prevent leaks, withstand high mechanical loads, and provide long-term durability. The appropriate face type is chosen based on factors such as pressure rating, sealing requirements, and environmental conditions."@en ;
    skos:prefLabel "Flange Face Type"@en,
        "Tipo da Face do Flange"@pt-br ;
    :hasAttributeScope :TypeLevelAttribute ;
    :hasTypedValue :stringValue ;
    :hasValueCardinality :singleValue .

:FlexibleStructureServicesList a owl:DatatypeProperty ;
    dcterms:accessRights "PUBLIC" ;
    dcterms:identifier "FlexibleStructureServicesList" ;
    rdfs:subPropertyOf :DomainAttribute ;
    skos:definition "Indicates the list of services that the flexible structure is capable of performing as part of a flexible pipeline. Multiple values can be selected, defining the operational roles the structure is designed to execute."@en ;
    skos:prefLabel "Flexible Structure Services List"@en,
        "Lista de Serviços da Estrutura Flexível"@pt-br ;
    :hasAttributeScope :TypeLevelAttribute ;
    :hasTypedValue :stringValue ;
    :hasValueCardinality :multiValue .

:FractureToughness a owl:DatatypeProperty ;
    dcterms:accessRights "PUBLIC" ;
    dcterms:identifier "FractureToughness" ;
    rdfs:subPropertyOf :DomainAttribute ;
    skos:definition "Represents the material's ability to resist fracture when subjected to stress, particularly in the presence of flaws or cracks. This property is essential for assessing the material's capacity to withstand cracking or failure under load conditions."@en,
        "Tenacidade à fratura (Específica para Materiais Metálicos)"@pt-br ;
    skos:prefLabel "Fracture Toughness"@en,
        "Tenacidade à Fratura"@pt-br ;
    :hasAttributeScope :TypeLevelAttribute ;
    :hasTypedValue :floatValue ;
    :hasValueCardinality :singleValue .

:FrictionCoefBetweenPipeAndTensioner a owl:DatatypeProperty ;
    dcterms:accessRights "PUBLIC" ;
    dcterms:identifier "FrictionCoefBetweenPipeAndTensioner" ;
    rdfs:subPropertyOf :DomainAttribute ;
    skos:definition "Represents the coefficient of friction between the pipe and the tensioner during installation or operation. This property is critical for determining the resistance to sliding between the two surfaces, influencing the tension control and handling of the pipe."@en,
        "Coeficiente de atrito entre a sapata e a capa externa (passagem tensionador)"@pt-br ;
    skos:prefLabel "Friction Coefficient Between Pipe And Tensioner"@en,
        "Coeficiente de Atrito entre o Duto e o Tensionador"@pt-br ;
    :hasAttributeScope :TypeLevelAttribute ;
    :hasTypedValue :floatValue ;
    :hasValueCardinality :singleValue .

:FrictionCoefficientTighteningTable_CoefficientOfFriction a owl:DatatypeProperty ;
    dcterms:accessRights "PUBLIC" ;
    dcterms:identifier "FrictionCoefficientTighteningTable_CoefficientOfFriction" ;
    rdfs:subClassOf :CrushingFrictionCoefficientTighteningTableColumn ;
    skos:definition "Represents the ratio that describes the force of friction between two surfaces in contact, relative to the normal force pressing them together. This property is important for evaluating the resistance to sliding or movement, ensuring proper performance of components under operational conditions."@en ;
    skos:prefLabel "Coefficient Of Friction"@en,
        "Coeficiente de Atrito"@pt-br ;
    :hasAttributeScope :TypeLevelAttribute ;
    :hasTypedValue :floatValue ;
    :hasValueCardinality :multiValue .

:FrictionCoefficientTighteningTable_TighteningPerTrack a owl:DatatypeProperty ;
    dcterms:accessRights "PUBLIC" ;
    dcterms:identifier "FrictionCoefficientTighteningTable_TighteningPerTrack" ;
    rdfs:subClassOf :CrushingFrictionCoefficientTighteningTableColumn ;
    skos:definition "Indicates the amount of tightening applied per track during an operation. This property is important for ensuring consistent force distribution across multiple tracks, helping to maintain proper alignment and secure attachment during the tightening process."@en ;
    skos:prefLabel "Tightening Per Track"@en,
        "Aperto por lagarta"@pt-br ;
    :hasAttributeScope :TypeLevelAttribute ;
    :hasTypedValue :floatValue ;
    :hasValueCardinality :multiValue .

:GalvanicMaterial a owl:DatatypeProperty ;
    dcterms:accessRights "PUBLIC" ;
    dcterms:identifier "GalvanicMaterial" ;
    rdfs:subPropertyOf :DomainAttribute ;
    skos:definition "Refers to the material used in galvanic protection systems, which is typically a metal or alloy designed to corrode in place of the protected structure. This material is selected for its ability to act as a sacrificial anode in a galvanic cell, thereby preventing corrosion of the primary structure, such as a subsea flexible pipeline. The choice of galvanic material is critical for the long-term protection and integrity of the pipeline system."@en ;
    skos:prefLabel "Galvanic Material"@en,
        "Material Galvânico"@pt-br ;
    :hasAttributeScope :TypeLevelAttribute ;
    :hasTypedValue :stringValue ;
    :hasValueCardinality :singleValue .

:GrooveDiameter a owl:DatatypeProperty ;
    dcterms:accessRights "PUBLIC" ;
    dcterms:identifier "GrooveDiameter" ;
    rdfs:subPropertyOf :DomainAttribute ;
    skos:definition "Specifies the diameter of the end fitting at the location where the groove is machined. This measurement is crucial for ensuring that the groove correctly accommodates the end fitting during installation on a vessel. The part diameter at the groove location ensures proper alignment and secure attachment of the end fitting to the installation equipment or support system."@en ;
    skos:prefLabel "Groove Diameter"@en,
        "Diâmetro do Groove"@pt-br ;
    :hasAttributeScope :InstanceLevelAttribute ;
    :hasTypedValue :floatValue ;
    :hasValueCardinality :singleValue .

:GrooveHeight a owl:DatatypeProperty ;
    dcterms:accessRights "PUBLIC" ;
    dcterms:identifier "GrooveHeight" ;
    rdfs:subPropertyOf :DomainAttribute ;
    skos:definition "Specifies the vertical dimension of the groove from its base to the top edge. This measurement is crucial for ensuring that the groove can accommodate the intended components or fittings properly, allowing for a secure and precise fit. The groove height helps to determine the correct depth and functionality of the groove in relation to the end fitting and the overall installation process."@en ;
    skos:prefLabel "Groove Height"@en,
        "Altura do Groove"@pt-br ;
    :hasAttributeScope :InstanceLevelAttribute ;
    :hasTypedValue :floatValue ;
    :hasValueCardinality :singleValue .

:GrooveMinimumSupportArea a owl:DatatypeProperty ;
    dcterms:accessRights "PUBLIC" ;
    dcterms:identifier "GrooveMinimumSupportArea" ;
    rdfs:subPropertyOf :DomainAttribute ;
    skos:definition "Specifies the minimum required area of the support surface within the groove. This measurement is crucial for ensuring that the groove provides adequate support and stability for the components or fittings it interfaces with. A sufficient support area helps prevent misalignment and ensures that the components are securely held in place during operation and installation."@en ;
    skos:prefLabel "Groove Minimum Support Area"@en,
        "Área Mínima de Apoio no Groove"@pt-br ;
    :hasAttributeScope :InstanceLevelAttribute ;
    :hasTypedValue :floatValue ;
    :hasValueCardinality :singleValue .

:GrooveSupportSurfaceDiameter a owl:DatatypeProperty ;
    dcterms:accessRights "PUBLIC" ;
    dcterms:identifier "GrooveSupportSurfaceDiameter" ;
    rdfs:subPropertyOf :DomainAttribute ;
    skos:definition "Indicates the diameter of the support surface within the groove. This measurement is critical for ensuring that the groove provides sufficient contact area for the components it interfaces with, contributing to a stable and secure fit."@en ;
    skos:prefLabel "Groove Support Surface Diameter"@en,
        "Diâmetro da superfície de apoio do acessório"@pt-br ;
    :hasAttributeScope :InstanceLevelAttribute ;
    :hasTypedValue :floatValue ;
    :hasValueCardinality :singleValue .

:GrooveSupportSurfaceFilletRadius a owl:DatatypeProperty ;
    dcterms:accessRights "PUBLIC" ;
    dcterms:identifier "GrooveSupportSurfaceFilletRadius" ;
    rdfs:subPropertyOf :DomainAttribute ;
    skos:definition "Indicates the radius of the fillet on the support surface of the end fitting. This fillet is a rounded corner or edge designed to reduce stress concentrations and enhance the structural integrity of the connection. The radius measurement is crucial for ensuring that the end fitting aligns properly with other components and provides a smooth, stable interface."@en,
        "Adoçamento (Superfície de apoio) do acessório"@pt-br ;
    skos:prefLabel "Groove Support Surface Fillet Radius"@en,
        "Raio de Chanframento (Superfície de Apoio) do Acessório"@pt-br ;
    :hasAttributeScope :InstanceLevelAttribute ;
    :hasTypedValue :floatValue ;
    :hasValueCardinality :singleValue .

:GrvCntrPntDstnceFrmTermFlange a owl:DatatypeProperty ;
    dcterms:accessRights "PUBLIC" ;
    dcterms:identifier "GrvCntrPntDstnceFrmTermFlange" ;
    rdfs:subPropertyOf :DomainAttribute ;
    skos:definition "Distance from the center of the groove to the outer edge of the termination flange, the flange where the other end fitting is connected. This measurement provides the position of the groove relative to the termination flange for precise identification of a specific groove within the end fitting"@en,
        "Distância do centro do groove até a borda externa do flange de terminação, o flange onde o outro end fitting é conectado. Esta medição fornece a posição do groove em relação ao flange para a identificação precisa de um groove específico dentro do end fitting."@pt-br ;
    skos:prefLabel "Groove Center Point Distance From Termination Flange"@en,
        "Distância do Ponto Central do Groove até o Flange de Terminação"@pt-br ;
    :hasAttributeScope :InstanceLevelAttribute ;
    :hasTypedValue :floatValue ;
    :hasValueCardinality :singleValue .

:H2SVolumeConcentration a owl:DatatypeProperty ;
    dcterms:accessRights "PUBLIC" ;
    dcterms:identifier "H2SVolumeConcentration" ;
    rdfs:subPropertyOf :DomainAttribute ;
    skos:definition "Represents the concentration of hydrogen sulfide (H2S) in the total volume of the gas mixture, expressed in parts per million by volume (ppmv). This value is crucial for assessing material compatibility and corrosion risks in subsea flexible pipelines, as H2S is highly corrosive and can significantly impact the integrity and lifespan of the pipeline. Accurate measurement of H2S concentration is essential for ensuring the safe and reliable operation of the pipeline in harsh environments."@en ;
    skos:prefLabel "Hydrogen Sulfide (H2S) Volume Concentration"@en,
        "Concentração Volumétrica de Sulfeto de Hidrogênio (H2S)"@pt-br ;
    :hasAttributeScope :InstanceLevelAttribute ;
    :hasTypedValue :floatValue ;
    :hasValueCardinality :singleValue .

:HardwareItem a owl:Class ;
    dcterms:identifier "HardwareItem" ;
    rdfs:subClassOf :Component ;
    skos:definition "Simple mechanical items such as pipe components, etc."@en ;
    skos:prefLabel "Hardware Item"@en,
        "Item de Hardware"@pt-br ;
    :hasAttribute :DisplacedVolume,
        :DrawingDimensionsTable_DimensionDescription,
        :DrawingDimensionsTable_DimensionName,
        :DrawingDimensionsTable_DimensionUnit,
        :DrawingDimensionsTable_DimensionValue,
        :IdInUnifilarDiagram,
        :InternalVolume,
        :ManufacturerDefinedMaterialName,
        :Mass,
        :MaterialSupplierName,
        :PartNumber,
        :ProjectDrawingCode,
        :ProjectDrawingRevision,
        :SupplierProvidedMaterialName .

:HasFaceORing a owl:DatatypeProperty ;
    dcterms:accessRights "PUBLIC" ;
    dcterms:identifier "HasFaceORing" ;
    rdfs:subPropertyOf :DomainAttribute ;
    skos:definition "Indicates whether the item has a face oring (TRUE) or not (FALSE)."@en ;
    skos:prefLabel "Has Face ORing"@en,
        "Possui ORing na Face"@pt-br ;
    :hasAttributeScope :TypeLevelAttribute ;
    :hasTypedValue :booleanValue ;
    :hasValueCardinality :singleValue .

:HasModaSensor a owl:DatatypeProperty ;
    dcterms:accessRights "PUBLIC" ;
    dcterms:identifier "HasModaSensor" ;
    rdfs:subPropertyOf :DomainAttribute ;
    skos:definition "Indicates whether the item includes a MODA sensor (TRUE) or Not (FALSE)."@en ;
    skos:prefLabel "Has Moda Sensor"@en,
        "Possui Sensor MODA"@pt-br ;
    :hasAttributeScope :TypeLevelAttribute ;
    :hasTypedValue :booleanValue ;
    :hasValueCardinality :singleValue .

:HasN2InjectionPort a owl:DatatypeProperty ;
    dcterms:accessRights "PUBLIC" ;
    dcterms:identifier "HasN2InjectionPort" ;
    rdfs:subPropertyOf :DomainAttribute ;
    skos:definition "Indicates whether the item includes a nitrogen (N2) injection port (TRUE) or Not (FALSE)."@en ;
    skos:prefLabel "Has N2 Injection Port"@en,
        "Possui Porta de Injeção de Nitrogênio"@pt-br ;
    :hasAttributeScope :TypeLevelAttribute ;
    :hasTypedValue :booleanValue ;
    :hasValueCardinality :singleValue .

:HasThermalInsulation a owl:DatatypeProperty ;
    dcterms:accessRights "PUBLIC" ;
    dcterms:identifier "HasThermalInsulation" ;
    rdfs:subPropertyOf :DomainAttribute ;
    skos:prefLabel "Has Thermal Insulation"@en,
        "Possui isolamento térmico"@pt-br ;
    :hasAttributeScope :TypeLevelAttribute ;
    :hasTypedValue :booleanValue ;
    :hasValueCardinality :singleValue .

:HydrostaticCollapseAbsPressDry a owl:DatatypeProperty ;
    dcterms:accessRights "PUBLIC" ;
    dcterms:identifier "HydrostaticCollapseAbsPressDry" ;
    rdfs:subPropertyOf :DomainAttribute ;
    skos:definition "Represents the absolute pressure at which a component or material will collapse under hydrostatic forces when in a dry state. This property is important for evaluating the material's ability to withstand external pressure without deformation or failure."@en,
        "Pressão Absoluta de colapso hidrostático, anular seco, linha reta"@pt-br ;
    skos:prefLabel "Hydrostatic Collapse Absolute Pressure Dry"@en,
        "Pressão Absoluta de Colapso Hidrostático a Seco"@pt-br ;
    :hasAttributeScope :TypeLevelAttribute ;
    :hasTypedValue :floatValue ;
    :hasValueCardinality :singleValue .

:IndividualAnodeMass a owl:DatatypeProperty ;
    dcterms:accessRights "PUBLIC" ;
    dcterms:identifier "IndividualAnodeMass" ;
    rdfs:subPropertyOf :DomainAttribute ;
    skos:definition "Total mass of the sacrificial anode material within each individual anode."@en ;
    skos:prefLabel "Individual Anode Mass"@en,
        "Massa Individual do Anodo"@pt-br ;
    :hasAttributeScope :TypeLevelAttribute ;
    :hasTypedValue :floatValue ;
    :hasValueCardinality :singleValue .

:InsideTemperature a owl:DatatypeProperty ;
    dcterms:accessRights "PUBLIC" ;
    dcterms:identifier "InsideTemperature" ;
    rdfs:subClassOf :BendingStiffnessAttribute ;
    skos:definition "Represents the internal temperature within a component or system. This property is important for assessing the thermal conditions inside the system, ensuring that it operates within safe temperature limits, particularly in subsea environments where temperature control is essential for maintaining performance and integrity."@en ;
    skos:prefLabel "Inside Temperature"@en,
        "Temperatura Interna"@pt-br ;
    :hasAttributeScope :TypeLevelAttribute ;
    :hasTypedValue :floatValue ;
    :hasValueCardinality :singleValue .

:IntermediateValuesStrategy a owl:DatatypeProperty ;
    dcterms:accessRights "PUBLIC" ;
    dcterms:identifier "IntermediateValuesStrategy" ;
    rdfs:subClassOf :BendingStiffnessAttribute,
        :CrushingFrictionCoefficientTighteningTableAttribute,
        :CrushingMaximumAllowableTensionTableAttribute,
        :CrushingMaximumAllowableTighteningTableAttribute ;
    skos:definition "Defines the approach used to handle or calculate intermediate values between specified data points. This property is important for ensuring accuracy in analysis or simulations, particularly when determining values that fall between measured or specified conditions."@en ;
    skos:prefLabel "Intermediate Values Strategy"@en,
        "Estratégia para Valores Intermediários"@pt-br ;
    :hasAttributeScope :TypeLevelAttribute ;
    :hasTypedValue :stringValue ;
    :hasValueCardinality :singleValue .

:InternalIncidentalPressureTable_PositionReference a owl:DatatypeProperty ;
    dcterms:accessRights "PUBLIC" ;
    dcterms:identifier "InternalIncidentalPressureTable_PositionReference" ;
    rdfs:subClassOf :InternalIncidentalPressureTable ;
    skos:definition "Identifies the specific point along the pipeline. This serves as the reference for vertical position and pressure values."@en,
        "Valores válidos:Top (Para a conexão topside - E.g. Conector superior)TDPSubSeaConnection (Ex. ANM)"@pt-br ;
    skos:prefLabel "Position Reference"@en,
        "Referência de Posição"@pt-br ;
    :hasAttributeScope :InstanceLevelAttribute ;
    :hasTypedValue :stringValue ;
    :hasValueCardinality :multiValue .

:InternalIncidentalPressureTable_Pressure a owl:DatatypeProperty ;
    dcterms:accessRights "PUBLIC" ;
    dcterms:identifier "InternalIncidentalPressureTable_Pressure" ;
    rdfs:subClassOf :InternalIncidentalPressureTable ;
    skos:definition "Indicates the force exerted per unit area on the surface of a material or component. This property is critical for evaluating how the component responds to external or internal forces, ensuring it can withstand operational pressure conditions."@en ;
    skos:prefLabel "Pressure"@en,
        "Pressão"@pt-br ;
    :hasAttributeScope :InstanceLevelAttribute ;
    :hasTypedValue :floatValue ;
    :hasValueCardinality :multiValue .

:InternalIncidentalPressureTable_VPosWRTWaterline a owl:DatatypeProperty ;
    dcterms:accessRights "PUBLIC" ;
    dcterms:identifier "InternalIncidentalPressureTable_VPosWRTWaterline" ;
    rdfs:subClassOf :InternalIncidentalPressureTable ;
    skos:definition "Vertical position with respect to the waterline, where positive values indicate points above the water and negative values indicate points below. The platform's maximum draft is considered when applicable."@en,
        "Valores negativos para pontos submersos, e valores positivos para pontos acima da água. Considerando calado máximo da plataforma, quando aplicável."@pt-br ;
    skos:prefLabel "Vertical Position With Respect To Waterline"@en,
        "Posição Vertical em Relação à Linha D'Água"@pt-br ;
    :hasAttributeScope :InstanceLevelAttribute ;
    :hasTypedValue :intValue ;
    :hasValueCardinality :multiValue .

:InternalVolume a owl:DatatypeProperty ;
    dcterms:accessRights "PUBLIC" ;
    dcterms:identifier "InternalVolume" ;
    rdfs:subPropertyOf :DomainAttribute ;
    skos:definition "Refers to the volume of space within an object that can be occupied by a fluid when the object is fully filled or immersed. This property is essential for understanding the capacity and fluid-holding capabilities of the accessory."@en ;
    skos:prefLabel "Internal Volume"@en,
        "Volume interno"@pt-br ;
    :hasAttributeScope :TypeLevelAttribute ;
    :hasTypedValue :floatValue ;
    :hasValueCardinality :singleValue .

:IsSpare a owl:DatatypeProperty ;
    dcterms:accessRights "PUBLIC" ;
    dcterms:identifier "IsSpare" ;
    rdfs:subPropertyOf :DomainAttribute ;
    skos:definition "Indicates whether the item is spare (TRUE) or not (FALSE)."@en ;
    skos:prefLabel "Is Spare"@en,
        "É um sobressalente"@pt-br ;
    :hasAttributeScope :InstanceLevelAttribute ;
    :hasTypedValue :booleanValue ;
    :hasValueCardinality :singleValue .

:LayerAnnular a owl:DatatypeProperty ;
    dcterms:accessRights "PUBLIC" ;
    dcterms:identifier "LayerAnnular" ;
    rdfs:subPropertyOf :DomainAttribute ;
    skos:definition "Indicates whether the layer is part of the annular structure of the tensile armours. If true, it confirms that the layer contributes to the annular arrangement, which is important for understanding its role in the structural integrity and load distribution."@en,
        "True se a camada faz parte do anular das armaduras de tração"@pt-br ;
    skos:prefLabel "Layer Annular"@en,
        "Camada Anular"@pt-br ;
    :hasAttributeScope :InstanceLevelAttribute ;
    :hasTypedValue :booleanValue ;
    :hasValueCardinality :singleValue .

:LayerAnnularType a owl:DatatypeProperty ;
    dcterms:accessRights "PUBLIC" ;
    dcterms:identifier "LayerAnnularType" ;
    rdfs:subPropertyOf :DomainAttribute ;
    skos:definition "Specifies the type of annular layer based on the condition it is designed for. This information is crucial for understanding the intended role of the layer in the overall structural configuration and how it is expected to perform under the projected operational conditions."@en,
        "Tipo de anular conforme o estado do anular: Não pertence ao anular; Anular nunca alagado; Anular sempre alagado; Anular possivelmente alagado"@pt-br ;
    skos:prefLabel "Layer Annular Type"@en,
        "Tipo de Anular"@pt-br ;
    :hasAttributeScope :InstanceLevelAttribute ;
    :hasTypedValue :stringValue ;
    :hasValueCardinality :singleValue .

:LayerContinuity a owl:DatatypeProperty ;
    dcterms:accessRights "PUBLIC" ;
    dcterms:identifier "LayerContinuity" ;
    rdfs:subPropertyOf :DomainAttribute ;
    skos:definition "Indicates whether the layer is continuous, such as when it is extruded. If true, it confirms that the layer has no interruptions or joints, which is important for ensuring uniformity and strength in the structure."@en,
        "True se a camada é contínua (extrudada)"@pt-br ;
    skos:prefLabel "Layer Continuity"@en,
        "Continuidade da Camada"@pt-br ;
    :hasAttributeScope :InstanceLevelAttribute ;
    :hasTypedValue :booleanValue ;
    :hasValueCardinality :singleValue .

:LayerGeometryCrossSection a owl:DatatypeProperty ;
    dcterms:accessRights "PUBLIC" ;
    dcterms:identifier "LayerGeometryCrossSection" ;
    rdfs:subClassOf :LayerGeometryAttribute ;
    skos:definition "Indicates the geometry of the layer's cross-section. This property provides detailed information about the shape and dimensions of the layer when viewed in cross-section, which is important for understanding how the layer contributes to the overall structure's performance and integrity."@en ;
    skos:prefLabel "Layer Geometry Cross Section"@en,
        "Seção Transversal da Geometria da Camada"@pt-br ;
    :hasAttributeScope :InstanceLevelAttribute ;
    :hasTypedValue :floatValue ;
    :hasValueCardinality :singleValue .

:LayerGeometryInertiaX a owl:DatatypeProperty ;
    dcterms:accessRights "PUBLIC" ;
    dcterms:identifier "LayerGeometryInertiaX" ;
    rdfs:subClassOf :LayerGeometryAttribute ;
    skos:definition "Indicates the moment of inertia of the layer's geometry around the X-axis. This property is crucial for understanding the layer's resistance to bending or deformation when subjected to forces along the X-axis, contributing to the structural stability and performance of the component."@en ;
    skos:prefLabel "Layer Geometry Inertia X"@en,
        "Inércia X da Geometria da Camada"@pt-br ;
    :hasAttributeScope :InstanceLevelAttribute ;
    :hasTypedValue :floatValue ;
    :hasValueCardinality :singleValue .

:LayerGeometryInertiaY a owl:DatatypeProperty ;
    dcterms:accessRights "PUBLIC" ;
    dcterms:identifier "LayerGeometryInertiaY" ;
    rdfs:subClassOf :LayerGeometryAttribute ;
    skos:definition "Indicates the moment of inertia of the layer's geometry around the Y-axis. This property is important for evaluating the layer's resistance to bending or deformation when subjected to forces along the Y-axis, helping to ensure the structural stability and performance of the component."@en ;
    skos:prefLabel "Layer Geometry Inertia Y"@en,
        "Inércia  Y da Geometria da Camada"@pt-br ;
    :hasAttributeScope :InstanceLevelAttribute ;
    :hasTypedValue :floatValue ;
    :hasValueCardinality :singleValue .

:LayerGeometryManufacturer a owl:DatatypeProperty ;
    dcterms:accessRights "PUBLIC" ;
    dcterms:identifier "LayerGeometryManufacturer" ;
    rdfs:subClassOf :LayerGeometryAttribute ;
    skos:definition "Indicates the manufacturer responsible for producing the layer's geometry. This property is important for tracking the origin and quality of the layer, providing key information about the source of the material or component used in the structure."@en ;
    skos:prefLabel "Layer Geometry Manufacturer"@en,
        "Fabricante da Geometria da Camada"@pt-br ;
    :hasAttributeScope :InstanceLevelAttribute ;
    :hasTypedValue :stringValue ;
    :hasValueCardinality :singleValue .

:LayerGeometryName a owl:DatatypeProperty ;
    dcterms:accessRights "PUBLIC" ;
    dcterms:identifier "LayerGeometryName" ;
    rdfs:subClassOf :LayerGeometryAttribute ;
    skos:definition "Indicates the name assigned to the layer's geometry. This property is used to identify and distinguish the specific geometry of the layer, helping with organization, tracking, and reference within the overall structure or design."@en ;
    skos:prefLabel "Layer Geometry Name"@en,
        "Nome da Geometria da Camada"@pt-br ;
    :hasAttributeScope :InstanceLevelAttribute ;
    :hasTypedValue :stringValue ;
    :hasValueCardinality :singleValue .

:LayerGeometryProfileThickness a owl:DatatypeProperty ;
    dcterms:accessRights "PUBLIC" ;
    dcterms:identifier "LayerGeometryProfileThickness" ;
    rdfs:subClassOf :LayerGeometryAttribute ;
    skos:definition "Indicates the thickness of the layer's geometric profile. This property is important for understanding the contribution of the layer to the overall structure, particularly in terms of strength, flexibility, and resistance to external forces."@en ;
    skos:prefLabel "Layer Geometry Profile Thickness"@en,
        "Espessura do Perfil da Geometria da Camada"@pt-br ;
    :hasAttributeScope :InstanceLevelAttribute ;
    :hasTypedValue :floatValue ;
    :hasValueCardinality :singleValue .

:LayerGeometryProfileWidth a owl:DatatypeProperty ;
    dcterms:accessRights "PUBLIC" ;
    dcterms:identifier "LayerGeometryProfileWidth" ;
    rdfs:subClassOf :LayerGeometryAttribute ;
    skos:definition "Indicates the width of the layer's geometric profile. This property is important for understanding the dimensions of the layer, contributing to the overall structural design, and influencing factors such as load distribution and mechanical performance."@en ;
    skos:prefLabel "Layer Geometry Profile Width"@en,
        "Largura do Perfil da Geometria da Camada"@pt-br ;
    :hasAttributeScope :InstanceLevelAttribute ;
    :hasTypedValue :floatValue ;
    :hasValueCardinality :singleValue .

:LayerGeometryThickness a owl:DatatypeProperty ;
    dcterms:accessRights "PUBLIC" ;
    dcterms:identifier "LayerGeometryThickness" ;
    rdfs:subClassOf :LayerGeometryAttribute ;
    skos:definition "Indicates the overall thickness of the layer's geometry. This property is critical for evaluating the structural contribution of the layer, including its strength, flexibility, and resistance to external forces."@en ;
    skos:prefLabel "Layer Geometry Thickness"@en,
        "Espessura da Geometria da Camada"@pt-br ;
    :hasAttributeScope :InstanceLevelAttribute ;
    :hasTypedValue :floatValue ;
    :hasValueCardinality :singleValue .

:LayerThickness a owl:DatatypeProperty ;
    dcterms:accessRights "PUBLIC" ;
    dcterms:identifier "LayerThickness" ;
    rdfs:subPropertyOf :DomainAttribute ;
    skos:definition "Indicates the thickness of the layer, providing a key dimension that affects the overall strength, flexibility, and performance of the structure. This value is critical for ensuring that the layer meets design requirements and operational conditions."@en ;
    skos:prefLabel "Layer Thickness"@en,
        "Espessura da camada"@pt-br ;
    :hasAttributeScope :InstanceLevelAttribute ;
    :hasTypedValue :floatValue ;
    :hasValueCardinality :singleValue .

:LayerWatertight a owl:DatatypeProperty ;
    dcterms:accessRights "PUBLIC" ;
    dcterms:identifier "LayerWatertight" ;
    rdfs:subPropertyOf :DomainAttribute ;
    skos:definition "Indicates whether the layer is designed to be watertight. This property is critical for assessing the layer's ability to prevent water ingress, ensuring protection and maintaining the integrity of the structure in environments where exposure to water or fluids is expected."@en ;
    skos:prefLabel "Layer Watertight"@en,
        "Camada Estanque"@pt-br ;
    :hasAttributeScope :InstanceLevelAttribute ;
    :hasTypedValue :booleanValue ;
    :hasValueCardinality :singleValue .

:LayerWatertightLowerLayerInternalFreeVolume a owl:DatatypeProperty ;
    dcterms:accessRights "PUBLIC" ;
    dcterms:identifier "LayerWatertightLowerLayerInternalFreeVolume" ;
    rdfs:subPropertyOf :DomainAttribute ;
    skos:definition "Indicates the free volume between this layer and the previous continuous or watertight lower layer. If this layer is not watertight, or if there is no previous watertight lower layer, the value should be indicated as zero. This property is important for assessing the space that may affect pressure distribution or fluid movement within the structure."@en,
        "Volume livre interno entre essa camada e a camada inferior estanque. Se essa camada não for estanque ou caso não tenha camada inferior estanque, indicar zero."@pt-br ;
    skos:prefLabel "Layer Watertight Lower Layer Internal Free Volume"@en,
        "Volume Livre Interno da Camada Inferior Estanque"@pt-br ;
    :hasAttributeScope :InstanceLevelAttribute ;
    :hasTypedValue :floatValue ;
    :hasValueCardinality :singleValue .

:LayingMinimumRadiusTable_AbsoluteExternalPressure a owl:DatatypeProperty ;
    dcterms:accessRights "PUBLIC" ;
    dcterms:identifier "LayingMinimumRadiusTable_AbsoluteExternalPressure" ;
    rdfs:subClassOf :LayingMinimumRadiusTableColumn ;
    skos:definition "Represents the total pressure exerted on a component or system from the external environment, including both atmospheric and hydrostatic pressures. This property is critical for assessing the ability of the system to withstand the full pressure load, ensuring that it maintains structural integrity under extreme conditions."@en ;
    skos:prefLabel "Absolute External Pressure"@en,
        "Pressão Externa absoluta"@pt-br ;
    :hasAttributeScope :TypeLevelAttribute ;
    :hasTypedValue :floatValue ;
    :hasValueCardinality :multiValue .

:LayingMinimumRadiusTable_AbsoluteInternalPressure a owl:DatatypeProperty ;
    dcterms:accessRights "PUBLIC" ;
    dcterms:identifier "LayingMinimumRadiusTable_AbsoluteInternalPressure" ;
    rdfs:subClassOf :LayingMinimumRadiusTableColumn ;
    skos:definition "Represents the total pressure exerted inside a component or system, accounting for both the atmospheric pressure and any additional internal pressure. This property is crucial for determining the system's ability to handle internal forces, ensuring safe operation under the expected pressure conditions."@en ;
    skos:prefLabel "Absolute Internal Pressure"@en,
        "Pressão interna absoluta"@pt-br ;
    :hasAttributeScope :TypeLevelAttribute ;
    :hasTypedValue :floatValue ;
    :hasValueCardinality :multiValue .

:LayingMinimumRadiusTable_Compression a owl:DatatypeProperty ;
    dcterms:accessRights "PUBLIC" ;
    dcterms:identifier "LayingMinimumRadiusTable_Compression" ;
    rdfs:subClassOf :LayingMinimumRadiusTableColumn ;
    skos:definition "Represents the force or stress applied to a material or component that causes it to decrease in size along a particular axis. This property is important for evaluating the material's ability to withstand compressive loads without failure."@en,
        "Nota: Devem ser informados valores negativos. Por exemplo, para uma compressão de 10kN, deve ser informado -10."@pt-br ;
    skos:prefLabel "Compression"@en,
        "Compressão"@pt-br ;
    :hasAttributeScope :TypeLevelAttribute ;
    :hasTypedValue :floatValue ;
    :hasValueCardinality :multiValue .

:LayingMinimumRadiusTable_MinimumAllowableBendingRadius a owl:DatatypeProperty ;
    dcterms:accessRights "PUBLIC" ;
    dcterms:identifier "LayingMinimumRadiusTable_MinimumAllowableBendingRadius" ;
    rdfs:subClassOf :LayingMinimumRadiusTableColumn ;
    skos:definition "Represents the smallest radius to which a component, such as a pipe or cable, can be bent without causing damage or compromising its structural integrity. This property is essential for determining handling and installation limits to avoid deformation or failure."@en ;
    skos:prefLabel "Minimum Allowable Bending Radius"@en,
        "Raio Mínimo de Curvatura Permitido"@pt-br ;
    :hasAttributeScope :TypeLevelAttribute ;
    :hasTypedValue :stringValue ;
    :hasValueCardinality :multiValue .

:LayingMinimumRadiusTable_SectionSupportedByRigidSupport a owl:DatatypeProperty ;
    dcterms:accessRights "PUBLIC" ;
    dcterms:identifier "LayingMinimumRadiusTable_SectionSupportedByRigidSupport" ;
    rdfs:subClassOf :LayingMinimumRadiusTableColumn ;
    skos:definition "Indicates whether the section is supported by a rigid support (TRUE) or not (FALSE)."@en ;
    skos:prefLabel "Section Supported By Rigid Support"@en,
        "Seção Suportada por um Suporte Rígido"@pt-br ;
    :hasAttributeScope :TypeLevelAttribute ;
    :hasTypedValue :booleanValue ;
    :hasValueCardinality :multiValue .

:LayingMinimumRadiusTable_TensileArmourAnnulusCondition a owl:DatatypeProperty ;
    dcterms:accessRights "PUBLIC" ;
    dcterms:identifier "LayingMinimumRadiusTable_TensileArmourAnnulusCondition" ;
    rdfs:subClassOf :LayingMinimumRadiusTableColumn ;
    skos:definition "Indicates the condition of the annulus in the tensile armour layer, which refers to the space between the tensile armour and other layers."@en,
        "Condição do anular das armaduras de tração, Alagado ou Seco"@pt-br ;
    skos:prefLabel "Tensile Armour Annulus Condition"@en,
        "Condição do Anular das Armaduras de Tração"@pt-br ;
    :hasAttributeScope :TypeLevelAttribute ;
    :hasTypedValue :stringValue ;
    :hasValueCardinality :multiValue .

:LimpTorsionalStiffnessAtSeaLevel a owl:DatatypeProperty ;
    dcterms:accessRights "PUBLIC" ;
    dcterms:identifier "LimpTorsionalStiffnessAtSeaLevel" ;
    rdfs:subPropertyOf :DomainAttribute ;
    skos:definition "Indicates the torsional stiffness of the structure when in a limp or flexible state at sea level conditions. This value is important for assessing how the structure resists twisting forces while maintaining flexibility during operations at sea level."@en,
        "Rigidez a torção (GJ) (menor valor) a 20°C e pressão atmosferica (dentro e fora)"@pt-br ;
    skos:prefLabel "Limp Torsional Stiffness At Sea Level"@en,
        "Rigidez à Torção em Estado Flexível ao Nível do Mar"@pt-br ;
    :hasAttributeScope :TypeLevelAttribute ;
    :hasTypedValue :floatValue ;
    :hasValueCardinality :singleValue .

:LinearLocation a owl:Class ;
    dcterms:identifier "LinearLocation" ;
    rdfs:subClassOf :Location ;
    skos:definition "Base for locations that extend along a geographically significant route."@en ;
    skos:prefLabel "Linear Location"@en,
        "Localização Linear"@pt-br .

:LongTermFloatDensity a owl:DatatypeProperty ;
    dcterms:accessRights "PUBLIC" ;
    dcterms:identifier "LongTermFloatDensity" ;
    rdfs:subPropertyOf :DomainAttribute ;
    skos:definition "The density of the float material over time, considering factors like water absorption and material degradation, which increase the density and reduce the buoyancy."@en,
        "A densidade do flutuador ao longo do tempo, considerando o acúmulo de água no material ou mudanças na estrutura interna devido à degradação. Isso aumenta a densidade e, portanto, reduz a flutuabilidade"@pt-br ;
    skos:prefLabel "Long Term Float Density"@en,
        "Densidade do Flutuador a Longo Prazo"@pt-br ;
    :hasAttributeScope :TypeLevelAttribute ;
    :hasTypedValue :floatValue ;
    :hasValueCardinality :singleValue .

:LongTermFloatVolume a owl:DatatypeProperty ;
    dcterms:accessRights "PUBLIC" ;
    dcterms:identifier "LongTermFloatVolume" ;
    rdfs:subPropertyOf :DomainAttribute ;
    skos:definition "The expected submerged volume of the float over time, taking into account factors like water absorption and structural deformations that may occur throughout its lifecycle."@en,
        "O volume esperado ao longo do tempo, após fatores como absorção de água e possíveis deformações. Este volume representa as condições do flutuador em sua fase de vida útil, quando a flutuabilidade tende a ser menor."@pt-br ;
    skos:prefLabel "Long Term Float Volume"@en,
        "Volume do Flutuador a Longo Prazo"@pt-br ;
    :hasAttributeScope :TypeLevelAttribute ;
    :hasTypedValue :floatValue ;
    :hasValueCardinality :singleValue .

:Manifold a owl:Class ;
    dcterms:identifier "Manifold" ;
    rdfs:subClassOf :FlowControlEquipment .

:ManufacturerDefinedMaterialName a owl:DatatypeProperty ;
    dcterms:accessRights "PUBLIC" ;
    dcterms:identifier "ManufacturerDefinedMaterialName" ;
    rdfs:subClassOf :MaterialManufacturerAttribute ;
    skos:definition "Name of the material as designated by the manufacturer of the final item. This property identifies the specific material name used by the manufacturer, providing clarity on the material specifications for the finished accessory."@en ;
    skos:prefLabel "Manufacturer Defined Material Name"@en,
        "Nome do material conforme designado pelo fabricante do item final"@pt-br ;
    :hasAttributeScope :TypeLevelAttribute ;
    :hasTypedValue :stringValue ;
    :hasValueCardinality :multiValue .

:ManufacturingDate a owl:DatatypeProperty ;
    dcterms:accessRights "PUBLIC" ;
    dcterms:identifier "ManufacturingDate" ;
    rdfs:subPropertyOf :DomainAttribute ;
    skos:definition "Manufacturing date refers to the specific date when an object or product was produced or fabricated. This information is essential for tracking production batches, ensuring quality control, and determining the product’s shelf life or warranty period."@en ;
    skos:prefLabel "Manufacturing Date"@en,
        "Data de Fabricação"@pt-br ;
    :hasAttributeScope :InstanceLevelAttribute ;
    :hasTypedValue :stringValue ;
    :hasValueCardinality :singleValue .

:ManufacturingNonConformities a owl:DatatypeProperty ;
    dcterms:accessRights "PUBLIC" ;
    dcterms:identifier "ManufacturingNonConformities" ;
    rdfs:subPropertyOf :DomainAttribute ;
    skos:definition "Indicates whether the item has manufacturing non-conformities (TRUE) or not (FALSE)."@en ;
    skos:prefLabel "Manufacturing Non Conformities"@en,
        "Não Conformidades de Fabricação"@pt-br ;
    :hasAttributeScope :InstanceLevelAttribute ;
    :hasTypedValue :booleanValue ;
    :hasValueCardinality :singleValue .

:Mass a owl:DatatypeProperty ;
    dcterms:accessRights "PUBLIC" ;
    dcterms:identifier "Mass" ;
    rdfs:subPropertyOf :DomainAttribute ;
    skos:definition "Amount of matter that makes up an object."@en ;
    skos:prefLabel "Mass"@en,
        "Massa"@pt-br ;
    :hasAttributeScope :TypeLevelAttribute ;
    :hasTypedValue :floatValue ;
    :hasValueCardinality :singleValue .

:MaterialComposition a owl:DatatypeProperty ;
    dcterms:accessRights "PUBLIC" ;
    dcterms:identifier "MaterialComposition" ;
    rdfs:subPropertyOf :DomainAttribute ;
    skos:definition "Indicates the composition of the fabrication material used. This property provides details about the specific material, helping to assess its mechanical, thermal, and chemical properties. It is crucial for evaluating the material's suitability for various operational conditions and services."@en,
        "Tipo do material."@pt-br ;
    skos:prefLabel "Material Composition"@en,
        "Composição do Material"@pt-br ;
    :hasAttributeScope :TypeLevelAttribute ;
    :hasTypedValue :stringValue ;
    :hasValueCardinality :singleValue .

:MaterialRequest a owl:DatatypeProperty ;
    dcterms:accessRights "PUBLIC" ;
    dcterms:identifier "MaterialRequest" ;
    rdfs:subPropertyOf :DomainAttribute ;
    skos:definition "Code used to identify the document that specifies the materials required for the project, serving as the basis for generating the purchase order. It ensures accurate tracking and procurement of necessary items for project execution."@en ;
    skos:prefLabel "Material Request"@en,
        "Código da Requisição de Material (RM)"@pt-br ;
    :hasAttributeScope :InstanceLevelAttribute ;
    :hasTypedValue :stringValue ;
    :hasValueCardinality :singleValue .

:MaterialRequestRev a owl:DatatypeProperty ;
    dcterms:accessRights "PUBLIC" ;
    dcterms:identifier "MaterialRequestRev" ;
    rdfs:subPropertyOf :DomainAttribute ;
    skos:definition "Indicates the revision number of the Material Request document, ensuring that the most up-to-date version is referenced during procurement and project execution."@en ;
    skos:prefLabel "Material Request Revision"@en,
        "Revisão da Requisição de Material (RM)"@pt-br ;
    :hasAttributeScope :InstanceLevelAttribute ;
    :hasTypedValue :stringValue ;
    :hasValueCardinality :singleValue .

:MaterialSupplierName a owl:DatatypeProperty ;
    dcterms:accessRights "PUBLIC" ;
    dcterms:identifier "MaterialSupplierName" ;
    rdfs:subClassOf :MaterialManufacturerAttribute ;
    skos:definition "Name of the company responsible for supplying the material. This property identifies the supplier of the material used in the accessory, ensuring traceability and accountability."@en ;
    skos:prefLabel "Material Supplier Name"@en,
        "Nome da empresa responsável por fornecer o material"@pt-br ;
    :hasAttributeScope :TypeLevelAttribute ;
    :hasTypedValue :stringValue ;
    :hasValueCardinality :singleValue .

:MaxDesignAbsIntPresTable_PositionReference a owl:DatatypeProperty ;
    dcterms:accessRights "PUBLIC" ;
    dcterms:identifier "MaxDesignAbsIntPresTable_PositionReference" ;
    rdfs:subClassOf :MaxDesignAbsIntPresTable ;
    skos:definition "Identifies the specific point along the pipeline, such as the topside connection, TDP (Touchdown Point), or subsea connection point. This serves as the reference for vertical position and pressure values."@en,
        "Ponto. Valores válidos:Top (Para a conexão topside - E.g. Conector superior)TDPSubSeaConnection (Ex. ANM)"@pt-br ;
    skos:prefLabel "Position Reference"@en,
        "Referência de Posição"@pt-br ;
    :hasAttributeScope :InstanceLevelAttribute ;
    :hasTypedValue :stringValue ;
    :hasValueCardinality :multiValue .

:MaxDesignAbsIntPresTable_Pressure a owl:DatatypeProperty ;
    dcterms:accessRights "PUBLIC" ;
    dcterms:identifier "MaxDesignAbsIntPresTable_Pressure" ;
    rdfs:subClassOf :MaxDesignAbsIntPresTable ;
    skos:definition "Indicates the force exerted per unit area on the surface of a material or component. This property is critical for evaluating how the component responds to external or internal forces, ensuring it can withstand operational pressure conditions."@en ;
    skos:prefLabel "Maximum Design Absolute Internal Pressure"@en,
        "Máxima Pressão Interna Absoluta de Projeto"@pt-br ;
    :hasAttributeScope :InstanceLevelAttribute ;
    :hasTypedValue :floatValue ;
    :hasValueCardinality :multiValue .

:MaxDesignAbsIntPresTable_VPosWRTWaterline a owl:DatatypeProperty ;
    dcterms:accessRights "PUBLIC" ;
    dcterms:identifier "MaxDesignAbsIntPresTable_VPosWRTWaterline" ;
    rdfs:subClassOf :MaxDesignAbsIntPresTable ;
    skos:definition "Vertical position with respect to the waterline, where positive values indicate points above the water and negative values indicate points below. The platform's maximum draft is considered when applicable."@en,
        "Valores negativos para pontos submersos, e valores positivos para pontos acima da água. Considerando calado máximo da plataforma, quando aplicável."@pt-br ;
    skos:prefLabel "Vertical Position With Respect To Waterline"@en,
        "Posição Vertical em Relação à Linha D'Água"@pt-br ;
    :hasAttributeScope :InstanceLevelAttribute ;
    :hasTypedValue :intValue ;
    :hasValueCardinality :multiValue .

:MaxDesignPressure a owl:DatatypeProperty ;
    dcterms:accessRights "PUBLIC" ;
    dcterms:identifier "MaxDesignPressure" ;
    rdfs:subPropertyOf :DomainAttribute ;
    skos:definition "The highest internal or external pressure that the component or system is designed to withstand under operational conditions, ensuring safety and reliability."@en ;
    skos:prefLabel "Maximum Design Pressure"@en,
        "Pressão Máxima de Projeto"@pt-br ;
    :hasAttributeScope :TypeLevelAttribute ;
    :hasTypedValue :floatValue ;
    :hasValueCardinality :singleValue .

:MaxDynamicLoad a owl:DatatypeProperty ;
    dcterms:accessRights "PUBLIC" ;
    dcterms:identifier "MaxDynamicLoad" ;
    rdfs:subPropertyOf :DomainAttribute ;
    skos:definition "Maximum Dynamic Load (MDL) that the component can endure during operation. This value indicates the highest load the component can support while experiencing varying forces or impacts. Understanding this limit is essential for ensuring the component’s safety, reliability, and structural integrity in dynamic environments."@en ;
    skos:prefLabel "Maximum Dynamic Load (MDL)"@en,
        "Carga Dinâmica Máxima (MDL)"@pt-br ;
    :hasAttributeScope :TypeLevelAttribute ;
    :hasTypedValue :floatValue ;
    :hasValueCardinality :singleValue .

:MaxLengthTolerance a owl:DatatypeProperty ;
    dcterms:accessRights "PUBLIC" ;
    dcterms:identifier "MaxLengthTolerance" ;
    rdfs:subPropertyOf :DomainAttribute ;
    skos:definition "Max length tolerance refers to the maximum allowable deviation from the specified or nominal length of an object. It defines the upper limit of acceptable variance during manufacturing or inspection, ensuring that the length stays within the defined range for quality control and compliance with design specifications."@en ;
    skos:prefLabel "Maximum Length Tolerance"@en,
        "Tolerância Máxima de Comprimento"@pt-br ;
    :hasAttributeScope :InstanceLevelAttribute ;
    :hasTypedValue :floatValue ;
    :hasValueCardinality :singleValue .

:MaxPermissibleDeformationDynamic a owl:DatatypeProperty ;
    dcterms:accessRights "PUBLIC" ;
    dcterms:identifier "MaxPermissibleDeformationDynamic" ;
    rdfs:subPropertyOf :DomainAttribute ;
    skos:definition "Maximum deformation that the material can undergo under dynamic loading conditions is specified. This property is crucial for assessing how the material will behave when subjected to varying forces or impacts, ensuring it maintains functionality and structural integrity without excessive deformation or failure."@en,
        "Máxima Deformação Admissível (Aplicações Dinâmicas) (Específica para Materiais Poliméricos)"@pt-br ;
    skos:prefLabel "Maximum Permissible Deformation Dynamic"@en,
        "Máxima Deformação Admissível"@pt-br ;
    :hasAttributeScope :TypeLevelAttribute ;
    :hasTypedValue :floatValue ;
    :hasValueCardinality :singleValue .

:MaxPermissibleDeformationStatic a owl:DatatypeProperty ;
    dcterms:accessRights "PUBLIC" ;
    dcterms:identifier "MaxPermissibleDeformationStatic" ;
    rdfs:subPropertyOf :DomainAttribute ;
    skos:definition "Indicates the maximum deformation the material can tolerate under static loading conditions. This property defines the extent to which the material can be deformed without failure or significant structural compromise when subjected to constant, non-varying forces or loads."@en,
        "Máxima Deformação Admissível (Aplicações Estáticas) (Específica para Materiais Poliméricos)"@pt-br ;
    skos:prefLabel "Maximum Permissible Deformation Static"@en,
        "Máxima Deformação Admissível em Aplicações Estáticas"@pt-br ;
    :hasAttributeScope :TypeLevelAttribute ;
    :hasTypedValue :floatValue ;
    :hasValueCardinality :singleValue .

:MaximumAllowableTensileForStraightLine a owl:DatatypeProperty ;
    dcterms:accessRights "PUBLIC" ;
    dcterms:identifier "MaximumAllowableTensileForStraightLine" ;
    rdfs:subPropertyOf :DomainAttribute ;
    skos:definition "MaximumAllowableTensileForStraightLine refers to the highest tensile force that can be applied to the flexible pipe in a straight-line configuration without risking damage or compromising the structural integrity of the pipe. This property is critical during installation and operation, ensuring that the pipe can withstand axial loads without overstressing or damaging its internal layers, such as the tensile armour, while maintaining safe handling limits."@en ;
    skos:prefLabel "Maximum Allowable Tensile For Straight Line"@en,
        "Tração Máxima Permitida para Linha Reta"@pt-br ;
    :hasAttributeScope :TypeLevelAttribute ;
    :hasTypedValue :floatValue ;
    :hasValueCardinality :singleValue .

:MaximumAllowableTensionTable_MaximumAllowableTensile a owl:DatatypeProperty ;
    dcterms:accessRights "PUBLIC" ;
    dcterms:identifier "MaximumAllowableTensionTable_MaximumAllowableTensile" ;
    rdfs:subClassOf :CrushingMaximumAllowableTensionTableColumn ;
    skos:definition "Indicates the highest tensile force a component can safely withstand without compromising its integrity."@en ;
    skos:prefLabel "Maximum Allowable Tensile"@en,
        "Tração Máxima Permitida"@pt-br ;
    :hasAttributeScope :TypeLevelAttribute ;
    :hasTypedValue :floatValue ;
    :hasValueCardinality :multiValue .

:MaximumAllowableTensionTable_PulleyRadius a owl:DatatypeProperty ;
    dcterms:accessRights "PUBLIC" ;
    dcterms:identifier "MaximumAllowableTensionTable_PulleyRadius" ;
    rdfs:subClassOf :CrushingMaximumAllowableTensionTableColumn ;
    skos:definition "The distance measured from the center of the pulley to the bottom of the \"V\" shape."@en ;
    skos:prefLabel "Pulley Radius"@en,
        "Raio da Polia"@pt-br ;
    :hasAttributeScope :TypeLevelAttribute ;
    :hasTypedValue :floatValue ;
    :hasValueCardinality :multiValue .

:MaximumAllowableTensionTable_PulleyVAngle a owl:DatatypeProperty ;
    dcterms:accessRights "PUBLIC" ;
    dcterms:identifier "MaximumAllowableTensionTable_PulleyVAngle" ;
    rdfs:subClassOf :CrushingMaximumAllowableTensionTableColumn ;
    skos:definition "The angle formed by the opening of the \"V\" Groove in the pulley, measured in degrees."@en ;
    skos:prefLabel "Pulley V Groove Angle"@en,
        "Ângulo do Sulco em V da Polia"@pt-br ;
    :hasAttributeScope :TypeLevelAttribute ;
    :hasTypedValue :floatValue ;
    :hasValueCardinality :multiValue .

:MaximumAllowableTighteningTable_AxialLoad a owl:DatatypeProperty ;
    dcterms:accessRights "PUBLIC" ;
    dcterms:identifier "MaximumAllowableTighteningTable_AxialLoad" ;
    rdfs:subClassOf :CrushingMaximumAllowableTighteningTableColumn ;
    skos:definition "Represents the force applied along the longitudinal axis of a component or system. This property is important for evaluating the ability of the structure to resist stretching or compression, ensuring it maintains integrity under operational loads."@en ;
    skos:prefLabel "Axial Load"@en,
        "Tabela de Aperto Máximo Permitido - Carga Axial"@pt-br ;
    :hasAttributeScope :TypeLevelAttribute ;
    :hasTypedValue :floatValue ;
    :hasValueCardinality :multiValue .

:MaximumAllowableTighteningTable_TighteningPerTrack a owl:DatatypeProperty ;
    dcterms:accessRights "PUBLIC" ;
    dcterms:identifier "MaximumAllowableTighteningTable_TighteningPerTrack" ;
    rdfs:subClassOf :CrushingMaximumAllowableTighteningTableColumn ;
    skos:definition "Indicates the amount of tightening applied per track during an operation. This property is important for ensuring consistent force distribution across multiple tracks, helping to maintain proper alignment and secure attachment during the tightening process."@en ;
    skos:prefLabel "Tightening Per Track"@en,
        "Tabela de Aperto Máximo Permitido - Aperto por Lagarta"@pt-br ;
    :hasAttributeScope :TypeLevelAttribute ;
    :hasTypedValue :floatValue ;
    :hasValueCardinality :multiValue .

:MaximumAmbientTemperature a owl:DatatypeProperty ;
    dcterms:accessRights "PUBLIC" ;
    dcterms:identifier "MaximumAmbientTemperature" ;
    rdfs:subClassOf :CrushingFrictionCoefficientTighteningTableAttribute,
        :CrushingMaximumAllowableTensionTableAttribute,
        :CrushingMaximumAllowableTighteningTableAttribute ;
    skos:definition "Represents the highest ambient temperature at which a component or material can operate effectively without risk of degradation or failure. This property is crucial for ensuring the material's performance and longevity under elevated temperature conditions."@en ;
    skos:prefLabel "Maximum Ambient Temperature"@en,
        "Temperatura ambiente máxima"@pt-br ;
    :hasAttributeScope :TypeLevelAttribute ;
    :hasTypedValue :floatValue ;
    :hasValueCardinality :singleValue .

:MaximumTemperature a owl:DatatypeProperty ;
    dcterms:accessRights "PUBLIC" ;
    dcterms:identifier "MaximumTemperature" ;
    rdfs:subPropertyOf :DomainAttribute ;
    skos:definition "Represents the highest temperature at which the structure or component can safely operate without compromising its integrity or performance. This value is critical for ensuring that materials and components maintain their mechanical properties and do not experience degradation, deformation, or failure under extreme thermal conditions."@en ;
    skos:prefLabel "Maximum Temperature"@en,
        "Temperatura Máxima"@pt-br ;
    :hasAttributeScope :InstanceLevelAttribute ;
    :hasTypedValue :floatValue ;
    :hasValueCardinality :singleValue .

:MaximumThermalExchangeCoefficient a owl:DatatypeProperty ;
    dcterms:accessRights "PUBLIC" ;
    dcterms:identifier "MaximumThermalExchangeCoefficient" ;
    rdfs:subPropertyOf :DomainAttribute ;
    skos:definition "Indicates the maximum allowable value for the Thermal Exchange Coefficient (TEC), specifying the upper limit for heat transfer in the design. This value ensures that the flexible pipeline meets thermal performance requirements without exceeding the permissible heat transfer rate, which could affect its integrity and operational efficiency."@en ;
    skos:prefLabel "Maximum Thermal Exchange Coefficient (TEC)"@en,
        "Coeficiente Máximo de Troca Térmica (TEC)"@pt-br ;
    :hasAttributeScope :InstanceLevelAttribute ;
    :hasTypedValue :floatValue ;
    :hasValueCardinality :singleValue .

:MetallicLayerMaterialType a owl:DatatypeProperty ;
    dcterms:accessRights "PUBLIC" ;
    dcterms:identifier "MetallicLayerMaterialType" ;
    rdfs:subPropertyOf :DomainAttribute ;
    skos:definition "Type of material from which an object is made, allowing for precise documentation and categorisation."@en ;
    skos:prefLabel "Metallic Layer Material Type"@en,
        "Tipo de Material da Camada Metálica"@pt-br ;
    :hasAttributeScope :TypeLevelAttribute ;
    :hasTypedValue :stringValue ;
    :hasValueCardinality :singleValue .

:MetallicLayerPitch a owl:DatatypeProperty ;
    dcterms:accessRights "PUBLIC" ;
    dcterms:identifier "MetallicLayerPitch" ;
    rdfs:subPropertyOf :DomainAttribute ;
    skos:definition "Indicates the distance between adjacent metallic elements in the layer, typically arranged helicoidally. This value is critical for determining the mechanical properties of the metallic layer, such as its flexibility, strength, and performance under load."@en ;
    skos:prefLabel "Metallic Layer Pitch"@en,
        "Passo da Camada Metálica"@pt-br ;
    :hasAttributeScope :InstanceLevelAttribute ;
    :hasTypedValue :floatValue ;
    :hasValueCardinality :singleValue .

:MetallicStrandLength a owl:DatatypeProperty ;
    dcterms:accessRights "PUBLIC" ;
    dcterms:identifier "MetallicStrandLength" ;
    rdfs:subPropertyOf :DomainAttribute ;
    skos:definition "The total length of the metallic strand used in the anode to endfittings connection"@en ;
    skos:prefLabel "Metallic Strand Length"@en,
        "Comprimento da Cordoalha Metálica"@pt-br ;
    :hasAttributeScope :TypeLevelAttribute ;
    :hasTypedValue :floatValue ;
    :hasValueCardinality :singleValue .

:MetallicStrandSpareQuantity a owl:DatatypeProperty ;
    dcterms:accessRights "PUBLIC" ;
    dcterms:identifier "MetallicStrandSpareQuantity" ;
    rdfs:subPropertyOf :DomainAttribute ;
    skos:definition "The additional quantity of metallic strands provided as spare material for contingency or repair purposes."@en ;
    skos:prefLabel "Metallic Strand Spare Quantity"@en,
        "Quantidade de Cordoalhas Metálicas Sobressalentes"@pt-br ;
    :hasAttributeScope :TypeLevelAttribute ;
    :hasTypedValue :intValue ;
    :hasValueCardinality :singleValue .

:MinimumBendingRadiusForStorage a owl:DatatypeProperty ;
    dcterms:accessRights "PUBLIC" ;
    dcterms:identifier "MinimumBendingRadiusForStorage" ;
    rdfs:subPropertyOf :DomainAttribute ;
    skos:definition "Represents the smallest radius to which a component can be bent during storage without causing damage or affecting its performance. This property is important for ensuring that the component maintains its integrity while in storage, preventing deformation or weakening."@en ;
    skos:prefLabel "Minimum Bending Radius For Storage"@en,
        "Raio Mínimo de Curvatura para Armazenamento"@pt-br ;
    :hasAttributeScope :TypeLevelAttribute ;
    :hasTypedValue :floatValue ;
    :hasValueCardinality :singleValue .

:MinimumTemperature a owl:DatatypeProperty ;
    dcterms:accessRights "PUBLIC" ;
    dcterms:identifier "MinimumTemperature" ;
    rdfs:subPropertyOf :DomainAttribute ;
    skos:definition "Represents the lowest temperature at which the structure or component can safely operate without experiencing performance degradation or failure. This value is important for ensuring that the materials maintain their properties and structural integrity when exposed to extremely low temperatures"@en ;
    skos:prefLabel "Minimum Temperature"@en,
        "Temperatura Mínima"@pt-br ;
    :hasAttributeScope :TypeLevelAttribute ;
    :hasTypedValue :floatValue ;
    :hasValueCardinality :singleValue .

:MinimumThermalExchangeCoefficient a owl:DatatypeProperty ;
    dcterms:accessRights "PUBLIC" ;
    dcterms:identifier "MinimumThermalExchangeCoefficient" ;
    rdfs:subPropertyOf :DomainAttribute ;
    skos:definition "Indicates the minimum allowable value for the Thermal Exchange Coefficient (TEC), specifying the lower limit for heat transfer in the design. This value ensures that the flexible pipeline maintains sufficient heat transfer capability to meet operational performance requirements."@en ;
    skos:prefLabel "Minimum Thermal Exchange Coefficient (TEC)"@en,
        "Coeficiente Mínimo de Troca Térmica (TEC)"@pt-br ;
    :hasAttributeScope :InstanceLevelAttribute ;
    :hasTypedValue :floatValue ;
    :hasValueCardinality :singleValue .

:ModelLocationPoint a owl:Class ;
    dcterms:identifier "ModelLocationPoint" ;
    rdfs:subClassOf :DomainElement ;
    skos:definition "A specific reference point or coordinate used to define the precise location of equipment, infrastructure, or components within a 3D model."@en ;
    skos:prefLabel "Model Location Point"@en,
        "Ponto de Localização no Modelo"@pt-br .

:ModulusOfElasticity a owl:DatatypeProperty ;
    dcterms:accessRights "PUBLIC" ;
    dcterms:identifier "ModulusOfElasticity" ;
    rdfs:subPropertyOf :DomainAttribute ;
    skos:definition "The modulus of elasticity represents the material's ability to resist deformation under stress. It quantifies the ratio of stress to strain within the elastic range of the material. This property is crucial for understanding how the material will behave under various loads and conditions."@en ;
    skos:prefLabel "Modulus Of Elasticity"@en,
        "Módulo de elasticidade"@pt-br ;
    :hasAttributeScope :InstanceLevelAttribute ;
    :hasTypedValue :floatValue ;
    :hasValueCardinality :singleValue .

:NominalFloatDensity a owl:DatatypeProperty ;
    dcterms:accessRights "PUBLIC" ;
    dcterms:identifier "NominalFloatDensity" ;
    rdfs:subPropertyOf :DomainAttribute ;
    skos:definition "The ideal density of the float material before any water absorption or degradation occurs. This is used to calculate the float's maximum buoyancy at the beginning of its use."@en,
        "A densidade ideal do flutuador antes de qualquer absorção de água ou degradação. Usada para calcular a flutuabilidade inicial máxima, idealmente no ponto de fabricação."@pt-br ;
    skos:prefLabel "Nominal Float Density"@en,
        "Densidade Nominal do Flutuador"@pt-br ;
    :hasAttributeScope :TypeLevelAttribute ;
    :hasTypedValue :floatValue ;
    :hasValueCardinality :singleValue .

:NominalFloatVolume a owl:DatatypeProperty ;
    dcterms:accessRights "PUBLIC" ;
    dcterms:identifier "NominalFloatVolume" ;
    rdfs:subPropertyOf :DomainAttribute ;
    skos:definition "The ideal or factory-specified volume of the float before any external effects like water absorption or deformation occur. This value is used to calculate the maximum buoyancy under perfect conditions."@en,
        "O volume ideal, ou \"de fábrica\", sem considerar a absorção de água ou deformações. É usado para calcular a flutuabilidade máxima possível, antes de qualquer degradação."@pt-br ;
    skos:prefLabel "Nominal Float Volume"@en,
        "Volume Nominal do Flutuador"@pt-br ;
    :hasAttributeScope :TypeLevelAttribute ;
    :hasTypedValue :floatValue ;
    :hasValueCardinality :singleValue .

:NumberOfChokeValves a owl:DatatypeProperty ;
    dcterms:accessRights "PUBLIC" ;
    dcterms:identifier "NumberOfChokeValves" ;
    rdfs:subPropertyOf :DomainAttribute ;
    skos:definition "Number of process choke valves"@en,
        "Número de válvulas choke"@pt-br ;
    skos:prefLabel "Number Of Choke Valves"@en,
        "Número de válvulas de estrangulamento"@pt-br ;
    :hasAttributeScope :TypeLevelAttribute ;
    :hasTypedValue :intValue ;
    :hasValueCardinality :singleValue .

:NumberOfRemoteProcessIsolationValves a owl:DatatypeProperty ;
    dcterms:accessRights "PUBLIC" ;
    dcterms:identifier "NumberOfRemoteProcessIsolationValves" ;
    rdfs:subPropertyOf :DomainAttribute ;
    skos:definition "Number of remotely-actuated process isolation valves"@en,
        "Número de válvulas de isolamento de processo com atuação remota"@pt-br ;
    skos:prefLabel "Number Of Remote Process Isolation Valves"@en,
        "Número de válvulas de isolamento de processo remoto"@pt-br ;
    :hasAttributeScope :TypeLevelAttribute ;
    :hasTypedValue :intValue ;
    :hasValueCardinality :singleValue .

:OffLeakPLevMaxPress a owl:DatatypeProperty ;
    dcterms:accessRights "PUBLIC" ;
    dcterms:identifier "OffLeakPLevMaxPress" ;
    rdfs:subClassOf :HydrostaticPressureTestsAttribute ;
    skos:definition "The maximum pressure applied during the Offshore Leak Test (at platform level), ensuring no leaks occur under extreme pressure."@en,
        "Condições de teste dos tramos para Pressão - Máxima - Teste de vazamento hidrostático offshore (no nível da plataforma)"@pt-br ;
    skos:prefLabel "Offshore Leak Test At Platform Level Maximum Pressure"@en,
        "Teste de Vazamento Offshore na Pressão Máxima no Nível da Plataforma"@pt-br ;
    :hasAttributeScope :InstanceLevelAttribute ;
    :hasTypedValue :floatValue ;
    :hasValueCardinality :singleValue .

:OffLeakPLevMaxPressValRef a owl:DatatypeProperty ;
    dcterms:accessRights "PUBLIC" ;
    dcterms:identifier "OffLeakPLevMaxPressValRef" ;
    rdfs:subClassOf :HydrostaticPressureTestsAttribute ;
    skos:definition "Specifies the reference pressure used to determine the Offshore Leak Test maximum pressure value."@en,
        "Comentários Condições de teste dos tramos para - Máximo - Teste de vazamento hidrostático offshore (no nível da plataforma)"@pt-br ;
    skos:prefLabel "Offshore Leak Test At Platform Level Maximum Pressure Value Reference"@en,
        "Referência de Valor de Pressão Máxima para Teste de Vazamento Offshore no Nível da Plataforma"@pt-br ;
    :hasAttributeScope :InstanceLevelAttribute ;
    :hasTypedValue :stringValue ;
    :hasValueCardinality :singleValue .

:OffLeakPLevMaxPressValRefMult a owl:DatatypeProperty ;
    dcterms:accessRights "PUBLIC" ;
    dcterms:identifier "OffLeakPLevMaxPressValRefMult" ;
    rdfs:subClassOf :HydrostaticPressureTestsAttribute ;
    skos:definition "The multiplier applied to the reference pressure to determine the Offshore Leak Test maximum pressure value."@en ;
    skos:prefLabel "Offshore Leak Test At Platform Level Maximum Pressure Value Reference Multiplier"@en,
        "Multiplicador de Referência de Valor de Pressão Máxima para Teste de Vazamento Offshore no Nível da Plataforma"@pt-br ;
    :hasAttributeScope :InstanceLevelAttribute ;
    :hasTypedValue :floatValue ;
    :hasValueCardinality :singleValue .

:OffLeakPLevNomPress a owl:DatatypeProperty ;
    dcterms:accessRights "PUBLIC" ;
    dcterms:identifier "OffLeakPLevNomPress" ;
    rdfs:subClassOf :HydrostaticPressureTestsAttribute ;
    skos:definition "The nominal pressure applied during the Offshore Leak Test (at platform level), simulating typical operating conditions to assess for leaks."@en,
        "Condições de teste dos tramos para Pressão - Nominal - Teste de vazamento hidrostático offshore (no nível da plataforma)"@pt-br ;
    skos:prefLabel "Offshore Leak Test At Platform Level Nominal Pressure"@en,
        "Pressão Nominal para Teste de Vazamento Offshore no Nível da Plataforma"@pt-br ;
    :hasAttributeScope :InstanceLevelAttribute ;
    :hasTypedValue :floatValue ;
    :hasValueCardinality :singleValue .

:OffLeakPLevNomPressValRef a owl:DatatypeProperty ;
    dcterms:accessRights "PUBLIC" ;
    dcterms:identifier "OffLeakPLevNomPressValRef" ;
    rdfs:subClassOf :HydrostaticPressureTestsAttribute ;
    skos:definition "Specifies the reference pressure used to determine the Offshore Leak Test nominal pressure value."@en,
        "Comentários Condições de teste dos tramos para - Nominal - Teste de vazamento hidrostático offshore (no nível da plataforma)"@pt-br ;
    skos:prefLabel "Offshore Leak Test At Platform Level Nominal Pressure Value Reference"@en,
        "Referência de Valor de Pressão Nominal para Teste de Vazamento Offshore no Nível da Plataforma"@pt-br ;
    :hasAttributeScope :InstanceLevelAttribute ;
    :hasTypedValue :stringValue ;
    :hasValueCardinality :singleValue .

:OffLeakPLevNomPressValRefMult a owl:DatatypeProperty ;
    dcterms:accessRights "PUBLIC" ;
    dcterms:identifier "OffLeakPLevNomPressValRefMult" ;
    rdfs:subClassOf :HydrostaticPressureTestsAttribute ;
    skos:definition "The multiplier applied to the reference pressure to determine the Offshore Leak Test nominal pressure value."@en ;
    skos:prefLabel "Offshore Leak Test At Platform Level Nominal Pressure Value Reference Multiplier"@en,
        "Multiplicador de Referência de Valor de Pressão Nominal para Teste de Vazamento Offshore no Nível da Plataforma"@pt-br ;
    :hasAttributeScope :InstanceLevelAttribute ;
    :hasTypedValue :floatValue ;
    :hasValueCardinality :singleValue .

:OuterDiameter a owl:DatatypeProperty ;
    dcterms:accessRights "PUBLIC" ;
    dcterms:identifier "OuterDiameter" ;
    rdfs:subPropertyOf :DomainAttribute ;
    skos:definition "Represents the external diameter of a component, typically measured from one outer edge to the opposite outer edge. This property is important for ensuring proper fit, compatibility, and performance within a system or assembly."@en ;
    skos:prefLabel "Outer Diameter"@en,
        "Diâmetro externo"@pt-br ;
    :hasAttributeScope :TypeLevelAttribute ;
    :hasTypedValue :floatValue ;
    :hasValueCardinality :singleValue .

:OutsideTemperature a owl:DatatypeProperty ;
    dcterms:accessRights "PUBLIC" ;
    dcterms:identifier "OutsideTemperature" ;
    rdfs:subClassOf :BendingStiffnessAttribute ;
    skos:definition "Represents the external temperature surrounding a component or system. This property is important for assessing the thermal conditions that the component is exposed to, ensuring it operates within safe temperature limits."@en ;
    skos:prefLabel "Outside Temperature"@en,
        "Temperatura Externa"@pt-br ;
    :hasAttributeScope :TypeLevelAttribute ;
    :hasTypedValue :floatValue ;
    :hasValueCardinality :singleValue .

:PartNumber a owl:DatatypeProperty ;
    dcterms:accessRights "PUBLIC" ;
    dcterms:identifier "PartNumber" ;
    rdfs:subPropertyOf :DomainAttribute ;
    skos:definition "The Part Number is a unique identifier assigned to each type of element, ensuring consistency and ease of reference. This identifier helps in categorizing, ordering, and tracking the accessory within the system. When the drawing code is used consistently across all projects for a specific type of accessory, it can also serve as the Part Number, facilitating uniformity in documentation and usage."@en ;
    skos:prefLabel "Part Number"@en,
        "Número da peça do acessório"@pt-br ;
    :hasAttributeScope :TypeLevelAttribute ;
    :hasTypedValue :stringValue ;
    :hasValueCardinality :singleValue .

:PermeabilityTable_MoleculeIdentifier a owl:DatatypeProperty ;
    dcterms:accessRights "PUBLIC" ;
    dcterms:identifier "PermeabilityTable_MoleculeIdentifier" ;
    rdfs:subClassOf :PermeabilityTableAttribute ;
    skos:definition "Specifies the type of molecule. This property identifies the particular molecule involved, which is crucial for understanding the material's interaction with or response to different chemical substances."@en,
        "tipo de molécula (co2, h2s, ch4, h2o,…)"@pt-br ;
    skos:prefLabel "Molecule Identifier"@en,
        "Identificador de Molécula"@pt-br ;
    :hasAttributeScope :TypeLevelAttribute ;
    :hasTypedValue :stringValue ;
    :hasValueCardinality :multiValue .

:PermeabilityTable_PermeabilityCoefficient a owl:DatatypeProperty ;
    dcterms:accessRights "PUBLIC" ;
    dcterms:identifier "PermeabilityTable_PermeabilityCoefficient" ;
    rdfs:subClassOf :PermeabilityTableAttribute ;
    skos:definition "Represents the rate at which a substance, such as a gas or liquid, can pass through a material. This property is crucial for understanding the material's resistance to permeation, helping to assess its suitability for containing or isolating specific substances."@en ;
    skos:prefLabel "Permeability Coefficient"@en,
        "Coeficiente de Permeabilidade"@pt-br ;
    :hasAttributeScope :TypeLevelAttribute ;
    :hasTypedValue :floatValue ;
    :hasValueCardinality :multiValue .

:PermeabilityTable_PolymerState a owl:DatatypeProperty ;
    dcterms:accessRights "PUBLIC" ;
    dcterms:identifier "PermeabilityTable_PolymerState" ;
    rdfs:subClassOf :PermeabilityTableAttribute ;
    skos:definition "The state of the polymeric material is specified.. This property is crucial for understanding how the material behaves under different conditions and its suitability for various applications."@en,
        "(plastificado, não plastificado,…)"@pt-br ;
    skos:prefLabel "Polymer State"@en,
        "Estado do Polímero"@pt-br ;
    :hasAttributeScope :TypeLevelAttribute ;
    :hasTypedValue :stringValue ;
    :hasValueCardinality :multiValue .

:PermeabilityTable_Temperature a owl:DatatypeProperty ;
    dcterms:accessRights "PUBLIC" ;
    dcterms:identifier "PermeabilityTable_Temperature" ;
    rdfs:subClassOf :PermeabilityTableAttribute ;
    skos:definition "Represents the thermal condition or measurement of heat for a component or system. This property is important for assessing how the component performs or operates under specific thermal conditions, ensuring it remains within safe and effective operating limits."@en ;
    skos:prefLabel "Temperature"@en,
        "Temperatura"@pt-br ;
    :hasAttributeScope :TypeLevelAttribute ;
    :hasTypedValue :floatValue ;
    :hasValueCardinality :multiValue .

:Piggable a owl:DatatypeProperty ;
    dcterms:accessRights "PUBLIC" ;
    dcterms:identifier "Piggable" ;
    rdfs:subPropertyOf :DomainAttribute ;
    skos:definition "Whether equipment has at least one internal flow circuit allowing pig runs"@en,
        "Especifica se o equipamento possui pelo menos um circuito interno de escoamento que permita passagem de pig"@pt-br ;
    skos:prefLabel "Piggable"@en,
        "Pigável"@pt-br ;
    :hasAttributeScope :TypeLevelAttribute ;
    :hasTypedValue :booleanValue ;
    :hasValueCardinality :singleValue .

:PipeSectionApplication a owl:DatatypeProperty ;
    dcterms:accessRights "PUBLIC" ;
    dcterms:identifier "PipeSectionApplication" ;
    rdfs:subPropertyOf :DomainAttribute ;
    skos:definition "Indicates the specific application of the flexible pipe section in the interconnection system, categorizing it based on its role or position within the riser or flowline."@en,
        "Aplicação do tramo, de acordo com as seguintes nomenclaturas: R (Riser); RT (seção de topo do riser); RI (seção intermediaria do riser); RF (seção de fundo do riser); F (Flowline)"@pt-br ;
    skos:prefLabel "Pipe Section Application"@en,
        "Aplicação do Tramo"@pt-br ;
    :hasAttributeScope :InstanceLevelAttribute ;
    :hasTypedValue :stringValue ;
    :hasValueCardinality :singleValue .

:PipeSegment a owl:Class ;
    dcterms:identifier "PipeSegment" ;
    rdfs:subClassOf :TransportLineSegment ;
    skos:definition "Pipeline segment for movement/flow of fluids."@en,
        "Segmento de Duto"@pt-br ;
    skos:prefLabel "Pipe Segment"@en,
        "Segmento de Duto"@pt-br .

:PipeTermination a owl:Class ;
    dcterms:identifier "PipeTermination" ;
    rdfs:subClassOf :LineTermination ;
    skos:definition "The Pipe Termination refers to the components at the end of a pipeline that provide the final connection to other equipment or systems. These terminations are crucial for ensuring a secure and reliable interface between the pipeline and surrounding infrastructure, allowing for the proper transfer of fluids or gases and maintaining the integrity of the overall system."@en ;
    skos:prefLabel "Pipe Termination"@en,
        "Terminador de Duto"@pt-br .

:Planned_Start_Timestamp a owl:DatatypeProperty ;
    dcterms:accessRights "PUBLIC" ;
    dcterms:identifier "Planned_Start_Timestamp" ;
    rdfs:subPropertyOf :DomainAttribute ;
    skos:prefLabel "Planned Start Timestamp"@en ;
    :hasAttributeScope :InstanceLevelAttribute ;
    :hasTypedValue :dateTimeValue ;
    :hasValueCardinality :singleValue .

:PointLocation a owl:Class ;
    dcterms:identifier "PointLocation" ;
    rdfs:subClassOf :Location ;
    skos:definition "Basis for all locations that can conventionally be situated at a single geographic point."@en ;
    skos:prefLabel "Point Location"@en,
        "Localização de Ponto"@pt-br .

:PoissonRatioAt23Degrees a owl:DatatypeProperty ;
    dcterms:accessRights "PUBLIC" ;
    dcterms:identifier "PoissonRatioAt23Degrees" ;
    rdfs:subPropertyOf :DomainAttribute ;
    skos:definition "Indicates Poisson's ratio of the material at 23 degrees Celsius, representing the ratio of transverse strain to axial strain when the material is subjected to stress. This property is essential for understanding the material's deformation behavior under load and its response to mechanical forces in subsea environments."@en,
        "Coeficiente de Poisson a 23 graus Celsius (Específica para Materiais Metálicos e Poliméricos)"@pt-br ;
    skos:prefLabel "Poisson Ratio At 23 Degrees"@en,
        "Coeficiente de Poisson a 23 Graus Celsius"@pt-br ;
    :hasAttributeScope :TypeLevelAttribute ;
    :hasTypedValue :floatValue ;
    :hasValueCardinality :singleValue .

:PolymericLayerMaterialType a owl:DatatypeProperty ;
    dcterms:accessRights "PUBLIC" ;
    dcterms:identifier "PolymericLayerMaterialType" ;
    rdfs:subPropertyOf :DomainAttribute ;
    skos:definition "Type of material from which an object is made, allowing for precise documentation and categorisation."@en ;
    skos:prefLabel "Polymeric Layer Material Type"@en,
        "Tipo de Material da Camada Polimérica"@pt-br ;
    :hasAttributeScope :TypeLevelAttribute ;
    :hasTypedValue :stringValue ;
    :hasValueCardinality :singleValue .

:PostSlippingBendingStiffness a owl:DatatypeProperty ;
    dcterms:accessRights "PUBLIC" ;
    dcterms:identifier "PostSlippingBendingStiffness" ;
    rdfs:subClassOf :BendingStiffnessAttribute ;
    skos:definition "Represents the stiffness of a component after slipping occurs during bending. This property is important for evaluating the structural response and stability of the component once it has experienced slippage, ensuring that it can still withstand bending loads without significant deformation."@en ;
    skos:prefLabel "Post Slipping Bending Stiffness"@en,
        "Rigidez de Flexão Pós-Escorregamento"@pt-br ;
    :hasAttributeScope :TypeLevelAttribute ;
    :hasTypedValue :floatValue ;
    :hasValueCardinality :singleValue .

:PowerMachine a owl:Class ;
    dcterms:identifier "PowerMachine" ;
    rdfs:subClassOf :PressureComponent .

:PreSlippingBendingStiffness a owl:DatatypeProperty ;
    dcterms:accessRights "PUBLIC" ;
    dcterms:identifier "PreSlippingBendingStiffness" ;
    rdfs:subClassOf :BendingStiffnessAttribute ;
    skos:definition "Represents the stiffness of a component before any slipping occurs during bending. This property is important for assessing how the component resists bending forces prior to slippage, ensuring that it maintains its shape and performance under load."@en ;
    skos:prefLabel "Pre Slipping Bending Stiffness"@en,
        "Rigidez de Flexão Pré-Escorregamento"@pt-br ;
    :hasAttributeScope :TypeLevelAttribute ;
    :hasTypedValue :floatValue ;
    :hasValueCardinality :singleValue .

:ProcessingModule a owl:Class ;
    dcterms:identifier "ProcessingModule" ;
    rdfs:subClassOf :FlowControlModule .

:ProjectAcronym a owl:DatatypeProperty ;
    dcterms:accessRights "PUBLIC" ;
    dcterms:identifier "ProjectAcronym" ;
    rdfs:subPropertyOf :DomainAttribute ;
    skos:definition "Indicates the unique identification code assigned to the operator's project. This property is used for tracking, managing, and referencing the project throughout all phases of its lifecycle, ensuring proper identification and organization."@en,
        "Abreviação do nome do projeto da Interligação Submarina. Ex., 'SEP' para o \"FPSO Carioca do campo de Sépia\""@pt-br ;
    skos:prefLabel "Project Acronym"@en,
        "Abreviação do Nome do Projeto da Interligação Submarina"@pt-br ;
    :hasAttributeScope :InstanceLevelAttribute ;
    :hasTypedValue :stringValue ;
    :hasValueCardinality :singleValue .

:ProjectCode a owl:DatatypeProperty ;
    dcterms:accessRights "PUBLIC" ;
    dcterms:identifier "ProjectCode" ;
    rdfs:subPropertyOf :DomainAttribute ;
    skos:definition "Unique identification code assigned to the operator's project, used for tracking, managing, and referencing the project across all phases of its lifecycle."@en ;
    skos:prefLabel "Project Code"@en,
        "Código Identificador único do projeto da operadora da Interligação Submarina"@pt-br ;
    :hasAttributeScope :InstanceLevelAttribute ;
    :hasTypedValue :stringValue ;
    :hasValueCardinality :singleValue .

:ProjectDrawingCode a owl:DatatypeProperty ;
    dcterms:accessRights "PUBLIC" ;
    dcterms:identifier "ProjectDrawingCode" ;
    rdfs:subPropertyOf :DomainAttribute ;
    skos:definition "Indicates the unique alphanumeric code assigned to the project drawing. This property is used to reference and locate the specific drawing associated with the item, providing a clear and organized method for tracking and accessing drawing documents."@en,
        "Número do desenho do projeto do acessório"@pt-br ;
    skos:prefLabel "Project Drawing Code"@en,
        "Número do Desenho do Projeto"@pt-br ;
    :hasAttributeScope :TypeLevelAttribute ;
    :hasTypedValue :stringValue ;
    :hasValueCardinality :singleValue .

:ProjectDrawingRevision a owl:DatatypeProperty ;
    dcterms:accessRights "PUBLIC" ;
    dcterms:identifier "ProjectDrawingRevision" ;
    rdfs:subPropertyOf :DomainAttribute ;
    skos:definition "Indicates the revision number or identifier of the project drawing. This property tracks the version of the drawing, providing essential information for identifying updates, changes, and the most current version of the drawing related to the item."@en ;
    skos:prefLabel "Project Drawing Revision"@en,
        "Revisão do Desenho do Projeto"@pt-br ;
    :hasAttributeScope :TypeLevelAttribute ;
    :hasTypedValue :stringValue ;
    :hasValueCardinality :singleValue .

:PullingHead a owl:Class ;
    dcterms:identifier "PullingHead" ;
    rdfs:subClassOf :LineAncillary ;
    skos:altLabel "Cable Head"@en,
        "Installation Head"@en,
        "Pulling Grip"@en,
        "Pulling Tool"@en ;
    skos:definition "A component used in subsea flexible pipe installations to provide a secure attachment point for pulling the pipe into position during installation or retrieval operations. The Pulling Head is fitted to the end of the flexible pipe, allowing connection to pulling equipment such as winches or cranes. It is designed to withstand high loads, ensuring that the pipe can be pulled safely without causing damage. The Pulling Head is essential for handling, testing, and securing the pipe in place during subsea installation."@en ;
    skos:prefLabel "Pulling Head"@en,
        "Cabeça de Tração"@pt-br .

:PullingHeadType a owl:DatatypeProperty ;
    dcterms:accessRights "PUBLIC" ;
    dcterms:identifier "PullingHeadType" ;
    rdfs:subPropertyOf :DomainAttribute ;
    skos:definition "Specifies the type of pulling head used for the installation or retrieval of subsea flexible structures. It describes the design and functionality of the pulling head, including details such as compatibility with specific installation methods, mechanical connections, and any special features or adaptations for handling loads during pulling operations. This property helps to ensure the correct pulling head is selected based on the requirements of the project and the conditions of the installation site."@en ;
    skos:prefLabel "Pulling Head Type"@en,
        "Tipo de Cabeça de Tração"@pt-br ;
    :hasAttributeScope :TypeLevelAttribute ;
    :hasTypedValue :stringValue ;
    :hasValueCardinality :singleValue .

:ROVTool a owl:Class ;
    dcterms:identifier "ROVTool" ;
    rdfs:subClassOf :Accessory .

:ReferenceDrawing a owl:Class ;
    dcterms:identifier "ReferenceDrawing" ;
    rdfs:subClassOf :DomainElement ;
    skos:definition "A technical drawing providing detailed information about a specific component, system, or assembly, used as a guide for manufacturing, installation, or maintenance in subsea projects."@en ;
    skos:prefLabel "Reference Drawing"@en,
        "Desenhos de Referência"@pt-br .

:RiserConfiguration a owl:DatatypeProperty ;
    dcterms:accessRights "PUBLIC" ;
    dcterms:identifier "RiserConfiguration" ;
    rdfs:subPropertyOf :DomainAttribute ;
    skos:definition "This property specifies the configuration type for the riser section of the pipeline. It provides key information on the structural design, indicating the arrangement and dynamic behaviour of the riser system. The chosen configuration affects how the structure responds to environmental forces, such as currents and pressure, and plays a critical role in determining the overall performance and durability of the system."@en ;
    skos:prefLabel "Riser Configuration"@en,
        "Configuração do Riser"@pt-br ;
    :hasAttributeScope :InstanceLevelAttribute ;
    :hasTypedValue :stringValue ;
    :hasValueCardinality :singleValue .

:RotatingMachine a owl:Class ;
    dcterms:identifier "RotatingMachine" ;
    rdfs:subClassOf :PowerMachine .

:RuptDefAlongFibers a owl:DatatypeProperty ;
    dcterms:accessRights "PUBLIC" ;
    dcterms:identifier "RuptDefAlongFibers" ;
    rdfs:subPropertyOf :DomainAttribute ;
    skos:definition "Describes the deformation that occurs when the composite material ruptures in a direction parallel to its fibers. This property is essential for assessing the material's behavior under stress aligned with the fiber orientation, providing insights into its performance and durability in subsea structures where axial forces are present."@en ;
    skos:prefLabel "Rupture Deformation Along Fibers"@en,
        "Deformação de Ruptura longitudinalmente às fibras"@pt-br ;
    :hasAttributeScope :TypeLevelAttribute ;
    :hasTypedValue :floatValue ;
    :hasValueCardinality :singleValue .

:RuptDefPerpendFibers a owl:DatatypeProperty ;
    dcterms:accessRights "PUBLIC" ;
    dcterms:identifier "RuptDefPerpendFibers" ;
    rdfs:subPropertyOf :DomainAttribute ;
    skos:definition "Describes the deformation that occurs when the composite material ruptures in a direction perpendicular to its fibers. This property is crucial for understanding the material's behavior under stress conditions that do not align with the fiber orientation, helping to assess its performance and failure limits in subsea structures."@en ;
    skos:prefLabel "Rupture Deformation Perpendicular To Fibers"@en,
        "Deformação de Ruptura perpendicularmente às fibras"@pt-br ;
    :hasAttributeScope :TypeLevelAttribute ;
    :hasTypedValue :floatValue ;
    :hasValueCardinality :singleValue .

:SerialNumber a owl:DatatypeProperty ;
    dcterms:accessRights "PUBLIC" ;
    dcterms:identifier "SerialNumber" ;
    rdfs:subPropertyOf :DomainAttribute ;
    skos:definition "A unique identifier assigned to each individual item, distinguishing it from all other units of the same type. The Serial Number is critical for traceability, maintenance, and warranty purposes, ensuring that the history, performance, and lifecycle of the equipment can be tracked. It is often used in conjunction with a Part Number, which identifies the type or model of the component."@en ;
    skos:prefLabel "Serial Number"@en,
        "Número de Série"@pt-br ;
    :hasAttributeScope :InstanceLevelAttribute ;
    :hasTypedValue :stringValue ;
    :hasValueCardinality :singleValue .

:Service a owl:DatatypeProperty ;
    dcterms:accessRights "PUBLIC" ;
    dcterms:identifier "Service" ;
    rdfs:subPropertyOf :DomainAttribute ;
    skos:definition "Indicates the type of service the pipeline is designated for, specifying its operational purpose within the project. This classification is used to ensure proper management, installation, and use of the pipeline according to its intended function."@en,
        "Escolha um da lista: IA (Injeção de água); IG (Injeção de Gás); LPO (Linha de Produção de Óleo); PG (Produtor de Gás); SE (Serviço); GAS (Gasoduto); UEH (Umbilical Eletro Hidráulico); CEP (Cabo Elétrico de Potência)"@pt-br ;
    skos:prefLabel "Service"@en,
        "Serviço"@pt-br ;
    :hasAttributeScope :InstanceLevelAttribute ;
    :hasTypedValue :stringValue ;
    :hasValueCardinality :singleValue .

:ShackleInnerDiameter a owl:DatatypeProperty ;
    dcterms:accessRights "PUBLIC" ;
    dcterms:identifier "ShackleInnerDiameter" ;
    rdfs:subPropertyOf :DomainAttribute ;
    skos:definition "Indicates the inner diameter of the shackle. This property measures the width of the space inside the shackle, which is important for ensuring compatibility with other components and for determining the appropriate fit and load distribution."@en ;
    skos:prefLabel "Shackle Inner Diameter"@en,
        "Diâmetro interno da furação do olhal"@pt-br ;
    :hasAttributeScope :InstanceLevelAttribute ;
    :hasTypedValue :floatValue ;
    :hasValueCardinality :singleValue .

:ShackleOpeningWidth a owl:DatatypeProperty ;
    dcterms:accessRights "PUBLIC" ;
    dcterms:identifier "ShackleOpeningWidth" ;
    rdfs:subPropertyOf :DomainAttribute ;
    skos:definition "Measures the width of the opening in the shackle where components, such as pins or cables, are inserted. This property is crucial for ensuring that the shackle can properly accommodate and secure the intended connecting elements."@en ;
    skos:prefLabel "Shackle Opening Width"@en,
        "Largura da Abertura"@pt-br ;
    :hasAttributeScope :InstanceLevelAttribute ;
    :hasTypedValue :floatValue ;
    :hasValueCardinality :singleValue .

:ShackleOuterDiameter a owl:DatatypeProperty ;
    dcterms:accessRights "PUBLIC" ;
    dcterms:identifier "ShackleOuterDiameter" ;
    rdfs:subPropertyOf :DomainAttribute ;
    skos:definition "Indicates the outer diameter of the shackle. This property provides the measurement of the overall width of the shackle, which is crucial for ensuring it fits properly with other components and meets the design specifications for load-bearing and connection requirements."@en ;
    skos:prefLabel "Shackle Outer Diameter"@en,
        "Diâmetro externo do olhal"@pt-br ;
    :hasAttributeScope :InstanceLevelAttribute ;
    :hasTypedValue :floatValue ;
    :hasValueCardinality :singleValue .

:ShackleThickness a owl:DatatypeProperty ;
    dcterms:accessRights "PUBLIC" ;
    dcterms:identifier "ShackleThickness" ;
    rdfs:subPropertyOf :DomainAttribute ;
    skos:definition "Specifies the thickness of the shackle material. This property measures the distance between the inner and outer surfaces of the shackle, which is essential for understanding its strength, durability, and ability to handle load stresses."@en ;
    skos:prefLabel "Shackle Thickness"@en,
        "Espessura do olhal"@pt-br ;
    :hasAttributeScope :InstanceLevelAttribute ;
    :hasTypedValue :floatValue ;
    :hasValueCardinality :singleValue .

:ShortTermFloatDensity a owl:DatatypeProperty ;
    dcterms:accessRights "PUBLIC" ;
    dcterms:identifier "ShortTermFloatDensity" ;
    rdfs:subPropertyOf :DomainAttribute ;
    skos:definition "The density of the float material in the early stages of operation, accounting for slight water absorption or other surface-level changes."@en,
        "Representa a densidade do flutuador logo após o início da operação, considerando um aumento de densidade devido à absorção de água em pequena quantidade ou outras alterações superficiais."@pt-br ;
    skos:prefLabel "Short Term Float Density"@en,
        "Densidade do Flutuador a Curto Prazo"@pt-br ;
    :hasAttributeScope :TypeLevelAttribute ;
    :hasTypedValue :floatValue ;
    :hasValueCardinality :singleValue .

:ShortTermFloatVolume a owl:DatatypeProperty ;
    dcterms:accessRights "PUBLIC" ;
    dcterms:identifier "ShortTermFloatVolume" ;
    rdfs:subPropertyOf :DomainAttribute ;
    skos:definition "The expected submerged volume of the float during the initial phase of operation, considering minor factors like slight water absorption or small deformations."@en,
        "O volume submerso esperado logo após o início da operação, levando em consideração pequenas variações iniciais, como a absorção mínima de água ou pequenas deformações. Serve para calcular a flutuabilidade em condições reais no curto prazo."@pt-br ;
    skos:prefLabel "Short Term Float Volume"@en,
        "Volume do Flutuador a Curto Prazo"@pt-br ;
    :hasAttributeScope :TypeLevelAttribute ;
    :hasTypedValue :floatValue ;
    :hasValueCardinality :singleValue .

:SolubilityTable_MoleculeIdentifier a owl:DatatypeProperty ;
    dcterms:accessRights "PUBLIC" ;
    dcterms:identifier "SolubilityTable_MoleculeIdentifier" ;
    rdfs:subClassOf :SolubilityTable ;
    skos:definition "Specifies the type of molecule. This property identifies the particular molecule involved, which is crucial for understanding the material's interaction with or response to different chemical substances."@en,
        "Tipo de Molécula (co2, h2s, ch4, h2o,…)"@pt-br ;
    skos:prefLabel "Molecule Identifier"@en,
        "Identificador de Molécula"@pt-br ;
    :hasAttributeScope :TypeLevelAttribute ;
    :hasTypedValue :stringValue ;
    :hasValueCardinality :multiValue .

:SolubilityTable_PolymerState a owl:DatatypeProperty ;
    dcterms:accessRights "PUBLIC" ;
    dcterms:identifier "SolubilityTable_PolymerState" ;
    rdfs:subClassOf :SolubilityTable ;
    skos:definition "The state of the polymeric material is specified.. This property is crucial for understanding how the material behaves under different conditions and its suitability for various applications."@en ;
    skos:prefLabel "Polymer State"@en,
        "Estado do Polímero"@pt-br ;
    :hasAttributeScope :TypeLevelAttribute ;
    :hasTypedValue :stringValue ;
    :hasValueCardinality :multiValue .

:SolubilityTable_SolubilityCoefficient a owl:DatatypeProperty ;
    dcterms:accessRights "PUBLIC" ;
    dcterms:identifier "SolubilityTable_SolubilityCoefficient" ;
    rdfs:subClassOf :SolubilityTable ;
    skos:definition "Represents the rate at which a substance dissolves in a specific material, indicating how much of the substance can be absorbed by the material. This property is important for understanding the material's chemical compatibility and behavior when exposed to various substances."@en ;
    skos:prefLabel "Solubility Coefficient"@en,
        "Coeficiente de solubilidade"@pt-br ;
    :hasAttributeScope :TypeLevelAttribute ;
    :hasTypedValue :floatValue ;
    :hasValueCardinality :multiValue .

:SolubilityTable_Temperature a owl:DatatypeProperty ;
    dcterms:accessRights "PUBLIC" ;
    dcterms:identifier "SolubilityTable_Temperature" ;
    rdfs:subClassOf :SolubilityTable ;
    skos:definition "Represents the thermal condition or measurement of heat for a component or system. This property is important for assessing how the component performs or operates under specific thermal conditions, ensuring it remains within safe and effective operating limits."@en ;
    skos:prefLabel "Temperature"@en,
        "Temperatura"@pt-br ;
    :hasAttributeScope :TypeLevelAttribute ;
    :hasTypedValue :floatValue ;
    :hasValueCardinality :multiValue .

:SpecialRequirements a owl:DatatypeProperty ;
    dcterms:accessRights "PUBLIC" ;
    dcterms:identifier "SpecialRequirements" ;
    rdfs:subPropertyOf :DomainAttribute ;
    skos:definition "Special requirements refer to specific conditions, standards, or instructions that must be met during the design, manufacturing, installation, or operation of an object or system. These can include unique technical specifications, safety measures, regulatory compliance, or client-specific requests that go beyond standard procedures."@en,
        "Requisitos especiais, Observações ou Documentos especiais para o tramo"@pt-br ;
    skos:prefLabel "Special Requirements"@en,
        "Requisitos Especiais"@pt-br ;
    :hasAttributeScope :InstanceLevelAttribute ;
    :hasTypedValue :stringValue ;
    :hasValueCardinality :singleValue .

:SpecificHeatCapacity a owl:DatatypeProperty ;
    dcterms:accessRights "PUBLIC" ;
    dcterms:identifier "SpecificHeatCapacity" ;
    rdfs:subPropertyOf :DomainAttribute ;
    skos:definition "Indicates the amount of heat required to raise the temperature of the material by a specific amount, typically measured per unit mass. This property is important for understanding the thermal behavior of the material.."@en,
        "Calor Específico do material"@pt-br ;
    skos:prefLabel "Specific Heat Capacity"@en,
        "Calor Específico"@pt-br ;
    :hasAttributeScope :TypeLevelAttribute ;
    :hasTypedValue :floatValue ;
    :hasValueCardinality :singleValue .

:SpecificWeight a owl:DatatypeProperty ;
    dcterms:accessRights "PUBLIC" ;
    dcterms:identifier "SpecificWeight" ;
    rdfs:subPropertyOf :DomainAttribute ;
    skos:definition "Indicates the weight of the material per unit volume. This property is crucial for understanding the material's density and its impact on the overall weight."@en,
        "Peso específico do material"@pt-br ;
    skos:prefLabel "Specific Weight"@en,
        "Peso Específico"@pt-br ;
    :hasAttributeScope :TypeLevelAttribute ;
    :hasTypedValue :floatValue ;
    :hasValueCardinality :singleValue .

:SpoolingTension a owl:DatatypeProperty ;
    dcterms:accessRights "PUBLIC" ;
    dcterms:identifier "SpoolingTension" ;
    rdfs:subPropertyOf :DomainAttribute ;
    skos:definition "Represents the tension applied to a flexible component during the spooling process. This property is crucial for ensuring that the material is wound onto the reel or spool without exceeding its mechanical limits, preventing damage or deformation during handling and storage."@en ;
    skos:prefLabel "Spooling Tension"@en,
        "Tração de Desenrolamento"@pt-br ;
    :hasAttributeScope :TypeLevelAttribute ;
    :hasTypedValue :floatValue ;
    :hasValueCardinality :singleValue .

:StiffTorsionalStiffnessAtSeaLevel a owl:DatatypeProperty ;
    dcterms:accessRights "PUBLIC" ;
    dcterms:identifier "StiffTorsionalStiffnessAtSeaLevel" ;
    rdfs:subPropertyOf :DomainAttribute ;
    skos:definition "Represents the torsional stiffness of a component when measured at sea level, indicating its resistance to twisting under applied torque. This property is important for ensuring that the component maintains its structural integrity and performance under rotational forces."@en,
        "Rigidez a torção (GJ) (maior valor) a 20°C e pressão atmosferica (dentro e fora)"@pt-br ;
    skos:prefLabel "Stiff Torsional Stiffness At Sea Level"@en,
        "Rigidez a Torção Rígida ao Nível do Mar"@pt-br ;
    :hasAttributeScope :TypeLevelAttribute ;
    :hasTypedValue :floatValue ;
    :hasValueCardinality :singleValue .

:StrIntOffPLevMaxPress a owl:DatatypeProperty ;
    dcterms:accessRights "PUBLIC" ;
    dcterms:identifier "StrIntOffPLevMaxPress" ;
    rdfs:subClassOf :HydrostaticPressureTestsAttribute ;
    skos:definition "The maximum pressure applied during the Structural Integrity Test (offshore, at platform level), ensuring structural integrity under extreme conditions."@en,
        "Condições de teste dos tramos para Pressão - Máxima - Teste de integridade estrutural hidrostática (off-shore, no nível da plataforma)"@pt-br ;
    skos:prefLabel "Structural Integrity Offshore Leak Test At Platform Level Maximum Pressure"@en,
        "Integridade Estrutural Offshore com Pressão Máxima no Nível da Plataforma"@pt-br ;
    :hasAttributeScope :InstanceLevelAttribute ;
    :hasTypedValue :floatValue ;
    :hasValueCardinality :singleValue .

:StrIntOffPLevMaxPressValRef a owl:DatatypeProperty ;
    dcterms:accessRights "PUBLIC" ;
    dcterms:identifier "StrIntOffPLevMaxPressValRef" ;
    rdfs:subClassOf :HydrostaticPressureTestsAttribute ;
    skos:definition "Specifies the reference pressure used to determine the Structural Offshore Maximum Pressure value."@en,
        "Comentários Condições de teste dos tramos para - Máximo - Teste de integridade estrutural hidrostática (off-shore, no nível da plataforma)"@pt-br ;
    skos:prefLabel "Structural Integrity Offshore Leak Test At Platform Level Maximum Pressure Value Reference"@en,
        "Referência de Valor de Pressão Máxima para Teste de Integridade Estrutural Offshore e de Vazamento no Nível da Plataforma"@pt-br ;
    :hasAttributeScope :InstanceLevelAttribute ;
    :hasTypedValue :stringValue ;
    :hasValueCardinality :singleValue .

:StrIntOffPLevMaxPressValRefMult a owl:DatatypeProperty ;
    dcterms:accessRights "PUBLIC" ;
    dcterms:identifier "StrIntOffPLevMaxPressValRefMult" ;
    rdfs:subClassOf :HydrostaticPressureTestsAttribute ;
    skos:definition "The multiplier applied to the reference pressure to determine the Structural Offshore Maximum Pressure value."@en ;
    skos:prefLabel "Structural Integrity Offshore Leak Test At Platform Level Maximum Pressure Value Reference Multiplier"@en,
        "Multiplicador de Referência de Valor de Pressão Máxima para Teste de Integridade Estrutural Offshore no Nível da Plataforma"@pt-br ;
    :hasAttributeScope :InstanceLevelAttribute ;
    :hasTypedValue :floatValue ;
    :hasValueCardinality :singleValue .

:StrIntOffPLevNomPress a owl:DatatypeProperty ;
    dcterms:accessRights "PUBLIC" ;
    dcterms:identifier "StrIntOffPLevNomPress" ;
    rdfs:subClassOf :HydrostaticPressureTestsAttribute ;
    skos:definition "The nominal pressure applied during the Structural Integrity Test (offshore, at platform level), simulating typical conditions to verify structural integrity."@en,
        "Condições de teste dos tramos para Pressão - Nominal - Teste de integridade estrutural hidrostática (off-shore, no nível da plataforma)"@pt-br ;
    skos:prefLabel "Structural Integrity Offshore Leak Test At Platform Level Nominal Pressure"@en,
        "Integridade Estrutural Offshore com Pressão Nominal no Nível da Plataforma"@pt-br ;
    :hasAttributeScope :InstanceLevelAttribute ;
    :hasTypedValue :floatValue ;
    :hasValueCardinality :singleValue .

:StrIntOffPLevNomPressValRef a owl:DatatypeProperty ;
    dcterms:accessRights "PUBLIC" ;
    dcterms:identifier "StrIntOffPLevNomPressValRef" ;
    rdfs:subClassOf :HydrostaticPressureTestsAttribute ;
    skos:definition "Specifies the reference pressure used to determine the Structural Offshore Leak Test Nominal Pressure value."@en,
        "Comentários Condições de teste dos tramos para - Nominal - Teste de integridade estrutural hidrostática (off-shore, no nível da plataforma)"@pt-br ;
    skos:prefLabel "Structural Integrity Offshore Leak Test At Platform Level Nominal Pressure Value Reference"@en,
        "Referência de Valor de Pressão Nominal para Teste de Integridade Estrutural Offshore no Nível da Plataforma"@pt-br ;
    :hasAttributeScope :InstanceLevelAttribute ;
    :hasTypedValue :stringValue ;
    :hasValueCardinality :singleValue .

:StrIntOffPLevNomPressValRefMult a owl:DatatypeProperty ;
    dcterms:accessRights "PUBLIC" ;
    dcterms:identifier "StrIntOffPLevNomPressValRefMult" ;
    rdfs:subClassOf :HydrostaticPressureTestsAttribute ;
    skos:definition "The multiplier applied to the reference pressure to determine the Structural Offshore Nominal Pressure value."@en ;
    skos:prefLabel "Structural Integrity Offshore Leak Test At Platform Level Nominal Pressure Value Reference Multiplier"@en,
        "Multiplicador de Referência de Valor de Pressão Nominal para Teste de Integridade Estrutural Offshore no Nível da Plataforma"@pt-br ;
    :hasAttributeScope :InstanceLevelAttribute ;
    :hasTypedValue :floatValue ;
    :hasValueCardinality :singleValue .

:StrIntOnNoTensMaxPress a owl:DatatypeProperty ;
    dcterms:accessRights "PUBLIC" ;
    dcterms:identifier "StrIntOnNoTensMaxPress" ;
    rdfs:subClassOf :HydrostaticPressureTestsAttribute ;
    skos:definition "The maximum pressure applied during the Structural Integrity Test (onboard, without tension), verifying performance under extreme conditions."@en,
        "Condições de teste dos tramos para Pressão - Máxima - Teste de integridade estrutural hidrostática (a bordo, sem tensão)"@pt-br ;
    skos:prefLabel "Structural Integrity Onboard With No Tension Maximum Pressure"@en,
        "Integridade Estrutural a Bordo sem Pressão Máxima de Tensão"@pt-br ;
    :hasAttributeScope :InstanceLevelAttribute ;
    :hasTypedValue :floatValue ;
    :hasValueCardinality :singleValue .

:StrIntOnNoTensMaxPressValRef a owl:DatatypeProperty ;
    dcterms:accessRights "PUBLIC" ;
    dcterms:identifier "StrIntOnNoTensMaxPressValRef" ;
    rdfs:subClassOf :HydrostaticPressureTestsAttribute ;
    skos:definition "Specifies the reference pressure used to determine the Structural Onboard Maximum Pressure value."@en,
        "Comentários Condições de teste dos tramos para - Máximo - Teste de integridade estrutural hidrostática (a bordo, sem tensão)"@pt-br ;
    skos:prefLabel "Structural Integrity Onboard With No Tension Maximum Pressure Value Reference"@en,
        "Referência de Valor de Pressão Máxima para Integridade Estrutural a Bordo sem Tensão"@pt-br ;
    :hasAttributeScope :InstanceLevelAttribute ;
    :hasTypedValue :stringValue ;
    :hasValueCardinality :singleValue .

:StrIntOnNoTensMaxPressValRefMult a owl:DatatypeProperty ;
    dcterms:accessRights "PUBLIC" ;
    dcterms:identifier "StrIntOnNoTensMaxPressValRefMult" ;
    rdfs:subClassOf :HydrostaticPressureTestsAttribute ;
    skos:definition "The multiplier applied to the reference pressure to determine the Structural Onboard Maximum Pressure value."@en ;
    skos:prefLabel "Structural Integrity Onboard With No Tension Maximum Pressure Value Reference Multiplier"@en,
        "Multiplicador de Referência de Valor de Pressão Máxima para Integridade Estrutural a Bordo sem Tensão"@pt-br ;
    :hasAttributeScope :InstanceLevelAttribute ;
    :hasTypedValue :floatValue ;
    :hasValueCardinality :singleValue .

:StrIntOnNoTensNomPress a owl:DatatypeProperty ;
    dcterms:accessRights "PUBLIC" ;
    dcterms:identifier "StrIntOnNoTensNomPress" ;
    rdfs:subClassOf :HydrostaticPressureTestsAttribute ;
    skos:definition "The nominal pressure applied during the Structural Integrity Test (onboard, without tension), simulating typical conditions to verify structural integrity."@en,
        "Condições de teste dos tramos para Pressão - Nominal - Teste de integridade estrutural hidrostática (on-board, sem tensão)"@pt-br ;
    skos:prefLabel "Structural Integrity Onboard With No Tension Nominal Pressure"@en,
        "Integridade Estrutural a Bordo sem Pressão Nominal de Tensão"@pt-br ;
    :hasAttributeScope :InstanceLevelAttribute ;
    :hasTypedValue :floatValue ;
    :hasValueCardinality :singleValue .

:StrIntOnNoTensNomPressValRef a owl:DatatypeProperty ;
    dcterms:accessRights "PUBLIC" ;
    dcterms:identifier "StrIntOnNoTensNomPressValRef" ;
    rdfs:subClassOf :HydrostaticPressureTestsAttribute ;
    skos:definition "Specifies the reference pressure used to determine the Structural Onboard Nominal Pressure value."@en,
        "Comentários Condições de teste dos tramos para - Nominal - Teste de integridade estrutural hidrostática (on-board, sem tensão)"@pt-br ;
    skos:prefLabel "Structural Integrity Onboard With No Tension Nominal Pressure Value Reference"@en,
        "Integridade Estrutural a Bordo sem Referência de Valor de Pressão Nominal de Tensão"@pt-br ;
    :hasAttributeScope :InstanceLevelAttribute ;
    :hasTypedValue :stringValue ;
    :hasValueCardinality :singleValue .

:StrIntOnNoTensNomPressValRefMult a owl:DatatypeProperty ;
    dcterms:accessRights "PUBLIC" ;
    dcterms:identifier "StrIntOnNoTensNomPressValRefMult" ;
    rdfs:subClassOf :HydrostaticPressureTestsAttribute ;
    skos:definition "The multiplier applied to the reference pressure to determine the Structural Onboard Nominal Pressure value."@en ;
    skos:prefLabel "Structural Integrity Onboard With No Tension Nominal Pressure Value Reference Multiplier"@en,
        "Multiplicador de Referência de Valor de Pressão Nominal para Integridade Estrutural a Bordo sem Tensão"@pt-br ;
    :hasAttributeScope :InstanceLevelAttribute ;
    :hasTypedValue :floatValue ;
    :hasValueCardinality :singleValue .

:StrandsTable_SpareQuantity a owl:DatatypeProperty ;
    dcterms:accessRights "PUBLIC" ;
    dcterms:identifier "StrandsTable_SpareQuantity" ;
    rdfs:subClassOf :StrandsTableAttribute ;
    skos:definition "Specifies the number of spare units available, ensuring adequate backup components are on hand for maintenance or replacement. This quantity helps in planning and minimizing downtime during operations in subsea environments."@en ;
    skos:prefLabel "Spare Quantity"@en,
        "Quantidade de Sobressalentes"@pt-br ;
    :hasAttributeScope :InstanceLevelAttribute ;
    :hasTypedValue :intValue ;
    :hasValueCardinality :multiValue .

:StrandsTable_StrandsLength a owl:DatatypeProperty ;
    dcterms:accessRights "PUBLIC" ;
    dcterms:identifier "StrandsTable_StrandsLength" ;
    rdfs:subClassOf :StrandsTableAttribute ;
    skos:definition "Length of the individual strands."@en ;
    skos:prefLabel "Strands Length"@en,
        "Comprimento das Cordoalhas"@pt-br ;
    :hasAttributeScope :InstanceLevelAttribute ;
    :hasTypedValue :floatValue ;
    :hasValueCardinality :multiValue .

:StrandsTable_StrandsQuantity a owl:DatatypeProperty ;
    dcterms:accessRights "PUBLIC" ;
    dcterms:identifier "StrandsTable_StrandsQuantity" ;
    rdfs:subClassOf :StrandsTableAttribute ;
    skos:definition "Number of individual strands used, determining the overall reinforcement and strength of the component."@en ;
    skos:prefLabel "Strands Quantity"@en,
        "Quantidade de Cordoalhas"@pt-br ;
    :hasAttributeScope :InstanceLevelAttribute ;
    :hasTypedValue :intValue ;
    :hasValueCardinality :multiValue .

:StructureApplicationsList a owl:DatatypeProperty ;
    dcterms:accessRights "PUBLIC" ;
    dcterms:identifier "StructureApplicationsList" ;
    rdfs:subPropertyOf :DomainAttribute ;
    skos:definition "Indicates the possible positions where the structure can be applied along the pipeline system. Multiple values can be selected to show in which sections, such as different parts of a riser or flowline, the structure is suitable for use."@en,
        "Lista de todas as possíveis aplicações para a estrutura Valores aplicáveis (Mais de um valor pode ser escolhido): R (Riser) RT (Para seção de topo do riser) RI (Para seção intermediaria do riser) RF (Para seção de fundo do riser) F (Para Flowline)"@pt-br ;
    skos:prefLabel "Structure Applications List"@en,
        "Lista de Aplicações da Estrutura"@pt-br ;
    :hasAttributeScope :TypeLevelAttribute ;
    :hasTypedValue :stringValue ;
    :hasValueCardinality :multiValue .

:StructureCode a owl:DatatypeProperty ;
    dcterms:accessRights "PUBLIC" ;
    dcterms:identifier "StructureCode" ;
    rdfs:subPropertyOf :DomainAttribute ;
    skos:definition "Indicates the code or identifier assigned to the structure. This property is used to uniquely identify and reference the structure within a system, ensuring proper tracking, documentation, and management."@en ;
    skos:prefLabel "Structure Code"@en,
        "Código da estrutura"@pt-br ;
    :hasAttributeScope :TypeLevelAttribute ;
    :hasTypedValue :stringValue ;
    :hasValueCardinality :singleValue .

:SubProjectId a owl:DatatypeProperty ;
    dcterms:accessRights "PUBLIC" ;
    dcterms:identifier "SubProjectId" ;
    rdfs:subPropertyOf :DomainAttribute ;
    skos:definition "Refers to the identification code assigned to the well or piece of equipment for which the interconnection is being designed. This code is often provisional, used during the initial stages of development, such as during the fabrication or installation of flexible pipelines, before a final approval or designation is granted. It serves as a reference point for all equipment and documentation until the well or equipment receives its definitive identification from the relevant regulatory authority. Examples include codes like LL-S.P6, LL-S.MSIAG1, or simpler identifiers such as P6 or MSIAG1."@en ;
    skos:prefLabel "Sub Project Id"@en,
        "Id do Subprojeto"@pt-br ;
    :hasAttributeScope :InstanceLevelAttribute ;
    :hasTypedValue :stringValue ;
    :hasValueCardinality :singleValue .

:SubseaLayout a owl:Class ;
    dcterms:identifier "SubseaLayout" ;
    rdfs:subClassOf :Location ;
    skos:definition "The arrangement or map of components and systems within a subsea environment, including pipelines, risers, manifolds, and other infrastructure."@en ;
    skos:prefLabel "Subsea Layout"@en,
        "Arranjo Submarino"@pt-br .

:SupplierProvidedMaterialName a owl:DatatypeProperty ;
    dcterms:accessRights "PUBLIC" ;
    dcterms:identifier "SupplierProvidedMaterialName" ;
    rdfs:subClassOf :MaterialManufacturerAttribute ;
    skos:definition "Name of the material as specified by the original supplier. This property identifies the exact material provided, ensuring it aligns with the required specifications for the accessory."@en ;
    skos:prefLabel "Supplier Provided Material Name"@en,
        "Nome do material conforme designado pelo fornecedor original do material"@pt-br ;
    :hasAttributeScope :TypeLevelAttribute ;
    :hasTypedValue :stringValue ;
    :hasValueCardinality :singleValue .

:TensileArmourAnnulusCondition a owl:DatatypeProperty ;
    dcterms:accessRights "PUBLIC" ;
    dcterms:identifier "TensileArmourAnnulusCondition" ;
    rdfs:subClassOf :BendingStiffnessAttribute ;
    skos:definition "Indicates the condition of the annulus in the tensile armour layer, which refers to the space between the tensile armour and other layers."@en,
        "Condição do anular das amarduras de tração, Alagado ou Seco"@pt-br ;
    skos:prefLabel "Tensile Armour Annulus Condition"@en,
        "Condição do Anular das Armaduras de Tração"@pt-br ;
    :hasAttributeScope :TypeLevelAttribute ;
    :hasTypedValue :stringValue ;
    :hasValueCardinality :singleValue .

:TensileArmourFreeAnnulusVolume a owl:DatatypeProperty ;
    dcterms:accessRights "PUBLIC" ;
    dcterms:identifier "TensileArmourFreeAnnulusVolume" ;
    rdfs:subPropertyOf :DomainAttribute ;
    skos:definition "Indicates the available volume within the annulus of the tensile armour layer that is not occupied by material."@en ;
    skos:prefLabel "Tensile Armour Free Annulus Volume"@en,
        "Volume livre do anular das armaduras de tração"@pt-br ;
    :hasAttributeScope :TypeLevelAttribute ;
    :hasTypedValue :floatValue ;
    :hasValueCardinality :singleValue .

:TensileWireLayAngle a owl:DatatypeProperty ;
    dcterms:accessRights "PUBLIC" ;
    dcterms:identifier "TensileWireLayAngle" ;
    rdfs:subPropertyOf :DomainAttribute ;
    skos:definition "Refers to the angle formed between the individual tensile wires and the longitudinal axis of the flexible pipe. This angle determines how the wires are arranged around the pipe, influencing its mechanical properties and performance under load."@en ;
    skos:prefLabel "Tensile Wire Lay Angle"@en,
        "Ângulo de Enrolamento dos Arames sob Tração"@pt-br ;
    :hasAttributeScope :InstanceLevelAttribute ;
    :hasTypedValue :floatValue ;
    :hasValueCardinality :singleValue .

:TensileWiresCount a owl:DatatypeProperty ;
    dcterms:accessRights "PUBLIC" ;
    dcterms:identifier "TensileWiresCount" ;
    rdfs:subPropertyOf :DomainAttribute ;
    skos:definition "Indicates the total number of tensile wires in the layer, which contributes to the mechanical strength and load-bearing capacity of the flexible pipe."@en ;
    skos:prefLabel "Tensile Wires Count"@en,
        "Quantidade de Arames de Tração"@pt-br ;
    :hasAttributeScope :InstanceLevelAttribute ;
    :hasTypedValue :intValue ;
    :hasValueCardinality :singleValue .

:TensionerPadsMaterial a owl:DatatypeProperty ;
    dcterms:accessRights "PUBLIC" ;
    dcterms:identifier "TensionerPadsMaterial" ;
    rdfs:subClassOf :CrushingFrictionCoefficientTighteningTableAttribute,
        :CrushingMaximumAllowableTighteningTableAttribute ;
    skos:definition "Indicates the fabrication material used for the tensioner pads. This property is important for assessing the durability, friction, and wear resistance of the pads, ensuring they perform effectively under operational conditions."@en,
        "Nome do material da sapata do tensionador (Por exemplo, Carbon Steel)"@pt-br ;
    skos:prefLabel "Tensioner Pads Material"@en,
        "Material das Sapatas do Tensionador"@pt-br ;
    :hasAttributeScope :TypeLevelAttribute ;
    :hasTypedValue :stringValue ;
    :hasValueCardinality :singleValue .

:TensionerPadsOpeningAngle a owl:DatatypeProperty ;
    dcterms:accessRights "PUBLIC" ;
    dcterms:identifier "TensionerPadsOpeningAngle" ;
    rdfs:subClassOf :CrushingFrictionCoefficientTighteningTableAttribute,
        :CrushingMaximumAllowableTighteningTableAttribute ;
    skos:definition "Defines the opening angle of the tensioner pads. This angle is crucial for determining how the pads make contact with the surface, affecting the distribution of force and the overall efficiency of the tightening process. Proper control of this angle ensures effective load application and surface protection during operation."@en ;
    skos:prefLabel "Tensioner Pads Opening Angle"@en,
        "Ângulo de Abertura das Sapatas do Tensionador"@pt-br ;
    :hasAttributeScope :TypeLevelAttribute ;
    :hasTypedValue :intValue ;
    :hasValueCardinality :singleValue .

:TensionerPadsShape a owl:DatatypeProperty ;
    dcterms:accessRights "PUBLIC" ;
    dcterms:identifier "TensionerPadsShape" ;
    rdfs:subClassOf :CrushingFrictionCoefficientTighteningTableAttribute,
        :CrushingMaximumAllowableTighteningTableAttribute ;
    skos:definition "Specifies the geometric shape of the tensioner pads. The shape affects the contact area, frictional performance, and overall effectiveness of the tightening process, influencing how forces are applied and distributed."@en,
        "Disposição geométrica da sapata (Por exemplo \"V\")"@pt-br ;
    skos:prefLabel "Tensioner Pads Shape"@en,
        "Forma das Sapatas do Tensionador"@pt-br ;
    :hasAttributeScope :TypeLevelAttribute ;
    :hasTypedValue :stringValue ;
    :hasValueCardinality :singleValue .

:TensionerTracksQuantity a owl:DatatypeProperty ;
    dcterms:accessRights "PUBLIC" ;
    dcterms:identifier "TensionerTracksQuantity" ;
    rdfs:subClassOf :CrushingFrictionCoefficientTighteningTableAttribute,
        :CrushingMaximumAllowableTighteningTableAttribute ;
    skos:definition "Indicates the quantity of tensioner tracks. This value is important for understanding the distribution of tightening forces and how evenly the load is applied across the structure during the tightening process."@en,
        "Quantidade de lagartas do tensionador (Por exemplo, 4)"@pt-br ;
    skos:prefLabel "Tensioner Tracks Quantity"@en,
        "Quantidade de Lagartas do Tensionador"@pt-br ;
    :hasAttributeScope :TypeLevelAttribute ;
    :hasTypedValue :intValue ;
    :hasValueCardinality :singleValue .

:TestConditions a owl:DatatypeProperty ;
    dcterms:accessRights "PUBLIC" ;
    dcterms:identifier "TestConditions" ;
    rdfs:subClassOf :BendingStiffnessAttribute,
        :CrushingFrictionCoefficientTighteningTableAttribute,
        :CrushingMaximumAllowableTensionTableAttribute,
        :CrushingMaximumAllowableTighteningTableAttribute,
        :LayingMinimumRadiusTableAttribute ;
    skos:definition "Specifies unstructured complementary information regarding the conditions under which a test is performed. This property may include additional details such as temperature, pressure, load, or other factors that could influence the test results, providing context for accurate interpretation of performance assessments."@en,
        "Descrição completa das condições para a execução do ensaio"@pt-br ;
    skos:prefLabel "Test Conditions"@en,
        "Condições de Teste"@pt-br ;
    :hasAttributeScope :TypeLevelAttribute ;
    :hasTypedValue :stringValue ;
    :hasValueCardinality :singleValue .

:TestEquipment a owl:Class ;
    dcterms:identifier "TestEquipment" ;
    rdfs:subClassOf :SurfaceEquipment .

:ThermalConductivityCoefficient a owl:DatatypeProperty ;
    dcterms:accessRights "PUBLIC" ;
    dcterms:identifier "ThermalConductivityCoefficient" ;
    rdfs:subPropertyOf :DomainAttribute ;
    skos:definition "Indicates the material's ability to conduct heat, measured as the rate at which heat passes through the material under a temperature gradient. This property is important for assessing how the material handles heat transfer in subsea environments, ensuring it can maintain performance under varying thermal conditions."@en,
        "Coeficiente de Condutividade Térmica do material (Obs. Para materiais compósitos, indicar o coefitiente no sentido longitudinal das fibras)"@pt-br ;
    skos:prefLabel "Thermal Conductivity Coefficient"@en,
        "Coeficiente de Condutividade Térmica"@pt-br ;
    :hasAttributeScope :TypeLevelAttribute ;
    :hasTypedValue :floatValue ;
    :hasValueCardinality :singleValue .

:ThermalExchangeCoefficientFlooded a owl:DatatypeProperty ;
    dcterms:accessRights "PUBLIC" ;
    dcterms:identifier "ThermalExchangeCoefficientFlooded" ;
    rdfs:subPropertyOf :DomainAttribute ;
    skos:definition "Indicates the rate at which heat is transferred through a material or component in flooded conditions. This property is essential for assessing the material's thermal performance, influencing its ability to manage heat effectively in operational scenarios where it is exposed to fluid filling."@en,
        "Coeficiente de troca térmica na temperatura máxima de projeto no interior, na temperatura da profundidade máxima especificada da água no exterior, com os anulares de isolamento e das armadura de tração alagados, no final da vida útil."@pt-br ;
    skos:prefLabel "Thermal Exchange Coefficient Flooded"@en,
        "Coeficiente de Troca Térmica em Condição Alagada"@pt-br ;
    :hasAttributeScope :TypeLevelAttribute ;
    :hasTypedValue :floatValue ;
    :hasValueCardinality :singleValue .

:Timestamp a owl:DatatypeProperty ;
    dcterms:accessRights "PUBLIC" ;
    dcterms:identifier "Timestamp" ;
    rdfs:subClassOf :JustificationAttribute,
        :Registry_GUIDAttribute,
        :StatusAttribute ;
    skos:definition "Exact date and time, providing a precise reference for tracking when an event or action occurred within the system."@en ;
    skos:prefLabel "Timestamp"@en ;
    :hasAttributeScope :InstanceLevelAttribute ;
    :hasTypedValue :dateTimeValue ;
    :hasValueCardinality :singleValue .

:UltTensStrAlongFibers a owl:DatatypeProperty ;
    dcterms:accessRights "PUBLIC" ;
    dcterms:identifier "UltTensStrAlongFibers" ;
    rdfs:subPropertyOf :DomainAttribute ;
    skos:definition "Indicates the maximum tensile stress a material can withstand along the direction of its fibers before breaking. This property is crucial for assessing the strength of fiber-reinforced materials, ensuring they can handle tensile loads effectively in the direction of fiber alignment."@en ;
    skos:prefLabel "Ultimate Tensile Strength Along Fibers"@en,
        "Tensão máxima de tração longitudinalmente às fibras"@pt-br ;
    :hasAttributeScope :TypeLevelAttribute ;
    :hasTypedValue :floatValue ;
    :hasValueCardinality :singleValue .

:UltTensStrPerpendFibers a owl:DatatypeProperty ;
    dcterms:accessRights "PUBLIC" ;
    dcterms:identifier "UltTensStrPerpendFibers" ;
    rdfs:subPropertyOf :DomainAttribute ;
    skos:definition "Indicates the maximum tensile stress a material can withstand when applied perpendicular to the direction of its fibers before breaking. This property is important for evaluating the strength and durability of fiber-reinforced materials under tensile loads that are not aligned with the fibers, providing insights into their performance in various loading conditions."@en ;
    skos:prefLabel "Ultimate Tensile Strength Perpendicular To Fibers"@en,
        "Tensão máxima de tração perpendicularmente às fibras"@pt-br ;
    :hasAttributeScope :TypeLevelAttribute ;
    :hasTypedValue :floatValue ;
    :hasValueCardinality :singleValue .

:UltimateTensileStress a owl:DatatypeProperty ;
    dcterms:accessRights "PUBLIC" ;
    dcterms:identifier "UltimateTensileStress" ;
    rdfs:subPropertyOf :DomainAttribute ;
    skos:definition "Indicates the maximum stress a material can withstand while being stretched or pulled before breaking. This property is essential for evaluating the material's strength and determining its ability to perform under tensile loads without failure."@en,
        "Tensão máxima de tração (Específica para Materiais Metálicos)"@pt-br ;
    skos:prefLabel "Ultimate Tensile Stress"@en,
        "Tensão Máxima de Tração"@pt-br ;
    :hasAttributeScope :TypeLevelAttribute ;
    :hasTypedValue :floatValue ;
    :hasValueCardinality :singleValue .

:UnifilarDiagram a owl:DatatypeProperty ;
    dcterms:accessRights "PUBLIC" ;
    dcterms:identifier "UnifilarDiagram" ;
    rdfs:subPropertyOf :DomainAttribute ;
    skos:definition "A simplified schematic illustrates the arrangement of flexible pipeline sections and their associated accessories, such as end fittings and clamps. This diagram shows how these sections and accessories are connected, providing a clear overview of the pipeline configuration without detailing internal structures. It is used to aid in planning, installation, and understanding of the flexible pipeline system by visualizing the main components and their positions."@en ;
    skos:prefLabel "Unifilar Diagram"@en,
        "Código do Diagrama Unifilar"@pt-br ;
    :hasAttributeScope :InstanceLevelAttribute ;
    :hasTypedValue :stringValue ;
    :hasValueCardinality :singleValue .

:UnifilarDiagramRev a owl:DatatypeProperty ;
    dcterms:accessRights "PUBLIC" ;
    dcterms:identifier "UnifilarDiagramRev" ;
    rdfs:subPropertyOf :DomainAttribute ;
    skos:definition "Indicates the revision number of the unifilar diagram, reflecting updates or changes made to the arrangement of pipeline sections and their accessories. Each revision ensures that the latest configuration is accurately documented for installation and planning purposes."@en ;
    skos:prefLabel "Unifilar Diagram Revision"@en,
        "Número da Revisão do Diagrama Unifilar"@pt-br ;
    :hasAttributeScope :InstanceLevelAttribute ;
    :hasTypedValue :stringValue ;
    :hasValueCardinality :singleValue .

:UpperItubeDiameter a owl:DatatypeProperty ;
    dcterms:accessRights "PUBLIC" ;
    dcterms:identifier "UpperItubeDiameter" ;
    rdfs:subPropertyOf :DomainAttribute ;
    skos:definition "Diameter of the upper section of the tube or pipe. This measurement is important for ensuring proper fit and compatibility with other components or connections. The diameter of the upper section affects the alignment and sealing capabilities of the assembly, and ensures that the tube or pipe meets the design and operational requirements for the installation or application."@en ;
    skos:prefLabel "Upper I-tube Diameter"@en,
        "Diâmetro do I-TUBE superior"@pt-br ;
    :hasAttributeScope :TypeLevelAttribute ;
    :hasTypedValue :floatValue ;
    :hasValueCardinality :singleValue .

:UtilizationFactor a owl:DatatypeProperty ;
    dcterms:accessRights "PUBLIC" ;
    dcterms:identifier "UtilizationFactor" ;
    rdfs:subClassOf :CrushingFrictionCoefficientTighteningTableAttribute,
        :CrushingMaximumAllowableTensionTableAttribute,
        :CrushingMaximumAllowableTighteningTableAttribute ;
    skos:definition "Represents the ratio used to determine the level of utilisation, indicating how much of the system’s capacity is being used under given conditions. This factor is crucial for assessing whether the structure operates within safe limits or approaching its maximum capacity."@en ;
    skos:prefLabel "Utilization Factor"@en,
        "Fator de Utilização"@pt-br ;
    :hasAttributeScope :TypeLevelAttribute ;
    :hasTypedValue :floatValue ;
    :hasValueCardinality :singleValue .

:Vessel a owl:Class ;
    dcterms:identifier "Vessel" ;
    rdfs:subClassOf :PressureComponent .

:WireLayer a owl:Class ;
    dcterms:identifier "WireLayer" ;
    rdfs:subClassOf :ArmourLayer ;
    skos:definition "Basis for all wired layers."@en ;
    skos:prefLabel "Wire Layer"@en,
        "Camada de Arame"@pt-br .

:WireRopeQuantity a owl:DatatypeProperty ;
    dcterms:accessRights "PUBLIC" ;
    dcterms:identifier "WireRopeQuantity" ;
    rdfs:subPropertyOf :DomainAttribute ;
    skos:definition "Indicates the number of wire ropes required or used for installation or operation"@en ;
    skos:prefLabel "Wire Rope Quantity"@en,
        "Quantidade de cordas de Aço"@pt-br ;
    :hasAttributeScope :TypeLevelAttribute ;
    :hasTypedValue :intValue ;
    :hasValueCardinality :singleValue .

:WireRopeSlingDiameter a owl:DatatypeProperty ;
    dcterms:accessRights "PUBLIC" ;
    dcterms:identifier "WireRopeSlingDiameter" ;
    rdfs:subPropertyOf :DomainAttribute ;
    skos:definition "Specifies the diameter of the wire rope sling. This property provides the measurement of the thickness of the wire rope, which is important for determining its strength and load-bearing capacity."@en,
        "Diâmetro do Estrobo de Corda de Aço"@pt-br ;
    skos:prefLabel "Wire Rope Sling Diameter"@en,
        "Diâmetro do Estrobo de Corda de Aço"@pt-br ;
    :hasAttributeScope :TypeLevelAttribute ;
    :hasTypedValue :floatValue ;
    :hasValueCardinality :singleValue .

:WireRopeSlingLength a owl:DatatypeProperty ;
    dcterms:accessRights "PUBLIC" ;
    dcterms:identifier "WireRopeSlingLength" ;
    rdfs:subPropertyOf :DomainAttribute ;
    skos:definition "Specifies the length of the wire rope sling used in the installation or operation. This property provides the measurement of the sling’s length, which is essential for ensuring proper fit and functionality during use."@en ;
    skos:prefLabel "Wire Rope Sling Length"@en,
        "Comprimento do Estrobo da Corda de Aço"@pt-br ;
    :hasAttributeScope :TypeLevelAttribute ;
    :hasTypedValue :floatValue ;
    :hasValueCardinality :singleValue .

:WorkingLoadLimit a owl:DatatypeProperty ;
    dcterms:accessRights "PUBLIC" ;
    dcterms:identifier "WorkingLoadLimit" ;
    rdfs:subPropertyOf :DomainAttribute ;
    skos:definition "The Working Load Limit (WLL) refers to the maximum load that a component, such as a shackle, lifting device, or anchor, is designed to safely support under normal operating conditions."@en ;
    skos:prefLabel "Working Load Limit (WLL)"@en,
        "Limite de Carga de Trabalho"@pt-br ;
    :hasAttributeScope :InstanceLevelAttribute ;
    :hasTypedValue :floatValue ;
    :hasValueCardinality :singleValue .

:ActuatedEquipment a owl:Class ;
    dcterms:identifier "ActuatedEquipment" ;
    rdfs:subClassOf :SubseaEquipment .

:ActuatedValve a owl:Class ;
    dcterms:identifier "ActuatedValve" ;
    rdfs:subClassOf :Valve .

:Anchor a owl:Class ;
    dcterms:identifier "Anchor" ;
    rdfs:subClassOf :Structure .

:ArmourLayer a owl:Class ;
    dcterms:identifier "ArmourLayer" ;
    rdfs:subClassOf :WoundLayer ;
    skos:definition "A reinforcement layer in subsea flexible pipes used in oil and gas exploration, designed to provide mechanical strength and protection against external forces, such as pressure and movement. It ensures structural integrity by preventing deformation and failure during operation. Typically made from high-strength metal wires, like carbon steel or stainless steel, the Armor Layer enhances the pipe's durability in harsh underwater conditions."@en ;
    skos:prefLabel "Armour Layer"@en,
        "Camada de Armadura"@pt-br .

:AssemblyTorque a owl:DatatypeProperty ;
    dcterms:accessRights "PUBLIC" ;
    dcterms:identifier "AssemblyTorque" ;
    rdfs:subPropertyOf :DomainAttribute ;
    skos:definition "Specifies the torque applied during assembly, ensuring proper tightening for secure connections. This value is critical for maintaining the structural integrity and reliability of the connection under operational loads."@en ;
    skos:prefLabel "Assembly Torque"@en,
        "Torque de montagem"@pt-br ;
    :hasAttributeScope :InstanceLevelAttribute ;
    :hasTypedValue :floatValue ;
    :hasValueCardinality :singleValue .

:Asset a owl:Class ;
    dcterms:identifier "Asset" ;
    rdfs:subClassOf :DomainElement ;
    skos:definition "An asset refers to valuable resources such as platforms, equipment, pipelines, and processing facilities crucial for production and transportation. These assets are managed to optimize performance, ensure safety, and maximize operational efficiency throughout their lifecycle."@en ;
    skos:prefLabel "Asset"@en,
        "Ativo"@pt-br ;
    :hasAttribute :IsSpare,
        :SerialNumber .

:BendMomentVsShearForceAttribute a owl:Class ;
    rdfs:label "Bending Moment Versus Shear Force Attribute"@en ;
    rdfs:subPropertyOf :DomainAttribute .

:BendMomentVsShearForceTableColumn a owl:Class ;
    dcterms:accessRights "PUBLIC" ;
    dcterms:identifier "BendMomentVsShearForceTable" ;
    rdfs:subClassOf :BendMomentVsShearForceAttribute ;
    skos:definition "Provides data on the relationship between bending moment and shear force, used to evaluate how the structure behaves under combined loading conditions. This information is critical for determining the structural integrity and performance under different operational stresses."@en ;
    skos:prefLabel "Bending moment vs Shear Force Table"@en,
        "Tabela de Momento de Curvatura em Função da Força Cisalhante"@pt-br ;
    :hasAttributeScope :TypeLevelAttribute .

:BendStiffener a owl:Class ;
    dcterms:identifier "BendStiffener" ;
    rdfs:subClassOf :LineAncillary ;
    skos:definition "Device used in subsea flexible pipes to provide gradual stiffness transition between the flexible pipe and a fixed structure, preventing excessive bending at critical areas such as terminations or connectors. The Bend Stiffener is designed to manage stress concentration by stiffening the pipe over a defined length, reducing the risk of damage due to repeated bending, fatigue, or over-flexing. Typically made from high-strength materials, it ensures the long-term structural integrity of the pipe in dynamic subsea environments."@en ;
    skos:prefLabel "Bend Stiffener"@en,
        "Enrijecedor de Curvatura"@pt-br .

:BendingStiffnessTableColumn a owl:Class ;
    rdfs:subClassOf :BendingStiffnessAttribute .

:BoltSet a owl:Class ;
    dcterms:identifier "BoltSet" ;
    rdfs:subClassOf :PhysicalConnection ;
    skos:definition "A collection of bolts and nuts, and washers designed for fastening components in subsea systems. Bolt sets are critical for ensuring structural integrity and are selected based on size, material, and application requirements."@en ;
    skos:prefLabel "Bolt Set"@en,
        "Conjunto de Parafusos"@pt-br ;
    :hasAttribute :AssemblyTorque,
        :FullyThreaded,
        :Lubricant,
        :LubricantFrictionFactor,
        :NominalLength,
        :Quantity,
        :SpareQuantity .

:CarcassLayer a owl:Class ;
    dcterms:identifier "CarcassLayer" ;
    rdfs:subClassOf :ArmourLayer ;
    skos:definition "A reinforcement layer in subsea flexible pipes that provides structural strength and stability. It helps maintain the shape and integrity of the pipe under operational pressure, ensuring the flexibility of the pipe while protecting the internal components. Typically made from metal or polymer materials, it acts as a foundation for the other protective layers."@en ;
    skos:prefLabel "Carcass Layer"@en,
        "Camada de Carcaça"@pt-br ;
    :hasAttribute :MetallicLayerPitch,
        :StressAtDesignPressure .

:Connection a owl:Class ;
    dcterms:identifier "Connection" ;
    rdfs:subClassOf :DomainElement ;
    skos:definition "The joining point between two components, enabling fluid, gas, or structural continuity. Connections are designed to ensure secure, leak-free operation in harsh subsea environments."@en ;
    skos:prefLabel "Connection"@en,
        "Conexão"@pt-br .

:ConnectionModule a owl:Class ;
    dcterms:identifier "ConnectionModule" ;
    rdfs:subClassOf :LineTerminationModule .

:CrushingFrictionCoefficientTighteningTableColumn a owl:Class ;
    rdfs:subClassOf :CrushingFrictionCoefficientTighteningTableAttribute .

:CrushingMaximumAllowableTighteningTableColumn a owl:Class ;
    rdfs:subClassOf :CrushingMaximumAllowableTighteningTableAttribute .

:DomainAuxiliarClass a owl:Class .

:DomainClassification a owl:Class .

:EarlyLeakMaxPressTableAttribute a owl:Class ;
    rdfs:subClassOf :HydrostaticPressureTestsAttribute .

:EarlyLeakNomPressTableAttribute a owl:Class ;
    rdfs:subClassOf :HydrostaticPressureTestsAttribute .

:Equipment a owl:Class ;
    dcterms:identifier "Equipment" ;
    rdfs:subClassOf :CompactObject .

:FlangeAttribute a owl:Class ;
    rdfs:label "Flange Attribute"@en ;
    rdfs:subPropertyOf :DomainAttribute .

:FlexibleStructureLayer a owl:Class ;
    dcterms:identifier "FlexibleStructureLayer" ;
    rdfs:subClassOf :DomainElement ;
    skos:definition "A specific layer within the structure of a subsea flexible pipe, each designed to fulfill a distinct function. These layers work together to provide essential properties such as pressure containment, reinforcement, and environmental protection. Engineered to withstand harsh underwater conditions, each layer contributes to the overall flexibility, durability, and performance of the subsea flexible pipe system."@en ;
    skos:prefLabel "Flexible Structure Layer"@en,
        "Camadas de Estruturas Flexíveis"@pt-br ;
    :hasAttribute :InternalDiameter,
        :LayerAnnular,
        :LayerAnnularType,
        :LayerContinuity,
        :LayerGeometryCrossSection,
        :LayerGeometryInertiaX,
        :LayerGeometryInertiaY,
        :LayerGeometryManufacturer,
        :LayerGeometryName,
        :LayerGeometryProfileThickness,
        :LayerGeometryProfileWidth,
        :LayerGeometryThickness,
        :LayerThickness,
        :LayerWatertight,
        :LayerWatertightLowerLayerInternalFreeVolume,
        :LinearMass .

:FullyThreaded a owl:DatatypeProperty ;
    dcterms:accessRights "PUBLIC" ;
    dcterms:identifier "FullyThreaded" ;
    rdfs:subPropertyOf :DomainAttribute ;
    skos:definition "Indicates whether the component will be used fully threaded (TRUE) or not (FALSE)."@en ;
    skos:prefLabel "Fully Threaded"@en,
        "Completamente Rosqueado"@pt-br ;
    :hasAttributeScope :InstanceLevelAttribute ;
    :hasTypedValue :booleanValue ;
    :hasValueCardinality :singleValue .

:IdInUnifilarDiagram a owl:DatatypeProperty ;
    dcterms:accessRights "PUBLIC" ;
    dcterms:identifier "IdInUnifilarDiagram" ;
    rdfs:subPropertyOf :DomainAttribute ;
    skos:definition "Numeric identifier used to represent the component in a unifilar diagram, ensuring clear reference and traceability within the diagram. This identifier allows for easy identification of the component's position and connection points in the simplified representation of the system."@en,
        "Identificador do item no diagrama unifilar (unifilar \"classico\", pre-existente) conforme a coluna \"item\" do unifilar."@pt-br ;
    skos:prefLabel "Id In Unifilar Diagram"@en,
        "Identificador no Diagrama Unifilar"@pt-br ;
    :hasAttributeScope :InstanceLevelAttribute,
        :TypeLevelAttribute ;
    :hasTypedValue :intValue ;
    :hasValueCardinality :singleValue .

:Interconnection a owl:Class ;
    dcterms:identifier "Interconnection" ;
    rdfs:subClassOf :LinearLocation ;
    skos:definition "Location that contains the entire length of an interconnection, with its various sections, terminations, inline equipment, etc."@en ;
    skos:prefLabel "Interconnection"@en,
        "Interligação"@pt-br .

:LineSpan a owl:Class ;
    dcterms:identifier "LineSpan" ;
    rdfs:subClassOf :Location .

:LineTermination a owl:Class ;
    dcterms:identifier "LineTermination" ;
    rdfs:subClassOf :ComponentDevice ;
    skos:definition "The Line Termination includes components at the endpoints of flexible and rigid pipelines, as well as umbilical systems. These terminations provide secure connections to other equipment, enabling the transfer of fluids, gases, or control signals. Designed for stability and integrity, Line Termination components ensure durable and reliable performance across various pipeline types."@en ;
    skos:prefLabel "Line Termination"@en,
        "Terminador de Linha"@pt-br .

:LineTerminationModule a owl:Class ;
    dcterms:identifier "LineTerminationModule" ;
    rdfs:subClassOf :TieInEquipment .

:LinearMass a owl:DatatypeProperty ;
    dcterms:accessRights "PUBLIC" ;
    dcterms:identifier "LinearMass" ;
    rdfs:subPropertyOf :DomainAttribute ;
    skos:definition "Indicates the mass per unit length, providing essential information for weight distribution and load calculations. This value is critical for evaluating how the structure will perform under various operational conditions, including installation and transport."@en ;
    skos:prefLabel "Linear Mass"@en,
        "Massa Linear"@pt-br ;
    :hasAttributeScope :InstanceLevelAttribute,
        :TypeLevelAttribute ;
    :hasTypedValue :floatValue ;
    :hasValueCardinality :singleValue .

:LocationType a owl:Class ;
    rdfs:label "Location Type"@en,
        "Tipo de Localização"@pt-br ;
    rdfs:subClassOf :ElementClassification ;
    skos:definition "Classification of industrial activities based on their geographical location."@en,
        "Classificação de atividades industriais baseada em sua localização geográfica."@pt-br .

:Lubricant a owl:DatatypeProperty ;
    dcterms:accessRights "PUBLIC" ;
    dcterms:identifier "Lubricant" ;
    rdfs:subPropertyOf :DomainAttribute ;
    skos:definition "Specifies the type of lubricant applied to reduce friction during tightening and ensure consistent torque application. The use of the correct lubricant is critical in preventing galling and corrosion, and helps to maintain the long-term integrity."@en ;
    skos:prefLabel "Lubricant"@en,
        "Nome do Lubrificante"@pt-br ;
    :hasAttributeScope :InstanceLevelAttribute ;
    :hasTypedValue :stringValue ;
    :hasValueCardinality :singleValue .

:LubricantFrictionFactor a owl:DatatypeProperty ;
    dcterms:accessRights "PUBLIC" ;
    dcterms:identifier "LubricantFrictionFactor" ;
    rdfs:subPropertyOf :DomainAttribute ;
    skos:definition "Indicates the friction factor of the lubricant applied, which affects the torque required to achieve proper tightening. This value is crucial for ensuring that the correct amount of torque is applied, accounting for the reduction in friction caused by the lubricant."@en ;
    skos:prefLabel "Lubricant Friction Factor"@en,
        "Fator de atrito do lubrificante"@pt-br ;
    :hasAttributeScope :InstanceLevelAttribute ;
    :hasTypedValue :floatValue ;
    :hasValueCardinality :singleValue .

:Nuclear a owl:Class ;
    rdfs:label "Nuclear Energy"@en,
        "Energia Nuclear"@pt-br ;
    rdfs:subClassOf :Domain ;
    skos:definition "Industrial domain covering the generation of energy from nuclear reactions, including fission and fusion."@en,
        "Domínio industrial que abrange a geração de energia a partir de reações nucleares, incluindo fissão e fusão."@pt-br .

:Pile a owl:Class ;
    dcterms:identifier "Pile" ;
    rdfs:subClassOf :Anchor .

:PipeMountPosition a owl:DatatypeProperty ;
    dcterms:accessRights "PUBLIC" ;
    dcterms:identifier "PipeMountPosition" ;
    rdfs:subPropertyOf :DomainAttribute ;
    skos:definition "Indicates the distance from the end fitting to the position of the accessory along the direction of fluid flow within the pipe body. This property specifies the precise location of the accessory relative to the end fitting, which is essential for accurate installation and alignment within the tubular body."@en,
        "Cota em metros da posição em que o item é montado no tramo no sentido do fluxo do fluido."@pt-br ;
    skos:prefLabel "Pipe Mount Position"@en,
        "Posição de Montagem no Duto"@pt-br ;
    :hasAttributeScope :InstanceLevelAttribute ;
    :hasTypedValue :floatValue ;
    :hasValueCardinality :singleValue .

:PipelineSpan a owl:Class ;
    dcterms:identifier "PipelineSpan" ;
    rdfs:subClassOf :LineSpan .

:PressureEquipment a owl:Class ;
    dcterms:identifier "PressureEquipment" ;
    rdfs:subClassOf :ActuatedEquipment .

:Quantity a owl:DatatypeProperty ;
    dcterms:accessRights "PUBLIC" ;
    dcterms:identifier "Quantity" ;
    rdfs:subPropertyOf :DomainAttribute ;
    skos:definition "Quantity of items."@en ;
    skos:prefLabel "Quantity"@en,
        "Quantidade de Itens"@pt-br ;
    :hasAttributeScope :InstanceLevelAttribute ;
    :hasTypedValue :intValue ;
    :hasValueCardinality :singleValue .

:RingGasketMaterial a owl:DatatypeProperty ;
    dcterms:accessRights "PUBLIC" ;
    dcterms:identifier "RingGasketMaterial" ;
    rdfs:subClassOf :RingGasketAttribute ;
    skos:definition "Type of material from which an object is made, allowing for precise documentation and categorisation."@en ;
    skos:prefLabel "Ring Gasket Material"@en,
        "Material da Junta de Vedação"@pt-br ;
    :hasAttributeScope :InstanceLevelAttribute,
        :TypeLevelAttribute ;
    :hasTypedValue :stringValue ;
    :hasValueCardinality :singleValue .

:RiserSupport a owl:Class ;
    dcterms:identifier "RiserSupport" ;
    rdfs:subClassOf :Component .

:RopeSegment a owl:Class ;
    dcterms:identifier "RopeSegment" ;
    rdfs:subClassOf :LinearObject .

:SpareQuantity a owl:DatatypeProperty ;
    dcterms:accessRights "PUBLIC" ;
    dcterms:identifier "SpareQuantity" ;
    rdfs:subPropertyOf :DomainAttribute ;
    skos:definition "Specifies the number of spare units available, ensuring adequate backup components are on hand for maintenance or replacement. This quantity helps in planning and minimizing downtime during operations."@en ;
    skos:prefLabel "Spare Quantity"@en,
        "Quantidade de Sobressalentes"@pt-br ;
    :hasAttributeScope :InstanceLevelAttribute ;
    :hasTypedValue :intValue ;
    :hasValueCardinality :singleValue .

:StressAtDesignPressure a owl:DatatypeProperty ;
    dcterms:accessRights "PUBLIC" ;
    dcterms:identifier "StressAtDesignPressure" ;
    rdfs:subPropertyOf :DomainAttribute ;
    skos:definition "Maximum stress that the material can withstand when subjected to design pressure is specified. This parameter is critical for ensuring that the material maintains its structural integrity and performs reliably under the operational pressure conditions specified in the design."@en ;
    skos:prefLabel "Stress At Design Pressure"@en,
        "Tensão na pressão de projeto"@pt-br ;
    :hasAttributeScope :InstanceLevelAttribute ;
    :hasTypedValue :floatValue ;
    :hasValueCardinality :singleValue .

:StudSet a owl:Class ;
    dcterms:identifier "StudSet" ;
    rdfs:subClassOf :PhysicalConnection ;
    skos:altLabel "Stud"@en,
        "Threaded Rod"@en ;
    skos:definition "Stud sets are essential fastening components used in subsea oil and gas interconnection end fittings to securely assemble and connect various parts of the equipment. Each set typically includes bolts, nuts, and washers, all made from high-strength, corrosion-resistant materials to endure the harsh subsea environment. These components are designed to provide reliable mechanical fastening, ensuring the structural integrity and leak-proof performance of the end fittings. The stud sets are carefully engineered to withstand high pressure and extreme temperatures, making them critical for maintaining the operational safety and longevity of subsea interconnections."@en ;
    skos:prefLabel "Stud Set"@en,
        "Estojos"@pt-br ;
    :hasAttribute :AssemblyTorque,
        :FullyThreaded,
        :Lubricant,
        :LubricantFrictionFactor,
        :NominalDiameter,
        :Quantity,
        :SpareQuantity .

:SurfaceEquipment a owl:Class ;
    dcterms:identifier "SurfaceEquipment" ;
    rdfs:subClassOf :Equipment .

:TapesQuantity a owl:DatatypeProperty ;
    dcterms:accessRights "PUBLIC" ;
    dcterms:identifier "TapesQuantity" ;
    rdfs:subPropertyOf :DomainAttribute ;
    skos:definition "Number of tapes applied within the structure, influencing factors such as insulation, protection, and reinforcement. "@en ;
    skos:prefLabel "Tapes Quantity"@en,
        "Quantidade de fitas"@pt-br ;
    :hasAttributeScope :InstanceLevelAttribute ;
    :hasTypedValue :intValue ;
    :hasValueCardinality :singleValue .

:TechnicalNotes a owl:DatatypeProperty ;
    dcterms:accessRights "PUBLIC" ;
    dcterms:identifier "TechnicalNotes" ;
    rdfs:subPropertyOf :DomainAttribute ;
    skos:definition "A field used to provide additional technical information or clarifications that may not be covered by other specific properties, to support a comprehensive understanding of the material’s behavior and suitability."@en ;
    skos:prefLabel "Technical Notes"@en,
        "Notas Técnicas"@pt-br ;
    :hasAttributeScope :InstanceLevelAttribute,
        :TypeLevelAttribute ;
    :hasTypedValue :stringValue ;
    :hasValueCardinality :singleValue .

:ThreadPitch a owl:DatatypeProperty ;
    dcterms:accessRights "PUBLIC" ;
    dcterms:identifier "ThreadPitch" ;
    rdfs:subPropertyOf :DomainAttribute ;
    skos:definition "The distance between adjacent thread crests, measured along the thread's axis, determining the threading's fineness or coarseness."@en ;
    skos:prefLabel "Thread Pitch"@en,
        "Passo da Rosca"@pt-br ;
    :hasAttributeScope :InstanceLevelAttribute ;
    :hasTypedValue :floatValue ;
    :hasValueCardinality :singleValue .

:ThreadsPerInch a owl:DatatypeProperty ;
    dcterms:accessRights "PUBLIC" ;
    dcterms:identifier "ThreadsPerInch" ;
    rdfs:subPropertyOf :DomainAttribute ;
    skos:definition "Threads per Inch. Indicates the number of threads present in one inch of the bolt"@en ;
    skos:prefLabel "Threads Per Inch"@en,
        "Fios por Polegada"@pt-br ;
    :hasAttributeScope :InstanceLevelAttribute ;
    :hasTypedValue :floatValue ;
    :hasValueCardinality :singleValue .

:TransportLineSegment a owl:Class ;
    dcterms:identifier "TransportLineSegment" ;
    rdfs:subClassOf :LinearObject ;
    skos:definition "Line for conducting some type of flow."@en ;
    skos:prefLabel "Transport Line Segment"@en,
        "Segmento de Linha de Transporte"@pt-br .

:UmbilicalComponent a owl:Class ;
    dcterms:identifier "UmbilicalComponent" ;
    rdfs:subClassOf :DomainElement .

:UmbilicalSpan a owl:Class ;
    dcterms:identifier "UmbilicalSpan" ;
    rdfs:subClassOf :LineSpan .

:ValueCardinality a owl:Class ;
    rdfs:label "Value Cardinality"@en ;
    rdfs:comment "Superclass for constraints on the cardinality of values (single or multiple)."@en ;
    rdfs:subClassOf :DomainAuxiliarClass .

:Valve a owl:Class ;
    dcterms:identifier "Valve" ;
    rdfs:subClassOf :PressureComponent .

:WoundLayer a owl:Class ;
    dcterms:identifier "WoundLayer" ;
    rdfs:subClassOf :FlexibleStructureLayer ;
    skos:definition "Basis for all layers constructed by helical winding of one or more elements."@en ;
    skos:prefLabel "Wound Layer"@en,
        "Camada Espiralada"@pt-br .

:dateTimeValue a owl:Class ;
    rdfs:label "DateTime Value"@en ;
    rdfs:comment "Constraint for xsd:dateTime (timestamps)"@en ;
    rdfs:subClassOf :TypedValue ;
    owl:equivalentClass [ a owl:Restriction ;
            owl:allValuesFrom xsd:dateTime ;
            owl:onProperty rdf:value ] .

:AttributeScope a owl:Class ;
    rdfs:label "Attribute Scope"@en,
        "Escopo do Atributo"@pt-br ;
    rdfs:comment "Defines whether the attribute applies to all instances of a type or to a specific instance."@en ;
    rdfs:subClassOf :AttributeClassification ;
    skos:definition "Defines whether the attribute applies to all instances of a type or to a specific instance"@en,
        "Define se o atributo se aplica a todas as instâncias de um tipo ou a uma instância específica"@pt-br .

:CrushingMaximumAllowableTensionTableColumn a owl:Class ;
    rdfs:subClassOf :CrushingMaximumAllowableTensionTableAttribute .

:DomainAnnotation a owl:AnnotationProperty .

:ElectronicDevice a owl:Class ;
    dcterms:identifier "ElectronicDevice" ;
    rdfs:subClassOf :ComponentDevice .

:ElementClassification a owl:Class ;
    rdfs:subClassOf :DomainClassification .

:EquipmentEngineering a owl:Class ;
    rdfs:label "Equipment Engineering"@en,
        "Engenharia de Equipamentos"@pt-br ;
    rdfs:subClassOf :TechnicalDiscipline ;
    skos:definition "Engineering discipline focused on the design and specification of industrial equipment."@en,
        "Disciplina de engenharia focada no projeto e especificação de equipamentos industriais."@pt-br .

:FlangeType a owl:DatatypeProperty ;
    dcterms:accessRights "PUBLIC" ;
    dcterms:identifier "FlangeType" ;
    rdfs:subClassOf :FlangeAttribute ;
    skos:definition "Specifies the type of flange within the Standard, which defines certain characteristics, like the Standard itself, Type or Class, Diameter and Operating Pressure."@en ;
    skos:prefLabel "Flange Type"@en,
        "Tipo de Flange"@pt-br ;
    :hasAttributeScope :TypeLevelAttribute ;
    :hasTypedValue :stringValue ;
    :hasValueCardinality :singleValue .

:FlexibleStructureLayerMaterial a owl:Class ;
    dcterms:identifier "FlexibleStructureLayerMaterial" ;
    rdfs:subClassOf :DomainElement ;
    skos:definition "Material used to fabricate the individual layers of a subsea flexible structure, each layer serving a distinct function such as pressure containment, tensile reinforcement, or external protection. The Flexible Structure Layer Material is selected based on its specific properties, such as strength, flexibility, corrosion resistance, or thermal insulation, to ensure the overall performance and durability of the flexible pipe in harsh subsea conditions. These materials may include polymers, metals, composites, or other high-performance substances tailored to the pipe's operational demands."@en ;
    skos:prefLabel "Flexible Structure Layer Material"@en,
        "Materiais de Camadas de Estruturas Flexíveis Submarinas"@pt-br ;
    :hasAttribute :ElasticityModulusAt23Degrees,
        :MaterialComposition,
        :PoissonRatioAt23Degrees,
        :SpecificHeatCapacity,
        :SpecificWeight,
        :TechnicalNotes,
        :ThermalConductivityCoefficient .

:FunctionLine a owl:Class ;
    dcterms:identifier "FunctionLine" ;
    rdfs:subClassOf :UmbilicalComponent .

:InternalDiameter a owl:DatatypeProperty ;
    dcterms:accessRights "PUBLIC" ;
    dcterms:identifier "InternalDiameter" ;
    rdfs:subPropertyOf :DomainAttribute ;
    skos:definition "Distance measured across the innermost points, passing through the center."@en ;
    skos:prefLabel "Internal Diameter"@en,
        "Diâmetro interno"@pt-br ;
    :hasAttributeScope :InstanceLevelAttribute,
        :TypeLevelAttribute ;
    :hasTypedValue :floatValue ;
    :hasValueCardinality :singleValue .

:Jumper a owl:Class ;
    dcterms:identifier "Jumper" ;
    rdfs:subClassOf :LinearObject .

:LayingMinimumRadiusTableAttribute a owl:Class ;
    rdfs:subPropertyOf :DomainAttribute .

:LogicalConnection a owl:Class ;
    dcterms:identifier "LogicalConnection" ;
    rdfs:subClassOf :Connection ;
    skos:definition "Represents a logical/functional connection between two installation locations."@en ;
    skos:prefLabel "Logical Connection"@en,
        "Conexão Lógica"@pt-br .

:MaterialManufacturerAttribute a owl:Class ;
    rdfs:label "Material Manufacturer"@en ;
    rdfs:subPropertyOf :DomainAttribute .

:NominalDiameter a owl:DatatypeProperty ;
    dcterms:accessRights "PUBLIC" ;
    dcterms:identifier "NominalDiameter" ;
    rdfs:subPropertyOf :DomainAttribute ;
    skos:definition "The standard diameter of the component or pipe, typically used for classification and specification purposes."@en ;
    skos:prefLabel "Nominal Diameter"@en,
        "Diâmetro Nominal"@pt-br ;
    :hasAttributeScope :InstanceLevelAttribute ;
    :hasTypedValue :stringValue ;
    :hasValueCardinality :singleValue .

:NominalLength a owl:DatatypeProperty ;
    dcterms:accessRights "PUBLIC" ;
    dcterms:identifier "NominalLength" ;
    rdfs:subPropertyOf :DomainAttribute ;
    skos:definition "Nominal length refers to the length of an object as designed, typically used as a reference value. It may not represent the exact physical measurement but serves as the standard or intended length for manufacturing, design, or specification purposes."@en ;
    skos:prefLabel "Nominal Length"@en,
        "Comprimento Nominal"@pt-br ;
    :hasAttributeScope :InstanceLevelAttribute ;
    :hasTypedValue :floatValue ;
    :hasValueCardinality :singleValue .

:OilAndGas a owl:Class ;
    rdfs:label "Oil & Gas"@en,
        "Petróleo & Gás"@pt-br ;
    rdfs:subClassOf :Domain ;
    skos:definition "Industrial domain covering all activities related to the exploration, production, refining, and distribution of oil and gas."@en,
        "Domínio industrial que abrange todas as atividades relacionadas à exploração, produção, refino e distribuição de petróleo e gás."@pt-br .

:PipeSupport a owl:Class ;
    dcterms:identifier "PipeSupport" ;
    rdfs:subClassOf :Structure .

:RingGasketInnerDIameter a owl:DatatypeProperty ;
    dcterms:accessRights "PUBLIC" ;
    dcterms:identifier "RingGasketInnerDIameter" ;
    rdfs:subClassOf :RingGasketAttribute ;
    skos:definition "The internal diameter, which determines the size of the bore it fits into. This dimension is crucial for ensuring a proper fit and effective sealing."@en ;
    skos:prefLabel "Ring Gasket Inner Diameter"@en,
        "Diâmetro Interno da Junta de Vedação"@pt-br ;
    :hasAttributeScope :InstanceLevelAttribute,
        :TypeLevelAttribute ;
    :hasTypedValue :floatValue ;
    :hasValueCardinality :singleValue .

:RingGasketOuterDiameter a owl:DatatypeProperty ;
    dcterms:accessRights "PUBLIC" ;
    dcterms:identifier "RingGasketOuterDiameter" ;
    rdfs:subClassOf :RingGasketAttribute ;
    skos:definition "The external diameter, which determines the size of the surface it seals against. This dimension is essential for providing a secure seal and preventing leakage."@en ;
    skos:prefLabel "Ring Gasket Outer Diameter"@en,
        "Diâmetro Externo da Junta de Vedação"@pt-br ;
    :hasAttributeScope :InstanceLevelAttribute,
        :TypeLevelAttribute ;
    :hasTypedValue :floatValue ;
    :hasValueCardinality :singleValue .

:RingGasketPressureRating a owl:DatatypeProperty ;
    dcterms:accessRights "PUBLIC" ;
    dcterms:identifier "RingGasketPressureRating" ;
    rdfs:subClassOf :RingGasketAttribute ;
    skos:definition "The maximum pressure it can withstand without failing. This rating is important for ensuring that the seal ring performs effectively under the operating pressures of the application."@en ;
    skos:prefLabel "Ring Gasket Pressure Rating"@en,
        "Classificação de Pressão da Junta de Vedação"@pt-br ;
    :hasAttributeScope :InstanceLevelAttribute,
        :TypeLevelAttribute ;
    :hasTypedValue :floatValue ;
    :hasValueCardinality :singleValue .

:RingGasketSpecification a owl:DatatypeProperty ;
    dcterms:accessRights "PUBLIC" ;
    dcterms:identifier "RingGasketSpecification" ;
    rdfs:subClassOf :RingGasketAttribute ;
    skos:definition "The detailed description of it's design and performance characteristics, including material, size, and pressure rating. This provides comprehensive information about the seal ring's suitability for specific applications."@en ;
    skos:prefLabel "Ring Gasket Specification"@en,
        "Especificação da Junta de Vedação"@pt-br ;
    :hasAttributeScope :InstanceLevelAttribute,
        :TypeLevelAttribute ;
    :hasTypedValue :stringValue ;
    :hasValueCardinality :singleValue .

:RingGasketStandard a owl:DatatypeProperty ;
    dcterms:accessRights "PUBLIC" ;
    dcterms:identifier "RingGasketStandard" ;
    rdfs:subClassOf :RingGasketAttribute ;
    skos:definition "The standard or specification it conforms to, such as API, ISO, or other industry standards. This indicates the compliance of the seal ring with established guidelines for quality and performance."@en ;
    skos:prefLabel "Ring Gasket Standard"@en,
        "Padrão da Junta de Vedação"@pt-br ;
    :hasAttributeScope :InstanceLevelAttribute,
        :TypeLevelAttribute ;
    :hasTypedValue :stringValue ;
    :hasValueCardinality :singleValue .

:RingGasketType a owl:DatatypeProperty ;
    dcterms:accessRights "PUBLIC" ;
    dcterms:identifier "RingGasketType" ;
    rdfs:subClassOf :RingGasketAttribute ;
    skos:definition "The specific type or design. This classification helps identify the appropriate seal ring based on its design and application requirements, ensuring it meets the sealing needs under various conditions."@en ;
    skos:prefLabel "Ring Gasket Type"@en,
        "Tipo de Junta de Vedação"@pt-br ;
    :hasAttributeScope :InstanceLevelAttribute,
        :TypeLevelAttribute ;
    :hasTypedValue :stringValue ;
    :hasValueCardinality :singleValue .

:StorageAccessory a owl:Class ;
    dcterms:identifier "StorageAccessory" ;
    rdfs:subClassOf :Accessory .

:StrandsTableAttribute a owl:Class ;
    dcterms:accessRights "PUBLIC" ;
    dcterms:identifier "StrandsTableAttribute" ;
    rdfs:subPropertyOf :DomainAttribute ;
    skos:definition "Provides detailed information about the mechanical and geometrical properties, including dimensions and material characteristics, necessary for understanding and evaluating the component's performance and suitability for its intended application."@en ;
    skos:prefLabel "Strands Table"@en,
        "Tabela de Propriedades das Cordoalhas"@pt-br ;
    :hasAttributeScope :InstanceLevelAttribute .

:TieInEquipment a owl:Class ;
    dcterms:identifier "TieInEquipment" ;
    rdfs:subClassOf :FlowControlModule .

:TopsideEquipment a owl:Class ;
    dcterms:identifier "TopsideEquipment" ;
    rdfs:subClassOf :SurfaceEquipment .

:AttributeClassification a owl:Class ;
    rdfs:subClassOf :DomainClassification .

:CompactObject a owl:Class ;
    rdfs:label "Compact Object"@en ;
    dcterms:identifier "CompactObject" ;
    rdfs:subClassOf :Asset ;
    skos:definition "A mobile physical object, usually manufactured in a standardized manner."@en ;
    skos:prefLabel "Compact Object"@en,
        "Objeto Compacto"@pt-br .

:Component a owl:Class ;
    dcterms:identifier "Component" ;
    rdfs:subClassOf :CompactObject ;
    skos:definition "Items always found as part of larger objects, with varying levels of complexity."@en ;
    skos:prefLabel "Component"@en,
        "Componente"@pt-br .

:ComponentDevice a owl:Class ;
    dcterms:identifier "ComponentDevice" ;
    rdfs:subClassOf :Component .

:DiffusionTableAttribute a owl:Class ;
    dcterms:accessRights "PUBLIC" ;
    dcterms:identifier "DiffusionTable" ;
    rdfs:subPropertyOf :DomainAttribute ;
    skos:definition "Provides data on the diffusion rates of substances through materials, used to assess how different fluids or gases permeate the structure over time. This information is crucial for evaluating material suitability and predicting long-term performance under specific environmental conditions."@en,
        "Difusão (Específica para Materiais Poliméricos)"@pt-br ;
    skos:prefLabel "Diffusion Table"@en,
        "Tabela de Difusão"@pt-br ;
    :hasAttributeScope :TypeLevelAttribute .

:DimensionsTableColumn a owl:Class ;
    rdfs:subClassOf :DrawingDimensionsTableAttribute .

:InternalIncidentalPressureTable a owl:Class ;
    dcterms:accessRights "PUBLIC" ;
    dcterms:identifier "InternalIncidentalPressureTable" ;
    rdfs:subPropertyOf :DomainAttribute ;
    skos:definition "Provides data on internal incidental pressures, which are temporary or unexpected pressure spikes within the structure. This information is crucial for understanding the pressure limits the structure may face and ensuring it can withstand short-term variations without compromising its integrity."@en ;
    skos:prefLabel "Internal Incidental Pressure Table"@en,
        "Tabela de Pressão Incidental Interna"@pt-br ;
    :hasAttributeScope :InstanceLevelAttribute .

:JustificationAttribute a owl:Class ;
    rdfs:subPropertyOf :DomainAttribute .

:MaxDesignAbsIntPresTable a owl:Class ;
    dcterms:accessRights "PUBLIC" ;
    dcterms:identifier "MaxDesignAbsIntPresTable" ;
    rdfs:subPropertyOf :DomainAttribute ;
    skos:definition "Provides data on the maximum design absolute internal pressure, used to evaluate the highest internal pressure the structure is designed to withstand. This information is critical for ensuring the structure's integrity and safety under the most demanding operational conditions."@en ;
    skos:prefLabel "Maximum Design Absolute Internal Pressure Table"@en,
        "Tabela da Máxima Pressão Interna Absoluta de Projeto"@pt-br ;
    :hasAttributeScope :InstanceLevelAttribute .

:MooringAccessory a owl:Class ;
    dcterms:identifier "MooringAccessory" ;
    rdfs:subClassOf :HardwareItem ;
    skos:definition "A Mooring Accessory includes components like anchors, chains, and connectors used to secure offshore platforms or vessels to the seabed, ensuring stability and safety in harsh marine conditions."@en ;
    skos:prefLabel "Mooring Accessory"@en,
        "Acessório de Amarração"@pt-br .

:PermeabilityTableAttribute a owl:Class ;
    dcterms:accessRights "PUBLIC" ;
    dcterms:identifier "PermeabilityTable" ;
    rdfs:subPropertyOf :DomainAttribute ;
    skos:definition "Provides data on the permeability of various substances through materials, helping to assess the rate at which fluids or gases can pass through the structure. This information is crucial for evaluating material performance, ensuring compatibility, and predicting long-term behavior under operational conditions."@en,
        "Permeabilidade (Específica para Materiais Poliméricos)"@pt-br ;
    skos:prefLabel "Permeability Table"@en,
        "Tabela de Permeabilidade"@pt-br ;
    :hasAttributeScope :TypeLevelAttribute .

:PhysicalConnection a owl:Class ;
    dcterms:identifier "PhysicalConnection" ;
    rdfs:subClassOf :Connection ;
    skos:definition "A Physical Connection refers to the actual link or interface between two or more components, such as pipes, equipment, or systems, that allows for the transfer of fluids, energy, or data."@en ;
    skos:prefLabel "Physical Connection"@en,
        "Conexão Física"@pt-br .

:PitchToleranceClass a owl:DatatypeProperty ;
    dcterms:accessRights "PUBLIC" ;
    dcterms:identifier "PitchToleranceClass" ;
    rdfs:subPropertyOf :DomainAttribute ;
    skos:definition "A classification defining the acceptable deviation range for the pitch measurement, ensuring consistency in the helical arrangement of wires or threads."@en ;
    skos:prefLabel "Pitch Tolerance Class"@en,
        "Classe de Tolerância de Passo"@pt-br ;
    :hasAttributeScope :InstanceLevelAttribute ;
    :hasTypedValue :stringValue ;
    :hasValueCardinality :singleValue .

:Registry_GUIDAttribute a owl:Class ;
    rdfs:subPropertyOf :DomainAttribute .

:SafeWorkingLoad a owl:DatatypeProperty ;
    dcterms:accessRights "PUBLIC" ;
    dcterms:identifier "SafeWorkingLoad" ;
    rdfs:subPropertyOf :DomainAttribute ;
    skos:definition "Safe Working Load (SWL) refers to the maximum load that can be safely handled under normal operating conditions. This value ensures the equipment operates within its designed capacity, preventing overloading and potential failure."@en ;
    skos:prefLabel "Safe Working Load"@en,
        "Carga Máxima Segura de Trabalho"@pt-br ;
    :hasAttributeScope :InstanceLevelAttribute,
        :TypeLevelAttribute ;
    :hasTypedValue :floatValue ;
    :hasValueCardinality :singleValue .

:Sensor a owl:Class ;
    dcterms:identifier "Sensor" ;
    rdfs:subClassOf :ElectronicDevice .

:StatusAttribute a owl:Class ;
    rdfs:label "Status Attribute"@en,
        "Atributo de Status"@pt-br ;
    rdfs:comment "Represents operational state, availability, or maintenance condition."@en ;
    rdfs:subClassOf :AttributeDomainCategory,
        :DomainAttribute ;
    skos:definition "Represents operational state, availability, or maintenance condition"@en,
        "Representa estado operacional, disponibilidade ou condição de manutenção"@pt-br .

:SubseaEngineering a owl:Class ;
    rdfs:label "Subsea Engineering"@en,
        "Engenharia Submarina"@pt-br ;
    rdfs:subClassOf :TechnicalDiscipline ;
    skos:definition "Engineering discipline focused on underwater systems and equipment for offshore operations."@en,
        "Disciplina de engenharia focada em sistemas e equipamentos subaquáticos para operações offshore."@pt-br .

:ThreadStandard a owl:DatatypeProperty ;
    dcterms:accessRights "PUBLIC" ;
    dcterms:identifier "ThreadStandard" ;
    rdfs:subPropertyOf :DomainAttribute ;
    skos:definition "The standard specification governing the design and dimensions of threads used in the component, ensuring compatibility and interchangeability."@en ;
    skos:prefLabel "Thread Standard"@en,
        "Padrão de Rosca"@pt-br ;
    :hasAttributeScope :InstanceLevelAttribute ;
    :hasTypedValue :stringValue ;
    :hasValueCardinality :singleValue .

:Tubing a owl:Class ;
    dcterms:identifier "Tubing" ;
    rdfs:subClassOf :FunctionLine .

:ValueOrigin a owl:Class ;
    rdfs:label "Value Origin"@en,
        "Origem do Valor"@pt-br ;
    rdfs:comment "Indicates how the value is obtained."@en ;
    rdfs:subClassOf :AttributeClassification ;
    skos:definition "Indicates how the value is obtained"@en,
        "Indica como o valor é obtido"@pt-br .

:Accessory a owl:Class ;
    dcterms:identifier "Accessory" ;
    rdfs:subClassOf :CompactObject .

:AuxiliaryModule a owl:Class ;
    dcterms:identifier "AuxiliaryModule" ;
    rdfs:subClassOf :SubseaEquipment .

:CrushingMaximumAllowableTensionTableAttribute a owl:Class ;
    rdfs:subPropertyOf :DomainAttribute .

:DomainAuxiliarAnnotation a owl:AnnotationProperty ;
    rdfs:subPropertyOf :DomainAnnotation .

:EarlyLeakMaxPressTableColumn a owl:Class ;
    rdfs:subClassOf :EarlyLeakMaxPressTableAttribute .

:EarlyLeakNomPressTableColumn a owl:Class ;
    rdfs:subClassOf :EarlyLeakNomPressTableAttribute .

:LinearObject a owl:Class ;
    dcterms:identifier "LinearObject" ;
    rdfs:subClassOf :Asset ;
    skos:definition "Base for any type of interconnecting element with linear geometry."@en ;
    skos:prefLabel "Linear Object"@en,
        "Objeto Linear"@pt-br .

:Renewable a owl:Class ;
    rdfs:label "Renewable Energy"@en,
        "Energia Renovável"@pt-br ;
    rdfs:subClassOf :Domain ;
    skos:definition "Industrial domain covering energy sources that are naturally replenished, such as solar, wind, and hydropower."@en,
        "Domínio industrial que abrange fontes de energia que são naturalmente reabastecidas, como solar, eólica e hidrelétrica."@pt-br .

:SolubilityTable a owl:Class ;
    dcterms:accessRights "PUBLIC" ;
    dcterms:identifier "SolubilityTable" ;
    rdfs:subPropertyOf :DomainAttribute ;
    skos:definition "Provides data on the solubility of various substances in a material, used to evaluate how different fluids or gases dissolve into the structure. This information is essential for assessing material compatibility and predicting the effects of prolonged exposure to specific substances under operational conditions."@en ;
    skos:prefLabel "Solubility Table (Specific for Polymeric Materials)"@en,
        "Tabela de Solubilidade (Específica para Materiais Poliméricos)"@pt-br ;
    :hasAttributeScope :TypeLevelAttribute .

:Structure a owl:Class ;
    dcterms:identifier "Structure" ;
    rdfs:subClassOf :CompactObject .

:TapeLayer a owl:Class ;
    dcterms:identifier "TapeLayer" ;
    rdfs:subClassOf :WoundLayer ;
    skos:definition "A layer within the structure of a subsea flexible pipe composed of tape-like materials. This layer is designed to provide additional reinforcement and protection. Typically made from high-strength polymers or other durable materials, the tape layer contributes to the pipe’s overall flexibility, structural integrity, and resistance to external environmental factors. Engineered for harsh underwater conditions, it helps maintain the performance and durability of the flexible pipe system."@en ;
    skos:prefLabel "Tape Layer"@en,
        "Camada de Fita"@pt-br .

:Domain a owl:Class ;
    rdfs:label "Industrial Domain"@en,
        "Domínio Industrial"@pt-br ;
    rdfs:comment "Represents a high-level industrial domain, such as Oil & Gas, Nuclear, or Renewable Energy."@en ;
    rdfs:subClassOf :ElementClassification ;
    skos:definition "A high-level industrial sector or application area."@en,
        "Um setor industrial ou área de aplicação de alto nível."@pt-br .

:FlowControlModule a owl:Class ;
    dcterms:identifier "FlowControlModule" ;
    rdfs:subClassOf :FlowControlEquipment .

:LayingMinimumRadiusTableColumn a owl:Class ;
    rdfs:subClassOf :LayingMinimumRadiusTableAttribute .

:LineAncillary a owl:Class ;
    dcterms:identifier "LineAncillary" ;
    rdfs:subClassOf :Component ;
    skos:definition "A component designed to complement and enhance the functionality of subsea flexible pipes. Line Ancillaries include a variety of parts such as connectors, clamps, or collars that facilitate the installation, operation, and maintenance of flexible pipes used in subsea systems. These ancillaries ensure proper alignment, secure connections, and protection against environmental factors, contributing to the reliable performance and integrity of the flexible pipe system in harsh underwater conditions."@en ;
    skos:prefLabel "Line Ancillary"@en,
        "Acessório de Linha"@pt-br .

:Location a owl:Class ;
    dcterms:identifier "Location" ;
    rdfs:subClassOf :DomainElement ;
    skos:definition "Basis for all model installation locations."@en ;
    skos:prefLabel "Location"@en,
        "Localização"@pt-br .

:SplitCollar a owl:Class ;
    dcterms:identifier "SplitCollar" ;
    rdfs:subClassOf :LineAncillary ;
    skos:definition "A component used to encircle and secure parts of subsea systems, such as flexible pipes, risers, or accessories. The Split Collar is designed with a split or gap, allowing it to be clamped around the pipe or component and then fastened together. This design facilitates easy installation and removal, making it useful for applications where adjustments or maintenance are required. The Split Collar provides structural support, alignment, and stability, ensuring that the connected components remain securely in place."@en ;
    skos:prefLabel "Split Collar"@en,
        "Colar Bipartido"@pt-br ;
    :hasAttribute :PipeMountPosition .

:SubseaEquipment a owl:Class ;
    dcterms:identifier "SubseaEquipment" ;
    rdfs:subClassOf :Equipment .

:RingGasketAttribute a owl:Class ;
    rdfs:label "Ring Gasket"@en ;
    rdfs:subPropertyOf :DomainAttribute .

:RunningTool a owl:Class ;
    dcterms:identifier "RunningTool" ;
    rdfs:subClassOf :ActuatedEquipment .

:SolidLayer a owl:Class ;
    dcterms:identifier "SolidLayer" ;
    rdfs:subClassOf :FlexibleStructureLayer ;
    skos:definition "Continuous layer used in subsea flexible pipes or similar structures, typically fabricated through extrusion. It provides structural reinforcement, pressure containment, or environmental protection, ensuring the integrity and performance of the pipe by offering consistent support or shielding."@en,
        "Camada maciça formada por extrusão contínua de um material"@pt-br ;
    skos:prefLabel "Solid Layer"@en,
        "Camada Sólida"@pt-br .

:AttributeDomainCategory a owl:Class ;
    rdfs:label "Attribute Domain Category"@en,
        "Categoria de Domínio do Atributo"@pt-br ;
    rdfs:comment "Classifies the nature or domain of the attribute's content."@en ;
    rdfs:subClassOf :AttributeClassification ;
    skos:definition "Classifies the nature or domain of the attribute's content"@en,
        "Classifica a natureza ou domínio do conteúdo do atributo"@pt-br .

:DomainEngineeringAnnotation a owl:AnnotationProperty ;
    rdfs:subPropertyOf :DomainAnnotation .

:LayerGeometryAttribute a owl:Class ;
    rdfs:subPropertyOf :DomainAttribute .

:CrushingFrictionCoefficientTighteningTableAttribute a owl:Class ;
    rdfs:subPropertyOf :DomainAttribute .

:CrushingMaximumAllowableTighteningTableAttribute a owl:Class ;
    rdfs:subPropertyOf :DomainAttribute .

:FlowControlEquipment a owl:Class ;
    dcterms:identifier "FlowControlEquipment" ;
    rdfs:subClassOf :PressureEquipment ;
    :hasAttribute :HasThermalInsulation,
        :NumberOfChokeValves,
        :NumberOfRemoteProcessIsolationValves,
        :Piggable .

:BendingStiffnessAttribute a owl:Class ;
    rdfs:label "Bending Stiffness Attribute"@en ;
    rdfs:subPropertyOf :DomainAttribute .

:PressureComponent a owl:Class ;
    dcterms:identifier "PressureComponent" ;
    rdfs:subClassOf :ComponentDevice .

rdf:value a owl:DatatypeProperty .

:DomainElement a owl:Class .

:TechnicalDiscipline a owl:Class ;
    rdfs:label "Technical Discipline"@en,
        "Disciplina Técnica"@pt-br ;
    rdfs:comment "Superclass for all technical engineering disciplines."@en ;
    rdfs:subClassOf :ElementClassification ;
    skos:definition "A specialized field of engineering or technical expertise within industrial projects."@en,
        "Um campo especializado de engenharia ou expertise técnica dentro de projetos industriais."@pt-br .

:TypedValue a owl:Class ;
    rdfs:label "Typed Value"@en ;
    rdfs:comment "Superclass for values constrained to a specific XSD datatype."@en ;
    rdfs:subClassOf :DomainAuxiliarClass .

:booleanValue a owl:Class ;
    rdfs:label "Boolean Value"@en ;
    rdfs:comment "Constraint for xsd:boolean (true/false)"@en ;
    rdfs:subClassOf :TypedValue ;
    owl:equivalentClass [ a owl:Restriction ;
            owl:allValuesFrom xsd:boolean ;
            owl:onProperty rdf:value ] .

:CommissioningObject a owl:Class ;
    rdfs:subClassOf :DomainElement .

:LifecyclePhase a owl:Class ;
    rdfs:label "Lifecycle Phase"@en,
        "Fase do Ciclo de Vida"@pt-br ;
    rdfs:comment "Represents a stage in the lifecycle of an industrial asset."@en ;
    rdfs:subClassOf :AttributeClassification ;
    skos:definition "A stage in the lifecycle of an industrial asset, from conception to decommissioning."@en,
        "Uma etapa no ciclo de vida de um ativo industrial, desde a concepção até a desativação."@pt-br .

:intValue a owl:Class ;
    rdfs:label "Integer Value"@en ;
    rdfs:comment "Constraint for xsd:int (32-bit integer)"@en ;
    rdfs:subClassOf :TypedValue ;
    owl:equivalentClass [ a owl:Restriction ;
            owl:allValuesFrom xsd:int ;
            owl:onProperty rdf:value ] .

:HydrostaticPressureTestsAttribute a owl:Class ;
    rdfs:subPropertyOf :DomainAttribute .

:multiValue a owl:Class ;
    rdfs:label "Multiple Values"@en ;
    rdfs:comment "Constraint allowing multiple values (RDF list)"@en ;
    rdfs:subClassOf :ValueCardinality .

:stringValue a owl:Class ;
    rdfs:label "String Value"@en ;
    rdfs:comment "Constraint for xsd:string (character strings)"@en ;
    rdfs:subClassOf :TypedValue ;
    owl:equivalentClass [ a owl:Restriction ;
            owl:allValuesFrom xsd:string ;
            owl:onProperty rdf:value ] .

:InstanceLevelAttribute a owl:Class ;
    rdfs:label "Instance-Level Attribute"@en,
        "Atributo de Instância"@pt-br ;
    rdfs:comment "Attribute specific to a real-world individual instance of item."@en ;
    rdfs:subClassOf :AttributeScope ;
    skos:definition "Attribute specific to a real-world individual instance of item"@en,
        "Atributo específico a uma instância individual no mundo real"@pt-br .

:TypeLevelAttribute a owl:Class ;
    rdfs:label "Type-Level Attribute"@en,
        "Atributo de Tipo"@pt-br ;
    rdfs:comment "Attribute common to all items of the same type."@en ;
    rdfs:subClassOf :AttributeScope ;
    skos:definition "Attribute common to all items of the same type"@en,
        "Atributo comum a todos os itens do mesmo tipo"@pt-br .

:floatValue a owl:Class ;
    rdfs:label "Float Value"@en ;
    rdfs:comment "Constraint for xsd:float (32-bit floating point)"@en ;
    rdfs:subClassOf :TypedValue ;
    owl:equivalentClass [ a owl:Restriction ;
            owl:allValuesFrom xsd:float ;
            owl:onProperty rdf:value ] .

:DomainAttribute a owl:DatatypeProperty .

:singleValue a owl:Class ;
    rdfs:label "Single Value"@en ;
    rdfs:comment "Constraint ensuring only one value (not a list)"@en ;
    rdfs:subClassOf :ValueCardinality .

