@prefix : <https://w3id.org/energy-domain/edo#> .
@prefix edo: <https://w3id.org/energy-domain/edo#> .
@prefix owl: <http://www.w3.org/2002/07/owl#> .
@prefix rdf: <http://www.w3.org/1999/02/22-rdf-syntax-ns#> .
@prefix sou: <http://qudt.org/vocab/sou/> .
@prefix xml: <http://www.w3.org/XML/1998/namespace> .
@prefix xsd: <http://www.w3.org/2001/XMLSchema#> .
@prefix qudt: <http://qudt.org/schema/qudt/> .
@prefix rdfs: <http://www.w3.org/2000/01/rdf-schema#> .
@prefix skos: <http://www.w3.org/2004/02/skos/core#> .
@prefix unit: <http://qudt.org/vocab/unit/> .
@prefix dcterms: <http://purl.org/dc/terms/> .
@prefix dimension: <http://qudt.org/schema/dimension/> .
@prefix quantitykind: <http://qudt.org/vocab/quantitykind/> .
@base <https://w3id.org/energy-domain/edo#> .

<https://w3id.org/energy-domain/edo> rdf:type owl:Ontology ;
                                      owl:versionIRI <https://w3id.org/energy-domain/edo/v0.0.2> ;
                                      dcterms:description "An ontology designed to represent the energy domain with semantic richness, supporting interoperability across engineering systems and standards (e.g., IFC, CFIHOS, ISO15926)." ;
                                      dcterms:title "EDO - Energy Domain Ontology" ;
                                      rdfs:label "Energy Domain Ontology" ;
                                      owl:versionInfo "v0.0.3" .

#################################################################
#    Annotation properties
#################################################################

###  http://purl.org/dc/terms/accessRights
dcterms:accessRights rdf:type owl:AnnotationProperty .


###  http://purl.org/dc/terms/description
dcterms:description rdf:type owl:AnnotationProperty .


###  http://purl.org/dc/terms/identifier
dcterms:identifier rdf:type owl:AnnotationProperty .


###  http://purl.org/dc/terms/source
dcterms:source rdf:type owl:AnnotationProperty .


###  http://purl.org/dc/terms/title
dcterms:title rdf:type owl:AnnotationProperty .


###  http://qudt.org/schema/qudt/conversionMultiplier
qudt:conversionMultiplier rdf:type owl:AnnotationProperty .


###  http://qudt.org/schema/qudt/definedUnitOfSystem
qudt:definedUnitOfSystem rdf:type owl:AnnotationProperty .


###  http://qudt.org/schema/qudt/exponent
qudt:exponent rdf:type owl:AnnotationProperty .


###  http://qudt.org/schema/qudt/hasFactorUnit
qudt:hasFactorUnit rdf:type owl:AnnotationProperty .


###  http://qudt.org/schema/qudt/hasQuantityKind
qudt:hasQuantityKind rdf:type owl:AnnotationProperty .


###  http://qudt.org/schema/qudt/hasUnit
qudt:hasUnit rdf:type owl:AnnotationProperty .


###  http://qudt.org/schema/qudt/symbol
qudt:symbol rdf:type owl:AnnotationProperty .


###  http://qudt.org/schema/qudt/ucumCode
qudt:ucumCode rdf:type owl:AnnotationProperty .


###  http://www.w3.org/2000/01/rdf-schema#subClassOf
rdfs:subClassOf rdf:type owl:AnnotationProperty .


###  http://www.w3.org/2002/07/owl#maxCardinality
owl:maxCardinality rdf:type owl:AnnotationProperty .


###  http://www.w3.org/2002/07/owl#minCardinality
owl:minCardinality rdf:type owl:AnnotationProperty .


###  http://www.w3.org/2004/02/skos/core#altLabel
skos:altLabel rdf:type owl:AnnotationProperty .


###  http://www.w3.org/2004/02/skos/core#definition
skos:definition rdf:type owl:AnnotationProperty .


###  http://www.w3.org/2004/02/skos/core#prefLabel
skos:prefLabel rdf:type owl:AnnotationProperty .


###  https://w3id.org/energy-domain/edo#DomainAnnotation
edo:DomainAnnotation rdf:type owl:AnnotationProperty .


###  https://w3id.org/energy-domain/edo#DomainAuxiliarAnnotation
edo:DomainAuxiliarAnnotation rdf:type owl:AnnotationProperty ;
                             rdfs:subPropertyOf edo:DomainAnnotation .


###  https://w3id.org/energy-domain/edo#DomainEngineeringAnnotation
edo:DomainEngineeringAnnotation rdf:type owl:AnnotationProperty ;
                                rdfs:subPropertyOf edo:DomainAnnotation .


###  https://w3id.org/energy-domain/edo#DomainRelationship
edo:DomainRelationship rdf:type owl:AnnotationProperty ;
                       rdfs:subPropertyOf edo:DomainAnnotation .


###  https://w3id.org/energy-domain/edo#appliesTo
edo:appliesTo rdf:type owl:AnnotationProperty ;
              rdfs:label "Applies to"@en ,
                         "Se aplica a"@pt-br ;
              skos:definition "Indica que o sujeito se aplica ao predicado"@pt-br ,
                              "Indicates that the subject applies to the object"@en ;
              rdfs:subPropertyOf edo:DomainAuxiliarAnnotation .


###  https://w3id.org/energy-domain/edo#defaultValidValues
edo:defaultValidValues rdf:type owl:AnnotationProperty ;
                       rdfs:subPropertyOf edo:DomainAuxiliarAnnotation .


###  https://w3id.org/energy-domain/edo#hasAttribute
edo:hasAttribute rdf:type owl:AnnotationProperty ;
                 rdfs:label "Has attribute"@en ,
                            "Possui atributo"@pt-br ;
                 skos:definition "Indica atributo(s) que a entidade possui"@pt-br ,
                                 "Indicates attribute(s) that the entity has"@en ;
                 rdfs:subPropertyOf edo:DomainAuxiliarAnnotation .


###  https://w3id.org/energy-domain/edo#hasAttributeCategory
edo:hasAttributeCategory rdf:type owl:AnnotationProperty ;
                         rdfs:label "has attribute category"@en ,
                                    "tem categoria de atributo"@pt-br ;
                         skos:definition "A categoria técnica do atributo (geométrica, funcional, etc.)"@pt-br ,
                                         "The technical category of the attribute (geometric, functional, etc.)"@en ;
                         rdfs:subPropertyOf edo:DomainEngineeringAnnotation .


###  https://w3id.org/energy-domain/edo#hasAttributeGroup
edo:hasAttributeGroup rdf:type owl:AnnotationProperty ;
                      rdfs:label "has attribute group"@en ,
                                 "tem grupo de atributo"@pt-br ;
                      skos:definition "Indica que o atributo tem um agrupamento especial para fins de organização"@pt-br ,
                                      "Indicates that the attribute has a special grouping for organizational purposes"@en ;
                      rdfs:subPropertyOf edo:DomainEngineeringAnnotation .


###  https://w3id.org/energy-domain/edo#hasAttributeScope
edo:hasAttributeScope rdf:type owl:AnnotationProperty ;
                      rdfs:label "has attribute scope"@en ,
                                 "tem escopo de atributo"@pt-br ;
                      skos:definition "Classifica se o atributo se aplica ao tipo de equipamento, instância ou lote"@pt-br ,
                                      "Classifies whether the attribute applies to equipment type, instance or batch"@en ;
                      rdfs:subPropertyOf edo:DomainEngineeringAnnotation .


###  https://w3id.org/energy-domain/edo#hasDiscipline
edo:hasDiscipline rdf:type owl:AnnotationProperty ;
                  rdfs:label "Has Discipline"@en ,
                             "Pertence a uma disciplina técnica"@pt-br ;
                  skos:definition "Associa a entidade a uma disciplina técnica"@pt-br ,
                                  "Belongs to a technical discipline"@en ;
                  rdfs:subPropertyOf edo:DomainEngineeringAnnotation .


###  https://w3id.org/energy-domain/edo#hasDomain
edo:hasDomain rdf:type owl:AnnotationProperty ;
              rdfs:label "Has Domain"@en ,
                         "Pertence a um domínio"@pt-br ;
              skos:definition "Associa a entidade a um ou mais domínios"@pt-br ,
                              "Belongs to one or more domains"@en ;
              rdfs:subPropertyOf edo:DomainEngineeringAnnotation .


###  https://w3id.org/energy-domain/edo#hasLifecycleCreationPhase
edo:hasLifecycleCreationPhase rdf:type owl:AnnotationProperty ;
                              rdfs:label "has lifecycle creation phase"@en ,
                                         "tem fase de criação no ciclo de vida"@pt-br ;
                              skos:definition "A fase do ciclo de vida quando o valor do atributo é criado"@pt-br ,
                                              "The lifecycle phase when the attribute value is created"@en ;
                              rdfs:subPropertyOf edo:DomainEngineeringAnnotation .


###  https://w3id.org/energy-domain/edo#hasLifecycleUsagePhase
edo:hasLifecycleUsagePhase rdf:type owl:AnnotationProperty ;
                           rdfs:label "has lifecycle usage phase"@en ,
                                      "tem fase de uso no ciclo de vida"@pt-br ;
                           skos:definition "A(s) fase(s) do ciclo de vida quando o valor do atributo é utilizado"@pt-br ,
                                           "The lifecycle phase(s) when the attribute value is used"@en ;
                           rdfs:subPropertyOf edo:DomainEngineeringAnnotation .


###  https://w3id.org/energy-domain/edo#hasLocationType
edo:hasLocationType rdf:type owl:AnnotationProperty ;
                    rdfs:label "Has Location Type"@en ,
                               "Pertence a um tipo de locação"@pt-br ;
                    skos:definition "Associa a entidade a um tipo de locação"@pt-br ,
                                    "Belongs to one or more Location Types"@en ;
                    rdfs:subPropertyOf edo:DomainEngineeringAnnotation .


###  https://w3id.org/energy-domain/edo#hasSubDomain
edo:hasSubDomain rdf:type owl:AnnotationProperty ;
                 rdfs:label "Has SubDomain"@en ,
                            "Pertence a um subdomínio"@pt-br ;
                 skos:definition "Associa a entidade a um ou mais subdomínios"@pt-br ,
                                 "Belongs to one or more subdomains"@en ;
                 rdfs:subPropertyOf edo:DomainEngineeringAnnotation .


###  https://w3id.org/energy-domain/edo#hasTypedValue
edo:hasTypedValue rdf:type owl:AnnotationProperty ;
                  rdfs:label "Has Typed Value"@en ,
                             "Possui tipo de valor"@pt-br ;
                  skos:definition "Indica que a entidade tem um valor como número real, inteiro, texto, booleano e etc."@pt-br ,
                                  "Indicates that the entity has a typed value, lik float, string, boolean, integer, etc."@en ;
                  rdfs:subPropertyOf edo:DomainAuxiliarAnnotation .


###  https://w3id.org/energy-domain/edo#hasUnit
edo:hasUnit rdf:type owl:AnnotationProperty ;
            rdfs:comment "Property for linking a DomainAttribute to its measurement unit."@en ;
            rdfs:label "has Unit"@en ;
            rdfs:subPropertyOf edo:DomainEngineeringAnnotation ;
            rdfs:range edo:DomainUnit ;
            rdfs:domain edo:DomainAttribute .


###  https://w3id.org/energy-domain/edo#hasValueCardinality
edo:hasValueCardinality rdf:type owl:AnnotationProperty ;
                        rdfs:label "Has Value Cardinality"@en ,
                                   "Possui cardinalidade de valor"@pt-br ;
                        skos:definition "Indica a quantidade de valores que a entidade possui"@pt-br ,
                                        "Indicates the quantity of values the entity support"@en ;
                        rdfs:subPropertyOf edo:DomainAuxiliarAnnotation .


###  https://w3id.org/energy-domain/edo#ifc_equivalentClass
edo:ifc_equivalentClass rdf:type owl:AnnotationProperty ;
                        rdfs:label "Classe IFC equivalente"@pt-br ,
                                   "IFC equivalent Class"@en ;
                        skos:definition "Classe IFC equivalente"@pt-br ,
                                        "IFC equivalent class"@en ;
                        rdfs:subPropertyOf edo:DomainEngineeringAnnotation .


###  https://w3id.org/energy-domain/edo#ifc_objectType
edo:ifc_objectType rdf:type owl:AnnotationProperty ;
                   rdfs:label "IFC ObjectType"@en ,
                              "ObjectType IFC"@pt-br ;
                   skos:definition "Object Type for IFC class customization"@en ,
                                   "Object Type para a customização de classes IFC"@pt-br ;
                   rdfs:subPropertyOf edo:DomainEngineeringAnnotation .


###  https://w3id.org/energy-domain/edo#ifc_predefinedType
edo:ifc_predefinedType rdf:type owl:AnnotationProperty ;
                       rdfs:label "IFC PredefinedType"@en ,
                                  "PredefinedType IFC"@pt-br ;
                       skos:definition "Predefined Type for IFC class customization"@en ,
                                       "Predefined Type para a customização de classes IFC"@pt-br ;
                       rdfs:subPropertyOf edo:DomainEngineeringAnnotation .


###  https://w3id.org/energy-domain/edo#specifiValidValues
edo:specifiValidValues rdf:type owl:AnnotationProperty ;
                       rdfs:subPropertyOf edo:DomainAuxiliarAnnotation .


###  https://w3id.org/energy-domain/edo#validValues
edo:validValues rdf:type owl:AnnotationProperty ;
                rdfs:label "Valid Values"@en ,
                           "Valores Válidos"@pt-br ;
                skos:definition "List of Valid Values for the Attribute"@en ,
                                "Lista de valores válidos para o atributo"@pt-br ;
                rdfs:subPropertyOf edo:DomainAuxiliarAnnotation .


#################################################################
#    Datatypes
#################################################################

###  http://www.w3.org/2001/XMLSchema#date
xsd:date rdf:type rdfs:Datatype .


###  http://www.w3.org/2001/XMLSchema#time
xsd:time rdf:type rdfs:Datatype .


#################################################################
#    Object Properties
#################################################################

###  https://w3id.org/energy-domain/edo#DomainAuxiliarProperty
edo:DomainAuxiliarProperty rdf:type owl:ObjectProperty .


#################################################################
#    Data properties
#################################################################

###  http://www.w3.org/1999/02/22-rdf-syntax-ns#value
rdf:value rdf:type owl:DatatypeProperty .


#################################################################
#    Classes
#################################################################

###  http://qudt.org/schema/qudt/Unit
qudt:Unit rdf:type owl:Class .


###  https://w3id.org/energy-domain/edo#AbandonmentCap
edo:AbandonmentCap rdf:type owl:Class ;
                   rdfs:subClassOf edo:HardwareItem ;
                   dcterms:identifier "AbandonmentCap" ;
                   skos:altLabel "Umbilical Abandonment Head"@en ;
                   skos:definition "Acessório de uso temporário para vedação da extremidade de um cabo, evitando ingresso de água."@pt-br ,
                                   "Temporary device used to seal the end of a cable, preventing water ingress."@en ;
                   skos:prefLabel "Abandonment Cap"@en ,
                                  "Capa de Abandono"@pt-br ;
                   edo:hasAttribute edo:MaximumHousedDiameter ,
                                    edo:MinimumHousedDiameter ,
                                    edo:VoltageRatingTableColumn ;
                   edo:hasDiscipline edo:SubseaUmbilicalsEngineering ;
                   edo:ifc_equivalentClass "IfcCableFitting" ;
                   edo:ifc_objectType "AbandonmentCap" .


###  https://w3id.org/energy-domain/edo#AbrasionProtector
edo:AbrasionProtector rdf:type owl:Class ;
                      rdfs:subClassOf edo:LineAncillary ;
                      dcterms:identifier "AbrasionProtector" ;
                      skos:altLabel "Abrasion Protection"@en ,
                                    "Protective Sleeve"@en ;
                      skos:definition "Component applied to cables or flexible pipes to reduce wear from friction and contact with surfaces, extending the service life of the system."@en ,
                                      "Componente aplicado sobre cabos ou dutos flexíveis para reduzir desgaste por atrito e contato com superfícies, aumentando a vida útil do sistema."@pt-br ;
                      skos:prefLabel "Abrasion Protector"@en ,
                                     "Protetor Anti-Abrasivo"@pt-br ;
                      edo:hasDiscipline edo:SubseaUmbilicalsEngineering ;
                      edo:ifc_equivalentClass "IfcProtectiveDevice" ;
                      edo:ifc_objectType "AbrasionProtector" .


###  https://w3id.org/energy-domain/edo#AbsoluteInsidePressure
edo:AbsoluteInsidePressure rdf:type owl:Class ;
                           rdfs:subClassOf edo:BendingStiffnessCurveAttribute ,
                                           edo:DomainAttribute ;
                           dcterms:accessRights "PUBLIC" ;
                           dcterms:identifier "AbsoluteInsidePressure" ;
                           skos:definition "Represents the absolute internal pressure exerted within a component or system. This property is crucial for evaluating the structural integrity and performance, ensuring that the system can withstand the specified pressure without failure, particularly in subsea environments where pressure management is critical."@en ;
                           skos:prefLabel "Absolute Inside Pressure"@en ,
                                          "Pressão Absoluta Interna"@pt-br ;
                           edo:hasAttributeScope edo:TypeLevelAttribute ;
                           edo:hasLifecycleCreationPhase edo:DetailedDesign ;
                           edo:hasTypedValue edo:FloatValue ;
                           edo:hasUnit unit:PA ;
                           edo:hasValueCardinality edo:SingleValue .


###  https://w3id.org/energy-domain/edo#AbsoluteOutsidePressure
edo:AbsoluteOutsidePressure rdf:type owl:Class ;
                            rdfs:subClassOf edo:BendingStiffnessCurveAttribute ,
                                            edo:DomainAttribute ;
                            dcterms:accessRights "PUBLIC" ;
                            dcterms:identifier "AbsoluteOutsidePressure" ;
                            skos:definition "Represents the absolute external pressure exerted on a component or system. This property is essential for evaluating how the system withstands pressure from its surrounding environment, particularly in subsea applications where external pressure can be significantly higher and impact the structural integrity of the system."@en ;
                            skos:prefLabel "Absolute Outside Pressure"@en ,
                                           "Pressão Absoluta Externa"@pt-br ;
                            edo:hasAttributeScope edo:TypeLevelAttribute ;
                            edo:hasLifecycleCreationPhase edo:DetailedDesign ;
                            edo:hasTypedValue edo:FloatValue ;
                            edo:hasUnit unit:PA ;
                            edo:hasValueCardinality edo:SingleValue .


###  https://w3id.org/energy-domain/edo#Accessory
edo:Accessory rdf:type owl:Class ;
              rdfs:subClassOf edo:CompactObject ;
              dcterms:identifier "Accessory" ;
              skos:definition "Items of reasonable complexity but not very large, including things for temporary/occasional use"@en ,
                              "Itens de razoável complexidade mas porte não muito grande, incluindo coisas de uso temporário/ocasional"@pt-br ;
              skos:prefLabel "Acessory"@en ,
                             "Acessório"@pt-br .


###  https://w3id.org/energy-domain/edo#ActuatedEquipment
edo:ActuatedEquipment rdf:type owl:Class ;
                      rdfs:subClassOf edo:SubseaEquipment ;
                      dcterms:identifier "ActuatedEquipment" ;
                      skos:definition "Equipamentos com funções atuáveis localmente ou remotamente"@pt-br ,
                                      "Equipment with locally- or remotely-actuatable functions"@en ;
                      skos:prefLabel "Actuated Equipment"@en ,
                                     "Equipamento Atuável"@pt-br .


###  https://w3id.org/energy-domain/edo#ActuatedValve
edo:ActuatedValve rdf:type owl:Class ;
                  rdfs:subClassOf edo:Valve ;
                  dcterms:identifier "ActuatedValve" ;
                  skos:definition "Base para todas as válvulas atuadas externamente, ou seja, que necessitam de ação externa para abrir/fechar"@pt-br ,
                                  "Externally-actuated valve. Base for all valves that require external action for opening/closing"@en ;
                  skos:prefLabel "Externally-actuated valve"@en ,
                                 "Válvula atuada externamente"@pt-br .


###  https://w3id.org/energy-domain/edo#AdministrativeAttribute
edo:AdministrativeAttribute rdf:type owl:Class ;
                            rdfs:subClassOf edo:AttributeNature .


###  https://w3id.org/energy-domain/edo#Anchor
edo:Anchor rdf:type owl:Class ;
           rdfs:subClassOf edo:Structure ;
           dcterms:identifier "Anchor" ;
           skos:definition "Estrutura de fundação cravada no leito marinho"@pt-br ,
                           "Foundation structure driven into seabed"@en ;
           skos:prefLabel "Anchor"@en ,
                          "Âncora"@pt-br .


###  https://w3id.org/energy-domain/edo#AnchoringCollar
edo:AnchoringCollar rdf:type owl:Class ;
                    rdfs:subClassOf edo:IfcInstanciableElement ,
                                    edo:SplitCollar ;
                    dcterms:identifier "AnchoringCollar" ;
                    skos:altLabel "Anchor Clamp"@en ,
                                  "Anchoring Device"@en ,
                                  "Fixation Collar"@en ,
                                  "Securing Collar"@en ;
                    skos:definition "A mechanical device used to stabilize and secure flexible pipes, risers, or umbilical systems to fixed structures in subsea applications. By clamping onto the outer layers of the pipe, it prevents unwanted movement during installation and operation, helping to maintain alignment and integrity under tension or compression."@en ,
                                    "Um dispositivo mecânico usado para estabilizar e fixar dutos flexíveis ou risers a estruturas fixas em aplicações submarinas, além de dar suporte aos sistemas umbilicais. Ao se prender às camadas externas do tubo, evita movimentos indesejados durante a instalação e operação, ajudando a manter o alinhamento e a integridade sob tensão ou compressão."@pt-br ;
                    skos:prefLabel "Anchoring Collar"@en ,
                                   "Colar de Ancoragem"@pt-br ;
                    edo:hasAttribute edo:SafeWorkingLoad ;
                    edo:hasDiscipline edo:SubseaFlexiblePipesEngineering ,
                                      edo:SubseaUmbilicalsEngineering ;
                    edo:ifc_equivalentClass "IfcPipeFitting" ;
                    edo:ifc_objectType "AnchoringCollar" ;
                    edo:ifc_predefinedType "USERDEFINED" .


###  https://w3id.org/energy-domain/edo#AnodeCollarSet
edo:AnodeCollarSet rdf:type owl:Class ;
                   rdfs:subClassOf edo:IfcInstanciableElement ,
                                   edo:SplitCollar ;
                   dcterms:identifier "AnodeCollarSet" ;
                   skos:altLabel "Anode Bracket"@en ,
                                 "Anode Clamp"@en ,
                                 "Cathodic Protection Collar"@en ;
                   skos:definition "Colar de anodo sacrifical usado para proteção contra corrosão em ambientes submarinos. É projetado para ser acoplado ao redor de tubos ou risers e sofrer corrosão controlada, protegendo assim as estruturas metálicas contra ferrugem e degradação. Geralmente fabricado de zinco ou alumínio, garante a longevidade dos equipamentos submarinos ao se sacrificar para evitar a corrosão em infraestruturas críticas."@pt-br ,
                                   "Sacrificial anode collar set used for corrosion protection in subsea environments. It is designed to attach around pipes or risers and undergo controlled corrosion, thus protecting the metallic structures from rust and degradation. Typically made from zinc or aluminum, it ensures the longevity of subsea equipment by sacrificing itself to prevent corrosion on critical infrastructure."@en ;
                   skos:prefLabel "Anode Collar Set"@en ,
                                  "Conjunto de Colares de Anodo"@pt-br ;
                   edo:hasAttribute edo:AnodeCollarsAxialSpacing ,
                                    edo:AnodeCollarsQuantity ,
                                    edo:ClampInternalDiameter ,
                                    edo:ExternalDiameter ,
                                    edo:GalvanicMaterial ,
                                    edo:IndividualAnodeMass ,
                                    edo:MetallicStrandLength ,
                                    edo:MetallicStrandSpareQuantity ;
                   edo:hasDiscipline edo:SubseaFlexiblePipesEngineering ,
                                     edo:SubseaUmbilicalsEngineering ;
                   edo:ifc_equivalentClass "IfcPipeFitting" ;
                   edo:ifc_objectType "AnodeCollarSet" ;
                   edo:ifc_predefinedType "USERDEFINED" .


###  https://w3id.org/energy-domain/edo#AnodeCollarsAxialSpacing
edo:AnodeCollarsAxialSpacing rdf:type owl:Class ;
                             rdfs:subClassOf edo:DomainAttribute ;
                             dcterms:accessRights "PUBLIC" ;
                             dcterms:identifier "AnodeCollarsAxialSpacing" ;
                             skos:definition "Axial distance between each individual collar."@en ;
                             skos:prefLabel "Anode Collars Axial Spacing"@en ,
                                            "Espaçamento Axial entre os Colares de Anodo"@pt-br ;
                             edo:hasAttributeScope edo:TypeLevelAttribute ;
                             edo:hasLifecycleCreationPhase edo:DetailedDesign ;
                             edo:hasTypedValue edo:FloatValue ;
                             edo:hasUnit unit:MilliM ;
                             edo:hasValueCardinality edo:SingleValue .


###  https://w3id.org/energy-domain/edo#AnodeCollarsQuantity
edo:AnodeCollarsQuantity rdf:type owl:Class ;
                         rdfs:subClassOf edo:DomainAttribute ;
                         dcterms:accessRights "PUBLIC" ;
                         dcterms:identifier "AnodeCollarsQuantity" ;
                         skos:definition "The total number of anode collars to provide cathodic protection against corrosion."@en ;
                         skos:prefLabel "Anode Collars Quantity"@en ,
                                        "Quantidade de Colares de Anodo"@pt-br ;
                         edo:hasAttributeScope edo:TypeLevelAttribute ;
                         edo:hasLifecycleCreationPhase edo:DetailedDesign ;
                         edo:hasTypedValue edo:IntValue ;
                         edo:hasValueCardinality edo:SingleValue .


###  https://w3id.org/energy-domain/edo#AnodeSled
edo:AnodeSled rdf:type owl:Class ;
              rdfs:subClassOf edo:Structure ;
              dcterms:identifier "AnodeSled" ;
              skos:prefLabel "Anode Sled"@en ,
                             "Trenó de Anodos"@pt-br .


###  https://w3id.org/energy-domain/edo#AntiCollapseSheath
edo:AntiCollapseSheath rdf:type owl:Class ;
                       rdfs:subClassOf edo:IfcInstanciableElement ,
                                       edo:SolidLayer ;
                       dcterms:identifier "AntiCollapseSheath" ;
                       skos:definition "Camada de reforço em dutos flexíveis submarinos usados na exploração de petróleo e gás, projetada para evitar o colapso do duto sob altas pressões externas, como as encontradas em ambientes de águas profundas. Sua função principal é fornecer suporte estrutural contra forças externas que poderiam comprimir ou deformar o duto, especialmente durante situações em que a pressão interna é reduzida ou ausente, como quando o duto está vazio. Normalmente feita de materiais metálicos ou poliméricos de alta resistência, a Capa Anti-Colapso garante a integridade do duto flexível em condições extremas."@pt-br ,
                                       "Reinforcement layer in subsea flexible pipes used in oil and gas exploration, designed to prevent the collapse of the pipe under high external pressure conditions, such as those encountered in deepwater environments. Its primary role is to provide structural support against external forces that could compress or deform the pipe, particularly during situations where the internal pressure is reduced or absent, like when the pipe is emptied. Typically made from high-strength metallic or polymeric materials, the Anti Collapse Sheath ensures the integrity of the flexible pipe under extreme conditions."@en ;
                       skos:prefLabel "Anti Collapse Sheath"@en ,
                                      "Capa Anti-Colapso"@pt-br ;
                       edo:hasDiscipline edo:SubseaFlexiblePipesEngineering ;
                       edo:ifc_equivalentClass "IfcPipeSegment" ;
                       edo:ifc_objectType "AntiCollapseSheath" ;
                       edo:ifc_predefinedType "USERDEFINED" .


###  https://w3id.org/energy-domain/edo#AntiWearSheath
edo:AntiWearSheath rdf:type owl:Class ;
                   rdfs:subClassOf edo:IfcInstanciableElement ,
                                   edo:SolidLayer ;
                   dcterms:identifier "AntiWearSheath" ;
                   skos:definition "Camada de reforço em dutos flexíveis usados na exploração de petróleo e gás, projetada para proteger o duto do desgaste externo e da abrasão causados pelo contato com o fundo marinho, equipamentos ou outros elementos submarinos. Seu papel principal é fornecer uma barreira protetora durável que protege as camadas subjacentes contra danos mecânicos, aumentando a vida útil do tubo flexível. Geralmente feita de materiais poliméricos resistentes ao desgaste, a Capa Anti-Atrito garante a integridade do duto ao reduzir o risco de danos na superfície em condições operacionais adversas."@pt-br ,
                                   "Reinforcement layer in subsea flexible pipes used in oil and gas exploration, designed to protect the pipe from external wear and abrasion caused by contact with the seabed, equipment, or other subsea elements. Its primary role is to provide a durable protective barrier that shields the underlying layers from mechanical damage, extending the lifespan of the flexible pipe. Typically made from wear-resistant polymeric materials, the Anti Wear Sheath ensures the pipe's integrity by reducing the risk of surface damage under harsh operating conditions."@en ;
                   skos:prefLabel "Anti Wear Sheath"@en ,
                                  "Capa Anti-Atrito"@pt-br ;
                   edo:hasAttribute edo:TapesQuantity ;
                   edo:hasDiscipline edo:SubseaFlexiblePipesEngineering ;
                   edo:ifc_equivalentClass "IfcPipeSegment" ;
                   edo:ifc_objectType "AntiWearSheath" ;
                   edo:ifc_predefinedType "USERDEFINED" .


###  https://w3id.org/energy-domain/edo#AnyURIType
edo:AnyURIType rdf:type owl:Class ;
               owl:equivalentClass [ rdf:type owl:Restriction ;
                                     owl:onProperty rdf:value ;
                                     owl:allValuesFrom xsd:anyURI
                                   ] ;
               rdfs:subClassOf edo:DataType ;
               rdfs:comment "Constraint for xsd:anyURI (URIs/IRIs)"@en ;
               rdfs:label "URI Value"@en .


###  https://w3id.org/energy-domain/edo#ArcAngle
edo:ArcAngle rdf:type owl:Class ;
             rdfs:subClassOf edo:DomainAttribute ;
             dcterms:accessRights "PUBLIC" ;
             dcterms:identifier "ArcAngle" ;
             skos:definition "Arc angle"@en ;
             skos:prefLabel "Arc angle"@en ,
                            "Ângulo do arco"@pt-br ;
             edo:hasAttributeScope edo:TypeLevelAttribute ;
             edo:hasLifecycleCreationPhase edo:DetailedDesign ;
             edo:hasTypedValue edo:FloatValue ;
             edo:hasUnit unit:DEG ;
             edo:hasValueCardinality edo:SingleValue .


###  https://w3id.org/energy-domain/edo#ArchitecturalEngineering
edo:ArchitecturalEngineering rdf:type owl:Class ;
                             rdfs:subClassOf edo:TechnicalDiscipline ;
                             rdfs:label "Architectural Engineering"@en ,
                                        "Engenharia Arquitetônica"@pt-br ;
                             skos:definition "Disciplina de engenharia focada no projeto de edifícios, construção e integração de sistemas."@pt-br ,
                                             "Engineering discipline focused on building design, construction and systems integration."@en .


###  https://w3id.org/energy-domain/edo#ArmorPot
edo:ArmorPot rdf:type owl:Class ;
             rdfs:subClassOf edo:IfcInstanciableElement ,
                             edo:LineTermination ;
             dcterms:identifier "ArmorPot" ;
             skos:definition "Elemento de terminação de armaduras de umbilical"@pt-br ,
                             "Umbilical armor termination element"@en ;
             skos:prefLabel "Armor Pot"@en ,
                            "Armor Pot"@pt-br ;
             edo:hasDiscipline edo:SubseaUmbilicalsEngineering ;
             edo:ifc_equivalentClass "IfcPipeFitting" ;
             edo:ifc_objectType "ArmorPot" ;
             edo:ifc_predefinedType "USERDEFINED" .


###  https://w3id.org/energy-domain/edo#ArmourLayer
edo:ArmourLayer rdf:type owl:Class ;
                rdfs:subClassOf edo:WoundLayer ;
                dcterms:identifier "ArmourLayer" ;
                skos:definition "A reinforcement layer in subsea flexible pipes used in oil and gas exploration, designed to provide mechanical strength and protection against external forces, such as pressure and movement. It ensures structural integrity by preventing deformation and failure during operation. Typically made from high-strength metal wires, like carbon steel or stainless steel, the Armor Layer enhances the pipe's durability in harsh underwater conditions."@en ;
                skos:prefLabel "Armour Layer"@en ,
                               "Camada de Armadura"@pt-br .


###  https://w3id.org/energy-domain/edo#AssemblyShouldObeyModelPolarity
edo:AssemblyShouldObeyModelPolarity rdf:type owl:Class ;
                                    rdfs:subClassOf edo:DomainAttribute ;
                                    dcterms:accessRights "PUBLIC" ;
                                    dcterms:identifier "AssemblyShouldObeyModelPolarity" ;
                                    skos:definition "If true, the pipe section must be assembled according to the polarity in the model. If false, it can be mounted in any polarity."@en ;
                                    skos:prefLabel "A Montagem Deve Obedecer à Polaridade do Modelo"@pt-br ,
                                                   "Assembly Should Obey Model Polarity"@en ;
                                    edo:hasAttributeScope edo:InstanceLevelAttribute ;
                                    edo:hasLifecycleCreationPhase edo:DetailedDesign ;
                                    edo:hasTypedValue edo:BooleanValue ;
                                    edo:hasValueCardinality edo:SingleValue .


###  https://w3id.org/energy-domain/edo#AssemblyTorque
edo:AssemblyTorque rdf:type owl:Class ;
                   rdfs:subClassOf edo:DomainAttribute ;
                   dcterms:accessRights "PUBLIC" ;
                   dcterms:identifier "AssemblyTorque" ;
                   skos:definition "Specifies the torque applied during assembly, ensuring proper tightening for secure connections. This value is critical for maintaining the structural integrity and reliability of the connection under operational loads."@en ;
                   skos:prefLabel "Assembly Torque"@en ,
                                  "Torque de montagem"@pt-br ;
                   edo:hasAttributeScope edo:InstanceLevelAttribute ;
                   edo:hasLifecycleCreationPhase edo:DetailedDesign ;
                   edo:hasTypedValue edo:FloatValue ;
                   edo:hasUnit unit:N-M ;
                   edo:hasValueCardinality edo:SingleValue .


###  https://w3id.org/energy-domain/edo#AssemblyType
edo:AssemblyType rdf:type owl:Class ;
                 rdfs:subClassOf edo:DomainAttribute ;
                 dcterms:accessRights "PUBLIC" ;
                 dcterms:identifier "AssemblyType" ;
                 rdfs:comment "Especifica o tipo construtivo do jumper"@pt-br ;
                 skos:definition "Especifica o tipo construtivo do jumper"@pt-br ,
                                 "Specifies jumper constructive type"@en ;
                 skos:prefLabel "Assembly type"@en ,
                                "Tipo de montagem"@pt-br ;
                 edo:hasAttributeScope edo:TypeLevelAttribute ;
                 edo:hasLifecycleCreationPhase edo:DetailedDesign ;
                 edo:hasTypedValue edo:StringValue ;
                 edo:hasValueCardinality edo:SingleValue .


###  https://w3id.org/energy-domain/edo#Asset
edo:Asset rdf:type owl:Class ;
          rdfs:subClassOf edo:DomainElement ;
          dcterms:identifier "Asset" ;
          skos:definition "An asset refers to Physical, Traceable, and Replaceable resources such as equipment and pipelines crucial for production and transportation. These assets are managed to optimize performance, ensure safety, and maximize operational efficiency throughout their lifecycle."@en ,
                          "Base para todos os ativos físicos tangíveis"@pt-br ;
          skos:prefLabel "Asset"@en ,
                         "Ativo"@pt-br ;
          edo:hasAttribute edo:DesignLifeSpan ,
                           edo:DisplacedVolume ,
                           edo:IdInUnifilarDiagram ,
                           edo:InternalVolume ,
                           edo:IsSpare ,
                           edo:Manufacturer ,
                           edo:ManufacturerDefinedMaterialName ,
                           edo:ManufacturerSerialNumber ,
                           edo:MaterialSupplierName ,
                           edo:PartNumber ,
                           edo:ProjectDrawingCode ,
                           edo:ProjectDrawingRevision ,
                           edo:SerialNumber ,
                           edo:SupplierProvidedMaterialName .


###  https://w3id.org/energy-domain/edo#AttenuationCoefficient
edo:AttenuationCoefficient rdf:type owl:Class ;
                           rdfs:subClassOf edo:DomainAttribute ;
                           dcterms:accessRights "PUBLIC" ;
                           dcterms:identifier "AttenuationCoefficient" ;
                           skos:definition "Nominal optical attentuation coefficient presented by fibers, in the wavelength range of interest"@en ;
                           skos:prefLabel "Attenuation coefficient"@en ;
                           edo:hasUnit unit:DB-PER-KM .


###  https://w3id.org/energy-domain/edo#AttributeClassification
edo:AttributeClassification rdf:type owl:Class ;
                            rdfs:subClassOf edo:DomainClassification ;
                            rdfs:label "Attribute Classification"@en ,
                                       "Classificação de Atributos"@pt-br ;
                            skos:definition "Axis dedicated to classifying attributes, their nature, scope, value origin and datatype aspects."@en ,
                                            "Eixo dedicado a classificar atributos, sua natureza, escopo, origem do valor e aspectos de tipo de dado."@pt-br .


###  https://w3id.org/energy-domain/edo#AttributeDomainCategory
edo:AttributeDomainCategory rdf:type owl:Class ;
                            rdfs:subClassOf edo:AttributeNature ;
                            rdfs:comment "Classifies the nature or domain of the attribute's content."@en ;
                            rdfs:label "Attribute Domain Category"@en ,
                                       "Categoria de Domínio do Atributo"@pt-br ;
                            skos:definition "Classifica a natureza ou domínio do conteúdo do atributo"@pt-br ,
                                            "Classifies the nature or domain of the attribute's content"@en .


###  https://w3id.org/energy-domain/edo#AttributeNature
edo:AttributeNature rdf:type owl:Class ;
                    rdfs:subClassOf edo:AttributeClassification ;
                    rdfs:label "Attribute Nature"@en ,
                               "Natureza do Atributo"@pt-br ;
                    skos:definition "High-level nature of attributes, including technical and administrative branches."@en ,
                                    "Natureza de alto nível dos atributos, incluindo ramos técnicos e administrativos."@pt-br .


###  https://w3id.org/energy-domain/edo#AttributeScope
edo:AttributeScope rdf:type owl:Class ;
                   rdfs:subClassOf edo:AttributeNature ;
                   rdfs:comment "Defines whether the attribute applies to all instances of a type or to a specific instance."@en ;
                   rdfs:label "Attribute Scope"@en ,
                              "Escopo do Atributo"@pt-br ;
                   skos:definition "Define se o atributo se aplica a todas as instâncias de um tipo ou a uma instância específica"@pt-br ,
                                   "Defines whether the attribute applies to all instances of a type or to a specific instance"@en .


###  https://w3id.org/energy-domain/edo#AttributeValueCardinality
edo:AttributeValueCardinality rdf:type owl:Class ;
                              rdfs:subClassOf edo:ValueNature ;
                              rdfs:comment "Superclass for constraints on the cardinality of values (single or multiple)."@en ;
                              rdfs:label "Value Cardinality"@en .


###  https://w3id.org/energy-domain/edo#AttributesGroup
edo:AttributesGroup rdf:type owl:Class ;
                    rdfs:subClassOf edo:ValueNature .


###  https://w3id.org/energy-domain/edo#AutomationControlEngineering
edo:AutomationControlEngineering rdf:type owl:Class ;
                                 rdfs:subClassOf edo:TechnicalDiscipline ;
                                 rdfs:label "Automation & Control Engineering"@en ,
                                            "Engenharia de Automação e Controle"@pt-br ;
                                 skos:definition "Disciplina de engenharia focada em sistemas de controle automatizado e automação de processos."@pt-br ,
                                                 "Engineering discipline focused on automated control systems and process automation."@en .


###  https://w3id.org/energy-domain/edo#AuxiliaryModule
edo:AuxiliaryModule rdf:type owl:Class ;
                    rdfs:subClassOf edo:SubseaEquipment ;
                    dcterms:identifier "AuxiliaryModule" ;
                    skos:definition "Module with auxiliary functions installed as part of some larger subsea equipment"@en ,
                                    "Módulo com funçõs auxiliares, instalado como parte de um equipamento submarino maior"@pt-br ;
                    skos:prefLabel "Auxiliary module"@en ,
                                   "Módulo auxiliar"@pt-br .


###  https://w3id.org/energy-domain/edo#AxialStiffness
edo:AxialStiffness rdf:type owl:Class ;
                   rdfs:subClassOf edo:DomainAttribute ;
                   dcterms:accessRights "PUBLIC" ;
                   dcterms:identifier "AxialStiffness" ;
                   skos:definition "Axial stiffness"@en ;
                   skos:prefLabel "Axial stiffness"@en ,
                                  "Rigidez axial"@pt-br ;
                   edo:hasAttributeScope edo:TypeLevelAttribute ;
                   edo:hasLifecycleCreationPhase edo:DetailedDesign ;
                   edo:hasTypedValue edo:FloatValue ;
                   edo:hasUnit unit:KiloN ;
                   edo:hasValueCardinality edo:SingleValue .


###  https://w3id.org/energy-domain/edo#AxialStiffnessUnderCompressionAtSeaLevel
edo:AxialStiffnessUnderCompressionAtSeaLevel rdf:type owl:Class ;
                                             rdfs:subClassOf edo:DomainAttribute ;
                                             dcterms:accessRights "PUBLIC" ;
                                             dcterms:identifier "AxialStiffnessUnderCompressionAtSeaLevel" ;
                                             skos:definition "Represents the resistance of a component or system to axial deformation under compression when measured at sea level. This property is essential for understanding how the structure behaves under compressive loads, ensuring that it can maintain stability and structural integrity."@en ,
                                                             "Rigidez axial (EA) duto comprimido, 20°C e pressão atmosferica (dentro e fora)"@pt-br ;
                                             skos:prefLabel "Axial Stiffness Under Compression At Sea Level"@en ,
                                                            "Rigidez Axial sob Compressão ao Nível do Mar"@pt-br ;
                                             edo:hasAttributeScope edo:TypeLevelAttribute ;
                                             edo:hasLifecycleCreationPhase edo:DetailedDesign ;
                                             edo:hasTypedValue edo:FloatValue ;
                                             edo:hasUnit unit:N ;
                                             edo:hasValueCardinality edo:SingleValue .


###  https://w3id.org/energy-domain/edo#AxialStiffnessUnderTensionAtSeaLevel
edo:AxialStiffnessUnderTensionAtSeaLevel rdf:type owl:Class ;
                                         rdfs:subClassOf edo:DomainAttribute ;
                                         dcterms:accessRights "PUBLIC" ;
                                         dcterms:identifier "AxialStiffnessUnderTensionAtSeaLevel" ;
                                         skos:definition "Represents the resistance of a component or system to axial deformation under tension when measured at sea level. This property is crucial for evaluating how the structure performs under tensile loads, ensuring it can withstand stretching forces while maintaining its integrity."@en ,
                                                         "Rigidez axial (EA) duto tracionado, 20°C e pressão atmosferica (dentro e fora)."@pt-br ;
                                         skos:prefLabel "Axial Stiffness Under Tension At Sea Level"@en ,
                                                        "Rigidez Axial sob Tração ao Nível do Mar"@pt-br ;
                                         edo:hasAttributeScope edo:TypeLevelAttribute ;
                                         edo:hasLifecycleCreationPhase edo:DetailedDesign ;
                                         edo:hasTypedValue edo:FloatValue ;
                                         edo:hasUnit unit:N ;
                                         edo:hasValueCardinality edo:SingleValue .


###  https://w3id.org/energy-domain/edo#BOP
edo:BOP rdf:type owl:Class ;
        rdfs:subClassOf edo:PressureEquipment ;
        dcterms:identifier "BOP" ;
        skos:prefLabel "Blowout preventer"@en ,
                       "Blowout preventer"@pt-br .


###  https://w3id.org/energy-domain/edo#Base64BinaryType
edo:Base64BinaryType rdf:type owl:Class ;
                     owl:equivalentClass [ rdf:type owl:Restriction ;
                                           owl:onProperty rdf:value ;
                                           owl:allValuesFrom xsd:base64Binary
                                         ] ;
                     rdfs:subClassOf edo:DataType ;
                     rdfs:comment "Constraint for xsd:base64Binary (binary data)"@en ;
                     rdfs:label "Base64 Binary"@en .


###  https://w3id.org/energy-domain/edo#BasicDesign
edo:BasicDesign rdf:type owl:Class ;
                rdfs:subClassOf edo:DesignPhase ;
                rdfs:label "Basic Design"@en ,
                           "Projeto Básico"@pt-br ;
                skos:definition "Fase onde são desenvolvidas especificações gerais de engenharia, layouts e listas de equipamentos principais."@pt-br ,
                                "Phase where general engineering specifications, layouts, and main equipment lists are developed."@en .


###  https://w3id.org/energy-domain/edo#BasicProjectRevision
edo:BasicProjectRevision rdf:type owl:Class ;
                         rdfs:subClassOf edo:DomainAttribute ;
                         dcterms:accessRights "PUBLIC" ;
                         dcterms:identifier "BasicProjectRevision" ;
                         skos:definition "Numeric value incremented with each new submission of the project (e.g., 0000, 0001, 0002, etc.), recorded as text. This value tracks revisions and ensures clarity in version control throughout the project lifecycle, allowing stakeholders to reference the most current or previous versions as needed."@en ,
                                         "Valor numérico incrementado a cada novo envio (0000, 0001, 0002 e etc.) como texto."@pt-br ;
                         skos:prefLabel "Basic Project Revision"@en ,
                                        "Revisão do Projeto Básico"@pt-br ;
                         edo:hasAttributeScope edo:InstanceLevelAttribute ;
                         edo:hasLifecycleCreationPhase edo:BasicDesign ;
                         edo:hasTypedValue edo:StringValue ;
                         edo:hasValueCardinality edo:SingleValue .


###  https://w3id.org/energy-domain/edo#BatchLevelAttribute
edo:BatchLevelAttribute rdf:type owl:Class ;
                        rdfs:subClassOf edo:AttributeScope ;
                        rdfs:comment "Attribute common to a batch of equipment instances."@en ;
                        rdfs:label "Atributo de Lote"@pt-br ,
                                   "Batch Attribute"@en ;
                        skos:definition "Atributo comum a um lote de instâncias de equipamento"@pt-br ,
                                        "Attribute common to a batch of equipment instances"@en .


###  https://w3id.org/energy-domain/edo#BellmouthDiameter
edo:BellmouthDiameter rdf:type owl:Class ;
                      rdfs:subClassOf edo:DomainAttribute ;
                      dcterms:accessRights "PUBLIC" ;
                      dcterms:identifier "BellmouthDiameter" ;
                      skos:definition "Compatible bellmouth diameter"@en ,
                                      "Diâmetro de boca de sino compatível"@pt-br ;
                      skos:prefLabel "Bellmouth diameter"@en ,
                                     "Diâmetro da boca de sino"@pt-br ;
                      edo:hasAttributeScope edo:TypeLevelAttribute ;
                      edo:hasLifecycleCreationPhase edo:DetailedDesign ;
                      edo:hasTypedValue edo:FloatValue ;
                      edo:hasValueCardinality edo:SingleValue .


###  https://w3id.org/energy-domain/edo#BendMomentVsShearForceCurveAttribute
edo:BendMomentVsShearForceCurveAttribute rdf:type owl:Class ;
                                         rdfs:subClassOf edo:DomainAttribute ;
                                         rdfs:label "Bending Moment Versus Shear Force Attribute"@en .


###  https://w3id.org/energy-domain/edo#BendMomentVsShearForceTableColumn
edo:BendMomentVsShearForceTableColumn rdf:type owl:Class ;
                                      rdfs:subClassOf edo:BendMomentVsShearForceCurveAttribute ;
                                      dcterms:accessRights "PUBLIC" ;
                                      dcterms:identifier "BendMomentVsShearForceTable" ;
                                      skos:definition "Provides data on the relationship between bending moment and shear force, used to evaluate how the structure behaves under combined loading conditions. This information is critical for determining the structural integrity and performance under different operational stresses."@en ;
                                      skos:prefLabel "Bending moment vs Shear Force Table"@en ,
                                                     "Tabela de Momento de Curvatura em Função da Força Cisalhante"@pt-br ;
                                      edo:hasAttributeScope edo:TypeLevelAttribute .


###  https://w3id.org/energy-domain/edo#BendMomentVsShearForceTable_BendingMoment
edo:BendMomentVsShearForceTable_BendingMoment rdf:type owl:Class ;
                                              rdfs:subClassOf edo:BendMomentVsShearForceTableColumn ;
                                              dcterms:accessRights "PUBLIC" ;
                                              dcterms:identifier "BendMomentVsShearForceTable_BendingMoment" ;
                                              skos:definition "Represents the moment generated by a force causing the component or system to bend around an axis. This property is critical for assessing the structure's ability to resist bending under operational loads, ensuring it maintains its shape and structural integrity."@en ;
                                              skos:prefLabel "Bending Moment"@en ,
                                                             "Momento de flexão"@pt-br ;
                                              edo:hasAttributeScope edo:TypeLevelAttribute ;
                                              edo:hasLifecycleCreationPhase edo:DetailedDesign ;
                                              edo:hasTypedValue edo:FloatValue ;
                                              edo:hasUnit unit:N-M ;
                                              edo:hasValueCardinality edo:MultiValue .


###  https://w3id.org/energy-domain/edo#BendMomentVsShearForceTable_Condition
edo:BendMomentVsShearForceTable_Condition rdf:type owl:Class ;
                                          rdfs:subClassOf edo:BendMomentVsShearForceTableColumn ;
                                          dcterms:accessRights "PUBLIC" ;
                                          dcterms:identifier "BendMomentVsShearForceTable_Condition" ;
                                          skos:definition "Curve data flexible pipe condition."@en ;
                                          skos:prefLabel "Condition"@en ,
                                                         "Condição do flexível para os dados da curva"@pt-br ;
                                          edo:hasAttributeScope edo:TypeLevelAttribute ;
                                          edo:hasLifecycleCreationPhase edo:DetailedDesign ;
                                          edo:hasTypedValue edo:StringValue ;
                                          edo:hasValueCardinality edo:SingleValue .


###  https://w3id.org/energy-domain/edo#BendMomentVsShearForceTable_ShearForce
edo:BendMomentVsShearForceTable_ShearForce rdf:type owl:Class ;
                                           rdfs:subClassOf edo:BendMomentVsShearForceTableColumn ;
                                           dcterms:accessRights "PUBLIC" ;
                                           dcterms:identifier "BendMomentVsShearForceTable_ShearForce" ;
                                           skos:definition "Força de cisalhamento (Obrigatório incluir o valor para força = 0)"@pt-br ,
                                                           "Represents the force applied parallel to the surface of a material or component, causing it to experience shear stress. This property is essential for evaluating the material's ability to resist sliding or deformation when subjected to external forces."@en ;
                                           skos:prefLabel "Força de Cisalhamento"@pt-br ,
                                                          "Shear Force"@en ;
                                           edo:hasAttributeScope edo:TypeLevelAttribute ;
                                           edo:hasLifecycleCreationPhase edo:DetailedDesign ;
                                           edo:hasTypedValue edo:FloatValue ;
                                           edo:hasUnit unit:N ;
                                           edo:hasValueCardinality edo:MultiValue .


###  https://w3id.org/energy-domain/edo#BendRestrictor
edo:BendRestrictor rdf:type owl:Class ;
                   rdfs:subClassOf edo:IfcInstanciableElement ,
                                   edo:LineAncillary ;
                   dcterms:identifier "BendRestrictor" ;
                   skos:altLabel "Bend Limiter"@en ,
                                 "Bending Restrictor"@en ,
                                 "Curvature Limiter"@en ;
                   skos:definition "Device used in subsea flexible pipes to limit the bending radius and prevent over-bending that could damage the pipe. Typically installed near critical areas such as connectors or end fittings, where excessive bending could compromise the structural integrity of the pipe. The Bend Restrictor consists of multiple interlocking segments that allow flexibility up to a certain radius, beyond which the segments lock to prevent further bending, protecting the pipe from deformation or failure in harsh subsea environments."@en ,
                                   "Dispositivo usado em dutos flexíveis para limitar o raio de curvatura e evitar curvaturas excessivas que poderiam danificar o duto. Normalmente instalado perto de áreas críticas, como conectores ou acessórios finais, onde curvaturas excessivas poderiam comprometer a integridade estrutural do duto. O Restritor de Curvatura consiste em múltiplos segmentos interligados que permitem flexibilidade até um certo raio, além do qual os segmentos se bloqueiam para impedir mais curvaturas, protegendo o duto contra deformações ou falhas em ambientes submarinos adversos."@pt-br ;
                   skos:prefLabel "Bend Restrictor"@en ,
                                  "Restritor de Curvatura"@pt-br ;
                   edo:hasAttribute edo:ArcAngle ,
                                    edo:BendMomentVsShearForceTableColumn ,
                                    edo:LockedLength ,
                                    edo:MaximumBendingMoment ,
                                    edo:MaximumBendingMomentLongTerm ,
                                    edo:MaximumLength ,
                                    edo:MaximumShearForce ,
                                    edo:MaximumShearForceLongTerm ,
                                    edo:MinimumBendingRadius ,
                                    edo:MinimumLength ,
                                    edo:WeightInWater ;
                   edo:hasDiscipline edo:SubseaFlexiblePipesEngineering ,
                                     edo:SubseaUmbilicalsEngineering ;
                   edo:ifc_equivalentClass "IfcPipeFitting" ;
                   edo:ifc_objectType "BendRestrictor" .


###  https://w3id.org/energy-domain/edo#BendStiffener
edo:BendStiffener rdf:type owl:Class ;
                  rdfs:subClassOf edo:LineAncillary ;
                  dcterms:identifier "BendStiffener" ;
                  skos:definition "Device used in subsea flexible pipes to provide gradual stiffness transition between the flexible pipe and a fixed structure, preventing excessive bending at critical areas such as terminations or connectors. The Bend Stiffener is designed to manage stress concentration by stiffening the pipe over a defined length, reducing the risk of damage due to repeated bending, fatigue, or over-flexing. Typically made from high-strength materials, it ensures the long-term structural integrity of the pipe in dynamic subsea environments."@en ;
                  skos:prefLabel "Bend Stiffener"@en ,
                                 "Enrijecedor de Curvatura"@pt-br ;
                  edo:hasAttribute edo:ReinforcementLength ,
                                   edo:ReinforcementOuterDiameter ,
                                   edo:WeightInWater .


###  https://w3id.org/energy-domain/edo#BendingMomentTable_BendingMoment
edo:BendingMomentTable_BendingMoment rdf:type owl:Class ;
                                     rdfs:subClassOf edo:BendingStiffnessTableColumn ;
                                     dcterms:accessRights "PUBLIC" ;
                                     dcterms:identifier "BendingMomentTable_BendingMoment" ;
                                     skos:definition "Represents the moment generated by a force causing the component or system to bend around an axis. This property is critical for assessing the structure's ability to resist bending under operational loads, ensuring it maintains its shape and structural integrity."@en ;
                                     skos:prefLabel "Bending Moment"@en ,
                                                    "Momento de Flexão"@pt-br ;
                                     edo:hasAttributeScope edo:TypeLevelAttribute ;
                                     edo:hasLifecycleCreationPhase edo:DetailedDesign ;
                                     edo:hasTypedValue edo:FloatValue ;
                                     edo:hasUnit unit:N-M ;
                                     edo:hasValueCardinality edo:MultiValue .


###  https://w3id.org/energy-domain/edo#BendingMomentTable_Curvature
edo:BendingMomentTable_Curvature rdf:type owl:Class ;
                                 rdfs:subClassOf edo:BendingStiffnessTableColumn ;
                                 dcterms:accessRights "PUBLIC" ;
                                 dcterms:identifier "BendingMomentTable_Curvature" ;
                                 skos:definition "Represents the degree to which a component or structure bends or curves along its length. This property is important for understanding the flexibility and bending behavior, ensuring that the structure can perform as required under operational conditions without exceeding its design limits."@en ;
                                 skos:prefLabel "Curvatura"@pt-br ,
                                                "Curvature"@en ;
                                 edo:hasAttributeScope edo:TypeLevelAttribute ;
                                 edo:hasLifecycleCreationPhase edo:DetailedDesign ;
                                 edo:hasTypedValue edo:FloatValue ;
                                 edo:hasUnit unit:PER-M ;
                                 edo:hasValueCardinality edo:MultiValue .


###  https://w3id.org/energy-domain/edo#BendingStiffnessCurveAttribute
edo:BendingStiffnessCurveAttribute rdf:type owl:Class ;
                                   rdfs:subClassOf edo:DomainAttribute ;
                                   rdfs:label "Bending Stiffness Attribute"@en .


###  https://w3id.org/energy-domain/edo#BendingStiffnessStorage
edo:BendingStiffnessStorage rdf:type owl:Class ;
                            rdfs:subClassOf edo:DomainAttribute ;
                            dcterms:accessRights "PUBLIC" ;
                            dcterms:identifier "BendingStiffnessStorage" ;
                            rdfs:comment "Rigidez flexional"@pt-br ;
                            skos:definition "Flexural rigidity"@en ;
                            skos:prefLabel "Bending stiffness, storage"@en ,
                                           "Rigidez flexional, estocagem"@pt-br ;
                            edo:hasAttributeScope edo:TypeLevelAttribute ;
                            edo:hasLifecycleCreationPhase edo:DetailedDesign ;
                            edo:hasTypedValue edo:FloatValue ;
                            edo:hasUnit unit:KiloN-M2 ;
                            edo:hasValueCardinality edo:SingleValue .


###  https://w3id.org/energy-domain/edo#BendingStiffnessTableColumn
edo:BendingStiffnessTableColumn rdf:type owl:Class ;
                                rdfs:subClassOf edo:BendingStiffnessCurveAttribute .


###  https://w3id.org/energy-domain/edo#Biofuels
edo:Biofuels rdf:type owl:Class ;
             rdfs:subClassOf edo:Biomass ;
             dcterms:identifier "Biofuels" ;
             skos:definition "Biocombustíveis são combustíveis líquidos derivados da biomassa, como etanol, biodiesel e combustíveis renováveis avançados. São usados principalmente no setor de transporte como substitutos ou complementos aos combustíveis fósseis."@pt-br ,
                             "Biofuels are liquid fuels derived from biomass, such as bioethanol, biodiesel, and advanced renewable fuels. They are used mainly in the transport sector as a substitute or complement to fossil fuels."@en ;
             skos:prefLabel "Biocombustíveis"@pt-br ,
                            "Biofuels"@en .


###  https://w3id.org/energy-domain/edo#Biogas
edo:Biogas rdf:type owl:Class ;
           rdfs:subClassOf edo:Biomass ;
           dcterms:identifier "Biogas" ;
           skos:definition "Biogas is produced by anaerobic digestion of organic matter such as agricultural residues, sewage, and food waste. It is composed mainly of methane and can be used for electricity, heating, or upgraded to biomethane for injection into gas grids."@en ,
                           "Biogás é produzido pela digestão anaeróbica de matéria orgânica como resíduos agrícolas, esgoto e restos de alimentos. É composto principalmente por metano e pode ser usado para eletricidade, aquecimento ou purificado para biometano injetado em redes de gás."@pt-br ;
           skos:prefLabel "Biogas"@en ,
                          "Biogás"@pt-br .


###  https://w3id.org/energy-domain/edo#Biomass
edo:Biomass rdf:type owl:Class ;
            rdfs:subClassOf edo:Renewable ;
            rdfs:label "Biomass Energy"@en ,
                       "Energia de Biomassa"@pt-br ;
            skos:definition "Energia produzida a partir de materiais orgânicos como madeira, resíduos agrícolas ou lixo."@pt-br ,
                            "Energy produced from organic materials such as wood, agricultural residues, or waste."@en .


###  https://w3id.org/energy-domain/edo#BlockValve
edo:BlockValve rdf:type owl:Class ;
               rdfs:subClassOf edo:ActuatedValve ;
               dcterms:identifier "BlockValve" ;
               skos:definition "An on-off valve, i.e. one which is designed to be either fully open or fully closed"@en ,
                               "Válvula projetada para operar totalmente aberta ou totalmente fechada"@pt-br ;
               skos:prefLabel "Block valve"@en ,
                              "Válvula de bloqueio"@pt-br .


###  https://w3id.org/energy-domain/edo#BoltSet
edo:BoltSet rdf:type owl:Class ;
            rdfs:subClassOf edo:PhysicalConnection ;
            dcterms:identifier "BoltSet" ;
            skos:definition "A collection of bolts and nuts, and washers designed for fastening components in subsea systems. Bolt sets are critical for ensuring structural integrity and are selected based on size, material, and application requirements."@en ;
            skos:prefLabel "Bolt Set"@en ,
                           "Conjunto de Parafusos"@pt-br ;
            edo:hasAttribute edo:AssemblyTorque ,
                             edo:FullyThreaded ,
                             edo:Lubricant ,
                             edo:LubricantFrictionFactor ,
                             edo:NominalLength ,
                             edo:Quantity ,
                             edo:SpareQuantity .


###  https://w3id.org/energy-domain/edo#BooleanValue
edo:BooleanValue rdf:type owl:Class ;
                 owl:equivalentClass [ rdf:type owl:Restriction ;
                                       owl:onProperty rdf:value ;
                                       owl:allValuesFrom xsd:boolean
                                     ] ;
                 rdfs:subClassOf edo:DataType ;
                 rdfs:comment "Constraint for xsd:boolean (true/false)"@en ;
                 rdfs:label "Boolean Value"@en .


###  https://w3id.org/energy-domain/edo#BoreDiameter
edo:BoreDiameter rdf:type owl:Class ;
                 rdfs:subClassOf edo:DomainAttribute ;
                 dcterms:accessRights "PUBLIC" ;
                 dcterms:identifier "BoreDiameter" ;
                 skos:definition "Internal diameter that defines the size of the passage through which fluids or gases can flow. This dimension is essential in industrial piping, as it determines flow capacity and impacts pressure and velocity within the system."@en ;
                 skos:prefLabel "Bore Diameter"@en ,
                                "Diâmetro do Furo"@pt-br ;
                 edo:hasAttributeScope edo:TypeLevelAttribute ;
                 edo:hasLifecycleCreationPhase edo:DetailedDesign ;
                 edo:hasTypedValue edo:FloatValue ;
                 edo:hasUnit unit:MilliM ;
                 edo:hasValueCardinality edo:SingleValue .


###  https://w3id.org/energy-domain/edo#BreakingTension
edo:BreakingTension rdf:type owl:Class ;
                    rdfs:subClassOf edo:DomainAttribute ;
                    dcterms:accessRights "PUBLIC" ;
                    dcterms:identifier "BreakingTension" ;
                    skos:definition "Breaking tension"@en ;
                    skos:prefLabel "Breaking tension"@en ,
                                   "Tensão de ruptura"@pt-br ;
                    edo:hasAttributeScope edo:TypeLevelAttribute ;
                    edo:hasLifecycleCreationPhase edo:DetailedDesign ;
                    edo:hasTypedValue edo:FloatValue ;
                    edo:hasUnit unit:KiloN ;
                    edo:hasValueCardinality edo:SingleValue .


###  https://w3id.org/energy-domain/edo#BsddDataDictionary
edo:BsddDataDictionary rdf:type owl:Class ;
                       rdfs:subClassOf edo:DataDictionary ;
                       dcterms:identifier "BsddDataDictionary"@en ;
                       skos:definition "Representa um tipo especializado de dicionário de dados seguindo o padrão BuildingSMART Data Dictionary (BSDD), fornecendo definições detalhadas, atributos padronizados e classificação para elementos de construção ou sistemas, apoiando modelagem consistente, interoperabilidade e integração semântica."@pt-br ,
                                       "Represents a specialized type of data dictionary following the BuildingSMART Data Dictionary (BSDD) standard, providing detailed definitions, standardized attributes, and classification for building or system elements, supporting consistent modeling, interoperability, and semantic integration."@en ;
                       skos:prefLabel "BSDD Data Dictionary"@en ,
                                      "Dicionário de Dados BSDD"@pt-br .


###  https://w3id.org/energy-domain/edo#BundleDiameter
edo:BundleDiameter rdf:type owl:Class ;
                   rdfs:subClassOf edo:DomainAttribute ;
                   dcterms:accessRights "PUBLIC" ;
                   dcterms:identifier "BundleDiameter" ;
                   skos:prefLabel "Bundle diameter"@en ,
                                  "Diâmetro do feixe"@pt-br ;
                   edo:hasAttributeScope edo:TypeLevelAttribute ;
                   edo:hasLifecycleCreationPhase edo:DetailedDesign ;
                   edo:hasTypedValue edo:FloatValue ;
                   edo:hasValueCardinality edo:SingleValue .


###  https://w3id.org/energy-domain/edo#BuoyancyModule
edo:BuoyancyModule rdf:type owl:Class ;
                   rdfs:subClassOf edo:IfcInstanciableElement ,
                                   edo:LineAncillary ;
                   dcterms:identifier "BuoyancyModule" ;
                   skos:altLabel "Buoyancy Element"@en ,
                                 "Buoyancy Unit"@en ,
                                 "Floatation Module"@en ,
                                 "Subsea Buoyancy Module"@en ;
                   skos:definition "Device used in subsea systems to provide controlled buoyancy to flexible pipes, risers, or umbilicals, reducing the load on the structure and managing the configuration of the line in the water column. The Buoyancy Module is typically composed of syntactic foam or other materials with low density, designed to withstand high external pressures while maintaining its buoyant properties over time. It plays a key role in optimizing the performance and positioning of subsea lines, ensuring they maintain the required shape and depth in dynamic ocean conditions."@en ,
                                   "Dispositivo utilizado em sistemas submarinos para fornecer flutuabilidade controlada a dutos flexíveis, risers ou umbilicais, reduzindo a carga na estrutura e gerenciando a configuração da linha na coluna d'água. O Módulo de Flutuação é tipicamente composto por espuma sintática ou outros materiais de baixa densidade, projetados para suportar altas pressões externas enquanto mantêm suas propriedades de flutuabilidade ao longo do tempo. Ele desempenha um papel fundamental na otimização do desempenho e do posicionamento das linhas subsea, garantindo que mantenham a forma e a profundidade necessárias em condições oceânicas dinâmicas."@pt-br ;
                   skos:prefLabel "Buoyancy Module"@en ,
                                  "Módulo de Flutuação"@pt-br ;
                   edo:hasAttribute edo:FinalBuoyancy ,
                                    edo:InitialBuoyancy ,
                                    edo:LongTermFloatDensity ,
                                    edo:LongTermFloatVolume ,
                                    edo:NominalFloatDensity ,
                                    edo:NominalFloatVolume ,
                                    edo:OuterDiameter ,
                                    edo:PipeMountPosition ,
                                    edo:ShortTermFloatDensity ,
                                    edo:ShortTermFloatVolume ;
                   edo:hasDiscipline edo:SubseaFlexiblePipesEngineering ,
                                     edo:SubseaUmbilicalsEngineering ;
                   edo:ifc_equivalentClass "IfcPipeFitting" ;
                   edo:ifc_objectType "BuoyancyModule" ;
                   edo:ifc_predefinedType "USERDEFINED" .


###  https://w3id.org/energy-domain/edo#BuoyancyTank
edo:BuoyancyTank rdf:type owl:Class ;
                 rdfs:subClassOf edo:SubseaEquipment ;
                 dcterms:identifier "BuoyancyTank" ;
                 skos:prefLabel "Buoyancy tank"@en ,
                                "Tanque de flutuação"@pt-br .


###  https://w3id.org/energy-domain/edo#BurstPressure
edo:BurstPressure rdf:type owl:Class ;
                  rdfs:subClassOf edo:DomainAttribute ;
                  dcterms:accessRights "PUBLIC" ;
                  dcterms:identifier "BurstPressure" ;
                  skos:definition "Burst Pressure"@en ;
                  skos:prefLabel "Burst Pressure"@en ,
                                 "Pressão de estouro"@pt-br ;
                  edo:hasAttributeScope edo:TypeLevelAttribute ;
                  edo:hasLifecycleCreationPhase edo:DetailedDesign ;
                  edo:hasTypedValue edo:FloatValue ;
                  edo:hasUnit unit:MPa ;
                  edo:hasValueCardinality edo:SingleValue .


###  https://w3id.org/energy-domain/edo#CO2VolumePercentage
edo:CO2VolumePercentage rdf:type owl:Class ;
                        rdfs:subClassOf edo:DomainAttribute ;
                        dcterms:accessRights "PUBLIC" ;
                        dcterms:identifier "CO2VolumePercentage" ;
                        skos:definition "Represents the percentage of carbon dioxide (CO2) in the total volume of the fluid or gas mixture within the pipeline. This value is essential for determining the material selection and design considerations for the flexible subsea pipeline, as CO2 can influence corrosion rates and impact the overall integrity and lifespan of the pipeline."@en ;
                        skos:prefLabel "Carbon Dioxide (CO2) Volume Percentage"@en ,
                                       "Porcentagem de Volume de Dióxido de Carbono (CO2)"@pt-br ;
                        edo:hasAttributeScope edo:InstanceLevelAttribute ;
                        edo:hasLifecycleCreationPhase edo:BasicDesign ;
                        edo:hasTypedValue edo:FloatValue ;
                        edo:hasUnit unit:PERCENT ;
                        edo:hasValueCardinality edo:SingleValue .


###  https://w3id.org/energy-domain/edo#CalculatedAbsoluteBurstPressure
edo:CalculatedAbsoluteBurstPressure rdf:type owl:Class ;
                                    rdfs:subClassOf edo:DomainAttribute ;
                                    dcterms:accessRights "PUBLIC" ;
                                    dcterms:identifier "CalculatedAbsoluteBurstPressure" ;
                                    skos:definition "Represents the estimated absolute pressure at which a component or system is expected to fail or rupture. This property is crucial for determining the maximum safe operating pressure, ensuring that the component can withstand internal forces without bursting."@en ;
                                    skos:prefLabel "Calculated Absolute Burst Pressure"@en ,
                                                   "Pressão Absoluta de Ruptura Calculada"@pt-br ;
                                    edo:hasAttributeScope edo:TypeLevelAttribute ;
                                    edo:hasLifecycleCreationPhase edo:DetailedDesign ;
                                    edo:hasTypedValue edo:FloatValue ;
                                    edo:hasUnit unit:PA ;
                                    edo:hasValueCardinality edo:SingleValue .


###  https://w3id.org/energy-domain/edo#CalculatedValue
edo:CalculatedValue rdf:type owl:Class ;
                    rdfs:subClassOf edo:ValueOrigin ;
                    rdfs:comment "Derived from other values."@en ;
                    rdfs:label "Calculado"@pt-br ,
                               "Calculated"@en ;
                    skos:definition "Derivado de outros valores"@pt-br ,
                                    "Derived from other values"@en .


###  https://w3id.org/energy-domain/edo#CarbonManagement
edo:CarbonManagement rdf:type owl:Class ;
                     rdfs:subClassOf edo:Domain ;
                     dcterms:identifier "CarbonManagement" ;
                     skos:definition "Carbon management encompasses the strategies, processes, and technologies used to measure, monitor, reduce, and offset carbon emissions within industrial, energy, and commercial sectors. It aims to minimize the environmental impact of human activities and support decarbonization goals."@en ,
                                     "Gestão de carbono engloba as estratégias, processos e tecnologias utilizados para medir, monitorar, reduzir e compensar as emissões de carbono nos setores industrial, energético e comercial. Tem como objetivo minimizar o impacto ambiental das atividades humanas e apoiar metas de descarbonização."@pt-br ;
                     skos:prefLabel "Carbon Management"@en ,
                                    "Gestão de Carbono"@pt-br .


###  https://w3id.org/energy-domain/edo#CarcassLayer
edo:CarcassLayer rdf:type owl:Class ;
                 rdfs:subClassOf edo:ArmourLayer ;
                 dcterms:identifier "CarcassLayer" ;
                 skos:definition "A reinforcement layer in subsea flexible pipes that provides structural strength and stability. It helps maintain the shape and integrity of the pipe under operational pressure, ensuring the flexibility of the pipe while protecting the internal components. Typically made from metal or polymer materials, it acts as a foundation for the other protective layers."@en ,
                                 "Camada formada por perfis intertravados"@pt-br ;
                 skos:prefLabel "Camada de Carcaça"@pt-br ,
                                "Carcass Layer"@en ;
                 edo:hasAttribute edo:MetallicLayerPitch ,
                                  edo:StressAtDesignPressure .


###  https://w3id.org/energy-domain/edo#CasingHanger
edo:CasingHanger rdf:type owl:Class ;
                 rdfs:subClassOf edo:PressureComponent ;
                 dcterms:identifier "CasingHanger" ;
                 skos:prefLabel "Casing hanger"@en ,
                                "Suspensor de revestimento"@pt-br .


###  https://w3id.org/energy-domain/edo#ChainSegment
edo:ChainSegment rdf:type owl:Class ;
                 rdfs:subClassOf edo:LinearObject ;
                 dcterms:identifier "ChainSegment" ;
                 skos:prefLabel "Chain segment"@en ,
                                "Tramo de corrente"@pt-br .


###  https://w3id.org/energy-domain/edo#CheckValve
edo:CheckValve rdf:type owl:Class ;
               rdfs:subClassOf edo:Valve ;
               dcterms:identifier "CheckValve" ;
               skos:definition "Self-actuated valve designed to allow fluid passage in only one direction"@en ,
                               "Válvula auto-atuada projetada para permitir passagem de fluidos em apenas uma direção"@pt-br ;
               skos:prefLabel "Check Valve"@en ,
                              "Válvula de Retenção"@pt-br .


###  https://w3id.org/energy-domain/edo#ChemicalInjectionUnit
edo:ChemicalInjectionUnit rdf:type owl:Class ;
                          rdfs:subClassOf edo:TopsideEquipment ;
                          dcterms:identifier "ChemicalInjectionUnit" ;
                          skos:definition "Equipamento de superfície para pressurização de produtos químicos para injeção"@pt-br ,
                                          "Topside equipment for pressurization of chemical injection products"@en ;
                          skos:prefLabel "Chemical injection unit"@en ,
                                         "Unidade de injeção de químicos"@pt-br .


###  https://w3id.org/energy-domain/edo#ChokeModule
edo:ChokeModule rdf:type owl:Class ;
                rdfs:subClassOf edo:FlowControlModule ;
                dcterms:identifier "ChokeModule" ;
                skos:definition "Módulo substituível com função principal de restrição ou regulagem de fluxo"@pt-br ,
                                "Replaceable module with flow restriction or regulation functions"@en ;
                skos:prefLabel "Choke module"@en ,
                               "Módulo de choke"@pt-br ;
                edo:hasDiscipline edo:WetChristmasTreesEngineering .


###  https://w3id.org/energy-domain/edo#ChokeValve
edo:ChokeValve rdf:type owl:Class ;
               rdfs:subClassOf edo:ActuatedValve ;
               dcterms:identifier "ChokeValve" ;
               skos:definition "Valve designed to gradually restrict fluid flow, adjusted either manually or automatically by an autonomous control system/loop"@en ,
                               "Válvula projetada para restringir gradualmente a passagem de fluidos, ajustada manualmente ou automaticamente por um sistema/malha de controle autônoma"@pt-br ;
               skos:prefLabel "Choke Valve"@en ,
                              "Válvula de Restrição"@pt-br .


###  https://w3id.org/energy-domain/edo#CivilEngineering
edo:CivilEngineering rdf:type owl:Class ;
                     rdfs:subClassOf edo:TechnicalDiscipline ;
                     rdfs:label "Civil Engineering"@en ,
                                "Engenharia Civil"@pt-br ;
                     skos:definition "Disciplina de engenharia focada no projeto e construção de infraestrutura."@pt-br ,
                                     "Engineering discipline focused on the design and construction of infrastructure."@en .


###  https://w3id.org/energy-domain/edo#CladdingDiameter
edo:CladdingDiameter rdf:type owl:Class ;
                     rdfs:subClassOf edo:DomainAttribute ;
                     dcterms:accessRights "PUBLIC" ;
                     dcterms:identifier "CladdingDiameter" ;
                     skos:definition "Cladding diameter"@en ;
                     skos:prefLabel "Cladding diameter"@en ;
                     edo:hasUnit unit:MicroM .


###  https://w3id.org/energy-domain/edo#ClampInternalDiameter
edo:ClampInternalDiameter rdf:type owl:Class ;
                          rdfs:subClassOf edo:DomainAttribute ;
                          dcterms:accessRights "PUBLIC" ;
                          dcterms:identifier "ClampInternalDiameter" ;
                          skos:definition "Is the clamp internal diameter"@en ;
                          skos:prefLabel "Clamp Internal Diameter"@en ,
                                         "Diâmetro interno do clamp"@pt-br ;
                          edo:hasAttributeScope edo:TypeLevelAttribute ;
                          edo:hasLifecycleCreationPhase edo:DetailedDesign ;
                          edo:hasTypedValue edo:FloatValue ;
                          edo:hasUnit unit:M ;
                          edo:hasValueCardinality edo:SingleValue .


###  https://w3id.org/energy-domain/edo#CntrPntDstnceFrmTermFlange
edo:CntrPntDstnceFrmTermFlange rdf:type owl:Class ;
                               rdfs:subClassOf edo:DomainAttribute ;
                               dcterms:accessRights "PUBLIC" ;
                               dcterms:identifier "CntrPntDstnceFrmTermFlange" ;
                               skos:definition "Distance between the center of the support region and a defined reference flange (e.g., termination flange). This measurement provides spatial positioning for accurate identification and alignment of the support region within the assembly."@en ,
                                               "Distância entre o centro da região de apoio e um flange de referência definido (por exemplo, o flange de terminação). Essa medição fornece a posição espacial para identificação e alinhamento precisos da região de apoio dentro do conjunto."@pt-br ;
                               skos:prefLabel "Center Point Distance from Reference Flange"@en ,
                                              "Distância do Ponto Central ao Flange de Referência"@pt-br ;
                               edo:hasAttributeScope edo:InstanceLevelAttribute ;
                               edo:hasLifecycleCreationPhase edo:DetailedDesign ;
                               edo:hasTypedValue edo:FloatValue ;
                               edo:hasUnit unit:MilliM ;
                               edo:hasValueCardinality edo:SingleValue .


###  https://w3id.org/energy-domain/edo#CollapsePressure
edo:CollapsePressure rdf:type owl:Class ;
                     rdfs:subClassOf edo:DomainAttribute ;
                     dcterms:accessRights "PUBLIC" ;
                     dcterms:identifier "CollapsePressure" ;
                     skos:definition "Collapse Pressure"@en ;
                     skos:prefLabel "Collapse Pressure"@en ,
                                    "Pressão mínima de colapso"@pt-br ;
                     edo:hasAttributeScope edo:TypeLevelAttribute ;
                     edo:hasLifecycleCreationPhase edo:DetailedDesign ;
                     edo:hasTypedValue edo:FloatValue ;
                     edo:hasUnit unit:MPa ;
                     edo:hasValueCardinality edo:SingleValue .


###  https://w3id.org/energy-domain/edo#CollarInternalDiameter
edo:CollarInternalDiameter rdf:type owl:Class ;
                           rdfs:subClassOf edo:DomainAttribute ;
                           dcterms:accessRights "PUBLIC" ;
                           dcterms:identifier "CollarInternalDiameter" ;
                           skos:definition "Inner dimension of the collar, to ensure proper fitting and secure attachment."@en ;
                           skos:prefLabel "Collar Internal Diameter"@en ,
                                          "Diâmetro Interno do Colar"@pt-br ;
                           edo:hasAttributeScope edo:TypeLevelAttribute ;
                           edo:hasLifecycleCreationPhase edo:DetailedDesign ;
                           edo:hasTypedValue edo:FloatValue ;
                           edo:hasUnit unit:MilliM ;
                           edo:hasValueCardinality edo:SingleValue .


###  https://w3id.org/energy-domain/edo#Commissioning
edo:Commissioning rdf:type owl:Class ;
                  rdfs:subClassOf edo:ConstructionPhase ;
                  rdfs:label "Comissionamento"@pt-br ,
                             "Commissioning"@en ;
                  skos:definition "Final testing and handover of the system into operational status."@en ,
                                  "Testes finais e entrega do sistema para status operacional."@pt-br .


###  https://w3id.org/energy-domain/edo#CommissioningActivity
edo:CommissioningActivity rdf:type owl:Class ;
                          rdfs:subClassOf edo:CommissioningElement ;
                          dcterms:identifier "CommissioningActivity" ;
                          skos:prefLabel "Atividade de Comissionamento"@pt-br ,
                                         "Commissioning Activity"@en ;
                          edo:hasAttribute edo:Planned_Start_Timestamp ;
                          edo:ifc_equivalentClass "IfcTask" ;
                          edo:ifc_objectType "Activity" ;
                          edo:ifc_predefinedType "USERDEFINED" .


###  https://w3id.org/energy-domain/edo#CommissioningContract
edo:CommissioningContract rdf:type owl:Class ;
                          rdfs:subClassOf edo:CommissioningElement ;
                          dcterms:identifier "CommissioningContract" ;
                          skos:prefLabel "Commissioning Contract"@en ,
                                         "Contrato de Comissionamento"@pt-br ;
                          edo:ifc_equivalentClass "IfcGroup" ;
                          edo:ifc_objectType "Contract" ;
                          edo:ifc_predefinedType "USERDEFINED" .


###  https://w3id.org/energy-domain/edo#CommissioningDigitalProcessStep
edo:CommissioningDigitalProcessStep rdf:type owl:Class ;
                                    rdfs:subClassOf edo:CommissioningElement ;
                                    dcterms:identifier "CommissioningDigitalProcessStep" ;
                                    skos:prefLabel "Commissioning Digital Process Step"@en ,
                                                   "Passo do Processo Digital"@pt-br ;
                                    edo:ifc_equivalentClass "IfcTask" ;
                                    edo:ifc_objectType "CommissioningDigitalProcessStep" ;
                                    edo:ifc_predefinedType "USERDEFINED" .


###  https://w3id.org/energy-domain/edo#CommissioningElement
edo:CommissioningElement rdf:type owl:Class ;
                         rdfs:subClassOf edo:DomainElement ;
                         dcterms:identifier "CommissioningObject"@en ;
                         skos:definition "Representa elementos físicos ou lógicos utilizados em atividades de comissionamento, como dispositivos temporários, bancadas de teste ou ferramentas de calibração, apoiando processos de teste, validação e preservação."@pt-br ,
                                         "Represents physical or logical elements used during commissioning activities, such as temporary fixtures, test rigs, or calibration tools, supporting testing, validation, and preservation processes."@en ;
                         skos:prefLabel "Commissioning Object"@en ,
                                        "Objeto de Comissionamento"@pt-br .


###  https://w3id.org/energy-domain/edo#CommissioningEvidence
edo:CommissioningEvidence rdf:type owl:Class ;
                          rdfs:subClassOf edo:CommissioningElement ;
                          dcterms:identifier "CommissioningEvidence" ;
                          skos:prefLabel "Commissioning Evidence"@en ,
                                         "Evidência de Comissionamento"@pt-br ;
                          edo:ifc_equivalentClass "IfcDocumentInformation" ;
                          edo:ifc_objectType "CommissioningEvidence" ;
                          edo:ifc_predefinedType "USERDEFINED" .


###  https://w3id.org/energy-domain/edo#CommissioningIssue
edo:CommissioningIssue rdf:type owl:Class ;
                       rdfs:subClassOf edo:CommissioningElement ;
                       dcterms:identifier "CommissioningIssue" ;
                       skos:prefLabel "Commissioning Issue"@en ,
                                      "Pendência de Comissionamento"@pt-br ;
                       edo:ifc_equivalentClass "IfcClassification" ;
                       edo:ifc_objectType "Pendency_Classification" ;
                       edo:ifc_predefinedType "USERDEFINED" .


###  https://w3id.org/energy-domain/edo#CommissioningItemCheck
edo:CommissioningItemCheck rdf:type owl:Class ;
                           rdfs:subClassOf edo:CommissioningElement ;
                           dcterms:identifier "CommissioningItemCheck" ;
                           skos:prefLabel "Commissioning Item Check"@en ,
                                          "Verificação de Item Comissionável"@pt-br ;
                           edo:ifc_equivalentClass "IfcClassificationReference" ;
                           edo:ifc_objectType "FVI" ;
                           edo:ifc_predefinedType "USERDEFINED" .


###  https://w3id.org/energy-domain/edo#CommissioningLoopCheck
edo:CommissioningLoopCheck rdf:type owl:Class ;
                           rdfs:subClassOf edo:CommissioningElement ;
                           dcterms:identifier "CommissioningLoopCheck" ;
                           skos:prefLabel "Commissioning Loop Check"@en ,
                                          "Verificação de Malha"@pt-br ;
                           edo:ifc_equivalentClass "IfcClassificationReference" ;
                           edo:ifc_objectType "FVM" ;
                           edo:ifc_predefinedType "USERDEFINED" .


###  https://w3id.org/energy-domain/edo#CommissioningPerson
edo:CommissioningPerson rdf:type owl:Class ;
                        rdfs:subClassOf edo:CommissioningElement ;
                        dcterms:identifier "CommissioningPerson" ;
                        skos:prefLabel "Commissioning Person"@en ,
                                       "Pessoa"@pt-br ;
                        edo:ifc_equivalentClass "IfcPerson" ;
                        edo:ifc_objectType "CommissioningPerson" ;
                        edo:ifc_predefinedType "USERDEFINED" .


###  https://w3id.org/energy-domain/edo#CommissioningPreservationOrder
edo:CommissioningPreservationOrder rdf:type owl:Class ;
                                   rdfs:subClassOf edo:CommissioningElement ;
                                   dcterms:identifier "CommissioningPreservationOrder" ;
                                   skos:prefLabel "Commissioning Preservation Order"@en ,
                                                  "Ordem de Preservação"@pt-br ;
                                   edo:ifc_equivalentClass "IfcClassificationReference" ;
                                   edo:ifc_objectType "OP" ;
                                   edo:ifc_predefinedType "USERDEFINED" .


###  https://w3id.org/energy-domain/edo#CommissioningProgram
edo:CommissioningProgram rdf:type owl:Class ;
                         rdfs:subClassOf edo:CommissioningElement ;
                         dcterms:identifier "CommissioningProgram" ;
                         skos:prefLabel "Commissioning Program"@en ,
                                        "Programa de Comissionamento"@pt-br ;
                         edo:ifc_equivalentClass "IfcGroup" ;
                         edo:ifc_objectType "Program" ;
                         edo:ifc_predefinedType "USERDEFINED" .


###  https://w3id.org/energy-domain/edo#CommissioningProject
edo:CommissioningProject rdf:type owl:Class ;
                         rdfs:subClassOf edo:CommissioningElement ;
                         dcterms:identifier "CommissioningProject" ;
                         skos:prefLabel "Commissioning Project"@en ,
                                        "Projeto de Comissionamento"@pt-br ;
                         edo:ifc_equivalentClass "IfcProject" ;
                         edo:ifc_objectType "Project" ;
                         edo:ifc_predefinedType "USERDEFINED" .


###  https://w3id.org/energy-domain/edo#CommissioningResponsibleActor
edo:CommissioningResponsibleActor rdf:type owl:Class ;
                                  rdfs:subClassOf edo:CommissioningElement ;
                                  dcterms:identifier "CommissioningResponsibleActor" ;
                                  skos:prefLabel "Ator Responsável"@pt-br ,
                                                 "Commissioning Responsible Actor"@en ;
                                  edo:ifc_equivalentClass "IfcActor" ;
                                  edo:ifc_objectType "CommissioningResponsibleActor" ;
                                  edo:ifc_predefinedType "USERDEFINED" .


###  https://w3id.org/energy-domain/edo#CommissioningResponsibleGroup
edo:CommissioningResponsibleGroup rdf:type owl:Class ;
                                  rdfs:subClassOf edo:CommissioningElement ;
                                  dcterms:identifier "CommissioningResponsibleGroup" ;
                                  skos:prefLabel "Commissioning Responsible Group"@en ,
                                                 "Grupo Responsável"@pt-br ;
                                  edo:ifc_equivalentClass "IfcGroup" ;
                                  edo:ifc_objectType "CommissioningResponsibleGroup" ;
                                  edo:ifc_predefinedType "USERDEFINED" .


###  https://w3id.org/energy-domain/edo#CommissioningTask
edo:CommissioningTask rdf:type owl:Class ;
                      rdfs:subClassOf edo:CommissioningElement ;
                      dcterms:identifier "CommissioningTask" ;
                      skos:prefLabel "Commissioning Task"@en ,
                                     "Tarefa de Comissionamento"@pt-br ;
                      edo:hasAttribute edo:Content ,
                                       edo:Creator ,
                                       edo:CreatorId ,
                                       edo:Timestamp ;
                      edo:ifc_equivalentClass "IfcTask" ;
                      edo:ifc_objectType "Task" ;
                      edo:ifc_predefinedType "USERDEFINED" .


###  https://w3id.org/energy-domain/edo#CompactObject
edo:CompactObject rdf:type owl:Class ;
                  rdfs:subClassOf edo:Asset ;
                  dcterms:identifier "CompactObject" ;
                  rdfs:label "Compact Object"@en ;
                  skos:definition "A mobile physical object, usually manufactured in a standardized manner."@en ,
                                  "Objeto físico móvel, geralmente fabricado de maneira padronizada."@pt-br ;
                  skos:prefLabel "Compact Object"@en ,
                                 "Objeto Compacto"@pt-br ;
                  edo:hasAttribute edo:DimensionsTableColumn ,
                                   edo:Mass .


###  https://w3id.org/energy-domain/edo#Component
edo:Component rdf:type owl:Class ;
              rdfs:subClassOf edo:CompactObject ;
              dcterms:identifier "Component" ;
              skos:definition "Items always found as part of larger objects, with varying levels of complexity."@en ,
                              "Itens sempre encontrados como parte de objetos maiores, com nível variado de complexidade"@pt-br ;
              skos:prefLabel "Component"@en ,
                             "Componente"@pt-br .


###  https://w3id.org/energy-domain/edo#ComponentDevice
edo:ComponentDevice rdf:type owl:Class ;
                    rdfs:subClassOf edo:Component ;
                    dcterms:identifier "ComponentDevice" ;
                    skos:definition "Complex devices incorporated as parts of larger equipment/systems"@en ,
                                    "Dispositivos complexos incorporados como parte de equipamentos/sistemas maiores"@pt-br ;
                    skos:prefLabel "Component Device"@en ,
                                   "Dispositivo Componente"@pt-br ;
                    edo:hasAttribute edo:MaxDepth ,
                                     edo:TemperatureRangeTableColumn .


###  https://w3id.org/energy-domain/edo#ComponentElement
edo:ComponentElement rdf:type owl:Class ;
                     rdfs:subClassOf edo:PartElement ;
                     skos:definition "Representa uma parte física que não é individualmente rastreável, mas pode ser substituída ou montada dentro de um sistema maior, atuando como um componente funcional em vez de um consumível."@pt-br ,
                                     "Represents a physical part that is not individually traceable but can be replaced or assembled within a larger system, serving as a functional component rather than a consumable."@en ;
                     skos:prefLabel "Component Element"@en ,
                                    "Elemento Componente"@pt-br .


###  https://w3id.org/energy-domain/edo#CompositeLayerMaterialType
edo:CompositeLayerMaterialType rdf:type owl:Class ;
                               rdfs:subClassOf edo:DomainAttribute ;
                               dcterms:accessRights "PUBLIC" ;
                               dcterms:identifier "CompositeLayerMaterialType" ;
                               skos:definition "Type of material from which an object is made, allowing for precise documentation and categorisation."@en ;
                               skos:prefLabel "Composite Layer Material Type"@en ,
                                              "Tipo de Material da Camada de Compósito"@pt-br ;
                               edo:hasAttributeScope edo:TypeLevelAttribute ;
                               edo:hasLifecycleCreationPhase edo:DetailedDesign ;
                               edo:hasTypedValue edo:StringValue ;
                               edo:hasValueCardinality edo:SingleValue .


###  https://w3id.org/energy-domain/edo#CompositeMaterial
edo:CompositeMaterial rdf:type owl:Class ;
                      rdfs:subClassOf edo:FlexibleStructureLayerMaterial ,
                                      edo:IfcInstanciableElement ;
                      dcterms:identifier "CompositeMaterial" ;
                      skos:definition "Material composto por dois ou mais componentes distintos, geralmente fibras de reforço e uma matriz, usado na construção de camadas em dutos flexíveis para aplicações subsea. O Material Compósito oferece uma combinação de alta resistência, resistência à corrosão e flexibilidade, tornando-o adequado para suportar as condições severas de ambientes de águas profundas. Seu uso nas camadas do duto flexível melhora a integridade estrutural do duto, resistência à pressão externa e durabilidade sob carregamento cíclico, ao mesmo tempo em que reduz o peso em comparação com materiais metálicos tradicionais."@pt-br ,
                                      "Material made from two or more distinct components, typically reinforcing fibers and a matrix, used in the construction of layers in flexible pipes for subsea applications. The Composite Material offers a combination of high strength, corrosion resistance, and flexibility, making it suitable for withstanding the harsh conditions of deepwater environments. Its use in flexible pipe layers enhances the pipe's structural integrity, resistance to external pressure, and durability under cyclical loading, while also reducing weight compared to traditional metallic materials."@en ;
                      skos:prefLabel "Composite Material"@en ,
                                     "Material Compósito"@pt-br ;
                      edo:hasAttribute edo:CompositeLayerMaterialType ,
                                       edo:RuptDefAlongFibers ,
                                       edo:RuptDefPerpendFibers ,
                                       edo:UltTensStrAlongFibers ,
                                       edo:UltTensStrPerpendFibers ;
                      edo:hasDiscipline edo:SubseaFlexiblePipesEngineering ,
                                        edo:SubseaUmbilicalsEngineering ;
                      edo:ifc_equivalentClass "IfcMaterial" ;
                      edo:ifc_objectType "CompositeMaterial" .


###  https://w3id.org/energy-domain/edo#ConceptualDesign
edo:ConceptualDesign rdf:type owl:Class ;
                     rdfs:subClassOf edo:DesignPhase ;
                     rdfs:label "Conceptual Design"@en ,
                                "Projeto Conceitual"@pt-br ;
                     skos:definition "Fase inicial de projeto focada em viabilidade, definição de escopo e seleção de tecnologia."@pt-br ,
                                     "Initial design phase focused on feasibility, scope definition, and technology selection."@en .


###  https://w3id.org/energy-domain/edo#ConceptualMarker
edo:ConceptualMarker rdf:type owl:Class ;
                     skos:definition "Representa um marcador abstrato usado para marcar ou classificar elementos para fins conceituais ou de manutenção, sem adicionar propriedades físicas ou lógicas."@pt-br ,
                                     "Represents an abstract marker used to tag or classify elements for conceptual or maintenance purposes, without adding physical or logical properties."@en ;
                     skos:prefLabel "Conceptual Marker"@en ,
                                    "Marcador Conceitual"@pt-br .


###  https://w3id.org/energy-domain/edo#ConductorCrossSection
edo:ConductorCrossSection rdf:type owl:Class ;
                          rdfs:subClassOf edo:DomainAttribute ;
                          dcterms:accessRights "PUBLIC" ;
                          dcterms:identifier "ConductorCrossSection" ;
                          rdfs:comment "Área da seção transversal de cada condutor individual"@pt-br ;
                          skos:definition "Cross-sectional area for each individual conductor"@en ;
                          skos:prefLabel "Conductor cross-section"@en ,
                                         "Seção transversal dos condutores"@pt-br ;
                          edo:hasAttributeScope edo:TypeLevelAttribute ;
                          edo:hasLifecycleCreationPhase edo:DetailedDesign ;
                          edo:hasTypedValue edo:FloatValue ;
                          edo:hasUnit unit:MM2 ;
                          edo:hasValueCardinality edo:SingleValue .


###  https://w3id.org/energy-domain/edo#ConnectionModule
edo:ConnectionModule rdf:type owl:Class ;
                     rdfs:subClassOf edo:LineTerminationModule ;
                     dcterms:identifier "ConnectionModule" ;
                     skos:definition "Equipamento de terminação de linha que permite sua ancoragem e conexão a um hub correspondente"@pt-br ,
                                     "Line termination equipment enabling anchoring and connection to a matching hub"@en ;
                     skos:prefLabel "Connection module"@en ,
                                    "Módulo de conexão"@pt-br .


###  https://w3id.org/energy-domain/edo#ConnectionPoint
edo:ConnectionPoint rdf:type owl:Class ;
                    rdfs:subClassOf edo:LogicalElement ;
                    dcterms:identifier "ConnectionPoint" ;
                    skos:definition "Representa um ponto utilizado para estabelecer conexão entre elementos, seja fisicamente ou logicamente."@pt-br ,
                                    "Represents a point used to establish a connection between elements, either physically or logically."@en ;
                    skos:prefLabel "Connection Point"@en ,
                                   "Ponto de Conexão"@pt-br .


###  https://w3id.org/energy-domain/edo#Connector
edo:Connector rdf:type owl:Class ;
              rdfs:subClassOf edo:ComponentDevice ;
              dcterms:identifier "Connector" ;
              skos:definition "Representa um componente físico usado para unir, ligar ou interligar dois ou mais elementos, permitindo conexão mecânica, elétrica ou de fluido."@pt-br ,
                              "Represents a physical component used to join, link, or interface two or more elements, enabling mechanical, electrical, or fluid connection."@en ;
              skos:prefLabel "Conector"@pt-br ,
                             "Connector"@en .


###  https://w3id.org/energy-domain/edo#ConstructionPhase
edo:ConstructionPhase rdf:type owl:Class ;
                      rdfs:subClassOf edo:LifecyclePhase ;
                      rdfs:label "Construction Phase"@en ,
                                 "Fase de Construção"@pt-br .


###  https://w3id.org/energy-domain/edo#ConsumableElement
edo:ConsumableElement rdf:type owl:Class ;
                      rdfs:subClassOf edo:PartElement ;
                      skos:definition "Physical, non-traceable, and replaceable elements. They typically correspond to items that are consumed, depleted, or exchanged during the lifecycle of a project or asset, without requiring individual identification or tracking. The purpose of this class is to distinguish such elements from assets that are uniquely traceable and from components that are permanently integrated, ensuring clarity in modeling and maintenance processes."@en ,
                                      "Representa elementos físicos, não rastreáveis e substituíveis. Normalmente correspondem a itens que são consumidos, desgastados ou trocados ao longo do ciclo de vida de um projeto ou ativo, sem necessidade de identificação ou rastreamento individual. O propósito dessa categoria é diferenciá-los de ativos que são rastreáveis de forma única e de componentes que são permanentemente integrados, garantindo clareza nos processos de modelagem e manutenção."@pt-br ;
                      skos:prefLabel "Consumable Element"@en ,
                                     "Elemento Consumível"@pt-br .


###  https://w3id.org/energy-domain/edo#Content
edo:Content rdf:type owl:Class ;
            rdfs:subClassOf edo:ContentManagementAttribute ;
            dcterms:accessRights "PUBLIC" ;
            dcterms:identifier "Content" ;
            skos:definition "Text field for capturing observations, notes, or details related to the work. It allows for unstructured information to be recorded."@en ;
            skos:prefLabel "Content"@en ;
            edo:hasAttributeScope edo:InstanceLevelAttribute ;
            edo:hasTypedValue edo:StringValue ;
            edo:hasValueCardinality edo:SingleValue .


###  https://w3id.org/energy-domain/edo#ContentManagementAttribute
edo:ContentManagementAttribute rdf:type owl:Class ;
                               rdfs:subClassOf edo:AdministrativeAttribute .


###  https://w3id.org/energy-domain/edo#ControlAndSignalLogic
edo:ControlAndSignalLogic rdf:type owl:Class ;
                          rdfs:subClassOf edo:LogicalElement ;
                          dcterms:identifier "ControlAndSignalLogic" ;
                          skos:definition "Representa elementos que implementam lógica de controle ou sinal dentro de um sistema, definindo comportamentos e relações entre componentes."@pt-br ,
                                          "Represents elements that implement control or signal logic within a system, defining behaviors and relationships between components."@en ;
                          skos:prefLabel "Control and Signal Logic"@en ,
                                         "Lógica de Controle e Sinal"@pt-br .


###  https://w3id.org/energy-domain/edo#ControlLoop
edo:ControlLoop rdf:type owl:Class ;
                rdfs:subClassOf edo:ControlAndSignalLogic ;
                dcterms:identifier "ControlLoop" ;
                skos:definition "Representa um loop de controle que implementa lógica automatizada, incluindo mecanismos de feedback e regulação."@pt-br ,
                                "Represents a control loop implementing automated control logic, including feedback and regulation mechanisms."@en ;
                skos:prefLabel "Control Loop"@en ,
                               "Loop de Controle"@pt-br .


###  https://w3id.org/energy-domain/edo#CoreDiameter
edo:CoreDiameter rdf:type owl:Class ;
                 rdfs:subClassOf edo:DomainAttribute ;
                 dcterms:accessRights "PUBLIC" ;
                 dcterms:identifier "CoreDiameter" ;
                 skos:definition "Core diameter"@en ;
                 skos:prefLabel "Core diameter"@en ;
                 edo:hasUnit unit:MicroM .


###  https://w3id.org/energy-domain/edo#Coupling
edo:Coupling rdf:type owl:Class ;
             rdfs:subClassOf edo:HardwareItem ;
             dcterms:identifier "Coupling" ;
             skos:definition "Base class for termination components of cables, hoses, etc., enabling connection to other components or systems."@en ,
                             "Classe-base para componentes de terminação de cabos, mangueiras, etc., permitindo conexão a outros componentes ou sistemas."@pt-br ;
             skos:prefLabel "Acoplamento"@pt-br ,
                            "Coupling"@en ;
             edo:hasAttribute edo:TemperatureRangeTableColumn .


###  https://w3id.org/energy-domain/edo#Creator
edo:Creator rdf:type owl:Class ;
            rdfs:subClassOf edo:ProvenanceAttribute ;
            dcterms:accessRights "PUBLIC" ;
            dcterms:identifier "Creator" ;
            skos:prefLabel "Creator"@en ;
            edo:hasAttributeScope edo:InstanceLevelAttribute ;
            edo:hasTypedValue edo:StringValue ;
            edo:hasValueCardinality edo:SingleValue .


###  https://w3id.org/energy-domain/edo#CreatorId
edo:CreatorId rdf:type owl:Class ;
              rdfs:subClassOf edo:ProvenanceAttribute ;
              dcterms:accessRights "PUBLIC" ;
              dcterms:identifier "CreatorId" ;
              skos:prefLabel "Creator Id"@en ;
              edo:hasAttributeScope edo:InstanceLevelAttribute ;
              edo:hasTypedValue edo:StringValue ;
              edo:hasValueCardinality edo:SingleValue .


###  https://w3id.org/energy-domain/edo#CriticalCurvatureOfSlipping
edo:CriticalCurvatureOfSlipping rdf:type owl:Class ;
                                rdfs:subClassOf edo:BendingStiffnessCurveAttribute ,
                                                edo:DomainAttribute ;
                                dcterms:accessRights "PUBLIC" ;
                                dcterms:identifier "CriticalCurvatureOfSlipping" ;
                                skos:definition "Represents the minimum curvature at which slipping or movement between layers or components begins to occur. This property is essential for assessing the flexibility and mechanical behavior of the structure, ensuring that it can maintain stability and performance under bending without experiencing slippage."@en ;
                                skos:prefLabel "Critical Curvature Of Slipping"@en ,
                                               "Curvatura crítica de escorregamento"@pt-br ;
                                edo:hasAttributeScope edo:TypeLevelAttribute ;
                                edo:hasLifecycleCreationPhase edo:DetailedDesign ;
                                edo:hasTypedValue edo:FloatValue ;
                                edo:hasUnit unit:PER-M ;
                                edo:hasValueCardinality edo:SingleValue .


###  https://w3id.org/energy-domain/edo#CrossoverModule
edo:CrossoverModule rdf:type owl:Class ;
                    rdfs:subClassOf edo:FlowControlModule ;
                    dcterms:identifier "CrossoverModule" ;
                    skos:definition "Módulo substituível que permite fechamento de um circuito de fluxo"@pt-br ,
                                    "Replaceable module that enables closure of a flow circuit"@en ;
                    skos:prefLabel "Cross-over module"@en ,
                                   "Módulo de cross-over"@pt-br ;
                    edo:hasDiscipline edo:WetChristmasTreesEngineering .


###  https://w3id.org/energy-domain/edo#CrushingCurveAttribute
edo:CrushingCurveAttribute rdf:type owl:Class ;
                           rdfs:subClassOf edo:DomainAttribute .


###  https://w3id.org/energy-domain/edo#CrushingFrictionCoefficientTighteningAttribute
edo:CrushingFrictionCoefficientTighteningAttribute rdf:type owl:Class ;
                                                   rdfs:subClassOf edo:CrushingCurveAttribute .


###  https://w3id.org/energy-domain/edo#CrushingFrictionCoefficientTighteningTableColumn
edo:CrushingFrictionCoefficientTighteningTableColumn rdf:type owl:Class ;
                                                     rdfs:subClassOf edo:CrushingFrictionCoefficientTighteningAttribute .


###  https://w3id.org/energy-domain/edo#CrushingLoad
edo:CrushingLoad rdf:type owl:Class ;
                 rdfs:subClassOf edo:DomainAttribute ;
                 dcterms:accessRights "PUBLIC" ;
                 dcterms:identifier "CrushingLoad" ;
                 rdfs:comment "Carga máxima de compressão para cada sapata do tensionador"@pt-br ;
                 skos:definition "Maximum compressive load for each tensioner pad"@en ;
                 skos:prefLabel "Carga de esmagamento"@pt-br ,
                                "Crushing load"@en ;
                 edo:hasAttributeScope edo:TypeLevelAttribute ;
                 edo:hasLifecycleCreationPhase edo:DetailedDesign ;
                 edo:hasTypedValue edo:FloatValue ;
                 edo:hasUnit unit:KiloN-PER-M ;
                 edo:hasValueCardinality edo:SingleValue .


###  https://w3id.org/energy-domain/edo#CrushingMaximumAllowableTensionAttribute
edo:CrushingMaximumAllowableTensionAttribute rdf:type owl:Class ;
                                             rdfs:subClassOf edo:CrushingCurveAttribute .


###  https://w3id.org/energy-domain/edo#CrushingMaximumAllowableTensionTableColumn
edo:CrushingMaximumAllowableTensionTableColumn rdf:type owl:Class ;
                                               rdfs:subClassOf edo:CrushingMaximumAllowableTensionAttribute .


###  https://w3id.org/energy-domain/edo#CrushingMaximumAllowableTighteningAttribute
edo:CrushingMaximumAllowableTighteningAttribute rdf:type owl:Class ;
                                                rdfs:subClassOf edo:CrushingCurveAttribute .


###  https://w3id.org/energy-domain/edo#CrushingMaximumAllowableTighteningTableColumn
edo:CrushingMaximumAllowableTighteningTableColumn rdf:type owl:Class ;
                                                  rdfs:subClassOf edo:CrushingMaximumAllowableTighteningAttribute .


###  https://w3id.org/energy-domain/edo#DamagingPullInStraightLine
edo:DamagingPullInStraightLine rdf:type owl:Class ;
                               rdfs:subClassOf edo:DomainAttribute ;
                               dcterms:accessRights "PUBLIC" ;
                               dcterms:identifier "DamagingPullInStraightLine" ;
                               skos:definition "Represents the force applied during a straight-line pull-in operation that could cause damage to a component or system. This property is critical for determining safe operational limits during installation, ensuring that the component can withstand the pulling force without suffering structural damage."@en ;
                               skos:prefLabel "Damaging Pull-In Straight Line"@en ,
                                              "Tração Crítica em Linha Reta"@pt-br ;
                               edo:hasAttributeScope edo:TypeLevelAttribute ;
                               edo:hasLifecycleCreationPhase edo:DetailedDesign ;
                               edo:hasTypedValue edo:FloatValue ;
                               edo:hasUnit unit:N ;
                               edo:hasValueCardinality edo:SingleValue .


###  https://w3id.org/energy-domain/edo#DamagingTension
edo:DamagingTension rdf:type owl:Class ;
                    rdfs:subClassOf edo:DomainAttribute ;
                    dcterms:accessRights "PUBLIC" ;
                    dcterms:identifier "DamagingTension" ;
                    skos:definition "Damaging tension, straight"@en ;
                    skos:prefLabel "Damaging tension, straight"@en ,
                                   "Tensão de dano, reto"@pt-br ;
                    edo:hasUnit unit:KiloN .


###  https://w3id.org/energy-domain/edo#DataDictionary
edo:DataDictionary rdf:type owl:Class ;
                   rdfs:subClassOf edo:ExternalReference ;
                   dcterms:identifier "DataDictionary"@en ;
                   skos:definition "Representa uma coleção estruturada de definições, atributos e regras que fornecem uma referência padronizada para elementos dentro de um projeto ou sistema."@pt-br ,
                                   "Represents a structured collection of definitions, attributes, and rules that provide a standardized reference for elements within a project or system."@en ;
                   skos:prefLabel "Data Dictionary"@en ,
                                  "Dicionário de Dados"@pt-br .


###  https://w3id.org/energy-domain/edo#DataPort
edo:DataPort rdf:type owl:Class ;
             rdfs:subClassOf edo:Port ;
             dcterms:identifier "DataPort" ;
             skos:definition "Representa uma porta que permite a troca de dados ou sinais entre elementos."@pt-br ,
                             "Represents a port that allows the exchange of data or signals between elements."@en ;
             skos:prefLabel "Data Port"@en ,
                            "Porta de Dados"@pt-br .


###  https://w3id.org/energy-domain/edo#DataType
edo:DataType rdf:type owl:Class ;
             rdfs:subClassOf edo:ValueNature ;
             rdfs:comment "Superclass for values constrained to a specific XSD datatype."@en ;
             rdfs:label "Typed Value"@en .


###  https://w3id.org/energy-domain/edo#DateTimeValue
edo:DateTimeValue rdf:type owl:Class ;
                  owl:equivalentClass [ rdf:type owl:Restriction ;
                                        owl:onProperty rdf:value ;
                                        owl:allValuesFrom xsd:dateTime
                                      ] ;
                  rdfs:subClassOf edo:DataType ;
                  rdfs:comment "Constraint for xsd:dateTime (timestamps)"@en ;
                  rdfs:label "DateTime Value"@en .


###  https://w3id.org/energy-domain/edo#DateValue
edo:DateValue rdf:type owl:Class ;
              owl:equivalentClass [ rdf:type owl:Restriction ;
                                    owl:onProperty rdf:value ;
                                    owl:allValuesFrom xsd:date
                                  ] ;
              rdfs:subClassOf edo:DataType ;
              rdfs:comment "Constraint for xsd:date (calendar dates)"@en ;
              rdfs:label "Date Value"@en .


###  https://w3id.org/energy-domain/edo#DeadweightCollar
edo:DeadweightCollar rdf:type owl:Class ;
                     rdfs:subClassOf edo:IfcInstanciableElement ,
                                     edo:SplitCollar ;
                     dcterms:identifier "DeadweightCollar" ;
                     skos:altLabel "Ballast Collar"@en ,
                                   "Dead Weight Clamp"@en ,
                                   "Sinking Collar"@en ,
                                   "Weight Collar"@en ;
                     skos:definition "Component used in subsea systems to provide additional weight to flexible pipes, risers, or umbilicals, ensuring proper stability and positioning on the seabed. The Deadweight Collar is designed to counteract buoyant forces, preventing unwanted movement of the pipe due to ocean currents or other environmental factors. Typically made from dense materials, it plays a crucial role in maintaining the alignment and stability of lines in dynamic environments, ensuring that the system remains securely anchored."@en ,
                                     "Componente utilizado em sistemas submersos para fornecer peso adicional a dutos flexíveis, risers ou umbilicais, garantindo a estabilidade e o posicionamento adequados no fundo marinho. O Colar de Peso Morto é projetado para contrabalançar as forças de flutuabilidade, prevenindo o movimento indesejado do duto devido a correntes oceânicas ou outros fatores ambientais. Geralmente feito de materiais densos, ele desempenha um papel crucial na manutenção do alinhamento e da estabilidade das linhas submersas em ambientes dinâmicos, garantindo que o sistema permaneça firmemente ancorado."@pt-br ;
                     skos:prefLabel "Colar de Peso Morto"@pt-br ,
                                    "Deadweight Collar"@en ;
                     edo:hasDiscipline edo:SubseaFlexiblePipesEngineering ,
                                       edo:SubseaUmbilicalsEngineering ;
                     edo:ifc_equivalentClass "IfcPipeFitting" ;
                     edo:ifc_objectType "DeadweightCollar" ;
                     edo:ifc_predefinedType "USERDEFINED" .


###  https://w3id.org/energy-domain/edo#DecimalValue
edo:DecimalValue rdf:type owl:Class ;
                 owl:equivalentClass [ rdf:type owl:Restriction ;
                                       owl:onProperty rdf:value ;
                                       owl:allValuesFrom xsd:decimal
                                     ] ;
                 rdfs:subClassOf edo:DataType ;
                 rdfs:comment "Constraint for xsd:decimal (arbitrary precision numbers)"@en ;
                 rdfs:label "Decimal Value"@en .


###  https://w3id.org/energy-domain/edo#DeclaredValue
edo:DeclaredValue rdf:type owl:Class ;
                  rdfs:subClassOf edo:ValueOrigin ;
                  rdfs:comment "Manually specified value."@en ;
                  rdfs:label "Declarado"@pt-br ,
                             "Declared"@en ;
                  skos:definition "Manually specified value"@en ,
                                  "Valor especificado manualmente"@pt-br .


###  https://w3id.org/energy-domain/edo#Decommissioning
edo:Decommissioning rdf:type owl:Class ;
                    rdfs:subClassOf edo:DecommissioningPhase ;
                    rdfs:label "Decommissioning"@en ,
                               "Descomissionamento"@pt-br ;
                    skos:definition "Permanent removal of the asset from service, including dismantling and disposal."@en ,
                                    "Remoção permanente do ativo do serviço, incluindo desmontagem e descarte."@pt-br .


###  https://w3id.org/energy-domain/edo#DecommissioningPhase
edo:DecommissioningPhase rdf:type owl:Class ;
                         rdfs:subClassOf edo:LifecyclePhase ;
                         rdfs:label "Decommissioning Phase"@en ,
                                    "Fase de Descomissionamento"@pt-br .


###  https://w3id.org/energy-domain/edo#DeploymentAccessory
edo:DeploymentAccessory rdf:type owl:Class ;
                        rdfs:subClassOf edo:Accessory ;
                        dcterms:identifier "DeploymentAccessory" ;
                        skos:prefLabel "Acessório de lançamento"@pt-br ,
                                       "Deployment accessory"@en .


###  https://w3id.org/energy-domain/edo#DesignConditionAttribute
edo:DesignConditionAttribute rdf:type owl:Class ;
                             rdfs:subClassOf edo:FunctionalAttribute .


###  https://w3id.org/energy-domain/edo#DesignLifeSpan
edo:DesignLifeSpan rdf:type owl:Class ;
                   rdfs:subClassOf edo:DomainAttribute ;
                   dcterms:accessRights "PUBLIC" ;
                   dcterms:identifier "DesignLifeSpan" ;
                   skos:definition "Design life span"@en ;
                   skos:prefLabel "Design life span"@en ,
                                  "Vida útil de projeto"@pt-br ;
                   edo:hasAttributeScope edo:TypeLevelAttribute ;
                   edo:hasLifecycleCreationPhase edo:DetailedDesign ;
                   edo:hasTypedValue edo:FloatValue ;
                   edo:hasUnit unit:YR_Common ;
                   edo:hasValueCardinality edo:SingleValue .


###  https://w3id.org/energy-domain/edo#DesignPhase
edo:DesignPhase rdf:type owl:Class ;
                rdfs:subClassOf edo:LifecyclePhase ;
                rdfs:label "Design Phase"@en ,
                           "Fase de Projeto"@pt-br .


###  https://w3id.org/energy-domain/edo#DestinationPigtailLength
edo:DestinationPigtailLength rdf:type owl:Class ;
                             rdfs:subClassOf edo:DomainAttribute ;
                             dcterms:accessRights "PUBLIC" ;
                             dcterms:identifier "DestinationPigtailLength" ;
                             skos:definition "Destination end pigtail length"@en ;
                             skos:prefLabel "Destination end pigtail length"@en ;
                             edo:hasAttributeScope edo:TypeLevelAttribute ;
                             edo:hasLifecycleCreationPhase edo:DetailedDesign ;
                             edo:hasTypedValue edo:FloatValue ;
                             edo:hasUnit unit:MilliM ;
                             edo:hasValueCardinality edo:SingleValue .


###  https://w3id.org/energy-domain/edo#DetailedDesign
edo:DetailedDesign rdf:type owl:Class ;
                   rdfs:subClassOf edo:DesignPhase ;
                   rdfs:label "Detailed Design"@en ,
                              "Projeto Detalhado"@pt-br ;
                   skos:definition "Comprehensive engineering phase producing detailed drawings, material specifications, and construction plans."@en ,
                                   "Fase abrangente de engenharia que produz desenhos detalhados, especificações de materiais e planos de construção."@pt-br .


###  https://w3id.org/energy-domain/edo#DiffusionCurveAttribute
edo:DiffusionCurveAttribute rdf:type owl:Class ;
                            rdfs:subClassOf edo:DomainAttribute .


###  https://w3id.org/energy-domain/edo#DiffusionTableColumn
edo:DiffusionTableColumn rdf:type owl:Class ;
                         rdfs:subClassOf edo:DiffusionCurveAttribute ;
                         dcterms:accessRights "PUBLIC" ;
                         dcterms:identifier "DiffusionTable" ;
                         skos:definition "Difusão (Específica para Materiais Poliméricos)"@pt-br ,
                                         "Provides data on the diffusion rates of substances through materials, used to assess how different fluids or gases permeate the structure over time. This information is crucial for evaluating material suitability and predicting long-term performance under specific environmental conditions."@en ;
                         skos:prefLabel "Diffusion Table"@en ,
                                        "Tabela de Difusão"@pt-br ;
                         edo:hasAttributeScope edo:TypeLevelAttribute .


###  https://w3id.org/energy-domain/edo#DiffusionTable_DiffusionCoefficient
edo:DiffusionTable_DiffusionCoefficient rdf:type owl:Class ;
                                        rdfs:subClassOf edo:DiffusionTableColumn ;
                                        dcterms:accessRights "PUBLIC" ;
                                        dcterms:identifier "DiffusionTable_DiffusionCoefficient" ;
                                        skos:definition "Represents the rate at which particles, molecules, or substances diffuse through a material. This property is important for evaluating how gases or liquids move within or through a material, helping to understand the behavior of the component, where diffusion can affect performance and integrity."@en ;
                                        skos:prefLabel "Coeficiente de difusão"@pt-br ,
                                                       "Diffusion Coefficient"@en ;
                                        edo:hasAttributeScope edo:TypeLevelAttribute ;
                                        edo:hasLifecycleCreationPhase edo:DetailedDesign ;
                                        edo:hasTypedValue edo:FloatValue ;
                                        edo:hasUnit unit:M2-PER-SEC ;
                                        edo:hasValueCardinality edo:MultiValue .


###  https://w3id.org/energy-domain/edo#DiffusionTable_MoleculeIdentifier
edo:DiffusionTable_MoleculeIdentifier rdf:type owl:Class ;
                                      rdfs:subClassOf edo:DiffusionTableColumn ;
                                      dcterms:accessRights "PUBLIC" ;
                                      dcterms:identifier "DiffusionTable_MoleculeIdentifier" ;
                                      skos:definition "Specifies the type of molecule. This property identifies the particular molecule involved, which is crucial for understanding the material's interaction with or response to different chemical substances."@en ,
                                                      "Tipo de Molécula (co2, h2s, ch4, h2o,…)"@pt-br ;
                                      skos:prefLabel "Identificador de Molécula"@pt-br ,
                                                     "Molecule Identifier"@en ;
                                      edo:hasAttributeScope edo:TypeLevelAttribute ;
                                      edo:hasLifecycleCreationPhase edo:DetailedDesign ;
                                      edo:hasTypedValue edo:StringValue ;
                                      edo:hasValueCardinality edo:MultiValue .


###  https://w3id.org/energy-domain/edo#DiffusionTable_PolymerState
edo:DiffusionTable_PolymerState rdf:type owl:Class ;
                                rdfs:subClassOf edo:DiffusionTableColumn ;
                                dcterms:accessRights "PUBLIC" ;
                                dcterms:identifier "DiffusionTable_PolymerState" ;
                                skos:definition "The state of the polymeric material is specified.. This property is crucial for understanding how the material behaves under different conditions and its suitability for various applications."@en ,
                                                "estado do polímero (plastificado, não plastificado,…)"@pt-br ;
                                skos:prefLabel "Estado do Polímero"@pt-br ,
                                               "Polymer State"@en ;
                                edo:hasAttributeScope edo:TypeLevelAttribute ;
                                edo:hasLifecycleCreationPhase edo:DetailedDesign ;
                                edo:hasTypedValue edo:StringValue ;
                                edo:hasValueCardinality edo:MultiValue .


###  https://w3id.org/energy-domain/edo#DiffusionTable_Temperature
edo:DiffusionTable_Temperature rdf:type owl:Class ;
                               rdfs:subClassOf edo:DiffusionTableColumn ;
                               dcterms:accessRights "PUBLIC" ;
                               dcterms:identifier "DiffusionTable_Temperature" ;
                               skos:definition "Represents the thermal condition or measurement of heat for a component or system. This property is important for assessing how the component performs or operates under specific thermal conditions, ensuring it remains within safe and effective operating limits."@en ;
                               skos:prefLabel "Temperatura"@pt-br ,
                                              "Temperature"@en ;
                               edo:hasAttributeScope edo:TypeLevelAttribute ;
                               edo:hasLifecycleCreationPhase edo:DetailedDesign ;
                               edo:hasTypedValue edo:FloatValue ;
                               edo:hasUnit unit:K ;
                               edo:hasValueCardinality edo:MultiValue .


###  https://w3id.org/energy-domain/edo#DimensionalAttribute
edo:DimensionalAttribute rdf:type owl:Class ;
                         rdfs:subClassOf edo:AttributeDomainCategory ;
                         rdfs:comment "Represents measurements such as length, diameter, volume."@en ;
                         rdfs:label "Atributo Dimensional"@pt-br ,
                                    "Dimensional Attribute"@en ;
                         skos:definition "Representa medições como comprimento, diâmetro, volume"@pt-br ,
                                         "Represents measurements such as length, diameter, volume"@en .


###  https://w3id.org/energy-domain/edo#DimensioningCriteria
edo:DimensioningCriteria rdf:type owl:Class ;
                         rdfs:subClassOf edo:LayingMinimumRadiusCurveAttribute ;
                         dcterms:accessRights "PUBLIC" ;
                         dcterms:identifier "DimensioningCriteria" ;
                         skos:definition "Critério de dimensionamento de raio mínimo de lançamento. Lista pré definida:Linear interpolation (curvature)Most restrictive value between the neighbouring values"@pt-br ,
                                         "Specifies the criteria used to determine the dimensions, providing guidelines and standards for accurate sizing and ensuring that the structure meets required performance and safety specifications."@en ;
                         skos:prefLabel "Critério de Dimensionamento"@pt-br ,
                                        "Dimensioning Criteria"@en ;
                         edo:hasAttributeScope edo:TypeLevelAttribute ;
                         edo:hasLifecycleCreationPhase edo:DetailedDesign ;
                         edo:hasTypedValue edo:StringValue ;
                         edo:hasValueCardinality edo:SingleValue .


###  https://w3id.org/energy-domain/edo#DimensionsDrawing
edo:DimensionsDrawing rdf:type owl:Class ;
                      rdfs:subClassOf edo:IfcInstanciableElement ,
                                      edo:ReferenceDocument ;
                      dcterms:identifier "DimensionsDrawing" ;
                      skos:definition "Desenho técnico que fornece medições detalhadas, especificações geométricas e dados angulares dos componentes utilizados. O Desenho de Cotas inclui informações críticas como comprimento, diâmetro, espessura e ângulos, garantindo a fabricação, montagem e instalação precisas das peças. Esse desenho é essencial para atender aos requisitos de projeto e garantir que todos os componentes se encaixem corretamente no sistema como um todo, apoiando a fabricação eficiente e o controle de qualidade."@pt-br ,
                                      "Technical drawing providing detailed measurements, geometric specifications, and angular data of components. The Dimensions Drawing includes critical information such as length, diameter, thickness, and angles, ensuring the precise fabrication, assembly, and installation of the parts. This drawing is essential for meeting design requirements and ensuring that all components fit accurately within the overall system, supporting efficient manufacturing and quality control."@en ;
                      skos:prefLabel "Desenho de Cotas"@pt-br ,
                                     "Dimensions Drawing"@en ;
                      edo:hasDiscipline edo:SubseaUmbilicalsEngineering ;
                      edo:ifc_equivalentClass "IfcDocumentInformation" ;
                      edo:ifc_objectType "DimensionsDrawing" .


###  https://w3id.org/energy-domain/edo#DimensionsTableColumn
edo:DimensionsTableColumn rdf:type owl:Class ;
                          rdfs:subClassOf edo:DrawingDimensionsTableAttribute .


###  https://w3id.org/energy-domain/edo#DisplacedVolume
edo:DisplacedVolume rdf:type owl:Class ;
                    rdfs:subClassOf edo:DomainAttribute ;
                    dcterms:accessRights "PUBLIC" ;
                    dcterms:identifier "DisplacedVolume" ;
                    skos:definition "Refers to the total volume of an object that is submerged or immersed in a fluid. This volume is used to calculate the buoyant force acting on the object and is crucial for understanding its buoyancy and stability in the fluid."@en ;
                    skos:prefLabel "Displaced Volume"@en ,
                                   "Volume Deslocado"@pt-br ;
                    edo:hasAttributeScope edo:TypeLevelAttribute ;
                    edo:hasLifecycleCreationPhase edo:DetailedDesign ;
                    edo:hasTypedValue edo:FloatValue ;
                    edo:hasUnit unit:M3 ,
                                edo:M3 ;
                    edo:hasValueCardinality edo:SingleValue .


###  https://w3id.org/energy-domain/edo#DistributionModule
edo:DistributionModule rdf:type owl:Class ;
                       rdfs:subClassOf edo:AuxiliaryModule ;
                       dcterms:identifier "DistributionModule" ;
                       skos:definition "Sub-module of larger equipment for distribution of hydraulic, chemical, electrical, etc. functions"@en ,
                                       "Sub-módulo de um equipamento maior para distribuição de funções hidráulicas, químicas, elétricas, etc."@pt-br ;
                       skos:prefLabel "Distribution module"@en ,
                                      "Módulo de distribuição"@pt-br .


###  https://w3id.org/energy-domain/edo#Domain
edo:Domain rdf:type owl:Class ;
           rdfs:subClassOf edo:ElementClassification ;
           rdfs:comment "Represents a high-level industrial domain, such as Oil & Gas, Nuclear, or Renewable Energy."@en ;
           rdfs:label "Domínio Industrial"@pt-br ,
                      "Industrial Domain"@en ;
           skos:definition "A high-level industrial sector or application area."@en ,
                           "Um setor industrial ou área de aplicação de alto nível."@pt-br .


###  https://w3id.org/energy-domain/edo#DomainAttribute
edo:DomainAttribute rdf:type owl:Class ;
                    skos:definition "Representa uma propriedade ou característica que pode ser atribuída a elementos de domínio, capturando informações específicas relevantes para seu projeto, função ou gestão."@pt-br ,
                                    "Represents a property or characteristic that can be assigned to domain elements, capturing specific information relevant to their design, function, or management."@en ;
                    skos:prefLabel "Atributo de Domínio"@pt-br ,
                                   "Domain Attribute"@en .


###  https://w3id.org/energy-domain/edo#DomainClassification
edo:DomainClassification rdf:type owl:Class ;
                         rdfs:label "Classificação de Domínio"@pt-br ,
                                    "Domain Classification"@en ;
                         skos:definition "Representa um esquema para organizar elementos e atributos de domínio em categorias, facilitando a classificação, recuperação e gestão consistente da informação."@pt-br ,
                                         "Represents a scheme for organizing domain elements and attributes into categories, facilitating consistent classification, retrieval, and management of information."@en ;
                         skos:prefLabel "Classificação de Domínio"@pt-br ,
                                        "Domain Classification"@en .


###  https://w3id.org/energy-domain/edo#DomainElement
edo:DomainElement rdf:type owl:Class ;
                  skos:definition "Representa um bloco fundamental de um projeto ou sistema, abrangendo entidades físicas, lógicas ou informacionais que podem ser modeladas, especificadas ou referenciadas."@pt-br ,
                                  "Represents a fundamental building block of a project or system, encompassing physical, logical, or informational entities that can be modeled, specified, or referenced."@en ;
                  skos:prefLabel "Domain Element"@en ,
                                 "Elemento de Domínio"@pt-br .


###  https://w3id.org/energy-domain/edo#DomainUnit
edo:DomainUnit rdf:type owl:Class ;
               rdfs:subClassOf qudt:Unit ;
               rdfs:comment "Represents a measurement unit used within the EDO domain. Subclass of QUDT Unit, allowing extension with domain-specific units."@en ;
               rdfs:label "Domain Unit"@en .


###  https://w3id.org/energy-domain/edo#DoubleValue
edo:DoubleValue rdf:type owl:Class ;
                owl:equivalentClass [ rdf:type owl:Restriction ;
                                      owl:onProperty rdf:value ;
                                      owl:allValuesFrom xsd:double
                                    ] ;
                rdfs:subClassOf edo:DataType ;
                rdfs:comment "Constraint for xsd:double (64-bit floating point)"@en ;
                rdfs:label "Double Value"@en .


###  https://w3id.org/energy-domain/edo#Downstream
edo:Downstream rdf:type owl:Class ;
               rdfs:subClassOf edo:OilAndGas ;
               rdfs:label "Downstream"@en ,
                          "Downstream"@pt-br ;
               skos:definition "Oil & Gas sector covering refining, processing, distribution, and retail of petroleum products."@en ,
                               "Setor de Petróleo & Gás que abrange refino, processamento, distribuição e varejo de produtos petrolíferos."@pt-br .


###  https://w3id.org/energy-domain/edo#DragAnchor
edo:DragAnchor rdf:type owl:Class ;
               rdfs:subClassOf edo:Anchor ;
               dcterms:identifier "DragAnchor" ;
               skos:prefLabel "Drag anchor"@en ,
                              "Âncora de arrasto"@pt-br .


###  https://w3id.org/energy-domain/edo#DrawingDimensionsTableAttribute
edo:DrawingDimensionsTableAttribute rdf:type owl:Class ;
                                    rdfs:subClassOf edo:DomainAttribute ;
                                    rdfs:label "Drawing Dimensions Table" .


###  https://w3id.org/energy-domain/edo#DrawingDimensionsTable_DimensionDescription
edo:DrawingDimensionsTable_DimensionDescription rdf:type owl:Class ;
                                                rdfs:subClassOf edo:DimensionsTableColumn ;
                                                dcterms:accessRights "PUBLIC" ;
                                                dcterms:identifier "DrawingDimensionsTable_DimensionDescription" ;
                                                skos:definition "Descrição (Exemplo: Cota do ponto A ao ponto B)"@pt-br ,
                                                                "Provides a detailed description of the dimension. This property explains what the dimension represents, including its relevance and how it relates to other features or components."@en ;
                                                skos:prefLabel "Descrição da Dimensão"@pt-br ,
                                                               "Dimension Description"@en ;
                                                edo:hasAttributeScope edo:TypeLevelAttribute ;
                                                edo:hasLifecycleCreationPhase edo:DetailedDesign ;
                                                edo:hasTypedValue edo:StringValue ;
                                                edo:hasValueCardinality edo:MultiValue .


###  https://w3id.org/energy-domain/edo#DrawingDimensionsTable_DimensionName
edo:DrawingDimensionsTable_DimensionName rdf:type owl:Class ;
                                         rdfs:subClassOf edo:DimensionsTableColumn ;
                                         dcterms:accessRights "PUBLIC" ;
                                         dcterms:identifier "DrawingDimensionsTable_DimensionName" ;
                                         skos:definition "Indicates the name or label assigned to the dimension. This property identifies the specific dimension, which helps in referencing and distinguishing it from other dimensions."@en ;
                                         skos:prefLabel "Dimension Name"@en ,
                                                        "Nome da dimensão"@pt-br ;
                                         edo:hasAttributeScope edo:TypeLevelAttribute ;
                                         edo:hasLifecycleCreationPhase edo:DetailedDesign ;
                                         edo:hasTypedValue edo:StringValue ;
                                         edo:hasValueCardinality edo:MultiValue .


###  https://w3id.org/energy-domain/edo#DrawingDimensionsTable_DimensionUnit
edo:DrawingDimensionsTable_DimensionUnit rdf:type owl:Class ;
                                         rdfs:subClassOf edo:DimensionsTableColumn ;
                                         dcterms:accessRights "PUBLIC" ;
                                         dcterms:identifier "DrawingDimensionsTable_DimensionUnit" ;
                                         skos:definition "A unidade pode qualquer uma do SI (Sistema Internacional de Unidades), por exemplo mm, °, etc."@pt-br ,
                                                         "Specifies the unit of measurement for the dimension value, expressed in SI units. For linear dimensions, this would be meters or millimeters, while for angles, it would be degrees. This property ensures that all measurements are clear, consistent, and standardized."@en ;
                                         skos:prefLabel "Dimension Unit"@en ,
                                                        "Unidade de Dimensão"@pt-br ;
                                         edo:hasAttributeScope edo:TypeLevelAttribute ;
                                         edo:hasLifecycleCreationPhase edo:DetailedDesign ;
                                         edo:hasTypedValue edo:StringValue ;
                                         edo:hasValueCardinality edo:MultiValue .


###  https://w3id.org/energy-domain/edo#DrawingDimensionsTable_DimensionValue
edo:DrawingDimensionsTable_DimensionValue rdf:type owl:Class ;
                                          rdfs:subClassOf edo:DimensionsTableColumn ;
                                          dcterms:accessRights "PUBLIC" ;
                                          dcterms:identifier "DrawingDimensionsTable_DimensionValue" ;
                                          skos:definition "Specifies the actual measurement value of the dimension. This property provides the numerical value for the dimension, which is critical for understanding the size and placement of components or features."@en ;
                                          skos:prefLabel "Dimension Value"@en ,
                                                         "Valor da dimensão"@pt-br ;
                                          edo:hasAttributeScope edo:TypeLevelAttribute ;
                                          edo:hasLifecycleCreationPhase edo:DetailedDesign ;
                                          edo:hasTypedValue edo:FloatValue ;
                                          edo:hasValueCardinality edo:MultiValue .


###  https://w3id.org/energy-domain/edo#DynamicUmbilicalSpan
edo:DynamicUmbilicalSpan rdf:type owl:Class ;
                         rdfs:subClassOf edo:IfcInstanciableElement ,
                                         edo:UmbilicalSpan ;
                         dcterms:identifier "DynamicUmbilicalSpan" ;
                         skos:definition "Suspended umbilical span, continuously subjected to dynamic loading"@en ,
                                         "Trecho de umbilical suspenso, sujeito continuamente a esforços dinâmicos"@pt-br ;
                         skos:prefLabel "Dynamic umbilical span"@en ,
                                        "Trecho dinâmico de umbilical"@pt-br ;
                         edo:hasDiscipline edo:SubseaUmbilicalsEngineering .


###  https://w3id.org/energy-domain/edo#EModVsTempCurveAttribute
edo:EModVsTempCurveAttribute rdf:type owl:Class ;
                             rdfs:subClassOf edo:DomainAttribute .


###  https://w3id.org/energy-domain/edo#EModVsTempTableColumn
edo:EModVsTempTableColumn rdf:type owl:Class ;
                          rdfs:subClassOf edo:EModVsTempCurveAttribute .


###  https://w3id.org/energy-domain/edo#EModVsTempTable_ElasticityModulus
edo:EModVsTempTable_ElasticityModulus rdf:type owl:Class ;
                                      rdfs:subClassOf edo:EModVsTempTableColumn ;
                                      dcterms:accessRights "PUBLIC" ;
                                      dcterms:identifier "EModVsTempTable_ElasticityModulus" ;
                                      skos:definition "Módulo de elasticidade em função da temperatura (Específica para Materiais Poliméricos)"@pt-br ,
                                                      "Represents the modulus of elasticity values corresponding to specific temperatures. This property provides the stiffness or resistance to deformation of the material at each listed temperature, ensuring that the material's mechanical response is understood under varying thermal conditions."@en ;
                                      skos:prefLabel "Elasticity Modulus Versus Temperature Table - Elasticity Modulus"@en ,
                                                     "Tabela do Módulo de Elasticidade em Função da Temperatura - Módulo de Elasticidade"@pt-br ;
                                      edo:hasAttributeScope edo:TypeLevelAttribute ;
                                      edo:hasLifecycleCreationPhase edo:DetailedDesign ;
                                      edo:hasTypedValue edo:FloatValue ;
                                      edo:hasUnit unit:PA ;
                                      edo:hasValueCardinality edo:MultiValue .


###  https://w3id.org/energy-domain/edo#EModVsTempTable_Temperature
edo:EModVsTempTable_Temperature rdf:type owl:Class ;
                                rdfs:subClassOf edo:EModVsTempTableColumn ;
                                dcterms:accessRights "PUBLIC" ;
                                dcterms:identifier "EModVsTempTable_Temperature" ;
                                skos:definition "Represents the thermal condition or measurement of heat for a component or system. This property is important for assessing how the component performs or operates under specific thermal conditions, ensuring it remains within safe and effective operating limits."@en ;
                                skos:prefLabel "Elasticity Modulus Versus Temperature Table - Temperature"@en ;
                                edo:hasAttributeScope edo:TypeLevelAttribute ;
                                edo:hasLifecycleCreationPhase edo:DetailedDesign ;
                                edo:hasTypedValue edo:FloatValue ;
                                edo:hasValueCardinality edo:MultiValue .


###  https://w3id.org/energy-domain/edo#EarlyLeakMaxPressTableAttribute
edo:EarlyLeakMaxPressTableAttribute rdf:type owl:Class ;
                                    rdfs:subClassOf edo:HydrostaticPressureTestsAttribute .


###  https://w3id.org/energy-domain/edo#EarlyLeakMaxPressTableColumn
edo:EarlyLeakMaxPressTableColumn rdf:type owl:Class ;
                                 rdfs:subClassOf edo:EarlyLeakMaxPressTableAttribute .


###  https://w3id.org/energy-domain/edo#EarlyLeakMaxPressTable_Press
edo:EarlyLeakMaxPressTable_Press rdf:type owl:Class ;
                                 rdfs:subClassOf edo:EarlyLeakMaxPressTableColumn ;
                                 dcterms:accessRights "PUBLIC" ;
                                 dcterms:identifier "EarlyLeakMaxPressTable_Press" ;
                                 skos:definition "Condições de teste dos tramos para Pressão - Máxima - Teste de vazamento hidrostático precoce"@pt-br ,
                                                 "The maximum pressure applied during the Early Leak Test, verifying resistance under extreme pressure conditions."@en ;
                                 skos:prefLabel "Early Leak Maximum Pressure Table - Pressure"@en ,
                                                "Tabela de Pressão Máxima de Vazamento Precoce - Pressão"@pt-br ;
                                 edo:hasAttributeScope edo:InstanceLevelAttribute ;
                                 edo:hasLifecycleCreationPhase edo:DetailedDesign ;
                                 edo:hasTypedValue edo:FloatValue ;
                                 edo:hasUnit unit:PA ;
                                 edo:hasValueCardinality edo:MultiValue .


###  https://w3id.org/energy-domain/edo#EarlyLeakMaxPressTable_PressIntValStrat
edo:EarlyLeakMaxPressTable_PressIntValStrat rdf:type owl:Class ;
                                            rdfs:subClassOf edo:EarlyLeakMaxPressTableAttribute ;
                                            dcterms:accessRights "PUBLIC" ;
                                            dcterms:identifier "EarlyLeakMaxPressTable_PressIntValStrat" ;
                                            skos:definition "Condições de teste dos tramos para Estratégia de valores intermediários - Máximo - Teste de vazamento hidrostático precoce"@pt-br ,
                                                            "Strategy used to calculate intermediate values between maximum conditions during the Early Leak Test."@en ;
                                            skos:prefLabel "Early Leak Maximum Pressure Table - Pressure Intermediate Values Strategy"@en ,
                                                           "Tabela de Pressão Máxima de Vazamento Precoce - Estratégia de Valores Intermediários de Pressão"@pt-br ;
                                            edo:hasAttributeScope edo:InstanceLevelAttribute ;
                                            edo:hasLifecycleCreationPhase edo:DetailedDesign ;
                                            edo:hasTypedValue edo:StringValue ;
                                            edo:hasValueCardinality edo:SingleValue .


###  https://w3id.org/energy-domain/edo#EarlyLeakMaxPressTable_PressValRef
edo:EarlyLeakMaxPressTable_PressValRef rdf:type owl:Class ;
                                       rdfs:subClassOf edo:EarlyLeakMaxPressTableColumn ;
                                       dcterms:accessRights "PUBLIC" ;
                                       dcterms:identifier "EarlyLeakMaxPressTable_PressValRef" ;
                                       skos:definition "Comentários Condições de teste dos tramos para - Máximo - Teste de vazamento hidrostático precoce"@pt-br ,
                                                       "Specifies the reference pressure used to determine the Early Leak Maximum Pressure value."@en ;
                                       skos:prefLabel "Early Leak Maximum Pressure Table - Pressure Value Reference"@en ,
                                                      "Tabela de Pressão Máxima de Vazamento Precoce - Referência de Valor de Pressão"@pt-br ;
                                       edo:hasAttributeScope edo:InstanceLevelAttribute ;
                                       edo:hasLifecycleCreationPhase edo:DetailedDesign ;
                                       edo:hasTypedValue edo:StringValue ;
                                       edo:hasValueCardinality edo:MultiValue .


###  https://w3id.org/energy-domain/edo#EarlyLeakMaxPressTable_PressValRefMult
edo:EarlyLeakMaxPressTable_PressValRefMult rdf:type owl:Class ;
                                           rdfs:subClassOf edo:EarlyLeakMaxPressTableColumn ;
                                           dcterms:accessRights "PUBLIC" ;
                                           dcterms:identifier "EarlyLeakMaxPressTable_PressValRefMult" ;
                                           skos:definition "Early Leak Maximum Pressure Table - Pressure Value Reference Multiplier"@pt-br ,
                                                           "The multiplier applied to the reference pressure to determine the Early Leak Maximum Pressure value."@en ;
                                           skos:prefLabel "Early Leak Maximum Pressure Table - Pressure Value Reference Multiplier"@en ,
                                                          "Tabela de Pressão Máxima de Vazamento Precoce - Multiplicador de Referência de Valor de Pressão"@pt-br ;
                                           edo:hasAttributeScope edo:InstanceLevelAttribute ;
                                           edo:hasLifecycleCreationPhase edo:DetailedDesign ;
                                           edo:hasTypedValue edo:FloatValue ;
                                           edo:hasUnit unit:PA ;
                                           edo:hasValueCardinality edo:MultiValue .


###  https://w3id.org/energy-domain/edo#EarlyLeakMaxPressTable_TensLimit
edo:EarlyLeakMaxPressTable_TensLimit rdf:type owl:Class ;
                                     rdfs:subClassOf edo:EarlyLeakMaxPressTableColumn ;
                                     dcterms:accessRights "PUBLIC" ;
                                     dcterms:identifier "EarlyLeakMaxPressTable_TensLimit" ;
                                     skos:definition "Condições de teste dos tramos para Tensão - Máxima - Teste de vazamento hidrostático precoce"@pt-br ,
                                                     "Tensile limit condition that must be respected to avoid damaging the tested product."@en ;
                                     skos:prefLabel "Early Leak Maximum Pressure Table - Tensile Limit"@en ,
                                                    "Tabela de Pressão Máxima de Vazamento Precoce - Limite de Tração"@pt-br ;
                                     edo:hasAttributeScope edo:InstanceLevelAttribute ;
                                     edo:hasLifecycleCreationPhase edo:DetailedDesign ;
                                     edo:hasTypedValue edo:FloatValue ;
                                     edo:hasUnit unit:N ;
                                     edo:hasValueCardinality edo:MultiValue .


###  https://w3id.org/energy-domain/edo#EarlyLeakMaxPressTable_TensLimitValRef
edo:EarlyLeakMaxPressTable_TensLimitValRef rdf:type owl:Class ;
                                           rdfs:subClassOf edo:EarlyLeakMaxPressTableColumn ;
                                           dcterms:accessRights "PUBLIC" ;
                                           dcterms:identifier "EarlyLeakMaxPressTable_TensLimitValRef" ;
                                           skos:definition "Indicates the basis used to establish the tensile limit value during the Early Leak Maximum Pressure Test, ensuring the product's tensile strength is respected to avoid damage."@en ;
                                           skos:prefLabel "Early Leak Maximum Pressure Table - Tensile Limit Value Reference"@en ,
                                                          "Tabela de Pressão Máxima de Vazamento Precoce - Referência do Limite de Tração"@pt-br ;
                                           edo:hasAttributeScope edo:InstanceLevelAttribute ;
                                           edo:hasLifecycleCreationPhase edo:DetailedDesign ;
                                           edo:hasTypedValue edo:StringValue ;
                                           edo:hasValueCardinality edo:MultiValue .


###  https://w3id.org/energy-domain/edo#EarlyLeakNomPressTableAttribute
edo:EarlyLeakNomPressTableAttribute rdf:type owl:Class ;
                                    rdfs:subClassOf edo:HydrostaticPressureTestsAttribute .


###  https://w3id.org/energy-domain/edo#EarlyLeakNomPressTableColumn
edo:EarlyLeakNomPressTableColumn rdf:type owl:Class ;
                                 rdfs:subClassOf edo:EarlyLeakNomPressTableAttribute .


###  https://w3id.org/energy-domain/edo#EarlyLeakNomPressTable_Press
edo:EarlyLeakNomPressTable_Press rdf:type owl:Class ;
                                 rdfs:subClassOf edo:EarlyLeakNomPressTableColumn ;
                                 dcterms:accessRights "PUBLIC" ;
                                 dcterms:identifier "EarlyLeakNomPressTable_Press" ;
                                 skos:definition "Condições de teste dos tramos para Pressão - Nominal - Teste de vazamento hidrostático precoce"@pt-br ,
                                                 "The nominal pressure applied during the Early Leak Test, verifying standard operational conditions for leakage detection."@en ;
                                 skos:prefLabel "Early Leak Nominal Pressure Table - Pressure"@en ,
                                                "Tabela de Pressão Nominal de Vazamento Precoce - Pressão"@pt-br ;
                                 edo:hasAttributeScope edo:InstanceLevelAttribute ;
                                 edo:hasLifecycleCreationPhase edo:DetailedDesign ;
                                 edo:hasTypedValue edo:FloatValue ;
                                 edo:hasUnit unit:PA ;
                                 edo:hasValueCardinality edo:MultiValue .


###  https://w3id.org/energy-domain/edo#EarlyLeakNomPressTable_PressIntValStrat
edo:EarlyLeakNomPressTable_PressIntValStrat rdf:type owl:Class ;
                                            rdfs:subClassOf edo:EarlyLeakNomPressTableAttribute ;
                                            dcterms:accessRights "PUBLIC" ;
                                            dcterms:identifier "EarlyLeakNomPressTable_PressIntValStrat" ;
                                            skos:definition "Condições de teste dos tramos para Estratégia de valores intermediários - Nominal - Teste de vazamento hidrostático precoce"@pt-br ,
                                                            "Strategy used to calculate intermediate Pressure values between nominal conditions during the Early Leak Test."@en ;
                                            skos:prefLabel "Early Leak Nominal Pressure Table - Pressure Intermediate Values Strategy"@en ,
                                                           "Tabela de Pressão Nominal de Vazamento Precoce - Estratégia de Valores Intermediários de Pressão"@pt-br ;
                                            edo:hasAttributeScope edo:InstanceLevelAttribute ;
                                            edo:hasLifecycleCreationPhase edo:DetailedDesign ;
                                            edo:hasTypedValue edo:StringValue ;
                                            edo:hasValueCardinality edo:SingleValue .


###  https://w3id.org/energy-domain/edo#EarlyLeakNomPressTable_PressValRef
edo:EarlyLeakNomPressTable_PressValRef rdf:type owl:Class ;
                                       rdfs:subClassOf edo:EarlyLeakNomPressTableColumn ;
                                       dcterms:accessRights "PUBLIC" ;
                                       dcterms:identifier "EarlyLeakNomPressTable_PressValRef" ;
                                       skos:definition "Comentários Condições de teste dos tramos para - Nominal - Teste de vazamento hidrostático precoce"@pt-br ,
                                                       "Specifies the reference pressure used to determine the Early Leak Nominal Pressure value."@en ;
                                       skos:prefLabel "Early Leak Nominal Pressure Table - Pressure Value Reference"@en ,
                                                      "Tabela de Pressão Nominal de Vazamento Precoce - Referência de Valor de Pressão"@pt-br ;
                                       edo:hasAttributeScope edo:InstanceLevelAttribute ;
                                       edo:hasLifecycleCreationPhase edo:DetailedDesign ;
                                       edo:hasTypedValue edo:StringValue ;
                                       edo:hasValueCardinality edo:MultiValue .


###  https://w3id.org/energy-domain/edo#EarlyLeakNomPressTable_PressValRefMult
edo:EarlyLeakNomPressTable_PressValRefMult rdf:type owl:Class ;
                                           rdfs:subClassOf edo:EarlyLeakNomPressTableColumn ;
                                           dcterms:accessRights "PUBLIC" ;
                                           dcterms:identifier "EarlyLeakNomPressTable_PressValRefMult" ;
                                           skos:definition "The multiplier applied to the reference pressure to determine the Early Leak Nominal Pressure value."@en ;
                                           skos:prefLabel "Early Leak Nominal Pressure Table - Pressure Value Reference Multiplier"@en ,
                                                          "Tabela de Pressão Nominal de Vazamento Precoce - Multiplicador de Referência de Valor de Pressão"@pt-br ;
                                           edo:hasAttributeScope edo:InstanceLevelAttribute ;
                                           edo:hasLifecycleCreationPhase edo:DetailedDesign ;
                                           edo:hasTypedValue edo:FloatValue ;
                                           edo:hasValueCardinality edo:MultiValue .


###  https://w3id.org/energy-domain/edo#EarlyLeakNomPressTable_TensLimit
edo:EarlyLeakNomPressTable_TensLimit rdf:type owl:Class ;
                                     rdfs:subClassOf edo:EarlyLeakNomPressTableColumn ;
                                     dcterms:accessRights "PUBLIC" ;
                                     dcterms:identifier "EarlyLeakNomPressTable_TensLimit" ;
                                     skos:definition "Condições de teste dos tramos para Tensão - Nominal - Teste de vazamento hidrostático precoce"@pt-br ,
                                                     "Tensile limit condition that must be respected to avoid damaging the tested product."@en ;
                                     skos:prefLabel "Early Leak Nominal Pressure Table - Tensile Limit"@en ,
                                                    "Tabela de Pressão Nominal de Vazamento Precoce - Limite de Tração"@pt-br ;
                                     edo:hasAttributeScope edo:InstanceLevelAttribute ;
                                     edo:hasLifecycleCreationPhase edo:DetailedDesign ;
                                     edo:hasTypedValue edo:FloatValue ;
                                     edo:hasUnit unit:N ;
                                     edo:hasValueCardinality edo:MultiValue .


###  https://w3id.org/energy-domain/edo#EarlyLeakNomPressTable_TensLimitValRef
edo:EarlyLeakNomPressTable_TensLimitValRef rdf:type owl:Class ;
                                           rdfs:subClassOf edo:EarlyLeakNomPressTableColumn ;
                                           dcterms:accessRights "PUBLIC" ;
                                           dcterms:identifier "EarlyLeakNomPressTable_TensLimitValRef" ;
                                           skos:definition "Indicates the basis used to establish the tensile limit value during the Early Leak Nominal Pressure Test, ensuring the product's tensile strength is respected to avoid damage."@en ;
                                           skos:prefLabel "Early Leak Nominal Pressure Table - Tensile Limit Value Reference"@en ,
                                                          "Tabela de Pressão Nominal de Vazamento Precoce - Referência do Limite de Tração"@pt-br ;
                                           edo:hasAttributeScope edo:InstanceLevelAttribute ;
                                           edo:hasLifecycleCreationPhase edo:DetailedDesign ;
                                           edo:hasTypedValue edo:StringValue ;
                                           edo:hasValueCardinality edo:MultiValue .


###  https://w3id.org/energy-domain/edo#ElasticityModulusAt23Degrees
edo:ElasticityModulusAt23Degrees rdf:type owl:Class ;
                                 rdfs:subClassOf edo:DomainAttribute ;
                                 dcterms:accessRights "PUBLIC" ;
                                 dcterms:identifier "ElasticityModulusAt23Degrees" ;
                                 skos:definition "Módulo de elasticidade a 23 graus Celsius (Específica para Materiais Metálicos e Poliméricos)"@pt-br ,
                                                 "Specifies the modulus of elasticity of the material at 23 degrees Celsius, indicating its stiffness or resistance to deformation under stress at this temperature. This property is crucial for determining how the flexible structure responds to mechanical loads, ensuring that it maintains structural integrity."@en ;
                                 skos:prefLabel "Elasticity Modulus At 23 Degrees"@en ,
                                                "Módulo de Elasticidade a 23 Graus Celsius"@pt-br ;
                                 edo:hasAttributeScope edo:TypeLevelAttribute ;
                                 edo:hasLifecycleCreationPhase edo:DetailedDesign ;
                                 edo:hasTypedValue edo:FloatValue ;
                                 edo:hasUnit unit:PA ;
                                 edo:hasValueCardinality edo:SingleValue .


###  https://w3id.org/energy-domain/edo#ElectricPort
edo:ElectricPort rdf:type owl:Class ;
                 rdfs:subClassOf edo:Port ;
                 dcterms:identifier "ElectricPort" ;
                 skos:definition "Representa uma porta usada para transmitir energia elétrica ou sinais entre elementos."@pt-br ,
                                 "Represents a port used for transmitting electrical power or signals between elements."@en ;
                 skos:prefLabel "Electric Port"@en ,
                                "Porta Elétrica"@pt-br .


###  https://w3id.org/energy-domain/edo#ElectricalCable
edo:ElectricalCable rdf:type owl:Class ;
                    rdfs:subClassOf edo:FunctionLine ,
                                    edo:IfcInstanciableElement ;
                    dcterms:identifier "ElectricalCable" ;
                    skos:definition "Representa um cabo elétrico dentro de uma linha funcional, transmitindo energia elétrica ou sinais."@pt-br ,
                                    "Represents an electrical cable within a function line, transmitting electrical power or signals."@en ;
                    skos:prefLabel "Cabo Elétrico"@pt-br ,
                                   "Cabo elétrico"@pt-br ,
                                   "Electrical Cable"@en ,
                                   "Electrical cable"@en ;
                    edo:hasAttribute edo:ConductorCrossSection ,
                                     edo:GroupShieldingType ,
                                     edo:NumGroupConductors ,
                                     edo:NumGroups ,
                                     edo:OverallShieldingType ,
                                     edo:VoltageRatingTableColumn ;
                    edo:hasDiscipline edo:SubseaUmbilicalsEngineering ;
                    edo:ifc_equivalentClass "IfcCableSegment" ;
                    edo:ifc_objectType "ElectricalCable" ;
                    edo:ifc_predefinedType "USERDEFINED" .


###  https://w3id.org/energy-domain/edo#ElectricalEngineering
edo:ElectricalEngineering rdf:type owl:Class ;
                          rdfs:subClassOf edo:TechnicalDiscipline ;
                          rdfs:label "Electrical Engineering"@en ,
                                     "Engenharia Elétrica"@pt-br ;
                          skos:definition "Disciplina de engenharia focada em sistemas elétricos, distribuição e geração de energia."@pt-br ,
                                          "Engineering discipline focused on electrical systems, power distribution and generation."@en .


###  https://w3id.org/energy-domain/edo#ElectricalJumper
edo:ElectricalJumper rdf:type owl:Class ;
                     rdfs:subClassOf edo:Jumper ;
                     dcterms:identifier "ElectricalJumper" ;
                     skos:definition "Jumper for signal transmission or low-power eletrical supply"@en ,
                                     "Jumper para transmissão de sinais ou alimentação elétrica de baixa potência"@pt-br ;
                     skos:prefLabel "Electrical jumper"@en ,
                                    "Jumper elétrico"@pt-br .


###  https://w3id.org/energy-domain/edo#ElectricalJumperConnector
edo:ElectricalJumperConnector rdf:type owl:Class ;
                              rdfs:subClassOf edo:JumperConnector ;
                              dcterms:identifier "ElectricalJumperConnector" ;
                              skos:definition "Conector para terminação de jumpers/cabos elétricos de sinal/baixa corrente."@pt-br ,
                                              "Connector for termination of electrical signal/low-current jumpers or cables."@en ;
                              skos:prefLabel "Conector de Jumper Elétrico"@pt-br ,
                                             "Electrical Jumper Connector"@en ;
                              edo:hasAttribute edo:MatingEnvironment ,
                                               edo:MechanicalGender ,
                                               edo:NumMatingCycles ;
                              edo:hasDiscipline edo:SubseaUmbilicalsEngineering ;
                              edo:ifc_equivalentClass "IfcCableFitting" ;
                              edo:ifc_objectType "ElectricalJumperConnector" .


###  https://w3id.org/energy-domain/edo#ElectricalPowerJumper
edo:ElectricalPowerJumper rdf:type owl:Class ;
                          rdfs:subClassOf edo:Jumper ;
                          dcterms:identifier "ElectricalPowerJumper" ;
                          skos:prefLabel "Electrical power jumper"@en ,
                                         "Jumper elétrico de potência"@pt-br .


###  https://w3id.org/energy-domain/edo#ElectricalPowerJumperConnector
edo:ElectricalPowerJumperConnector rdf:type owl:Class ;
                                   rdfs:subClassOf edo:JumperConnector ;
                                   dcterms:identifier "ElectricalPowerJumperConnector" ;
                                   skos:definition "Conector para terminação de jumpers/cabos elétricos de alta tensão/corrente."@pt-br ,
                                                   "Connector for termination of high-voltage/high-current electrical jumpers or cables."@en ;
                                   skos:prefLabel "Conector de Jumper Elétrico de Potência"@pt-br ,
                                                  "Electrical Power Jumper Connector"@en ;
                                   edo:hasAttribute edo:AssemblyType ,
                                                    edo:MaxCurrent ,
                                                    edo:NumPhases ,
                                                    edo:PowerRating ,
                                                    edo:TemperatureClass ,
                                                    edo:VoltageRatingTableColumn ;
                                   edo:hasDiscipline edo:SubseaUmbilicalsEngineering ;
                                   edo:ifc_equivalentClass "IfcCableFitting" ;
                                   edo:ifc_objectType "ElectricalPowerJumperConnector" .


###  https://w3id.org/energy-domain/edo#ElectronicDevice
edo:ElectronicDevice rdf:type owl:Class ;
                     rdfs:subClassOf edo:ComponentDevice ;
                     dcterms:identifier "ElectronicDevice" ;
                     skos:prefLabel "Dispositivo eletrônico"@pt-br ,
                                    "Electronic device"@en .


###  https://w3id.org/energy-domain/edo#ElementClassification
edo:ElementClassification rdf:type owl:Class ;
                          rdfs:subClassOf edo:DomainClassification .


###  https://w3id.org/energy-domain/edo#EndFitting
edo:EndFitting rdf:type owl:Class ;
               rdfs:subClassOf edo:IfcInstanciableElement ,
                               edo:PipeTermination ;
               dcterms:identifier "EndFitting" ;
               skos:altLabel "Connector Fitting"@en ,
                             "End Termination"@en ,
                             "Termination Assembly"@en ,
                             "Termination Fitting"@en ;
               skos:definition "Component used in subsea flexible pipes to provide a secure transition between the flexible pipe and rigid structures, such as subsea equipment or topside facilities, as well as to connect two sections of flexible pipe. The End Fitting ensures the structural integrity and sealing of the pipe, allowing for the connection of the flexible line to other equipment or sections while withstanding internal pressures and environmental forces. It is a critical interface that accommodates the pipe's mechanical, hydraulic, and thermal loads, ensuring long-term reliable performance in harsh subsea conditions."@en ,
                               "Componente utilizado em dutos flexíveis para fornecer uma transição segura entre o duto flexível e estruturas rígidas, como equipamentos submersos ou instalações no topo, bem como para conectar duas seções de duto flexível. O Terminador garante a integridade estrutural e o vedamento do duto, permitindo a conexão da linha flexível a outros equipamentos ou seções, resistindo a pressões internas e forças ambientais. É uma interface crítica que acomoda as cargas mecânicas, hidráulicas e térmicas do duto, garantindo desempenho confiável a longo prazo em condições submarinas adversas."@pt-br ;
               skos:prefLabel "Conector de Extremidade"@pt-br ,
                              "End fitting"@en ;
               edo:hasAttribute edo:BoreDiameter ,
                                edo:FlangeFaceType ,
                                edo:FlangeType ,
                                edo:HasFaceORing ,
                                edo:HasModaSensor ,
                                edo:HasN2InjectionPort ,
                                edo:RingGasketInnerDIameter ,
                                edo:RingGasketOuterDiameter ,
                                edo:RingGasketPressureRating ,
                                edo:RingGasketSpecification ,
                                edo:RingGasketStandard ,
                                edo:RingGasketType ;
               edo:hasDiscipline edo:SubseaFlexiblePipesEngineering ;
               edo:ifc_equivalentClass "IfcPipeFitting" ;
               edo:ifc_objectType "EndFitting" ;
               edo:ifc_predefinedType "USERDEFINED" .


###  https://w3id.org/energy-domain/edo#EnergyStorage
edo:EnergyStorage rdf:type owl:Class ;
                  rdfs:subClassOf edo:Domain ;
                  rdfs:label "Armazenamento de Energia"@pt-br ,
                             "Energy Storage"@en ;
                  skos:definition "Technologies for storing energy, such as batteries, pumped hydro, or compressed air."@en ,
                                  "Tecnologias para armazenamento de energia, como baterias, hidroelétricas reversíveis ou ar comprimido."@pt-br .


###  https://w3id.org/energy-domain/edo#EnhancedGeothermalSystems
edo:EnhancedGeothermalSystems rdf:type owl:Class ;
                              rdfs:subClassOf edo:Geothermal ;
                              dcterms:identifier "EnhancedGeothermalSystems" ;
                              skos:definition "Enhanced geothermal systems (EGS) create artificial reservoirs in hot dry rock by injecting water at high pressure, enabling the extraction of geothermal energy in areas without naturally occurring hydrothermal resources."@en ,
                                              "Sistemas geotérmicos estimulados (EGS) criam reservatórios artificiais em rochas secas quentes através da injeção de água em alta pressão, possibilitando a extração de energia geotérmica em áreas sem recursos hidrotermais naturais."@pt-br ;
                              skos:prefLabel "Enhanced Geothermal Systems"@en ,
                                             "Sistemas Geotérmicos Estimulados"@pt-br .


###  https://w3id.org/energy-domain/edo#Equipment
edo:Equipment rdf:type owl:Class ;
              rdfs:subClassOf edo:CompactObject ;
              dcterms:identifier "Equipment" ;
              skos:definition "Large and complex objects for permanent or temporary use"@en ,
                              "Objetos de grande porte e complexidade, para uso permanente ou temporário"@pt-br ;
              skos:prefLabel "Equipamento"@pt-br ,
                             "Equipment"@en ;
              edo:hasAttribute edo:TemperatureRangeTableColumn .


###  https://w3id.org/energy-domain/edo#EquipmentEngineering
edo:EquipmentEngineering rdf:type owl:Class ;
                         rdfs:subClassOf edo:TechnicalDiscipline ;
                         rdfs:label "Engenharia de Equipamentos"@pt-br ,
                                    "Equipment Engineering"@en ;
                         skos:definition "Disciplina de engenharia focada no projeto e especificação de equipamentos industriais."@pt-br ,
                                         "Engineering discipline focused on the design and specification of industrial equipment."@en .


###  https://w3id.org/energy-domain/edo#EquipmentLocation
edo:EquipmentLocation rdf:type owl:Class ;
                      rdfs:subClassOf edo:PointLocation ;
                      dcterms:identifier "EquipmentLocation" ;
                      skos:definition "Base for installation sites for large underwater equipment."@en ,
                                      "Base para locais de instalação de grandes equipamentos submarinos"@pt-br ;
                      skos:prefLabel "Equipment Location"@en ,
                                     "Localização de Equipamento"@pt-br .


###  https://w3id.org/energy-domain/edo#ErosionalVelocity
edo:ErosionalVelocity rdf:type owl:Class ;
                      rdfs:subClassOf edo:DomainAttribute ;
                      dcterms:accessRights "PUBLIC" ;
                      dcterms:identifier "ErosionalVelocity" ;
                      skos:definition "Represents the maximum velocity of a fluid at which erosion of the material begins to occur. This property is crucial for determining the operational limits of the system, ensuring that the material can withstand fluid flow without suffering erosive damage."@en ;
                      skos:prefLabel "Erosional Velocity"@en ,
                                     "Velocidade erosional"@pt-br ;
                      edo:hasAttributeScope edo:TypeLevelAttribute ;
                      edo:hasLifecycleCreationPhase edo:DetailedDesign ;
                      edo:hasTypedValue edo:StringValue ;
                      edo:hasValueCardinality edo:SingleValue .


###  https://w3id.org/energy-domain/edo#ExecutiveProjectRevision
edo:ExecutiveProjectRevision rdf:type owl:Class ;
                             rdfs:subClassOf edo:DomainAttribute ;
                             dcterms:accessRights "PUBLIC" ;
                             dcterms:identifier "ExecutiveProjectRevision" ;
                             skos:definition "Indicates the revision number of the executive project, represented as a numeric value that is incremented with each new submission (e.g., 0000, 0001, 0002), stored as text for consistency in formatting."@en ,
                                             "Revisão do projeto executivo  Valor numérico incrementado a cada novo envio (0000, 0001, 0002 e etc.) como texto"@pt-br ;
                             skos:prefLabel "Executive Project Revision"@en ,
                                            "Revisão do Projeto Executivo"@pt-br ;
                             edo:hasAttributeScope edo:InstanceLevelAttribute ;
                             edo:hasLifecycleCreationPhase edo:DetailedDesign ;
                             edo:hasTypedValue edo:StringValue ;
                             edo:hasValueCardinality edo:SingleValue .


###  https://w3id.org/energy-domain/edo#ExternalDiameter
edo:ExternalDiameter rdf:type owl:Class ;
                     rdfs:subClassOf edo:DomainAttribute ;
                     dcterms:accessRights "PUBLIC" ;
                     dcterms:identifier "ExternalDiameter" ;
                     skos:definition "Distance measured across the outermost points, passing through the center."@en ;
                     skos:prefLabel "Diâmetro externo"@pt-br ,
                                    "External Diameter"@en ;
                     edo:hasAttributeScope edo:TypeLevelAttribute ;
                     edo:hasLifecycleCreationPhase edo:DetailedDesign ;
                     edo:hasTypedValue edo:FloatValue ;
                     edo:hasUnit unit:M ;
                     edo:hasValueCardinality edo:SingleValue .


###  https://w3id.org/energy-domain/edo#ExternalReference
edo:ExternalReference rdf:type owl:Class ;
                      rdfs:subClassOf edo:DomainElement ;
                      skos:definition "Representa entidades que funcionam como referências externas dentro de um projeto ou modelo. Não são elementos físicos nem lógicos em si, mas fornecem vínculos para informações de apoio, como documentos, dicionários de dados ou normas. Seu propósito é conectar o modelo a fontes externas de conhecimento, garantindo rastreabilidade, conformidade e compreensão contextual."@pt-br ,
                                      "Represents entities that serve as external references within a project or model. They are not physical or logical elements themselves but provide links to supporting information such as documents, data dictionaries, or standards. Their purpose is to connect the model to external sources of knowledge, ensuring traceability, compliance, and contextual understanding."@en ;
                      skos:prefLabel "External Reference"@en ,
                                     "Referência Externa"@pt-br .


###  https://w3id.org/energy-domain/edo#FEED
edo:FEED rdf:type owl:Class ;
         rdfs:subClassOf edo:DesignPhase ;
         rdfs:label "FEED (Front-End Engineering Design)"@en ,
                    "FEED (Projeto Básico de Engenharia)"@pt-br ;
         skos:definition "Fase intermediária entre o projeto conceitual e detalhado, refinando detalhes técnicos e de custo."@pt-br ,
                         "Intermediate phase between conceptual and detailed design, refining technical and cost details."@en .


###  https://w3id.org/energy-domain/edo#FSHRLowerAssembly
edo:FSHRLowerAssembly rdf:type owl:Class ;
                      rdfs:subClassOf edo:FlowControlEquipment ;
                      dcterms:identifier "FSHRLowerAssembly" ;
                      skos:prefLabel "Estrutura inferior de RHAS"@pt-br ,
                                     "FSHR lower assembly"@en .


###  https://w3id.org/energy-domain/edo#FSHRUpperAssembly
edo:FSHRUpperAssembly rdf:type owl:Class ;
                      rdfs:subClassOf edo:FlowControlEquipment ;
                      dcterms:identifier "FSHRUpperAssembly" ;
                      skos:prefLabel "Estrutura de topo de RHAS"@pt-br ,
                                     "FSHR upper assembly"@en .


###  https://w3id.org/energy-domain/edo#FabricTape
edo:FabricTape rdf:type owl:Class ;
               rdfs:subClassOf edo:IfcInstanciableElement ,
                               edo:TapeLayer ;
               dcterms:identifier "FabricTape" ;
               skos:definition "Material used in subsea flexible pipe construction, typically applied as a wrapping layer to provide protection and containment for internal components. Fabric Tape is designed to secure and hold various layers of the pipe in place during manufacturing and operation, preventing displacement or damage to the underlying layers. It also adds a layer of abrasion resistance, contributing to the overall durability of the pipe in dynamic subsea environments. Made from high-strength, flexible materials, Fabric Tape plays a key role in maintaining the integrity of the flexible pipe structure."@en ,
                               "Material utilizado na construção de dutos flexíveis, geralmente aplicado como uma camada de envolvimento para fornecer proteção e contenção para os componentes internos. A Fita Construtiva é projetada para segurar e manter as várias camadas do duto no lugar durante a fabricação e operação, evitando o deslocamento ou danos às camadas subjacentes. Ela também adiciona uma camada de resistência à abrasão, contribuindo para a durabilidade geral do duto em ambientes dinâmicos. Feita de materiais flexíveis e de alta resistência, a Fita Construtiva desempenha um papel crucial na manutenção da integridade da estrutura do duto flexível."@pt-br ;
               skos:prefLabel "Fabric Tape"@en ,
                              "Fita Construtiva"@pt-br ;
               edo:hasDiscipline edo:SubseaFlexiblePipesEngineering ,
                                 edo:SubseaUmbilicalsEngineering ;
               edo:ifc_equivalentClass "IfcPipeSegment" ;
               edo:ifc_objectType "FabricTape" ;
               edo:ifc_predefinedType "USERDEFINED" .


###  https://w3id.org/energy-domain/edo#Fabrication
edo:Fabrication rdf:type owl:Class ;
                rdfs:subClassOf edo:ConstructionPhase ;
                rdfs:label "Fabrication"@en ,
                           "Fabricação"@pt-br ;
                skos:definition "Fabricação e montagem de componentes, módulos ou estruturas em oficinas ou estaleiros."@pt-br ,
                                "Manufacturing and assembly of components, modules, or structures in workshops or yards."@en .


###  https://w3id.org/energy-domain/edo#FabricationComponent
edo:FabricationComponent rdf:type owl:Class ;
                         rdfs:subClassOf edo:DomainElement ;
                         skos:definition "Representa elementos físicos, não rastreáveis e não substituíveis. Normalmente correspondem a partes fabricadas ou montadas que se integram permanentemente a um sistema ou estrutura maior, sem serem rastreadas ou substituídas individualmente. Seu propósito é representar componentes essenciais para a fabricação, mas que não existem como unidades gerenciáveis de forma independente após sua incorporação."@pt-br ,
                                         "Represents elements that are physical, non-traceable, and non-replaceable. They are typically manufactured or assembled parts that become permanently integrated into a larger system or structure, without being individually tracked or substituted. Their purpose is to capture components that are essential for fabrication but do not exist as independently manageable units once incorporated."@en ;
                         skos:prefLabel "Componente de Fabricação"@pt-br ,
                                        "Fabrication Component"@en .


###  https://w3id.org/energy-domain/edo#FatMaxPress
edo:FatMaxPress rdf:type owl:Class ;
                rdfs:subClassOf edo:HydrostaticPressureTestsAttribute ;
                dcterms:accessRights "PUBLIC" ;
                dcterms:identifier "FatMaxPress" ;
                skos:definition "Condições de teste dos tramos para Pressão - Máxima - FAT hidrostática"@pt-br ,
                                "The maximum pressure applied during the Factory Acceptance Test (FAT) to ensure the equipment can withstand extreme conditions."@en ;
                skos:prefLabel "Factory Acceptance Test Maximum Pressure"@en ,
                               "Pressão Máxima para o Teste de Aceitação na Fábrica"@pt-br ;
                edo:hasAttributeScope edo:InstanceLevelAttribute ;
                edo:hasLifecycleCreationPhase edo:DetailedDesign ;
                edo:hasTypedValue edo:FloatValue ;
                edo:hasUnit unit:PA ;
                edo:hasValueCardinality edo:SingleValue .


###  https://w3id.org/energy-domain/edo#FatMaxPressValRef
edo:FatMaxPressValRef rdf:type owl:Class ;
                      rdfs:subClassOf edo:HydrostaticPressureTestsAttribute ;
                      dcterms:accessRights "PUBLIC" ;
                      dcterms:identifier "FatMaxPressValRef" ;
                      skos:definition "Comentários Condições de teste dos tramos para - Máximo - FAT hidrostático"@pt-br ,
                                      "Specifies the reference pressure used to determine the FAT maximum pressure value."@en ;
                      skos:prefLabel "Factory Acceptance Test Maximum Pressure Value Reference"@en ,
                                     "Referência de Valor de Pressão Máxima para o Teste de Aceitação na Fábrica"@pt-br ;
                      edo:hasAttributeScope edo:InstanceLevelAttribute ;
                      edo:hasLifecycleCreationPhase edo:DetailedDesign ;
                      edo:hasTypedValue edo:StringValue ;
                      edo:hasValueCardinality edo:SingleValue .


###  https://w3id.org/energy-domain/edo#FatMaxPressValRefMult
edo:FatMaxPressValRefMult rdf:type owl:Class ;
                          rdfs:subClassOf edo:HydrostaticPressureTestsAttribute ;
                          dcterms:accessRights "PUBLIC" ;
                          dcterms:identifier "FatMaxPressValRefMult" ;
                          skos:definition "The multiplier applied to the reference pressure to determine the FAT maximum pressure value."@en ;
                          skos:prefLabel "Factory Acceptance Test Maximum Pressure Value Reference Multiplier"@en ,
                                         "Multiplicador de Referência de Valor de Pressão Máxima para Teste de Aceitação na Fábrica"@pt-br ;
                          edo:hasAttributeScope edo:InstanceLevelAttribute ;
                          edo:hasLifecycleCreationPhase edo:DetailedDesign ;
                          edo:hasTypedValue edo:FloatValue ;
                          edo:hasValueCardinality edo:SingleValue .


###  https://w3id.org/energy-domain/edo#FatNomPress
edo:FatNomPress rdf:type owl:Class ;
                rdfs:subClassOf edo:HydrostaticPressureTestsAttribute ;
                dcterms:accessRights "PUBLIC" ;
                dcterms:identifier "FatNomPress" ;
                skos:definition "Condições de teste dos tramos para Pressão - Nominal - FAT hidrostático"@pt-br ,
                                "The nominal pressure applied during the Factory Acceptance Test (FAT), simulating typical operating conditions to verify equipment performance."@en ;
                skos:prefLabel "Factory Acceptance Test Nominal Pressure"@en ,
                               "Pressão Nominal para o Teste de Aceitação na Fábrica"@pt-br ;
                edo:hasAttributeScope edo:InstanceLevelAttribute ;
                edo:hasLifecycleCreationPhase edo:DetailedDesign ;
                edo:hasTypedValue edo:FloatValue ;
                edo:hasUnit unit:PA ;
                edo:hasValueCardinality edo:SingleValue .


###  https://w3id.org/energy-domain/edo#FatNomPressValRef
edo:FatNomPressValRef rdf:type owl:Class ;
                      rdfs:subClassOf edo:HydrostaticPressureTestsAttribute ;
                      dcterms:accessRights "PUBLIC" ;
                      dcterms:identifier "FatNomPressValRef" ;
                      skos:definition "Comentários Condições de teste dos tramos para - Nominal - FAT hidrostático"@pt-br ,
                                      "Specifies the reference pressure used to determine the FAT nominal pressure value."@en ;
                      skos:prefLabel "Factory Acceptance Test Nominal Pressure Value Reference"@en ,
                                     "Referência de Valor de Pressão Nominal para o Teste de Aceitação na Fábrica"@pt-br ;
                      edo:hasAttributeScope edo:InstanceLevelAttribute ;
                      edo:hasLifecycleCreationPhase edo:DetailedDesign ;
                      edo:hasTypedValue edo:StringValue ;
                      edo:hasValueCardinality edo:SingleValue .


###  https://w3id.org/energy-domain/edo#FatNomPressValRefMult
edo:FatNomPressValRefMult rdf:type owl:Class ;
                          rdfs:subClassOf edo:HydrostaticPressureTestsAttribute ;
                          dcterms:accessRights "PUBLIC" ;
                          dcterms:identifier "FatNomPressValRefMult" ;
                          skos:definition "The multiplier applied to the reference pressure to determine the FAT nominal pressure value."@en ;
                          skos:prefLabel "Factory Acceptance Test Nominal Pressure Value Reference Multiplier"@en ,
                                         "Multiplicador de Referência de Valor de Pressão Nominal para Teste de Aceitação na Fábrica"@pt-br ;
                          edo:hasAttributeScope edo:InstanceLevelAttribute ;
                          edo:hasLifecycleCreationPhase edo:DetailedDesign ;
                          edo:hasTypedValue edo:FloatValue ;
                          edo:hasValueCardinality edo:SingleValue .


###  https://w3id.org/energy-domain/edo#FiberOpticJumper
edo:FiberOpticJumper rdf:type owl:Class ;
                     rdfs:subClassOf edo:LinearObject ;
                     dcterms:identifier "FiberOpticJumper" ;
                     skos:prefLabel "Jumper Ótico"@pt-br ,
                                    "Optical Jumper"@en .


###  https://w3id.org/energy-domain/edo#FiberRopeSegment
edo:FiberRopeSegment rdf:type owl:Class ;
                     rdfs:subClassOf edo:RopeSegment ;
                     dcterms:identifier "FiberRopeSegment" ;
                     skos:prefLabel "Fiber rope segment"@en ,
                                    "Tramo de cabo de fibra"@pt-br .


###  https://w3id.org/energy-domain/edo#FiberType
edo:FiberType rdf:type owl:Class ;
              rdfs:subClassOf edo:DomainAttribute ;
              dcterms:accessRights "PUBLIC" ;
              dcterms:identifier "FiberType" ;
              rdfs:comment "Tipo de fibra"@pt-br ;
              skos:definition "Fibre type"@en ;
              skos:prefLabel "Fiber type"@en ;
              edo:hasAttributeScope edo:TypeLevelAttribute ;
              edo:hasLifecycleCreationPhase edo:DetailedDesign ;
              edo:hasTypedValue edo:StringValue ;
              edo:hasValueCardinality edo:SingleValue .


###  https://w3id.org/energy-domain/edo#Filler
edo:Filler rdf:type owl:Class ;
           rdfs:subClassOf edo:IfcInstanciableElement ,
                           edo:UmbilicalComponent ;
           dcterms:identifier "Filler" ;
           skos:definition "Representa material de preenchimento utilizado em um componente umbilical para fornecer suporte estrutural ou separação entre linhas funcionais."@pt-br ,
                           "Represents filler material used within an umbilical component to provide structural support or separation between functional lines."@en ;
           skos:prefLabel "Enchimento"@pt-br ,
                          "Filler"@en ,
                          "Preenchimento"@pt-br ;
           edo:hasDiscipline edo:SubseaUmbilicalsEngineering .


###  https://w3id.org/energy-domain/edo#FinalBuoyancy
edo:FinalBuoyancy rdf:type owl:Class ;
                  rdfs:subClassOf edo:DomainAttribute ;
                  dcterms:accessRights "PUBLIC" ;
                  dcterms:identifier "FinalBuoyancy (EOF)" ;
                  rdfs:comment "Empuxo nominal fornecido pelo flutuador no final da vida útil"@pt-br ;
                  skos:definition "Empuxo nominal fornecido pelo módulo de flutuabilidade no final de sua vida útil"@pt-br ,
                                  "Nominal upthrust supplied by buoyancy module late in its lifespan"@en ;
                  skos:prefLabel "Final buoyancy"@en ,
                                 "Flutuabilidade final"@pt-br ;
                  edo:hasAttributeScope edo:TypeLevelAttribute ;
                  edo:hasLifecycleCreationPhase edo:DetailedDesign ;
                  edo:hasTypedValue edo:FloatValue ;
                  edo:hasValueCardinality edo:SingleValue .


###  https://w3id.org/energy-domain/edo#FinancialAttribute
edo:FinancialAttribute rdf:type owl:Class ;
                       rdfs:subClassOf edo:AttributeDomainCategory ;
                       rdfs:comment "Represents costs, prices, depreciation."@en ;
                       rdfs:label "Atributo Financeiro"@pt-br ,
                                  "Financial Attribute"@en ;
                       skos:definition "Representa custos, preços, depreciação"@pt-br ,
                                       "Represents costs, prices, depreciation"@en .


###  https://w3id.org/energy-domain/edo#FlangeAdapter
edo:FlangeAdapter rdf:type owl:Class ;
                  rdfs:subClassOf edo:PressureComponent ;
                  dcterms:identifier "FlangeAdapter" ;
                  skos:definition "Component enabling connection between two different flanges."@en ,
                                  "Peça que permite a conexão entre dois flanges diferentes."@pt-br ;
                  skos:prefLabel "Adaptador de Flange"@pt-br ,
                                 "Flange Adapter"@en ;
                  edo:hasAttribute edo:InnerDiameter ,
                                   edo:Length ;
                  edo:hasDiscipline edo:SubseaFlexiblePipesEngineering ,
                                    edo:SubseaUmbilicalsEngineering ;
                  edo:ifc_equivalentClass "IfcPipeFitting" ;
                  edo:ifc_objectType "FlangeAdapter" ;
                  edo:ifc_predefinedType "USERDEFINED" .


###  https://w3id.org/energy-domain/edo#FlangeAttribute
edo:FlangeAttribute rdf:type owl:Class ;
                    rdfs:subClassOf edo:DomainAttribute ;
                    rdfs:label "Flange Attribute"@en .


###  https://w3id.org/energy-domain/edo#FlangeConnection
edo:FlangeConnection rdf:type owl:Class ;
                     rdfs:subClassOf edo:FluidPort ;
                     dcterms:identifier "FlangeConnection" ;
                     skos:definition "Representa uma conexão lógica de porta de fluido definida por uma interface flangeada. Indica a localização lógica precisa em um modelo onde os componentes de distribuição de fluido são conectados, garantindo o alinhamento e a funcionalidade corretos do sistema durante a montagem e a instalação. Esse tipo de conexão define a interface entre os elementos de distribuição de fluido em sistemas submarinos ou outros sistemas de manuseio de fluido."@pt-br ,
                                     "Represents a logical fluid port connection defined by a flange interface. It indicates the precise logical location within a model where fluid distribution components are connected, ensuring correct alignment and functionality of the system during assembly and installation. This connection type defines the interface between fluid distribution elements in subsea or other fluid-handling systems."@en ;
                     skos:prefLabel "Conexão Flangeada"@pt-br ,
                                    "Flange Connection"@en ;
                     edo:hasDiscipline edo:SubseaUmbilicalsEngineering ;
                     edo:ifc_equivalentClass "IfcDistributionPort" ;
                     edo:ifc_objectType "FlangeConnection" ;
                     edo:ifc_predefinedType "USERDEFINED" .


###  https://w3id.org/energy-domain/edo#FlangeFaceType
edo:FlangeFaceType rdf:type owl:Class ;
                   rdfs:subClassOf edo:FlangeAttribute ;
                   dcterms:accessRights "PUBLIC" ;
                   dcterms:identifier "FlangeFaceType" ;
                   skos:definition "Specific design of the sealing surface used to ensure a secure, leak-tight connection. The face type plays a crucial role in maintaining the integrity of the seal under the extreme pressures and temperatures. It is engineered to prevent leaks, withstand high mechanical loads, and provide long-term durability. The appropriate face type is chosen based on factors such as pressure rating, sealing requirements, and environmental conditions."@en ;
                   skos:prefLabel "Flange Face Type"@en ,
                                  "Tipo da Face do Flange"@pt-br ;
                   edo:hasAttributeScope edo:TypeLevelAttribute ;
                   edo:hasLifecycleCreationPhase edo:DetailedDesign ;
                   edo:hasTypedValue edo:StringValue ;
                   edo:hasValueCardinality edo:SingleValue .


###  https://w3id.org/energy-domain/edo#FlangeType
edo:FlangeType rdf:type owl:Class ;
               rdfs:subClassOf edo:FlangeAttribute ;
               dcterms:accessRights "PUBLIC" ;
               dcterms:identifier "FlangeType" ;
               skos:definition "Specifies the type of flange within the Standard, which defines certain characteristics, like the Standard itself, Type or Class, Diameter and Operating Pressure."@en ;
               skos:prefLabel "Flange Type"@en ,
                              "Tipo de Flange"@pt-br ;
               edo:hasAttributeScope edo:TypeLevelAttribute ;
               edo:hasLifecycleCreationPhase edo:DetailedDesign ;
               edo:hasTypedValue edo:StringValue ;
               edo:hasValueCardinality edo:SingleValue .


###  https://w3id.org/energy-domain/edo#FlexiblePipeSegment
edo:FlexiblePipeSegment rdf:type owl:Class ;
                        rdfs:subClassOf edo:IfcInstanciableElement ,
                                        edo:PipeSegment ;
                        dcterms:identifier "FlexiblePipeSegment" ;
                        skos:altLabel "Flexible Line Section"@en ,
                                      "Flexible Pipe Section"@en ,
                                      "Flexible Pipe Segment"@en ,
                                      "Subsea Pipe Segment"@en ;
                        skos:definition "A segment of a flexible pipe that forms part of the overall pipeline system. The Flexible Pipe Segment is designed to transport fluids or gases over varying distances and conditions on the seafloor. Each section is engineered to handle specific environmental and operational requirements, contributing to the flexibility, durability, and performance of the subsea pipeline system."@en ,
                                        "Um segmento de duto flexível que faz parte do sistema de pipeline geral. O Tramo Flexível é projetado para transportar fluidos ou gases por distâncias e condições variadas no fundo do mar. Cada seção é projetada para atender a requisitos ambientais e operacionais específicos, contribuindo para a flexibilidade, durabilidade e desempenho do sistema de dutos submarinos."@pt-br ;
                        skos:prefLabel "Flexible Pipe Segment"@en ,
                                       "Tramo de Duto Flexível"@pt-br ;
                        edo:hasAttribute edo:AssemblyShouldObeyModelPolarity ,
                                         edo:EarlyLeakMaxPressTable_Press ,
                                         edo:EarlyLeakMaxPressTable_PressIntValStrat ,
                                         edo:EarlyLeakMaxPressTable_PressValRef ,
                                         edo:EarlyLeakMaxPressTable_PressValRefMult ,
                                         edo:EarlyLeakMaxPressTable_TensLimit ,
                                         edo:EarlyLeakMaxPressTable_TensLimitValRef ,
                                         edo:EarlyLeakNomPressTable_Press ,
                                         edo:EarlyLeakNomPressTable_PressIntValStrat ,
                                         edo:EarlyLeakNomPressTable_PressValRef ,
                                         edo:EarlyLeakNomPressTable_PressValRefMult ,
                                         edo:EarlyLeakNomPressTable_TensLimit ,
                                         edo:EarlyLeakNomPressTable_TensLimitValRef ,
                                         edo:FatMaxPress ,
                                         edo:FatMaxPressValRef ,
                                         edo:FatMaxPressValRefMult ,
                                         edo:FatNomPress ,
                                         edo:FatNomPressValRef ,
                                         edo:FatNomPressValRefMult ,
                                         edo:IdInUnifilarDiagram ,
                                         edo:ManufacturingDate ,
                                         edo:ManufacturingNonConformities ,
                                         edo:MaxLengthTolerance ,
                                         edo:NominalLength ,
                                         edo:OffLeakPLevMaxPress ,
                                         edo:OffLeakPLevMaxPressValRef ,
                                         edo:OffLeakPLevMaxPressValRefMult ,
                                         edo:OffLeakPLevNomPress ,
                                         edo:OffLeakPLevNomPressValRef ,
                                         edo:OffLeakPLevNomPressValRefMult ,
                                         edo:PipeSectionApplication ,
                                         edo:SpecialRequirements ,
                                         edo:StrIntOffPLevMaxPress ,
                                         edo:StrIntOffPLevMaxPressValRef ,
                                         edo:StrIntOffPLevMaxPressValRefMult ,
                                         edo:StrIntOffPLevNomPress ,
                                         edo:StrIntOffPLevNomPressValRef ,
                                         edo:StrIntOffPLevNomPressValRefMult ,
                                         edo:StrIntOnNoTensMaxPress ,
                                         edo:StrIntOnNoTensMaxPressValRef ,
                                         edo:StrIntOnNoTensMaxPressValRefMult ,
                                         edo:StrIntOnNoTensNomPress ,
                                         edo:StrIntOnNoTensNomPressValRef ,
                                         edo:StrIntOnNoTensNomPressValRefMult ;
                        edo:hasDiscipline edo:SubseaFlexiblePipesEngineering ;
                        edo:ifc_equivalentClass "IfcPipeSegment" ;
                        edo:ifc_objectType "FlexiblePipeSegment" ;
                        edo:ifc_predefinedType "USERDEFINED" .


###  https://w3id.org/energy-domain/edo#FlexiblePipeStructure
edo:FlexiblePipeStructure rdf:type owl:Class ;
                          rdfs:subClassOf edo:FlexibleStructure ,
                                          edo:IfcInstanciableElement ;
                          dcterms:identifier "FlexiblePipeStructure" ;
                          skos:altLabel "Flexible Structure"@en ,
                                        "Subsea Flexible Configuration"@en ,
                                        "Subsea Flexible Design"@en ;
                          skos:definition "A estrutura do duto flexível é a configuração em camadas, a SPEC, de um duto flexível, projetada para fornecer flexibilidade e resistência em ambientes subsea. Ela consiste em múltiplas camadas, cada uma servindo a uma função específica, como contenção de pressão, proteção ou reforço. Essa estrutura é projetada para atender às exigências das condições de águas profundas, incluindo alta pressão e movimentos dinâmicos, garantindo a integridade e o desempenho do duto."@pt-br ,
                                          "The Flexible Pipe Structure is the layered configuration, the specification, of a flexible pipe, designed to provide flexibility and strength in subsea environments. It consists of multiple layers, each serving a specific function, such as pressure containment, protection, or reinforcement. This structure is engineered to handle the demands of deepwater conditions, including high pressure and dynamic movements, ensuring the pipe's integrity and performance."@en ;
                          skos:prefLabel "Estrutura de Duto Flexível"@pt-br ,
                                         "Flexible Pipe Structure"@en ;
                          edo:hasAttribute edo:AxialStiffnessUnderCompressionAtSeaLevel ,
                                           edo:AxialStiffnessUnderTensionAtSeaLevel ,
                                           edo:CalculatedAbsoluteBurstPressure ,
                                           edo:DamagingPullInStraightLine ,
                                           edo:ErosionalVelocity ,
                                           edo:FlexibleStructureServicesList ,
                                           edo:FrictionCoefBetweenPipeAndTensioner ,
                                           edo:HydrostaticCollapseAbsPressDry ,
                                           edo:InternalDiameter ,
                                           edo:LimpTorsionalStiffnessAtSeaLevel ,
                                           edo:LinearMass ,
                                           edo:MaxDesignPressure ,
                                           edo:MaximumAllowableTensileForStraightLine ,
                                           edo:MinimumBendingRadiusForStorage ,
                                           edo:OuterDiameter ,
                                           edo:SpoolingTension ,
                                           edo:StiffTorsionalStiffnessAtSeaLevel ,
                                           edo:StructureApplicationsList ,
                                           edo:StructureCode ,
                                           edo:TensileArmourFreeAnnulusVolume ,
                                           edo:ThermalExchangeCoefficientFlooded ;
                          edo:hasDiscipline edo:SubseaFlexiblePipesEngineering ;
                          edo:ifc_equivalentClass "IfcPipeSegmentType" ;
                          edo:ifc_objectType "FlexiblePipeStructure" ;
                          edo:ifc_predefinedType "USERDEFINED" .


###  https://w3id.org/energy-domain/edo#FlexibleSegmentStatus
edo:FlexibleSegmentStatus rdf:type owl:Class ;
                          rdfs:subClassOf edo:DomainAttribute ;
                          dcterms:accessRights "PUBLIC" ;
                          dcterms:identifier "FlexibleSegmentStatus" ;
                          skos:definition "Status do tramo individual"@pt-br ,
                                          "Status of individual line segment"@en ;
                          skos:prefLabel "Status"@en ,
                                         "Status"@pt-br ;
                          edo:hasAttributeScope edo:TypeLevelAttribute ;
                          edo:hasLifecycleCreationPhase edo:DetailedDesign ;
                          edo:hasTypedValue edo:StringValue ;
                          edo:hasValueCardinality edo:SingleValue .


###  https://w3id.org/energy-domain/edo#FlexibleStructure
edo:FlexibleStructure rdf:type owl:Class ;
                      rdfs:subClassOf edo:Specification ;
                      skos:definition "A Estrutura Flexível é a configuração em camadas, a especificação, de um sistema flexível projetado para oferecer resistência, proteção e adaptabilidade em ambientes exigentes. Ela é composta por múltiplas camadas ou componentes, cada um desempenhando uma função específica, como reforço, contenção de pressão, isolamento ou comunicação. Projetada para acomodar movimentos, variações de pressão e cargas mecânicas, a estrutura flexível garante confiabilidade, durabilidade e desempenho em diferentes aplicações, incluindo dutos e umbilicais submarinos."@pt-br ,
                                      "The Flexible Structure is the layered configuration, the specification, of a flexible system designed to provide strength, protection, and adaptability in demanding environments. It consists of multiple layers or components, each performing a specific function such as reinforcement, pressure containment, insulation, or communication. Engineered to accommodate movement, pressure variations, and mechanical loads, the flexible structure ensures reliability, durability, and performance across different applications, including subsea pipelines and umbilicals."@en ;
                      skos:prefLabel "Estrutura Flexível"@pt-br ,
                                     "FlexibleStructure"@en ;
                      edo:hasAttribute edo:BendingStiffnessCurveAttribute ,
                                       edo:CrushingCurveAttribute ,
                                       edo:LayingMinimumRadiusCurveAttribute .


###  https://w3id.org/energy-domain/edo#FlexibleStructureLayer
edo:FlexibleStructureLayer rdf:type owl:Class ;
                           rdfs:subClassOf edo:FabricationComponent ;
                           dcterms:identifier "FlexibleStructureLayer" ;
                           skos:definition "A specific layer within the structure of a subsea flexible pipe, each designed to fulfill a distinct function. These layers work together to provide essential properties such as pressure containment, reinforcement, and environmental protection. Engineered to withstand harsh underwater conditions, each layer contributes to the overall flexibility, durability, and performance of the subsea flexible pipe system."@en ;
                           skos:prefLabel "Camadas de Estruturas Flexíveis"@pt-br ,
                                          "Flexible Structure Layer"@en ;
                           edo:hasAttribute edo:InternalDiameter ,
                                            edo:LayerAnnular ,
                                            edo:LayerAnnularType ,
                                            edo:LayerContinuity ,
                                            edo:LayerGeometryAttribute ,
                                            edo:LayerThickness ,
                                            edo:LayerWatertight ,
                                            edo:LayerWatertightLowerLayerInternalFreeVolume ,
                                            edo:LinearMass .


###  https://w3id.org/energy-domain/edo#FlexibleStructureLayerMaterial
edo:FlexibleStructureLayerMaterial rdf:type owl:Class ;
                                   rdfs:subClassOf edo:MaterialType ;
                                   dcterms:identifier "FlexibleStructureLayerMaterial" ;
                                   skos:definition "Material used to fabricate the individual layers of a subsea flexible structure, each layer serving a distinct function such as pressure containment, tensile reinforcement, or external protection. The Flexible Structure Layer Material is selected based on its specific properties, such as strength, flexibility, corrosion resistance, or thermal insulation, to ensure the overall performance and durability of the flexible pipe in harsh subsea conditions. These materials may include polymers, metals, composites, or other high-performance substances tailored to the pipe's operational demands."@en ;
                                   skos:prefLabel "Flexible Structure Layer Material"@en ,
                                                  "Materiais de Camadas de Estruturas Flexíveis Submarinas"@pt-br ;
                                   edo:hasAttribute edo:ElasticityModulusAt23Degrees ,
                                                    edo:MaterialComposition ,
                                                    edo:PoissonRatioAt23Degrees ,
                                                    edo:SpecificHeatCapacity ,
                                                    edo:SpecificWeight ,
                                                    edo:TechnicalNotes ,
                                                    edo:ThermalConductivityCoefficient .


###  https://w3id.org/energy-domain/edo#FlexibleStructureServicesList
edo:FlexibleStructureServicesList rdf:type owl:Class ;
                                  rdfs:subClassOf edo:DomainAttribute ;
                                  dcterms:accessRights "PUBLIC" ;
                                  dcterms:identifier "FlexibleStructureServicesList" ;
                                  skos:definition "Indicates the list of services that the flexible structure is capable of performing as part of a flexible pipeline. Multiple values can be selected, defining the operational roles the structure is designed to execute."@en ;
                                  skos:prefLabel "Flexible Structure Services List"@en ,
                                                 "Lista de Serviços da Estrutura Flexível"@pt-br ;
                                  edo:hasAttributeScope edo:TypeLevelAttribute ;
                                  edo:hasLifecycleCreationPhase edo:DetailedDesign ;
                                  edo:hasTypedValue edo:StringValue ;
                                  edo:hasValueCardinality edo:MultiValue .


###  https://w3id.org/energy-domain/edo#FloatValue
edo:FloatValue rdf:type owl:Class ;
               owl:equivalentClass [ rdf:type owl:Restriction ;
                                     owl:onProperty rdf:value ;
                                     owl:allValuesFrom xsd:float
                                   ] ;
               rdfs:subClassOf edo:DataType ;
               rdfs:comment "Constraint for xsd:float (32-bit floating point)"@en ;
               rdfs:label "Float Value"@en .


###  https://w3id.org/energy-domain/edo#FloatingProductionUnit
edo:FloatingProductionUnit rdf:type owl:Class ;
                           rdfs:subClassOf edo:IfcInstanciableElement ,
                                           edo:Location ;
                           dcterms:identifier "FloatingProductionUnit" ;
                           skos:altLabel "FLNG"@en ,
                                         "FPSO"@en ,
                                         "FPU"@en ,
                                         "Floating Platform"@en ,
                                         "Floating Production Facility"@en ;
                           skos:definition "Offshore platform used in oil and gas exploration and production, designed to extract, process, and store hydrocarbons. The Floating Production Unit (FPU) is anchored or moored to the seabed and can operate in deep waters, often connected to subsea wells via flexible pipes and umbilicals. It accommodates processing equipment for separating oil, gas, and water, as well as facilities for temporary storage or transfer of processed hydrocarbons to tankers or pipelines. FPUs are essential for the efficient and safe production of oil and gas in challenging offshore environments."@en ,
                                           "Plataforma offshore usada na exploração e produção de petróleo e gás, projetada para extrair, processar e armazenar hidrocarbonetos. A Unidade de Produção Flutuante (FPU) é ancorada ou amarrada ao leito marinho e pode operar em águas profundas, frequentemente conectada a poços submarinos por meio de dutos flexíveis e umbilicais. Ela acomoda equipamentos de processamento para separação de petróleo, gás e água, bem como instalações para armazenamento temporário ou transferência de hidrocarbonetos processados para navios-tanque ou dutos. As FPUs são essenciais para a produção eficiente e segura de petróleo e gás em ambientes offshore desafiadores."@pt-br ;
                           skos:prefLabel "Floating Production Unit"@en ,
                                          "Unidade de Produção Flutuante (UEP)"@pt-br ;
                           edo:hasDiscipline edo:SubseaUmbilicalsEngineering ;
                           edo:ifc_equivalentClass "IfcBuilding" ;
                           edo:ifc_objectType "FloatingProductionUnit" ;
                           edo:ifc_predefinedType "USERDEFINED" .


###  https://w3id.org/energy-domain/edo#FlowBase
edo:FlowBase rdf:type owl:Class ;
             rdfs:subClassOf edo:FlowControlEquipment ;
             dcterms:identifier "FlowBase" ;
             edo:hasDiscipline edo:WetChristmasTreesEngineering .


###  https://w3id.org/energy-domain/edo#FlowConnector
edo:FlowConnector rdf:type owl:Class ;
                  rdfs:subClassOf edo:PressureComponent ;
                  dcterms:identifier "FlowConnector" ;
                  skos:definition "Conector de grande porte para acoplamento submarino com um hub/mandril correspondente"@pt-br ,
                                  "Major connector for subsea tie-in to a corresponding hub"@en ;
                  skos:prefLabel "Conector de Fluxo"@pt-br ,
                                 "Flow Connector"@en .


###  https://w3id.org/energy-domain/edo#FlowControlEquipment
edo:FlowControlEquipment rdf:type owl:Class ;
                         rdfs:subClassOf edo:PressureEquipment ;
                         dcterms:identifier "FlowControlEquipment" ;
                         skos:definition "Equipamentos de uso permanente com funções de controle de fluidos de processo"@pt-br ,
                                         "Permament-use equipment with process fluid control functions"@en ;
                         skos:prefLabel "Equipamento de controle de fluxo"@pt-br ,
                                        "Flow control equipment"@en ;
                         edo:hasAttribute edo:HasThermalInsulation ,
                                          edo:NumberOfChokeValves ,
                                          edo:NumberOfRemoteProcessIsolationValves ,
                                          edo:Piggable .


###  https://w3id.org/energy-domain/edo#FlowControlModule
edo:FlowControlModule rdf:type owl:Class ;
                      rdfs:subClassOf edo:FlowControlEquipment ;
                      dcterms:identifier "FlowControlModule" ;
                      skos:definition "Module with pressure containment or flow control functions, installed as part of some larger unit or equipment"@en ,
                                      "Módulo com funções de contenção de pressão ou controle de fluxo, instalado como parte de uma unidade ou equipamento maior"@pt-br ;
                      skos:prefLabel "Flow control module"@en ,
                                     "Módulo de controle de fluxo"@pt-br .


###  https://w3id.org/energy-domain/edo#FlowLineMandrel
edo:FlowLineMandrel rdf:type owl:Class ;
                    rdfs:subClassOf edo:TieInEquipment ;
                    dcterms:identifier "FlowLineMandrel" ;
                    skos:definition "Equipamento para terminação e interligação de várias linhas simultaneamente"@pt-br ,
                                    "Equipment for terminating and connecting multiple lines simultaneously"@en ;
                    skos:prefLabel "Flow line mandrel"@en ,
                                   "Mandril das linhas de fluxo"@pt-br ;
                    edo:hasDiscipline edo:WetChristmasTreesEngineering .


###  https://w3id.org/energy-domain/edo#FlowbaseRunningTool
edo:FlowbaseRunningTool rdf:type owl:Class ;
                        rdfs:subClassOf edo:RunningTool ;
                        dcterms:identifier "FlowbaseRunningTool" ;
                        skos:prefLabel "Ferramenta de instalação de BAP"@pt-br ,
                                       "Flowbase running tool"@en .


###  https://w3id.org/energy-domain/edo#FlowlineSpan
edo:FlowlineSpan rdf:type owl:Class ;
                 rdfs:subClassOf edo:IfcInstanciableElement ,
                                 edo:PipelineSpan ;
                 dcterms:identifier "FlowlineSpan" ;
                 skos:definition "Trecho de duto não suspenso, estendido sobre ou sob o solo"@pt-br ,
                                 "Unsuspended pipeline span, laid over or under ground"@en ;
                 skos:prefLabel "Flowline span"@en ,
                                "Trecho flowline"@pt-br ;
                 edo:hasDiscipline edo:SubseaFlexiblePipesEngineering .


###  https://w3id.org/energy-domain/edo#FluidPort
edo:FluidPort rdf:type owl:Class ;
              rdfs:subClassOf edo:Port ;
              dcterms:identifier "FluidPort" ;
              skos:definition "Elemento lógico que representa uma interface de conexão destinada ao fluxo de fluidos, descrevendo a capacidade de ligação entre sistemas ou componentes."@pt-br ,
                              "Logical element representing a connection interface for fluid flow, defining the capability to link systems or components."@en ;
              skos:prefLabel "Fluid Port"@en ,
                             "Ponto de Conexão de Distribuição"@pt-br .


###  https://w3id.org/energy-domain/edo#FractureToughness
edo:FractureToughness rdf:type owl:Class ;
                      rdfs:subClassOf edo:DomainAttribute ;
                      dcterms:accessRights "PUBLIC" ;
                      dcterms:identifier "FractureToughness" ;
                      skos:definition "Represents the material's ability to resist fracture when subjected to stress, particularly in the presence of flaws or cracks. This property is essential for assessing the material's capacity to withstand cracking or failure under load conditions."@en ,
                                      "Tenacidade à fratura (Específica para Materiais Metálicos)."@pt-br ;
                      skos:prefLabel "Fracture Toughness"@en ,
                                     "Tenacidade à Fratura"@pt-br ;
                      edo:hasAttributeScope edo:TypeLevelAttribute ;
                      edo:hasLifecycleCreationPhase edo:DetailedDesign ;
                      edo:hasTypedValue edo:FloatValue ;
                      edo:hasUnit unit:PA ,
                                  unit:PA-M0dot5 ;
                      edo:hasValueCardinality edo:SingleValue .


###  https://w3id.org/energy-domain/edo#FrictionCoefBetweenPipeAndTensioner
edo:FrictionCoefBetweenPipeAndTensioner rdf:type owl:Class ;
                                        rdfs:subClassOf edo:DomainAttribute ;
                                        dcterms:accessRights "PUBLIC" ;
                                        dcterms:identifier "FrictionCoefBetweenPipeAndTensioner" ;
                                        skos:definition "Coeficiente de atrito entre a sapata e a capa externa (passagem tensionador)."@pt-br ,
                                                        "Represents the coefficient of friction between the pipe and the tensioner during installation or operation. This property is critical for determining the resistance to sliding between the two surfaces, influencing the tension control and handling of the pipe."@en ;
                                        skos:prefLabel "Coeficiente de Atrito entre o Duto e o Tensionador"@pt-br ,
                                                       "Friction Coefficient Between Pipe And Tensioner"@en ;
                                        edo:hasAttributeScope edo:TypeLevelAttribute ;
                                        edo:hasLifecycleCreationPhase edo:DetailedDesign ;
                                        edo:hasTypedValue edo:FloatValue ;
                                        edo:hasValueCardinality edo:SingleValue .


###  https://w3id.org/energy-domain/edo#FrictionCoeffSheathArmor
edo:FrictionCoeffSheathArmor rdf:type owl:Class ;
                             rdfs:subClassOf edo:DomainAttribute ;
                             dcterms:accessRights "PUBLIC" ;
                             dcterms:identifier "FrictionCoeffSheathArmor" ;
                             rdfs:comment "Coeficiente de atrito entre capa externa e a camada de armadura imediatamente abaixo dela"@pt-br ;
                             skos:definition "Friction coefficient between outer sheath and immediately underlying armor layer"@en ;
                             skos:prefLabel "Coeficiente de atrito, capa externa vs. armadura"@pt-br ,
                                            "Friction coefficient, outer sheath vs. armor"@en ;
                             edo:hasAttributeScope edo:TypeLevelAttribute ;
                             edo:hasLifecycleCreationPhase edo:DetailedDesign ;
                             edo:hasTypedValue edo:FloatValue ;
                             edo:hasValueCardinality edo:SingleValue .


###  https://w3id.org/energy-domain/edo#FrictionCoeffSheathTensioner
edo:FrictionCoeffSheathTensioner rdf:type owl:Class ;
                                 rdfs:subClassOf edo:DomainAttribute ;
                                 dcterms:accessRights "PUBLIC" ;
                                 dcterms:identifier "FrictionCoeffSheathTensioner" ;
                                 rdfs:comment "Coeficiente de atrito entre capa externa e sapata do tensionador"@pt-br ;
                                 skos:definition "Fricion coefficient between outer sheath and tensioner pads"@en ;
                                 skos:prefLabel "Coeficiente de atrito, capa externa vs. tensionador"@pt-br ,
                                                "Friction coefficient, outer sheath vs. tensioner"@en ;
                                 edo:hasAttributeScope edo:TypeLevelAttribute ;
                                 edo:hasLifecycleCreationPhase edo:DetailedDesign ;
                                 edo:hasTypedValue edo:FloatValue ;
                                 edo:hasValueCardinality edo:SingleValue .


###  https://w3id.org/energy-domain/edo#FrictionCoefficientTighteningTable_CoefficientOfFriction
edo:FrictionCoefficientTighteningTable_CoefficientOfFriction rdf:type owl:Class ;
                                                             rdfs:subClassOf edo:CrushingFrictionCoefficientTighteningTableColumn ;
                                                             dcterms:accessRights "PUBLIC" ;
                                                             dcterms:identifier "FrictionCoefficientTighteningTable_CoefficientOfFriction" ;
                                                             skos:definition "Represents the ratio that describes the force of friction between two surfaces in contact, relative to the normal force pressing them together. This property is important for evaluating the resistance to sliding or movement, ensuring proper performance of components under operational conditions."@en ;
                                                             skos:prefLabel "Coefficient Of Friction"@en ,
                                                                            "Coeficiente de Atrito"@pt-br ;
                                                             edo:hasAttributeScope edo:TypeLevelAttribute ;
                                                             edo:hasLifecycleCreationPhase edo:DetailedDesign ;
                                                             edo:hasTypedValue edo:FloatValue ;
                                                             edo:hasValueCardinality edo:MultiValue .


###  https://w3id.org/energy-domain/edo#FrictionCoefficientTighteningTable_TighteningPerTrack
edo:FrictionCoefficientTighteningTable_TighteningPerTrack rdf:type owl:Class ;
                                                          rdfs:subClassOf edo:CrushingFrictionCoefficientTighteningTableColumn ;
                                                          dcterms:accessRights "PUBLIC" ;
                                                          dcterms:identifier "FrictionCoefficientTighteningTable_TighteningPerTrack" ;
                                                          skos:definition "Indicates the amount of tightening applied per track during an operation. This property is important for ensuring consistent force distribution across multiple tracks, helping to maintain proper alignment and secure attachment during the tightening process."@en ;
                                                          skos:prefLabel "Aperto por lagarta"@pt-br ,
                                                                         "Tightening Per Track"@en ;
                                                          edo:hasAttributeScope edo:TypeLevelAttribute ;
                                                          edo:hasLifecycleCreationPhase edo:DetailedDesign ;
                                                          edo:hasTypedValue edo:FloatValue ;
                                                          edo:hasUnit unit:N-PER-M ;
                                                          edo:hasValueCardinality edo:MultiValue .


###  https://w3id.org/energy-domain/edo#FullyThreaded
edo:FullyThreaded rdf:type owl:Class ;
                  rdfs:subClassOf edo:DomainAttribute ;
                  dcterms:accessRights "PUBLIC" ;
                  dcterms:identifier "FullyThreaded" ;
                  skos:definition "Indicates whether the component will be used fully threaded (TRUE) or not (FALSE)."@en ;
                  skos:prefLabel "Completamente Rosqueado"@pt-br ,
                                 "Fully Threaded"@en ;
                  edo:hasAttributeScope edo:InstanceLevelAttribute ;
                  edo:hasLifecycleCreationPhase edo:DetailedDesign ;
                  edo:hasTypedValue edo:BooleanValue ;
                  edo:hasValueCardinality edo:SingleValue .


###  https://w3id.org/energy-domain/edo#FunctionLine
edo:FunctionLine rdf:type owl:Class ;
                 rdfs:subClassOf edo:UmbilicalComponent ;
                 dcterms:identifier "FunctionLine" ;
                 skos:definition "Representa uma linha dentro de um componente umbilical que desempenha uma função específica, como transmissão elétrica, óptica ou de fluido."@pt-br ,
                                 "Represents a line within an umbilical component that carries a specific function, such as electrical, optical, or fluid transmission."@en ;
                 skos:prefLabel "Function Line"@en ,
                                "Function line"@en ,
                                "Linha Funcional"@pt-br ,
                                "Linha de função"@pt-br ;
                 edo:hasAttribute edo:DestinationPigtailLength ,
                                  edo:MinimumBendingRadius ,
                                  edo:SourcePigtailLength .


###  https://w3id.org/energy-domain/edo#FunctionalAttribute
edo:FunctionalAttribute rdf:type owl:Class ;
                        rdfs:subClassOf edo:AttributeDomainCategory ;
                        rdfs:comment "Describes how the equipment functions or performs its intended purpose."@en ;
                        rdfs:label "Atributo Funcional"@pt-br ,
                                   "Functional Attribute"@en ;
                        skos:definition "Representa características operacionais e capacidades do equipamento"@pt-br ,
                                        "Represents operational characteristics and capabilities of the equipment"@en .


###  https://w3id.org/energy-domain/edo#GalvanicMaterial
edo:GalvanicMaterial rdf:type owl:Class ;
                     rdfs:subClassOf edo:DomainAttribute ;
                     dcterms:accessRights "PUBLIC" ;
                     dcterms:identifier "GalvanicMaterial" ;
                     skos:definition "Refers to the material used in galvanic protection systems, which is typically a metal or alloy designed to corrode in place of the protected structure. This material is selected for its ability to act as a sacrificial anode in a galvanic cell, thereby preventing corrosion of the primary structure, such as a subsea flexible pipeline. The choice of galvanic material is critical for the long-term protection and integrity of the pipeline system."@en ;
                     skos:prefLabel "Galvanic Material"@en ,
                                    "Material Galvânico"@pt-br ;
                     edo:hasAttributeScope edo:TypeLevelAttribute ;
                     edo:hasLifecycleCreationPhase edo:DetailedDesign ;
                     edo:hasTypedValue edo:StringValue ;
                     edo:hasValueCardinality edo:SingleValue .


###  https://w3id.org/energy-domain/edo#Gender
edo:Gender rdf:type owl:Class ;
           rdfs:subClassOf edo:HoseFittingSpecTableColumn ;
           dcterms:accessRights "PUBLIC" ;
           dcterms:identifier "Gender" ;
           skos:prefLabel "Gender"@en ,
                          "Gênero"@pt-br ;
           edo:hasAttributeScope edo:TypeLevelAttribute ;
           edo:hasLifecycleCreationPhase edo:DetailedDesign ;
           edo:hasTypedValue edo:StringValue ;
           edo:hasValueCardinality edo:SingleValue .


###  https://w3id.org/energy-domain/edo#Geothermal
edo:Geothermal rdf:type owl:Class ;
               rdfs:subClassOf edo:Renewable ;
               rdfs:label "Energia Geotérmica"@pt-br ,
                          "Geothermal Energy"@en ;
               skos:definition "Energia derivada do calor armazenado abaixo da superfície da Terra."@pt-br ,
                               "Energy derived from heat stored beneath the Earth's surface."@en .


###  https://w3id.org/energy-domain/edo#GeothermalDirectUse
edo:GeothermalDirectUse rdf:type owl:Class ;
                        rdfs:subClassOf edo:Geothermal ;
                        dcterms:identifier "GeothermalDirectUse" ;
                        skos:definition "Direct use of geothermal energy takes advantage of low or medium temperature geothermal resources for heating buildings, greenhouses, aquaculture facilities, or industrial processes."@en ,
                                        "O uso direto da energia geotérmica aproveita recursos geotérmicos de baixa ou média temperatura para aquecer edifícios, estufas, instalações de aquicultura ou processos industriais."@pt-br ;
                        skos:prefLabel "Geothermal Direct Use"@en ,
                                       "Uso Direto Geotérmico"@pt-br .


###  https://w3id.org/energy-domain/edo#GeothermalElectricity
edo:GeothermalElectricity rdf:type owl:Class ;
                          rdfs:subClassOf edo:Geothermal ;
                          dcterms:identifier "GeothermalElectricity" ;
                          skos:definition "A geração elétrica geotérmica utiliza recursos geotérmicos de alta entalpia para produzir vapor que aciona turbinas e gera energia renovável. É aplicada principalmente em regiões vulcânicas com reservatórios geotérmicos acessíveis."@pt-br ,
                                          "Geothermal electricity generation uses high-enthalpy geothermal resources to produce steam that drives turbines and generates renewable power. It is mainly applied in volcanic regions with accessible geothermal reservoirs."@en ;
                          skos:prefLabel "Geothermal Electricity Generation"@en ,
                                         "Geração Elétrica Geotérmica"@pt-br .


###  https://w3id.org/energy-domain/edo#GrooveHeight
edo:GrooveHeight rdf:type owl:Class ;
                 rdfs:subClassOf edo:DomainAttribute ;
                 dcterms:accessRights "PUBLIC" ;
                 dcterms:identifier "GrooveHeight" ;
                 skos:definition "Specifies the vertical dimension of the groove from its base to the top edge. This measurement is crucial for ensuring that the groove can accommodate the intended components or fittings properly, allowing for a secure and precise fit. The groove height helps to determine the correct depth and functionality of the groove in relation to the end fitting and the overall installation process."@en ;
                 skos:prefLabel "Altura do Groove"@pt-br ,
                                "Groove Height"@en ;
                 edo:hasAttributeScope edo:InstanceLevelAttribute ;
                 edo:hasLifecycleCreationPhase edo:DetailedDesign ;
                 edo:hasTypedValue edo:FloatValue ;
                 edo:hasUnit unit:M ;
                 edo:hasValueCardinality edo:SingleValue .


###  https://w3id.org/energy-domain/edo#GroovePoint
edo:GroovePoint rdf:type owl:Class ;
                rdfs:subClassOf edo:IfcInstanciableElement ,
                                edo:SupportRegion ;
                dcterms:identifier "GroovePoint" ;
                skos:definition "O Groove Point é um ponto designado na linha de centro do componente, usado para indicar a posição exata de um sulco. O sulco em si é uma área rebaixada projetada para auxiliar na fixação do componente durante a instalação, garantindo que ele permaneça firmemente no lugar durante o processo. O Groove Support Point fornece uma referência para localizar o sulco, facilitando o alinhamento e o posicionamento precisos necessários para uma instalação adequada."@en ,
                                "Ponto na linha de centro do End Fitting para indicar a posição do Groove"@pt-br ;
                skos:prefLabel "Groove Point"@en ,
                               "Ponto de Groove"@pt-br ;
                edo:hasAttribute edo:GrooveHeight ;
                edo:hasDiscipline edo:SubseaFlexiblePipesEngineering ,
                                  edo:SubseaUmbilicalsEngineering ;
                edo:ifc_equivalentClass "IfcDistributionPort" ;
                edo:ifc_objectType "GroovePoint" ;
                edo:ifc_predefinedType "USERDEFINED" .


###  https://w3id.org/energy-domain/edo#GroupShieldingType
edo:GroupShieldingType rdf:type owl:Class ;
                       rdfs:subClassOf edo:DomainAttribute ;
                       dcterms:accessRights "PUBLIC" ;
                       dcterms:identifier "GroupShieldingType" ;
                       rdfs:comment "Especifica o tipo de blindagem eletromagnética aplicada a cada grupo de condutores relacionados"@pt-br ;
                       skos:definition "Specifies the type of electromagnetic shielding applied to each group of related conductors"@en ;
                       skos:prefLabel "Group shielding type"@en ,
                                      "Tipo de blindagem dos grupos"@pt-br ;
                       edo:hasAttributeScope edo:TypeLevelAttribute ;
                       edo:hasLifecycleCreationPhase edo:DetailedDesign ;
                       edo:hasTypedValue edo:StringValue ;
                       edo:hasValueCardinality edo:SingleValue .


###  https://w3id.org/energy-domain/edo#GroutBag
edo:GroutBag rdf:type owl:Class ;
             rdfs:subClassOf edo:PipeSupport ;
             dcterms:identifier "GroutBag" ;
             skos:prefLabel "Grout bag"@en ,
                            "Grout bag"@pt-br .


###  https://w3id.org/energy-domain/edo#GuideBase
edo:GuideBase rdf:type owl:Class ;
              rdfs:subClassOf edo:Structure ;
              dcterms:identifier "GuideBase" ;
              skos:prefLabel "Base-guia"@pt-br ,
                             "Guide base"@en .


###  https://w3id.org/energy-domain/edo#H2SVolumeConcentration
edo:H2SVolumeConcentration rdf:type owl:Class ;
                           rdfs:subClassOf edo:DomainAttribute ;
                           dcterms:accessRights "PUBLIC" ;
                           dcterms:identifier "H2SVolumeConcentration" ;
                           skos:definition "Represents the concentration of hydrogen sulfide (H2S) in the total volume of the gas mixture, expressed in parts per million by volume (ppmv). This value is crucial for assessing material compatibility and corrosion risks in subsea flexible pipelines, as H2S is highly corrosive and can significantly impact the integrity and lifespan of the pipeline. Accurate measurement of H2S concentration is essential for ensuring the safe and reliable operation of the pipeline in harsh environments."@en ;
                           skos:prefLabel "Concentração Volumétrica de Sulfeto de Hidrogênio (H2S)"@pt-br ,
                                          "Hydrogen Sulfide (H2S) Volume Concentration"@en ;
                           edo:hasAttributeScope edo:InstanceLevelAttribute ;
                           edo:hasLifecycleCreationPhase edo:BasicDesign ;
                           edo:hasTypedValue edo:FloatValue ;
                           edo:hasUnit unit:MicroM3-PER-M3 ;
                           edo:hasValueCardinality edo:SingleValue .


###  https://w3id.org/energy-domain/edo#HCM
edo:HCM rdf:type owl:Class ;
        rdfs:subClassOf edo:ConnectionModule ;
        dcterms:identifier "HCM" ;
        skos:prefLabel "Horizontal connection module"@en ,
                       "Módulo de conexão horizontal"@pt-br ;
        edo:hasDiscipline edo:WetChristmasTreesEngineering .


###  https://w3id.org/energy-domain/edo#HCRHose
edo:HCRHose rdf:type owl:Class ;
            rdfs:subClassOf edo:IfcInstanciableElement ,
                            edo:Tubing ;
            dcterms:identifier "HCRHose" ;
            skos:definition "High Collapse Resistant Hose"@en ,
                            "Representa uma mangueira de borracha de alta pressão utilizada em tubulações para transporte de fluido em sistemas umbilicais."@pt-br ,
                            "Represents a high-pressure rubber hose used within tubing for fluid transport in umbilical systems."@en ;
            skos:prefLabel "HCR Hose"@en ,
                           "Mangueira HCR"@pt-br ;
            edo:hasDiscipline edo:SubseaUmbilicalsEngineering ;
            edo:ifc_equivalentClass "IfcPipeSegment" ;
            edo:ifc_objectType "HCRHose" ;
            edo:ifc_predefinedType "USERDEFINED" .


###  https://w3id.org/energy-domain/edo#HPHousing
edo:HPHousing rdf:type owl:Class ;
              rdfs:subClassOf edo:PressureComponent ;
              dcterms:identifier "HPHousing" ;
              skos:prefLabel "Alojador de alta pressão"@pt-br ,
                             "High-pressure housing"@en .


###  https://w3id.org/energy-domain/edo#HVACEngineering
edo:HVACEngineering rdf:type owl:Class ;
                    rdfs:subClassOf edo:TechnicalDiscipline ;
                    rdfs:label "Engenharia de HVAC"@pt-br ,
                               "HVAC Engineering"@en ;
                    skos:definition "Disciplina de engenharia focada em sistemas de aquecimento, ventilação e ar condicionado."@pt-br ,
                                    "Engineering discipline focused on heating, ventilation and air conditioning systems."@en .


###  https://w3id.org/energy-domain/edo#HandlingCollar
edo:HandlingCollar rdf:type owl:Class ;
                   rdfs:subClassOf edo:IfcInstanciableElement ,
                                   edo:SplitCollar ;
                   dcterms:identifier "HandlingCollar" ;
                   skos:altLabel "Handling Clamp"@en ,
                                 "Installation Collar"@en ,
                                 "Lifting Collar"@en ,
                                 "Support Collar"@en ;
                   skos:definition "Device used in subsea operations to facilitate the safe handling, lifting, and maneuvering of flexible pipes or heavy components during installation or retrieval. Typically attached around the pipe or component, it provides secure lifting points for cranes or other lifting equipment. Designed to distribute the load evenly, it prevents damage to the pipe or equipment while ensuring efficient and controlled movements in subsea environments."@en ;
                   skos:prefLabel "Colar de Manuseio"@pt-br ,
                                  "Handling Collar"@en ;
                   edo:hasAttribute edo:FlangeType ,
                                    edo:InternalDiameter ,
                                    edo:MaxDynamicLoad ,
                                    edo:SafeWorkingLoad ,
                                    edo:UpperItubeDiameter ;
                   edo:hasDiscipline edo:SubseaFlexiblePipesEngineering ,
                                     edo:SubseaUmbilicalsEngineering ;
                   edo:ifc_equivalentClass "IfcPipeFitting" ;
                   edo:ifc_objectType "HandlingCollar" ;
                   edo:ifc_predefinedType "USERDEFINED" .


###  https://w3id.org/energy-domain/edo#HangOffCollar
edo:HangOffCollar rdf:type owl:Class ;
                  rdfs:subClassOf edo:IfcInstanciableElement ,
                                  edo:LineAncillary ;
                  dcterms:identifier "HangOffCollar" ;
                  skos:altLabel "Hang-Off Clamp"@en ,
                                "Hang-Off Device"@en ,
                                "Support Collar"@en ,
                                "Termination Collar"@en ;
                  skos:definition "Device used to secure and support flexible pipes or risers during installation, particularly when they are suspended from a platform or vessel. It provides a stable attachment point, distributing the load and preventing excessive movement or strain on the pipe. The Hang Off Collar is crucial for maintaining the integrity of the pipe while it is held in place before final connection or during temporary suspension in subsea operations."@en ,
                                  "Flange bipartido para suporte de um riser"@pt-br ;
                  skos:prefLabel "Hang Off Collar"@en ,
                                 "Sistema de Suspensão"@pt-br ;
                  edo:hasAttribute edo:CollarInternalDiameter ,
                                   edo:FlangeType ,
                                   edo:MaxDynamicLoad ,
                                   edo:SafeWorkingLoad ,
                                   edo:UpperItubeDiameter ;
                  edo:hasDiscipline edo:SubseaFlexiblePipesEngineering ,
                                    edo:SubseaUmbilicalsEngineering ;
                  edo:ifc_equivalentClass "IfcPipeFitting" ;
                  edo:ifc_objectType "HangOffCollar" ;
                  edo:ifc_predefinedType "USERDEFINED" .


###  https://w3id.org/energy-domain/edo#HardwareItem
edo:HardwareItem rdf:type owl:Class ;
                 rdfs:subClassOf edo:Component ;
                 dcterms:identifier "HardwareItem" ;
                 skos:definition "Itens mecânicos simples como ferragens, fixadores, vedações, etc."@pt-br ,
                                 "Simple mechanical items such as pipe components, etc."@en ;
                 skos:prefLabel "Hardware Item"@en ,
                                "Item de Hardware"@pt-br .


###  https://w3id.org/energy-domain/edo#HasFaceORing
edo:HasFaceORing rdf:type owl:Class ;
                 rdfs:subClassOf edo:DomainAttribute ;
                 dcterms:accessRights "PUBLIC" ;
                 dcterms:identifier "HasFaceORing" ;
                 skos:definition "Indicates whether the item has a face o-ring (TRUE) or not (FALSE)."@en ;
                 skos:prefLabel "Has Face O-Ring"@en ,
                                "Possui O-Ring na Face"@pt-br ;
                 edo:hasAttributeScope edo:TypeLevelAttribute ;
                 edo:hasLifecycleCreationPhase edo:DetailedDesign ;
                 edo:hasTypedValue edo:BooleanValue ;
                 edo:hasValueCardinality edo:SingleValue .


###  https://w3id.org/energy-domain/edo#HasModaSensor
edo:HasModaSensor rdf:type owl:Class ;
                  rdfs:subClassOf edo:DomainAttribute ;
                  dcterms:accessRights "PUBLIC" ;
                  dcterms:identifier "HasModaSensor" ;
                  skos:definition "Indicates whether the item includes a MODA sensor (TRUE) or Not (FALSE)."@en ;
                  skos:prefLabel "Has Moda Sensor"@en ,
                                 "Possui Sensor MODA"@pt-br ;
                  edo:hasAttributeScope edo:TypeLevelAttribute ;
                  edo:hasLifecycleCreationPhase edo:DetailedDesign ;
                  edo:hasTypedValue edo:BooleanValue ;
                  edo:hasValueCardinality edo:SingleValue .


###  https://w3id.org/energy-domain/edo#HasN2InjectionPort
edo:HasN2InjectionPort rdf:type owl:Class ;
                       rdfs:subClassOf edo:DomainAttribute ;
                       dcterms:accessRights "PUBLIC" ;
                       dcterms:identifier "HasN2InjectionPort" ;
                       skos:definition "Indicates whether the item includes a nitrogen (N2) injection port (TRUE) or Not (FALSE)."@en ;
                       skos:prefLabel "Has N2 Injection Port"@en ,
                                      "Possui Porta de Injeção de Nitrogênio"@pt-br ;
                       edo:hasAttributeScope edo:TypeLevelAttribute ;
                       edo:hasLifecycleCreationPhase edo:DetailedDesign ;
                       edo:hasTypedValue edo:BooleanValue ;
                       edo:hasValueCardinality edo:SingleValue .


###  https://w3id.org/energy-domain/edo#HasThermalInsulation
edo:HasThermalInsulation rdf:type owl:Class ;
                         rdfs:subClassOf edo:DomainAttribute ;
                         dcterms:accessRights "PUBLIC" ;
                         dcterms:identifier "HasThermalInsulation" ;
                         skos:prefLabel "Has Thermal Insulation"@en ,
                                        "Possui isolamento térmico"@pt-br ;
                         edo:hasAttributeScope edo:TypeLevelAttribute ;
                         edo:hasLifecycleCreationPhase edo:DetailedDesign ;
                         edo:hasTypedValue edo:BooleanValue ;
                         edo:hasValueCardinality edo:SingleValue .


###  https://w3id.org/energy-domain/edo#HighStrengthTape
edo:HighStrengthTape rdf:type owl:Class ;
                     rdfs:subClassOf edo:IfcInstanciableElement ,
                                     edo:TapeLayer ;
                     dcterms:identifier "HighStrengthTape" ;
                     skos:definition "Material used in subsea flexible pipes, typically applied as a reinforcing layer to provide additional strength and resistance to external forces. High Strength Tape is designed to improve the tensile properties of the flexible pipe, enhancing its ability to withstand high internal pressures, tension, and dynamic loads in harsh subsea environments. It is typically made from advanced fibers or composite materials, ensuring durability and long-term performance in demanding conditions."@en ;
                     skos:prefLabel "Fita de Alta Resistência"@pt-br ,
                                    "High Strength Tape"@en ;
                     edo:hasDiscipline edo:SubseaFlexiblePipesEngineering ;
                     edo:ifc_equivalentClass "IfcPipeSegment" ;
                     edo:ifc_objectType "HighStrengthTape" ;
                     edo:ifc_predefinedType "USERDEFINED" .


###  https://w3id.org/energy-domain/edo#HistoricalAttribute
edo:HistoricalAttribute rdf:type owl:Class ;
                        rdfs:subClassOf edo:AttributeDomainCategory ;
                        rdfs:comment "Represents records of past events, inspections, or modifications."@en ;
                        rdfs:label "Atributo Histórico"@pt-br ,
                                   "Historical Attribute"@en ;
                        skos:definition "Representa registros de eventos passados, inspeções ou modificações"@pt-br ,
                                        "Represents records of past events, inspections, or modifications"@en .


###  https://w3id.org/energy-domain/edo#HoldingBandage
edo:HoldingBandage rdf:type owl:Class ;
                   rdfs:subClassOf edo:IfcInstanciableElement ,
                                   edo:TapeLayer ;
                   dcterms:identifier "HoldingBandage" ;
                   skos:definition "Reinforcement layer used in subsea flexible pipes to secure and hold internal components in place during manufacturing and operation. The Holding Bandage helps maintain the alignment and stability of the various layers of the pipe, preventing displacement or movement under dynamic conditions. Typically made from high-strength, flexible materials, it contributes to the overall durability and structural integrity of the pipe, ensuring reliable performance in harsh subsea environments."@en ;
                   skos:prefLabel "Bandagem de Reforço"@pt-br ,
                                  "Holding Bandage"@en ;
                   edo:hasAttribute edo:ModulusOfElasticity ,
                                    edo:StressAtDesignPressure ,
                                    edo:TapesQuantity ;
                   edo:hasDiscipline edo:SubseaFlexiblePipesEngineering ;
                   edo:ifc_equivalentClass "IfcPipeSegment" ;
                   edo:ifc_objectType "HoldingBandage" ;
                   edo:ifc_predefinedType "USERDEFINED" .


###  https://w3id.org/energy-domain/edo#Hook
edo:Hook rdf:type owl:Class ;
         rdfs:subClassOf edo:MooringAccessory ;
         dcterms:identifier "Hook" ;
         skos:prefLabel "Gancho"@pt-br ,
                        "Hook"@en .


###  https://w3id.org/energy-domain/edo#HoseFittingSpecTableAttribute
edo:HoseFittingSpecTableAttribute rdf:type owl:Class ;
                                  rdfs:subClassOf edo:DomainAttribute ;
                                  rdfs:label "Hose Fitting Spec Table" .


###  https://w3id.org/energy-domain/edo#HoseFittingSpecTableColumn
edo:HoseFittingSpecTableColumn rdf:type owl:Class ;
                               rdfs:subClassOf edo:HoseFittingSpecTableAttribute .


###  https://w3id.org/energy-domain/edo#HotStab
edo:HotStab rdf:type owl:Class ;
            rdfs:subClassOf edo:HydraulicJumperConnector ;
            dcterms:identifier "HotStab" ;
            skos:definition "Representa um tipo de conector jumper hidráulico projetado para operações de conexão/desconexão rápida sob pressão."@pt-br ,
                            "Represents a type of hydraulic jumper connector designed for quick connect/disconnect operations under pressure."@en ;
            skos:prefLabel "Hot Stab"@en ,
                           "Hot Stab"@pt-br ;
            edo:hasDiscipline edo:SubseaFlexiblePipesEngineering ,
                              edo:SubseaUmbilicalsEngineering ;
            edo:ifc_equivalentClass "IfcPipeFitting" ;
            edo:ifc_objectType "HotStab" .


###  https://w3id.org/energy-domain/edo#HotStabReceptacle
edo:HotStabReceptacle rdf:type owl:Class ;
                      rdfs:subClassOf edo:PanelHydraulicConnector ;
                      dcterms:identifier "HotStabReceptacle" ;
                      skos:definition "Interface for receiving a hydraulic connector, such as a hot stab."@en ,
                                      "Interface para receber um conector hidráulico tipo hot stab."@pt-br ;
                      skos:prefLabel "Hot Stab Receptacle"@en ,
                                     "Receptáculo de Hot Stab"@pt-br ;
                      edo:hasDiscipline edo:SubseaFlexiblePipesEngineering ,
                                        edo:SubseaUmbilicalsEngineering ;
                      edo:ifc_equivalentClass "IfcPipeFitting" ;
                      edo:ifc_objectType "HotStabReceptacle" .


###  https://w3id.org/energy-domain/edo#Hub
edo:Hub rdf:type owl:Class ;
        rdfs:subClassOf edo:PressureComponent ;
        dcterms:identifier "Hub" ;
        skos:definition "Interface for mating of a matching major connector"@en ,
                        "Interface para acoplamento de um conector de grande porte correspondente"@pt-br ;
        skos:prefLabel "Hub"@en ,
                       "Hub"@pt-br .


###  https://w3id.org/energy-domain/edo#HubBlockCap
edo:HubBlockCap rdf:type owl:Class ;
                rdfs:subClassOf edo:FlowControlModule ;
                dcterms:identifier "HubBlockCap" ;
                skos:definition "Cobertura que pode ser instalada e travada sobre um hub/mandril, capaz de conter as pressões de operação a longo prazo"@pt-br ,
                                "Cover that may be installed and locked over a hub, being able to withstand operation pressures in the long term"@en ;
                skos:prefLabel "Capa de bloqueio de hub"@pt-br ,
                               "Hub block cap"@en ;
                edo:hasDiscipline edo:WetChristmasTreesEngineering .


###  https://w3id.org/energy-domain/edo#HubProtectionCap
edo:HubProtectionCap rdf:type owl:Class ;
                     rdfs:subClassOf edo:Accessory ;
                     dcterms:identifier "HubProtectionCap" ;
                     skos:definition "Dispositivo simples, não resistente a pressões de trabalho, para proteção de um hub/mandril contra agentes externos (detritos, corrosão, etc.), geralmente temporariamente"@pt-br ,
                                     "Simple, non-pressure-containing device for usually temporary protection of a hub against external agents (such as debris, corrosion etc.)"@en ;
                     skos:prefLabel "Capa de proteção de hub"@pt-br ,
                                    "Hub protection cap"@en .


###  https://w3id.org/energy-domain/edo#HybridRenewables
edo:HybridRenewables rdf:type owl:Class ;
                     rdfs:subClassOf edo:Renewable ;
                     dcterms:identifier "HybridRenewables" ;
                     skos:definition "Hybrid renewables are systems that combine two or more renewable energy sources, such as solar and wind, in order to improve reliability, efficiency and land use. They represent a growing field of integration that enables more flexible and resilient energy generation."@en ,
                                     "Renováveis híbridas são sistemas que combinam duas ou mais fontes de energia renovável, como solar e eólica, com o objetivo de melhorar a confiabilidade, a eficiência e o uso do solo. Representam um campo crescente de integração que permite uma geração de energia mais flexível e resiliente."@pt-br ;
                     skos:prefLabel "Hybrid Renewables"@en ,
                                    "Renováveis Híbridas"@pt-br .


###  https://w3id.org/energy-domain/edo#HydraulicJumper
edo:HydraulicJumper rdf:type owl:Class ;
                    rdfs:subClassOf edo:Jumper ;
                    dcterms:identifier "HydraulicJumper" ;
                    skos:prefLabel "Hydraulic jumper"@en ,
                                   "Jumper hidráulico"@pt-br ;
                    edo:hasAttribute edo:BundleDiameter ,
                                     edo:MinimumBendingRadius ,
                                     edo:WeightInWater ;
                    edo:hasDiscipline edo:SubseaUmbilicalsEngineering .


###  https://w3id.org/energy-domain/edo#HydraulicJumperConnector
edo:HydraulicJumperConnector rdf:type owl:Class ;
                             rdfs:subClassOf edo:JumperConnector ;
                             dcterms:identifier "HydraulicJumperConnector" ;
                             skos:definition "Conector para terminação de jumpers hidráulicos."@pt-br ,
                                             "Connector for hydraulic jumper termination."@en ;
                             skos:prefLabel "Conector de Jumper Hidráulico"@pt-br ,
                                            "Hydraulic Jumper Connector"@en ;
                             edo:hasAttribute edo:MaxPressure .


###  https://w3id.org/energy-domain/edo#HydraulicPowerUnit
edo:HydraulicPowerUnit rdf:type owl:Class ;
                       rdfs:subClassOf edo:TopsideEquipment ;
                       dcterms:identifier "HydraulicPowerUnit" ;
                       skos:definition "Equipamento de superfície para geração, controle e distribuição de potência hidráulica"@pt-br ,
                                       "Topside equipment for generation, control and distribution of hydraulic power"@en ;
                       skos:prefLabel "Hydraulic power unit"@en ,
                                      "Unidade de potência hidráulica"@pt-br .


###  https://w3id.org/energy-domain/edo#HydrogenEnergy
edo:HydrogenEnergy rdf:type owl:Class ;
                   rdfs:subClassOf edo:Domain ;
                   rdfs:label "Energia de Hidrogênio"@pt-br ,
                              "Hydrogen Energy"@en ;
                   skos:definition "Production, storage, and utilization of hydrogen as an energy carrier."@en ,
                                   "Produção, armazenamento e utilização de hidrogênio como vetor energético."@pt-br .


###  https://w3id.org/energy-domain/edo#Hydropower
edo:Hydropower rdf:type owl:Class ;
               rdfs:subClassOf edo:Renewable ;
               rdfs:label "Energia Hidrelétrica"@pt-br ,
                          "Hydropower"@en ;
               skos:definition "Energia gerada a partir da água em movimento, incluindo barragens e energia das marés."@pt-br ,
                               "Energy generated from moving water, including dams and tidal power."@en .


###  https://w3id.org/energy-domain/edo#HydrostaticCollapseAbsPressDry
edo:HydrostaticCollapseAbsPressDry rdf:type owl:Class ;
                                   rdfs:subClassOf edo:DomainAttribute ;
                                   dcterms:accessRights "PUBLIC" ;
                                   dcterms:identifier "HydrostaticCollapseAbsPressDry" ;
                                   skos:definition "Pressão Absoluta de colapso hidrostático, anular seco, linha reta"@pt-br ,
                                                   "Represents the absolute pressure at which a component or material will collapse under hydrostatic forces when in a dry state. This property is important for evaluating the material's ability to withstand external pressure without deformation or failure."@en ;
                                   skos:prefLabel "Hydrostatic Collapse Absolute Pressure Dry"@en ,
                                                  "Pressão Absoluta de Colapso Hidrostático a Seco"@pt-br ;
                                   edo:hasAttributeScope edo:TypeLevelAttribute ;
                                   edo:hasLifecycleCreationPhase edo:DetailedDesign ;
                                   edo:hasTypedValue edo:FloatValue ;
                                   edo:hasUnit unit:PA ;
                                   edo:hasValueCardinality edo:SingleValue .


###  https://w3id.org/energy-domain/edo#HydrostaticPressureTestsAttribute
edo:HydrostaticPressureTestsAttribute rdf:type owl:Class ;
                                      rdfs:subClassOf edo:DomainAttribute .


###  https://w3id.org/energy-domain/edo#IMUX
edo:IMUX rdf:type owl:Class ;
         rdfs:subClassOf edo:ElectronicDevice ;
         dcterms:identifier "IMUX" ;
         skos:definition "Communications conversion module for downhole sensors and components"@en ,
                         "Módulo de conversão para comunicação com sensores e componentes de poço (downhole)"@pt-br ;
         skos:prefLabel "IWIS multiplexer"@en ,
                        "Multiplexador IWIS"@pt-br .


###  https://w3id.org/energy-domain/edo#ITube
edo:ITube rdf:type owl:Class ;
          rdfs:subClassOf edo:RiserSupport ;
          dcterms:identifier "ITube" ;
          skos:prefLabel "I-tube"@en ,
                         "I-tube"@pt-br .


###  https://w3id.org/energy-domain/edo#IdInUnifilarDiagram
edo:IdInUnifilarDiagram rdf:type owl:Class ;
                        rdfs:subClassOf edo:DomainAttribute ;
                        dcterms:accessRights "PUBLIC" ;
                        dcterms:identifier "IdInUnifilarDiagram" ;
                        skos:definition "Identificador do item no diagrama unifilar (unifilar \"classico\", pre-existente) conforme a coluna \"item\" do unifilar."@pt-br ,
                                        "Numeric identifier used to represent the component in a unifilar diagram, ensuring clear reference and traceability within the diagram. This identifier allows for easy identification of the component's position and connection points in the simplified representation of the system."@en ;
                        skos:prefLabel "Id In Unifilar Diagram"@en ,
                                       "Identificador no Diagrama Unifilar"@pt-br ;
                        edo:hasAttributeScope edo:TypeLevelAttribute ;
                        edo:hasLifecycleCreationPhase edo:DetailedDesign ;
                        edo:hasTypedValue edo:IntValue ;
                        edo:hasValueCardinality edo:SingleValue .


###  https://w3id.org/energy-domain/edo#IdentificationAttribute
edo:IdentificationAttribute rdf:type owl:Class ;
                            rdfs:subClassOf edo:AttributeDomainCategory ;
                            rdfs:comment "Represents identifiers, codes, names."@en ;
                            rdfs:label "Atributo de Identificação"@pt-br ,
                                       "Identification Attribute"@en ;
                            skos:definition "Representa identificadores, códigos, nomes"@pt-br ,
                                            "Represents identifiers, codes, names"@en .


###  https://w3id.org/energy-domain/edo#IfcInstanciableElement
edo:IfcInstanciableElement rdf:type owl:Class ;
                           rdfs:subClassOf edo:InstanciableElement ;
                           skos:definition "Representa um elemento de domínio que pode ser instanciado em projetos IFC, fornecendo anotações de configuração para suas instâncias específicas e permitindo a gestão consistente de propriedades entre múltiplas instâncias."@pt-br ,
                                           "Represents a domain element that can be instantiated in IFC projects, providing configuration annotations for its specific instances and enabling consistent property management across multiple instances."@en ;
                           skos:prefLabel "Elemento Instanciável IFC"@pt-br ,
                                          "IFC Instanciable Element"@en ;
                           edo:ifc_equivalentClass "-" ;
                           edo:ifc_objectType "-" ;
                           edo:ifc_predefinedType "-" .


###  https://w3id.org/energy-domain/edo#ImportedValue
edo:ImportedValue rdf:type owl:Class ;
                  rdfs:subClassOf edo:ValueOrigin ;
                  rdfs:comment "Imported from another system."@en ;
                  rdfs:label "Importado"@pt-br ,
                             "Imported"@en ;
                  skos:definition "Importado de outro sistema"@pt-br ,
                                  "Imported from another system"@en .


###  https://w3id.org/energy-domain/edo#IndividualAnodeMass
edo:IndividualAnodeMass rdf:type owl:Class ;
                        rdfs:subClassOf edo:DomainAttribute ;
                        dcterms:accessRights "PUBLIC" ;
                        dcterms:identifier "IndividualAnodeMass" ;
                        skos:definition "Total mass of the sacrificial anode material within each individual anode."@en ;
                        skos:prefLabel "Individual Anode Mass"@en ,
                                       "Massa Individual do Anodo"@pt-br ;
                        edo:hasAttributeScope edo:TypeLevelAttribute ;
                        edo:hasLifecycleCreationPhase edo:DetailedDesign ;
                        edo:hasTypedValue edo:FloatValue ;
                        edo:hasUnit unit:KiloGM ;
                        edo:hasValueCardinality edo:SingleValue .


###  https://w3id.org/energy-domain/edo#InitialBuoyancy
edo:InitialBuoyancy rdf:type owl:Class ;
                    rdfs:subClassOf edo:DomainAttribute ;
                    dcterms:accessRights "PUBLIC" ;
                    dcterms:identifier "InitialBuoyancy (SOL)" ;
                    rdfs:comment "Empuxo nominal fornecido pelo flutuador no começo da vida útil"@pt-br ;
                    skos:definition "Empuxo nominal fornecido pelo módulo de flutuabilidade no início de sua vida útil"@pt-br ,
                                    "Nominal upthrust supplied by buoyancy module early in its lifespan"@en ;
                    skos:prefLabel "Flutuabilidade inicial"@pt-br ,
                                   "Initial buoyancy"@en ;
                    edo:hasAttributeScope edo:TypeLevelAttribute ;
                    edo:hasLifecycleCreationPhase edo:DetailedDesign ;
                    edo:hasTypedValue edo:FloatValue ;
                    edo:hasValueCardinality edo:SingleValue .


###  https://w3id.org/energy-domain/edo#InlineT
edo:InlineT rdf:type owl:Class ;
            rdfs:subClassOf edo:FlowControlEquipment ;
            dcterms:identifier "InlineT" ;
            skos:definition "Derivation of a main pipeline at an approximately right angle (90°)"@en ,
                            "Derivação de um duto principal em ângulo aproximadamente reto (90°)"@pt-br ;
            skos:prefLabel "'T' em linha"@pt-br ,
                           "Inline tee"@en .


###  https://w3id.org/energy-domain/edo#InlineValve
edo:InlineValve rdf:type owl:Class ;
                rdfs:subClassOf edo:FlowControlEquipment ;
                dcterms:identifier "InlineValve" ;
                skos:definition "Equipamento inline que contém uma válvula como seu principal elemento, e ainda acessórios, sistemas de atuação etc."@pt-br ,
                                "Inline equipment containing a valve as main element plus accessories, actuation systems etc."@en ;
                skos:prefLabel "Inline valve"@en ,
                               "Válvula inline"@pt-br .


###  https://w3id.org/energy-domain/edo#InlineY
edo:InlineY rdf:type owl:Class ;
            rdfs:subClassOf edo:FlowControlEquipment ;
            dcterms:identifier "InlineY" ;
            skos:definition "Bifurcação de duto que permite passagem de pig"@pt-br ,
                            "Pipeline bifurcation that allows pigging"@en ;
            skos:prefLabel "'Y' em linha"@pt-br ,
                           "Inline wye"@en .


###  https://w3id.org/energy-domain/edo#InnerDiameter
edo:InnerDiameter rdf:type owl:Class ;
                  rdfs:subClassOf edo:DomainAttribute ;
                  dcterms:accessRights "PUBLIC" ;
                  dcterms:identifier "InnerDiameter" ;
                  skos:definition "Inner diameter"@en ;
                  skos:prefLabel "Diâmetro Interno"@pt-br ,
                                 "Inner diameter"@en ;
                  edo:hasAttributeScope edo:TypeLevelAttribute ;
                  edo:hasLifecycleCreationPhase edo:DetailedDesign ;
                  edo:hasTypedValue edo:FloatValue ;
                  edo:hasUnit unit:MilliM ;
                  edo:hasValueCardinality edo:MultiValue .


###  https://w3id.org/energy-domain/edo#InnerTube
edo:InnerTube rdf:type owl:Class ;
              rdfs:subClassOf edo:IfcInstanciableElement ,
                              edo:SolidLayer ;
              dcterms:identifier "InnerTube" ;
              skos:definition "The Inner Tube is the innermost layer of a subsea flexible pipe, responsible for containing and transporting the fluid, such as oil or gas. It is designed to withstand internal pressures and prevent fluid leakage while offering resistance to the corrosive and abrasive nature of the transported substances. The Inner Tube is typically made from high-performance polymeric materials that ensure durability, flexibility, and chemical resistance, making it a critical component in maintaining the integrity of the flexible pipe in subsea operations."@en ;
              skos:prefLabel "Inner Tube"@en ,
                             "Tubo Interno"@pt-br ;
              edo:hasDiscipline edo:SubseaFlexiblePipesEngineering ;
              edo:ifc_equivalentClass "IfcPipeSegment" ;
              edo:ifc_objectType "InnerTube" ;
              edo:ifc_predefinedType "USERDEFINED" .


###  https://w3id.org/energy-domain/edo#InsideTemperature
edo:InsideTemperature rdf:type owl:Class ;
                      rdfs:subClassOf edo:BendingStiffnessCurveAttribute ,
                                      edo:DomainAttribute ;
                      dcterms:accessRights "PUBLIC" ;
                      dcterms:identifier "InsideTemperature" ;
                      skos:definition "Represents the internal temperature within a component or system. This property is important for assessing the thermal conditions inside the system, ensuring that it operates within safe temperature limits, particularly in subsea environments where temperature control is essential for maintaining performance and integrity."@en ;
                      skos:prefLabel "Inside Temperature"@en ,
                                     "Temperatura Interna"@pt-br ;
                      edo:hasAttributeScope edo:TypeLevelAttribute ;
                      edo:hasLifecycleCreationPhase edo:DetailedDesign ;
                      edo:hasTypedValue edo:FloatValue ;
                      edo:hasUnit unit:K ;
                      edo:hasValueCardinality edo:SingleValue .


###  https://w3id.org/energy-domain/edo#Installation
edo:Installation rdf:type owl:Class ;
                 rdfs:subClassOf edo:ConstructionPhase ;
                 rdfs:label "Instalação"@pt-br ,
                            "Installation"@en ;
                 skos:definition "Placement and integration of equipment, piping, and structures at the site."@en ,
                                 "Posicionamento e integração de equipamentos, tubulações e estruturas no local."@pt-br .


###  https://w3id.org/energy-domain/edo#InstanceLevelAttribute
edo:InstanceLevelAttribute rdf:type owl:Class ;
                           rdfs:subClassOf edo:AttributeScope ;
                           rdfs:comment "Attribute specific to a real-world individual instance of item."@en ;
                           rdfs:label "Atributo de Instância"@pt-br ,
                                      "Instance-Level Attribute"@en ;
                           skos:definition "Atributo específico a uma instância individual no mundo real"@pt-br ,
                                           "Attribute specific to a real-world individual instance of item"@en .


###  https://w3id.org/energy-domain/edo#InstanciableElement
edo:InstanciableElement rdf:type owl:Class ;
                        rdfs:subClassOf edo:ConceptualMarker ;
                        skos:definition "Abstract conceptual marker that designates which domain elements are intended to be instantiated within projects. Its purpose is to distinguish between purely conceptual classes and those that represent concrete entities in project contexts. By providing a structured way to identify instantiable entities, it supports consistency in modeling, validation, and maintenance processes, while remaining flexible for use across different domains and applications."@en ,
                                        "Marcador conceitual abstrato que designa quais elementos de domínio devem ser instanciados em projetos. Seu propósito é distinguir entre classes puramente conceituais e aquelas que representam entidades concretas em contextos de projeto. Ao fornecer uma forma estruturada de identificar entidades instanciáveis, ele apoia a consistência em processos de modelagem, validação e manutenção, mantendo-se flexível para uso em diferentes domínios e aplicações."@pt-br ;
                        skos:prefLabel "Elemento Instanciável"@pt-br ,
                                       "Instanciable Element"@en .


###  https://w3id.org/energy-domain/edo#InstrumentationEngineering
edo:InstrumentationEngineering rdf:type owl:Class ;
                               rdfs:subClassOf edo:TechnicalDiscipline ;
                               rdfs:label "Engenharia de Instrumentação"@pt-br ,
                                          "Instrumentation Engineering"@en ;
                               skos:definition "Disciplina de engenharia focada em sistemas de instrumentação de medição e controle."@pt-br ,
                                               "Engineering discipline focused on measurement and control instrumentation systems."@en .


###  https://w3id.org/energy-domain/edo#InsulationTape
edo:InsulationTape rdf:type owl:Class ;
                   rdfs:subClassOf edo:IfcInstanciableElement ,
                                   edo:TapeLayer ;
                   dcterms:identifier "InsulationTape" ;
                   skos:definition "Material used in subsea flexible pipes to provide thermal insulation, ensuring that the temperature of the transported fluids remains stable during flow. Insulation Tape is applied in layers around the pipe to minimize heat loss or gain, which is critical for maintaining the fluid's properties, such as viscosity, in deepwater environments. It is typically made from materials with low thermal conductivity, such as polymers or composites, and is essential for enhancing the efficiency and performance of subsea pipelines in harsh temperature conditions."@en ;
                   skos:prefLabel "Fita de Isolamento"@pt-br ,
                                  "Insulation Tape"@en ;
                   edo:hasDiscipline edo:SubseaFlexiblePipesEngineering ;
                   edo:ifc_equivalentClass "IfcPipeSegment" ;
                   edo:ifc_objectType "InsulationTape" ;
                   edo:ifc_predefinedType "USERDEFINED" .


###  https://w3id.org/energy-domain/edo#IntValue
edo:IntValue rdf:type owl:Class ;
             owl:equivalentClass [ rdf:type owl:Restriction ;
                                   owl:onProperty rdf:value ;
                                   owl:allValuesFrom xsd:int
                                 ] ;
             rdfs:subClassOf edo:DataType ;
             rdfs:comment "Constraint for xsd:int (32-bit integer)"@en ;
             rdfs:label "Integer Value"@en .


###  https://w3id.org/energy-domain/edo#IntegratedPipe
edo:IntegratedPipe rdf:type owl:Class ;
                   rdfs:subClassOf edo:IfcInstanciableElement ,
                                   edo:Tubing ;
                   dcterms:identifier "IntegratedPipe" ;
                   skos:definition "Representa um tubo integrado dentro de uma tubulação para finalidades estruturais e funcionais combinadas."@pt-br ,
                                   "Represents a pipe integrated within tubing for combined structural and functional purposes."@en ;
                   skos:prefLabel "Duto integrado"@pt-br ,
                                  "Integrated Pipe"@en ,
                                  "Integrated pipe"@en ,
                                  "Tubo Integrado"@pt-br ;
                   edo:hasDiscipline edo:SubseaUmbilicalsEngineering ;
                   edo:ifc_equivalentClass "IfcPipeSegment" ;
                   edo:ifc_objectType "IntegratedPipe" ;
                   edo:ifc_predefinedType "USERDEFINED" .


###  https://w3id.org/energy-domain/edo#Interconnection
edo:Interconnection rdf:type owl:Class ;
                    rdfs:subClassOf edo:LinearLocation ;
                    dcterms:identifier "Interconnection" ;
                    skos:definition "Local que contém toda a extensão de uma interligação, com seus diversos trechos, terminações, equipamentos inline, etc."@pt-br ,
                                    "Location that contains the entire length of an interconnection, with its various sections, terminations, inline equipment, etc."@en ;
                    skos:prefLabel "Interconnection"@en ,
                                   "Interligação"@pt-br .


###  https://w3id.org/energy-domain/edo#InterlockedCarcass
edo:InterlockedCarcass rdf:type owl:Class ;
                       rdfs:subClassOf edo:CarcassLayer ,
                                       edo:IfcInstanciableElement ;
                       dcterms:identifier "InterlockedCarcass" ;
                       skos:definition "The Interlocked Carcass is a metallic layer used in certain subsea flexible pipes to provide internal pressure resistance and prevent collapse. It is designed with interlocking metal strips that offer high strength while maintaining flexibility. This layer enhances the structural integrity of the flexible pipe, protecting it from external pressures and harsh subsea conditions. The Interlocked Carcass allows the pipe to bend without losing its shape or collapsing under deepwater pressure."@en ;
                       skos:prefLabel "Carcaça"@pt-br ,
                                      "Interlocked Carcass"@en ;
                       edo:hasDiscipline edo:SubseaFlexiblePipesEngineering ;
                       edo:ifc_equivalentClass "IfcPipeSegment" ;
                       edo:ifc_objectType "InterlockedCarcass" ;
                       edo:ifc_predefinedType "USERDEFINED" .


###  https://w3id.org/energy-domain/edo#IntermediateBendStiffener
edo:IntermediateBendStiffener rdf:type owl:Class ;
                              rdfs:subClassOf edo:BendStiffener ,
                                              edo:IfcInstanciableElement ;
                              dcterms:identifier "IntermediateBendStiffener" ;
                              skos:altLabel "Curvature Stiffener"@en ,
                                            "Intermediate Bending Stiffener"@en ,
                                            "Stiffener"@en ;
                              skos:definition "A device used in subsea flexible pipes to provide localized stiffness at specific points along the length of the pipe, preventing excessive bending and reducing stress concentration. The Intermediate Bend Stiffener is typically installed between critical areas to ensure that the pipe maintains a controlled bending radius, protecting it from over-flexing or fatigue. Made from durable materials, it helps prolong the service life of the flexible pipe by distributing loads more evenly and reducing the risk of damage in dynamic subsea environments."@en ,
                                              "Dispositivo usado em tubos flexíveis submarinos para fornecer rigidez localizada em pontos específicos ao longo do comprimento do tubo, evitando dobras excessivas e reduzindo a concentração de tensões. O Enrijecedor de Curvatura Intermediário é tipicamente instalado entre áreas críticas para garantir que o tubo mantenha um raio de curvatura controlado, protegendo-o contra flexões excessivas ou fadiga. Feito de materiais duráveis, ajuda a prolongar a vida útil do tubo flexível, distribuindo as cargas de forma mais uniforme e reduzindo o risco de danos em ambientes submarinos dinâmicos."@pt-br ;
                              skos:prefLabel "Enrijecedor de Curvatura Intermediário"@pt-br ,
                                             "Intermediate Bend Stiffener"@en ;
                              edo:hasDiscipline edo:SubseaFlexiblePipesEngineering ,
                                                edo:SubseaUmbilicalsEngineering ;
                              edo:ifc_equivalentClass "IfcPipeFitting" ;
                              edo:ifc_objectType "IntermediateBendStiffener" .


###  https://w3id.org/energy-domain/edo#IntermediateSheath
edo:IntermediateSheath rdf:type owl:Class ;
                       rdfs:subClassOf edo:IfcInstanciableElement ,
                                       edo:SolidLayer ;
                       dcterms:identifier "IntermediateSheath" ;
                       skos:definition "A protective layer within a subsea flexible pipe, positioned between other structural layers to provide additional protection and separation. The Intermediate Sheath serves to isolate different layers, preventing abrasion, wear, or interaction that could compromise the integrity of the pipe. Typically made from polymeric materials, this sheath also contributes to the overall durability and flexibility of the pipe, ensuring it can withstand the dynamic conditions of subsea environments while maintaining the performance of the internal and external layers."@en ;
                       skos:prefLabel "Barreira Intermediária de Vedação"@pt-br ,
                                      "Intermediate Sheath"@en ;
                       edo:hasDiscipline edo:SubseaFlexiblePipesEngineering ,
                                         edo:SubseaUmbilicalsEngineering ;
                       edo:ifc_equivalentClass "IfcPipeSegment" ;
                       edo:ifc_objectType "IntermediateSheath" ;
                       edo:ifc_predefinedType "USERDEFINED" .


###  https://w3id.org/energy-domain/edo#IntermediateValuesStrategy
edo:IntermediateValuesStrategy rdf:type owl:Class ;
                               rdfs:subClassOf edo:BendingStiffnessCurveAttribute ,
                                               edo:CrushingFrictionCoefficientTighteningAttribute ,
                                               edo:CrushingMaximumAllowableTensionAttribute ,
                                               edo:CrushingMaximumAllowableTighteningAttribute ,
                                               edo:DomainAttribute ;
                               dcterms:accessRights "PUBLIC" ;
                               dcterms:identifier "IntermediateValuesStrategy" ;
                               skos:definition "Defines the approach used to handle or calculate intermediate values between specified data points. This property is important for ensuring accuracy in analysis or simulations, particularly when determining values that fall between measured or specified conditions."@en ;
                               skos:prefLabel "Estratégia para Valores Intermediários"@pt-br ,
                                              "Intermediate Values Strategy"@en ;
                               edo:hasAttributeScope edo:TypeLevelAttribute ;
                               edo:hasLifecycleCreationPhase edo:DetailedDesign ;
                               edo:hasTypedValue edo:StringValue ;
                               edo:hasValueCardinality edo:SingleValue .


###  https://w3id.org/energy-domain/edo#InternalDiameter
edo:InternalDiameter rdf:type owl:Class ;
                     rdfs:subClassOf edo:DomainAttribute ;
                     dcterms:accessRights "PUBLIC" ;
                     dcterms:identifier "InternalDiameter" ;
                     skos:definition "Distance measured across the innermost points, passing through the center."@en ;
                     skos:prefLabel "Diâmetro interno"@pt-br ,
                                    "Internal Diameter"@en ;
                     edo:hasAttributeScope edo:TypeLevelAttribute ;
                     edo:hasLifecycleCreationPhase edo:BasicDesign ,
                                                   edo:DetailedDesign ;
                     edo:hasTypedValue edo:FloatValue ;
                     edo:hasUnit unit:M ;
                     edo:hasValueCardinality edo:SingleValue .


###  https://w3id.org/energy-domain/edo#InternalIncidentalPressureCurveAttribute
edo:InternalIncidentalPressureCurveAttribute rdf:type owl:Class ;
                                             rdfs:subClassOf edo:DomainAttribute ;
                                             dcterms:accessRights "PUBLIC" ;
                                             dcterms:identifier "InternalIncidentalPressureTable" ;
                                             skos:definition "Provides data on internal incidental pressures, which are temporary or unexpected pressure spikes within the structure. This information is crucial for understanding the pressure limits the structure may face and ensuring it can withstand short-term variations without compromising its integrity."@en ;
                                             skos:prefLabel "Internal Incidental Pressure Table"@en ,
                                                            "Tabela de Pressão Incidental Interna"@pt-br ;
                                             edo:hasAttributeScope edo:InstanceLevelAttribute ;
                                             edo:hasLifecycleCreationPhase edo:BasicDesign .


###  https://w3id.org/energy-domain/edo#InternalIncidentalPressureTableColumn
edo:InternalIncidentalPressureTableColumn rdf:type owl:Class ;
                                          rdfs:subClassOf edo:InternalIncidentalPressureCurveAttribute ;
                                          edo:hasLifecycleCreationPhase edo:BasicDesign .


###  https://w3id.org/energy-domain/edo#InternalIncidentalPressureTable_PositionReference
edo:InternalIncidentalPressureTable_PositionReference rdf:type owl:Class ;
                                                      rdfs:subClassOf edo:InternalIncidentalPressureTableColumn ;
                                                      dcterms:accessRights "PUBLIC" ;
                                                      dcterms:identifier "InternalIncidentalPressureTable_PositionReference" ;
                                                      skos:definition "Identifies the specific point along the pipeline. This serves as the reference for vertical position and pressure values."@en ,
                                                                      "Valores válidos:Top (Para a conexão topside - E.g. Conector superior)TDPSubSeaConnection (Ex. ANM)"@pt-br ;
                                                      skos:prefLabel "Position Reference"@en ,
                                                                     "Referência de Posição"@pt-br ;
                                                      edo:hasAttributeScope edo:InstanceLevelAttribute ;
                                                      edo:hasLifecycleCreationPhase edo:BasicDesign ;
                                                      edo:hasTypedValue edo:StringValue ;
                                                      edo:hasValueCardinality edo:MultiValue .


###  https://w3id.org/energy-domain/edo#InternalIncidentalPressureTable_Pressure
edo:InternalIncidentalPressureTable_Pressure rdf:type owl:Class ;
                                             rdfs:subClassOf edo:InternalIncidentalPressureTableColumn ;
                                             dcterms:accessRights "PUBLIC" ;
                                             dcterms:identifier "InternalIncidentalPressureTable_Pressure" ;
                                             skos:definition "Indicates the force exerted per unit area on the surface of a material or component. This property is critical for evaluating how the component responds to external or internal forces, ensuring it can withstand operational pressure conditions."@en ;
                                             skos:prefLabel "Pressure"@en ,
                                                            "Pressão"@pt-br ;
                                             edo:hasAttributeScope edo:InstanceLevelAttribute ;
                                             edo:hasLifecycleCreationPhase edo:BasicDesign ;
                                             edo:hasTypedValue edo:FloatValue ;
                                             edo:hasUnit unit:PA ;
                                             edo:hasValueCardinality edo:MultiValue .


###  https://w3id.org/energy-domain/edo#InternalIncidentalPressureTable_VPosWRTWaterline
edo:InternalIncidentalPressureTable_VPosWRTWaterline rdf:type owl:Class ;
                                                     rdfs:subClassOf edo:InternalIncidentalPressureTableColumn ;
                                                     dcterms:accessRights "PUBLIC" ;
                                                     dcterms:identifier "InternalIncidentalPressureTable_VPosWRTWaterline" ;
                                                     skos:definition "Valores negativos para pontos submersos, e valores positivos para pontos acima da água. Considerando calado máximo da plataforma, quando aplicável."@pt-br ,
                                                                     "Vertical position with respect to the waterline, where positive values indicate points above the water and negative values indicate points below. The platform's maximum draft is considered when applicable."@en ;
                                                     skos:prefLabel "Posição Vertical em Relação à Linha D'Água"@pt-br ,
                                                                    "Vertical Position With Respect To Waterline"@en ;
                                                     edo:hasAttributeScope edo:InstanceLevelAttribute ;
                                                     edo:hasLifecycleCreationPhase edo:BasicDesign ;
                                                     edo:hasTypedValue edo:IntValue ;
                                                     edo:hasUnit unit:M ;
                                                     edo:hasValueCardinality edo:MultiValue .


###  https://w3id.org/energy-domain/edo#InternalLength
edo:InternalLength rdf:type owl:Class ;
                   rdfs:subClassOf edo:DomainAttribute ;
                   dcterms:accessRights "PUBLIC" ;
                   dcterms:identifier "InternalLength" ;
                   skos:definition "Comprimento interno disponível para acomodação de pigtails, etc."@pt-br ,
                                   "Internal length available for accommodating pigtails etc."@en ;
                   skos:prefLabel "Comprimento interno"@pt-br ,
                                  "Internal length"@en ;
                   edo:hasAttributeScope edo:TypeLevelAttribute ;
                   edo:hasLifecycleCreationPhase edo:DetailedDesign ;
                   edo:hasTypedValue edo:FloatValue ;
                   edo:hasValueCardinality edo:SingleValue .


###  https://w3id.org/energy-domain/edo#InternalPressureSheath
edo:InternalPressureSheath rdf:type owl:Class ;
                           rdfs:subClassOf edo:IfcInstanciableElement ,
                                           edo:SolidLayer ;
                           dcterms:identifier "InternalPressureSheath" ;
                           skos:altLabel "Inner Sheath" ;
                           skos:definition "A layer within a subsea flexible pipe designed to contain the internal fluid and withstand the internal pressure exerted by the transported medium, such as oil, gas, or water. The Internal Pressure Sheath plays a crucial role in preventing fluid leakage and maintaining pressure integrity within the pipe. Typically made from high-performance polymeric materials, it ensures the safe transport of fluids under high-pressure conditions, contributing to the pipe's overall structural stability and long-term reliability in harsh subsea environments."@en ;
                           skos:prefLabel "Barreira Interna de Pressão"@pt-br ,
                                          "Internal Pressure Sheath"@en ;
                           edo:hasDiscipline edo:SubseaFlexiblePipesEngineering ,
                                             edo:SubseaUmbilicalsEngineering ;
                           edo:ifc_equivalentClass "IfcPipeSegment" ;
                           edo:ifc_objectType "InternalPressureSheath" ;
                           edo:ifc_predefinedType "USERDEFINED" .


###  https://w3id.org/energy-domain/edo#InternalVolume
edo:InternalVolume rdf:type owl:Class ;
                   rdfs:subClassOf edo:DomainAttribute ;
                   dcterms:accessRights "PUBLIC" ;
                   dcterms:identifier "InternalVolume" ;
                   skos:definition "Refers to the volume of space within an object that can be occupied by a fluid when the object is fully filled or immersed. This property is essential for understanding the capacity and fluid-holding capabilities of the accessory."@en ;
                   skos:prefLabel "Internal Volume"@en ,
                                  "Volume interno"@pt-br ;
                   edo:hasAttributeScope edo:TypeLevelAttribute ;
                   edo:hasLifecycleCreationPhase edo:DetailedDesign ;
                   edo:hasTypedValue edo:FloatValue ;
                   edo:hasUnit unit:M3 ;
                   edo:hasValueCardinality edo:SingleValue .


###  https://w3id.org/energy-domain/edo#IsDummy
edo:IsDummy rdf:type owl:Class ;
            rdfs:subClassOf edo:DomainAttribute ;
            dcterms:accessRights "PUBLIC" ;
            dcterms:identifier "IsDummy" ;
            rdfs:comment "Especifica se este é um conector 'dummy', apenas para ocupação/proteção de uma posição, e não terminação de jumpers"@pt-br ;
            skos:definition "Specifies whether this is a dummy connector only for parking/protection of a slot, and not jumper termination"@en ;
            skos:prefLabel "Is Dummy"@en ,
                           "É dummy"@pt-br ;
            edo:hasTypedValue edo:IfcBoolean .


###  https://w3id.org/energy-domain/edo#IsParkingPlace
edo:IsParkingPlace rdf:type owl:Class ;
                   rdfs:subClassOf edo:DomainAttribute ;
                   dcterms:accessRights "PUBLIC" ;
                   dcterms:identifier "IsParkingPlace" ;
                   rdfs:comment "Especifica se este conector é apenas para estacionamento mecânico de dummies/jumpers, sem outras funções no sistema do qual é parte"@pt-br ;
                   skos:definition "Specifies whether this connector is only for mechanical parking of dummies/jumpers, without further functions in its parent system"@en ;
                   skos:prefLabel "Is parking place"@en ,
                                  "É parking place"@pt-br ;
                   edo:hasTypedValue edo:IfcBoolean .


###  https://w3id.org/energy-domain/edo#IsSpare
edo:IsSpare rdf:type owl:Class ;
            rdfs:subClassOf edo:DomainAttribute ;
            dcterms:accessRights "PUBLIC" ;
            dcterms:identifier "IsSpare" ;
            skos:definition "Indicates whether the item is spare (TRUE) or not (FALSE)."@en ;
            skos:prefLabel "Is Spare"@en ,
                           "É um sobressalente"@pt-br ;
            edo:hasAttributeScope edo:InstanceLevelAttribute ;
            edo:hasLifecycleCreationPhase edo:DetailedDesign ;
            edo:hasTypedValue edo:BooleanValue ;
            edo:hasValueCardinality edo:SingleValue .


###  https://w3id.org/energy-domain/edo#Jumper
edo:Jumper rdf:type owl:Class ;
           rdfs:subClassOf edo:LinearObject ;
           dcterms:identifier "Jumper" ;
           skos:altLabel "Flying lead"@en ;
           skos:definition "Interconexões elétricas, hidráulicas, óticas, etc. de menor porte, geralmente manipuláveis no ambiente submarino diretamente por ROV/mergulho"@pt-br ,
                           "Short electrical, hydraulic, optical etc. interconnections, usually directly manipulated in the subsea environment by ROV/diver"@en ;
           skos:prefLabel "Jumper de controle/sinal"@pt-br ,
                          "Signal/control jumper"@en ;
           edo:hasAttribute edo:MaxDepth ,
                            edo:NumWays .


###  https://w3id.org/energy-domain/edo#JumperConnector
edo:JumperConnector rdf:type owl:Class ;
                    rdfs:subClassOf edo:Connector ;
                    dcterms:identifier "JumperConnector" ;
                    skos:definition "Representa um conector projetado para ligar temporariamente elementos, normalmente para testes, comissionamento ou configurações flexíveis de sistemas."@pt-br ,
                                    "Represents a connector designed to temporarily link elements, typically for testing, commissioning, or flexible system configurations."@en ;
                    skos:prefLabel "Conector Jumper"@pt-br ,
                                   "Jumper Connector"@en ;
                    edo:hasAttribute edo:IsDummy .


###  https://w3id.org/energy-domain/edo#JunctionBox
edo:JunctionBox rdf:type owl:Class ;
                rdfs:subClassOf edo:ComponentDevice ;
                dcterms:identifier "JunctionBox" ;
                skos:prefLabel "Caixa de emenda"@pt-br ,
                               "Junction box"@en ;
                edo:hasAttribute edo:WeightInWater ;
                edo:hasDiscipline edo:SubseaUmbilicalsEngineering ;
                edo:ifc_equivalentClass "IfcJunctionBox" ;
                edo:ifc_objectType "JunctionBox" ;
                edo:ifc_predefinedType "USERDEFINED" .


###  https://w3id.org/energy-domain/edo#LPHousing
edo:LPHousing rdf:type owl:Class ;
              rdfs:subClassOf edo:PressureComponent ;
              dcterms:identifier "LPHousing" ;
              skos:prefLabel "Alojador de baixa pressão"@pt-br ,
                             "Low-pressure housing"@en .


###  https://w3id.org/energy-domain/edo#LargeHydropower
edo:LargeHydropower rdf:type owl:Class ;
                    rdfs:subClassOf edo:Hydropower ;
                    dcterms:identifier "LargeHydropower" ;
                    skos:definition "Large hydropower plants generate electricity by harnessing the kinetic and potential energy of rivers using large dams and reservoirs, typically above 30 MW capacity. They provide reliable energy but may cause significant environmental and social impacts."@en ,
                                    "Usinas hidrelétricas de grande porte geram eletricidade aproveitando a energia cinética e potencial dos rios por meio de grandes barragens e reservatórios, geralmente acima de 30 MW de capacidade. Fornecem energia confiável, mas podem causar impactos ambientais e sociais significativos."@pt-br ;
                    skos:prefLabel "Hidrelétrica de Grande Porte"@pt-br ,
                                   "Large Hydropower"@en .


###  https://w3id.org/energy-domain/edo#LayAngle
edo:LayAngle rdf:type owl:Class ;
             rdfs:subClassOf edo:DomainAttribute ;
             dcterms:accessRights "PUBLIC" ;
             dcterms:identifier "LayAngle" ;
             skos:definition "Lay angle"@en ;
             skos:prefLabel "Lay angle"@en ,
                            "Ângulo de enrolamento"@pt-br ;
             edo:hasAttributeScope edo:TypeLevelAttribute ;
             edo:hasLifecycleCreationPhase edo:DetailedDesign ;
             edo:hasTypedValue edo:FloatValue ;
             edo:hasUnit unit:DEG ;
             edo:hasValueCardinality edo:SingleValue .


###  https://w3id.org/energy-domain/edo#LayDirection
edo:LayDirection rdf:type owl:Class ;
                 rdfs:subClassOf edo:DomainAttribute ;
                 dcterms:accessRights "PUBLIC" ;
                 dcterms:identifier "LayDirection" ;
                 skos:definition "Lay direction"@en ;
                 skos:prefLabel "Direção de enrolamento"@pt-br ,
                                "Lay direction"@en ;
                 edo:hasAttributeScope edo:TypeLevelAttribute ;
                 edo:hasLifecycleCreationPhase edo:DetailedDesign ;
                 edo:hasTypedValue edo:StringValue ;
                 edo:hasValueCardinality edo:SingleValue .


###  https://w3id.org/energy-domain/edo#LayerAnnular
edo:LayerAnnular rdf:type owl:Class ;
                 rdfs:subClassOf edo:DomainAttribute ;
                 dcterms:accessRights "PUBLIC" ;
                 dcterms:identifier "LayerAnnular" ;
                 skos:definition "Indicates whether the layer is part of the annular structure of the tensile armours. If true, it confirms that the layer contributes to the annular arrangement, which is important for understanding its role in the structural integrity and load distribution."@en ,
                                 "True se a camada faz parte do anular das armaduras de tração"@pt-br ;
                 skos:prefLabel "Camada Anular"@pt-br ,
                                "Layer Annular"@en ;
                 edo:hasAttributeScope edo:InstanceLevelAttribute ;
                 edo:hasLifecycleCreationPhase edo:DetailedDesign ;
                 edo:hasTypedValue edo:BooleanValue ;
                 edo:hasValueCardinality edo:SingleValue .


###  https://w3id.org/energy-domain/edo#LayerAnnularType
edo:LayerAnnularType rdf:type owl:Class ;
                     rdfs:subClassOf edo:DomainAttribute ;
                     dcterms:accessRights "PUBLIC" ;
                     dcterms:identifier "LayerAnnularType" ;
                     skos:definition "Specifies the type of annular layer based on the condition it is designed for. This information is crucial for understanding the intended role of the layer in the overall structural configuration and how it is expected to perform under the projected operational conditions."@en ,
                                     "Tipo de anular conforme o estado do anular: Não pertence ao anular; Anular nunca alagado; Anular sempre alagado; Anular possivelmente alagado"@pt-br ;
                     skos:prefLabel "Layer Annular Type"@en ,
                                    "Tipo de Anular"@pt-br ;
                     edo:hasAttributeScope edo:InstanceLevelAttribute ;
                     edo:hasLifecycleCreationPhase edo:DetailedDesign ;
                     edo:hasTypedValue edo:StringValue ;
                     edo:hasValueCardinality edo:SingleValue .


###  https://w3id.org/energy-domain/edo#LayerContinuity
edo:LayerContinuity rdf:type owl:Class ;
                    rdfs:subClassOf edo:DomainAttribute ;
                    dcterms:accessRights "PUBLIC" ;
                    dcterms:identifier "LayerContinuity" ;
                    skos:definition "Indicates whether the layer is continuous, such as when it is extruded. If true, it confirms that the layer has no interruptions or joints, which is important for ensuring uniformity and strength in the structure."@en ,
                                    "True se a camada é contínua (extrudada)"@pt-br ;
                    skos:prefLabel "Continuidade da Camada"@pt-br ,
                                   "Layer Continuity"@en ;
                    edo:hasAttributeScope edo:InstanceLevelAttribute ;
                    edo:hasLifecycleCreationPhase edo:DetailedDesign ;
                    edo:hasTypedValue edo:BooleanValue ;
                    edo:hasValueCardinality edo:SingleValue .


###  https://w3id.org/energy-domain/edo#LayerGeometryAttribute
edo:LayerGeometryAttribute rdf:type owl:Class ;
                           rdfs:subClassOf edo:DomainAttribute .


###  https://w3id.org/energy-domain/edo#LayerGeometryCrossSection
edo:LayerGeometryCrossSection rdf:type owl:Class ;
                              rdfs:subClassOf edo:LayerGeometryAttribute ;
                              dcterms:accessRights "PUBLIC" ;
                              dcterms:identifier "LayerGeometryCrossSection" ;
                              skos:definition "Indicates the geometry of the layer's cross-section. This property provides detailed information about the shape and dimensions of the layer when viewed in cross-section, which is important for understanding how the layer contributes to the overall structure's performance and integrity."@en ;
                              skos:prefLabel "Layer Geometry Cross Section"@en ,
                                             "Seção Transversal da Geometria da Camada"@pt-br ;
                              edo:hasAttributeScope edo:InstanceLevelAttribute ;
                              edo:hasLifecycleCreationPhase edo:DetailedDesign ;
                              edo:hasTypedValue edo:FloatValue ;
                              edo:hasUnit unit:M2 ;
                              edo:hasValueCardinality edo:SingleValue .


###  https://w3id.org/energy-domain/edo#LayerGeometryInertiaX
edo:LayerGeometryInertiaX rdf:type owl:Class ;
                          rdfs:subClassOf edo:LayerGeometryAttribute ;
                          dcterms:accessRights "PUBLIC" ;
                          dcterms:identifier "LayerGeometryInertiaX" ;
                          skos:definition "Indicates the moment of inertia of the layer's geometry around the X-axis. This property is crucial for understanding the layer's resistance to bending or deformation when subjected to forces along the X-axis, contributing to the structural stability and performance of the component."@en ;
                          skos:prefLabel "Inércia X da Geometria da Camada"@pt-br ,
                                         "Layer Geometry Inertia X"@en ;
                          edo:hasAttributeScope edo:InstanceLevelAttribute ;
                          edo:hasLifecycleCreationPhase edo:DetailedDesign ;
                          edo:hasTypedValue edo:FloatValue ;
                          edo:hasUnit unit:M4 ;
                          edo:hasValueCardinality edo:SingleValue .


###  https://w3id.org/energy-domain/edo#LayerGeometryInertiaY
edo:LayerGeometryInertiaY rdf:type owl:Class ;
                          rdfs:subClassOf edo:LayerGeometryAttribute ;
                          dcterms:accessRights "PUBLIC" ;
                          dcterms:identifier "LayerGeometryInertiaY" ;
                          skos:definition "Indicates the moment of inertia of the layer's geometry around the Y-axis. This property is important for evaluating the layer's resistance to bending or deformation when subjected to forces along the Y-axis, helping to ensure the structural stability and performance of the component."@en ;
                          skos:prefLabel "Inércia  Y da Geometria da Camada"@pt-br ,
                                         "Layer Geometry Inertia Y"@en ;
                          edo:hasAttributeScope edo:InstanceLevelAttribute ;
                          edo:hasLifecycleCreationPhase edo:DetailedDesign ;
                          edo:hasTypedValue edo:FloatValue ;
                          edo:hasUnit unit:M4 ;
                          edo:hasValueCardinality edo:SingleValue .


###  https://w3id.org/energy-domain/edo#LayerGeometryManufacturer
edo:LayerGeometryManufacturer rdf:type owl:Class ;
                              rdfs:subClassOf edo:LayerGeometryAttribute ;
                              dcterms:accessRights "PUBLIC" ;
                              dcterms:identifier "LayerGeometryManufacturer" ;
                              skos:definition "Indicates the manufacturer responsible for producing the layer's geometry. This property is important for tracking the origin and quality of the layer, providing key information about the source of the material or component used in the structure."@en ;
                              skos:prefLabel "Fabricante da Geometria da Camada"@pt-br ,
                                             "Layer Geometry Manufacturer"@en ;
                              edo:hasAttributeScope edo:InstanceLevelAttribute ;
                              edo:hasLifecycleCreationPhase edo:DetailedDesign ;
                              edo:hasTypedValue edo:StringValue ;
                              edo:hasValueCardinality edo:SingleValue .


###  https://w3id.org/energy-domain/edo#LayerGeometryName
edo:LayerGeometryName rdf:type owl:Class ;
                      rdfs:subClassOf edo:LayerGeometryAttribute ;
                      dcterms:accessRights "PUBLIC" ;
                      dcterms:identifier "LayerGeometryName" ;
                      skos:definition "Indicates the name assigned to the layer's geometry. This property is used to identify and distinguish the specific geometry of the layer, helping with organization, tracking, and reference within the overall structure or design."@en ;
                      skos:prefLabel "Layer Geometry Name"@en ,
                                     "Nome da Geometria da Camada"@pt-br ;
                      edo:hasAttributeScope edo:InstanceLevelAttribute ;
                      edo:hasLifecycleCreationPhase edo:DetailedDesign ;
                      edo:hasTypedValue edo:StringValue ;
                      edo:hasValueCardinality edo:SingleValue .


###  https://w3id.org/energy-domain/edo#LayerGeometryProfileThickness
edo:LayerGeometryProfileThickness rdf:type owl:Class ;
                                  rdfs:subClassOf edo:LayerGeometryAttribute ;
                                  dcterms:accessRights "PUBLIC" ;
                                  dcterms:identifier "LayerGeometryProfileThickness" ;
                                  skos:definition "Indicates the thickness of the layer's geometric profile. This property is important for understanding the contribution of the layer to the overall structure, particularly in terms of strength, flexibility, and resistance to external forces."@en ;
                                  skos:prefLabel "Espessura do Perfil da Geometria da Camada"@pt-br ,
                                                 "Layer Geometry Profile Thickness"@en ;
                                  edo:hasAttributeScope edo:InstanceLevelAttribute ;
                                  edo:hasLifecycleCreationPhase edo:DetailedDesign ;
                                  edo:hasTypedValue edo:FloatValue ;
                                  edo:hasUnit unit:M ;
                                  edo:hasValueCardinality edo:SingleValue .


###  https://w3id.org/energy-domain/edo#LayerGeometryProfileWidth
edo:LayerGeometryProfileWidth rdf:type owl:Class ;
                              rdfs:subClassOf edo:LayerGeometryAttribute ;
                              dcterms:accessRights "PUBLIC" ;
                              dcterms:identifier "LayerGeometryProfileWidth" ;
                              skos:definition "Indicates the width of the layer's geometric profile. This property is important for understanding the dimensions of the layer, contributing to the overall structural design, and influencing factors such as load distribution and mechanical performance."@en ;
                              skos:prefLabel "Largura do Perfil da Geometria da Camada"@pt-br ,
                                             "Layer Geometry Profile Width"@en ;
                              edo:hasAttributeScope edo:InstanceLevelAttribute ;
                              edo:hasLifecycleCreationPhase edo:DetailedDesign ;
                              edo:hasTypedValue edo:FloatValue ;
                              edo:hasUnit unit:M ;
                              edo:hasValueCardinality edo:SingleValue .


###  https://w3id.org/energy-domain/edo#LayerGeometryThickness
edo:LayerGeometryThickness rdf:type owl:Class ;
                           rdfs:subClassOf edo:LayerGeometryAttribute ;
                           dcterms:accessRights "PUBLIC" ;
                           dcterms:identifier "LayerGeometryThickness" ;
                           skos:definition "Indicates the overall thickness of the layer's geometry. This property is critical for evaluating the structural contribution of the layer, including its strength, flexibility, and resistance to external forces."@en ;
                           skos:prefLabel "Espessura da Geometria da Camada"@pt-br ,
                                          "Layer Geometry Thickness"@en ;
                           edo:hasAttributeScope edo:InstanceLevelAttribute ;
                           edo:hasLifecycleCreationPhase edo:DetailedDesign ;
                           edo:hasTypedValue edo:FloatValue ;
                           edo:hasUnit unit:M ;
                           edo:hasValueCardinality edo:SingleValue .


###  https://w3id.org/energy-domain/edo#LayerThickness
edo:LayerThickness rdf:type owl:Class ;
                   rdfs:subClassOf edo:DomainAttribute ;
                   dcterms:accessRights "PUBLIC" ;
                   dcterms:identifier "LayerThickness" ;
                   skos:definition "Indicates the thickness of the layer, providing a key dimension that affects the overall strength, flexibility, and performance of the structure. This value is critical for ensuring that the layer meets design requirements and operational conditions."@en ;
                   skos:prefLabel "Espessura da camada"@pt-br ,
                                  "Layer Thickness"@en ;
                   edo:hasAttributeScope edo:InstanceLevelAttribute ;
                   edo:hasLifecycleCreationPhase edo:DetailedDesign ;
                   edo:hasTypedValue edo:FloatValue ;
                   edo:hasUnit unit:M ;
                   edo:hasValueCardinality edo:SingleValue .


###  https://w3id.org/energy-domain/edo#LayerWatertight
edo:LayerWatertight rdf:type owl:Class ;
                    rdfs:subClassOf edo:DomainAttribute ;
                    dcterms:accessRights "PUBLIC" ;
                    dcterms:identifier "LayerWatertight" ;
                    skos:definition "Indicates whether the layer is designed to be watertight. This property is critical for assessing the layer's ability to prevent water ingress, ensuring protection and maintaining the integrity of the structure in environments where exposure to water or fluids is expected."@en ;
                    skos:prefLabel "Camada Estanque"@pt-br ,
                                   "Layer Watertight"@en ;
                    edo:hasAttributeScope edo:InstanceLevelAttribute ;
                    edo:hasLifecycleCreationPhase edo:DetailedDesign ;
                    edo:hasTypedValue edo:BooleanValue ;
                    edo:hasValueCardinality edo:SingleValue .


###  https://w3id.org/energy-domain/edo#LayerWatertightLowerLayerInternalFreeVolume
edo:LayerWatertightLowerLayerInternalFreeVolume rdf:type owl:Class ;
                                                rdfs:subClassOf edo:DomainAttribute ;
                                                dcterms:accessRights "PUBLIC" ;
                                                dcterms:identifier "LayerWatertightLowerLayerInternalFreeVolume" ;
                                                skos:definition "Indicates the free volume between this layer and the previous continuous or watertight lower layer. If this layer is not watertight, or if there is no previous watertight lower layer, the value should be indicated as zero. This property is important for assessing the space that may affect pressure distribution or fluid movement within the structure."@en ,
                                                                "Volume livre interno entre essa camada e a camada inferior estanque. Se essa camada não for estanque ou caso não tenha camada inferior estanque, indicar zero."@pt-br ;
                                                skos:prefLabel "Layer Watertight Lower Layer Internal Free Volume"@en ,
                                                               "Volume Livre Interno da Camada Inferior Estanque"@pt-br ;
                                                edo:hasAttributeScope edo:InstanceLevelAttribute ;
                                                edo:hasLifecycleCreationPhase edo:DetailedDesign ;
                                                edo:hasTypedValue edo:FloatValue ;
                                                edo:hasUnit unit:M3-PER-M ,
                                                            edo:M3-PER-M ;
                                                edo:hasValueCardinality edo:SingleValue .


###  https://w3id.org/energy-domain/edo#LayingMinimumRadiusCurveAttribute
edo:LayingMinimumRadiusCurveAttribute rdf:type owl:Class ;
                                      rdfs:subClassOf edo:DomainAttribute .


###  https://w3id.org/energy-domain/edo#LayingMinimumRadiusTableColumn
edo:LayingMinimumRadiusTableColumn rdf:type owl:Class ;
                                   rdfs:subClassOf edo:LayingMinimumRadiusCurveAttribute .


###  https://w3id.org/energy-domain/edo#LayingMinimumRadiusTable_AbsoluteExternalPressure
edo:LayingMinimumRadiusTable_AbsoluteExternalPressure rdf:type owl:Class ;
                                                      rdfs:subClassOf edo:LayingMinimumRadiusTableColumn ;
                                                      dcterms:accessRights "PUBLIC" ;
                                                      dcterms:identifier "LayingMinimumRadiusTable_AbsoluteExternalPressure" ;
                                                      skos:definition "Represents the total pressure exerted on a component or system from the external environment, including both atmospheric and hydrostatic pressures. This property is critical for assessing the ability of the system to withstand the full pressure load, ensuring that it maintains structural integrity under extreme conditions."@en ;
                                                      skos:prefLabel "Absolute External Pressure"@en ,
                                                                     "Pressão Externa absoluta"@pt-br ;
                                                      edo:hasAttributeScope edo:TypeLevelAttribute ;
                                                      edo:hasLifecycleCreationPhase edo:DetailedDesign ;
                                                      edo:hasTypedValue edo:FloatValue ;
                                                      edo:hasUnit unit:PA ;
                                                      edo:hasValueCardinality edo:MultiValue .


###  https://w3id.org/energy-domain/edo#LayingMinimumRadiusTable_AbsoluteInternalPressure
edo:LayingMinimumRadiusTable_AbsoluteInternalPressure rdf:type owl:Class ;
                                                      rdfs:subClassOf edo:LayingMinimumRadiusTableColumn ;
                                                      dcterms:accessRights "PUBLIC" ;
                                                      dcterms:identifier "LayingMinimumRadiusTable_AbsoluteInternalPressure" ;
                                                      skos:definition "Represents the total pressure exerted inside a component or system, accounting for both the atmospheric pressure and any additional internal pressure. This property is crucial for determining the system's ability to handle internal forces, ensuring safe operation under the expected pressure conditions."@en ;
                                                      skos:prefLabel "Absolute Internal Pressure"@en ,
                                                                     "Pressão interna absoluta"@pt-br ;
                                                      edo:hasAttributeScope edo:TypeLevelAttribute ;
                                                      edo:hasLifecycleCreationPhase edo:DetailedDesign ;
                                                      edo:hasTypedValue edo:FloatValue ;
                                                      edo:hasUnit unit:PA ;
                                                      edo:hasValueCardinality edo:MultiValue .


###  https://w3id.org/energy-domain/edo#LayingMinimumRadiusTable_Compression
edo:LayingMinimumRadiusTable_Compression rdf:type owl:Class ;
                                         rdfs:subClassOf edo:LayingMinimumRadiusTableColumn ;
                                         dcterms:accessRights "PUBLIC" ;
                                         dcterms:identifier "LayingMinimumRadiusTable_Compression" ;
                                         skos:definition "Nota: Devem ser informados valores negativos. Por exemplo, para uma compressão de 10kN, deve ser informado -10."@pt-br ,
                                                         "Represents the force or stress applied to a material or component that causes it to decrease in size along a particular axis. This property is important for evaluating the material's ability to withstand compressive loads without failure."@en ;
                                         skos:prefLabel "Compression"@en ,
                                                        "Compressão"@pt-br ;
                                         edo:hasAttributeScope edo:TypeLevelAttribute ;
                                         edo:hasLifecycleCreationPhase edo:DetailedDesign ;
                                         edo:hasTypedValue edo:FloatValue ;
                                         edo:hasUnit unit:N ;
                                         edo:hasValueCardinality edo:MultiValue .


###  https://w3id.org/energy-domain/edo#LayingMinimumRadiusTable_MinimumAllowableBendingRadius
edo:LayingMinimumRadiusTable_MinimumAllowableBendingRadius rdf:type owl:Class ;
                                                           rdfs:subClassOf edo:LayingMinimumRadiusTableColumn ;
                                                           dcterms:accessRights "PUBLIC" ;
                                                           dcterms:identifier "LayingMinimumRadiusTable_MinimumAllowableBendingRadius" ;
                                                           skos:definition "Represents the smallest radius to which a component, such as a pipe or cable, can be bent without causing damage or compromising its structural integrity. This property is essential for determining handling and installation limits to avoid deformation or failure."@en ;
                                                           skos:prefLabel "Minimum Allowable Bending Radius"@en ,
                                                                          "Raio Mínimo de Curvatura Permitido"@pt-br ;
                                                           edo:hasAttributeScope edo:TypeLevelAttribute ;
                                                           edo:hasLifecycleCreationPhase edo:DetailedDesign ;
                                                           edo:hasTypedValue edo:StringValue ;
                                                           edo:hasValueCardinality edo:MultiValue .


###  https://w3id.org/energy-domain/edo#LayingMinimumRadiusTable_SectionSupportedByRigidSupport
edo:LayingMinimumRadiusTable_SectionSupportedByRigidSupport rdf:type owl:Class ;
                                                            rdfs:subClassOf edo:LayingMinimumRadiusTableColumn ;
                                                            dcterms:accessRights "PUBLIC" ;
                                                            dcterms:identifier "LayingMinimumRadiusTable_SectionSupportedByRigidSupport" ;
                                                            skos:definition "Indicates whether the section is supported by a rigid support (TRUE) or not (FALSE)."@en ;
                                                            skos:prefLabel "Section Supported By Rigid Support"@en ,
                                                                           "Seção Suportada por um Suporte Rígido"@pt-br ;
                                                            edo:hasAttributeScope edo:TypeLevelAttribute ;
                                                            edo:hasLifecycleCreationPhase edo:DetailedDesign ;
                                                            edo:hasTypedValue edo:BooleanValue ;
                                                            edo:hasValueCardinality edo:MultiValue .


###  https://w3id.org/energy-domain/edo#LayingMinimumRadiusTable_TensileArmourAnnulusCondition
edo:LayingMinimumRadiusTable_TensileArmourAnnulusCondition rdf:type owl:Class ;
                                                           rdfs:subClassOf edo:LayingMinimumRadiusTableColumn ;
                                                           dcterms:accessRights "PUBLIC" ;
                                                           dcterms:identifier "LayingMinimumRadiusTable_TensileArmourAnnulusCondition" ;
                                                           skos:definition "Condição do anular das armaduras de tração, Alagado ou Seco"@pt-br ,
                                                                           "Indicates the condition of the annulus in the tensile armour layer, which refers to the space between the tensile armour and other layers."@en ;
                                                           skos:prefLabel "Condição do Anular das Armaduras de Tração"@pt-br ,
                                                                          "Tensile Armour Annulus Condition"@en ;
                                                           edo:hasAttributeScope edo:TypeLevelAttribute ;
                                                           edo:hasLifecycleCreationPhase edo:DetailedDesign ;
                                                           edo:hasTypedValue edo:StringValue ;
                                                           edo:hasValueCardinality edo:MultiValue .


###  https://w3id.org/energy-domain/edo#Length
edo:Length rdf:type owl:Class ;
           rdfs:subClassOf edo:DomainAttribute ;
           dcterms:accessRights "PUBLIC" ;
           dcterms:identifier "Length" ;
           skos:definition "Length"@en ;
           skos:prefLabel "Comprimento"@pt-br ,
                          "Length"@en ;
           edo:hasAttributeScope edo:TypeLevelAttribute ;
           edo:hasLifecycleCreationPhase edo:DetailedDesign ;
           edo:hasTypedValue edo:FloatValue ;
           edo:hasUnit unit:M ,
                       unit:MilliM ;
           edo:hasValueCardinality edo:SingleValue .


###  https://w3id.org/energy-domain/edo#LifecyclePhase
edo:LifecyclePhase rdf:type owl:Class ;
                   rdfs:subClassOf edo:AttributeNature ;
                   rdfs:comment "Represents a stage in the lifecycle of an industrial asset."@en ;
                   rdfs:label "Fase do Ciclo de Vida"@pt-br ,
                              "Lifecycle Phase"@en ;
                   skos:definition "A stage in the lifecycle of an industrial asset, from conception to decommissioning."@en ,
                                   "Uma etapa no ciclo de vida de um ativo industrial, desde a concepção até a desativação."@pt-br .


###  https://w3id.org/energy-domain/edo#LiftingPoint
edo:LiftingPoint rdf:type owl:Class ;
                 rdfs:subClassOf edo:SupportPoint ;
                 dcterms:identifier "LiftingPoint" ;
                 skos:definition "Representa um ponto utilizado especificamente para operações de elevação."@pt-br ,
                                 "Represents a point used specifically for lifting operations."@en ;
                 skos:prefLabel "Lifting Point"@en ,
                                "Ponto de Elevação"@pt-br .


###  https://w3id.org/energy-domain/edo#LimpTorsionalStiffnessAtSeaLevel
edo:LimpTorsionalStiffnessAtSeaLevel rdf:type owl:Class ;
                                     rdfs:subClassOf edo:DomainAttribute ;
                                     dcterms:accessRights "PUBLIC" ;
                                     dcterms:identifier "LimpTorsionalStiffnessAtSeaLevel" ;
                                     skos:definition "Indicates the torsional stiffness of the structure when in a limp or flexible state at sea level conditions. This value is important for assessing how the structure resists twisting forces while maintaining flexibility during operations at sea level."@en ,
                                                     "Rigidez a torção (GJ) (menor valor) a 20°C e pressão atmosferica (dentro e fora)"@pt-br ;
                                     skos:prefLabel "Limp Torsional Stiffness At Sea Level"@en ,
                                                    "Rigidez à Torção em Estado Flexível ao Nível do Mar"@pt-br ;
                                     edo:hasAttributeScope edo:TypeLevelAttribute ;
                                     edo:hasLifecycleCreationPhase edo:DetailedDesign ;
                                     edo:hasTypedValue edo:FloatValue ;
                                     edo:hasUnit unit:N-M2-PER-RAD ,
                                                 edo:N-M2-PER-RAD ;
                                     edo:hasValueCardinality edo:SingleValue .


###  https://w3id.org/energy-domain/edo#LineAncillary
edo:LineAncillary rdf:type owl:Class ;
                  rdfs:subClassOf edo:Component ;
                  dcterms:identifier "LineAncillary" ;
                  skos:definition "A component designed to complement and enhance the functionality of subsea flexible pipes. Line Ancillaries include a variety of parts such as connectors, clamps, or collars that facilitate the installation, operation, and maintenance of flexible pipes used in subsea systems. These ancillaries ensure proper alignment, secure connections, and protection against environmental factors, contributing to the reliable performance and integrity of the flexible pipe system in harsh underwater conditions."@en ;
                  skos:prefLabel "Acessório de Linha"@pt-br ,
                                 "Line Ancillary"@en .


###  https://w3id.org/energy-domain/edo#LineSpan
edo:LineSpan rdf:type owl:Class ;
             rdfs:subClassOf edo:Location ;
             dcterms:identifier "LineSpan" ;
             skos:definition "Individual span of a complete line, with own characteristics"@en ,
                             "Trecho individual, com características particulares, de uma linha completa"@pt-br ;
             skos:prefLabel "Line span"@en ,
                            "Trecho de linha"@pt-br .


###  https://w3id.org/energy-domain/edo#LineTermination
edo:LineTermination rdf:type owl:Class ;
                    rdfs:subClassOf edo:ComponentDevice ;
                    dcterms:identifier "LineTermination" ;
                    skos:definition "Elemento de terminação integral a uma linha"@pt-br ,
                                    "The Line Termination includes components at the endpoints of flexible and rigid pipelines, as well as umbilical systems. These terminations provide secure connections to other equipment, enabling the transfer of fluids, gases, or control signals. Designed for stability and integrity, Line Termination components ensure durable and reliable performance across various pipeline types."@en ;
                    skos:prefLabel "Line Termination"@en ,
                                   "Terminador de Linha"@pt-br ;
                    edo:hasAttribute edo:OuterDiameter ,
                                     edo:WeightInWater .


###  https://w3id.org/energy-domain/edo#LineTerminationModule
edo:LineTerminationModule rdf:type owl:Class ;
                          rdfs:subClassOf edo:TieInEquipment ;
                          dcterms:identifier "LineTerminationModule" ;
                          skos:prefLabel "Line termination module"@en ,
                                         "Módulo de terminação de linha"@pt-br .


###  https://w3id.org/energy-domain/edo#LinearLocation
edo:LinearLocation rdf:type owl:Class ;
                   rdfs:subClassOf edo:Location ;
                   dcterms:identifier "LinearLocation" ;
                   skos:definition "Base for locations that extend along a geographically significant route."@en ,
                                   "Base para locais que se estendem ao longo de um percurso geograficamente significativo"@pt-br ;
                   skos:prefLabel "Linear Location"@en ,
                                  "Localização Linear"@pt-br .


###  https://w3id.org/energy-domain/edo#LinearMass
edo:LinearMass rdf:type owl:Class ;
               rdfs:subClassOf edo:DomainAttribute ;
               dcterms:accessRights "PUBLIC" ;
               dcterms:identifier "LinearMass" ;
               skos:definition "Indicates the mass per unit length, providing essential information for weight distribution and load calculations. This value is critical for evaluating how the structure will perform under various operational conditions, including installation and transport."@en ;
               skos:prefLabel "Linear Mass"@en ,
                              "Massa Linear"@pt-br ;
               edo:hasAttributeScope edo:TypeLevelAttribute ;
               edo:hasLifecycleCreationPhase edo:DetailedDesign ;
               edo:hasTypedValue edo:FloatValue ;
               edo:hasUnit unit:KiloGM-PER-M ;
               edo:hasValueCardinality edo:SingleValue .


###  https://w3id.org/energy-domain/edo#LinearObject
edo:LinearObject rdf:type owl:Class ;
                 rdfs:subClassOf edo:Asset ;
                 dcterms:identifier "LinearObject" ;
                 skos:definition "Base for any type of interconnecting element with linear geometry."@en ,
                                 "Base para qualquer tipo de elemento de interconexão com geometria linear"@pt-br ;
                 skos:prefLabel "Linear Object"@en ,
                                "Objeto Linear"@pt-br ;
                 edo:hasAttribute edo:Length .


###  https://w3id.org/energy-domain/edo#LinearWeight
edo:LinearWeight rdf:type owl:Class ;
                 rdfs:subClassOf edo:DomainAttribute ;
                 dcterms:accessRights "PUBLIC" ;
                 dcterms:identifier "LinearWeight" ;
                 skos:definition "Basic linear weight"@en ;
                 skos:prefLabel "Basic linear weight"@en ,
                                "Peso linear básico"@pt-br ;
                 edo:hasAttributeScope edo:TypeLevelAttribute ;
                 edo:hasLifecycleCreationPhase edo:DetailedDesign ;
                 edo:hasTypedValue edo:FloatValue ;
                 edo:hasUnit unit:KiloGM_F-PER-M ;
                 edo:hasValueCardinality edo:SingleValue .


###  https://w3id.org/energy-domain/edo#LinearWeightEmptySubmerged
edo:LinearWeightEmptySubmerged rdf:type owl:Class ;
                               rdfs:subClassOf edo:DomainAttribute ;
                               dcterms:accessRights "PUBLIC" ;
                               dcterms:identifier "LinearWeightEmptySubmerged" ;
                               skos:definition "Basic linear, empty, submerged"@en ;
                               skos:prefLabel "Basic linear, empty, submerged"@en ,
                                              "Peso linear, vazia, submersa"@pt-br ;
                               edo:hasAttributeScope edo:TypeLevelAttribute ;
                               edo:hasLifecycleCreationPhase edo:DetailedDesign ;
                               edo:hasTypedValue edo:FloatValue ;
                               edo:hasUnit unit:KiloGM_F-PER-M ;
                               edo:hasValueCardinality edo:SingleValue .


###  https://w3id.org/energy-domain/edo#LinearWeightFilled
edo:LinearWeightFilled rdf:type owl:Class ;
                       rdfs:subClassOf edo:DomainAttribute ;
                       dcterms:accessRights "PUBLIC" ;
                       dcterms:identifier "LinearWeightFilled" ;
                       rdfs:comment "Peso linear da estrutura, não submersa, mangueiras preenchidas com fluido hidráulico"@pt-br ;
                       skos:definition "Structure linear weight, unsubmerged, hoses filled with hydraulic fluid"@en ;
                       skos:prefLabel "Linear weight, filled, in air"@en ,
                                      "Peso linear, preenchido, no ar"@pt-br ;
                       edo:hasAttributeScope edo:TypeLevelAttribute ;
                       edo:hasLifecycleCreationPhase edo:DetailedDesign ;
                       edo:hasTypedValue edo:FloatValue ;
                       edo:hasUnit unit:KiloGM_F-PER-M ;
                       edo:hasValueCardinality edo:SingleValue .


###  https://w3id.org/energy-domain/edo#LinearWeightFilledAir
edo:LinearWeightFilledAir rdf:type owl:Class ;
                          rdfs:subClassOf edo:DomainAttribute ;
                          dcterms:accessRights "PUBLIC" ;
                          dcterms:identifier "LinearWeightFilledAir" ;
                          skos:definition "Basic linear, filled, in air"@en ;
                          skos:prefLabel "Basic linear, filled, in air"@en ,
                                         "Peso linear, preenchida, no ar"@pt-br ;
                          edo:hasAttributeScope edo:TypeLevelAttribute ;
                          edo:hasLifecycleCreationPhase edo:DetailedDesign ;
                          edo:hasTypedValue edo:FloatValue ;
                          edo:hasUnit unit:KiloGM_F-PER-M ;
                          edo:hasValueCardinality edo:SingleValue .


###  https://w3id.org/energy-domain/edo#LinearWeightFilledSubmerged
edo:LinearWeightFilledSubmerged rdf:type owl:Class ;
                                rdfs:subClassOf edo:DomainAttribute ;
                                dcterms:accessRights "PUBLIC" ;
                                dcterms:identifier "LinearWeightFilledSubmerged" ;
                                rdfs:comment "Peso linear efetivo da estrutura (descontando empuxo), submersa na água do mar, com mangueiras preenchidas com fluido hidráulico"@pt-br ;
                                skos:definition "Effective structure linear weight (subtracting upthrust), submerged into seawater and with hoses filled with hydraulic fluid"@en ;
                                skos:prefLabel "Linear weight, filled, submerged"@en ,
                                               "Peso linear, preenchido, submerso"@pt-br ;
                                edo:hasAttributeScope edo:TypeLevelAttribute ;
                                edo:hasLifecycleCreationPhase edo:DetailedDesign ;
                                edo:hasTypedValue edo:FloatValue ;
                                edo:hasUnit unit:KiloGM_F-PER-M ;
                                edo:hasValueCardinality edo:SingleValue .


###  https://w3id.org/energy-domain/edo#LinearWeightFilledSubmergedFlooded
edo:LinearWeightFilledSubmergedFlooded rdf:type owl:Class ;
                                       rdfs:subClassOf edo:DomainAttribute ;
                                       dcterms:accessRights "PUBLIC" ;
                                       dcterms:identifier "LinearWeightFilledSubmergedFlooded" ;
                                       rdfs:comment "Peso linear efetivo da estrutura (descontando empuxo), submersa na água do mar, com mangueiras preenchidas com fluido hidráulico e interstícios alagados"@pt-br ;
                                       skos:definition "Effective structure linear weight (subtracting upthrust), submerged into seawater, hoses filled with hydraulic fluid and flooded interstices"@en ;
                                       skos:prefLabel "Linear weight, filled, submerged, flooded"@en ,
                                                      "Peso linear, preenchido, submerso, alagado"@pt-br ;
                                       edo:hasAttributeScope edo:TypeLevelAttribute ;
                                       edo:hasLifecycleCreationPhase edo:DetailedDesign ;
                                       edo:hasTypedValue edo:FloatValue ;
                                       edo:hasUnit unit:KiloGM_F-PER-M ;
                                       edo:hasValueCardinality edo:SingleValue .


###  https://w3id.org/energy-domain/edo#LinearWeightSubmerged
edo:LinearWeightSubmerged rdf:type owl:Class ;
                          rdfs:subClassOf edo:DomainAttribute ;
                          dcterms:accessRights "PUBLIC" ;
                          dcterms:identifier "LinearWeightSubmerged" ;
                          rdfs:comment "Peso linear efetivo da estrutura (descontando empuxo), sem preenchimento com líquidos e submersa na água do mar"@pt-br ;
                          skos:definition "Effective structure linear weight (subtracting upthrust), empty of liquid and submerged into seawater"@en ;
                          skos:prefLabel "Linear weight, empty, submerged"@en ,
                                         "Peso linear, vazio, submerso"@pt-br ;
                          edo:hasAttributeScope edo:TypeLevelAttribute ;
                          edo:hasLifecycleCreationPhase edo:DetailedDesign ;
                          edo:hasTypedValue edo:FloatValue ;
                          edo:hasUnit unit:KiloGM_F-PER-M ;
                          edo:hasValueCardinality edo:SingleValue .


###  https://w3id.org/energy-domain/edo#Location
edo:Location rdf:type owl:Class ;
             rdfs:subClassOf edo:DomainElement ;
             dcterms:identifier "Location" ;
             skos:definition "Base para todos os locais de instalação neste modelo"@pt-br ,
                             "Basis for all model installation locations."@en ;
             skos:prefLabel "Localização"@pt-br ,
                            "Location"@en .


###  https://w3id.org/energy-domain/edo#LocationType
edo:LocationType rdf:type owl:Class ;
                 rdfs:subClassOf edo:ElementClassification ;
                 rdfs:label "Location Type"@en ,
                            "Tipo de Localização"@pt-br ;
                 skos:definition "Classification of industrial activities based on their geographical location."@en ,
                                 "Classificação de atividades industriais baseada em sua localização geográfica."@pt-br .


###  https://w3id.org/energy-domain/edo#LockedLength
edo:LockedLength rdf:type owl:Class ;
                 rdfs:subClassOf edo:DomainAttribute ;
                 dcterms:accessRights "PUBLIC" ;
                 dcterms:identifier "LockedLength" ;
                 rdfs:comment "Comprimido Restringido (vértebra \"travada\")"@pt-br ;
                 skos:definition "Comprimento de arco do restritor na configuração travada (restrita)"@en ;
                 skos:prefLabel "Comprimento travado"@pt-br ,
                                "Locked length"@en ;
                 edo:hasAttributeScope edo:TypeLevelAttribute ;
                 edo:hasLifecycleCreationPhase edo:DetailedDesign ;
                 edo:hasTypedValue edo:FloatValue ;
                 edo:hasUnit unit:M ;
                 edo:hasValueCardinality edo:SingleValue .


###  https://w3id.org/energy-domain/edo#LogicCap
edo:LogicCap rdf:type owl:Class ;
             rdfs:subClassOf edo:AuxiliaryModule ;
             dcterms:identifier "LogicCap" ;
             skos:prefLabel "Capa lógica"@pt-br ,
                            "Logic cap"@en .


###  https://w3id.org/energy-domain/edo#LogicalElement
edo:LogicalElement rdf:type owl:Class ;
                   rdfs:subClassOf edo:DomainElement ;
                   dcterms:identifier "LogicalElement" ;
                   skos:definition "Representa elementos de natureza não física, descrevendo aspectos funcionais, lógicos ou informacionais de um projeto ou sistema, apoiando projeto, operação e análise."@pt-br ,
                                   "Representa elementos de natureza não física, descrevendo aspectos funcionais, lógicos ou informacionais de um projeto ou sistema."@pt-br ,
                                   "Represents elements of a non-physical nature, describing functional, logical, or informational aspects of a project or system."@en ,
                                   "Represents elements that are non-physical, describing functional, logical, or informational aspects of a project or system, supporting design, operation, and analysis."@en ;
                   skos:prefLabel "Elemento Lógico"@pt-br ,
                                  "Logical Element"@en .


###  https://w3id.org/energy-domain/edo#LongTermFloatDensity
edo:LongTermFloatDensity rdf:type owl:Class ;
                         rdfs:subClassOf edo:DomainAttribute ;
                         dcterms:accessRights "PUBLIC" ;
                         dcterms:identifier "LongTermFloatDensity" ;
                         skos:definition "A densidade do flutuador ao longo do tempo, considerando o acúmulo de água no material ou mudanças na estrutura interna devido à degradação. Isso aumenta a densidade e, portanto, reduz a flutuabilidade"@pt-br ,
                                         "The density of the float material over time, considering factors like water absorption and material degradation, which increase the density and reduce the buoyancy."@en ;
                         skos:prefLabel "Densidade do Flutuador a Longo Prazo"@pt-br ,
                                        "Long Term Float Density"@en ;
                         edo:hasAttributeScope edo:TypeLevelAttribute ;
                         edo:hasLifecycleCreationPhase edo:DetailedDesign ;
                         edo:hasTypedValue edo:FloatValue ;
                         edo:hasUnit unit:KiloGM-PER-M3 ;
                         edo:hasValueCardinality edo:SingleValue .


###  https://w3id.org/energy-domain/edo#LongTermFloatVolume
edo:LongTermFloatVolume rdf:type owl:Class ;
                        rdfs:subClassOf edo:DomainAttribute ;
                        dcterms:accessRights "PUBLIC" ;
                        dcterms:identifier "LongTermFloatVolume" ;
                        skos:definition "O volume esperado ao longo do tempo, após fatores como absorção de água e possíveis deformações. Este volume representa as condições do flutuador em sua fase de vida útil, quando a flutuabilidade tende a ser menor."@pt-br ,
                                        "The expected submerged volume of the float over time, taking into account factors like water absorption and structural deformations that may occur throughout its lifecycle."@en ;
                        skos:prefLabel "Long Term Float Volume"@en ,
                                       "Volume do Flutuador a Longo Prazo"@pt-br ;
                        edo:hasAttributeScope edo:TypeLevelAttribute ;
                        edo:hasLifecycleCreationPhase edo:DetailedDesign ;
                        edo:hasTypedValue edo:FloatValue ;
                        edo:hasUnit unit:M3 ;
                        edo:hasValueCardinality edo:SingleValue .


###  https://w3id.org/energy-domain/edo#LongValue
edo:LongValue rdf:type owl:Class ;
              owl:equivalentClass [ rdf:type owl:Restriction ;
                                    owl:onProperty rdf:value ;
                                    owl:allValuesFrom xsd:long
                                  ] ;
              rdfs:subClassOf edo:DataType ;
              rdfs:comment "Constraint for xsd:long (64-bit integer)"@en ;
              rdfs:label "Long Value"@en .


###  https://w3id.org/energy-domain/edo#LowResistanceTape
edo:LowResistanceTape rdf:type owl:Class ;
                      rdfs:subClassOf edo:IfcInstanciableElement ,
                                      edo:TapeLayer ;
                      dcterms:identifier "LowResistanceTape" ;
                      skos:definition "A layer used in subsea flexible pipes to reduce friction between different components or layers, enhancing the overall flexibility and durability of the pipe. The Low Resistance Tape minimizes wear and abrasion caused by the movement of adjacent layers during operation, particularly in dynamic subsea conditions. Made from materials with low friction properties, it helps extend the lifespan of the pipe by reducing internal stresses and preventing damage to critical layers, ensuring smooth and efficient operation under harsh underwater conditions."@en ;
                      skos:prefLabel "Fita de Baixa Resistência"@pt-br ,
                                     "Low Resistance Tape"@en ;
                      edo:hasDiscipline edo:SubseaFlexiblePipesEngineering ;
                      edo:ifc_equivalentClass "IfcPipeSegment" ;
                      edo:ifc_objectType "LowResistanceTape" ;
                      edo:ifc_predefinedType "USERDEFINED" .


###  https://w3id.org/energy-domain/edo#Lubricant
edo:Lubricant rdf:type owl:Class ;
              rdfs:subClassOf edo:DomainAttribute ;
              dcterms:accessRights "PUBLIC" ;
              dcterms:identifier "Lubricant" ;
              skos:definition "Specifies the type of lubricant applied to reduce friction during tightening and ensure consistent torque application. The use of the correct lubricant is critical in preventing galling and corrosion, and helps to maintain the long-term integrity."@en ;
              skos:prefLabel "Lubricant"@en ,
                             "Nome do Lubrificante"@pt-br ;
              edo:hasAttributeScope edo:InstanceLevelAttribute ;
              edo:hasLifecycleCreationPhase edo:DetailedDesign ;
              edo:hasTypedValue edo:StringValue ;
              edo:hasValueCardinality edo:SingleValue .


###  https://w3id.org/energy-domain/edo#LubricantFrictionFactor
edo:LubricantFrictionFactor rdf:type owl:Class ;
                            rdfs:subClassOf edo:DomainAttribute ;
                            dcterms:accessRights "PUBLIC" ;
                            dcterms:identifier "LubricantFrictionFactor" ;
                            skos:definition "Indicates the friction factor of the lubricant applied, which affects the torque required to achieve proper tightening. This value is crucial for ensuring that the correct amount of torque is applied, accounting for the reduction in friction caused by the lubricant."@en ;
                            skos:prefLabel "Fator de atrito do lubrificante"@pt-br ,
                                           "Lubricant Friction Factor"@en ;
                            edo:hasAttributeScope edo:InstanceLevelAttribute ;
                            edo:hasLifecycleCreationPhase edo:DetailedDesign ;
                            edo:hasTypedValue edo:FloatValue ;
                            edo:hasValueCardinality edo:SingleValue .


###  https://w3id.org/energy-domain/edo#MainDesignNorm
edo:MainDesignNorm rdf:type owl:Class ;
                   rdfs:subClassOf edo:DomainAttribute ;
                   dcterms:accessRights "PUBLIC" ;
                   dcterms:identifier "MainDesignNorm" ;
                   rdfs:comment "Código ou norma de projeto principal utilizada para orientar o projeto e a construção da estrutura"@pt-br ;
                   skos:definition "Main design code or norm used as guidance for structure design and construction"@en ;
                   skos:prefLabel "Main design norm"@en ,
                                  "Norma principal de projeto"@pt-br ;
                   edo:hasAttributeScope edo:TypeLevelAttribute ;
                   edo:hasLifecycleCreationPhase edo:DetailedDesign ;
                   edo:hasTypedValue edo:StringValue ;
                   edo:hasValueCardinality edo:SingleValue .


###  https://w3id.org/energy-domain/edo#Maintenance
edo:Maintenance rdf:type owl:Class ;
                rdfs:subClassOf edo:OperationPhase ;
                rdfs:label "Maintenance"@en ,
                           "Manutenção"@pt-br ;
                skos:definition "Intervenções planejadas ou corretivas para preservar a funcionalidade e segurança do ativo."@pt-br ,
                                "Planned or corrective interventions to preserve asset functionality and safety."@en .


###  https://w3id.org/energy-domain/edo#MaintenancePoint
edo:MaintenancePoint rdf:type owl:Class ;
                     rdfs:subClassOf edo:SupportPoint ;
                     dcterms:identifier "MaintenancePoint" ;
                     skos:definition "Representa um ponto designado para fins de manutenção ou inspeção."@pt-br ,
                                     "Represents a point designated for maintenance or inspection purposes."@en ;
                     skos:prefLabel "Maintenance Point"@en ,
                                    "Ponto de Manutenção"@pt-br .


###  https://w3id.org/energy-domain/edo#Manifold
edo:Manifold rdf:type owl:Class ;
             rdfs:subClassOf edo:FlowControlEquipment ;
             dcterms:identifier "Manifold" ;
             skos:definition "Equipamento que concentra ou divide fluxos"@pt-br ,
                             "Equipment to join or split flows"@en ;
             skos:prefLabel "Manifold"@en ,
                            "Manifold"@pt-br .


###  https://w3id.org/energy-domain/edo#Manufacturer
edo:Manufacturer rdf:type owl:Class ;
                 rdfs:subClassOf edo:DomainAttribute ;
                 dcterms:accessRights "PUBLIC" ;
                 dcterms:identifier "Manufacturer" ;
                 skos:definition "Manufacturer"@en ;
                 skos:prefLabel "Fabricante"@pt-br ,
                                "Manufacturer"@en ;
                 edo:hasAttributeScope edo:TypeLevelAttribute ;
                 edo:hasLifecycleCreationPhase edo:DetailedDesign ;
                 edo:hasTypedValue edo:StringValue ;
                 edo:hasValueCardinality edo:SingleValue .


###  https://w3id.org/energy-domain/edo#ManufacturerDefinedMaterialName
edo:ManufacturerDefinedMaterialName rdf:type owl:Class ;
                                    rdfs:subClassOf edo:MaterialManufacturerAttribute ;
                                    dcterms:accessRights "PUBLIC" ;
                                    dcterms:identifier "ManufacturerDefinedMaterialName" ;
                                    skos:definition "Name of the material as designated by the manufacturer of the final item. This property identifies the specific material name used by the manufacturer, providing clarity on the material specifications for the finished accessory."@en ;
                                    skos:prefLabel "Manufacturer Defined Material Name"@en ,
                                                   "Nome do material conforme designado pelo fabricante do item final"@pt-br ;
                                    edo:hasAttributeScope edo:TypeLevelAttribute ;
                                    edo:hasLifecycleCreationPhase edo:DetailedDesign ;
                                    edo:hasTypedValue edo:StringValue ;
                                    edo:hasValueCardinality edo:MultiValue .


###  https://w3id.org/energy-domain/edo#ManufacturerSerialNumber
edo:ManufacturerSerialNumber rdf:type owl:Class ;
                             rdfs:subClassOf edo:DomainAttribute ;
                             dcterms:accessRights "PUBLIC" ;
                             dcterms:identifier "ManufacturerSerialNumber" ;
                             skos:definition "Identificador da unidade física atribuído pelo fabricante."@pt-br ,
                                             "Identifier of the physical unit assigned by the manufacturer."@en ;
                             skos:prefLabel "Manufacturer serial number"@en ,
                                            "Número de série do fabricante"@pt-br ;
                             edo:hasAttributeScope edo:InstanceLevelAttribute ;
                             edo:hasLifecycleCreationPhase edo:DetailedDesign ;
                             edo:hasTypedValue edo:StringValue ;
                             edo:hasValueCardinality edo:SingleValue .


###  https://w3id.org/energy-domain/edo#ManufacturingDate
edo:ManufacturingDate rdf:type owl:Class ;
                      rdfs:subClassOf edo:DomainAttribute ;
                      dcterms:accessRights "PUBLIC" ;
                      dcterms:identifier "ManufacturingDate" ;
                      skos:definition "Manufacturing date refers to the specific date when an object or product was produced or fabricated. This information is essential for tracking production batches, ensuring quality control, and determining the product’s shelf life or warranty period."@en ;
                      skos:prefLabel "Data de Fabricação"@pt-br ,
                                     "Manufacturing Date"@en ;
                      edo:hasAttributeScope edo:InstanceLevelAttribute ;
                      edo:hasLifecycleCreationPhase edo:DetailedDesign ;
                      edo:hasTypedValue edo:StringValue ;
                      edo:hasValueCardinality edo:SingleValue .


###  https://w3id.org/energy-domain/edo#ManufacturingNonConformities
edo:ManufacturingNonConformities rdf:type owl:Class ;
                                 rdfs:subClassOf edo:DomainAttribute ;
                                 dcterms:accessRights "PUBLIC" ;
                                 dcterms:identifier "ManufacturingNonConformities" ;
                                 skos:definition "Indicates whether the item has manufacturing non-conformities (TRUE) or not (FALSE)."@en ;
                                 skos:prefLabel "Manufacturing Non Conformities"@en ,
                                                "Não Conformidades de Fabricação"@pt-br ;
                                 edo:hasAttributeScope edo:InstanceLevelAttribute ;
                                 edo:hasLifecycleCreationPhase edo:DetailedDesign ;
                                 edo:hasTypedValue edo:BooleanValue ;
                                 edo:hasValueCardinality edo:SingleValue .


###  https://w3id.org/energy-domain/edo#Marine
edo:Marine rdf:type owl:Class ;
           rdfs:subClassOf edo:Renewable ;
           dcterms:identifier "Marine" ;
           skos:definition "Energia marinha refere-se à energia renovável aproveitada dos oceanos e mares, incluindo fluxos de marés, movimento das ondas, correntes oceânicas, gradientes térmicos e diferenças de salinidade. Representa um conjunto diversificado de tecnologias em desenvolvimento que visam complementar as fontes renováveis tradicionais ao explorar o vasto e previsível potencial energético do ambiente marinho."@pt-br ,
                           "Marine energy refers to renewable energy harnessed from the oceans and seas, including tidal flows, wave motion, ocean currents, thermal gradients and salinity differences. It represents a diverse set of technologies under development that aim to complement traditional renewable energy sources by exploiting the vast and predictable energy potential of the marine environment."@en ;
           skos:prefLabel "Energia Marinha"@pt-br ,
                          "Marine Energy"@en .


###  https://w3id.org/energy-domain/edo#Mass
edo:Mass rdf:type owl:Class ;
         rdfs:subClassOf edo:DomainAttribute ;
         dcterms:accessRights "PUBLIC" ;
         dcterms:identifier "Mass" ;
         skos:definition "Amount of matter that makes up an object."@en ;
         skos:prefLabel "Mass"@en ,
                        "Massa"@pt-br ;
         edo:hasAttributeScope edo:TypeLevelAttribute ;
         edo:hasLifecycleCreationPhase edo:DetailedDesign ;
         edo:hasTypedValue edo:FloatValue ;
         edo:hasUnit unit:KiloGM ,
                     edo:KiloGM ;
         edo:hasValueCardinality edo:SingleValue .


###  https://w3id.org/energy-domain/edo#MasterControlStation
edo:MasterControlStation rdf:type owl:Class ;
                         rdfs:subClassOf edo:TopsideEquipment ;
                         dcterms:identifier "MasterControlStation" ;
                         skos:definition "Painel elétrico de superfície que efetua o controle de sistemas multiplexados submarinos"@pt-br ,
                                         "Topside electrical panel for controlling subsea multiplexed systems"@en ;
                         skos:prefLabel "Estação de controle mestra"@pt-br ,
                                        "Master control station"@en .


###  https://w3id.org/energy-domain/edo#MaterialComposition
edo:MaterialComposition rdf:type owl:Class ;
                        rdfs:subClassOf edo:DomainAttribute ;
                        dcterms:accessRights "PUBLIC" ;
                        dcterms:identifier "MaterialComposition" ;
                        skos:definition "Indicates the composition of the fabrication material used. This property provides details about the specific material, helping to assess its mechanical, thermal, and chemical properties. It is crucial for evaluating the material's suitability for various operational conditions and services."@en ,
                                        "Tipo do material."@pt-br ;
                        skos:prefLabel "Composição do Material"@pt-br ,
                                       "Material Composition"@en ;
                        edo:hasAttributeScope edo:TypeLevelAttribute ;
                        edo:hasLifecycleCreationPhase edo:DetailedDesign ;
                        edo:hasTypedValue edo:StringValue ;
                        edo:hasValueCardinality edo:SingleValue .


###  https://w3id.org/energy-domain/edo#MaterialManufacturerAttribute
edo:MaterialManufacturerAttribute rdf:type owl:Class ;
                                  rdfs:subClassOf edo:DomainAttribute ;
                                  rdfs:label "Material Manufacturer"@en .


###  https://w3id.org/energy-domain/edo#MaterialRequest
edo:MaterialRequest rdf:type owl:Class ;
                    rdfs:subClassOf edo:DomainAttribute ;
                    dcterms:accessRights "PUBLIC" ;
                    dcterms:identifier "MaterialRequest" ;
                    skos:definition "Code used to identify the document that specifies the materials required for the project, serving as the basis for generating the purchase order. It ensures accurate tracking and procurement of necessary items for project execution."@en ;
                    skos:prefLabel "Código da Requisição de Material (RM)"@pt-br ,
                                   "Material Request"@en ;
                    edo:hasAttributeScope edo:InstanceLevelAttribute ;
                    edo:hasLifecycleCreationPhase edo:BasicDesign ;
                    edo:hasTypedValue edo:StringValue ;
                    edo:hasValueCardinality edo:SingleValue .


###  https://w3id.org/energy-domain/edo#MaterialRequestRev
edo:MaterialRequestRev rdf:type owl:Class ;
                       rdfs:subClassOf edo:DomainAttribute ;
                       dcterms:accessRights "PUBLIC" ;
                       dcterms:identifier "MaterialRequestRev" ;
                       skos:definition "Indicates the revision number of the Material Request document, ensuring that the most up-to-date version is referenced during procurement and project execution."@en ;
                       skos:prefLabel "Material Request Revision"@en ,
                                      "Revisão da Requisição de Material (RM)"@pt-br ;
                       edo:hasAttributeScope edo:InstanceLevelAttribute ;
                       edo:hasLifecycleCreationPhase edo:BasicDesign ;
                       edo:hasTypedValue edo:StringValue ;
                       edo:hasValueCardinality edo:SingleValue .


###  https://w3id.org/energy-domain/edo#MaterialSupplierName
edo:MaterialSupplierName rdf:type owl:Class ;
                         rdfs:subClassOf edo:MaterialManufacturerAttribute ;
                         dcterms:accessRights "PUBLIC" ;
                         dcterms:identifier "MaterialSupplierName" ;
                         skos:definition "Name of the company responsible for supplying the material. This property identifies the supplier of the material used in the accessory, ensuring traceability and accountability."@en ;
                         skos:prefLabel "Material Supplier Name"@en ,
                                        "Nome da empresa responsável por fornecer o material"@pt-br ;
                         edo:hasAttributeScope edo:TypeLevelAttribute ;
                         edo:hasLifecycleCreationPhase edo:DetailedDesign ;
                         edo:hasTypedValue edo:StringValue ;
                         edo:hasValueCardinality edo:SingleValue .


###  https://w3id.org/energy-domain/edo#MaterialType
edo:MaterialType rdf:type owl:Class ;
                 rdfs:subClassOf edo:DomainElement ;
                 skos:definition "Representa catálogos de materiais utilizados em projetos, fornecendo referências padrão para composição, propriedades e classificação."@pt-br ,
                                 "Represents catalogs of materials used within projects, providing standard references for composition, properties, and classification."@en ;
                 skos:prefLabel "Material Type"@en ,
                                "Tipo de Material"@pt-br .


###  https://w3id.org/energy-domain/edo#MatingEnvironment
edo:MatingEnvironment rdf:type owl:Class ;
                      rdfs:subClassOf edo:DomainAttribute ;
                      dcterms:accessRights "PUBLIC" ;
                      dcterms:identifier "MatingEnvironment" ;
                      rdfs:comment "Ambiente de conexão para o qual o conector foi projetado"@pt-br ;
                      skos:definition "Design mating environment for connector"@en ;
                      skos:prefLabel "Ambiente de conexão"@pt-br ,
                                     "Mating environment"@en ;
                      edo:hasAttributeScope edo:TypeLevelAttribute ;
                      edo:hasLifecycleCreationPhase edo:DetailedDesign ;
                      edo:hasTypedValue edo:StringValue ;
                      edo:hasValueCardinality edo:SingleValue .


###  https://w3id.org/energy-domain/edo#Mattress
edo:Mattress rdf:type owl:Class ;
             rdfs:subClassOf edo:PipeSupport ;
             dcterms:identifier "Mattress" ;
             skos:definition "Malleable mattress used to provide support or weight over a section of pipe"@en ,
                             "Manta maleável usada para prover suporte ou peso sobre uma seção de duto"@pt-br ;
             skos:prefLabel "Manta"@pt-br ,
                            "Mattress"@en .


###  https://w3id.org/energy-domain/edo#MaxCurrent
edo:MaxCurrent rdf:type owl:Class ;
               rdfs:subClassOf edo:DomainAttribute ;
               dcterms:accessRights "PUBLIC" ;
               dcterms:identifier "MaxCurrent" ;
               skos:prefLabel "Corrente máxima"@pt-br ,
                              "Maximum current"@en ;
               edo:hasAttributeScope edo:TypeLevelAttribute ;
               edo:hasLifecycleCreationPhase edo:DetailedDesign ;
               edo:hasTypedValue edo:FloatValue ;
               edo:hasValueCardinality edo:SingleValue .


###  https://w3id.org/energy-domain/edo#MaxDepth
edo:MaxDepth rdf:type owl:Class ;
             rdfs:subClassOf edo:DomainAttribute ;
             dcterms:accessRights "PUBLIC" ;
             dcterms:identifier "MaxDepth" ;
             rdfs:comment "Máxima profundidade de imersão tolerada por projeto"@pt-br ;
             skos:definition "Maximum immersion depth tolerated by design"@en ;
             skos:prefLabel "Maximum project depth"@en ,
                            "Profundidade máxima de projeto"@pt-br ;
             edo:hasAttributeScope edo:TypeLevelAttribute ;
             edo:hasLifecycleCreationPhase edo:DetailedDesign ;
             edo:hasTypedValue edo:FloatValue ;
             edo:hasUnit unit:M ;
             edo:hasValueCardinality edo:SingleValue .


###  https://w3id.org/energy-domain/edo#MaxDesignAbsIntPresCurveAttribute
edo:MaxDesignAbsIntPresCurveAttribute rdf:type owl:Class ;
                                      rdfs:subClassOf edo:DomainAttribute ;
                                      dcterms:accessRights "PUBLIC" ;
                                      dcterms:identifier "MaxDesignAbsIntPresTable" ;
                                      skos:definition "Provides data on the maximum design absolute internal pressure, used to evaluate the highest internal pressure the structure is designed to withstand. This information is critical for ensuring the structure's integrity and safety under the most demanding operational conditions."@en ;
                                      skos:prefLabel "Maximum Design Absolute Internal Pressure Table"@en ,
                                                     "Tabela da Máxima Pressão Interna Absoluta de Projeto"@pt-br ;
                                      edo:hasAttributeScope edo:InstanceLevelAttribute ;
                                      edo:hasLifecycleCreationPhase edo:BasicDesign .


###  https://w3id.org/energy-domain/edo#MaxDesignAbsIntPresTableColumn
edo:MaxDesignAbsIntPresTableColumn rdf:type owl:Class ;
                                   rdfs:subClassOf edo:MaxDesignAbsIntPresCurveAttribute ;
                                   edo:hasLifecycleCreationPhase edo:BasicDesign .


###  https://w3id.org/energy-domain/edo#MaxDesignAbsIntPresTable_PositionReference
edo:MaxDesignAbsIntPresTable_PositionReference rdf:type owl:Class ;
                                               rdfs:subClassOf edo:MaxDesignAbsIntPresTableColumn ;
                                               dcterms:accessRights "PUBLIC" ;
                                               dcterms:identifier "MaxDesignAbsIntPresTable_PositionReference" ;
                                               skos:definition "Identifies the specific point along the pipeline, such as the topside connection, TDP (Touchdown Point), or subsea connection point. This serves as the reference for vertical position and pressure values."@en ,
                                                               "Ponto. Valores válidos:Top (Para a conexão topside - E.g. Conector superior)TDPSubSeaConnection (Ex. ANM)"@pt-br ;
                                               skos:prefLabel "Position Reference"@en ,
                                                              "Referência de Posição"@pt-br ;
                                               edo:hasAttributeScope edo:InstanceLevelAttribute ;
                                               edo:hasLifecycleCreationPhase edo:BasicDesign ;
                                               edo:hasTypedValue edo:StringValue ;
                                               edo:hasValueCardinality edo:MultiValue .


###  https://w3id.org/energy-domain/edo#MaxDesignAbsIntPresTable_Pressure
edo:MaxDesignAbsIntPresTable_Pressure rdf:type owl:Class ;
                                      rdfs:subClassOf edo:MaxDesignAbsIntPresTableColumn ;
                                      dcterms:accessRights "PUBLIC" ;
                                      dcterms:identifier "MaxDesignAbsIntPresTable_Pressure" ;
                                      skos:definition "Indicates the force exerted per unit area on the surface of a material or component. This property is critical for evaluating how the component responds to external or internal forces, ensuring it can withstand operational pressure conditions."@en ;
                                      skos:prefLabel "Maximum Design Absolute Internal Pressure"@en ,
                                                     "Máxima Pressão Interna Absoluta de Projeto"@pt-br ;
                                      edo:hasAttributeScope edo:InstanceLevelAttribute ;
                                      edo:hasLifecycleCreationPhase edo:BasicDesign ;
                                      edo:hasTypedValue edo:FloatValue ;
                                      edo:hasUnit unit:PA ;
                                      edo:hasValueCardinality edo:MultiValue .


###  https://w3id.org/energy-domain/edo#MaxDesignAbsIntPresTable_VPosWRTWaterline
edo:MaxDesignAbsIntPresTable_VPosWRTWaterline rdf:type owl:Class ;
                                              rdfs:subClassOf edo:MaxDesignAbsIntPresTableColumn ;
                                              dcterms:accessRights "PUBLIC" ;
                                              dcterms:identifier "MaxDesignAbsIntPresTable_VPosWRTWaterline" ;
                                              skos:definition "Valores negativos para pontos submersos, e valores positivos para pontos acima da água. Considerando calado máximo da plataforma, quando aplicável."@pt-br ,
                                                              "Vertical position with respect to the waterline, where positive values indicate points above the water and negative values indicate points below. The platform's maximum draft is considered when applicable."@en ;
                                              skos:prefLabel "Posição Vertical em Relação à Linha D'Água"@pt-br ,
                                                             "Vertical Position With Respect To Waterline"@en ;
                                              edo:hasAttributeScope edo:InstanceLevelAttribute ;
                                              edo:hasLifecycleCreationPhase edo:BasicDesign ;
                                              edo:hasTypedValue edo:IntValue ;
                                              edo:hasUnit unit:M ;
                                              edo:hasValueCardinality edo:MultiValue .


###  https://w3id.org/energy-domain/edo#MaxDesignPressure
edo:MaxDesignPressure rdf:type owl:Class ;
                      rdfs:subClassOf edo:DomainAttribute ;
                      dcterms:accessRights "PUBLIC" ;
                      dcterms:identifier "MaxDesignPressure" ;
                      skos:definition "The highest internal or external pressure that the component or system is designed to withstand under operational conditions, ensuring safety and reliability."@en ;
                      skos:prefLabel "Maximum Design Pressure"@en ,
                                     "Pressão Máxima de Projeto"@pt-br ;
                      edo:hasAttributeScope edo:TypeLevelAttribute ;
                      edo:hasLifecycleCreationPhase edo:DetailedDesign ;
                      edo:hasTypedValue edo:FloatValue ;
                      edo:hasUnit unit:PA ;
                      edo:hasValueCardinality edo:SingleValue .


###  https://w3id.org/energy-domain/edo#MaxDragCoeff
edo:MaxDragCoeff rdf:type owl:Class ;
                 rdfs:subClassOf edo:DomainAttribute ;
                 dcterms:accessRights "PUBLIC" ;
                 dcterms:identifier "MaxDragCoeff" ;
                 skos:definition "Maximum drag coefficient"@en ;
                 skos:prefLabel "Coeficiente de arrasto máximo"@pt-br ,
                                "Maximum drag coefficient"@en ;
                 edo:hasAttributeScope edo:TypeLevelAttribute ;
                 edo:hasLifecycleCreationPhase edo:DetailedDesign ;
                 edo:hasTypedValue edo:FloatValue ;
                 edo:hasValueCardinality edo:SingleValue .


###  https://w3id.org/energy-domain/edo#MaxDynamicLoad
edo:MaxDynamicLoad rdf:type owl:Class ;
                   rdfs:subClassOf edo:DomainAttribute ;
                   dcterms:accessRights "PUBLIC" ;
                   dcterms:identifier "MaxDynamicLoad" ;
                   skos:definition "Maximum Dynamic Load (MDL) that the component can endure during operation. This value indicates the highest load the component can support while experiencing varying forces or impacts. Understanding this limit is essential for ensuring the component’s safety, reliability, and structural integrity in dynamic environments."@en ;
                   skos:prefLabel "Carga Dinâmica Máxima (MDL)"@pt-br ,
                                  "Maximum Dynamic Load (MDL)"@en ;
                   edo:hasAttributeScope edo:TypeLevelAttribute ;
                   edo:hasLifecycleCreationPhase edo:DetailedDesign ;
                   edo:hasTypedValue edo:FloatValue ;
                   edo:hasUnit unit:N ;
                   edo:hasValueCardinality edo:SingleValue .


###  https://w3id.org/energy-domain/edo#MaxLengthTolerance
edo:MaxLengthTolerance rdf:type owl:Class ;
                       rdfs:subClassOf edo:DomainAttribute ;
                       dcterms:accessRights "PUBLIC" ;
                       dcterms:identifier "MaxLengthTolerance" ;
                       skos:definition "Max length tolerance refers to the maximum allowable deviation from the specified or nominal length of an object. It defines the upper limit of acceptable variance during manufacturing or inspection, ensuring that the length stays within the defined range for quality control and compliance with design specifications."@en ;
                       skos:prefLabel "Maximum Length Tolerance"@en ,
                                      "Tolerância Máxima de Comprimento"@pt-br ;
                       edo:hasAttributeScope edo:InstanceLevelAttribute ;
                       edo:hasLifecycleCreationPhase edo:DetailedDesign ;
                       edo:hasTypedValue edo:FloatValue ;
                       edo:hasUnit unit:M ;
                       edo:hasValueCardinality edo:SingleValue .


###  https://w3id.org/energy-domain/edo#MaxPermissibleDeformationDynamic
edo:MaxPermissibleDeformationDynamic rdf:type owl:Class ;
                                     rdfs:subClassOf edo:DomainAttribute ;
                                     dcterms:accessRights "PUBLIC" ;
                                     dcterms:identifier "MaxPermissibleDeformationDynamic" ;
                                     skos:definition "Maximum deformation that the material can undergo under dynamic loading conditions is specified. This property is crucial for assessing how the material will behave when subjected to varying forces or impacts, ensuring it maintains functionality and structural integrity without excessive deformation or failure."@en ,
                                                     "Máxima Deformação Admissível (Aplicações Dinâmicas) (Específica para Materiais Poliméricos)"@pt-br ;
                                     skos:prefLabel "Maximum Permissible Deformation Dynamic"@en ,
                                                    "Máxima Deformação Admissível"@pt-br ;
                                     edo:hasAttributeScope edo:TypeLevelAttribute ;
                                     edo:hasLifecycleCreationPhase edo:DetailedDesign ;
                                     edo:hasTypedValue edo:FloatValue ;
                                     edo:hasUnit unit:PERCENT ;
                                     edo:hasValueCardinality edo:SingleValue .


###  https://w3id.org/energy-domain/edo#MaxPermissibleDeformationStatic
edo:MaxPermissibleDeformationStatic rdf:type owl:Class ;
                                    rdfs:subClassOf edo:DomainAttribute ;
                                    dcterms:accessRights "PUBLIC" ;
                                    dcterms:identifier "MaxPermissibleDeformationStatic" ;
                                    skos:definition "Indicates the maximum deformation the material can tolerate under static loading conditions. This property defines the extent to which the material can be deformed without failure or significant structural compromise when subjected to constant, non-varying forces or loads."@en ,
                                                    "Máxima Deformação Admissível (Aplicações Estáticas) (Específica para Materiais Poliméricos)"@pt-br ;
                                    skos:prefLabel "Maximum Permissible Deformation Static"@en ,
                                                   "Máxima Deformação Admissível em Aplicações Estáticas"@pt-br ;
                                    edo:hasAttributeScope edo:TypeLevelAttribute ;
                                    edo:hasLifecycleCreationPhase edo:DetailedDesign ;
                                    edo:hasTypedValue edo:FloatValue ;
                                    edo:hasUnit unit:PERCENT ;
                                    edo:hasValueCardinality edo:SingleValue .


###  https://w3id.org/energy-domain/edo#MaxPressure
edo:MaxPressure rdf:type owl:Class ;
                rdfs:subClassOf edo:DomainAttribute ;
                dcterms:accessRights "PUBLIC" ;
                dcterms:identifier "MaxPressure" ;
                rdfs:comment "Pressão máxima de projeto para as linhas hidráulicas"@pt-br ;
                skos:definition "Maximum design pressure for hydraulic lines"@en ;
                skos:prefLabel "Maximum design pressure"@en ,
                               "Pressão máxima de projeto"@pt-br ;
                edo:hasAttributeScope edo:TypeLevelAttribute ;
                edo:hasLifecycleCreationPhase edo:DetailedDesign ;
                edo:hasTypedValue edo:FloatValue ;
                edo:hasUnit unit:PSI ;
                edo:hasValueCardinality edo:SingleValue .


###  https://w3id.org/energy-domain/edo#MaximumAllowableTensileForStraightLine
edo:MaximumAllowableTensileForStraightLine rdf:type owl:Class ;
                                           rdfs:subClassOf edo:CrushingCurveAttribute ;
                                           dcterms:accessRights "PUBLIC" ;
                                           dcterms:identifier "MaximumAllowableTensileForStraightLine" ;
                                           skos:definition "MaximumAllowableTensileForStraightLine refers to the highest tensile force that can be applied to the flexible pipe in a straight-line configuration without risking damage or compromising the structural integrity of the pipe. This property is critical during installation and operation, ensuring that the pipe can withstand axial loads without overstressing or damaging its internal layers, such as the tensile armour, while maintaining safe handling limits."@en ;
                                           skos:prefLabel "Maximum Allowable Tensile For Straight Line"@en ,
                                                          "Tração Máxima Permitida para Linha Reta"@pt-br ;
                                           edo:hasAttributeScope edo:TypeLevelAttribute ;
                                           edo:hasLifecycleCreationPhase edo:DetailedDesign ;
                                           edo:hasTypedValue edo:FloatValue ;
                                           edo:hasUnit unit:N ;
                                           edo:hasValueCardinality edo:SingleValue .


###  https://w3id.org/energy-domain/edo#MaximumAllowableTensionTable_MaximumAllowableTensile
edo:MaximumAllowableTensionTable_MaximumAllowableTensile rdf:type owl:Class ;
                                                         rdfs:subClassOf edo:CrushingMaximumAllowableTensionTableColumn ;
                                                         dcterms:accessRights "PUBLIC" ;
                                                         dcterms:identifier "MaximumAllowableTensionTable_MaximumAllowableTensile" ;
                                                         skos:definition "Indicates the highest tensile force a component can safely withstand without compromising its integrity."@en ;
                                                         skos:prefLabel "Maximum Allowable Tensile"@en ,
                                                                        "Tração Máxima Permitida"@pt-br ;
                                                         edo:hasAttributeScope edo:TypeLevelAttribute ;
                                                         edo:hasLifecycleCreationPhase edo:DetailedDesign ;
                                                         edo:hasTypedValue edo:FloatValue ;
                                                         edo:hasUnit unit:N ;
                                                         edo:hasValueCardinality edo:MultiValue .


###  https://w3id.org/energy-domain/edo#MaximumAllowableTensionTable_PulleyRadius
edo:MaximumAllowableTensionTable_PulleyRadius rdf:type owl:Class ;
                                              rdfs:subClassOf edo:CrushingMaximumAllowableTensionTableColumn ;
                                              dcterms:accessRights "PUBLIC" ;
                                              dcterms:identifier "MaximumAllowableTensionTable_PulleyRadius" ;
                                              skos:definition "The distance measured from the center of the pulley to the bottom of the \"V\" shape."@en ;
                                              skos:prefLabel "Pulley Radius"@en ,
                                                             "Raio da Polia"@pt-br ;
                                              edo:hasAttributeScope edo:TypeLevelAttribute ;
                                              edo:hasLifecycleCreationPhase edo:DetailedDesign ;
                                              edo:hasTypedValue edo:FloatValue ;
                                              edo:hasUnit unit:M ;
                                              edo:hasValueCardinality edo:MultiValue .


###  https://w3id.org/energy-domain/edo#MaximumAllowableTensionTable_PulleyVAngle
edo:MaximumAllowableTensionTable_PulleyVAngle rdf:type owl:Class ;
                                              rdfs:subClassOf edo:CrushingMaximumAllowableTensionTableColumn ;
                                              dcterms:accessRights "PUBLIC" ;
                                              dcterms:identifier "MaximumAllowableTensionTable_PulleyVAngle" ;
                                              skos:definition "The angle formed by the opening of the \"V\" Groove in the pulley, measured in degrees."@en ;
                                              skos:prefLabel "Pulley V Groove Angle"@en ,
                                                             "Ângulo do Sulco em V da Polia"@pt-br ;
                                              edo:hasAttributeScope edo:TypeLevelAttribute ;
                                              edo:hasLifecycleCreationPhase edo:DetailedDesign ;
                                              edo:hasTypedValue edo:FloatValue ;
                                              edo:hasUnit unit:DEG ;
                                              edo:hasValueCardinality edo:MultiValue .


###  https://w3id.org/energy-domain/edo#MaximumAllowableTighteningTable_AxialLoad
edo:MaximumAllowableTighteningTable_AxialLoad rdf:type owl:Class ;
                                              rdfs:subClassOf edo:CrushingMaximumAllowableTighteningTableColumn ;
                                              dcterms:accessRights "PUBLIC" ;
                                              dcterms:identifier "MaximumAllowableTighteningTable_AxialLoad" ;
                                              skos:definition "Represents the force applied along the longitudinal axis of a component or system. This property is important for evaluating the ability of the structure to resist stretching or compression, ensuring it maintains integrity under operational loads."@en ;
                                              skos:prefLabel "Axial Load"@en ,
                                                             "Tabela de Aperto Máximo Permitido - Carga Axial"@pt-br ;
                                              edo:hasAttributeScope edo:TypeLevelAttribute ;
                                              edo:hasLifecycleCreationPhase edo:DetailedDesign ;
                                              edo:hasTypedValue edo:FloatValue ;
                                              edo:hasUnit unit:N ;
                                              edo:hasValueCardinality edo:MultiValue .


###  https://w3id.org/energy-domain/edo#MaximumAllowableTighteningTable_TighteningPerTrack
edo:MaximumAllowableTighteningTable_TighteningPerTrack rdf:type owl:Class ;
                                                       rdfs:subClassOf edo:CrushingMaximumAllowableTighteningTableColumn ;
                                                       dcterms:accessRights "PUBLIC" ;
                                                       dcterms:identifier "MaximumAllowableTighteningTable_TighteningPerTrack" ;
                                                       skos:definition "Indicates the amount of tightening applied per track during an operation. This property is important for ensuring consistent force distribution across multiple tracks, helping to maintain proper alignment and secure attachment during the tightening process."@en ;
                                                       skos:prefLabel "Tabela de Aperto Máximo Permitido - Aperto por Lagarta"@pt-br ,
                                                                      "Tightening Per Track"@en ;
                                                       edo:hasAttributeScope edo:TypeLevelAttribute ;
                                                       edo:hasLifecycleCreationPhase edo:DetailedDesign ;
                                                       edo:hasTypedValue edo:FloatValue ;
                                                       edo:hasUnit unit:N-PER-M ;
                                                       edo:hasValueCardinality edo:MultiValue .


###  https://w3id.org/energy-domain/edo#MaximumAmbientTemperature
edo:MaximumAmbientTemperature rdf:type owl:Class ;
                              rdfs:subClassOf edo:CrushingFrictionCoefficientTighteningAttribute ,
                                              edo:CrushingMaximumAllowableTensionAttribute ,
                                              edo:CrushingMaximumAllowableTighteningAttribute ;
                              dcterms:accessRights "PUBLIC" ;
                              dcterms:identifier "MaximumAmbientTemperature" ;
                              skos:definition "Represents the highest ambient temperature at which a component or material can operate effectively without risk of degradation or failure. This property is crucial for ensuring the material's performance and longevity under elevated temperature conditions."@en ;
                              skos:prefLabel "Maximum Ambient Temperature"@en ,
                                             "Temperatura ambiente máxima"@pt-br ;
                              edo:hasAttributeScope edo:TypeLevelAttribute ;
                              edo:hasLifecycleCreationPhase edo:DetailedDesign ;
                              edo:hasTypedValue edo:FloatValue ;
                              edo:hasUnit unit:K ;
                              edo:hasValueCardinality edo:SingleValue .


###  https://w3id.org/energy-domain/edo#MaximumBendingMoment
edo:MaximumBendingMoment rdf:type owl:Class ;
                         rdfs:subClassOf edo:DomainAttribute ;
                         dcterms:accessRights "PUBLIC" ;
                         dcterms:identifier "MaximumBendingMoment" ;
                         rdfs:comment "Momento fletor máximo de projeto (curto prazo)"@pt-br ;
                         skos:definition "Momento de curvatura máximo suportado pelo restritor, considerando uma força cisalhante nula"@en ;
                         skos:prefLabel "Maximum bending moment"@en ,
                                        "Momento de curvatura máximo"@pt-br ;
                         edo:hasAttributeScope edo:TypeLevelAttribute ;
                         edo:hasLifecycleCreationPhase edo:DetailedDesign ;
                         edo:hasTypedValue edo:FloatValue ;
                         edo:hasUnit unit:KiloN-M ;
                         edo:hasValueCardinality edo:SingleValue .


###  https://w3id.org/energy-domain/edo#MaximumBendingMomentLongTerm
edo:MaximumBendingMomentLongTerm rdf:type owl:Class ;
                                 rdfs:subClassOf edo:DomainAttribute ;
                                 dcterms:accessRights "PUBLIC" ;
                                 dcterms:identifier "MaximumBendingMomentLongTerm" ;
                                 rdfs:comment "Momento fletor máximo de projeto (longo prazo)"@pt-br ;
                                 skos:definition "Maximum long-term bending moment"@en ;
                                 skos:prefLabel "Maximum long-term bending moment"@en ,
                                                "Momento de curvatura máximo a longo prazo"@pt-br ;
                                 edo:hasAttributeScope edo:TypeLevelAttribute ;
                                 edo:hasLifecycleCreationPhase edo:DetailedDesign ;
                                 edo:hasTypedValue edo:FloatValue ;
                                 edo:hasUnit unit:KiloN-M ;
                                 edo:hasValueCardinality edo:SingleValue .


###  https://w3id.org/energy-domain/edo#MaximumHousedDiameter
edo:MaximumHousedDiameter rdf:type owl:Class ;
                          rdfs:subClassOf edo:DomainAttribute ;
                          dcterms:accessRights "PUBLIC" ;
                          dcterms:identifier "MaximumHousedDiameter" ;
                          rdfs:comment "Diâmetro externo máximo de cabo que pode ser acomodado pela capa"@pt-br ;
                          skos:definition "Maximum cable outer diameter which may be housed in cap"@en ;
                          skos:prefLabel "Diâmetro máximo acomodado"@pt-br ,
                                         "Maximum housed diameter"@en ;
                          edo:hasAttributeScope edo:TypeLevelAttribute ;
                          edo:hasLifecycleCreationPhase edo:DetailedDesign ;
                          edo:hasTypedValue edo:FloatValue ;
                          edo:hasUnit unit:MilliM ;
                          edo:hasValueCardinality edo:SingleValue .


###  https://w3id.org/energy-domain/edo#MaximumLength
edo:MaximumLength rdf:type owl:Class ;
                  rdfs:subClassOf edo:DomainAttribute ;
                  dcterms:accessRights "PUBLIC" ;
                  dcterms:identifier "MaximumLength" ;
                  rdfs:comment "Comprimido Livre (vértebra \"esticada\")"@pt-br ;
                  skos:definition "Comprimento reto assumido pelo restritor na configuração mais estendida"@en ;
                  skos:prefLabel "Comprimento máximo"@pt-br ,
                                 "Maximum length"@en ;
                  edo:hasAttributeScope edo:TypeLevelAttribute ;
                  edo:hasLifecycleCreationPhase edo:DetailedDesign ;
                  edo:hasTypedValue edo:FloatValue ;
                  edo:hasUnit unit:M ;
                  edo:hasValueCardinality edo:SingleValue .


###  https://w3id.org/energy-domain/edo#MaximumShearForce
edo:MaximumShearForce rdf:type owl:Class ;
                      rdfs:subClassOf edo:DomainAttribute ;
                      dcterms:accessRights "PUBLIC" ;
                      dcterms:identifier "MaximumShearForce" ;
                      rdfs:comment "Força de cisalhamento máxima de projeto (curto prazo)"@pt-br ;
                      skos:definition "Força cisalhante máxima suportada pelo restritor, considerando um momento de curvatura nulo"@en ;
                      skos:prefLabel "Força de cisalhamento máxima"@pt-br ,
                                     "Maximum shear force"@en ;
                      edo:hasAttributeScope edo:TypeLevelAttribute ;
                      edo:hasLifecycleCreationPhase edo:DetailedDesign ;
                      edo:hasTypedValue edo:FloatValue ;
                      edo:hasUnit unit:KiloN ;
                      edo:hasValueCardinality edo:SingleValue .


###  https://w3id.org/energy-domain/edo#MaximumShearForceLongTerm
edo:MaximumShearForceLongTerm rdf:type owl:Class ;
                              rdfs:subClassOf edo:DomainAttribute ;
                              dcterms:accessRights "PUBLIC" ;
                              dcterms:identifier "MaximumShearForceLongTerm" ;
                              rdfs:comment "Força de cisalhamento máxima de projeto (longo prazo)"@pt-br ;
                              skos:definition "Maximum long-term shear force"@en ;
                              skos:prefLabel "Força de cisalhamento máxima a longo prazo"@pt-br ,
                                             "Maximum long-term shear force"@en ;
                              edo:hasAttributeScope edo:TypeLevelAttribute ;
                              edo:hasLifecycleCreationPhase edo:DetailedDesign ;
                              edo:hasTypedValue edo:FloatValue ;
                              edo:hasUnit unit:KiloN ;
                              edo:hasValueCardinality edo:SingleValue .


###  https://w3id.org/energy-domain/edo#MaximumTemperature
edo:MaximumTemperature rdf:type owl:Class ;
                       rdfs:subClassOf edo:DomainAttribute ;
                       dcterms:accessRights "PUBLIC" ;
                       dcterms:identifier "MaximumTemperature" ;
                       skos:definition "Represents the highest temperature at which the structure or component can safely operate without compromising its integrity or performance. This value is critical for ensuring that materials and components maintain their mechanical properties and do not experience degradation, deformation, or failure under extreme thermal conditions."@en ;
                       skos:prefLabel "Maximum Temperature"@en ,
                                      "Temperatura Máxima"@pt-br ;
                       edo:hasAttributeScope edo:InstanceLevelAttribute ;
                       edo:hasLifecycleCreationPhase edo:BasicDesign ;
                       edo:hasTypedValue edo:FloatValue ;
                       edo:hasUnit unit:K ;
                       edo:hasValueCardinality edo:SingleValue .


###  https://w3id.org/energy-domain/edo#MaximumThermalExchangeCoefficient
edo:MaximumThermalExchangeCoefficient rdf:type owl:Class ;
                                      rdfs:subClassOf edo:DomainAttribute ;
                                      dcterms:accessRights "PUBLIC" ;
                                      dcterms:identifier "MaximumThermalExchangeCoefficient" ;
                                      skos:definition "Indicates the maximum allowable value for the Thermal Exchange Coefficient (TEC), specifying the upper limit for heat transfer in the design. This value ensures that the flexible pipeline meets thermal performance requirements without exceeding the permissible heat transfer rate, which could affect its integrity and operational efficiency."@en ;
                                      skos:prefLabel "Coeficiente Máximo de Troca Térmica (TEC)"@pt-br ,
                                                     "Maximum Thermal Exchange Coefficient (TEC)"@en ;
                                      edo:hasAttributeScope edo:InstanceLevelAttribute ;
                                      edo:hasLifecycleCreationPhase edo:BasicDesign ;
                                      edo:hasTypedValue edo:FloatValue ;
                                      edo:hasUnit unit:W-PER-M-K ;
                                      edo:hasValueCardinality edo:SingleValue .


###  https://w3id.org/energy-domain/edo#MbrDynamicOperation
edo:MbrDynamicOperation rdf:type owl:Class ;
                        rdfs:subClassOf edo:DomainAttribute ;
                        dcterms:accessRights "PUBLIC" ;
                        dcterms:identifier "MbrDynamicOperation" ;
                        skos:definition "Minimum bending radius, operation, dynamic"@en ;
                        skos:prefLabel "Minimum bending radius, operation, dynamic"@en ,
                                       "Raio de curvatura mínimo, operação, dinâmico"@pt-br ;
                        edo:hasAttributeScope edo:TypeLevelAttribute ;
                        edo:hasLifecycleCreationPhase edo:DetailedDesign ;
                        edo:hasTypedValue edo:FloatValue ;
                        edo:hasUnit unit:M ;
                        edo:hasValueCardinality edo:SingleValue .


###  https://w3id.org/energy-domain/edo#MbrStaticOperation
edo:MbrStaticOperation rdf:type owl:Class ;
                       rdfs:subClassOf edo:DomainAttribute ;
                       dcterms:accessRights "PUBLIC" ;
                       dcterms:identifier "MbrStaticOperation" ;
                       skos:definition "Minimum bending radius, operation, static"@en ;
                       skos:prefLabel "Minimum bending radius, operation, static"@en ,
                                      "Raio de curvatura mínimo, operação, estático"@pt-br ;
                       edo:hasAttributeScope edo:TypeLevelAttribute ;
                       edo:hasLifecycleCreationPhase edo:DetailedDesign ;
                       edo:hasTypedValue edo:FloatValue ;
                       edo:hasUnit unit:M ;
                       edo:hasValueCardinality edo:SingleValue .


###  https://w3id.org/energy-domain/edo#MeasuredValue
edo:MeasuredValue rdf:type owl:Class ;
                  rdfs:subClassOf edo:ValueOrigin ;
                  rdfs:comment "Obtained by direct measurement."@en ;
                  rdfs:label "Measured"@en ,
                             "Medido"@pt-br ;
                  skos:definition "Obtained by direct measurement"@en ,
                                  "Obtido por medição direta"@pt-br .


###  https://w3id.org/energy-domain/edo#MechanicalGender
edo:MechanicalGender rdf:type owl:Class ;
                     rdfs:subClassOf edo:DomainAttribute ;
                     dcterms:accessRights "PUBLIC" ;
                     dcterms:identifier "MechanicalGender" ;
                     skos:definition "Mechanical gender"@en ;
                     skos:prefLabel "Gênero mecânico"@pt-br ,
                                    "Mechanical gender"@en ;
                     edo:hasAttributeScope edo:TypeLevelAttribute ;
                     edo:hasLifecycleCreationPhase edo:DetailedDesign ;
                     edo:hasTypedValue edo:StringValue ;
                     edo:hasValueCardinality edo:SingleValue .


###  https://w3id.org/energy-domain/edo#MetallicLayerMaterialType
edo:MetallicLayerMaterialType rdf:type owl:Class ;
                              rdfs:subClassOf edo:DomainAttribute ;
                              dcterms:accessRights "PUBLIC" ;
                              dcterms:identifier "MetallicLayerMaterialType" ;
                              skos:definition "Type of material from which an object is made, allowing for precise documentation and categorisation."@en ;
                              skos:prefLabel "Metallic Layer Material Type"@en ,
                                             "Tipo de Material da Camada Metálica"@pt-br ;
                              edo:hasAttributeScope edo:TypeLevelAttribute ;
                              edo:hasLifecycleCreationPhase edo:DetailedDesign ;
                              edo:hasTypedValue edo:StringValue ;
                              edo:hasValueCardinality edo:SingleValue .


###  https://w3id.org/energy-domain/edo#MetallicLayerPitch
edo:MetallicLayerPitch rdf:type owl:Class ;
                       rdfs:subClassOf edo:DomainAttribute ;
                       dcterms:accessRights "PUBLIC" ;
                       dcterms:identifier "MetallicLayerPitch" ;
                       skos:definition "Indicates the distance between adjacent metallic elements in the layer, typically arranged helicoidally. This value is critical for determining the mechanical properties of the metallic layer, such as its flexibility, strength, and performance under load."@en ;
                       skos:prefLabel "Metallic Layer Pitch"@en ,
                                      "Passo da Camada Metálica"@pt-br ;
                       edo:hasAttributeScope edo:InstanceLevelAttribute ;
                       edo:hasLifecycleCreationPhase edo:DetailedDesign ;
                       edo:hasTypedValue edo:FloatValue ;
                       edo:hasUnit unit:M ;
                       edo:hasValueCardinality edo:SingleValue .


###  https://w3id.org/energy-domain/edo#MetallicMaterial
edo:MetallicMaterial rdf:type owl:Class ;
                     rdfs:subClassOf edo:FlexibleStructureLayerMaterial ,
                                     edo:IfcInstanciableElement ;
                     dcterms:identifier "MetallicMaterial" ;
                     skos:definition "Material used in the fabrication of metallic layers in subsea flexible pipes, chosen for its strength, durability, and resistance to harsh environmental conditions. The Metallic Material provides structural reinforcement, enhances pressure resistance, and supports the pipe's overall integrity. Commonly used materials include stainless steel, carbon steel, or other corrosion-resistant alloys, which are selected based on their ability to withstand the operational demands of deepwater environments, such as high pressure, tension, and dynamic loading."@en ;
                     skos:prefLabel "Material Metálico"@pt-br ,
                                    "Metallic Material"@en ;
                     edo:hasAttribute edo:FractureToughness ,
                                      edo:MetallicLayerMaterialType ,
                                      edo:UltimateTensileStress ;
                     edo:hasDiscipline edo:SubseaFlexiblePipesEngineering ,
                                       edo:SubseaUmbilicalsEngineering ;
                     edo:ifc_equivalentClass "IfcMaterial" ;
                     edo:ifc_objectType "MetallicMaterial" .


###  https://w3id.org/energy-domain/edo#MetallicStrandLength
edo:MetallicStrandLength rdf:type owl:Class ;
                         rdfs:subClassOf edo:DomainAttribute ;
                         dcterms:accessRights "PUBLIC" ;
                         dcterms:identifier "MetallicStrandLength" ;
                         skos:definition "The total length of the metallic strand used in the anode to endfittings connection"@en ;
                         skos:prefLabel "Comprimento da Cordoalha Metálica"@pt-br ,
                                        "Metallic Strand Length"@en ;
                         edo:hasAttributeScope edo:TypeLevelAttribute ;
                         edo:hasLifecycleCreationPhase edo:DetailedDesign ;
                         edo:hasTypedValue edo:FloatValue ;
                         edo:hasUnit unit:MilliM ;
                         edo:hasValueCardinality edo:SingleValue .


###  https://w3id.org/energy-domain/edo#MetallicStrandSet
edo:MetallicStrandSet rdf:type owl:Class ;
                      rdfs:subClassOf edo:IfcInstanciableElement ,
                                      edo:PhysicalConnection ;
                      dcterms:identifier "MetallicStrandSet" ;
                      skos:definition "Galvanic connection cables set providing reliable electrical link between anodes and metal infrastructure for effective corrosion mitigation."@en ;
                      skos:prefLabel "Conjunto de Cordoalhas de Continuidade"@pt-br ,
                                     "Metallic Strand Set"@en ;
                      edo:hasAttribute edo:StrandsTableAttribute ;
                      edo:hasDiscipline edo:SubseaFlexiblePipesEngineering ,
                                        edo:SubseaUmbilicalsEngineering ;
                      edo:ifc_equivalentClass "IfcCableSegment" ;
                      edo:ifc_objectType "MetallicStrandSet" ;
                      edo:ifc_predefinedType "USERDEFINED" .


###  https://w3id.org/energy-domain/edo#MetallicStrandSpareQuantity
edo:MetallicStrandSpareQuantity rdf:type owl:Class ;
                                rdfs:subClassOf edo:DomainAttribute ;
                                dcterms:accessRights "PUBLIC" ;
                                dcterms:identifier "MetallicStrandSpareQuantity" ;
                                skos:definition "The additional quantity of metallic strands provided as spare material for contingency or repair purposes."@en ;
                                skos:prefLabel "Metallic Strand Spare Quantity"@en ,
                                               "Quantidade de Cordoalhas Metálicas Sobressalentes"@pt-br ;
                                edo:hasAttributeScope edo:TypeLevelAttribute ;
                                edo:hasLifecycleCreationPhase edo:DetailedDesign ;
                                edo:hasTypedValue edo:IntValue ;
                                edo:hasValueCardinality edo:SingleValue .


###  https://w3id.org/energy-domain/edo#MetallicTubing
edo:MetallicTubing rdf:type owl:Class ;
                   rdfs:subClassOf edo:IfcInstanciableElement ,
                                   edo:Tubing ;
                   dcterms:identifier "MetallicTubing" ;
                   skos:definition "Representa um tubo metálico utilizado para transmissão de fluido ou suporte estrutural dentro de uma linha funcional umbilical."@pt-br ,
                                   "Represents a metallic tube used for fluid transmission or structural support within an umbilical function line."@en ;
                   skos:prefLabel "Metallic Tubing"@en ,
                                  "Metallic tubing"@en ,
                                  "Tubulação Metálica"@pt-br ,
                                  "Tubulação metálica"@pt-br ;
                   edo:hasDiscipline edo:SubseaUmbilicalsEngineering ;
                   edo:ifc_equivalentClass "IfcPipeSegment" ;
                   edo:ifc_objectType "MetallicTubing" ;
                   edo:ifc_predefinedType "USERDEFINED" .


###  https://w3id.org/energy-domain/edo#MetricBoltSet
edo:MetricBoltSet rdf:type owl:Class ;
                  rdfs:subClassOf edo:BoltSet ,
                                  edo:IfcInstanciableElement ;
                  dcterms:identifier "MetricBoltSet" ;
                  skos:definition "A set of bolts and accompanying hardware sized using the metric measurement system, commonly used in subsea applications for international compatibility and standardization."@en ;
                  skos:prefLabel "Conjunto de Parafusos Métrico"@pt-br ,
                                 "Metric Bolt Set"@en ;
                  edo:hasAttribute edo:NominalDiameter ,
                                   edo:PitchToleranceClass ,
                                   edo:ThreadPitch ,
                                   edo:ThreadStandard ;
                  edo:hasDiscipline edo:SubseaFlexiblePipesEngineering ,
                                    edo:SubseaUmbilicalsEngineering ;
                  edo:ifc_equivalentClass "IfcMechanicalFastener" ;
                  edo:ifc_objectType "MetricBoltSet" ;
                  edo:ifc_predefinedType "USERDEFINED" .


###  https://w3id.org/energy-domain/edo#MetricStudSet
edo:MetricStudSet rdf:type owl:Class ;
                  rdfs:subClassOf edo:IfcInstanciableElement ,
                                  edo:StudSet ;
                  dcterms:identifier "MetricStudSet" ;
                  skos:altLabel "Metric Stud"@en ,
                                "Metric Threaded Rod"@en ;
                  skos:definition "Metric studs are crucial fastening components for subsea oil and gas components, designed specifically to secure equipment parts. Each set includes bolts, nuts, and washers in metric sizing, made from high-strength, corrosion-resistant materials to withstand the demanding subsea environment. These components offer dependable fastening, ensuring structural integrity and leak prevention in end fittings. Metric stud sets are engineered to endure high pressure and extreme temperatures, making them essential for the safety and durability of subsea interconnections."@en ;
                  skos:prefLabel "Conjunto de Estojos Métrico"@pt-br ,
                                 "Metric Stud Set"@en ;
                  edo:hasAttribute edo:PitchToleranceClass ,
                                   edo:ThreadPitch ,
                                   edo:ThreadStandard ;
                  edo:hasDiscipline edo:SubseaFlexiblePipesEngineering ,
                                    edo:SubseaUmbilicalsEngineering ;
                  edo:ifc_equivalentClass "IfcMechanicalFastener" ;
                  edo:ifc_objectType "MetricStudSet" ;
                  edo:ifc_predefinedType "USERDEFINED" .


###  https://w3id.org/energy-domain/edo#Midstream
edo:Midstream rdf:type owl:Class ;
              rdfs:subClassOf edo:OilAndGas ;
              rdfs:label "Midstream"@en ,
                         "Midstream"@pt-br ;
              skos:definition "Oil & Gas sector covering transportation, storage, and wholesale marketing of crude or refined petroleum products."@en ,
                              "Setor de Petróleo & Gás que abrange transporte, armazenamento e comercialização atacadista de produtos petrolíferos brutos ou refinados."@pt-br .


###  https://w3id.org/energy-domain/edo#MinDragoeff
edo:MinDragoeff rdf:type owl:Class ;
                rdfs:subClassOf edo:DomainAttribute ;
                dcterms:accessRights "PUBLIC" ;
                dcterms:identifier "MinDragoeff" ;
                skos:definition "Minimum drag coefficient"@en ;
                skos:prefLabel "Coeficiente de arrasto mínimo"@pt-br ,
                               "Minimum drag coefficient"@en ;
                edo:hasAttributeScope edo:TypeLevelAttribute ;
                edo:hasLifecycleCreationPhase edo:DetailedDesign ;
                edo:hasTypedValue edo:FloatValue ;
                edo:hasValueCardinality edo:SingleValue .


###  https://w3id.org/energy-domain/edo#MinimumBendingRadius
edo:MinimumBendingRadius rdf:type owl:Class ;
                         rdfs:subClassOf edo:DomainAttribute ;
                         dcterms:accessRights "PUBLIC" ;
                         dcterms:identifier "MinimumBendingRadius" ;
                         rdfs:comment "MBR mínimo de cobertura"@pt-br ;
                         skos:definition "Raio de curvatura mínimo imposto pelo restritor"@en ;
                         skos:prefLabel "Minimum bending radius"@en ,
                                        "Raio de curvatura mínimo"@pt-br ;
                         edo:hasAttributeScope edo:TypeLevelAttribute ;
                         edo:hasLifecycleCreationPhase edo:DetailedDesign ;
                         edo:hasTypedValue edo:FloatValue ;
                         edo:hasUnit unit:M ;
                         edo:hasValueCardinality edo:SingleValue .


###  https://w3id.org/energy-domain/edo#MinimumBendingRadiusForStorage
edo:MinimumBendingRadiusForStorage rdf:type owl:Class ;
                                   rdfs:subClassOf edo:DomainAttribute ;
                                   dcterms:accessRights "PUBLIC" ;
                                   dcterms:identifier "MinimumBendingRadiusForStorage" ;
                                   skos:definition "Represents the smallest radius to which a component can be bent during storage without causing damage or affecting its performance. This property is important for ensuring that the component maintains its integrity while in storage, preventing deformation or weakening."@en ;
                                   skos:prefLabel "Minimum Bending Radius For Storage"@en ,
                                                  "Raio Mínimo de Curvatura para Armazenamento"@pt-br ;
                                   edo:hasAttributeScope edo:TypeLevelAttribute ;
                                   edo:hasLifecycleCreationPhase edo:DetailedDesign ;
                                   edo:hasTypedValue edo:FloatValue ;
                                   edo:hasUnit unit:M ;
                                   edo:hasValueCardinality edo:SingleValue .


###  https://w3id.org/energy-domain/edo#MinimumHousedDiameter
edo:MinimumHousedDiameter rdf:type owl:Class ;
                          rdfs:subClassOf edo:DomainAttribute ;
                          dcterms:accessRights "PUBLIC" ;
                          dcterms:identifier "MinimumHousedDiameter" ;
                          rdfs:comment "Diâmetro externo mínimo de cabo que pode ser acomodado pela capa"@pt-br ;
                          skos:definition "Minimum cable outer diameter which may be housed in cap"@en ;
                          skos:prefLabel "Diâmetro mínimo acomodado"@pt-br ,
                                         "Minimum housed diameter"@en ;
                          edo:hasAttributeScope edo:TypeLevelAttribute ;
                          edo:hasLifecycleCreationPhase edo:DetailedDesign ;
                          edo:hasTypedValue edo:FloatValue ;
                          edo:hasUnit unit:MilliM ;
                          edo:hasValueCardinality edo:SingleValue .


###  https://w3id.org/energy-domain/edo#MinimumLength
edo:MinimumLength rdf:type owl:Class ;
                  rdfs:subClassOf edo:DomainAttribute ;
                  dcterms:accessRights "PUBLIC" ;
                  dcterms:identifier "MinimumLength" ;
                  skos:definition "Comprimento reto assumido pelo restritor na configuração mais comprimida"@en ;
                  skos:prefLabel "Comprimento mínimo"@pt-br ,
                                 "Minimum length"@en ;
                  edo:hasAttributeScope edo:TypeLevelAttribute ;
                  edo:hasLifecycleCreationPhase edo:DetailedDesign ;
                  edo:hasTypedValue edo:FloatValue ;
                  edo:hasUnit unit:M ;
                  edo:hasValueCardinality edo:SingleValue .


###  https://w3id.org/energy-domain/edo#MinimumTemperature
edo:MinimumTemperature rdf:type owl:Class ;
                       rdfs:subClassOf edo:DomainAttribute ;
                       dcterms:accessRights "PUBLIC" ;
                       dcterms:identifier "MinimumTemperature" ;
                       skos:definition "Represents the lowest temperature at which the structure or component can safely operate without experiencing performance degradation or failure. This value is important for ensuring that the materials maintain their properties and structural integrity when exposed to extremely low temperatures"@en ;
                       skos:prefLabel "Minimum Temperature"@en ,
                                      "Temperatura Mínima"@pt-br ;
                       edo:hasAttributeScope edo:TypeLevelAttribute ;
                       edo:hasLifecycleCreationPhase edo:DetailedDesign ;
                       edo:hasTypedValue edo:FloatValue ;
                       edo:hasUnit unit:K ;
                       edo:hasValueCardinality edo:SingleValue .


###  https://w3id.org/energy-domain/edo#MinimumThermalExchangeCoefficient
edo:MinimumThermalExchangeCoefficient rdf:type owl:Class ;
                                      rdfs:subClassOf edo:DomainAttribute ;
                                      dcterms:accessRights "PUBLIC" ;
                                      dcterms:identifier "MinimumThermalExchangeCoefficient" ;
                                      skos:definition "Indicates the minimum allowable value for the Thermal Exchange Coefficient (TEC), specifying the lower limit for heat transfer in the design. This value ensures that the flexible pipeline maintains sufficient heat transfer capability to meet operational performance requirements."@en ;
                                      skos:prefLabel "Coeficiente Mínimo de Troca Térmica (TEC)"@pt-br ,
                                                     "Minimum Thermal Exchange Coefficient (TEC)"@en ;
                                      edo:hasAttributeScope edo:InstanceLevelAttribute ;
                                      edo:hasLifecycleCreationPhase edo:BasicDesign ;
                                      edo:hasTypedValue edo:FloatValue ;
                                      edo:hasUnit unit:W-PER-M-K ;
                                      edo:hasValueCardinality edo:SingleValue .


###  https://w3id.org/energy-domain/edo#ModulusOfElasticity
edo:ModulusOfElasticity rdf:type owl:Class ;
                        rdfs:subClassOf edo:DomainAttribute ;
                        dcterms:accessRights "PUBLIC" ;
                        dcterms:identifier "ModulusOfElasticity" ;
                        skos:definition "The modulus of elasticity represents the material's ability to resist deformation under stress. It quantifies the ratio of stress to strain within the elastic range of the material. This property is crucial for understanding how the material will behave under various loads and conditions."@en ;
                        skos:prefLabel "Modulus Of Elasticity"@en ,
                                       "Módulo de elasticidade"@pt-br ;
                        edo:hasAttributeScope edo:InstanceLevelAttribute ;
                        edo:hasLifecycleCreationPhase edo:DetailedDesign ;
                        edo:hasTypedValue edo:FloatValue ;
                        edo:hasUnit unit:PA ;
                        edo:hasValueCardinality edo:SingleValue .


###  https://w3id.org/energy-domain/edo#MooringAccessory
edo:MooringAccessory rdf:type owl:Class ;
                     rdfs:subClassOf edo:HardwareItem ;
                     dcterms:identifier "MooringAccessory" ;
                     skos:definition "A Mooring Accessory includes components like anchors, chains, and connectors used to secure offshore platforms or vessels to the seabed, ensuring stability and safety in harsh marine conditions."@en ;
                     skos:prefLabel "Acessório de Amarração"@pt-br ,
                                    "Mooring Accessory"@en .


###  https://w3id.org/energy-domain/edo#MultiValue
edo:MultiValue rdf:type owl:Class ;
               rdfs:subClassOf edo:AttributeValueCardinality ;
               rdfs:comment "Constraint allowing multiple values"@en ,
                            "Restrição para permitir múltiplos valores"@pt-br ;
               rdfs:label "Multiple Values"@en ,
                          "Múltiplos Valores"@pt-bt .


###  https://w3id.org/energy-domain/edo#NominalDiameter
edo:NominalDiameter rdf:type owl:Class ;
                    rdfs:subClassOf edo:DomainAttribute ;
                    dcterms:accessRights "PUBLIC" ;
                    dcterms:identifier "NominalDiameter" ;
                    skos:definition "The standard diameter of the component or pipe, typically used for classification and specification purposes."@en ;
                    skos:prefLabel "Diâmetro Nominal"@pt-br ,
                                   "Nominal Diameter"@en ;
                    edo:hasAttributeScope edo:InstanceLevelAttribute ;
                    edo:hasLifecycleCreationPhase edo:DetailedDesign ;
                    edo:hasTypedValue edo:StringValue ;
                    edo:hasUnit unit:MilliM ;
                    edo:hasValueCardinality edo:SingleValue .


###  https://w3id.org/energy-domain/edo#NominalFloatDensity
edo:NominalFloatDensity rdf:type owl:Class ;
                        rdfs:subClassOf edo:DomainAttribute ;
                        dcterms:accessRights "PUBLIC" ;
                        dcterms:identifier "NominalFloatDensity" ;
                        skos:definition "A densidade ideal do flutuador antes de qualquer absorção de água ou degradação. Usada para calcular a flutuabilidade inicial máxima, idealmente no ponto de fabricação."@pt-br ,
                                        "The ideal density of the float material before any water absorption or degradation occurs. This is used to calculate the float's maximum buoyancy at the beginning of its use."@en ;
                        skos:prefLabel "Densidade Nominal do Flutuador"@pt-br ,
                                       "Nominal Float Density"@en ;
                        edo:hasAttributeScope edo:TypeLevelAttribute ;
                        edo:hasLifecycleCreationPhase edo:DetailedDesign ;
                        edo:hasTypedValue edo:FloatValue ;
                        edo:hasUnit unit:KiloGM-PER-M3 ;
                        edo:hasValueCardinality edo:SingleValue .


###  https://w3id.org/energy-domain/edo#NominalFloatVolume
edo:NominalFloatVolume rdf:type owl:Class ;
                       rdfs:subClassOf edo:DomainAttribute ;
                       dcterms:accessRights "PUBLIC" ;
                       dcterms:identifier "NominalFloatVolume" ;
                       skos:definition "O volume ideal, ou \"de fábrica\", sem considerar a absorção de água ou deformações. É usado para calcular a flutuabilidade máxima possível, antes de qualquer degradação."@pt-br ,
                                       "The ideal or factory-specified volume of the float before any external effects like water absorption or deformation occur. This value is used to calculate the maximum buoyancy under perfect conditions."@en ;
                       skos:prefLabel "Nominal Float Volume"@en ,
                                      "Volume Nominal do Flutuador"@pt-br ;
                       edo:hasAttributeScope edo:TypeLevelAttribute ;
                       edo:hasLifecycleCreationPhase edo:DetailedDesign ;
                       edo:hasTypedValue edo:FloatValue ;
                       edo:hasUnit unit:M3 ,
                                   unit:m3 ;
                       edo:hasValueCardinality edo:SingleValue .


###  https://w3id.org/energy-domain/edo#NominalLength
edo:NominalLength rdf:type owl:Class ;
                  rdfs:subClassOf edo:DomainAttribute ;
                  dcterms:accessRights "PUBLIC" ;
                  dcterms:identifier "NominalLength" ;
                  skos:definition "Nominal length refers to the length of an object as designed, typically used as a reference value. It may not represent the exact physical measurement but serves as the standard or intended length for manufacturing, design, or specification purposes."@en ;
                  skos:prefLabel "Comprimento Nominal"@pt-br ,
                                 "Nominal Length"@en ;
                  edo:hasAttributeScope edo:InstanceLevelAttribute ;
                  edo:hasLifecycleCreationPhase edo:BasicDesign ,
                                                edo:DetailedDesign ;
                  edo:hasTypedValue edo:FloatValue ;
                  edo:hasUnit unit:M ;
                  edo:hasValueCardinality edo:SingleValue .


###  https://w3id.org/energy-domain/edo#Nuclear
edo:Nuclear rdf:type owl:Class ;
            rdfs:subClassOf edo:Domain ;
            rdfs:label "Energia Nuclear"@pt-br ,
                       "Nuclear Energy"@en ;
            skos:definition "Domínio industrial que abrange a geração de energia a partir de reações nucleares, incluindo fissão e fusão."@pt-br ,
                            "Industrial domain covering the generation of energy from nuclear reactions, including fission and fusion."@en .


###  https://w3id.org/energy-domain/edo#NuclearFuelCycle
edo:NuclearFuelCycle rdf:type owl:Class ;
                     rdfs:subClassOf edo:Nuclear ;
                     rdfs:label "Ciclo do Combustível Nuclear"@pt-br ,
                                "Nuclear Fuel Cycle"@en ;
                     skos:definition "Processes involved in mining, processing, enrichment, and disposal of nuclear fuel."@en ,
                                     "Processos envolvidos na mineração, processamento, enriquecimento e descarte de combustível nuclear."@pt-br .


###  https://w3id.org/energy-domain/edo#NuclearPowerGeneration
edo:NuclearPowerGeneration rdf:type owl:Class ;
                           rdfs:subClassOf edo:Nuclear ;
                           rdfs:label "Geração de Energia Nuclear"@pt-br ,
                                      "Nuclear Power Generation"@en ;
                           skos:definition "Operation and maintenance of nuclear power plants for electricity production."@en ,
                                           "Operação e manutenção de usinas nucleares para produção de eletricidade."@pt-br .


###  https://w3id.org/energy-domain/edo#NumFibers
edo:NumFibers rdf:type owl:Class ;
              rdfs:subClassOf edo:DomainAttribute ;
              dcterms:accessRights "PUBLIC" ;
              dcterms:identifier "NumFibers" ;
              rdfs:comment "Número de fibras"@pt-br ;
              skos:definition "Number of fibers"@en ;
              skos:prefLabel "Number of fibers"@en ;
              edo:hasAttributeScope edo:TypeLevelAttribute ;
              edo:hasLifecycleCreationPhase edo:DetailedDesign ;
              edo:hasTypedValue edo:StringValue ;
              edo:hasValueCardinality edo:SingleValue .


###  https://w3id.org/energy-domain/edo#NumGroupConductors
edo:NumGroupConductors rdf:type owl:Class ;
                       rdfs:subClassOf edo:DomainAttribute ;
                       dcterms:accessRights "PUBLIC" ;
                       dcterms:identifier "NumGroupConductors" ;
                       rdfs:comment "Número de condutores elétricos individuais que compõem cada agrupamento"@pt-br ;
                       skos:definition "Number of discrete electrical conductors that compose each grouping"@en ;
                       skos:prefLabel "Number of conductors per group"@en ,
                                      "Número de condutores por grupo"@pt-br ;
                       edo:hasTypedValue edo:IfcInteger .


###  https://w3id.org/energy-domain/edo#NumGroups
edo:NumGroups rdf:type owl:Class ;
              rdfs:subClassOf edo:DomainAttribute ;
              dcterms:accessRights "PUBLIC" ;
              dcterms:identifier "NumGroups" ;
              rdfs:comment "Número de agrupamentos de condutores elétricos contidos no cabo"@pt-br ;
              skos:definition "Number of electrical conductor groupings contained in the cable"@en ;
              skos:prefLabel "Number of conductor groups"@en ,
                             "Número de grupos de condutores"@pt-br ;
              edo:hasTypedValue edo:IfcInteger .


###  https://w3id.org/energy-domain/edo#NumMatingCycles
edo:NumMatingCycles rdf:type owl:Class ;
                    rdfs:subClassOf edo:DomainAttribute ;
                    dcterms:accessRights "PUBLIC" ;
                    dcterms:identifier "NumMatingCycles" ;
                    rdfs:comment "Número mínimo de ciclos de conexão/desconexão suportados pelo conector"@pt-br ;
                    skos:definition "Minimum number of mating/de-mating cycles withstood by connector"@en ;
                    skos:prefLabel "Number of withstood mating cycles"@en ,
                                   "Número de ciclos de conexão suportados"@pt-br ;
                    edo:hasTypedValue edo:IfcInteger .


###  https://w3id.org/energy-domain/edo#NumPhases
edo:NumPhases rdf:type owl:Class ;
              rdfs:subClassOf edo:DomainAttribute ;
              dcterms:accessRights "PUBLIC" ;
              dcterms:identifier "NumPhases" ;
              skos:prefLabel "Number of phases"@en ,
                             "Número de fases"@pt-br ;
              edo:hasAttributeScope edo:TypeLevelAttribute ;
              edo:hasLifecycleCreationPhase edo:DetailedDesign ;
              edo:hasTypedValue edo:StringValue .


###  https://w3id.org/energy-domain/edo#NumWays
edo:NumWays rdf:type owl:Class ;
            rdfs:subClassOf edo:DomainAttribute ;
            dcterms:accessRights "PUBLIC" ;
            dcterms:identifier "NumWays" ;
            skos:definition "Number of ways"@en ;
            skos:prefLabel "Number of ways"@en ,
                           "Número de vias"@pt-br ;
            edo:hasTypedValue edo:IfcInteger .


###  https://w3id.org/energy-domain/edo#NumberOfChokeValves
edo:NumberOfChokeValves rdf:type owl:Class ;
                        rdfs:subClassOf edo:DomainAttribute ;
                        dcterms:accessRights "PUBLIC" ;
                        dcterms:identifier "NumberOfChokeValves" ;
                        skos:definition "Number of process choke valves"@en ,
                                        "Número de válvulas choke"@pt-br ;
                        skos:prefLabel "Number Of Choke Valves"@en ,
                                       "Número de válvulas de estrangulamento"@pt-br ;
                        edo:hasAttributeScope edo:TypeLevelAttribute ;
                        edo:hasLifecycleCreationPhase edo:DetailedDesign ;
                        edo:hasTypedValue edo:IntValue ;
                        edo:hasValueCardinality edo:SingleValue .


###  https://w3id.org/energy-domain/edo#NumberOfRemoteProcessIsolationValves
edo:NumberOfRemoteProcessIsolationValves rdf:type owl:Class ;
                                         rdfs:subClassOf edo:DomainAttribute ;
                                         dcterms:accessRights "PUBLIC" ;
                                         dcterms:identifier "NumberOfRemoteProcessIsolationValves" ;
                                         skos:definition "Number of remotely-actuated process isolation valves"@en ,
                                                         "Número de válvulas de isolamento de processo com atuação remota"@pt-br ;
                                         skos:prefLabel "Number Of Remote Process Isolation Valves"@en ,
                                                        "Número de válvulas de isolamento de processo remoto"@pt-br ;
                                         edo:hasAttributeScope edo:TypeLevelAttribute ;
                                         edo:hasLifecycleCreationPhase edo:DetailedDesign ;
                                         edo:hasTypedValue edo:IntValue ;
                                         edo:hasValueCardinality edo:SingleValue .


###  https://w3id.org/energy-domain/edo#OceanCurrents
edo:OceanCurrents rdf:type owl:Class ;
                  rdfs:subClassOf edo:Marine ;
                  dcterms:identifier "OceanCurrents" ;
                  skos:definition "Energia das correntes oceânicas aproveita o fluxo contínuo das massas de água do oceano impulsionado por ventos, temperatura, salinidade e rotação da Terra. Turbinas instaladas em passagens marítimas estratégicas podem capturar esse recurso constante e previsível para gerar eletricidade renovável."@pt-br ,
                                  "Ocean currents energy harnesses the continuous flow of ocean water masses driven by wind, temperature, salinity and Earth’s rotation. Turbines placed in strategic marine passages can capture this steady and predictable resource to generate renewable electricity."@en ;
                  skos:prefLabel "Energia das Correntes Oceânicas"@pt-br ,
                                 "Ocean Currents Energy"@en .


###  https://w3id.org/energy-domain/edo#OceanThermal
edo:OceanThermal rdf:type owl:Class ;
                 rdfs:subClassOf edo:Marine ;
                 dcterms:identifier "OceanThermal" ;
                 skos:definition "A conversão de energia térmica oceânica (OTEC) explora a diferença de temperatura entre as águas superficiais quentes e as águas profundas frias para acionar um ciclo termodinâmico e produzir eletricidade. Oferece um vasto potencial de energia renovável ainda pouco explorado em regiões tropicais."@pt-br ,
                                 "Ocean thermal energy conversion (OTEC) exploits the temperature difference between warm surface waters and cold deep waters to drive a thermodynamic cycle and produce electricity. It offers a vast, largely untapped renewable energy potential in tropical regions."@en ;
                 skos:prefLabel "Conversão de Energia Térmica Oceânica"@pt-br ,
                                "Ocean Thermal Energy Conversion"@en .


###  https://w3id.org/energy-domain/edo#OffLeakPLevMaxPress
edo:OffLeakPLevMaxPress rdf:type owl:Class ;
                        rdfs:subClassOf edo:HydrostaticPressureTestsAttribute ;
                        dcterms:accessRights "PUBLIC" ;
                        dcterms:identifier "OffLeakPLevMaxPress" ;
                        skos:definition "Condições de teste dos tramos para Pressão - Máxima - Teste de vazamento hidrostático offshore (no nível da plataforma)"@pt-br ,
                                        "The maximum pressure applied during the Offshore Leak Test (at platform level), ensuring no leaks occur under extreme pressure."@en ;
                        skos:prefLabel "Offshore Leak Test At Platform Level Maximum Pressure"@en ,
                                       "Teste de Vazamento Offshore na Pressão Máxima no Nível da Plataforma"@pt-br ;
                        edo:hasAttributeScope edo:InstanceLevelAttribute ;
                        edo:hasLifecycleCreationPhase edo:DetailedDesign ;
                        edo:hasTypedValue edo:FloatValue ;
                        edo:hasUnit unit:PA ;
                        edo:hasValueCardinality edo:SingleValue .


###  https://w3id.org/energy-domain/edo#OffLeakPLevMaxPressValRef
edo:OffLeakPLevMaxPressValRef rdf:type owl:Class ;
                              rdfs:subClassOf edo:HydrostaticPressureTestsAttribute ;
                              dcterms:accessRights "PUBLIC" ;
                              dcterms:identifier "OffLeakPLevMaxPressValRef" ;
                              skos:definition "Comentários Condições de teste dos tramos para - Máximo - Teste de vazamento hidrostático offshore (no nível da plataforma)"@pt-br ,
                                              "Specifies the reference pressure used to determine the Offshore Leak Test maximum pressure value."@en ;
                              skos:prefLabel "Offshore Leak Test At Platform Level Maximum Pressure Value Reference"@en ,
                                             "Referência de Valor de Pressão Máxima para Teste de Vazamento Offshore no Nível da Plataforma"@pt-br ;
                              edo:hasAttributeScope edo:InstanceLevelAttribute ;
                              edo:hasLifecycleCreationPhase edo:DetailedDesign ;
                              edo:hasTypedValue edo:StringValue ;
                              edo:hasValueCardinality edo:SingleValue .


###  https://w3id.org/energy-domain/edo#OffLeakPLevMaxPressValRefMult
edo:OffLeakPLevMaxPressValRefMult rdf:type owl:Class ;
                                  rdfs:subClassOf edo:HydrostaticPressureTestsAttribute ;
                                  dcterms:accessRights "PUBLIC" ;
                                  dcterms:identifier "OffLeakPLevMaxPressValRefMult" ;
                                  skos:definition "The multiplier applied to the reference pressure to determine the Offshore Leak Test maximum pressure value."@en ;
                                  skos:prefLabel "Multiplicador de Referência de Valor de Pressão Máxima para Teste de Vazamento Offshore no Nível da Plataforma"@pt-br ,
                                                 "Offshore Leak Test At Platform Level Maximum Pressure Value Reference Multiplier"@en ;
                                  edo:hasAttributeScope edo:InstanceLevelAttribute ;
                                  edo:hasLifecycleCreationPhase edo:DetailedDesign ;
                                  edo:hasTypedValue edo:FloatValue ;
                                  edo:hasValueCardinality edo:SingleValue .


###  https://w3id.org/energy-domain/edo#OffLeakPLevNomPress
edo:OffLeakPLevNomPress rdf:type owl:Class ;
                        rdfs:subClassOf edo:HydrostaticPressureTestsAttribute ;
                        dcterms:accessRights "PUBLIC" ;
                        dcterms:identifier "OffLeakPLevNomPress" ;
                        skos:definition "Condições de teste dos tramos para Pressão - Nominal - Teste de vazamento hidrostático offshore (no nível da plataforma)"@pt-br ,
                                        "The nominal pressure applied during the Offshore Leak Test (at platform level), simulating typical operating conditions to assess for leaks."@en ;
                        skos:prefLabel "Offshore Leak Test At Platform Level Nominal Pressure"@en ,
                                       "Pressão Nominal para Teste de Vazamento Offshore no Nível da Plataforma"@pt-br ;
                        edo:hasAttributeScope edo:InstanceLevelAttribute ;
                        edo:hasLifecycleCreationPhase edo:DetailedDesign ;
                        edo:hasTypedValue edo:FloatValue ;
                        edo:hasUnit unit:PA ;
                        edo:hasValueCardinality edo:SingleValue .


###  https://w3id.org/energy-domain/edo#OffLeakPLevNomPressValRef
edo:OffLeakPLevNomPressValRef rdf:type owl:Class ;
                              rdfs:subClassOf edo:HydrostaticPressureTestsAttribute ;
                              dcterms:accessRights "PUBLIC" ;
                              dcterms:identifier "OffLeakPLevNomPressValRef" ;
                              skos:definition "Comentários Condições de teste dos tramos para - Nominal - Teste de vazamento hidrostático offshore (no nível da plataforma)"@pt-br ,
                                              "Specifies the reference pressure used to determine the Offshore Leak Test nominal pressure value."@en ;
                              skos:prefLabel "Offshore Leak Test At Platform Level Nominal Pressure Value Reference"@en ,
                                             "Referência de Valor de Pressão Nominal para Teste de Vazamento Offshore no Nível da Plataforma"@pt-br ;
                              edo:hasAttributeScope edo:InstanceLevelAttribute ;
                              edo:hasLifecycleCreationPhase edo:DetailedDesign ;
                              edo:hasTypedValue edo:StringValue ;
                              edo:hasValueCardinality edo:SingleValue .


###  https://w3id.org/energy-domain/edo#OffLeakPLevNomPressValRefMult
edo:OffLeakPLevNomPressValRefMult rdf:type owl:Class ;
                                  rdfs:subClassOf edo:HydrostaticPressureTestsAttribute ;
                                  dcterms:accessRights "PUBLIC" ;
                                  dcterms:identifier "OffLeakPLevNomPressValRefMult" ;
                                  skos:definition "The multiplier applied to the reference pressure to determine the Offshore Leak Test nominal pressure value."@en ;
                                  skos:prefLabel "Multiplicador de Referência de Valor de Pressão Nominal para Teste de Vazamento Offshore no Nível da Plataforma"@pt-br ,
                                                 "Offshore Leak Test At Platform Level Nominal Pressure Value Reference Multiplier"@en ;
                                  edo:hasAttributeScope edo:InstanceLevelAttribute ;
                                  edo:hasLifecycleCreationPhase edo:DetailedDesign ;
                                  edo:hasTypedValue edo:FloatValue ;
                                  edo:hasValueCardinality edo:SingleValue .


###  https://w3id.org/energy-domain/edo#Offshore
edo:Offshore rdf:type owl:Class ;
             rdfs:subClassOf edo:LocationType ;
             rdfs:label "Offshore"@en ,
                        "Offshore"@pt-br ;
             skos:definition "Atividades industriais realizadas no mar, tipicamente para produção de petróleo & gás ou energia eólica."@pt-br ,
                             "Industrial activities conducted at sea, typically for oil & gas or wind energy production."@en .


###  https://w3id.org/energy-domain/edo#OffshoreWind
edo:OffshoreWind rdf:type owl:Class ;
                 rdfs:subClassOf edo:Wind ;
                 dcterms:identifier "OffshoreWind" ;
                 skos:definition "Energia eólica offshore é gerada por turbinas localizadas em corpos d’água, geralmente em áreas costeiras rasas, onde os ventos são mais fortes e estáveis, permitindo a geração de energia em grande escala."@pt-br ,
                                 "Offshore wind energy is generated by turbines located in bodies of water, usually in shallow coastal areas, where winds are stronger and more stable, enabling large-scale power generation."@en ;
                 skos:prefLabel "Eólica Offshore"@pt-br ,
                                "Offshore Wind"@en .


###  https://w3id.org/energy-domain/edo#OilAndGas
edo:OilAndGas rdf:type owl:Class ;
              rdfs:subClassOf edo:Domain ;
              rdfs:label "Oil & Gas"@en ,
                         "Petróleo & Gás"@pt-br ;
              skos:definition "Domínio industrial que abrange todas as atividades relacionadas à exploração, produção, refino e distribuição de petróleo e gás."@pt-br ,
                              "Industrial domain covering all activities related to the exploration, production, refining, and distribution of oil and gas."@en .


###  https://w3id.org/energy-domain/edo#OilAndGasDevelopment
edo:OilAndGasDevelopment rdf:type owl:Class ;
                         rdfs:subClassOf edo:Upstream ;
                         dcterms:identifier "OilAndGasDevelopment" ;
                         skos:definition "Desenvolvimento de óleo e gás refere-se ao planejamento, engenharia, construção e comissionamento de instalações para explorar recursos hidrocarbonetos descobertos. Inclui perfuração de poços de desenvolvimento, instalação de instalações de produção e estabelecimento de infraestrutura de apoio para permitir extração e processamento."@pt-br ,
                                         "Oil and gas development refers to the planning, engineering, construction, and commissioning of facilities to exploit discovered hydrocarbon resources. It includes drilling development wells, installing production facilities, and establishing supporting infrastructure to enable extraction and processing."@en ;
                         skos:prefLabel "Desenvolvimento de Óleo e Gás"@pt-br ,
                                        "Oil and Gas Development"@en .


###  https://w3id.org/energy-domain/edo#OilAndGasDistribution
edo:OilAndGasDistribution rdf:type owl:Class ;
                          rdfs:subClassOf edo:Downstream ;
                          dcterms:identifier "OilAndGasDistribution" ;
                          skos:definition "Distribuição de óleo e gás abrange o transporte, armazenamento e entrega de produtos petrolíferos das unidades de processamento até os consumidores finais. Envolve dutos, terminais, navios-tanque e logística associada para garantir fornecimento seguro, confiável e eficiente de combustíveis e matérias-primas."@pt-br ,
                                          "Oil and gas distribution covers the transportation, storage, and delivery of petroleum products from processing facilities to end users. It involves pipelines, terminals, tankers, and associated logistics to ensure safe, reliable, and efficient supply of fuels and feedstocks."@en ;
                          skos:prefLabel "Distribuição de Óleo e Gás"@pt-br ,
                                         "Oil and Gas Distribution"@en .


###  https://w3id.org/energy-domain/edo#OilAndGasExploration
edo:OilAndGasExploration rdf:type owl:Class ;
                         rdfs:subClassOf edo:Upstream ;
                         dcterms:identifier "OilAndGasExploration" ;
                         skos:definition "Exploração de óleo e gás envolve a identificação e avaliação de potenciais reservas de hidrocarbonetos usando métodos geológicos, geofísicos e geoquímicos. As atividades incluem levantamentos sísmicos, perfuração exploratória e caracterização de reservatórios para avaliar a viabilidade da extração."@pt-br ,
                                         "Oil and gas exploration involves identifying and evaluating potential hydrocarbon reserves using geological, geophysical, and geochemical methods. Activities include seismic surveys, exploratory drilling, and reservoir characterization to assess the viability of extraction."@en ;
                         skos:prefLabel "Exploração de Óleo e Gás"@pt-br ,
                                        "Oil and Gas Exploration"@en .


###  https://w3id.org/energy-domain/edo#OilAndGasProduction
edo:OilAndGasProduction rdf:type owl:Class ;
                        rdfs:subClassOf edo:Upstream ;
                        dcterms:identifier "OilAndGasProduction" ;
                        skos:definition "Oil and gas production encompasses the extraction of hydrocarbons from reservoirs, including well operations, artificial lift, and initial processing to separate oil, gas, and water. It ensures the continuous supply of raw materials for downstream processing and energy generation."@en ,
                                        "Produção de óleo e gás engloba a extração de hidrocarbonetos dos reservatórios, incluindo operações de poços, elevação artificial e processamento inicial para separar óleo, gás e água. Garante o fornecimento contínuo de matérias-primas para processamento downstream e geração de energia."@pt-br ;
                        skos:prefLabel "Oil and Gas Production"@en ,
                                       "Produção de Óleo e Gás"@pt-br .


###  https://w3id.org/energy-domain/edo#OilAndGasRefining
edo:OilAndGasRefining rdf:type owl:Class ;
                      rdfs:subClassOf edo:Downstream ;
                      dcterms:identifier "OilAndGasRefining" ;
                      skos:definition "Oil and gas refining involves the conversion of crude oil and natural gas liquids into usable products such as gasoline, diesel, jet fuel, and petrochemicals. Refining processes include distillation, cracking, reforming, and treatment to meet product specifications and environmental standards."@en ,
                                      "Refino de óleo e gás envolve a conversão de petróleo bruto e líquidos de gás natural em produtos utilizáveis, como gasolina, diesel, querosene e petroquímicos. Os processos de refino incluem destilação, craqueamento, reforma e tratamento para atender especificações de produtos e padrões ambientais."@pt-br ;
                      skos:prefLabel "Oil and Gas Refining"@en ,
                                     "Refino de Óleo e Gás"@pt-br .


###  https://w3id.org/energy-domain/edo#Onshore
edo:Onshore rdf:type owl:Class ;
            rdfs:subClassOf edo:LocationType ;
            rdfs:label "Onshore"@en ,
                       "Onshore"@pt-br ;
            skos:definition "Atividades industriais realizadas em terra."@pt-br ,
                            "Industrial activities conducted on land."@en .


###  https://w3id.org/energy-domain/edo#OnshoreWind
edo:OnshoreWind rdf:type owl:Class ;
                rdfs:subClassOf edo:Wind ;
                dcterms:identifier "OnshoreWind" ;
                skos:definition "Energia eólica onshore é produzida por turbinas eólicas instaladas em terra, geralmente em regiões com recursos eólicos elevados e consistentes. É uma das fontes de energia renovável mais maduras e economicamente viáveis."@pt-br ,
                                "Onshore wind energy is produced by wind turbines installed on land, typically in areas with high and consistent wind resources. It is one of the most mature and cost-effective renewable energy sources."@en ;
                skos:prefLabel "Eólica Onshore"@pt-br ,
                               "Onshore Wind"@en .


###  https://w3id.org/energy-domain/edo#OpenReceptacle
edo:OpenReceptacle rdf:type owl:Class ;
                   rdfs:subClassOf edo:RiserSupport ;
                   dcterms:identifier "OpenReceptacle" ;
                   skos:prefLabel "Open receptacle"@en ,
                                  "Receptáculo aberto"@pt-br .


###  https://w3id.org/energy-domain/edo#Operation
edo:Operation rdf:type owl:Class ;
              rdfs:subClassOf edo:OperationPhase ;
              rdfs:label "Operation"@en ,
                         "Operação"@pt-br ;
              skos:definition "Normal use of the asset for its intended purpose, including monitoring and control."@en ,
                              "Uso normal do ativo para seu propósito pretendido, incluindo monitoramento e controle."@pt-br .


###  https://w3id.org/energy-domain/edo#OperationPhase
edo:OperationPhase rdf:type owl:Class ;
                   rdfs:subClassOf edo:LifecyclePhase ;
                   rdfs:label "Fase de Operação"@pt-br ,
                              "Operation Phase"@en .


###  https://w3id.org/energy-domain/edo#OpticalFiberCable
edo:OpticalFiberCable rdf:type owl:Class ;
                      rdfs:subClassOf edo:FunctionLine ,
                                      edo:IfcInstanciableElement ;
                      dcterms:identifier "OpticalFiberCable" ;
                      skos:definition "Representa um cabo de fibra óptica dentro de uma linha funcional, transmitindo sinais ópticos para comunicação ou monitoramento."@pt-br ,
                                      "Represents an optical fiber cable within a function line, transmitting optical signals for communication or sensing purposes."@en ;
                      skos:prefLabel "Cabo de Fibra Óptica"@pt-br ,
                                     "Cabo de fibra ótica"@pt-br ,
                                     "Optical Fiber Cable"@en ,
                                     "Optical fiber cable"@en ;
                      edo:hasAttribute edo:AttenuationCoefficient ,
                                       edo:CladdingDiameter ,
                                       edo:CoreDiameter ,
                                       edo:FiberType ,
                                       edo:NumFibers ;
                      edo:hasDiscipline edo:SubseaUmbilicalsEngineering ;
                      edo:ifc_equivalentClass "IfcCableSegment" ;
                      edo:ifc_objectType "OpticalFiberCable" ;
                      edo:ifc_predefinedType "USERDEFINED" .


###  https://w3id.org/energy-domain/edo#OuterArea
edo:OuterArea rdf:type owl:Class ;
              rdfs:subClassOf edo:DomainAttribute ;
              dcterms:accessRights "PUBLIC" ;
              dcterms:identifier "OuterArea" ;
              rdfs:comment "Área ocupada pela seção transversal completa da estrutura"@pt-br ;
              skos:definition "Area occupied by entire structure cross-section"@en ;
              skos:prefLabel "Outer section area"@en ,
                             "Área da seção externa"@pt-br ;
              edo:hasAttributeScope edo:TypeLevelAttribute ;
              edo:hasLifecycleCreationPhase edo:DetailedDesign ;
              edo:hasTypedValue edo:FloatValue ;
              edo:hasUnit unit:L-PER-M ;
              edo:hasValueCardinality edo:SingleValue .


###  https://w3id.org/energy-domain/edo#OuterDiameter
edo:OuterDiameter rdf:type owl:Class ;
                  rdfs:subClassOf edo:DomainAttribute ;
                  dcterms:accessRights "PUBLIC" ;
                  dcterms:identifier "OuterDiameter" ;
                  skos:definition "Represents the external diameter of a component, typically measured from one outer edge to the opposite outer edge. This property is important for ensuring proper fit, compatibility, and performance within a system or assembly."@en ;
                  skos:prefLabel "Diâmetro externo"@pt-br ,
                                 "Outer Diameter"@en ;
                  edo:hasAttributeScope edo:TypeLevelAttribute ;
                  edo:hasLifecycleCreationPhase edo:DetailedDesign ;
                  edo:hasTypedValue edo:FloatValue ;
                  edo:hasUnit unit:M ,
                              unit:MilliM ;
                  edo:hasValueCardinality edo:SingleValue .


###  https://w3id.org/energy-domain/edo#OutsideTemperature
edo:OutsideTemperature rdf:type owl:Class ;
                       rdfs:subClassOf edo:BendingStiffnessCurveAttribute ,
                                       edo:DomainAttribute ;
                       dcterms:accessRights "PUBLIC" ;
                       dcterms:identifier "OutsideTemperature" ;
                       skos:definition "Represents the external temperature surrounding a component or system. This property is important for assessing the thermal conditions that the component is exposed to, ensuring it operates within safe temperature limits."@en ;
                       skos:prefLabel "Outside Temperature"@en ,
                                      "Temperatura Externa"@pt-br ;
                       edo:hasAttributeScope edo:TypeLevelAttribute ;
                       edo:hasLifecycleCreationPhase edo:DetailedDesign ;
                       edo:hasTypedValue edo:FloatValue ;
                       edo:hasUnit unit:K ;
                       edo:hasValueCardinality edo:SingleValue .


###  https://w3id.org/energy-domain/edo#OverallShieldingType
edo:OverallShieldingType rdf:type owl:Class ;
                         rdfs:subClassOf edo:DomainAttribute ;
                         dcterms:accessRights "PUBLIC" ;
                         dcterms:identifier "OverallShieldingTypeShieldingType" ;
                         rdfs:comment "Especifica o tipo de blindagem eletromagnética aplicada globalmente ao feixe completo de condutores"@pt-br ;
                         skos:definition "Specifies the type of electromagnetic shielding applied globally to the entire conductor bundle"@en ;
                         skos:prefLabel "General shielding type"@en ,
                                        "Tipo de blindagem geral"@pt-br ;
                         edo:hasAttributeScope edo:TypeLevelAttribute ;
                         edo:hasLifecycleCreationPhase edo:DetailedDesign ;
                         edo:hasTypedValue edo:StringValue ;
                         edo:hasValueCardinality edo:SingleValue .


###  https://w3id.org/energy-domain/edo#OverrideTool
edo:OverrideTool rdf:type owl:Class ;
                 rdfs:subClassOf edo:ROVTool ;
                 dcterms:identifier "OverrideTool" ;
                 skos:prefLabel "Ferramenta de Override"@pt-br ,
                                "Override Tool"@en .


###  https://w3id.org/energy-domain/edo#PLEM
edo:PLEM rdf:type owl:Class ;
         rdfs:subClassOf edo:Manifold ;
         dcterms:identifier "PLEM" ;
         skos:definition "Manifold instalado no final de uma linha rígida, servindo também como elemento de ancoragem"@pt-br ,
                         "Manifold installed at the end of a rigid pipeline, also serving as an anchoring element"@en ;
         skos:prefLabel "PLEM"@en ,
                        "PLEM"@pt-br ;
         edo:hasDiscipline edo:SubseaManifoldsEngineering .


###  https://w3id.org/energy-domain/edo#PLET
edo:PLET rdf:type owl:Class ;
         rdfs:subClassOf edo:FlowControlEquipment ;
         dcterms:identifier "PLET" ;
         skos:definition "Equipamento para terminação e ancoragem de um duto que oferece uma interface para conexão externa"@pt-br ,
                         "Equipment for pipeline termination and anchoring, offering an interface for external connection"@en ;
         skos:prefLabel "PLET"@en ,
                        "PLET"@pt-br ;
         edo:hasDiscipline edo:SubseaManifoldsEngineering .


###  https://w3id.org/energy-domain/edo#PackageEquipmentEngineering
edo:PackageEquipmentEngineering rdf:type owl:Class ;
                                rdfs:subClassOf edo:EquipmentEngineering ;
                                rdfs:label "Engenharia de Equipamentos Modulares"@pt-br ,
                                           "Package Equipment Engineering"@en ;
                                skos:definition "Engenharia de sistemas de equipamentos modulares ou montados em skids."@pt-br ,
                                                "Engineering of skid-mounted or modular equipment systems."@en .


###  https://w3id.org/energy-domain/edo#PanelConnector
edo:PanelConnector rdf:type owl:Class ;
                   rdfs:subClassOf edo:Connector ;
                   dcterms:identifier "PanelConnector" ;
                   skos:definition "Conectores para instalação em painéis ou outras posições estacionárias."@pt-br ,
                                   "Connectors for installation in panels or other stationary positions."@en ;
                   skos:prefLabel "Conector de Painel"@pt-br ,
                                  "Panel Connector"@en ;
                   edo:hasAttribute edo:IsParkingPlace .


###  https://w3id.org/energy-domain/edo#PanelHydraulicConnector
edo:PanelHydraulicConnector rdf:type owl:Class ;
                            rdfs:subClassOf edo:PanelConnector ;
                            dcterms:identifier "PanelHydraulicConnector" ;
                            skos:definition "Conector hidráulico estacionário ou montado em painel."@pt-br ,
                                            "Stationary or panel-mounted hydraulic connector."@en ;
                            skos:prefLabel "Conector Hidráulico de Painel"@pt-br ,
                                           "Panel Hydraulic Connector"@en ;
                            edo:hasAttribute edo:MaxPressure .


###  https://w3id.org/energy-domain/edo#PartElement
edo:PartElement rdf:type owl:Class ;
                rdfs:subClassOf edo:DomainElement ;
                skos:definition "Representa um componente físico que não é individualmente rastreável, mas constitui parte essencial de um elemento maior, como conectores, juntas ou acessórios."@pt-br ,
                                "Represents a physical component that is not individually traceable but forms an essential part of a larger element, such as connectors, joints, or fittings."@en ;
                skos:prefLabel "Elemento Parte"@pt-br ,
                               "Part Element"@en .


###  https://w3id.org/energy-domain/edo#PartNumber
edo:PartNumber rdf:type owl:Class ;
               rdfs:subClassOf edo:DomainAttribute ;
               dcterms:accessRights "PUBLIC" ;
               dcterms:identifier "PartNumber" ;
               skos:definition "The Part Number is a unique identifier assigned to each type of element, ensuring consistency and ease of reference. This identifier helps in categorizing, ordering, and tracking the accessory within the system. When the drawing code is used consistently across all projects for a specific type of accessory, it can also serve as the Part Number, facilitating uniformity in documentation and usage."@en ;
               skos:prefLabel "Número da peça do acessório"@pt-br ,
                              "Part Number"@en ;
               edo:hasAttributeScope edo:TypeLevelAttribute ;
               edo:hasLifecycleCreationPhase edo:DetailedDesign ;
               edo:hasTypedValue edo:StringValue ;
               edo:hasValueCardinality edo:SingleValue .


###  https://w3id.org/energy-domain/edo#PerformanceAttribute
edo:PerformanceAttribute rdf:type owl:Class ;
                         rdfs:subClassOf edo:AttributeDomainCategory ;
                         rdfs:comment "Represents performance or capacity values such as pressure rating or power."@en ;
                         rdfs:label "Atributo de Desempenho"@pt-br ,
                                    "Performance Attribute"@en ;
                         skos:definition "Representa valores de desempenho ou capacidade como pressão nominal ou potência"@pt-br ,
                                         "Represents performance or capacity values such as pressure rating or power"@en .


###  https://w3id.org/energy-domain/edo#PermeabilityCurveAttribute
edo:PermeabilityCurveAttribute rdf:type owl:Class ;
                               rdfs:subClassOf edo:DomainAttribute ;
                               dcterms:accessRights "PUBLIC" ;
                               dcterms:identifier "PermeabilityTable" ;
                               skos:definition "Permeabilidade (Específica para Materiais Poliméricos)"@pt-br ,
                                               "Provides data on the permeability of various substances through materials, helping to assess the rate at which fluids or gases can pass through the structure. This information is crucial for evaluating material performance, ensuring compatibility, and predicting long-term behavior under operational conditions."@en ;
                               skos:prefLabel "Permeability Table"@en ,
                                              "Tabela de Permeabilidade"@pt-br ;
                               edo:hasAttributeScope edo:TypeLevelAttribute .


###  https://w3id.org/energy-domain/edo#PermeabilityTableColumn
edo:PermeabilityTableColumn rdf:type owl:Class ;
                            rdfs:subClassOf edo:PermeabilityCurveAttribute .


###  https://w3id.org/energy-domain/edo#PermeabilityTable_MoleculeIdentifier
edo:PermeabilityTable_MoleculeIdentifier rdf:type owl:Class ;
                                         rdfs:subClassOf edo:PermeabilityTableColumn ;
                                         dcterms:accessRights "PUBLIC" ;
                                         dcterms:identifier "PermeabilityTable_MoleculeIdentifier" ;
                                         skos:definition "Specifies the type of molecule. This property identifies the particular molecule involved, which is crucial for understanding the material's interaction with or response to different chemical substances."@en ,
                                                         "tipo de molécula (co2, h2s, ch4, h2o,…)"@pt-br ;
                                         skos:prefLabel "Identificador de Molécula"@pt-br ,
                                                        "Molecule Identifier"@en ;
                                         edo:hasAttributeScope edo:TypeLevelAttribute ;
                                         edo:hasLifecycleCreationPhase edo:DetailedDesign ;
                                         edo:hasTypedValue edo:StringValue ;
                                         edo:hasValueCardinality edo:MultiValue .


###  https://w3id.org/energy-domain/edo#PermeabilityTable_PermeabilityCoefficient
edo:PermeabilityTable_PermeabilityCoefficient rdf:type owl:Class ;
                                              rdfs:subClassOf edo:PermeabilityTableColumn ;
                                              dcterms:accessRights "PUBLIC" ;
                                              dcterms:identifier "PermeabilityTable_PermeabilityCoefficient" ;
                                              skos:definition "Represents the rate at which a substance, such as a gas or liquid, can pass through a material. This property is crucial for understanding the material's resistance to permeation, helping to assess its suitability for containing or isolating specific substances."@en ;
                                              skos:prefLabel "Coeficiente de Permeabilidade"@pt-br ,
                                                             "Permeability Coefficient"@en ;
                                              edo:hasAttributeScope edo:TypeLevelAttribute ;
                                              edo:hasLifecycleCreationPhase edo:DetailedDesign ;
                                              edo:hasTypedValue edo:FloatValue ;
                                              edo:hasUnit edo:MOL-PER-M-SEC-PA ;
                                              edo:hasValueCardinality edo:MultiValue .


###  https://w3id.org/energy-domain/edo#PermeabilityTable_PolymerState
edo:PermeabilityTable_PolymerState rdf:type owl:Class ;
                                   rdfs:subClassOf edo:PermeabilityTableColumn ;
                                   dcterms:accessRights "PUBLIC" ;
                                   dcterms:identifier "PermeabilityTable_PolymerState" ;
                                   skos:definition "(plastificado, não plastificado,…)"@pt-br ,
                                                   "The state of the polymeric material is specified.. This property is crucial for understanding how the material behaves under different conditions and its suitability for various applications."@en ;
                                   skos:prefLabel "Estado do Polímero"@pt-br ,
                                                  "Polymer State"@en ;
                                   edo:hasAttributeScope edo:TypeLevelAttribute ;
                                   edo:hasLifecycleCreationPhase edo:DetailedDesign ;
                                   edo:hasTypedValue edo:StringValue ;
                                   edo:hasValueCardinality edo:MultiValue .


###  https://w3id.org/energy-domain/edo#PermeabilityTable_Temperature
edo:PermeabilityTable_Temperature rdf:type owl:Class ;
                                  rdfs:subClassOf edo:PermeabilityTableColumn ;
                                  dcterms:accessRights "PUBLIC" ;
                                  dcterms:identifier "PermeabilityTable_Temperature" ;
                                  skos:definition "Represents the thermal condition or measurement of heat for a component or system. This property is important for assessing how the component performs or operates under specific thermal conditions, ensuring it remains within safe and effective operating limits."@en ;
                                  skos:prefLabel "Temperatura"@pt-br ,
                                                 "Temperature"@en ;
                                  edo:hasAttributeScope edo:TypeLevelAttribute ;
                                  edo:hasLifecycleCreationPhase edo:DetailedDesign ;
                                  edo:hasTypedValue edo:FloatValue ;
                                  edo:hasUnit unit:K ;
                                  edo:hasValueCardinality edo:MultiValue .


###  https://w3id.org/energy-domain/edo#Photovoltaic
edo:Photovoltaic rdf:type owl:Class ;
                 rdfs:subClassOf edo:Solar ;
                 dcterms:identifier "Photovoltaic" ;
                 skos:definition "Energia fotovoltaica é gerada pela conversão direta da luz solar em eletricidade usando materiais semicondutores como o silício. É uma das tecnologias renováveis de crescimento mais rápido, aplicável em escalas que variam de telhados residenciais a grandes usinas solares."@pt-br ,
                                 "Photovoltaic energy is generated by converting sunlight directly into electricity using semiconductor materials such as silicon. It is one of the fastest growing renewable technologies, applicable at scales ranging from rooftop panels to utility-scale solar farms."@en ;
                 skos:prefLabel "Fotovoltaica"@pt-br ,
                                "Photovoltaic"@en .


###  https://w3id.org/energy-domain/edo#PhysicalConnection
edo:PhysicalConnection rdf:type owl:Class ;
                       rdfs:subClassOf edo:ConsumableElement ;
                       dcterms:identifier "PhysicalConnection" ;
                       skos:definition "A Physical Connection refers to the actual link or interface between two or more components, such as pipes, equipment, or systems, that allows for the transfer of fluids, energy, or data."@en ,
                                       "Representa uma conexão entre dois ativos físicos"@pt-br ;
                       skos:prefLabel "Conexão Física"@pt-br ,
                                      "Physical Connection"@en .


###  https://w3id.org/energy-domain/edo#PhysicalPropertyAttribute
edo:PhysicalPropertyAttribute rdf:type owl:Class ;
                              rdfs:subClassOf edo:AttributeDomainCategory ;
                              rdfs:comment "Represents intrinsic physical properties such as mass, density, material."@en ;
                              rdfs:label "Atributo de Propriedade Física"@pt-br ,
                                         "Physical Property Attribute"@en ;
                              skos:definition "Representa propriedades físicas intrínsecas como massa, densidade, material"@pt-br ,
                                              "Represents intrinsic physical properties such as mass, density, material"@en .


###  https://w3id.org/energy-domain/edo#Piggable
edo:Piggable rdf:type owl:Class ;
             rdfs:subClassOf edo:DomainAttribute ;
             dcterms:accessRights "PUBLIC" ;
             dcterms:identifier "Piggable" ;
             skos:definition "Especifica se o equipamento possui pelo menos um circuito interno de escoamento que permita passagem de pig"@pt-br ,
                             "Whether equipment has at least one internal flow circuit allowing pig runs"@en ;
             skos:prefLabel "Piggable"@en ,
                            "Pigável"@pt-br ;
             edo:hasAttributeScope edo:TypeLevelAttribute ;
             edo:hasLifecycleCreationPhase edo:DetailedDesign ;
             edo:hasTypedValue edo:BooleanValue ;
             edo:hasValueCardinality edo:SingleValue .


###  https://w3id.org/energy-domain/edo#Pile
edo:Pile rdf:type owl:Class ;
         rdfs:subClassOf edo:Anchor ;
         dcterms:identifier "Pile" ;
         skos:prefLabel "Estaca"@pt-br ,
                        "Pile"@en .


###  https://w3id.org/energy-domain/edo#PipeMechanicalSupport
edo:PipeMechanicalSupport rdf:type owl:Class ;
                          rdfs:subClassOf edo:PipeSupport ;
                          dcterms:identifier "PipeMechanicalSupport" .


###  https://w3id.org/energy-domain/edo#PipeMountPosition
edo:PipeMountPosition rdf:type owl:Class ;
                      rdfs:subClassOf edo:DomainAttribute ;
                      dcterms:accessRights "PUBLIC" ;
                      dcterms:identifier "PipeMountPosition" ;
                      skos:definition "Cota em metros da posição em que o item é montado no tramo no sentido do fluxo do fluido."@pt-br ,
                                      "Indicates the distance from the end fitting to the position of the accessory along the direction of fluid flow within the pipe body. This property specifies the precise location of the accessory relative to the end fitting, which is essential for accurate installation and alignment within the tubular body."@en ;
                      skos:prefLabel "Pipe Mount Position"@en ,
                                     "Posição de Montagem no Duto"@pt-br ;
                      edo:hasAttributeScope edo:InstanceLevelAttribute ;
                      edo:hasLifecycleCreationPhase edo:DetailedDesign ;
                      edo:hasTypedValue edo:FloatValue ;
                      edo:hasUnit unit:M ;
                      edo:hasValueCardinality edo:SingleValue .


###  https://w3id.org/energy-domain/edo#PipePullingHead
edo:PipePullingHead rdf:type owl:Class ;
                    rdfs:subClassOf edo:IfcInstanciableElement ,
                                    edo:PullingHead ;
                    dcterms:identifier "PipePullingHead" ;
                    skos:altLabel "Cable Head"@en ,
                                  "Installation Head"@en ,
                                  "Pull Head"@en ,
                                  "Pulling Grip"@en ,
                                  "Pulling Tool"@en ;
                    skos:definition "A component used in subsea flexible pipe installations to provide a secure attachment point for pulling the pipe into position during installation or retrieval operations. The Pulling Head is fitted to the end of the flexible pipe, allowing connection to pulling equipment such as winches or cranes. It is designed to withstand high loads, ensuring that the pipe can be pulled safely without causing damage. The Pulling Head is essential for handling, testing, and securing the pipe in place during subsea installation."@en ,
                                    "Cabeça de tração tipo tampa, usada para dutos flexíveis etc."@pt-br ;
                    skos:prefLabel "Cabeça de Tração do Duto"@pt-br ,
                                   "Pipe Pulling Head"@en ;
                    edo:hasAttribute edo:FlangeType ,
                                     edo:PullingHeadType ,
                                     edo:RingGasketInnerDIameter ,
                                     edo:RingGasketMaterial ,
                                     edo:RingGasketOuterDiameter ,
                                     edo:RingGasketPressureRating ,
                                     edo:RingGasketSpecification ,
                                     edo:RingGasketStandard ,
                                     edo:RingGasketType ,
                                     edo:SafeWorkingLoad ;
                    edo:hasDiscipline edo:SubseaFlexiblePipesEngineering ;
                    edo:ifc_equivalentClass "IfcPipeFitting" ;
                    edo:ifc_objectType "PipePullingHead" ;
                    edo:ifc_predefinedType "USERDEFINED" .


###  https://w3id.org/energy-domain/edo#PipeSectionApplication
edo:PipeSectionApplication rdf:type owl:Class ;
                           rdfs:subClassOf edo:DomainAttribute ;
                           dcterms:accessRights "PUBLIC" ;
                           dcterms:identifier "PipeSectionApplication" ;
                           skos:definition "Aplicação do tramo, de acordo com as seguintes nomenclaturas: R (Riser); RT (seção de topo do riser); RI (seção intermediaria do riser); RF (seção de fundo do riser); F (Flowline)"@pt-br ,
                                           "Indicates the specific application of the flexible pipe section in the interconnection system, categorizing it based on its role or position within the riser or flowline."@en ;
                           skos:prefLabel "Aplicação do Tramo"@pt-br ,
                                          "Pipe Section Application"@en ;
                           edo:hasAttributeScope edo:InstanceLevelAttribute ;
                           edo:hasLifecycleCreationPhase edo:DetailedDesign ;
                           edo:hasTypedValue edo:StringValue ;
                           edo:hasValueCardinality edo:SingleValue .


###  https://w3id.org/energy-domain/edo#PipeSegment
edo:PipeSegment rdf:type owl:Class ;
                rdfs:subClassOf edo:TransportLineSegment ;
                dcterms:identifier "PipeSegment" ;
                skos:definition "Pipeline segment for movement/flow of fluids."@en ,
                                "Segmento de Duto"@pt-br ;
                skos:prefLabel "Pipe Segment"@en ,
                               "Segmento de Duto"@pt-br .


###  https://w3id.org/energy-domain/edo#PipeSupport
edo:PipeSupport rdf:type owl:Class ;
                rdfs:subClassOf edo:Structure ;
                dcterms:identifier "PipeSupport" .


###  https://w3id.org/energy-domain/edo#PipeTermination
edo:PipeTermination rdf:type owl:Class ;
                    rdfs:subClassOf edo:LineTermination ;
                    dcterms:identifier "PipeTermination" ;
                    skos:definition "The Pipe Termination refers to the components at the end of a pipeline that provide the final connection to other equipment or systems. These terminations are crucial for ensuring a secure and reliable interface between the pipeline and surrounding infrastructure, allowing for the proper transfer of fluids or gases and maintaining the integrity of the overall system."@en ;
                    skos:prefLabel "Pipe Termination"@en ,
                                   "Terminador de Duto"@pt-br .


###  https://w3id.org/energy-domain/edo#PipelineSpan
edo:PipelineSpan rdf:type owl:Class ;
                 rdfs:subClassOf edo:LineSpan ;
                 dcterms:identifier "PipelineSpan" ;
                 skos:definition "Local que representa um duto de escoamento de fluidos completo"@pt-br ,
                                 "Location representing a complete pipeline for fluid transport"@en ;
                 skos:prefLabel "Pipeline span"@en ,
                                "Trecho de duto"@pt-br .


###  https://w3id.org/energy-domain/edo#PipingSpool
edo:PipingSpool rdf:type owl:Class ;
                rdfs:subClassOf edo:PressureComponent ;
                dcterms:identifier "PipingSpool" ;
                skos:definition "Piping section internal to some equipment"@en ,
                                "Trecho de tubulação interno a um equipamento"@pt-br ;
                skos:prefLabel "Piping spool"@en ,
                               "Trecho de tubulação"@pt-br .


###  https://w3id.org/energy-domain/edo#PitchToleranceClass
edo:PitchToleranceClass rdf:type owl:Class ;
                        rdfs:subClassOf edo:DomainAttribute ;
                        dcterms:accessRights "PUBLIC" ;
                        dcterms:identifier "PitchToleranceClass" ;
                        skos:definition "A classification defining the acceptable deviation range for the pitch measurement, ensuring consistency in the helical arrangement of wires or threads."@en ;
                        skos:prefLabel "Classe de Tolerância de Passo"@pt-br ,
                                       "Pitch Tolerance Class"@en ;
                        edo:hasAttributeScope edo:InstanceLevelAttribute ;
                        edo:hasLifecycleCreationPhase edo:DetailedDesign ;
                        edo:hasTypedValue edo:StringValue ;
                        edo:hasValueCardinality edo:SingleValue .


###  https://w3id.org/energy-domain/edo#Planned_Start_Timestamp
edo:Planned_Start_Timestamp rdf:type owl:Class ;
                            rdfs:subClassOf edo:DomainAttribute ;
                            dcterms:accessRights "PUBLIC" ;
                            dcterms:identifier "Planned_Start_Timestamp" ;
                            skos:prefLabel "Planned Start Timestamp"@en ;
                            edo:hasAttributeScope edo:InstanceLevelAttribute ;
                            edo:hasTypedValue edo:DateTimeValue ;
                            edo:hasValueCardinality edo:SingleValue .


###  https://w3id.org/energy-domain/edo#PlasticHose
edo:PlasticHose rdf:type owl:Class ;
                rdfs:subClassOf edo:IfcInstanciableElement ,
                                edo:Tubing ;
                dcterms:identifier "PlasticHose" ;
                skos:definition "Representa uma mangueira plástica utilizada em tubulações para transporte de fluido, tipicamente flexível e leve."@pt-br ,
                                "Represents a plastic hose used within tubing for fluid transport, typically flexible and lightweight."@en ;
                skos:prefLabel "Mangueira Plástica"@pt-br ,
                               "Mangueira plástica"@pt-br ,
                               "Plastic Hose"@en ;
                edo:hasDiscipline edo:SubseaUmbilicalsEngineering ;
                edo:ifc_equivalentClass "IfcPipeSegment" ;
                edo:ifc_objectType "PlasticHose" ;
                edo:ifc_predefinedType "USERDEFINED" .


###  https://w3id.org/energy-domain/edo#PointLocation
edo:PointLocation rdf:type owl:Class ;
                  rdfs:subClassOf edo:PartElement ;
                  dcterms:identifier "PointLocation" ;
                  skos:definition "Base para todos os locais que podem ser convencionalmente situados em um único ponto geográfico"@pt-br ,
                                  "Basis for all locations that can conventionally be situated at a single geographic point."@en ;
                  skos:prefLabel "Localização de Ponto"@pt-br ,
                                 "Point Location"@en .


###  https://w3id.org/energy-domain/edo#PoissonRatioAt23Degrees
edo:PoissonRatioAt23Degrees rdf:type owl:Class ;
                            rdfs:subClassOf edo:DomainAttribute ;
                            dcterms:accessRights "PUBLIC" ;
                            dcterms:identifier "PoissonRatioAt23Degrees" ;
                            skos:definition "Coeficiente de Poisson a 23 graus Celsius (Específica para Materiais Metálicos e Poliméricos)"@pt-br ,
                                            "Indicates Poisson's ratio of the material at 23 degrees Celsius, representing the ratio of transverse strain to axial strain when the material is subjected to stress. This property is essential for understanding the material's deformation behavior under load and its response to mechanical forces in subsea environments."@en ;
                            skos:prefLabel "Coeficiente de Poisson a 23 Graus Celsius"@pt-br ,
                                           "Poisson Ratio At 23 Degrees"@en ;
                            edo:hasAttributeScope edo:TypeLevelAttribute ;
                            edo:hasLifecycleCreationPhase edo:DetailedDesign ;
                            edo:hasTypedValue edo:FloatValue ;
                            edo:hasValueCardinality edo:SingleValue .


###  https://w3id.org/energy-domain/edo#PolymericLayerMaterialType
edo:PolymericLayerMaterialType rdf:type owl:Class ;
                               rdfs:subClassOf edo:DomainAttribute ;
                               dcterms:accessRights "PUBLIC" ;
                               dcterms:identifier "PolymericLayerMaterialType" ;
                               skos:definition "Type of material from which an object is made, allowing for precise documentation and categorisation."@en ;
                               skos:prefLabel "Polymeric Layer Material Type"@en ,
                                              "Tipo de Material da Camada Polimérica"@pt-br ;
                               edo:hasAttributeScope edo:TypeLevelAttribute ;
                               edo:hasLifecycleCreationPhase edo:DetailedDesign ;
                               edo:hasTypedValue edo:StringValue ;
                               edo:hasValueCardinality edo:SingleValue .


###  https://w3id.org/energy-domain/edo#PolymericMaterial
edo:PolymericMaterial rdf:type owl:Class ;
                      rdfs:subClassOf edo:FlexibleStructureLayerMaterial ,
                                      edo:IfcInstanciableElement ;
                      dcterms:identifier "PolymericMaterial" ;
                      skos:definition "Material made from polymers, used to fabricate flexible layers in subsea flexible pipes. Polymeric Material is selected for its properties such as flexibility, chemical resistance, and durability, making it suitable for withstanding the harsh conditions of subsea environments. These materials are commonly used in layers that provide insulation, protection, or pressure containment, ensuring the overall performance and integrity of the flexible pipe under dynamic loads and extreme underwater conditions."@en ;
                      skos:prefLabel "Material Polimérico"@pt-br ,
                                     "Polymeric Material"@en ;
                      edo:hasAttribute edo:DiffusionTableColumn ,
                                       edo:EModVsTempTableColumn ,
                                       edo:MaxPermissibleDeformationDynamic ,
                                       edo:MaxPermissibleDeformationStatic ,
                                       edo:MinimumTemperature ,
                                       edo:PermeabilityTableColumn ,
                                       edo:PolymericLayerMaterialType ,
                                       edo:SolubilityTableColumn ;
                      edo:hasDiscipline edo:SubseaFlexiblePipesEngineering ,
                                        edo:SubseaUmbilicalsEngineering ;
                      edo:ifc_equivalentClass "IfcMaterial" ;
                      edo:ifc_objectType "PolymericMaterial" .


###  https://w3id.org/energy-domain/edo#Port
edo:Port rdf:type owl:Class ;
         rdfs:subClassOf edo:LogicalElement ;
         skos:definition "Representa um ponto de interface através do qual um elemento pode trocar dados, energia ou fluidos."@pt-br ,
                         "Represents an interface point through which an element can exchange data, energy, or fluids."@en ;
         skos:prefLabel "Port"@en ,
                        "Porta"@pt-br .


###  https://w3id.org/energy-domain/edo#PostSlippingBendingStiffness
edo:PostSlippingBendingStiffness rdf:type owl:Class ;
                                 rdfs:subClassOf edo:BendingStiffnessCurveAttribute ;
                                 dcterms:accessRights "PUBLIC" ;
                                 dcterms:identifier "PostSlippingBendingStiffness" ;
                                 skos:definition "Represents the stiffness of a component after slipping occurs during bending. This property is important for evaluating the structural response and stability of the component once it has experienced slippage, ensuring that it can still withstand bending loads without significant deformation."@en ;
                                 skos:prefLabel "Post Slipping Bending Stiffness"@en ,
                                                "Rigidez de Flexão Pós-Escorregamento"@pt-br ;
                                 edo:hasAttributeScope edo:TypeLevelAttribute ;
                                 edo:hasLifecycleCreationPhase edo:DetailedDesign ;
                                 edo:hasTypedValue edo:FloatValue ;
                                 edo:hasUnit unit:N-M2 ;
                                 edo:hasValueCardinality edo:SingleValue .


###  https://w3id.org/energy-domain/edo#PowerMachine
edo:PowerMachine rdf:type owl:Class ;
                 rdfs:subClassOf edo:PressureComponent ;
                 dcterms:identifier "PowerMachine" ;
                 skos:definition "Machine that consumes externally-supplied power in order to execute mechanical work"@en ,
                                 "Máquina que consome potência fornecida externamente para realização de trabalho mecânico"@pt-br ;
                 skos:prefLabel "Máquina de potência"@pt-br ,
                                "Power machine"@en .


###  https://w3id.org/energy-domain/edo#PowerRating
edo:PowerRating rdf:type owl:Class ;
                rdfs:subClassOf edo:DomainAttribute ;
                dcterms:accessRights "PUBLIC" ;
                dcterms:identifier "PowerRating" ;
                skos:prefLabel "Potência nominal"@pt-br ,
                               "Power rating"@en ;
                edo:hasAttributeScope edo:TypeLevelAttribute ;
                edo:hasLifecycleCreationPhase edo:DetailedDesign ;
                edo:hasTypedValue edo:FloatValue ;
                edo:hasValueCardinality edo:SingleValue .


###  https://w3id.org/energy-domain/edo#PreCommissioning
edo:PreCommissioning rdf:type owl:Class ;
                     rdfs:subClassOf edo:ConstructionPhase ;
                     rdfs:label "Pre-Commissioning"@en ,
                                "Pré-Comissionamento"@pt-br ;
                     skos:definition "Verification and functional testing before introducing operational fluids or energy."@en ,
                                     "Verificação e testes funcionais antes da introdução de fluidos ou energia operacionais."@pt-br .


###  https://w3id.org/energy-domain/edo#PreSlippingBendingStiffness
edo:PreSlippingBendingStiffness rdf:type owl:Class ;
                                rdfs:subClassOf edo:BendingStiffnessCurveAttribute ;
                                dcterms:accessRights "PUBLIC" ;
                                dcterms:identifier "PreSlippingBendingStiffness" ;
                                skos:definition "Represents the stiffness of a component before any slipping occurs during bending. This property is important for assessing how the component resists bending forces prior to slippage, ensuring that it maintains its shape and performance under load."@en ;
                                skos:prefLabel "Pre Slipping Bending Stiffness"@en ,
                                               "Rigidez de Flexão Pré-Escorregamento"@pt-br ;
                                edo:hasAttributeScope edo:TypeLevelAttribute ;
                                edo:hasLifecycleCreationPhase edo:DetailedDesign ;
                                edo:hasTypedValue edo:FloatValue ;
                                edo:hasUnit unit:N-M2 ;
                                edo:hasValueCardinality edo:SingleValue .


###  https://w3id.org/energy-domain/edo#PressureArmour
edo:PressureArmour rdf:type owl:Class ;
                   rdfs:subClassOf edo:CarcassLayer ,
                                   edo:IfcInstanciableElement ;
                   dcterms:identifier "PressureArmour" ;
                   skos:definition "A high-strength, metallic layer used in subsea flexible pipes to provide resistance against both internal and external pressure. The Pressure Armour prevents the pipe from expanding under high internal pressures and protects against collapse due to external pressure. Typically made from helically wound steel or other strong materials, it supports the pipe's structural integrity and ensures reliable operation in harsh subsea environments."@en ;
                   skos:prefLabel "Armadura de Pressão"@pt-br ,
                                  "Pressure Armour"@en ;
                   edo:hasDiscipline edo:SubseaFlexiblePipesEngineering ;
                   edo:ifc_equivalentClass "IfcPipeSegment" ;
                   edo:ifc_objectType "PressureArmour" ;
                   edo:ifc_predefinedType "USERDEFINED" .


###  https://w3id.org/energy-domain/edo#PressureComponent
edo:PressureComponent rdf:type owl:Class ;
                      rdfs:subClassOf edo:ComponentDevice ;
                      dcterms:identifier "PressureComponent" ;
                      skos:prefLabel "Component de contenção de pressão"@pt-br ,
                                     "Pressure-containing component"@en ;
                      edo:hasAttribute edo:MaxPressure .


###  https://w3id.org/energy-domain/edo#PressureEquipment
edo:PressureEquipment rdf:type owl:Class ;
                      rdfs:subClassOf edo:ActuatedEquipment ;
                      dcterms:identifier "PressureEquipment" ;
                      skos:definition "Equipamentos cuja função principal envolve contenção de fluidos, ainda que não destinados a instalação permanente"@pt-br ,
                                      "Equipment whose main function involves fluid containment, even if not meant for permanent installation"@en ;
                      skos:prefLabel "Equipamentos de contenção de pressão"@pt-br ,
                                     "Pressure-containing equipment"@en .


###  https://w3id.org/energy-domain/edo#PressureSensor
edo:PressureSensor rdf:type owl:Class ;
                   rdfs:subClassOf edo:Sensor ;
                   dcterms:identifier "PressureSensor" ;
                   skos:prefLabel "Pressure sensor"@en ,
                                  "Sensor de pressão"@pt-br .


###  https://w3id.org/energy-domain/edo#ProcessEngineering
edo:ProcessEngineering rdf:type owl:Class ;
                       rdfs:subClassOf edo:TechnicalDiscipline ;
                       rdfs:label "Engenharia de Processos"@pt-br ,
                                  "Process Engineering"@en ;
                       skos:definition "Disciplina de engenharia focada no projeto e otimização de processos industriais."@pt-br ,
                                       "Engineering discipline focused on the design and optimization of industrial processes."@en .


###  https://w3id.org/energy-domain/edo#ProcessPipeSpec
edo:ProcessPipeSpec rdf:type owl:Class ;
                    rdfs:subClassOf edo:Specification ;
                    skos:definition "Representa a especificação para tubulação de processo, incluindo materiais, classes de pressão, dimensões e normas para processos industriais."@pt-br ,
                                    "Represents the specification for process pipes, including materials, pressure ratings, dimensions, and standards for industrial processes."@en ;
                    skos:prefLabel "Especificação de Tubo de Processo"@pt-br ,
                                   "Process Pipe Specification"@en .


###  https://w3id.org/energy-domain/edo#ProcessPipingEngineering
edo:ProcessPipingEngineering rdf:type owl:Class ;
                             rdfs:subClassOf edo:TechnicalDiscipline ;
                             rdfs:label "Engenharia de Tubulação de Processo"@pt-br ,
                                        "Process Piping Engineering"@en ;
                             skos:definition "Disciplina de engenharia focada no projeto de sistemas de tubulação para fluidos de processo."@pt-br ,
                                             "Engineering discipline focused on the design of piping systems for process fluids."@en .


###  https://w3id.org/energy-domain/edo#ProcessingModule
edo:ProcessingModule rdf:type owl:Class ;
                     rdfs:subClassOf edo:FlowControlModule ;
                     dcterms:identifier "ProcessingModule" ;
                     skos:definition "Module installed as part of some larger equipment and designed to produce physical or chemical changes upon fluids"@en ,
                                     "Módulo instalado como parte de um equipamento maior e projetado para produzir mudanças físicas ou químicas sobre fluidos"@pt-br ;
                     skos:prefLabel "Módulo de processamento"@pt-br ,
                                    "Processing module"@en .


###  https://w3id.org/energy-domain/edo#Procurement
edo:Procurement rdf:type owl:Class ;
                rdfs:subClassOf edo:ConstructionPhase ;
                rdfs:label "Aquisição"@pt-br ,
                           "Procurement"@en ;
                skos:definition "Acquisition of materials, equipment, and services required for project execution."@en ,
                                "Aquisição de materiais, equipamentos e serviços necessários para execução do projeto."@pt-br .


###  https://w3id.org/energy-domain/edo#Project
edo:Project rdf:type owl:Class ;
            rdfs:subClassOf edo:Location ;
            dcterms:identifier "Project" ;
            skos:definition "A broad concept that encompasses the design, development, and planning of various components or systems."@en ;
            skos:prefLabel "Project"@en ,
                           "Projeto"@pt-br ;
            edo:hasDiscipline edo:SubseaUmbilicalsEngineering ;
            edo:ifc_equivalentClass "IfcProject" .


###  https://w3id.org/energy-domain/edo#ProjectAcronym
edo:ProjectAcronym rdf:type owl:Class ;
                   rdfs:subClassOf edo:DomainAttribute ;
                   dcterms:accessRights "PUBLIC" ;
                   dcterms:identifier "ProjectAcronym" ;
                   skos:definition "Abreviação do nome do projeto da Interligação Submarina. Ex., 'SEP' para o \"FPSO Carioca do campo de Sépia\""@pt-br ,
                                   "Indicates the unique identification code assigned to the operator's project. This property is used for tracking, managing, and referencing the project throughout all phases of its lifecycle, ensuring proper identification and organization."@en ;
                   skos:prefLabel "Abreviação do Nome do Projeto da Interligação Submarina"@pt-br ,
                                  "Project Acronym"@en ;
                   edo:hasAttributeScope edo:InstanceLevelAttribute ;
                   edo:hasLifecycleCreationPhase edo:BasicDesign ;
                   edo:hasTypedValue edo:StringValue ;
                   edo:hasValueCardinality edo:SingleValue .


###  https://w3id.org/energy-domain/edo#ProjectCode
edo:ProjectCode rdf:type owl:Class ;
                rdfs:subClassOf edo:DomainAttribute ;
                dcterms:accessRights "PUBLIC" ;
                dcterms:identifier "ProjectCode" ;
                skos:definition "Unique identification code assigned to the operator's project, used for tracking, managing, and referencing the project across all phases of its lifecycle."@en ;
                skos:prefLabel "Código Identificador único do projeto da operadora da Interligação Submarina"@pt-br ,
                               "Project Code"@en ;
                edo:hasAttributeScope edo:InstanceLevelAttribute ;
                edo:hasLifecycleCreationPhase edo:BasicDesign ;
                edo:hasTypedValue edo:StringValue ;
                edo:hasValueCardinality edo:SingleValue .


###  https://w3id.org/energy-domain/edo#ProjectDrawingCode
edo:ProjectDrawingCode rdf:type owl:Class ;
                       rdfs:subClassOf edo:DomainAttribute ;
                       dcterms:accessRights "PUBLIC" ;
                       dcterms:identifier "ProjectDrawingCode" ;
                       skos:definition "Indicates the unique alphanumeric code assigned to the project drawing. This property is used to reference and locate the specific drawing associated with the item, providing a clear and organized method for tracking and accessing drawing documents."@en ,
                                       "Número do desenho do projeto do acessório"@pt-br ;
                       skos:prefLabel "Número do Desenho do Projeto"@pt-br ,
                                      "Project Drawing Code"@en ;
                       edo:hasAttributeScope edo:TypeLevelAttribute ;
                       edo:hasLifecycleCreationPhase edo:DetailedDesign ;
                       edo:hasTypedValue edo:StringValue ;
                       edo:hasValueCardinality edo:SingleValue .


###  https://w3id.org/energy-domain/edo#ProjectDrawingRevision
edo:ProjectDrawingRevision rdf:type owl:Class ;
                           rdfs:subClassOf edo:DomainAttribute ;
                           dcterms:accessRights "PUBLIC" ;
                           dcterms:identifier "ProjectDrawingRevision" ;
                           skos:definition "Indicates the revision number or identifier of the project drawing. This property tracks the version of the drawing, providing essential information for identifying updates, changes, and the most current version of the drawing related to the item."@en ;
                           skos:prefLabel "Project Drawing Revision"@en ,
                                          "Revisão do Desenho do Projeto"@pt-br ;
                           edo:hasAttributeScope edo:TypeLevelAttribute ;
                           edo:hasLifecycleCreationPhase edo:DetailedDesign ;
                           edo:hasTypedValue edo:StringValue ;
                           edo:hasValueCardinality edo:SingleValue .


###  https://w3id.org/energy-domain/edo#ProtectiveSheath
edo:ProtectiveSheath rdf:type owl:Class ;
                     rdfs:subClassOf edo:IfcInstanciableElement ,
                                     edo:SolidLayer ;
                     dcterms:identifier "ProtectiveSheath" ;
                     skos:altLabel "Outer Sheath" ;
                     skos:definition "A layer in subsea flexible pipes designed to shield internal components from external environmental factors such as abrasion, mechanical damage, or chemical exposure. The Protective Sheath serves as the outermost barrier, providing defense against harsh subsea conditions while preserving the integrity of the underlying layers. Typically made from durable polymeric materials, it plays a critical role in extending the lifespan of the flexible pipe by protecting it from physical and chemical wear."@en ;
                     skos:prefLabel "Capa de Proteção"@pt-br ,
                                    "Protective Sheath"@en ;
                     edo:hasDiscipline edo:SubseaFlexiblePipesEngineering ,
                                       edo:SubseaUmbilicalsEngineering ;
                     edo:ifc_equivalentClass "IfcPipeSegment" ;
                     edo:ifc_objectType "ProtectiveSheath" ;
                     edo:ifc_predefinedType "USERDEFINED" .


###  https://w3id.org/energy-domain/edo#ProvenanceAttribute
edo:ProvenanceAttribute rdf:type owl:Class ;
                        rdfs:subClassOf edo:AdministrativeAttribute .


###  https://w3id.org/energy-domain/edo#PullInCollar
edo:PullInCollar rdf:type owl:Class ;
                 rdfs:subClassOf edo:IfcInstanciableElement ,
                                 edo:SplitCollar ;
                 dcterms:identifier "PullInCollar" ;
                 skos:altLabel "Installation Collar"@en ,
                               "Pull-In Clamp"@en ,
                               "Pulling Collar"@en ,
                               "Tension Collar"@en ;
                 skos:definition "A device used in subsea operations to assist in the installation of flexible pipes or risers by providing a secure attachment point for pulling the pipe into position. The Pull-In Collar is typically installed around the pipe and serves as a handling point for pulling equipment during installation. It ensures a controlled and secure method of pulling the pipe into place, preventing damage to the pipe while facilitating smooth and efficient installation in subsea environments."@en ;
                 skos:prefLabel "Colar de Pull-In"@pt-br ,
                                "Pull-In Collar"@en ;
                 edo:hasAttribute edo:WireRopeQuantity ,
                                  edo:WireRopeSlingDiameter ,
                                  edo:WireRopeSlingLength ;
                 edo:hasDiscipline edo:SubseaFlexiblePipesEngineering ,
                                   edo:SubseaUmbilicalsEngineering ;
                 edo:ifc_equivalentClass "IfcPipeFitting" ;
                 edo:ifc_objectType "PullInCollar" ;
                 edo:ifc_predefinedType "USERDEFINED" .


###  https://w3id.org/energy-domain/edo#PullingHead
edo:PullingHead rdf:type owl:Class ;
                rdfs:subClassOf edo:LineAncillary ;
                dcterms:identifier "PullingHead" ;
                skos:altLabel "Cable Head"@en ,
                              "Installation Head"@en ,
                              "Pulling Grip"@en ,
                              "Pulling Tool"@en ;
                skos:definition "A component used in subsea flexible pipe installations to provide a secure attachment point for pulling the pipe into position during installation or retrieval operations. The Pulling Head is fitted to the end of the flexible pipe, allowing connection to pulling equipment such as winches or cranes. It is designed to withstand high loads, ensuring that the pipe can be pulled safely without causing damage. The Pulling Head is essential for handling, testing, and securing the pipe in place during subsea installation."@en ;
                skos:prefLabel "Cabeça de Tração"@pt-br ,
                               "Pulling Head"@en ;
                edo:hasAttribute edo:SafeWorkingLoad ,
                                 edo:WeightInWater .


###  https://w3id.org/energy-domain/edo#PullingHeadType
edo:PullingHeadType rdf:type owl:Class ;
                    rdfs:subClassOf edo:DomainAttribute ;
                    dcterms:accessRights "PUBLIC" ;
                    dcterms:identifier "PullingHeadType" ;
                    skos:definition "Specifies the type of pulling head used for the installation or retrieval of subsea flexible structures. It describes the design and functionality of the pulling head, including details such as compatibility with specific installation methods, mechanical connections, and any special features or adaptations for handling loads during pulling operations. This property helps to ensure the correct pulling head is selected based on the requirements of the project and the conditions of the installation site."@en ;
                    skos:prefLabel "Pulling Head Type"@en ,
                                   "Tipo de Cabeça de Tração"@pt-br ;
                    edo:hasAttributeScope edo:TypeLevelAttribute ;
                    edo:hasLifecycleCreationPhase edo:DetailedDesign ;
                    edo:hasTypedValue edo:StringValue ;
                    edo:hasValueCardinality edo:SingleValue .


###  https://w3id.org/energy-domain/edo#Pump
edo:Pump rdf:type owl:Class ;
         rdfs:subClassOf edo:RotatingMachine ;
         dcterms:identifier "Pump" ;
         skos:prefLabel "Bomba"@pt-br ,
                        "Pump"@en .


###  https://w3id.org/energy-domain/edo#PumpedStorage
edo:PumpedStorage rdf:type owl:Class ;
                  rdfs:subClassOf edo:Hydropower ;
                  dcterms:identifier "PumpedStorage" ;
                  skos:definition "Hidrelétricas de bombeamento armazenam energia ao bombear água de um reservatório inferior para um superior em períodos de baixa demanda, liberando-a através de turbinas para gerar eletricidade em períodos de pico. Funcionam como um sistema de armazenamento de energia em larga escala."@pt-br ,
                                  "Pumped storage hydropower stores energy by pumping water from a lower reservoir to a higher one during low demand, and releasing it through turbines to generate electricity during peak demand. It acts as a large-scale energy storage system."@en ;
                  skos:prefLabel "Hidrelétrica de Bombeamento"@pt-br ,
                                 "Pumped Storage"@en .


###  https://w3id.org/energy-domain/edo#PumpingModule
edo:PumpingModule rdf:type owl:Class ;
                  rdfs:subClassOf edo:ProcessingModule ;
                  dcterms:identifier "PumpingModule" ;
                  skos:definition "Fluid pumping module installed as part of some larger equipment"@en ,
                                  "Módulo com função de bombeamento de fluidos instalado como parte de um equipamento maior"@pt-br ;
                  skos:prefLabel "Módulo de bombeamento"@pt-br ,
                                 "Pumping module"@en .


###  https://w3id.org/energy-domain/edo#Quantity
edo:Quantity rdf:type owl:Class ;
             rdfs:subClassOf edo:DomainAttribute ;
             dcterms:accessRights "PUBLIC" ;
             dcterms:identifier "Quantity" ;
             skos:definition "Quantity of items."@en ;
             skos:prefLabel "Quantidade de Itens"@pt-br ,
                            "Quantity"@en ;
             edo:hasAttributeScope edo:InstanceLevelAttribute ;
             edo:hasLifecycleCreationPhase edo:DetailedDesign ;
             edo:hasTypedValue edo:IntValue ;
             edo:hasValueCardinality edo:SingleValue .


###  https://w3id.org/energy-domain/edo#QuickConnectCoupling
edo:QuickConnectCoupling rdf:type owl:Class ;
                         rdfs:subClassOf edo:TubingCoupling ;
                         dcterms:identifier "QuickConnectCoupling" ;
                         skos:definition "Acoplamento de engate rápido utilizado para conectar ou desconectar linhas de fluido ou gás de forma prática e segura, garantindo vedação e minimizando vazamentos durante a operação."@pt-br ,
                                         "Quick connect coupling used to connect or disconnect fluid or gas lines in a practical and safe way, ensuring sealing and minimising leakage during operation."@en ;
                         skos:prefLabel "Engate Rápido"@pt-br ,
                                        "Quick Connect Coupling"@en ;
                         edo:hasAttribute edo:HoseFittingSpecTableColumn ,
                                          edo:StandardType ;
                         edo:hasDiscipline edo:SubseaUmbilicalsEngineering ;
                         edo:ifc_equivalentClass "IfcPipeFitting" ;
                         edo:ifc_objectType "QuickConnectCoupling" .


###  https://w3id.org/energy-domain/edo#QuickDisconnectionTool
edo:QuickDisconnectionTool rdf:type owl:Class ;
                           rdfs:subClassOf edo:RunningTool ;
                           dcterms:identifier "QuickDisconnectionTool" ;
                           skos:prefLabel "Ferramenta de desconexão rápida"@pt-br ,
                                          "Quick disconnection tool"@en .


###  https://w3id.org/energy-domain/edo#ROVTool
edo:ROVTool rdf:type owl:Class ;
            rdfs:subClassOf edo:Accessory ;
            dcterms:identifier "ROVTool" ;
            skos:definition "Ferramentas submarinas operadas por ROV para funções de instalação, destravamento, atuação, override, etc."@pt-br ,
                            "ROV-operated subsea tools for installation, release, actuation, override, etc. functions"@en ;
            skos:prefLabel "Ferramenta de ROV"@pt-br ,
                           "ROV tool"@en .


###  https://w3id.org/energy-domain/edo#RearPoint
edo:RearPoint rdf:type owl:Class ;
              rdfs:subClassOf edo:IfcInstanciableElement ,
                              edo:SupportRegion ;
              dcterms:identifier "RearPoint" ;
              skos:definition "A parte traseira do componente pode ser utilizada para travar o elemento durante a instalação, garantindo que ele permaneça firmemente no lugar durante o processo. O Ponto Traseiro fornece uma referência na parte posterior ao longo da linha de centro do componente, facilitando o alinhamento e o posicionamento precisos necessários para uma instalação adequada."@pt-br ,
                              "The rear part of the component can be used to secure the element during installation, ensuring it remains firmly in place throughout the process. The Rear Point provides a reference on the rear part along the component's centre line, facilitating precise alignment and positioning required for proper installation."@en ;
              skos:prefLabel "Ponto Traseiro"@pt-br ,
                             "Rear Point"@en ;
              edo:hasDiscipline edo:SubseaFlexiblePipesEngineering ,
                                edo:SubseaUmbilicalsEngineering ;
              edo:ifc_equivalentClass "IfcDistributionPort" ;
              edo:ifc_objectType "RearPoint" ;
              edo:ifc_predefinedType "USERDEFINED" .


###  https://w3id.org/energy-domain/edo#Recycling
edo:Recycling rdf:type owl:Class ;
              rdfs:subClassOf edo:DecommissioningPhase ;
              rdfs:label "Reciclagem"@pt-br ,
                         "Recycling"@en ;
              skos:definition "Processamento e reutilização de materiais recuperados durante o descomissionamento."@pt-br ,
                              "Processing and reusing materials recovered during decommissioning."@en .


###  https://w3id.org/energy-domain/edo#ReferenceDocument
edo:ReferenceDocument rdf:type owl:Class ;
                      rdfs:subClassOf edo:ExternalReference ;
                      skos:definition "Representa um documento ou publicação que serve como fonte de informação, diretrizes ou normas, fornecendo contexto e apoiando a tomada de decisão dentro de um projeto ou sistema."@pt-br ,
                                      "Represents a document or publication that serves as a source of information, guidelines, or standards, providing context and supporting decision-making within a project or system."@en ;
                      skos:prefLabel "Documento de Referência"@pt-br ,
                                     "Reference Document"@en .


###  https://w3id.org/energy-domain/edo#ReinforcementLength
edo:ReinforcementLength rdf:type owl:Class ;
                        rdfs:subClassOf edo:DomainAttribute ;
                        dcterms:accessRights "PUBLIC" ;
                        dcterms:identifier "ReinforcementLength" ;
                        skos:definition "Comprimento da seção de reforço em torno da linha"@pt-br ,
                                        "Length of reinforcement section around the line"@en ;
                        skos:prefLabel "Comprimento do reforço"@pt-br ,
                                       "Reinforcement length"@en ;
                        edo:hasAttributeScope edo:TypeLevelAttribute ;
                        edo:hasLifecycleCreationPhase edo:DetailedDesign ;
                        edo:hasTypedValue edo:FloatValue ;
                        edo:hasUnit unit:MilliM ;
                        edo:hasValueCardinality edo:SingleValue .


###  https://w3id.org/energy-domain/edo#ReinforcementOuterDiameter
edo:ReinforcementOuterDiameter rdf:type owl:Class ;
                               rdfs:subClassOf edo:DomainAttribute ;
                               dcterms:accessRights "PUBLIC" ;
                               dcterms:identifier "ReinforcementOuterDiameter" ;
                               skos:definition "Maximum outer diameter of reinforcement section around the line"@en ,
                                               "Máximo diâmetro externo da seção de reforço em torno da linha"@pt-br ;
                               skos:prefLabel "Diâmetro externo do reforço"@pt-br ,
                                              "Reinforcement outer diameter"@en ;
                               edo:hasAttributeScope edo:TypeLevelAttribute ;
                               edo:hasLifecycleCreationPhase edo:DetailedDesign ;
                               edo:hasTypedValue edo:FloatValue ;
                               edo:hasUnit unit:MilliM ;
                               edo:hasValueCardinality edo:SingleValue .


###  https://w3id.org/energy-domain/edo#ReliefValve
edo:ReliefValve rdf:type owl:Class ;
                rdfs:subClassOf edo:CheckValve ;
                dcterms:identifier "ReliefValve" ;
                skos:definition "Automatic pressure relief valve"@en ,
                                "Válvula automática de alívio de pressão"@pt-br ;
                skos:prefLabel "Relief valve"@en ,
                               "Válvula de alívio"@pt-br .


###  https://w3id.org/energy-domain/edo#Renewable
edo:Renewable rdf:type owl:Class ;
              rdfs:subClassOf edo:Domain ;
              rdfs:label "Energia Renovável"@pt-br ,
                         "Renewable Energy"@en ;
              skos:definition "Domínio industrial que abrange fontes de energia que são naturalmente reabastecidas, como solar, eólica e hidrelétrica."@pt-br ,
                              "Industrial domain covering energy sources that are naturally replenished, such as solar, wind, and hydropower."@en .


###  https://w3id.org/energy-domain/edo#Reused
edo:Reused rdf:type owl:Class ;
           rdfs:subClassOf edo:DomainAttribute ;
           dcterms:accessRights "PUBLIC" ;
           dcterms:identifier "Reused" ;
           rdfs:comment "Especifica se este segmento/tramo já foi utilizado anteriormente em uma outra localização"@pt-br ;
           skos:definition "Specifies whether this segment/segment has already been used previously in another location"@en ;
           skos:prefLabel "Reused"@en ,
                          "Reutilizado"@pt-br ;
           edo:hasAttributeScope edo:TypeLevelAttribute ;
           edo:hasLifecycleCreationPhase edo:DetailedDesign ;
           edo:hasTypedValue edo:IfcBoolean ;
           edo:hasValueCardinality edo:SingleValue .


###  https://w3id.org/energy-domain/edo#RigidJoint
edo:RigidJoint rdf:type owl:Class ;
               rdfs:subClassOf edo:LineAncillary ;
               dcterms:identifier "RigidJoint" ;
               skos:definition "Acessório de uso temporário para conexão entre armor pot e enrijecedor abaixo dele, a fim de prevenir curvatura excessiva da linha durante operações de manuseio."@pt-br ,
                               "Temporary accessory for connection between the armour pot and the bend stiffener below it, in order to prevent excessive line bending during handling operations."@en ;
               skos:prefLabel "Junta Rígida"@pt-br ,
                              "Rigid Joint"@en ;
               edo:hasDiscipline edo:SubseaUmbilicalsEngineering ;
               edo:ifc_equivalentClass "IfcPipeFitting" ;
               edo:ifc_objectType "RigidJoint" .


###  https://w3id.org/energy-domain/edo#RigidJumper
edo:RigidJumper rdf:type owl:Class ;
                rdfs:subClassOf edo:TieInEquipment ;
                dcterms:identifier "RigidJumper" ;
                skos:definition "Elemento de interligação composto de tubulação rígida e conectores, instalável entre hubs de equipamentos submarinos"@pt-br ,
                                "Tie-in element composed of rigid piping and connectors, installed between subsea equipment hubs"@en ;
                skos:prefLabel "Jumper rígido"@pt-br ,
                               "Rigid jumper"@en .


###  https://w3id.org/energy-domain/edo#RingGasket
edo:RingGasket rdf:type owl:Class ;
               rdfs:subClassOf edo:IfcInstanciableElement ,
                               edo:PhysicalConnection ;
               dcterms:identifier "RingGasket" ;
               skos:altLabel " Seal Ring"@en ,
                             "Gasket"@en ,
                             "O-Ring"@en ,
                             "Packing Ring"@en ,
                             "Seal Gasket"@en ,
                             "Sealing Ring"@en ;
               skos:definition "The seal ring is a crucial component used in subsea oil and gas interconnection end fittings to ensure a secure and leak-proof connection between pipes or equipment. Typically made from high-performance materials such as elastomers or metals, the seal ring is designed to withstand extreme pressure, temperature, and environmental conditions found in subsea operations. It is installed within the end fitting to create a reliable seal that prevents fluid leakage and maintains the integrity of the interconnection. The seal ring’s precise design and material selection are essential for ensuring long-term durability and performance in harsh subsea environments."@en ;
               skos:prefLabel "Junta de Conexão"@pt-br ,
                              "Ring Gasket"@en ;
               edo:hasAttribute edo:RingGasketInnerDIameter ,
                                edo:RingGasketMaterial ,
                                edo:RingGasketOuterDiameter ,
                                edo:RingGasketPressureRating ,
                                edo:RingGasketSpecification ,
                                edo:RingGasketStandard ,
                                edo:RingGasketType ;
               edo:hasDiscipline edo:SubseaFlexiblePipesEngineering ,
                                 edo:SubseaUmbilicalsEngineering ;
               edo:ifc_equivalentClass "IfcMechanicalFastener" ;
               edo:ifc_objectType "RingGasket" ;
               edo:ifc_predefinedType "USERDEFINED" .


###  https://w3id.org/energy-domain/edo#RingGasketAttribute
edo:RingGasketAttribute rdf:type owl:Class ;
                        rdfs:subClassOf edo:DomainAttribute ;
                        rdfs:label "Ring Gasket"@en .


###  https://w3id.org/energy-domain/edo#RingGasketInnerDIameter
edo:RingGasketInnerDIameter rdf:type owl:Class ;
                            rdfs:subClassOf edo:RingGasketAttribute ;
                            dcterms:accessRights "PUBLIC" ;
                            dcterms:identifier "RingGasketInnerDIameter" ;
                            skos:definition "The internal diameter, which determines the size of the bore it fits into. This dimension is crucial for ensuring a proper fit and effective sealing."@en ;
                            skos:prefLabel "Diâmetro Interno da Junta de Vedação"@pt-br ,
                                           "Ring Gasket Inner Diameter"@en ;
                            edo:hasAttributeScope edo:TypeLevelAttribute ;
                            edo:hasLifecycleCreationPhase edo:DetailedDesign ;
                            edo:hasTypedValue edo:FloatValue ;
                            edo:hasUnit unit:MilliM ;
                            edo:hasValueCardinality edo:SingleValue .


###  https://w3id.org/energy-domain/edo#RingGasketMaterial
edo:RingGasketMaterial rdf:type owl:Class ;
                       rdfs:subClassOf edo:RingGasketAttribute ;
                       dcterms:accessRights "PUBLIC" ;
                       dcterms:identifier "RingGasketMaterial" ;
                       skos:definition "Type of material from which an object is made, allowing for precise documentation and categorisation."@en ;
                       skos:prefLabel "Material da Junta de Vedação"@pt-br ,
                                      "Ring Gasket Material"@en ;
                       edo:hasAttributeScope edo:TypeLevelAttribute ;
                       edo:hasLifecycleCreationPhase edo:DetailedDesign ;
                       edo:hasTypedValue edo:StringValue ;
                       edo:hasValueCardinality edo:SingleValue .


###  https://w3id.org/energy-domain/edo#RingGasketOuterDiameter
edo:RingGasketOuterDiameter rdf:type owl:Class ;
                            rdfs:subClassOf edo:RingGasketAttribute ;
                            dcterms:accessRights "PUBLIC" ;
                            dcterms:identifier "RingGasketOuterDiameter" ;
                            skos:definition "The external diameter, which determines the size of the surface it seals against. This dimension is essential for providing a secure seal and preventing leakage."@en ;
                            skos:prefLabel "Diâmetro Externo da Junta de Vedação"@pt-br ,
                                           "Ring Gasket Outer Diameter"@en ;
                            edo:hasAttributeScope edo:TypeLevelAttribute ;
                            edo:hasLifecycleCreationPhase edo:DetailedDesign ;
                            edo:hasTypedValue edo:FloatValue ;
                            edo:hasUnit unit:MilliM ;
                            edo:hasValueCardinality edo:SingleValue .


###  https://w3id.org/energy-domain/edo#RingGasketPressureRating
edo:RingGasketPressureRating rdf:type owl:Class ;
                             rdfs:subClassOf edo:RingGasketAttribute ;
                             dcterms:accessRights "PUBLIC" ;
                             dcterms:identifier "RingGasketPressureRating" ;
                             skos:definition "The maximum pressure it can withstand without failing. This rating is important for ensuring that the seal ring performs effectively under the operating pressures of the application."@en ;
                             skos:prefLabel "Classificação de Pressão da Junta de Vedação"@pt-br ,
                                            "Ring Gasket Pressure Rating"@en ;
                             edo:hasAttributeScope edo:TypeLevelAttribute ;
                             edo:hasLifecycleCreationPhase edo:DetailedDesign ;
                             edo:hasTypedValue edo:FloatValue ;
                             edo:hasUnit unit:PA ;
                             edo:hasValueCardinality edo:SingleValue .


###  https://w3id.org/energy-domain/edo#RingGasketSpecification
edo:RingGasketSpecification rdf:type owl:Class ;
                            rdfs:subClassOf edo:RingGasketAttribute ;
                            dcterms:accessRights "PUBLIC" ;
                            dcterms:identifier "RingGasketSpecification" ;
                            skos:definition "The detailed description of it's design and performance characteristics, including material, size, and pressure rating. This provides comprehensive information about the seal ring's suitability for specific applications."@en ;
                            skos:prefLabel "Especificação da Junta de Vedação"@pt-br ,
                                           "Ring Gasket Specification"@en ;
                            edo:hasAttributeScope edo:TypeLevelAttribute ;
                            edo:hasLifecycleCreationPhase edo:DetailedDesign ;
                            edo:hasTypedValue edo:StringValue ;
                            edo:hasValueCardinality edo:SingleValue .


###  https://w3id.org/energy-domain/edo#RingGasketStandard
edo:RingGasketStandard rdf:type owl:Class ;
                       rdfs:subClassOf edo:RingGasketAttribute ;
                       dcterms:accessRights "PUBLIC" ;
                       dcterms:identifier "RingGasketStandard" ;
                       skos:definition "The standard or specification it conforms to, such as API, ISO, or other industry standards. This indicates the compliance of the seal ring with established guidelines for quality and performance."@en ;
                       skos:prefLabel "Padrão da Junta de Vedação"@pt-br ,
                                      "Ring Gasket Standard"@en ;
                       edo:hasAttributeScope edo:TypeLevelAttribute ;
                       edo:hasLifecycleCreationPhase edo:DetailedDesign ;
                       edo:hasTypedValue edo:StringValue ;
                       edo:hasValueCardinality edo:SingleValue .


###  https://w3id.org/energy-domain/edo#RingGasketType
edo:RingGasketType rdf:type owl:Class ;
                   rdfs:subClassOf edo:RingGasketAttribute ;
                   dcterms:accessRights "PUBLIC" ;
                   dcterms:identifier "RingGasketType" ;
                   skos:definition "The specific type or design. This classification helps identify the appropriate seal ring based on its design and application requirements, ensuring it meets the sealing needs under various conditions."@en ;
                   skos:prefLabel "Ring Gasket Type"@en ,
                                  "Tipo de Junta de Vedação"@pt-br ;
                   edo:hasAttributeScope edo:TypeLevelAttribute ;
                   edo:hasLifecycleCreationPhase edo:DetailedDesign ;
                   edo:hasTypedValue edo:StringValue ;
                   edo:hasValueCardinality edo:SingleValue .


###  https://w3id.org/energy-domain/edo#RiserBalcony
edo:RiserBalcony rdf:type owl:Class ;
                 rdfs:subClassOf edo:Location ;
                 dcterms:identifier "RiserBalcony" ;
                 skos:definition "Installation location for supports and accessories on the riser balcony of the production unit."@en ,
                                 "Local de instalação para suportes e acessórios no riser balcony da unidade de produção"@pt-br ;
                 skos:prefLabel "Plataforma do Riser"@pt-br ,
                                "Riser Balcony"@en .


###  https://w3id.org/energy-domain/edo#RiserConfiguration
edo:RiserConfiguration rdf:type owl:Class ;
                       rdfs:subClassOf edo:DomainAttribute ;
                       dcterms:accessRights "PUBLIC" ;
                       dcterms:identifier "RiserConfiguration" ;
                       skos:definition "This property specifies the configuration type for the riser section of the pipeline. It provides key information on the structural design, indicating the arrangement and dynamic behaviour of the riser system. The chosen configuration affects how the structure responds to environmental forces, such as currents and pressure, and plays a critical role in determining the overall performance and durability of the system."@en ;
                       skos:prefLabel "Configuração do Riser"@pt-br ,
                                      "Riser Configuration"@en ;
                       edo:hasAttributeScope edo:InstanceLevelAttribute ;
                       edo:hasLifecycleCreationPhase edo:BasicDesign ;
                       edo:hasTypedValue edo:StringValue ;
                       edo:hasValueCardinality edo:SingleValue .


###  https://w3id.org/energy-domain/edo#RiserSpan
edo:RiserSpan rdf:type owl:Class ;
              rdfs:subClassOf edo:IfcInstanciableElement ,
                              edo:PipelineSpan ;
              dcterms:identifier "RiserSpan" ;
              skos:definition "Suspended pipeline span, continuously subjected to dynamic loading"@en ,
                              "Trecho de duto suspenso, sujeito continuamente a esforços dinâmicos"@pt-br ;
              skos:prefLabel "Riser span"@en ,
                             "Trecho riser"@pt-br ;
              edo:hasDiscipline edo:SubseaFlexiblePipesEngineering .


###  https://w3id.org/energy-domain/edo#RiserSupport
edo:RiserSupport rdf:type owl:Class ;
                 rdfs:subClassOf edo:Component ;
                 dcterms:identifier "RiserSupport" ;
                 skos:definition "Interface at the production unit for coupling and support of a riser"@en ,
                                 "Interface na unidade de produção para acoplamento e suporte de um riser"@pt-br ;
                 skos:prefLabel "Riser support"@en ,
                                "Suporte de riser"@pt-br .


###  https://w3id.org/energy-domain/edo#RiserSupportBuoy
edo:RiserSupportBuoy rdf:type owl:Class ;
                     rdfs:subClassOf edo:BuoyancyTank ;
                     dcterms:identifier "RiserSupportBuoy" ;
                     skos:prefLabel "Bóia de sustentação de risers"@pt-br ,
                                    "Riser support buoy"@en .


###  https://w3id.org/energy-domain/edo#RoboticActuator
edo:RoboticActuator rdf:type owl:Class ;
                    rdfs:subClassOf edo:AuxiliaryModule ;
                    dcterms:identifier "RoboticActuator" ;
                    skos:definition "Shared actuation system able to serve multiple final control elements (e.g. valves)"@en ,
                                    "Sistema de atuação compartilhada capaz de servir a múltiplos elementos de controle finais (ex.: válvulas)"@pt-br ;
                    skos:prefLabel "Atuador robótico"@pt-br ,
                                   "Robotic actuator"@en .


###  https://w3id.org/energy-domain/edo#RopeSegment
edo:RopeSegment rdf:type owl:Class ;
                rdfs:subClassOf edo:LinearObject ;
                dcterms:identifier "RopeSegment" ;
                skos:prefLabel "Rope segment"@en ,
                               "Tramo de cabo"@pt-br .


###  https://w3id.org/energy-domain/edo#RotatingEquipmentEngineering
edo:RotatingEquipmentEngineering rdf:type owl:Class ;
                                 rdfs:subClassOf edo:EquipmentEngineering ;
                                 rdfs:label "Engenharia de Equipamentos Rotativos"@pt-br ,
                                            "Rotating Equipment Engineering"@en ;
                                 skos:definition "Engenharia de equipamentos mecânicos com componentes rotativos como bombas, compressores e turbinas."@pt-br ,
                                                 "Engineering of mechanical equipment with rotating components such as pumps, compressors, and turbines."@en .


###  https://w3id.org/energy-domain/edo#RotatingMachine
edo:RotatingMachine rdf:type owl:Class ;
                    rdfs:subClassOf edo:PowerMachine ;
                    dcterms:identifier "RotatingMachine" ;
                    skos:prefLabel "Máquina rotativa"@pt-br ,
                                   "Rotating machine"@en .


###  https://w3id.org/energy-domain/edo#RunOfRiver
edo:RunOfRiver rdf:type owl:Class ;
               rdfs:subClassOf edo:Hydropower ;
               dcterms:identifier "RunOfRiver" ;
               skos:definition "Run-of-river hydropower plants generate electricity directly from the natural flow of rivers without creating large reservoirs, minimizing flooding but making output dependent on seasonal water levels."@en ,
                               "Usinas hidrelétricas a fio d’água geram eletricidade diretamente a partir do fluxo natural dos rios, sem criar grandes reservatórios, minimizando alagamentos mas tornando a produção dependente da sazonalidade hídrica."@pt-br ;
               skos:prefLabel "Hidrelétrica a Fio d’Água"@pt-br ,
                              "Run-of-River Hydropower"@en .


###  https://w3id.org/energy-domain/edo#RunningTool
edo:RunningTool rdf:type owl:Class ;
                rdfs:subClassOf edo:ActuatedEquipment ;
                dcterms:identifier "RunningTool" ;
                skos:definition "Ferramenta de grande porte para instalação ou recuperação de equipamentos no ambiente submarino"@pt-br ,
                                "Major tools for installation or retrieval of equipment in the subsea environment"@en ;
                skos:prefLabel "Ferramenta submarina de instalação"@pt-br ,
                               "Subsea running tool"@en .


###  https://w3id.org/energy-domain/edo#RuptDefAlongFibers
edo:RuptDefAlongFibers rdf:type owl:Class ;
                       rdfs:subClassOf edo:DomainAttribute ;
                       dcterms:accessRights "PUBLIC" ;
                       dcterms:identifier "RuptDefAlongFibers" ;
                       skos:definition "Describes the deformation that occurs when the composite material ruptures in a direction parallel to its fibers. This property is essential for assessing the material's behavior under stress aligned with the fiber orientation, providing insights into its performance and durability in subsea structures where axial forces are present."@en ;
                       skos:prefLabel "Deformação de Ruptura longitudinalmente às fibras"@pt-br ,
                                      "Rupture Deformation Along Fibers"@en ;
                       edo:hasAttributeScope edo:TypeLevelAttribute ;
                       edo:hasLifecycleCreationPhase edo:DetailedDesign ;
                       edo:hasTypedValue edo:FloatValue ;
                       edo:hasUnit unit:PERCENT ;
                       edo:hasValueCardinality edo:SingleValue .


###  https://w3id.org/energy-domain/edo#RuptDefPerpendFibers
edo:RuptDefPerpendFibers rdf:type owl:Class ;
                         rdfs:subClassOf edo:DomainAttribute ;
                         dcterms:accessRights "PUBLIC" ;
                         dcterms:identifier "RuptDefPerpendFibers" ;
                         skos:definition "Describes the deformation that occurs when the composite material ruptures in a direction perpendicular to its fibers. This property is crucial for understanding the material's behavior under stress conditions that do not align with the fiber orientation, helping to assess its performance and failure limits in subsea structures."@en ;
                         skos:prefLabel "Deformação de Ruptura perpendicularmente às fibras"@pt-br ,
                                        "Rupture Deformation Perpendicular To Fibers"@en ;
                         edo:hasAttributeScope edo:TypeLevelAttribute ;
                         edo:hasLifecycleCreationPhase edo:DetailedDesign ;
                         edo:hasTypedValue edo:FloatValue ;
                         edo:hasUnit unit:PERCENT ;
                         edo:hasValueCardinality edo:SingleValue .


###  https://w3id.org/energy-domain/edo#SCM
edo:SCM rdf:type owl:Class ;
        rdfs:subClassOf edo:AuxiliaryModule ;
        dcterms:identifier "SCM" ;
        skos:definition "Distribution module for control and monitoring functions in subsea equipment"@en ,
                        "Módulo de distribuição de funções de controle e monitoramento em um equipamento submarino"@pt-br ;
        skos:prefLabel "Módulo de controle submarino"@pt-br ,
                       "Subsea control module"@en ;
        edo:hasDiscipline edo:WetChristmasTreesEngineering .


###  https://w3id.org/energy-domain/edo#SCMMB
edo:SCMMB rdf:type owl:Class ;
          rdfs:subClassOf edo:AuxiliaryModule ;
          dcterms:identifier "SCMMB" ;
          skos:definition "Equipamento para instalação indireta de um SCM"@pt-br ,
                          "Equipment for indirect SCM installation"@en ;
          skos:prefLabel "Base de montagem de SCM"@pt-br ,
                         "SCM mounting base"@en ;
          edo:hasDiscipline edo:WetChristmasTreesEngineering .


###  https://w3id.org/energy-domain/edo#SCMRunningTool
edo:SCMRunningTool rdf:type owl:Class ;
                   rdfs:subClassOf edo:RunningTool ;
                   dcterms:identifier "SCMRunningTool" ;
                   skos:prefLabel "Ferramenta de instalação de SCM"@pt-br ,
                                  "SCM running tool"@en .


###  https://w3id.org/energy-domain/edo#SDU
edo:SDU rdf:type owl:Class ;
        rdfs:subClassOf edo:SubseaEquipment ;
        dcterms:identifier "SDU" ;
        skos:prefLabel "Subsea distribution unit"@en ,
                       "Unidade de distribuição submarina"@pt-br .


###  https://w3id.org/energy-domain/edo#SEM
edo:SEM rdf:type owl:Class ;
        rdfs:subClassOf edo:ElectronicDevice ;
        dcterms:identifier "SEM" ;
        skos:prefLabel "Módulo eletrônico submarino"@pt-br ,
                       "Subsea electronic module"@en .


###  https://w3id.org/energy-domain/edo#SacrificialSheath
edo:SacrificialSheath rdf:type owl:Class ;
                      rdfs:subClassOf edo:IfcInstanciableElement ,
                                      edo:SolidLayer ;
                      dcterms:identifier "SacrificialSheath" ;
                      skos:definition "A protective layer in subsea flexible pipes designed to absorb damage from external environmental factors, such as abrasion or impact, over time. The Sacrificial Sheath is intended to wear out or degrade under harsh conditions, thereby preserving the integrity of the underlying layers and prolonging the overall lifespan of the pipe. Made from durable materials, this sheath acts as the first line of defense, allowing for the controlled degradation of the pipe's outer surface without affecting its core structural or functional performance."@en ;
                      skos:prefLabel "Camada de Sacrifício"@pt-br ,
                                     "Sacrificial Sheath"@en ;
                      edo:hasDiscipline edo:SubseaFlexiblePipesEngineering ;
                      edo:ifc_equivalentClass "IfcPipeSegment" ;
                      edo:ifc_objectType "SacrificialSheath" ;
                      edo:ifc_predefinedType "USERDEFINED" .


###  https://w3id.org/energy-domain/edo#SafeWorkingLoad
edo:SafeWorkingLoad rdf:type owl:Class ;
                    rdfs:subClassOf edo:DomainAttribute ;
                    dcterms:accessRights "PUBLIC" ;
                    dcterms:identifier "SafeWorkingLoad" ;
                    skos:definition "Safe Working Load (SWL) refers to the maximum load that can be safely handled under normal operating conditions. This value ensures the equipment operates within its designed capacity, preventing overloading and potential failure."@en ;
                    skos:prefLabel "Carga Máxima Segura de Trabalho"@pt-br ,
                                   "Safe Working Load"@en ;
                    edo:hasAttributeScope edo:TypeLevelAttribute ;
                    edo:hasLifecycleCreationPhase edo:DetailedDesign ;
                    edo:hasTypedValue edo:FloatValue ;
                    edo:hasUnit unit:KiloGM_F ,
                                unit:TONNE_F ;
                    edo:hasValueCardinality edo:SingleValue .


###  https://w3id.org/energy-domain/edo#SafetyLossPreventionEngineering
edo:SafetyLossPreventionEngineering rdf:type owl:Class ;
                                    rdfs:subClassOf edo:TechnicalDiscipline ;
                                    rdfs:label "Engenharia de Segurança e Prevenção de Perdas"@pt-br ,
                                               "Safety & Loss Prevention Engineering"@en ;
                                    skos:definition "Disciplina de engenharia focada em avaliação de riscos, sistemas de segurança e prevenção de perdas."@pt-br ,
                                                    "Engineering discipline focused on risk assessment, safety systems and loss prevention."@en .


###  https://w3id.org/energy-domain/edo#SalinityGradient
edo:SalinityGradient rdf:type owl:Class ;
                     rdfs:subClassOf edo:Marine ;
                     dcterms:identifier "SalinityGradient" ;
                     skos:definition "Energia de gradiente de salinidade, também chamada de energia azul, é obtida aproveitando a diferença de concentração de sal entre a água do mar e a água doce em estuários. Tecnologias como eletrodiálise reversa ou osmose com pressão retardada podem converter esse potencial químico em energia renovável."@pt-br ,
                                     "Salinity gradient energy, also called blue energy, is obtained by exploiting the difference in salt concentration between seawater and freshwater at estuaries. Technologies such as reverse electrodialysis or pressure-retarded osmosis can convert this chemical potential into renewable power."@en ;
                     skos:prefLabel "Energia de Gradiente de Salinidade"@pt-br ,
                                    "Salinity Gradient Energy"@en .


###  https://w3id.org/energy-domain/edo#SandDetector
edo:SandDetector rdf:type owl:Class ;
                 rdfs:subClassOf edo:Sensor ;
                 dcterms:identifier "SandDetector" ;
                 skos:prefLabel "Detector de areia"@pt-br ,
                                "Sand detector"@en .


###  https://w3id.org/energy-domain/edo#Sensor
edo:Sensor rdf:type owl:Class ;
           rdfs:subClassOf edo:ElectronicDevice ;
           dcterms:identifier "Sensor" ;
           skos:prefLabel "Sensor"@en ,
                          "Sensor"@pt-br .


###  https://w3id.org/energy-domain/edo#SeparatorVessel
edo:SeparatorVessel rdf:type owl:Class ;
                    rdfs:subClassOf edo:Vessel ;
                    dcterms:identifier "SeparatorVessel" ;
                    skos:prefLabel "Seaparator vessel"@en ,
                                   "Vaso separador"@pt-br .


###  https://w3id.org/energy-domain/edo#SerialNumber
edo:SerialNumber rdf:type owl:Class ;
                 rdfs:subClassOf edo:DomainAttribute ;
                 dcterms:accessRights "PUBLIC" ;
                 dcterms:identifier "SerialNumber" ;
                 skos:definition "A unique identifier assigned to each individual item, distinguishing it from all other units of the same type. The Serial Number is critical for traceability, maintenance, and warranty purposes, ensuring that the history, performance, and lifecycle of the equipment can be tracked. It is often used in conjunction with a Part Number, which identifies the type or model of the component."@en ;
                 skos:prefLabel "Número de Série"@pt-br ,
                                "Serial Number"@en ;
                 edo:hasAttributeScope edo:InstanceLevelAttribute ;
                 edo:hasLifecycleCreationPhase edo:DetailedDesign ;
                 edo:hasTypedValue edo:StringValue ;
                 edo:hasValueCardinality edo:SingleValue .


###  https://w3id.org/energy-domain/edo#Service
edo:Service rdf:type owl:Class ;
            rdfs:subClassOf edo:DomainAttribute ;
            dcterms:accessRights "PUBLIC" ;
            dcterms:identifier "Service" ;
            skos:definition "Escolha um da lista: IA (Injeção de água); IG (Injeção de Gás); LPO (Linha de Produção de Óleo); PG (Produtor de Gás); SE (Serviço); GAS (Gasoduto); UEH (Umbilical Eletro Hidráulico); CEP (Cabo Elétrico de Potência)"@pt-br ,
                            "Indicates the type of service the pipeline is designated for, specifying its operational purpose within the project. This classification is used to ensure proper management, installation, and use of the pipeline according to its intended function."@en ;
            skos:prefLabel "Service"@en ,
                           "Serviço"@pt-br ;
            edo:hasAttributeScope edo:InstanceLevelAttribute ;
            edo:hasLifecycleCreationPhase edo:BasicDesign ;
            edo:hasTypedValue edo:StringValue ;
            edo:hasValueCardinality edo:SingleValue .


###  https://w3id.org/energy-domain/edo#Shackle
edo:Shackle rdf:type owl:Class ;
            rdfs:subClassOf edo:IfcInstanciableElement ,
                            edo:MooringAccessory ;
            dcterms:identifier "Shackle" ;
            skos:altLabel "Anchor Shackle"@en ,
                          "Bow Shackle"@en ,
                          "Clevis"@en ,
                          "D-Shackle"@en ,
                          "U-Bolt"@en ;
            skos:definition "A device used to connect and secure components in subsea systems, particularly during lifting, handling, or mooring operations. The Shackle typically consists of a U-shaped metal piece with a removable pin or bolt, allowing it to link components such as chains, slings, or cables. It provides a strong and reliable connection point, ensuring that loads can be safely transferred or lifted without risk of detachment or failure. Shackles are essential for securing flexible lines and other equipment during installation and maintenance in subsea environments."@en ,
                            "Elemento para permitir conexão de uma corrente ou cabo adequadamente terminado a outros elementos"@pt-br ;
            skos:prefLabel "Manilha"@pt-br ,
                           "Shackle"@en ;
            edo:hasAttribute edo:ShackleInnerDiameter ,
                             edo:ShackleOpeningWidth ,
                             edo:ShackleOuterDiameter ,
                             edo:ShackleThickness ,
                             edo:WorkingLoadLimit ;
            edo:hasDiscipline edo:SubseaFlexiblePipesEngineering ;
            edo:ifc_equivalentClass "IfcMechanicalFastener" ;
            edo:ifc_objectType "Shackle" ;
            edo:ifc_predefinedType "USERDEFINED" .


###  https://w3id.org/energy-domain/edo#ShackleInnerDiameter
edo:ShackleInnerDiameter rdf:type owl:Class ;
                         rdfs:subClassOf edo:DomainAttribute ;
                         dcterms:accessRights "PUBLIC" ;
                         dcterms:identifier "ShackleInnerDiameter" ;
                         skos:definition "Indicates the inner diameter of the shackle. This property measures the width of the space inside the shackle, which is important for ensuring compatibility with other components and for determining the appropriate fit and load distribution."@en ;
                         skos:prefLabel "Diâmetro interno da furação do olhal"@pt-br ,
                                        "Shackle Inner Diameter"@en ;
                         edo:hasAttributeScope edo:InstanceLevelAttribute ;
                         edo:hasLifecycleCreationPhase edo:DetailedDesign ;
                         edo:hasTypedValue edo:FloatValue ;
                         edo:hasUnit unit:M ;
                         edo:hasValueCardinality edo:SingleValue .


###  https://w3id.org/energy-domain/edo#ShackleOpeningWidth
edo:ShackleOpeningWidth rdf:type owl:Class ;
                        rdfs:subClassOf edo:DomainAttribute ;
                        dcterms:accessRights "PUBLIC" ;
                        dcterms:identifier "ShackleOpeningWidth" ;
                        skos:definition "Measures the width of the opening in the shackle where components, such as pins or cables, are inserted. This property is crucial for ensuring that the shackle can properly accommodate and secure the intended connecting elements."@en ;
                        skos:prefLabel "Largura da Abertura"@pt-br ,
                                       "Shackle Opening Width"@en ;
                        edo:hasAttributeScope edo:InstanceLevelAttribute ;
                        edo:hasLifecycleCreationPhase edo:DetailedDesign ;
                        edo:hasTypedValue edo:FloatValue ;
                        edo:hasUnit unit:M ;
                        edo:hasValueCardinality edo:SingleValue .


###  https://w3id.org/energy-domain/edo#ShackleOuterDiameter
edo:ShackleOuterDiameter rdf:type owl:Class ;
                         rdfs:subClassOf edo:DomainAttribute ;
                         dcterms:accessRights "PUBLIC" ;
                         dcterms:identifier "ShackleOuterDiameter" ;
                         skos:definition "Indicates the outer diameter of the shackle. This property provides the measurement of the overall width of the shackle, which is crucial for ensuring it fits properly with other components and meets the design specifications for load-bearing and connection requirements."@en ;
                         skos:prefLabel "Diâmetro externo do olhal"@pt-br ,
                                        "Shackle Outer Diameter"@en ;
                         edo:hasAttributeScope edo:InstanceLevelAttribute ;
                         edo:hasLifecycleCreationPhase edo:DetailedDesign ;
                         edo:hasTypedValue edo:FloatValue ;
                         edo:hasUnit unit:M ;
                         edo:hasValueCardinality edo:SingleValue .


###  https://w3id.org/energy-domain/edo#ShackleThickness
edo:ShackleThickness rdf:type owl:Class ;
                     rdfs:subClassOf edo:DomainAttribute ;
                     dcterms:accessRights "PUBLIC" ;
                     dcterms:identifier "ShackleThickness" ;
                     skos:definition "Specifies the thickness of the shackle material. This property measures the distance between the inner and outer surfaces of the shackle, which is essential for understanding its strength, durability, and ability to handle load stresses."@en ;
                     skos:prefLabel "Espessura do olhal"@pt-br ,
                                    "Shackle Thickness"@en ;
                     edo:hasAttributeScope edo:InstanceLevelAttribute ;
                     edo:hasLifecycleCreationPhase edo:DetailedDesign ;
                     edo:hasTypedValue edo:FloatValue ;
                     edo:hasUnit unit:M ;
                     edo:hasValueCardinality edo:SingleValue .


###  https://w3id.org/energy-domain/edo#ShearableRiserJoint
edo:ShearableRiserJoint rdf:type owl:Class ;
                        rdfs:subClassOf edo:RunningTool ;
                        dcterms:identifier "ShearableRiserJoint" ;
                        skos:prefLabel "Junta riser cisalhável"@pt-br ,
                                       "Shearable riser joint"@en .


###  https://w3id.org/energy-domain/edo#ShortTermFloatDensity
edo:ShortTermFloatDensity rdf:type owl:Class ;
                          rdfs:subClassOf edo:DomainAttribute ;
                          dcterms:accessRights "PUBLIC" ;
                          dcterms:identifier "ShortTermFloatDensity" ;
                          skos:definition "Representa a densidade do flutuador logo após o início da operação, considerando um aumento de densidade devido à absorção de água em pequena quantidade ou outras alterações superficiais."@pt-br ,
                                          "The density of the float material in the early stages of operation, accounting for slight water absorption or other surface-level changes."@en ;
                          skos:prefLabel "Densidade do Flutuador a Curto Prazo"@pt-br ,
                                         "Short Term Float Density"@en ;
                          edo:hasAttributeScope edo:TypeLevelAttribute ;
                          edo:hasLifecycleCreationPhase edo:DetailedDesign ;
                          edo:hasTypedValue edo:FloatValue ;
                          edo:hasUnit unit:KiloGM-PER-M3 ;
                          edo:hasValueCardinality edo:SingleValue .


###  https://w3id.org/energy-domain/edo#ShortTermFloatVolume
edo:ShortTermFloatVolume rdf:type owl:Class ;
                         rdfs:subClassOf edo:DomainAttribute ;
                         dcterms:accessRights "PUBLIC" ;
                         dcterms:identifier "ShortTermFloatVolume" ;
                         skos:definition "O volume submerso esperado logo após o início da operação, levando em consideração pequenas variações iniciais, como a absorção mínima de água ou pequenas deformações. Serve para calcular a flutuabilidade em condições reais no curto prazo."@pt-br ,
                                         "The expected submerged volume of the float during the initial phase of operation, considering minor factors like slight water absorption or small deformations."@en ;
                         skos:prefLabel "Short Term Float Volume"@en ,
                                        "Volume do Flutuador a Curto Prazo"@pt-br ;
                         edo:hasAttributeScope edo:TypeLevelAttribute ;
                         edo:hasLifecycleCreationPhase edo:DetailedDesign ;
                         edo:hasTypedValue edo:FloatValue ;
                         edo:hasUnit unit:M3 ,
                                     unit:m3 ;
                         edo:hasValueCardinality edo:SingleValue .


###  https://w3id.org/energy-domain/edo#SingleValue
edo:SingleValue rdf:type owl:Class ;
                rdfs:subClassOf edo:AttributeValueCardinality ;
                rdfs:comment "Constraint ensuring only one value (not a list)"@en ,
                             "Restrição assegurando apenas um valor (não uma lista)"@pt-br ;
                rdfs:label "Single Value"@en ,
                           "Valor Simples"@pt-br .


###  https://w3id.org/energy-domain/edo#SmallHydropower
edo:SmallHydropower rdf:type owl:Class ;
                    rdfs:subClassOf edo:Hydropower ;
                    dcterms:identifier "SmallHydropower" ;
                    skos:definition "Pequenas centrais hidrelétricas, frequentemente chamadas de PCH, possuem tipicamente capacidade abaixo de 30 MW. Utilizam o fluxo dos rios com infraestrutura reduzida, diminuindo o impacto ambiental em comparação às grandes barragens."@pt-br ,
                                    "Small hydropower plants, often called small hydro or PCH, typically have capacities below 30 MW. They use river flow with smaller infrastructure, reducing environmental impact compared to large dams."@en ;
                    skos:prefLabel "Pequena Central Hidrelétrica"@pt-br ,
                                   "Small Hydropower"@en .


###  https://w3id.org/energy-domain/edo#SmallWind
edo:SmallWind rdf:type owl:Class ;
              rdfs:subClassOf edo:Wind ;
              dcterms:identifier "SmallWind" ;
              skos:definition "Sistemas de pequena escala eólica referem-se a microturbinas projetadas para uso residencial, agrícola ou em pequenos negócios. Eles oferecem geração descentralizada de eletricidade renovável e podem operar de forma independente ou conectados à rede."@pt-br ,
                              "Small wind systems refer to microturbines designed for residential, agricultural, or small business use. They provide decentralized renewable electricity generation and can operate independently or connected to the grid."@en ;
              skos:prefLabel "Eólica de Pequena Escala"@pt-br ,
                             "Small Wind"@en .


###  https://w3id.org/energy-domain/edo#Socket
edo:Socket rdf:type owl:Class ;
           rdfs:subClassOf edo:MooringAccessory ;
           dcterms:identifier "Socket" ;
           skos:definition "Elemento de terminação para uma extremidade de um cabo de ancoragem"@pt-br ,
                           "End termination element for a mooring rope"@en ;
           skos:prefLabel "Socket"@en ,
                          "Soquete"@pt-br .


###  https://w3id.org/energy-domain/edo#Solar
edo:Solar rdf:type owl:Class ;
          rdfs:subClassOf edo:Renewable ;
          rdfs:label "Energia Solar"@pt-br ,
                     "Solar Energy"@en ;
          skos:definition "Energia obtida da luz solar, incluindo sistemas fotovoltaicos e térmicos."@pt-br ,
                          "Energy harnessed from sunlight, including photovoltaic and thermal systems."@en .


###  https://w3id.org/energy-domain/edo#SolarHeatingCooling
edo:SolarHeatingCooling rdf:type owl:Class ;
                        rdfs:subClassOf edo:Solar ;
                        dcterms:identifier "SolarHeatingCooling" ;
                        skos:definition "Solar heating and cooling technologies capture solar radiation at low or medium temperatures to provide hot water, space heating, or cooling through solar thermal collectors and absorption systems."@en ,
                                        "Tecnologias de aquecimento e resfriamento solar capturam radiação solar em baixa ou média temperatura para fornecer água quente, aquecimento de ambientes ou resfriamento por meio de coletores solares térmicos e sistemas de absorção."@pt-br ;
                        skos:prefLabel "Aquecimento e Resfriamento Solar"@pt-br ,
                                       "Solar Heating and Cooling"@en .


###  https://w3id.org/energy-domain/edo#SolarThermal
edo:SolarThermal rdf:type owl:Class ;
                 rdfs:subClassOf edo:Solar ;
                 dcterms:identifier "SolarThermal" ;
                 skos:definition "Energia solar térmica, também conhecida como concentração solar (CSP), utiliza espelhos ou lentes para concentrar a luz solar e gerar calor em alta temperatura, que depois é convertido em eletricidade por meio de um ciclo termodinâmico."@pt-br ,
                                 "Solar thermal energy, also known as concentrated solar power (CSP), uses mirrors or lenses to concentrate sunlight and produce high-temperature heat, which is then converted into electricity through a thermodynamic cycle."@en ;
                 skos:prefLabel "Solar Thermal"@en ,
                                "Solar Térmica"@pt-br .


###  https://w3id.org/energy-domain/edo#SolidBiomass
edo:SolidBiomass rdf:type owl:Class ;
                 rdfs:subClassOf edo:Biomass ;
                 dcterms:identifier "SolidBiomass" ;
                 skos:definition "Energia de biomassa sólida vem da combustão ou processamento de materiais orgânicos como madeira, resíduos florestais e agrícolas. É uma das formas mais antigas de energia renovável, ainda amplamente utilizada para aquecimento e geração elétrica."@pt-br ,
                                 "Solid biomass energy comes from the combustion or processing of organic materials such as wood, forestry residues, and agricultural waste. It is one of the oldest forms of renewable energy, still widely used for heating and power generation."@en ;
                 skos:prefLabel "Biomassa Sólida"@pt-br ,
                                "Solid Biomass"@en .


###  https://w3id.org/energy-domain/edo#SolidLayer
edo:SolidLayer rdf:type owl:Class ;
               rdfs:subClassOf edo:FlexibleStructureLayer ;
               dcterms:identifier "SolidLayer" ;
               skos:definition "Camada maciça formada por extrusão contínua de um material"@pt-br ,
                               "Continuous layer used in subsea flexible pipes or similar structures, typically fabricated through extrusion. It provides structural reinforcement, pressure containment, or environmental protection, ensuring the integrity and performance of the pipe by offering consistent support or shielding."@en ;
               skos:prefLabel "Camada Sólida"@pt-br ,
                              "Solid Layer"@en .


###  https://w3id.org/energy-domain/edo#SolubilityCurveAttribute
edo:SolubilityCurveAttribute rdf:type owl:Class ;
                             rdfs:subClassOf edo:DomainAttribute ;
                             dcterms:accessRights "PUBLIC" ;
                             dcterms:identifier "SolubilityTable" ;
                             skos:definition "Provides data on the solubility of various substances in a material, used to evaluate how different fluids or gases dissolve into the structure. This information is essential for assessing material compatibility and predicting the effects of prolonged exposure to specific substances under operational conditions."@en ;
                             skos:prefLabel "Solubility Table (Specific for Polymeric Materials)"@en ,
                                            "Tabela de Solubilidade (Específica para Materiais Poliméricos)"@pt-br ;
                             edo:hasAttributeScope edo:TypeLevelAttribute .


###  https://w3id.org/energy-domain/edo#SolubilityTableColumn
edo:SolubilityTableColumn rdf:type owl:Class ;
                          rdfs:subClassOf edo:SolubilityCurveAttribute .


###  https://w3id.org/energy-domain/edo#SolubilityTable_MoleculeIdentifier
edo:SolubilityTable_MoleculeIdentifier rdf:type owl:Class ;
                                       rdfs:subClassOf edo:SolubilityTableColumn ;
                                       dcterms:accessRights "PUBLIC" ;
                                       dcterms:identifier "SolubilityTable_MoleculeIdentifier" ;
                                       skos:definition "Specifies the type of molecule. This property identifies the particular molecule involved, which is crucial for understanding the material's interaction with or response to different chemical substances."@en ,
                                                       "Tipo de Molécula (co2, h2s, ch4, h2o,…)"@pt-br ;
                                       skos:prefLabel "Identificador de Molécula"@pt-br ,
                                                      "Molecule Identifier"@en ;
                                       edo:hasAttributeScope edo:TypeLevelAttribute ;
                                       edo:hasLifecycleCreationPhase edo:DetailedDesign ;
                                       edo:hasTypedValue edo:StringValue ;
                                       edo:hasValueCardinality edo:MultiValue .


###  https://w3id.org/energy-domain/edo#SolubilityTable_PolymerState
edo:SolubilityTable_PolymerState rdf:type owl:Class ;
                                 rdfs:subClassOf edo:SolubilityTableColumn ;
                                 dcterms:accessRights "PUBLIC" ;
                                 dcterms:identifier "SolubilityTable_PolymerState" ;
                                 skos:definition "The state of the polymeric material is specified.. This property is crucial for understanding how the material behaves under different conditions and its suitability for various applications."@en ;
                                 skos:prefLabel "Estado do Polímero"@pt-br ,
                                                "Polymer State"@en ;
                                 edo:hasAttributeScope edo:TypeLevelAttribute ;
                                 edo:hasLifecycleCreationPhase edo:DetailedDesign ;
                                 edo:hasTypedValue edo:StringValue ;
                                 edo:hasValueCardinality edo:MultiValue .


###  https://w3id.org/energy-domain/edo#SolubilityTable_SolubilityCoefficient
edo:SolubilityTable_SolubilityCoefficient rdf:type owl:Class ;
                                          rdfs:subClassOf edo:SolubilityTableColumn ;
                                          dcterms:accessRights "PUBLIC" ;
                                          dcterms:identifier "SolubilityTable_SolubilityCoefficient" ;
                                          skos:definition "Represents the rate at which a substance dissolves in a specific material, indicating how much of the substance can be absorbed by the material. This property is important for understanding the material's chemical compatibility and behavior when exposed to various substances."@en ;
                                          skos:prefLabel "Coeficiente de solubilidade"@pt-br ,
                                                         "Solubility Coefficient"@en ;
                                          edo:hasAttributeScope edo:TypeLevelAttribute ;
                                          edo:hasLifecycleCreationPhase edo:DetailedDesign ;
                                          edo:hasTypedValue edo:FloatValue ;
                                          edo:hasUnit unit:MOL-PER-M3-PA ;
                                          edo:hasValueCardinality edo:MultiValue .


###  https://w3id.org/energy-domain/edo#SolubilityTable_Temperature
edo:SolubilityTable_Temperature rdf:type owl:Class ;
                                rdfs:subClassOf edo:SolubilityTableColumn ;
                                dcterms:accessRights "PUBLIC" ;
                                dcterms:identifier "SolubilityTable_Temperature" ;
                                skos:definition "Represents the thermal condition or measurement of heat for a component or system. This property is important for assessing how the component performs or operates under specific thermal conditions, ensuring it remains within safe and effective operating limits."@en ;
                                skos:prefLabel "Temperatura"@pt-br ,
                                               "Temperature"@en ;
                                edo:hasAttributeScope edo:TypeLevelAttribute ;
                                edo:hasLifecycleCreationPhase edo:DetailedDesign ;
                                edo:hasTypedValue edo:FloatValue ;
                                edo:hasUnit unit:K ;
                                edo:hasValueCardinality edo:MultiValue .


###  https://w3id.org/energy-domain/edo#SourcePigtailLength
edo:SourcePigtailLength rdf:type owl:Class ;
                        rdfs:subClassOf edo:DomainAttribute ;
                        dcterms:accessRights "PUBLIC" ;
                        dcterms:identifier "SourcePigtailLength" ;
                        skos:definition "Source end pigtail length"@en ;
                        skos:prefLabel "Source end pigtail length"@en ;
                        edo:hasAttributeScope edo:TypeLevelAttribute ;
                        edo:hasLifecycleCreationPhase edo:DetailedDesign ;
                        edo:hasTypedValue edo:FloatValue ;
                        edo:hasUnit unit:MilliM ;
                        edo:hasValueCardinality edo:SingleValue .


###  https://w3id.org/energy-domain/edo#SpareQuantity
edo:SpareQuantity rdf:type owl:Class ;
                  rdfs:subClassOf edo:DomainAttribute ;
                  dcterms:accessRights "PUBLIC" ;
                  dcterms:identifier "SpareQuantity" ;
                  skos:definition "Specifies the number of spare units available, ensuring adequate backup components are on hand for maintenance or replacement. This quantity helps in planning and minimizing downtime during operations."@en ;
                  skos:prefLabel "Quantidade de Sobressalentes"@pt-br ,
                                 "Spare Quantity"@en ;
                  edo:hasAttributeScope edo:InstanceLevelAttribute ;
                  edo:hasLifecycleCreationPhase edo:DetailedDesign ;
                  edo:hasTypedValue edo:IntValue ;
                  edo:hasValueCardinality edo:SingleValue .


###  https://w3id.org/energy-domain/edo#SpatialAttribute
edo:SpatialAttribute rdf:type owl:Class ;
                     rdfs:subClassOf edo:AttributeDomainCategory ;
                     rdfs:comment """Exemplos:
Location (geográfica, coordenada, planta, offshore, subsea, etc.)
Orientation (posição angular, direção)
Position (posição relativa dentro de um sistema)
Georeference (lat/long, UTM)
Installation site (onshore, offshore, módulo de planta)"""@pt-br .


###  https://w3id.org/energy-domain/edo#SpecialRequirements
edo:SpecialRequirements rdf:type owl:Class ;
                        rdfs:subClassOf edo:DomainAttribute ;
                        dcterms:accessRights "PUBLIC" ;
                        dcterms:identifier "SpecialRequirements" ;
                        skos:definition "Requisitos especiais, Observações ou Documentos especiais para o tramo"@pt-br ,
                                        "Special requirements refer to specific conditions, standards, or instructions that must be met during the design, manufacturing, installation, or operation of an object or system. These can include unique technical specifications, safety measures, regulatory compliance, or client-specific requests that go beyond standard procedures."@en ;
                        skos:prefLabel "Requisitos Especiais"@pt-br ,
                                       "Special Requirements"@en ;
                        edo:hasAttributeScope edo:InstanceLevelAttribute ;
                        edo:hasLifecycleCreationPhase edo:DetailedDesign ;
                        edo:hasTypedValue edo:StringValue ;
                        edo:hasValueCardinality edo:SingleValue .


###  https://w3id.org/energy-domain/edo#SpecificHeatCapacity
edo:SpecificHeatCapacity rdf:type owl:Class ;
                         rdfs:subClassOf edo:DomainAttribute ;
                         dcterms:accessRights "PUBLIC" ;
                         dcterms:identifier "SpecificHeatCapacity" ;
                         skos:definition "Calor Específico do material"@pt-br ,
                                         "Indicates the amount of heat required to raise the temperature of the material by a specific amount, typically measured per unit mass. This property is important for understanding the thermal behavior of the material.."@en ;
                         skos:prefLabel "Calor Específico"@pt-br ,
                                        "Specific Heat Capacity"@en ;
                         edo:hasAttributeScope edo:TypeLevelAttribute ;
                         edo:hasLifecycleCreationPhase edo:DetailedDesign ;
                         edo:hasTypedValue edo:FloatValue ;
                         edo:hasUnit unit:J-PER-KiloGM-K ;
                         edo:hasValueCardinality edo:SingleValue .


###  https://w3id.org/energy-domain/edo#SpecificMass
edo:SpecificMass rdf:type owl:Class ;
                 rdfs:subClassOf edo:DomainAttribute ;
                 dcterms:accessRights "PUBLIC" ;
                 dcterms:identifier "SpecificMass" ;
                 rdfs:comment "Massa específica equivalente"@pt-br ;
                 skos:definition "Equivalent specific mass"@en ;
                 skos:prefLabel "Equivalent specific mass"@en ,
                                "Massa específica equivalente"@pt-br ;
                 edo:hasAttributeScope edo:TypeLevelAttribute ;
                 edo:hasLifecycleCreationPhase edo:DetailedDesign ;
                 edo:hasTypedValue edo:FloatValue ;
                 edo:hasUnit unit:KiloGM-PER-M3 ;
                 edo:hasValueCardinality edo:SingleValue .


###  https://w3id.org/energy-domain/edo#SpecificWeight
edo:SpecificWeight rdf:type owl:Class ;
                   rdfs:subClassOf edo:DomainAttribute ;
                   dcterms:accessRights "PUBLIC" ;
                   dcterms:identifier "SpecificWeight" ;
                   skos:definition "Indicates the weight of the material per unit volume. This property is crucial for understanding the material's density and its impact on the overall weight."@en ,
                                   "Peso específico do material"@pt-br ;
                   skos:prefLabel "Peso Específico"@pt-br ,
                                  "Specific Weight"@en ;
                   edo:hasAttributeScope edo:TypeLevelAttribute ;
                   edo:hasLifecycleCreationPhase edo:DetailedDesign ;
                   edo:hasTypedValue edo:FloatValue ;
                   edo:hasUnit unit:N-PER-M3 ;
                   edo:hasValueCardinality edo:SingleValue .


###  https://w3id.org/energy-domain/edo#Specification
edo:Specification rdf:type owl:Class ;
                  rdfs:subClassOf edo:DomainElement ;
                  skos:definition "Representa uma especificação detalhada ou definição de projeto para um elemento de domínio, fornecendo requisitos, dimensões e normas para sua construção ou implementação."@pt-br ,
                                  "Represents a detailed specification or design definition for a domain element, providing requirements, dimensions, and standards for its construction or implementation."@en ;
                  skos:prefLabel "Especificação"@pt-br ,
                                 "Specification"@en .


###  https://w3id.org/energy-domain/edo#SpliceBox
edo:SpliceBox rdf:type owl:Class ;
              rdfs:subClassOf edo:ComponentDevice ;
              dcterms:identifier "SpliceBox" ;
              skos:prefLabel "Caixa de emenda"@pt-br ,
                             "Splice box"@en .


###  https://w3id.org/energy-domain/edo#SplitCollar
edo:SplitCollar rdf:type owl:Class ;
                rdfs:subClassOf edo:LineAncillary ;
                dcterms:identifier "SplitCollar" ;
                skos:definition "A component used to encircle and secure parts of subsea systems, such as flexible pipes, risers, or accessories. The Split Collar is designed with a split or gap, allowing it to be clamped around the pipe or component and then fastened together. This design facilitates easy installation and removal, making it useful for applications where adjustments or maintenance are required. The Split Collar provides structural support, alignment, and stability, ensuring that the connected components remain securely in place."@en ;
                skos:prefLabel "Colar Bipartido"@pt-br ,
                               "Split Collar"@en ;
                edo:hasAttribute edo:PipeMountPosition ,
                                 edo:WeightInWater .


###  https://w3id.org/energy-domain/edo#SpoolingTension
edo:SpoolingTension rdf:type owl:Class ;
                    rdfs:subClassOf edo:DomainAttribute ;
                    dcterms:accessRights "PUBLIC" ;
                    dcterms:identifier "SpoolingTension" ;
                    skos:definition "Represents the tension applied to a flexible component during the spooling process. This property is crucial for ensuring that the material is wound onto the reel or spool without exceeding its mechanical limits, preventing damage or deformation during handling and storage."@en ;
                    skos:prefLabel "Spooling Tension"@en ,
                                   "Tração de Desenrolamento"@pt-br ;
                    edo:hasAttributeScope edo:TypeLevelAttribute ;
                    edo:hasLifecycleCreationPhase edo:DetailedDesign ;
                    edo:hasTypedValue edo:FloatValue ;
                    edo:hasUnit unit:KiloN ,
                                unit:N ;
                    edo:hasValueCardinality edo:SingleValue .


###  https://w3id.org/energy-domain/edo#StandardType
edo:StandardType rdf:type owl:Class ;
                 rdfs:subClassOf edo:DomainAttribute ;
                 dcterms:accessRights "PUBLIC" ;
                 dcterms:identifier "StandardType" ;
                 skos:definition "Especifica o tipo de engate rápido conforme padronização Petrobras"@pt-br ,
                                 "Specifies the type of quick connect coupling as per Petrobras standardization"@en ;
                 skos:prefLabel "Quick connect coupling standard type"@en ,
                                "Tipo padronizado de engate rápido"@pt-br ;
                 edo:hasAttributeScope edo:TypeLevelAttribute ;
                 edo:hasLifecycleCreationPhase edo:DetailedDesign ;
                 edo:hasTypedValue edo:StringValue ;
                 edo:hasValueCardinality edo:SingleValue .


###  https://w3id.org/energy-domain/edo#StaticEquipmentEngineering
edo:StaticEquipmentEngineering rdf:type owl:Class ;
                               rdfs:subClassOf edo:EquipmentEngineering ;
                               rdfs:label "Engenharia de Equipamentos Estáticos"@pt-br ,
                                          "Static Equipment Engineering"@en ;
                               skos:definition "Engenharia de equipamentos industriais sem partes móveis como vasos de pressão, tanques e trocadores de calor."@pt-br ,
                                               "Engineering of non-moving industrial equipment such as pressure vessels, tanks, and heat exchangers."@en .


###  https://w3id.org/energy-domain/edo#StaticUmbilicalSpan
edo:StaticUmbilicalSpan rdf:type owl:Class ;
                        rdfs:subClassOf edo:IfcInstanciableElement ,
                                        edo:UmbilicalSpan ;
                        dcterms:identifier "StaticUmbilicalSpan" ;
                        skos:definition "Trecho de umbilical não suspenso, estendido sobre ou sob o solo"@pt-br ,
                                        "Unsuspended umbilical span, laid over or under ground"@en ;
                        skos:prefLabel "Static umbilical span"@en ,
                                       "Trecho estático de umbilical"@pt-br ;
                        edo:hasDiscipline edo:SubseaUmbilicalsEngineering .


###  https://w3id.org/energy-domain/edo#Status
edo:Status rdf:type owl:Class ;
           rdfs:subClassOf edo:ContentManagementAttribute .


###  https://w3id.org/energy-domain/edo#StdUmbilicalType
edo:StdUmbilicalType rdf:type owl:Class ;
                     rdfs:subClassOf edo:DomainAttribute ;
                     dcterms:accessRights "PUBLIC" ;
                     dcterms:identifier "StdUmbilicalType" ;
                     skos:definition "Standard umbilical type"@en ;
                     skos:prefLabel "Standard umbilical type"@en ,
                                    "Tipo padronizado de umbilical"@pt-br ;
                     edo:hasAttributeScope edo:TypeLevelAttribute ;
                     edo:hasLifecycleCreationPhase edo:DetailedDesign ;
                     edo:hasTypedValue edo:StringValue ;
                     edo:hasValueCardinality edo:SingleValue .


###  https://w3id.org/energy-domain/edo#StiffTorsionalStiffnessAtSeaLevel
edo:StiffTorsionalStiffnessAtSeaLevel rdf:type owl:Class ;
                                      rdfs:subClassOf edo:DomainAttribute ;
                                      dcterms:accessRights "PUBLIC" ;
                                      dcterms:identifier "StiffTorsionalStiffnessAtSeaLevel" ;
                                      skos:definition "Represents the torsional stiffness of a component when measured at sea level, indicating its resistance to twisting under applied torque. This property is important for ensuring that the component maintains its structural integrity and performance under rotational forces."@en ,
                                                      "Rigidez a torção (GJ) (maior valor) a 20°C e pressão atmosferica (dentro e fora)"@pt-br ;
                                      skos:prefLabel "Rigidez a Torção Rígida ao Nível do Mar"@pt-br ,
                                                     "Stiff Torsional Stiffness At Sea Level"@en ;
                                      edo:hasAttributeScope edo:TypeLevelAttribute ;
                                      edo:hasLifecycleCreationPhase edo:DetailedDesign ;
                                      edo:hasTypedValue edo:FloatValue ;
                                      edo:hasUnit unit:N-M2-PER-RAD ,
                                                  edo:N-M2-PER-RAD ;
                                      edo:hasValueCardinality edo:SingleValue .


###  https://w3id.org/energy-domain/edo#StopperCollar
edo:StopperCollar rdf:type owl:Class ;
                  rdfs:subClassOf edo:IfcInstanciableElement ,
                                  edo:SplitCollar ;
                  dcterms:identifier "StopperCollar" ;
                  skos:altLabel "Locking Collar"@en ,
                                "Positioning Collar"@en ,
                                "Retention Collar"@en ,
                                "Stopper Clamp"@en ,
                                "Stopping Collar"@en ;
                  skos:definition "A component used to prevent the movement or displacement of other parts in subsea systems. The Stopper Collar is installed around the pipe or component and acts as a physical barrier to stop or limit movement, ensuring components stay in their intended positions. It is crucial for maintaining alignment and stability during installation, operation, or maintenance, providing secure positioning and preventing unwanted shifts or displacements."@en ;
                  skos:prefLabel "Colar Batente"@pt-br ,
                                 "Stopper Collar"@en ;
                  edo:hasDiscipline edo:SubseaFlexiblePipesEngineering ,
                                    edo:SubseaUmbilicalsEngineering ;
                  edo:ifc_equivalentClass "IfcPipeFitting" ;
                  edo:ifc_objectType "StopperCollar" ;
                  edo:ifc_predefinedType "USERDEFINED" .


###  https://w3id.org/energy-domain/edo#StorageAccessory
edo:StorageAccessory rdf:type owl:Class ;
                     rdfs:subClassOf edo:Accessory ;
                     dcterms:identifier "StorageAccessory" ;
                     skos:prefLabel "Acessório de armazenamento/transporte"@pt-br ,
                                    "Storage/transportation accessory"@en .


###  https://w3id.org/energy-domain/edo#StorageBox
edo:StorageBox rdf:type owl:Class ;
               rdfs:subClassOf edo:StorageAccessory ;
               dcterms:identifier "StorageBox" ;
               skos:prefLabel "Caixa de armazenamento"@pt-br ,
                              "Storage box"@en .


###  https://w3id.org/energy-domain/edo#StorageSkid
edo:StorageSkid rdf:type owl:Class ;
                rdfs:subClassOf edo:StorageAccessory ;
                dcterms:identifier "StorageSkid" ;
                skos:definition "Estrutura de proteção para transporte e armazenamento de equipamentos"@pt-br ,
                                "Protective structure for equipment storage and transportation"@en ;
                skos:prefLabel "Skid de armazenamento"@pt-br ,
                               "Storage skid"@en .


###  https://w3id.org/energy-domain/edo#StorageSpool
edo:StorageSpool rdf:type owl:Class ;
                 rdfs:subClassOf edo:StorageAccessory ;
                 dcterms:identifier "StorageSpool" ;
                 skos:definition "Carretel/bobina para transporte e armazenamento de linhas"@pt-br ,
                                 "Spool for line storage and transportation"@en ;
                 skos:prefLabel "Carretel de armazenamento"@pt-br ,
                                "Storage spool"@en .


###  https://w3id.org/energy-domain/edo#StrIntOffPLevMaxPress
edo:StrIntOffPLevMaxPress rdf:type owl:Class ;
                          rdfs:subClassOf edo:HydrostaticPressureTestsAttribute ;
                          dcterms:accessRights "PUBLIC" ;
                          dcterms:identifier "StrIntOffPLevMaxPress" ;
                          skos:definition "Condições de teste dos tramos para Pressão - Máxima - Teste de integridade estrutural hidrostática (off-shore, no nível da plataforma)"@pt-br ,
                                          "The maximum pressure applied during the Structural Integrity Test (offshore, at platform level), ensuring structural integrity under extreme conditions."@en ;
                          skos:prefLabel "Integridade Estrutural Offshore com Pressão Máxima no Nível da Plataforma"@pt-br ,
                                         "Structural Integrity Offshore Leak Test At Platform Level Maximum Pressure"@en ;
                          edo:hasAttributeScope edo:InstanceLevelAttribute ;
                          edo:hasLifecycleCreationPhase edo:DetailedDesign ;
                          edo:hasTypedValue edo:FloatValue ;
                          edo:hasUnit unit:PA ;
                          edo:hasValueCardinality edo:SingleValue .


###  https://w3id.org/energy-domain/edo#StrIntOffPLevMaxPressValRef
edo:StrIntOffPLevMaxPressValRef rdf:type owl:Class ;
                                rdfs:subClassOf edo:HydrostaticPressureTestsAttribute ;
                                dcterms:accessRights "PUBLIC" ;
                                dcterms:identifier "StrIntOffPLevMaxPressValRef" ;
                                skos:definition "Comentários Condições de teste dos tramos para - Máximo - Teste de integridade estrutural hidrostática (off-shore, no nível da plataforma)"@pt-br ,
                                                "Specifies the reference pressure used to determine the Structural Offshore Maximum Pressure value."@en ;
                                skos:prefLabel "Referência de Valor de Pressão Máxima para Teste de Integridade Estrutural Offshore e de Vazamento no Nível da Plataforma"@pt-br ,
                                               "Structural Integrity Offshore Leak Test At Platform Level Maximum Pressure Value Reference"@en ;
                                edo:hasAttributeScope edo:InstanceLevelAttribute ;
                                edo:hasLifecycleCreationPhase edo:DetailedDesign ;
                                edo:hasTypedValue edo:StringValue ;
                                edo:hasValueCardinality edo:SingleValue .


###  https://w3id.org/energy-domain/edo#StrIntOffPLevMaxPressValRefMult
edo:StrIntOffPLevMaxPressValRefMult rdf:type owl:Class ;
                                    rdfs:subClassOf edo:HydrostaticPressureTestsAttribute ;
                                    dcterms:accessRights "PUBLIC" ;
                                    dcterms:identifier "StrIntOffPLevMaxPressValRefMult" ;
                                    skos:definition "The multiplier applied to the reference pressure to determine the Structural Offshore Maximum Pressure value."@en ;
                                    skos:prefLabel "Multiplicador de Referência de Valor de Pressão Máxima para Teste de Integridade Estrutural Offshore no Nível da Plataforma"@pt-br ,
                                                   "Structural Integrity Offshore Leak Test At Platform Level Maximum Pressure Value Reference Multiplier"@en ;
                                    edo:hasAttributeScope edo:InstanceLevelAttribute ;
                                    edo:hasLifecycleCreationPhase edo:DetailedDesign ;
                                    edo:hasTypedValue edo:FloatValue ;
                                    edo:hasValueCardinality edo:SingleValue .


###  https://w3id.org/energy-domain/edo#StrIntOffPLevNomPress
edo:StrIntOffPLevNomPress rdf:type owl:Class ;
                          rdfs:subClassOf edo:HydrostaticPressureTestsAttribute ;
                          dcterms:accessRights "PUBLIC" ;
                          dcterms:identifier "StrIntOffPLevNomPress" ;
                          skos:definition "Condições de teste dos tramos para Pressão - Nominal - Teste de integridade estrutural hidrostática (off-shore, no nível da plataforma)"@pt-br ,
                                          "The nominal pressure applied during the Structural Integrity Test (offshore, at platform level), simulating typical conditions to verify structural integrity."@en ;
                          skos:prefLabel "Integridade Estrutural Offshore com Pressão Nominal no Nível da Plataforma"@pt-br ,
                                         "Structural Integrity Offshore Leak Test At Platform Level Nominal Pressure"@en ;
                          edo:hasAttributeScope edo:InstanceLevelAttribute ;
                          edo:hasLifecycleCreationPhase edo:DetailedDesign ;
                          edo:hasTypedValue edo:FloatValue ;
                          edo:hasUnit unit:PA ;
                          edo:hasValueCardinality edo:SingleValue .


###  https://w3id.org/energy-domain/edo#StrIntOffPLevNomPressValRef
edo:StrIntOffPLevNomPressValRef rdf:type owl:Class ;
                                rdfs:subClassOf edo:HydrostaticPressureTestsAttribute ;
                                dcterms:accessRights "PUBLIC" ;
                                dcterms:identifier "StrIntOffPLevNomPressValRef" ;
                                skos:definition "Comentários Condições de teste dos tramos para - Nominal - Teste de integridade estrutural hidrostática (off-shore, no nível da plataforma)"@pt-br ,
                                                "Specifies the reference pressure used to determine the Structural Offshore Leak Test Nominal Pressure value."@en ;
                                skos:prefLabel "Referência de Valor de Pressão Nominal para Teste de Integridade Estrutural Offshore no Nível da Plataforma"@pt-br ,
                                               "Structural Integrity Offshore Leak Test At Platform Level Nominal Pressure Value Reference"@en ;
                                edo:hasAttributeScope edo:InstanceLevelAttribute ;
                                edo:hasLifecycleCreationPhase edo:DetailedDesign ;
                                edo:hasTypedValue edo:StringValue ;
                                edo:hasValueCardinality edo:SingleValue .


###  https://w3id.org/energy-domain/edo#StrIntOffPLevNomPressValRefMult
edo:StrIntOffPLevNomPressValRefMult rdf:type owl:Class ;
                                    rdfs:subClassOf edo:HydrostaticPressureTestsAttribute ;
                                    dcterms:accessRights "PUBLIC" ;
                                    dcterms:identifier "StrIntOffPLevNomPressValRefMult" ;
                                    skos:definition "The multiplier applied to the reference pressure to determine the Structural Offshore Nominal Pressure value."@en ;
                                    skos:prefLabel "Multiplicador de Referência de Valor de Pressão Nominal para Teste de Integridade Estrutural Offshore no Nível da Plataforma"@pt-br ,
                                                   "Structural Integrity Offshore Leak Test At Platform Level Nominal Pressure Value Reference Multiplier"@en ;
                                    edo:hasAttributeScope edo:InstanceLevelAttribute ;
                                    edo:hasLifecycleCreationPhase edo:DetailedDesign ;
                                    edo:hasTypedValue edo:FloatValue ;
                                    edo:hasValueCardinality edo:SingleValue .


###  https://w3id.org/energy-domain/edo#StrIntOnNoTensMaxPress
edo:StrIntOnNoTensMaxPress rdf:type owl:Class ;
                           rdfs:subClassOf edo:HydrostaticPressureTestsAttribute ;
                           dcterms:accessRights "PUBLIC" ;
                           dcterms:identifier "StrIntOnNoTensMaxPress" ;
                           skos:definition "Condições de teste dos tramos para Pressão - Máxima - Teste de integridade estrutural hidrostática (a bordo, sem tensão)"@pt-br ,
                                           "The maximum pressure applied during the Structural Integrity Test (onboard, without tension), verifying performance under extreme conditions."@en ;
                           skos:prefLabel "Integridade Estrutural a Bordo sem Pressão Máxima de Tensão"@pt-br ,
                                          "Structural Integrity Onboard With No Tension Maximum Pressure"@en ;
                           edo:hasAttributeScope edo:InstanceLevelAttribute ;
                           edo:hasLifecycleCreationPhase edo:DetailedDesign ;
                           edo:hasTypedValue edo:FloatValue ;
                           edo:hasUnit unit:PA ;
                           edo:hasValueCardinality edo:SingleValue .


###  https://w3id.org/energy-domain/edo#StrIntOnNoTensMaxPressValRef
edo:StrIntOnNoTensMaxPressValRef rdf:type owl:Class ;
                                 rdfs:subClassOf edo:HydrostaticPressureTestsAttribute ;
                                 dcterms:accessRights "PUBLIC" ;
                                 dcterms:identifier "StrIntOnNoTensMaxPressValRef" ;
                                 skos:definition "Comentários Condições de teste dos tramos para - Máximo - Teste de integridade estrutural hidrostática (a bordo, sem tensão)"@pt-br ,
                                                 "Specifies the reference pressure used to determine the Structural Onboard Maximum Pressure value."@en ;
                                 skos:prefLabel "Referência de Valor de Pressão Máxima para Integridade Estrutural a Bordo sem Tensão"@pt-br ,
                                                "Structural Integrity Onboard With No Tension Maximum Pressure Value Reference"@en ;
                                 edo:hasAttributeScope edo:InstanceLevelAttribute ;
                                 edo:hasLifecycleCreationPhase edo:DetailedDesign ;
                                 edo:hasTypedValue edo:StringValue ;
                                 edo:hasValueCardinality edo:SingleValue .


###  https://w3id.org/energy-domain/edo#StrIntOnNoTensMaxPressValRefMult
edo:StrIntOnNoTensMaxPressValRefMult rdf:type owl:Class ;
                                     rdfs:subClassOf edo:HydrostaticPressureTestsAttribute ;
                                     dcterms:accessRights "PUBLIC" ;
                                     dcterms:identifier "StrIntOnNoTensMaxPressValRefMult" ;
                                     skos:definition "The multiplier applied to the reference pressure to determine the Structural Onboard Maximum Pressure value."@en ;
                                     skos:prefLabel "Multiplicador de Referência de Valor de Pressão Máxima para Integridade Estrutural a Bordo sem Tensão"@pt-br ,
                                                    "Structural Integrity Onboard With No Tension Maximum Pressure Value Reference Multiplier"@en ;
                                     edo:hasAttributeScope edo:InstanceLevelAttribute ;
                                     edo:hasLifecycleCreationPhase edo:DetailedDesign ;
                                     edo:hasTypedValue edo:FloatValue ;
                                     edo:hasValueCardinality edo:SingleValue .


###  https://w3id.org/energy-domain/edo#StrIntOnNoTensNomPress
edo:StrIntOnNoTensNomPress rdf:type owl:Class ;
                           rdfs:subClassOf edo:HydrostaticPressureTestsAttribute ;
                           dcterms:accessRights "PUBLIC" ;
                           dcterms:identifier "StrIntOnNoTensNomPress" ;
                           skos:definition "Condições de teste dos tramos para Pressão - Nominal - Teste de integridade estrutural hidrostática (on-board, sem tensão)"@pt-br ,
                                           "The nominal pressure applied during the Structural Integrity Test (onboard, without tension), simulating typical conditions to verify structural integrity."@en ;
                           skos:prefLabel "Integridade Estrutural a Bordo sem Pressão Nominal de Tensão"@pt-br ,
                                          "Structural Integrity Onboard With No Tension Nominal Pressure"@en ;
                           edo:hasAttributeScope edo:InstanceLevelAttribute ;
                           edo:hasLifecycleCreationPhase edo:DetailedDesign ;
                           edo:hasTypedValue edo:FloatValue ;
                           edo:hasUnit unit:PA ;
                           edo:hasValueCardinality edo:SingleValue .


###  https://w3id.org/energy-domain/edo#StrIntOnNoTensNomPressValRef
edo:StrIntOnNoTensNomPressValRef rdf:type owl:Class ;
                                 rdfs:subClassOf edo:HydrostaticPressureTestsAttribute ;
                                 dcterms:accessRights "PUBLIC" ;
                                 dcterms:identifier "StrIntOnNoTensNomPressValRef" ;
                                 skos:definition "Comentários Condições de teste dos tramos para - Nominal - Teste de integridade estrutural hidrostática (on-board, sem tensão)"@pt-br ,
                                                 "Specifies the reference pressure used to determine the Structural Onboard Nominal Pressure value."@en ;
                                 skos:prefLabel "Integridade Estrutural a Bordo sem Referência de Valor de Pressão Nominal de Tensão"@pt-br ,
                                                "Structural Integrity Onboard With No Tension Nominal Pressure Value Reference"@en ;
                                 edo:hasAttributeScope edo:InstanceLevelAttribute ;
                                 edo:hasLifecycleCreationPhase edo:DetailedDesign ;
                                 edo:hasTypedValue edo:StringValue ;
                                 edo:hasValueCardinality edo:SingleValue .


###  https://w3id.org/energy-domain/edo#StrIntOnNoTensNomPressValRefMult
edo:StrIntOnNoTensNomPressValRefMult rdf:type owl:Class ;
                                     rdfs:subClassOf edo:HydrostaticPressureTestsAttribute ;
                                     dcterms:accessRights "PUBLIC" ;
                                     dcterms:identifier "StrIntOnNoTensNomPressValRefMult" ;
                                     skos:definition "The multiplier applied to the reference pressure to determine the Structural Onboard Nominal Pressure value."@en ;
                                     skos:prefLabel "Multiplicador de Referência de Valor de Pressão Nominal para Integridade Estrutural a Bordo sem Tensão"@pt-br ,
                                                    "Structural Integrity Onboard With No Tension Nominal Pressure Value Reference Multiplier"@en ;
                                     edo:hasAttributeScope edo:InstanceLevelAttribute ;
                                     edo:hasLifecycleCreationPhase edo:DetailedDesign ;
                                     edo:hasTypedValue edo:FloatValue ;
                                     edo:hasValueCardinality edo:SingleValue .


###  https://w3id.org/energy-domain/edo#StrandsTableAttribute
edo:StrandsTableAttribute rdf:type owl:Class ;
                          rdfs:subClassOf edo:DomainAttribute ;
                          dcterms:accessRights "PUBLIC" ;
                          dcterms:identifier "StrandsTableAttribute" ;
                          skos:definition "Provides detailed information about the mechanical and geometrical properties, including dimensions and material characteristics, necessary for understanding and evaluating the component's performance and suitability for its intended application."@en ;
                          skos:prefLabel "Strands Table"@en ,
                                         "Tabela de Propriedades das Cordoalhas"@pt-br ;
                          edo:hasAttributeScope edo:InstanceLevelAttribute .


###  https://w3id.org/energy-domain/edo#StrandsTableColumn
edo:StrandsTableColumn rdf:type owl:Class ;
                       rdfs:subClassOf edo:StrandsTableAttribute .


###  https://w3id.org/energy-domain/edo#StrandsTable_SpareQuantity
edo:StrandsTable_SpareQuantity rdf:type owl:Class ;
                               rdfs:subClassOf edo:StrandsTableColumn ;
                               dcterms:accessRights "PUBLIC" ;
                               dcterms:identifier "StrandsTable_SpareQuantity" ;
                               skos:definition "Specifies the number of spare units available, ensuring adequate backup components are on hand for maintenance or replacement. This quantity helps in planning and minimizing downtime during operations in subsea environments."@en ;
                               skos:prefLabel "Quantidade de Sobressalentes"@pt-br ,
                                              "Spare Quantity"@en ;
                               edo:hasAttributeScope edo:InstanceLevelAttribute ;
                               edo:hasLifecycleCreationPhase edo:DetailedDesign ;
                               edo:hasTypedValue edo:IntValue ;
                               edo:hasValueCardinality edo:MultiValue .


###  https://w3id.org/energy-domain/edo#StrandsTable_StrandsLength
edo:StrandsTable_StrandsLength rdf:type owl:Class ;
                               rdfs:subClassOf edo:StrandsTableColumn ;
                               dcterms:accessRights "PUBLIC" ;
                               dcterms:identifier "StrandsTable_StrandsLength" ;
                               skos:definition "Length of the individual strands."@en ;
                               skos:prefLabel "Comprimento das Cordoalhas"@pt-br ,
                                              "Strands Length"@en ;
                               edo:hasAttributeScope edo:InstanceLevelAttribute ;
                               edo:hasLifecycleCreationPhase edo:DetailedDesign ;
                               edo:hasTypedValue edo:FloatValue ;
                               edo:hasUnit unit:MilliM ;
                               edo:hasValueCardinality edo:MultiValue .


###  https://w3id.org/energy-domain/edo#StrandsTable_StrandsQuantity
edo:StrandsTable_StrandsQuantity rdf:type owl:Class ;
                                 rdfs:subClassOf edo:StrandsTableColumn ;
                                 dcterms:accessRights "PUBLIC" ;
                                 dcterms:identifier "StrandsTable_StrandsQuantity" ;
                                 skos:definition "Number of individual strands used, determining the overall reinforcement and strength of the component."@en ;
                                 skos:prefLabel "Quantidade de Cordoalhas"@pt-br ,
                                                "Strands Quantity"@en ;
                                 edo:hasAttributeScope edo:InstanceLevelAttribute ;
                                 edo:hasLifecycleCreationPhase edo:DetailedDesign ;
                                 edo:hasTypedValue edo:IntValue ;
                                 edo:hasValueCardinality edo:MultiValue .


###  https://w3id.org/energy-domain/edo#StressAtDesignPressure
edo:StressAtDesignPressure rdf:type owl:Class ;
                           rdfs:subClassOf edo:DomainAttribute ;
                           dcterms:accessRights "PUBLIC" ;
                           dcterms:identifier "StressAtDesignPressure" ;
                           skos:definition "Maximum stress that the material can withstand when subjected to design pressure is specified. This parameter is critical for ensuring that the material maintains its structural integrity and performs reliably under the operational pressure conditions specified in the design."@en ;
                           skos:prefLabel "Stress At Design Pressure"@en ,
                                          "Tensão na pressão de projeto"@pt-br ;
                           edo:hasAttributeScope edo:InstanceLevelAttribute ;
                           edo:hasLifecycleCreationPhase edo:DetailedDesign ;
                           edo:hasTypedValue edo:FloatValue ;
                           edo:hasUnit unit:PA ;
                           edo:hasValueCardinality edo:SingleValue .


###  https://w3id.org/energy-domain/edo#StringValue
edo:StringValue rdf:type owl:Class ;
                owl:equivalentClass [ rdf:type owl:Restriction ;
                                      owl:onProperty rdf:value ;
                                      owl:allValuesFrom xsd:string
                                    ] ;
                rdfs:subClassOf edo:DataType ;
                rdfs:comment "Constraint for xsd:string (character strings)"@en ;
                rdfs:label "String Value"@en .


###  https://w3id.org/energy-domain/edo#StructuralEngineering
edo:StructuralEngineering rdf:type owl:Class ;
                          rdfs:subClassOf edo:CivilEngineering ;
                          rdfs:label "Engenharia Estrutural"@pt-br ,
                                     "Structural Engineering"@en ;
                          skos:definition "Disciplina de engenharia focada na integridade estrutural e projeto de edifícios e infraestrutura."@pt-br ,
                                          "Engineering discipline focused on the structural integrity and design of buildings and infrastructure."@en .


###  https://w3id.org/energy-domain/edo#Structure
edo:Structure rdf:type owl:Class ;
              rdfs:subClassOf edo:CompactObject ;
              dcterms:identifier "Structure" ;
              skos:definition "Itens de grande porte mas não muito complexos, para uso permanente"@pt-br ,
                              "Large but not very complex items for permanent use"@en ;
              skos:prefLabel "Estrutura"@pt-br ,
                             "Structure"@en .


###  https://w3id.org/energy-domain/edo#StructureApplication
edo:StructureApplication rdf:type owl:Class ;
                         rdfs:subClassOf edo:DomainAttribute ;
                         dcterms:accessRights "PUBLIC" ;
                         dcterms:identifier "StructureApplication" ;
                         rdfs:comment "Especifica a aplicação para a qual a estrutura é projetada"@pt-br ;
                         skos:definition "Especifica a aplicação para a qual a estrutura é projetada"@pt-br ,
                                         "Specifies application for which structure is designed"@en ;
                         skos:prefLabel "Aplicação da estrutura"@pt-br ,
                                        "Structure application"@en ;
                         edo:hasAttributeScope edo:TypeLevelAttribute ;
                         edo:hasLifecycleCreationPhase edo:DetailedDesign ;
                         edo:hasTypedValue edo:StringValue ;
                         edo:hasValueCardinality edo:SingleValue .


###  https://w3id.org/energy-domain/edo#StructureApplicationsList
edo:StructureApplicationsList rdf:type owl:Class ;
                              rdfs:subClassOf edo:DomainAttribute ;
                              dcterms:accessRights "PUBLIC" ;
                              dcterms:identifier "StructureApplicationsList" ;
                              skos:definition "Indicates the possible positions where the structure can be applied along the pipeline system. Multiple values can be selected to show in which sections, such as different parts of a riser or flowline, the structure is suitable for use."@en ,
                                              "Lista de todas as possíveis aplicações para a estrutura Valores aplicáveis (Mais de um valor pode ser escolhido): R (Riser) RT (Para seção de topo do riser) RI (Para seção intermediaria do riser) RF (Para seção de fundo do riser) F (Para Flowline)"@pt-br ;
                              skos:prefLabel "Lista de Aplicações da Estrutura"@pt-br ,
                                             "Structure Applications List"@en ;
                              edo:hasAttributeScope edo:TypeLevelAttribute ;
                              edo:hasLifecycleCreationPhase edo:DetailedDesign ;
                              edo:hasTypedValue edo:StringValue ;
                              edo:hasValueCardinality edo:MultiValue .


###  https://w3id.org/energy-domain/edo#StructureCode
edo:StructureCode rdf:type owl:Class ;
                  rdfs:subClassOf edo:DomainAttribute ;
                  dcterms:accessRights "PUBLIC" ;
                  dcterms:identifier "StructureCode" ;
                  skos:definition "Indicates the code or identifier assigned to the structure. This property is used to uniquely identify and reference the structure within a system, ensuring proper tracking, documentation, and management."@en ;
                  skos:prefLabel "Código da estrutura"@pt-br ,
                                 "Structure Code"@en ;
                  edo:hasAttributeScope edo:TypeLevelAttribute ;
                  edo:hasLifecycleCreationPhase edo:DetailedDesign ;
                  edo:hasTypedValue edo:StringValue ;
                  edo:hasValueCardinality edo:SingleValue .


###  https://w3id.org/energy-domain/edo#StudSet
edo:StudSet rdf:type owl:Class ;
            rdfs:subClassOf edo:PhysicalConnection ;
            dcterms:identifier "StudSet" ;
            skos:altLabel "Stud"@en ,
                          "Threaded Rod"@en ;
            skos:definition "Stud sets are essential fastening components used in subsea oil and gas interconnection end fittings to securely assemble and connect various parts of the equipment. Each set typically includes bolts, nuts, and washers, all made from high-strength, corrosion-resistant materials to endure the harsh subsea environment. These components are designed to provide reliable mechanical fastening, ensuring the structural integrity and leak-proof performance of the end fittings. The stud sets are carefully engineered to withstand high pressure and extreme temperatures, making them critical for maintaining the operational safety and longevity of subsea interconnections."@en ;
            skos:prefLabel "Estojos"@pt-br ,
                           "Stud Set"@en ;
            edo:hasAttribute edo:AssemblyTorque ,
                             edo:FullyThreaded ,
                             edo:Lubricant ,
                             edo:LubricantFrictionFactor ,
                             edo:NominalDiameter ,
                             edo:Quantity ,
                             edo:SpareQuantity .


###  https://w3id.org/energy-domain/edo#SubProjectId
edo:SubProjectId rdf:type owl:Class ;
                 rdfs:subClassOf edo:DomainAttribute ;
                 dcterms:accessRights "PUBLIC" ;
                 dcterms:identifier "SubProjectId" ;
                 skos:definition "Refers to the identification code assigned to the well or piece of equipment for which the interconnection is being designed. This code is often provisional, used during the initial stages of development, such as during the fabrication or installation of flexible pipelines, before a final approval or designation is granted. It serves as a reference point for all equipment and documentation until the well or equipment receives its definitive identification from the relevant regulatory authority. Examples include codes like LL-S.P6, LL-S.MSIAG1, or simpler identifiers such as P6 or MSIAG1."@en ;
                 skos:prefLabel "Id do Subprojeto"@pt-br ,
                                "Sub Project Id"@en ;
                 edo:hasAttributeScope edo:InstanceLevelAttribute ;
                 edo:hasLifecycleCreationPhase edo:BasicDesign ;
                 edo:hasTypedValue edo:StringValue ;
                 edo:hasValueCardinality edo:SingleValue .


###  https://w3id.org/energy-domain/edo#SubseaConnectionPoint
edo:SubseaConnectionPoint rdf:type owl:Class ;
                          rdfs:subClassOf edo:ConnectionPoint ,
                                          edo:IfcInstanciableElement ;
                          dcterms:identifier "SubseaConnectionPoint" ;
                          skos:definition "Representa um ponto de conexão localizado em ambientes submarinos, usado para ligar componentes submarinos."@pt-br ,
                                          "Represents a connection point located in subsea environments, used to link subsea components."@en ;
                          skos:prefLabel "Ponto de Conexão Submarino"@pt-br ,
                                         "Subsea Connection Point"@en ;
                          edo:hasDiscipline edo:SubseaUmbilicalsEngineering ;
                          edo:ifc_equivalentClass "IfcPipeFitting" ;
                          edo:ifc_objectType "SubseaConnectionPoint" ;
                          edo:ifc_predefinedType "USERDEFINED" .


###  https://w3id.org/energy-domain/edo#SubseaEngineering
edo:SubseaEngineering rdf:type owl:Class ;
                      rdfs:subClassOf edo:TechnicalDiscipline ;
                      rdfs:label "Engenharia Submarina"@pt-br ,
                                 "Subsea Engineering"@en ;
                      skos:definition "Disciplina de engenharia focada em sistemas e equipamentos subaquáticos para operações offshore."@pt-br ,
                                      "Engineering discipline focused on underwater systems and equipment for offshore operations."@en .


###  https://w3id.org/energy-domain/edo#SubseaEquipment
edo:SubseaEquipment rdf:type owl:Class ;
                    rdfs:subClassOf edo:Equipment ;
                    dcterms:identifier "SubseaEquipment" ;
                    skos:definition "Complex equipment for subsea use"@en ,
                                    "Equipamentos complexos para uso submarino"@pt-br ;
                    skos:prefLabel "Equipamento Submarino"@pt-br ,
                                   "Subsea Equipment"@en ;
                    edo:hasAttribute edo:MaxDepth ,
                                     edo:WeightInWater .


###  https://w3id.org/energy-domain/edo#SubseaFlexiblePipesBsddDictionary
edo:SubseaFlexiblePipesBsddDictionary rdf:type owl:Class ;
                                      rdfs:subClassOf edo:BsddDataDictionary ;
                                      dcterms:identifier "SubseaFlexiblePipesBsddDictionary" ;
                                      skos:definition "Bsdd Dictionary of Subsea Flexible Pipelines."@en ;
                                      skos:prefLabel "Dicionário Bsdd de Dutos Flexíveis Submarinos"@pt-br ,
                                                     "Subsea Flexible Pipes Bsdd Dictionary"@en ;
                                      edo:ifc_equivalentClass "IfcClassification" ;
                                      edo:ifc_objectType "SubseaFlexiblePipesBsddDictionary" ;
                                      edo:ifc_predefinedType "USERDEFINED" .


###  https://w3id.org/energy-domain/edo#SubseaFlexiblePipesEngineering
edo:SubseaFlexiblePipesEngineering rdf:type owl:Class ;
                                   rdfs:subClassOf edo:SubseaEngineering ;
                                   rdfs:label "Engenharia de Tubos Flexíveis Submarinos"@pt-br ,
                                              "Subsea Flexible Pipes Engineering"@en ;
                                   skos:definition "Engenharia de sistemas de tubos flexíveis utilizados em aplicações submarinas."@pt-br ,
                                                   "Engineering of flexible pipe systems used in subsea applications."@en .


###  https://w3id.org/energy-domain/edo#SubseaLayout
edo:SubseaLayout rdf:type owl:Class ;
                 rdfs:subClassOf edo:Location ;
                 dcterms:identifier "SubseaLayout" ;
                 skos:definition "The arrangement or map of components and systems within a subsea environment, including pipelines, risers, manifolds, and other infrastructure."@en ;
                 skos:prefLabel "Arranjo Submarino"@pt-br ,
                                "Subsea Layout"@en .


###  https://w3id.org/energy-domain/edo#SubseaManifoldsEngineering
edo:SubseaManifoldsEngineering rdf:type owl:Class ;
                               rdfs:subClassOf edo:SubseaEngineering .


###  https://w3id.org/energy-domain/edo#SubseaOilField
edo:SubseaOilField rdf:type owl:Class ;
                   rdfs:subClassOf edo:IfcInstanciableElement ,
                                   edo:SubseaLayout ;
                   dcterms:identifier "SubseaOilField" ;
                   skos:altLabel "Subsea Hydrocarbon Field"@en ,
                                 "Subsea Oil Reservoir"@en ,
                                 "Subsea Oil Site"@en ,
                                 "Subsea Petroleum Field"@en ;
                   skos:definition "A subsea oil field refers to an underwater reservoir of hydrocarbons located beneath the seabed. It involves the extraction of oil and gas from deposits situated in deepwater or shallow marine environments. The subsea oil field includes a range of equipment and infrastructure, such as subsea wells, pipelines, and production systems, all designed to safely and efficiently extract and transport hydrocarbons to processing facilities on the surface or shore. The development and operation of subsea oil fields require specialized technology and expertise to manage the challenges of deepwater environments and ensure the successful production and handling of resources."@en ;
                   skos:prefLabel "Campo de Petróleo Submarino"@pt-br ,
                                  "Subsea Oil Field"@en ;
                   edo:hasDiscipline edo:SubseaUmbilicalsEngineering ;
                   edo:ifc_equivalentClass "IfcSite" ;
                   edo:ifc_objectType "SubseaOilField" .


###  https://w3id.org/energy-domain/edo#SubseaPipeline
edo:SubseaPipeline rdf:type owl:Class ;
                   rdfs:subClassOf edo:IfcInstanciableElement ,
                                   edo:Interconnection ;
                   dcterms:identifier "SubseaPipeline" ;
                   skos:definition "A Subsea Pipeline is a conduit installed on the seafloor designed to transport oil, gas, or other fluids from underwater production facilities to processing or storage locations on the surface or shore. Engineered to withstand harsh underwater conditions, including high pressures, corrosive environments, and dynamic movements, the Subsea Pipeline is constructed with durable materials and advanced technologies to ensure reliable and efficient fluid transfer."@en ;
                   skos:prefLabel "Linha Submarina"@pt-br ,
                                  "Subsea Pipeline"@en ;
                   edo:hasAttribute edo:BasicProjectRevision ,
                                    edo:CO2VolumePercentage ,
                                    edo:ExecutiveProjectRevision ,
                                    edo:H2SVolumeConcentration ,
                                    edo:InternalDiameter ,
                                    edo:InternalIncidentalPressureCurveAttribute ,
                                    edo:MaterialRequest ,
                                    edo:MaterialRequestRev ,
                                    edo:MaxDesignAbsIntPresTable ,
                                    edo:MaxDesignAbsIntPresTable_PositionReference ,
                                    edo:MaxDesignAbsIntPresTable_Pressure ,
                                    edo:MaxDesignAbsIntPresTable_VPosWRTWaterline ,
                                    edo:MaximumTemperature ,
                                    edo:MaximumThermalExchangeCoefficient ,
                                    edo:MinimumThermalExchangeCoefficient ,
                                    edo:NominalLength ,
                                    edo:ProjectAcronym ,
                                    edo:ProjectCode ,
                                    edo:RiserConfiguration ,
                                    edo:Service ,
                                    edo:SubProjectId ,
                                    edo:UnifilarDiagram ,
                                    edo:UnifilarDiagramRev ;
                   edo:hasDiscipline edo:SubseaFlexiblePipesEngineering ;
                   edo:ifc_equivalentClass "IfcBuilding" ;
                   edo:ifc_objectType "SubseaPipeline" ;
                   edo:ifc_predefinedType "USERDEFINED" .


###  https://w3id.org/energy-domain/edo#SubseaRigidPipeSpec
edo:SubseaRigidPipeSpec rdf:type owl:Class ;
                        rdfs:subClassOf edo:Specification ;
                        skos:definition "Representa a especificação para dutos rígidos submarinos, definindo materiais, propriedades mecânicas, dimensões e requisitos de instalação."@pt-br ,
                                        "Represents the specification for subsea rigid pipes, defining materials, mechanical properties, dimensions, and installation requirements."@en ;
                        skos:prefLabel "Especificação de Tubo Rígido Submarino"@pt-br ,
                                       "Subsea Rigid Pipe Specification"@en .


###  https://w3id.org/energy-domain/edo#SubseaRigidPipesEngineering
edo:SubseaRigidPipesEngineering rdf:type owl:Class ;
                                rdfs:subClassOf edo:SubseaEngineering ;
                                rdfs:label "Engenharia de Tubos Rígidos Submarinos"@pt-br ,
                                           "Subsea Rigid Pipes Engineering"@en ;
                                skos:definition "Engenharia de sistemas de tubulações rígidas utilizadas em aplicações submarinas."@pt-br ,
                                                "Engineering of rigid pipeline systems used in subsea applications."@en .


###  https://w3id.org/energy-domain/edo#SubseaStructuresEngineering
edo:SubseaStructuresEngineering rdf:type owl:Class ;
                                rdfs:subClassOf edo:SubseaEngineering ;
                                rdfs:label "Engenharia de Estruturas Submarinas"@pt-br ,
                                           "Subsea Structures Engineering"@en ;
                                skos:definition "Engenharia de manifolds submarinos, árvores de natal e outros componentes estruturais."@pt-br ,
                                                "Engineering of subsea manifolds, christmas trees, and other structural components."@en .


###  https://w3id.org/energy-domain/edo#SubseaUmbilical
edo:SubseaUmbilical rdf:type owl:Class ;
                    rdfs:subClassOf edo:IfcInstanciableElement ,
                                    edo:Interconnection ;
                    dcterms:identifier "SubseaUmbilical" ;
                    skos:definition "A Subsea Umbilical is a composite cable system installed on the seafloor that provides vital control, power, and communication connections between topside facilities and subsea production systems. Designed to transmit hydraulic fluids, electrical power, and data signals, the Subsea Umbilical enables the remote operation and monitoring of subsea equipment such as valves, manifolds, and control modules. Engineered for long-term reliability in extreme underwater environments, it is constructed using multiple layers of protective sheathing, armoring, and insulation materials to resist mechanical stress, corrosion, and hydrostatic pressure, ensuring safe and continuous operation throughout the field’s lifecycle."@en ;
                    skos:prefLabel "Subsea Umbilical"@en ,
                                   "Umbilical Submarino"@pt-br ;
                    edo:hasAttribute edo:BasicProjectRevision ,
                                     edo:CO2VolumePercentage ,
                                     edo:ExecutiveProjectRevision ,
                                     edo:H2SVolumeConcentration ,
                                     edo:InternalDiameter ,
                                     edo:InternalIncidentalPressureTableColumn ,
                                     edo:MaterialRequest ,
                                     edo:MaterialRequestRev ,
                                     edo:MaxDesignAbsIntPresTableColumn ,
                                     edo:MaximumTemperature ,
                                     edo:MaximumThermalExchangeCoefficient ,
                                     edo:MinimumThermalExchangeCoefficient ,
                                     edo:NominalLength ,
                                     edo:ProjectAcronym ,
                                     edo:ProjectCode ,
                                     edo:RiserConfiguration ,
                                     edo:Service ,
                                     edo:SubProjectId ,
                                     edo:UnifilarDiagram ,
                                     edo:UnifilarDiagramRev ;
                    edo:hasDiscipline edo:SubseaUmbilicalsEngineering ;
                    edo:ifc_equivalentClass "IfcBuilding" ;
                    edo:ifc_objectType "SubseaUmbilical" ;
                    edo:ifc_predefinedType "USERDEFINED" .


###  https://w3id.org/energy-domain/edo#SubseaUmbilicalBsddDictionary
edo:SubseaUmbilicalBsddDictionary rdf:type owl:Class ;
                                  rdfs:subClassOf edo:BsddDataDictionary ;
                                  dcterms:identifier "SubseaUmbilicalBsddDictionary" ;
                                  skos:definition "Bsdd Dictionary of Subsea Flexible Pipelines."@en ;
                                  skos:prefLabel "Dicionário Bsdd de Umbilicais Submarinos"@pt-br ,
                                                 "Subsea Umbilical Bsdd Dictionary"@en ;
                                  edo:ifc_equivalentClass "IfcClassification" ;
                                  edo:ifc_objectType "SubseaUmbilicalBsddDictionary" ;
                                  edo:ifc_predefinedType "USERDEFINED" .


###  https://w3id.org/energy-domain/edo#SubseaUmbilicalsEngineering
edo:SubseaUmbilicalsEngineering rdf:type owl:Class ;
                                rdfs:subClassOf edo:SubseaEngineering ;
                                rdfs:label "Engenharia de Umbilicais Submarinos"@pt-br ,
                                           "Subsea Umbilicals Engineering"@en ;
                                skos:definition "Engenharia de sistemas de umbilicais submarinos fornecendo controle, energia e injeção química."@pt-br ,
                                                "Engineering of subsea umbilical systems providing control, power and chemical injection."@en .


###  https://w3id.org/energy-domain/edo#SubseaWell
edo:SubseaWell rdf:type owl:Class ;
               rdfs:subClassOf edo:EquipmentLocation ,
                               edo:IfcInstanciableElement ;
               dcterms:identifier "SubseaWell" ;
               skos:definition "A Subsea Well is a well located on the seafloor from which hydrocarbons such as oil and gas are extracted. Positioned underwater, it typically involves a wellhead assembly that includes valves, controls, and monitoring equipment to manage the extraction process. The Subsea Well is connected to surface facilities via pipelines and umbilicals, which facilitate the transport of extracted resources and the provision of necessary services like power and communication. Designed to operate under high pressure and harsh marine conditions, the subsea well is a critical component of offshore oil and gas production systems."@en ;
               skos:prefLabel "Poço"@pt-br ,
                              "Subsea Well"@en ;
               edo:hasDiscipline edo:SubseaUmbilicalsEngineering ;
               edo:ifc_equivalentClass "IfcBuilding" ;
               edo:ifc_objectType "SubseaWell" ;
               edo:ifc_predefinedType "USERDEFINED" .


###  https://w3id.org/energy-domain/edo#SuctionPile
edo:SuctionPile rdf:type owl:Class ;
                rdfs:subClassOf edo:Pile ;
                dcterms:identifier "SuctionPile" ;
                skos:definition "Anchoring pile driven into seabed by hydrostatic pressure, by applying suction to an underside cavity"@en ,
                                "Estaca de ancoragem cravada no solo pela pressão hidrostática, mediante aplicação de sucção a uma cavidade em seu lado inferior"@pt-br ;
                skos:prefLabel "Estaca de sucção"@pt-br ,
                               "Suction pile"@en .


###  https://w3id.org/energy-domain/edo#SupplierProvidedMaterialName
edo:SupplierProvidedMaterialName rdf:type owl:Class ;
                                 rdfs:subClassOf edo:MaterialManufacturerAttribute ;
                                 dcterms:accessRights "PUBLIC" ;
                                 dcterms:identifier "SupplierProvidedMaterialName" ;
                                 skos:definition "Name of the material as specified by the original supplier. This property identifies the exact material provided, ensuring it aligns with the required specifications for the accessory."@en ;
                                 skos:prefLabel "Nome do material conforme designado pelo fornecedor original do material"@pt-br ,
                                                "Supplier Provided Material Name"@en ;
                                 edo:hasAttributeScope edo:TypeLevelAttribute ;
                                 edo:hasLifecycleCreationPhase edo:DetailedDesign ;
                                 edo:hasTypedValue edo:StringValue ;
                                 edo:hasValueCardinality edo:SingleValue .


###  https://w3id.org/energy-domain/edo#SupportPoint
edo:SupportPoint rdf:type owl:Class ;
                 rdfs:subClassOf edo:LogicalElement ;
                 dcterms:identifier "SupportPoint" ;
                 skos:definition "Representa um ponto utilizado para apoiar, levantar ou posicionar elementos dentro de um projeto."@pt-br ,
                                 "Represents a point used to support, lift, or position elements within a project."@en ;
                 skos:prefLabel "Ponto de Apoio"@pt-br ,
                                "Support Point"@en .


###  https://w3id.org/energy-domain/edo#SupportRegion
edo:SupportRegion rdf:type owl:Class ;
                  rdfs:subClassOf edo:SupportPoint ;
                  dcterms:identifier "SupportRegion" ;
                  skos:definition "A specific region used to define the support location of the components within a 3D model."@en ,
                                  "Uma região específica usada para definir a localização de suporte dos componentes dentro de um modelo 3D."@pt-br ;
                  skos:prefLabel "Região de suporte no Modelo"@pt-br ,
                                 "Support Region"@en ;
                  edo:hasAttribute edo:CntrPntDstnceFrmTermFlange ,
                                   edo:SafeWorkingLoad ,
                                   edo:SupportRegionDiameter ,
                                   edo:SupportRegionMinimumArea ,
                                   edo:SupportSurfaceDiameter ,
                                   edo:SupportSurfaceFilletRadius ,
                                   edo:TechnicalNotes .


###  https://w3id.org/energy-domain/edo#SupportRegionDiameter
edo:SupportRegionDiameter rdf:type owl:Class ;
                          rdfs:subClassOf edo:DomainAttribute ;
                          dcterms:accessRights "PUBLIC" ;
                          dcterms:identifier "SupportRegionDiameter" ;
                          skos:definition "Especifica o diâmetro do componente na região onde o apoio é definido. Essa medição é essencial para garantir o alinhamento e o encaixe corretos entre a região de apoio e o componente ou equipamento de instalação associado"@pt-br ,
                                          "Specifies the diameter of the component at the location where the support region is defined. This measurement is crucial to ensure proper alignment and fit between the support region and the interfacing component or installation equipment"@en ;
                          skos:prefLabel "Diâmetro da Região de Apoio"@pt-br ,
                                         "Support Region Diameter"@en ;
                          edo:hasAttributeScope edo:InstanceLevelAttribute ;
                          edo:hasLifecycleCreationPhase edo:DetailedDesign ;
                          edo:hasTypedValue edo:FloatValue ;
                          edo:hasUnit unit:M ;
                          edo:hasValueCardinality edo:SingleValue .


###  https://w3id.org/energy-domain/edo#SupportRegionMinimumArea
edo:SupportRegionMinimumArea rdf:type owl:Class ;
                             rdfs:subClassOf edo:DomainAttribute ;
                             dcterms:accessRights "PUBLIC" ;
                             dcterms:identifier "SupportRegionMinimumArea" ;
                             skos:definition "Define a área mínima necessária da superfície de apoio para garantir estabilidade e adequada distribuição de carga. Assegura que a região de apoio suporte os esforços operacionais e evite desalinhamento ou deslizamento."@pt-br ,
                                             "Defines the minimum required area of the support surface necessary to provide adequate stability and load distribution. Ensures that the support region can sustain operational stresses and prevent misalignment or slippage."@en ;
                             skos:prefLabel "Minimum Support Area"@en ,
                                            "Área Mínima de Apoio"@pt-br ;
                             edo:hasAttributeScope edo:InstanceLevelAttribute ;
                             edo:hasLifecycleCreationPhase edo:DetailedDesign ;
                             edo:hasTypedValue edo:FloatValue ;
                             edo:hasUnit unit:M2 ;
                             edo:hasValueCardinality edo:SingleValue .


###  https://w3id.org/energy-domain/edo#SupportSurfaceDiameter
edo:SupportSurfaceDiameter rdf:type owl:Class ;
                           rdfs:subClassOf edo:DomainAttribute ;
                           dcterms:accessRights "PUBLIC" ;
                           dcterms:identifier "SupportSurfaceDiameter" ;
                           skos:definition "Indica o diâmetro da superfície de contato dentro da região de apoio. Essa medição garante que a interface proporcione área de contato suficiente para transferência de carga e conexão estável entre componentes adjacentes."@pt-br ,
                                           "Indicates the diameter of the contact surface within the support region. This measurement ensures that the interface provides sufficient contact area for load transfer and a stable connection between adjacent components."@en ;
                           skos:prefLabel "Diâmetro da superfície de apoio"@pt-br ,
                                          "Support Surface Diameter"@en ;
                           edo:hasAttributeScope edo:InstanceLevelAttribute ;
                           edo:hasLifecycleCreationPhase edo:DetailedDesign ;
                           edo:hasTypedValue edo:FloatValue ;
                           edo:hasUnit unit:M ;
                           edo:hasValueCardinality edo:SingleValue .


###  https://w3id.org/energy-domain/edo#SupportSurfaceFilletRadius
edo:SupportSurfaceFilletRadius rdf:type owl:Class ;
                               rdfs:subClassOf edo:DomainAttribute ;
                               dcterms:accessRights "PUBLIC" ;
                               dcterms:identifier "SupportSurfaceFilletRadius" ;
                               skos:definition "Representa o raio do chanfro ou transição arredondada na borda da superfície de apoio. Um raio adequado reduz a concentração de tensões, melhorando a integridade estrutural e a resistência à fadiga do componente."@pt-br ,
                                               "Represents the radius of the fillet or rounded transition at the edge of the support surface. A proper fillet radius reduces stress concentration, improving the structural integrity and fatigue resistance of the component."@en ;
                               skos:prefLabel "Raio de Chanframento da Superfície de Apoio"@pt-br ,
                                              "Support Surface Fillet Radius"@en ;
                               edo:hasAttributeScope edo:InstanceLevelAttribute ;
                               edo:hasLifecycleCreationPhase edo:DetailedDesign ;
                               edo:hasTypedValue edo:FloatValue ;
                               edo:hasUnit unit:M ;
                               edo:hasValueCardinality edo:SingleValue .


###  https://w3id.org/energy-domain/edo#SurfaceEquipment
edo:SurfaceEquipment rdf:type owl:Class ;
                     rdfs:subClassOf edo:Equipment ;
                     dcterms:identifier "SurfaceEquipment" ;
                     skos:prefLabel "Equipamento de Superfície"@pt-br ,
                                    "Surface Equipment"@en .


###  https://w3id.org/energy-domain/edo#TPT
edo:TPT rdf:type owl:Class ;
        rdfs:subClassOf edo:Sensor ;
        dcterms:identifier "TPT" ;
        skos:prefLabel "Pressure and temperature sensor"@en ,
                       "Sensor de pressão e temperatura"@pt-br .


###  https://w3id.org/energy-domain/edo#Table
edo:Table rdf:type owl:Class ;
          rdfs:subClassOf edo:ValueNature ;
          rdfs:comment "A table composed by columns (lists of values)"@en ,
                       "Uma tabela composta por colunas (listas de valores)"@en ;
          rdfs:label "Tabela"@pt-br ,
                     "Table"@en .


###  https://w3id.org/energy-domain/edo#TableColumn
edo:TableColumn rdf:type owl:Class ;
                rdfs:subClassOf edo:ValueNature ;
                rdfs:comment "A column of a table"@en ,
                             "Uma coluna de uma tabela"@pt-br ;
                rdfs:label "Coluna de tabela"@pt-br ,
                           "Table Column"@en .


###  https://w3id.org/energy-domain/edo#TapeLayer
edo:TapeLayer rdf:type owl:Class ;
              rdfs:subClassOf edo:WoundLayer ;
              dcterms:identifier "TapeLayer" ;
              skos:definition "A layer within the structure of a subsea flexible pipe composed of tape-like materials. This layer is designed to provide additional reinforcement and protection. Typically made from high-strength polymers or other durable materials, the tape layer contributes to the pipe’s overall flexibility, structural integrity, and resistance to external environmental factors. Engineered for harsh underwater conditions, it helps maintain the performance and durability of the flexible pipe system."@en ;
              skos:prefLabel "Camada de Fita"@pt-br ,
                             "Tape Layer"@en .


###  https://w3id.org/energy-domain/edo#TapesQuantity
edo:TapesQuantity rdf:type owl:Class ;
                  rdfs:subClassOf edo:DomainAttribute ;
                  dcterms:accessRights "PUBLIC" ;
                  dcterms:identifier "TapesQuantity" ;
                  skos:definition "Number of tapes applied within the structure, influencing factors such as insulation, protection, and reinforcement. "@en ;
                  skos:prefLabel "Quantidade de fitas"@pt-br ,
                                 "Tapes Quantity"@en ;
                  edo:hasAttributeScope edo:InstanceLevelAttribute ;
                  edo:hasLifecycleCreationPhase edo:DetailedDesign ;
                  edo:hasTypedValue edo:IntValue ;
                  edo:hasValueCardinality edo:SingleValue .


###  https://w3id.org/energy-domain/edo#TechnicalDiscipline
edo:TechnicalDiscipline rdf:type owl:Class ;
                        rdfs:subClassOf edo:ElementClassification ;
                        rdfs:comment "Superclass for all technical engineering disciplines."@en ;
                        rdfs:label "Disciplina Técnica"@pt-br ,
                                   "Technical Discipline"@en ;
                        skos:definition "A specialized field of engineering or technical expertise within industrial projects."@en ,
                                        "Um campo especializado de engenharia ou expertise técnica dentro de projetos industriais."@pt-br .


###  https://w3id.org/energy-domain/edo#TechnicalNotes
edo:TechnicalNotes rdf:type owl:Class ;
                   rdfs:subClassOf edo:DomainAttribute ;
                   dcterms:accessRights "PUBLIC" ;
                   dcterms:identifier "TechnicalNotes" ;
                   skos:definition "A field used to provide additional technical information or clarifications that may not be covered by other specific properties, to support a comprehensive understanding of the material’s behavior and suitability."@en ;
                   skos:prefLabel "Notas Técnicas"@pt-br ,
                                  "Technical Notes"@en ;
                   edo:hasAttributeScope edo:TypeLevelAttribute ;
                   edo:hasLifecycleCreationPhase edo:DetailedDesign ;
                   edo:hasTypedValue edo:StringValue ;
                   edo:hasValueCardinality edo:SingleValue .


###  https://w3id.org/energy-domain/edo#TemperatureClass
edo:TemperatureClass rdf:type owl:Class ;
                     rdfs:subClassOf edo:DomainAttribute ;
                     dcterms:accessRights "PUBLIC" ;
                     dcterms:identifier "TemperatureClass" ;
                     skos:definition "Classe de temperatura conforme IEC 61886-1"@pt-br ,
                                     "Temperature class as per IEC 61886-1"@en ;
                     skos:prefLabel "Classe de temperatura"@pt-br ,
                                    "Temperature class"@en ;
                     edo:hasAttributeScope edo:TypeLevelAttribute ;
                     edo:hasLifecycleCreationPhase edo:DetailedDesign ;
                     edo:hasTypedValue edo:StringValue .


###  https://w3id.org/energy-domain/edo#TemperatureRangeTableAttribute
edo:TemperatureRangeTableAttribute rdf:type owl:Class ;
                                   rdfs:subClassOf edo:DomainAttribute ;
                                   rdfs:label "Temperature Range Table" .


###  https://w3id.org/energy-domain/edo#TemperatureRangeTableColumn
edo:TemperatureRangeTableColumn rdf:type owl:Class ;
                                rdfs:subClassOf edo:TemperatureRangeTableAttribute .


###  https://w3id.org/energy-domain/edo#TemperatureRange_MaxTemperature
edo:TemperatureRange_MaxTemperature rdf:type owl:Class ;
                                    rdfs:subClassOf edo:TemperatureRangeTableColumn ;
                                    dcterms:accessRights "PUBLIC" ;
                                    dcterms:identifier "TemperatureRange_MaxTemperature" ;
                                    rdfs:comment "Máxima temperatura de operação tolerada por projeto"@pt-br ;
                                    skos:definition "Maximum operation temperature tolerated by design"@en ;
                                    skos:prefLabel "Maximum operating temperature"@en ,
                                                   "Temperatura máxima de operação"@pt-br ;
                                    edo:hasAttributeScope edo:TypeLevelAttribute ;
                                    edo:hasLifecycleCreationPhase edo:DetailedDesign ;
                                    edo:hasTypedValue edo:FloatValue ;
                                    edo:hasUnit unit:DEG_C ;
                                    edo:hasValueCardinality edo:SingleValue .


###  https://w3id.org/energy-domain/edo#TemperatureRange_MinTemperature
edo:TemperatureRange_MinTemperature rdf:type owl:Class ;
                                    rdfs:subClassOf edo:TemperatureRangeTableColumn ;
                                    dcterms:accessRights "PUBLIC" ;
                                    dcterms:identifier "TemperatureRange_MinTemperature" ;
                                    rdfs:comment "Mínima temperatura de operação tolerada por projeto"@pt-br ;
                                    skos:definition "Minimum operation temperature tolerated by design"@en ;
                                    skos:prefLabel "Minimum operation temperature"@en ,
                                                   "Temperatura mínima de operação"@pt-br ;
                                    edo:hasAttributeScope edo:TypeLevelAttribute ;
                                    edo:hasLifecycleCreationPhase edo:DetailedDesign ;
                                    edo:hasTypedValue edo:FloatValue ;
                                    edo:hasUnit unit:DEG_C ;
                                    edo:hasValueCardinality edo:SingleValue .


###  https://w3id.org/energy-domain/edo#TemperatureSensor
edo:TemperatureSensor rdf:type owl:Class ;
                      rdfs:subClassOf edo:Sensor ;
                      dcterms:identifier "TemperatureSensor" ;
                      skos:prefLabel "Sensor de temperatura"@pt-br ,
                                     "Temperature sensor"@en .


###  https://w3id.org/energy-domain/edo#TensileArmour
edo:TensileArmour rdf:type owl:Class ;
                  rdfs:subClassOf edo:IfcInstanciableElement ,
                                  edo:WireLayer ;
                  dcterms:identifier "TensileArmour" ;
                  skos:definition "Protective layer designed to withstand high tensile stresses and mechanical loads, Tensile Armour is composed of high-strength steel wires or reinforced materials arranged in a helical configuration around the riser. It provides essential resistance to tension and shields the inner layers from mechanical damage and wear, ensuring the riser's integrity and durability during installation and operation in extreme underwater conditions."@en ;
                  skos:prefLabel "Armadura de Tração"@pt-br ,
                                 "Tensile Armour"@en ;
                  edo:hasAttribute edo:TensileWireLayAngle ,
                                   edo:TensileWiresCount ;
                  edo:hasDiscipline edo:SubseaFlexiblePipesEngineering ,
                                    edo:SubseaUmbilicalsEngineering ;
                  edo:ifc_equivalentClass "IfcPipeSegment" ;
                  edo:ifc_objectType "TensileArmour" ;
                  edo:ifc_predefinedType "USERDEFINED" .


###  https://w3id.org/energy-domain/edo#TensileArmourAnnulusCondition
edo:TensileArmourAnnulusCondition rdf:type owl:Class ;
                                  rdfs:subClassOf edo:BendingStiffnessCurveAttribute ,
                                                  edo:DomainAttribute ;
                                  dcterms:accessRights "PUBLIC" ;
                                  dcterms:identifier "TensileArmourAnnulusCondition" ;
                                  skos:definition "Condição do anular das amarduras de tração, Alagado ou Seco"@pt-br ,
                                                  "Indicates the condition of the annulus in the tensile armour layer, which refers to the space between the tensile armour and other layers."@en ;
                                  skos:prefLabel "Condição do Anular das Armaduras de Tração"@pt-br ,
                                                 "Tensile Armour Annulus Condition"@en ;
                                  edo:hasAttributeScope edo:TypeLevelAttribute ;
                                  edo:hasLifecycleCreationPhase edo:DetailedDesign ;
                                  edo:hasTypedValue edo:StringValue ;
                                  edo:hasValueCardinality edo:SingleValue .


###  https://w3id.org/energy-domain/edo#TensileArmourFreeAnnulusVolume
edo:TensileArmourFreeAnnulusVolume rdf:type owl:Class ;
                                   rdfs:subClassOf edo:DomainAttribute ;
                                   dcterms:accessRights "PUBLIC" ;
                                   dcterms:identifier "TensileArmourFreeAnnulusVolume" ;
                                   skos:definition "Indicates the available volume within the annulus of the tensile armour layer that is not occupied by material."@en ;
                                   skos:prefLabel "Tensile Armour Free Annulus Volume"@en ,
                                                  "Volume livre do anular das armaduras de tração"@pt-br ;
                                   edo:hasAttributeScope edo:TypeLevelAttribute ;
                                   edo:hasLifecycleCreationPhase edo:DetailedDesign ;
                                   edo:hasTypedValue edo:FloatValue ;
                                   edo:hasUnit unit:M3-PER-M ,
                                               edo:M3-PER-M ;
                                   edo:hasValueCardinality edo:SingleValue .


###  https://w3id.org/energy-domain/edo#TensileWireLayAngle
edo:TensileWireLayAngle rdf:type owl:Class ;
                        rdfs:subClassOf edo:DomainAttribute ;
                        dcterms:accessRights "PUBLIC" ;
                        dcterms:identifier "TensileWireLayAngle" ;
                        skos:definition "Refers to the angle formed between the individual tensile wires and the longitudinal axis of the flexible pipe. This angle determines how the wires are arranged around the pipe, influencing its mechanical properties and performance under load."@en ;
                        skos:prefLabel "Tensile Wire Lay Angle"@en ,
                                       "Ângulo de Enrolamento dos Arames sob Tração"@pt-br ;
                        edo:hasAttributeScope edo:InstanceLevelAttribute ;
                        edo:hasLifecycleCreationPhase edo:DetailedDesign ;
                        edo:hasTypedValue edo:FloatValue ;
                        edo:hasUnit unit:DEG ;
                        edo:hasValueCardinality edo:SingleValue .


###  https://w3id.org/energy-domain/edo#TensileWiresCount
edo:TensileWiresCount rdf:type owl:Class ;
                      rdfs:subClassOf edo:DomainAttribute ;
                      dcterms:accessRights "PUBLIC" ;
                      dcterms:identifier "TensileWiresCount" ;
                      skos:definition "Indicates the total number of tensile wires in the layer, which contributes to the mechanical strength and load-bearing capacity of the flexible pipe."@en ;
                      skos:prefLabel "Quantidade de Arames de Tração"@pt-br ,
                                     "Tensile Wires Count"@en ;
                      edo:hasAttributeScope edo:InstanceLevelAttribute ;
                      edo:hasLifecycleCreationPhase edo:DetailedDesign ;
                      edo:hasTypedValue edo:IntValue ;
                      edo:hasValueCardinality edo:SingleValue .


###  https://w3id.org/energy-domain/edo#TensionerPadsMaterial
edo:TensionerPadsMaterial rdf:type owl:Class ;
                          rdfs:subClassOf edo:CrushingFrictionCoefficientTighteningAttribute ,
                                          edo:CrushingMaximumAllowableTighteningAttribute ;
                          dcterms:accessRights "PUBLIC" ;
                          dcterms:identifier "TensionerPadsMaterial" ;
                          skos:definition "Indicates the fabrication material used for the tensioner pads. This property is important for assessing the durability, friction, and wear resistance of the pads, ensuring they perform effectively under operational conditions."@en ,
                                          "Nome do material da sapata do tensionador (Por exemplo, Carbon Steel)"@pt-br ;
                          skos:prefLabel "Material das Sapatas do Tensionador"@pt-br ,
                                         "Tensioner Pads Material"@en ;
                          edo:hasAttributeScope edo:TypeLevelAttribute ;
                          edo:hasLifecycleCreationPhase edo:DetailedDesign ;
                          edo:hasTypedValue edo:StringValue ;
                          edo:hasValueCardinality edo:SingleValue .


###  https://w3id.org/energy-domain/edo#TensionerPadsOpeningAngle
edo:TensionerPadsOpeningAngle rdf:type owl:Class ;
                              rdfs:subClassOf edo:CrushingFrictionCoefficientTighteningAttribute ,
                                              edo:CrushingMaximumAllowableTighteningAttribute ;
                              dcterms:accessRights "PUBLIC" ;
                              dcterms:identifier "TensionerPadsOpeningAngle" ;
                              skos:definition "Defines the opening angle of the tensioner pads. This angle is crucial for determining how the pads make contact with the surface, affecting the distribution of force and the overall efficiency of the tightening process. Proper control of this angle ensures effective load application and surface protection during operation."@en ;
                              skos:prefLabel "Tensioner Pads Opening Angle"@en ,
                                             "Ângulo de Abertura das Sapatas do Tensionador"@pt-br ;
                              edo:hasAttributeScope edo:TypeLevelAttribute ;
                              edo:hasLifecycleCreationPhase edo:DetailedDesign ;
                              edo:hasTypedValue edo:IntValue ;
                              edo:hasUnit unit:DEG ;
                              edo:hasValueCardinality edo:SingleValue .


###  https://w3id.org/energy-domain/edo#TensionerPadsShape
edo:TensionerPadsShape rdf:type owl:Class ;
                       rdfs:subClassOf edo:CrushingFrictionCoefficientTighteningAttribute ,
                                       edo:CrushingMaximumAllowableTighteningAttribute ;
                       dcterms:accessRights "PUBLIC" ;
                       dcterms:identifier "TensionerPadsShape" ;
                       skos:definition "Disposição geométrica da sapata (Por exemplo \"V\")"@pt-br ,
                                       "Specifies the geometric shape of the tensioner pads. The shape affects the contact area, frictional performance, and overall effectiveness of the tightening process, influencing how forces are applied and distributed."@en ;
                       skos:prefLabel "Forma das Sapatas do Tensionador"@pt-br ,
                                      "Tensioner Pads Shape"@en ;
                       edo:hasAttributeScope edo:TypeLevelAttribute ;
                       edo:hasLifecycleCreationPhase edo:DetailedDesign ;
                       edo:hasTypedValue edo:StringValue ;
                       edo:hasValueCardinality edo:SingleValue .


###  https://w3id.org/energy-domain/edo#TensionerTracksQuantity
edo:TensionerTracksQuantity rdf:type owl:Class ;
                            rdfs:subClassOf edo:CrushingFrictionCoefficientTighteningAttribute ,
                                            edo:CrushingMaximumAllowableTighteningAttribute ;
                            dcterms:accessRights "PUBLIC" ;
                            dcterms:identifier "TensionerTracksQuantity" ;
                            skos:definition "Indicates the quantity of tensioner tracks. This value is important for understanding the distribution of tightening forces and how evenly the load is applied across the structure during the tightening process."@en ,
                                            "Quantidade de lagartas do tensionador (Por exemplo, 4)"@pt-br ;
                            skos:prefLabel "Quantidade de Lagartas do Tensionador"@pt-br ,
                                           "Tensioner Tracks Quantity"@en ;
                            edo:hasAttributeScope edo:TypeLevelAttribute ;
                            edo:hasLifecycleCreationPhase edo:DetailedDesign ;
                            edo:hasTypedValue edo:IntValue ;
                            edo:hasValueCardinality edo:SingleValue .


###  https://w3id.org/energy-domain/edo#TestBase
edo:TestBase rdf:type owl:Class ;
             rdfs:subClassOf edo:TestEquipment ;
             dcterms:identifier "TestBase" ;
             skos:prefLabel "Base de teste"@pt-br ,
                            "Test base"@en .


###  https://w3id.org/energy-domain/edo#TestConditions
edo:TestConditions rdf:type owl:Class ;
                   rdfs:subClassOf edo:BendingStiffnessCurveAttribute ,
                                   edo:CrushingFrictionCoefficientTighteningAttribute ,
                                   edo:CrushingMaximumAllowableTensionAttribute ,
                                   edo:CrushingMaximumAllowableTighteningAttribute ,
                                   edo:DomainAttribute ,
                                   edo:LayingMinimumRadiusCurveAttribute ;
                   dcterms:accessRights "PUBLIC" ;
                   dcterms:identifier "TestConditions" ;
                   skos:definition "Descrição completa das condições para a execução do ensaio"@pt-br ,
                                   "Specifies unstructured complementary information regarding the conditions under which a test is performed. This property may include additional details such as temperature, pressure, load, or other factors that could influence the test results, providing context for accurate interpretation of performance assessments."@en ;
                   skos:prefLabel "Condições de Teste"@pt-br ,
                                  "Test Conditions"@en ;
                   edo:hasAttributeScope edo:TypeLevelAttribute ;
                   edo:hasLifecycleCreationPhase edo:DetailedDesign ;
                   edo:hasTypedValue edo:StringValue ;
                   edo:hasValueCardinality edo:SingleValue .


###  https://w3id.org/energy-domain/edo#TestEquipment
edo:TestEquipment rdf:type owl:Class ;
                  rdfs:subClassOf edo:SurfaceEquipment ;
                  dcterms:identifier "TestEquipment" ;
                  skos:prefLabel "Equipamento de teste"@pt-br ,
                                 "Test equipment"@en .


###  https://w3id.org/energy-domain/edo#TestPressure
edo:TestPressure rdf:type owl:Class ;
                 rdfs:subClassOf edo:DomainAttribute ;
                 dcterms:accessRights "PUBLIC" ;
                 dcterms:identifier "TestPressure" ;
                 skos:prefLabel "Pressão de teste"@pt-br ;
                 edo:hasAttributeScope edo:TypeLevelAttribute ;
                 edo:hasLifecycleCreationPhase edo:DetailedDesign ;
                 edo:hasTypedValue edo:FloatValue ;
                 edo:hasUnit unit:MPa ;
                 edo:hasValueCardinality edo:SingleValue .


###  https://w3id.org/energy-domain/edo#ThermalConductivityCoefficient
edo:ThermalConductivityCoefficient rdf:type owl:Class ;
                                   rdfs:subClassOf edo:DomainAttribute ;
                                   dcterms:accessRights "PUBLIC" ;
                                   dcterms:identifier "ThermalConductivityCoefficient" ;
                                   skos:definition "Coeficiente de Condutividade Térmica do material (Obs. Para materiais compósitos, indicar o coefitiente no sentido longitudinal das fibras)"@pt-br ,
                                                   "Indicates the material's ability to conduct heat, measured as the rate at which heat passes through the material under a temperature gradient. This property is important for assessing how the material handles heat transfer in subsea environments, ensuring it can maintain performance under varying thermal conditions."@en ;
                                   skos:prefLabel "Coeficiente de Condutividade Térmica"@pt-br ,
                                                  "Thermal Conductivity Coefficient"@en ;
                                   edo:hasAttributeScope edo:TypeLevelAttribute ;
                                   edo:hasLifecycleCreationPhase edo:DetailedDesign ;
                                   edo:hasTypedValue edo:FloatValue ;
                                   edo:hasUnit unit:W-PER-M-K ;
                                   edo:hasValueCardinality edo:SingleValue .


###  https://w3id.org/energy-domain/edo#ThermalExchangeCoefficientFlooded
edo:ThermalExchangeCoefficientFlooded rdf:type owl:Class ;
                                      rdfs:subClassOf edo:DomainAttribute ;
                                      dcterms:accessRights "PUBLIC" ;
                                      dcterms:identifier "ThermalExchangeCoefficientFlooded" ;
                                      skos:definition "Coeficiente de troca térmica na temperatura máxima de projeto no interior, na temperatura da profundidade máxima especificada da água no exterior, com os anulares de isolamento e das armadura de tração alagados, no final da vida útil."@pt-br ,
                                                      "Indicates the rate at which heat is transferred through a material or component in flooded conditions. This property is essential for assessing the material's thermal performance, influencing its ability to manage heat effectively in operational scenarios where it is exposed to fluid filling."@en ;
                                      skos:prefLabel "Coeficiente de Troca Térmica em Condição Alagada"@pt-br ,
                                                     "Thermal Exchange Coefficient Flooded"@en ;
                                      edo:hasAttributeScope edo:TypeLevelAttribute ;
                                      edo:hasLifecycleCreationPhase edo:DetailedDesign ;
                                      edo:hasTypedValue edo:FloatValue ;
                                      edo:hasUnit unit:W-PER-M-K ;
                                      edo:hasValueCardinality edo:SingleValue .


###  https://w3id.org/energy-domain/edo#ThermalPower
edo:ThermalPower rdf:type owl:Class ;
                 rdfs:subClassOf edo:Domain ;
                 rdfs:label "Energia Térmica"@pt-br ,
                            "Thermal Power"@en ;
                 skos:definition "Energy production from fossil fuels (coal, natural gas) through thermal conversion."@en ,
                                 "Produção de energia a partir de combustíveis fósseis (carvão, gás natural) através de conversão térmica."@pt-br .


###  https://w3id.org/energy-domain/edo#ThreadPitch
edo:ThreadPitch rdf:type owl:Class ;
                rdfs:subClassOf edo:DomainAttribute ;
                dcterms:accessRights "PUBLIC" ;
                dcterms:identifier "ThreadPitch" ;
                skos:definition "The distance between adjacent thread crests, measured along the thread's axis, determining the threading's fineness or coarseness."@en ;
                skos:prefLabel "Passo da Rosca"@pt-br ,
                               "Thread Pitch"@en ;
                edo:hasAttributeScope edo:InstanceLevelAttribute ;
                edo:hasLifecycleCreationPhase edo:DetailedDesign ;
                edo:hasTypedValue edo:FloatValue ;
                edo:hasUnit unit:MilliM ;
                edo:hasValueCardinality edo:SingleValue .


###  https://w3id.org/energy-domain/edo#ThreadStandard
edo:ThreadStandard rdf:type owl:Class ;
                   rdfs:subClassOf edo:DomainAttribute ;
                   dcterms:accessRights "PUBLIC" ;
                   dcterms:identifier "ThreadStandard" ;
                   skos:definition "The standard specification governing the design and dimensions of threads used in the component, ensuring compatibility and interchangeability."@en ;
                   skos:prefLabel "Padrão de Rosca"@pt-br ,
                                  "Thread Standard"@en ;
                   edo:hasAttributeScope edo:InstanceLevelAttribute ;
                   edo:hasLifecycleCreationPhase edo:DetailedDesign ;
                   edo:hasTypedValue edo:StringValue ;
                   edo:hasValueCardinality edo:SingleValue .


###  https://w3id.org/energy-domain/edo#ThreadType
edo:ThreadType rdf:type owl:Class ;
               rdfs:subClassOf edo:HoseFittingSpecTableColumn ;
               dcterms:accessRights "PUBLIC" ;
               dcterms:identifier "ThreadType" ;
               skos:prefLabel "Thread type"@en ,
                              "Tipo de rosca"@pt-br ;
               edo:hasAttributeScope edo:TypeLevelAttribute ;
               edo:hasLifecycleCreationPhase edo:DetailedDesign ;
               edo:hasTypedValue edo:StringValue ;
               edo:hasValueCardinality edo:SingleValue .


###  https://w3id.org/energy-domain/edo#ThreadedFitting
edo:ThreadedFitting rdf:type owl:Class ;
                    rdfs:subClassOf edo:TubingCoupling ;
                    dcterms:identifier "ThreadedFitting" ;
                    skos:definition "A Threaded Fitting is a connector used to join fluid or gas lines through screw threads, providing a secure and leak-tight connection that can be easily assembled or disassembled during installation or maintenance."@en ,
                                    "Um Engate Rosqueado é um conector usado para unir linhas de fluido ou gás por meio de roscas, garantindo uma conexão segura e vedada que pode ser facilmente montada ou desmontada durante a instalação ou manutenção."@pt-br ;
                    skos:prefLabel "Engate Rosqueado"@pt-br ,
                                   "Threaded Fitting"@en ;
                    edo:hasAttribute edo:HoseFittingSpecTableColumn ;
                    edo:hasDiscipline edo:SubseaUmbilicalsEngineering ;
                    edo:ifc_equivalentClass "IfcPipeFitting" ;
                    edo:ifc_objectType "ThreadedFitting" .


###  https://w3id.org/energy-domain/edo#ThreadsPerInch
edo:ThreadsPerInch rdf:type owl:Class ;
                   rdfs:subClassOf edo:DomainAttribute ;
                   dcterms:accessRights "PUBLIC" ;
                   dcterms:identifier "ThreadsPerInch" ;
                   skos:definition "Threads per Inch. Indicates the number of threads present in one inch of the bolt"@en ;
                   skos:prefLabel "Fios por Polegada"@pt-br ,
                                  "Threads Per Inch"@en ;
                   edo:hasAttributeScope edo:InstanceLevelAttribute ;
                   edo:hasLifecycleCreationPhase edo:DetailedDesign ;
                   edo:hasTypedValue edo:FloatValue ;
                   edo:hasValueCardinality edo:SingleValue .


###  https://w3id.org/energy-domain/edo#Tidal
edo:Tidal rdf:type owl:Class ;
          rdfs:subClassOf edo:Marine ;
          dcterms:identifier "Tidal" ;
          skos:definition "Energia das marés é gerada aproveitando a previsível subida e descida das marés oceânicas, geralmente por meio de barragens, cercas de marés ou turbinas de corrente de maré. Oferece uma fonte altamente confiável de energia renovável devido aos ciclos gravitacionais naturais da Terra, da Lua e do Sol."@pt-br ,
                          "Tidal energy is generated by harnessing the predictable rise and fall of ocean tides, typically using barrages, tidal fences, or tidal stream turbines. It offers a highly reliable source of renewable energy due to the natural gravitational cycles of the Earth, Moon and Sun."@en ;
          skos:prefLabel "Energia das Marés"@pt-br ,
                         "Tidal Energy"@en .


###  https://w3id.org/energy-domain/edo#TieIn
edo:TieIn rdf:type owl:Class ;
          rdfs:subClassOf edo:PressureComponent ;
          dcterms:identifier "TieIn" ;
          skos:prefLabel "Tie-in"@en ,
                         "Tie-in"@pt-br .


###  https://w3id.org/energy-domain/edo#TieInEquipment
edo:TieInEquipment rdf:type owl:Class ;
                   rdfs:subClassOf edo:FlowControlModule ;
                   dcterms:identifier "TieInEquipment" ;
                   skos:prefLabel "Equipamento de interligação"@pt-br ,
                                  "Tie-in equipment"@en .


###  https://w3id.org/energy-domain/edo#TimeValue
edo:TimeValue rdf:type owl:Class ;
              owl:equivalentClass [ rdf:type owl:Restriction ;
                                    owl:onProperty rdf:value ;
                                    owl:allValuesFrom xsd:time
                                  ] ;
              rdfs:subClassOf edo:DataType ;
              rdfs:comment "Constraint for xsd:time (time of day)"@en ;
              rdfs:label "Time Value"@en .


###  https://w3id.org/energy-domain/edo#Timestamp
edo:Timestamp rdf:type owl:Class ;
              rdfs:subClassOf edo:ProvenanceAttribute ;
              dcterms:accessRights "PUBLIC" ;
              dcterms:identifier "Timestamp" ;
              skos:definition "Exact date and time, providing a precise reference for tracking when an event or action occurred within the system."@en ;
              skos:prefLabel "Timestamp"@en ;
              edo:hasAttributeScope edo:InstanceLevelAttribute ;
              edo:hasTypedValue edo:DateTimeValue ;
              edo:hasValueCardinality edo:SingleValue .


###  https://w3id.org/energy-domain/edo#ToBeDeprecated
edo:ToBeDeprecated rdf:type owl:Class ;
                   rdfs:subClassOf edo:ConceptualMarker ;
                   skos:definition "Representa um marcador usado para identificar elementos que estão planejados para remoção ou substituição futura, sem afetar seu uso ou propriedades atuais."@pt-br ,
                                   "Represents a marker used to identify elements that are planned to be removed or replaced in the future, without affecting their current use or properties."@en ;
                   skos:prefLabel "A Ser Depreciado"@pt-br ,
                                  "To Be Deprecated"@en .


###  https://w3id.org/energy-domain/edo#TopBendStiffener
edo:TopBendStiffener rdf:type owl:Class ;
                     rdfs:subClassOf edo:BendStiffener ,
                                     edo:IfcInstanciableElement ;
                     dcterms:identifier "TopBendStiffener" ;
                     skos:altLabel "Curvature Stiffener"@en ,
                                   "Stiffener"@en ,
                                   "Top Bending Stiffener"@en ;
                     skos:definition "Designed to support and stabilize the riser where it transitions from the seabed to the floating platform or vessel, the Top Bend Stiffener is composed of high-strength materials such as steel or composites. It helps prevent excessive bending, distributes mechanical loads, and enhances flexibility management, ensuring the riser's structural integrity and performance during installation and operation in dynamic offshore conditions."@en ;
                     skos:prefLabel "Enrijecedor de Curvatura de Topo"@pt-br ,
                                    "Top Bend Stiffener"@en ;
                     edo:hasAttribute edo:BellmouthDiameter ;
                     edo:hasDiscipline edo:SubseaFlexiblePipesEngineering ,
                                       edo:SubseaUmbilicalsEngineering ;
                     edo:ifc_equivalentClass "IfcPipeFitting" ;
                     edo:ifc_objectType "TopBendStiffener" .


###  https://w3id.org/energy-domain/edo#TopsideConnectionPoint
edo:TopsideConnectionPoint rdf:type owl:Class ;
                           rdfs:subClassOf edo:ConnectionPoint ,
                                           edo:IfcInstanciableElement ;
                           dcterms:identifier "TopsideConnectionPoint" ;
                           skos:definition "Representa um ponto de conexão localizado em instalações topside ou de superfície, conectando elementos acima da água ou do solo."@pt-br ,
                                           "Represents a connection point located on topside or surface facilities, linking elements above water or ground."@en ;
                           skos:prefLabel "Ponto de Conexão em Topside"@pt-br ,
                                          "Topside Connection Point"@en ;
                           edo:hasDiscipline edo:SubseaFlexiblePipesEngineering ,
                                             edo:SubseaUmbilicalsEngineering ;
                           edo:ifc_equivalentClass "IfcPipeFitting" ;
                           edo:ifc_objectType "TopsideConnectionPoint" ;
                           edo:ifc_predefinedType "USERDEFINED" .


###  https://w3id.org/energy-domain/edo#TopsideEquipment
edo:TopsideEquipment rdf:type owl:Class ;
                     rdfs:subClassOf edo:SurfaceEquipment ;
                     dcterms:identifier "TopsideEquipment" ;
                     skos:prefLabel "Equipamento de Topside"@pt-br ,
                                    "Topside Equipment"@en .


###  https://w3id.org/energy-domain/edo#TorpedoPile
edo:TorpedoPile rdf:type owl:Class ;
                rdfs:subClassOf edo:Pile ;
                dcterms:identifier "TorpedoPile" ;
                skos:definition "Anchoring pile driven into seabed by free fall"@en ,
                                "Estaca de ancoragem cravada no solo por queda livre"@pt-br ;
                skos:prefLabel "Estaca-torpedo"@pt-br ,
                               "Torpedo pile"@en .


###  https://w3id.org/energy-domain/edo#TorsionalStiffnessHigherStorage
edo:TorsionalStiffnessHigherStorage rdf:type owl:Class ;
                                    rdfs:subClassOf edo:DomainAttribute ;
                                    dcterms:accessRights "PUBLIC" ;
                                    dcterms:identifier "TorsionalStiffnessHigherStorage" ;
                                    rdfs:comment "Valor maior da rigidez torsional (em um sentido particular de torção) nas condições de estocagem"@pt-br ;
                                    skos:definition "Higher torsional stiffness value (in a particular twist direction) at storage conditions"@en ;
                                    skos:prefLabel "Rigidez torsional, valor maior, estocagem"@pt-br ,
                                                   "Torsional stiffness, higher value, storage"@en ;
                                    edo:hasAttributeScope edo:TypeLevelAttribute ;
                                    edo:hasLifecycleCreationPhase edo:DetailedDesign ;
                                    edo:hasTypedValue edo:FloatValue ;
                                    edo:hasUnit unit:N-M2-PER-RAD ;
                                    edo:hasValueCardinality edo:SingleValue .


###  https://w3id.org/energy-domain/edo#TorsionalStiffnessLowerStorage
edo:TorsionalStiffnessLowerStorage rdf:type owl:Class ;
                                   rdfs:subClassOf edo:DomainAttribute ;
                                   dcterms:accessRights "PUBLIC" ;
                                   dcterms:identifier "TorsionalStiffnessLowerStorage" ;
                                   rdfs:comment "Valor menor da rigidez torsional (em um sentido particular de torção) nas condições de estocagem"@pt-br ;
                                   skos:definition "Lower torsional stiffness value (in a particular twist direction) at storage conditions"@en ;
                                   skos:prefLabel "Rigidez torsional, valor menor, estocagem"@pt-br ,
                                                  "Torsional stiffness, lower value, storage"@en ;
                                   edo:hasAttributeScope edo:TypeLevelAttribute ;
                                   edo:hasLifecycleCreationPhase edo:DetailedDesign ;
                                   edo:hasTypedValue edo:FloatValue ;
                                   edo:hasUnit unit:N-M2-PER-RAD ;
                                   edo:hasValueCardinality edo:SingleValue .


###  https://w3id.org/energy-domain/edo#TransitionSpool
edo:TransitionSpool rdf:type owl:Class ;
                    rdfs:subClassOf edo:LineAncillary ;
                    dcterms:identifier "TransitionSpool" ;
                    skos:prefLabel "Prolongador Bipartido Type"@pt-br ;
                    edo:hasDiscipline edo:SubseaUmbilicalsEngineering ;
                    edo:ifc_equivalentClass "IfcPipeFitting" ;
                    edo:ifc_objectType "TransitionSpool" ;
                    edo:ifc_predefinedType "USERDEFINED" .


###  https://w3id.org/energy-domain/edo#TransportLineSegment
edo:TransportLineSegment rdf:type owl:Class ;
                         rdfs:subClassOf edo:LinearObject ;
                         dcterms:identifier "TransportLineSegment" ;
                         skos:definition "Line for conducting some type of flow."@en ,
                                         "Linha para condução de algum tipo de fluxo"@pt-br ;
                         skos:prefLabel "Segmento de Linha de Transporte"@pt-br ,
                                        "Transport Line Segment"@en ;
                         edo:hasAttribute edo:MaxDepth ,
                                          edo:OuterDiameter ,
                                          edo:Reused ,
                                          edo:TemperatureRangeTableColumn .


###  https://w3id.org/energy-domain/edo#TransportSupportPoint
edo:TransportSupportPoint rdf:type owl:Class ;
                          rdfs:subClassOf edo:SupportPoint ;
                          dcterms:identifier "TransportSupportPoint" ;
                          skos:definition "Representa um ponto de apoio utilizado especificamente durante o transporte ou manuseio de elementos."@pt-br ,
                                          "Represents a support point used specifically during transportation or handling of elements."@en ;
                          skos:prefLabel "Ponto de Apoio para Transporte"@pt-br ,
                                         "Transport Support Point"@en .


###  https://w3id.org/energy-domain/edo#Transportation
edo:Transportation rdf:type owl:Class ;
                   rdfs:subClassOf edo:ConstructionPhase ;
                   rdfs:label "Transportation"@en ,
                              "Transporte"@pt-br ;
                   skos:definition "Logistics and transport of materials and equipment to the construction or installation site."@en ,
                                   "Logística e transporte de materiais e equipamentos para o local de construção ou instalação."@pt-br .


###  https://w3id.org/energy-domain/edo#TreeCap
edo:TreeCap rdf:type owl:Class ;
            rdfs:subClassOf edo:FlowControlModule ;
            dcterms:identifier "TreeCap" ;
            edo:hasDiscipline edo:WetChristmasTreesEngineering .


###  https://w3id.org/energy-domain/edo#TreeRunningTool
edo:TreeRunningTool rdf:type owl:Class ;
                    rdfs:subClassOf edo:RunningTool ;
                    dcterms:identifier "TreeRunningTool" ;
                    skos:prefLabel "Ferramenta de instalação de ANM"@pt-br ,
                                   "Wet Christmas tree running tool"@en .


###  https://w3id.org/energy-domain/edo#TrianglePlate
edo:TrianglePlate rdf:type owl:Class ;
                  rdfs:subClassOf edo:MooringAccessory ;
                  dcterms:identifier "TrianglePlate" ;
                  skos:prefLabel "Placa triangular"@pt-br ,
                                 "Triangle plate"@en .


###  https://w3id.org/energy-domain/edo#Tubing
edo:Tubing rdf:type owl:Class ;
           rdfs:subClassOf edo:FunctionLine ;
           dcterms:identifier "Tubing" ;
           skos:definition "Representa um tubo condutor de fluido dentro de uma linha funcional de um componente umbilical."@pt-br ,
                           "Represents a fluid-carrying tube within a function line of an umbilical component."@en ;
           skos:prefLabel "Tubing"@en ,
                          "Tubulação"@pt-br ;
           edo:hasAttribute edo:BurstPressure ,
                            edo:CollapsePressure ,
                            edo:InternalDiameter ,
                            edo:LinearWeightEmptySubmerged ,
                            edo:LinearWeightFilledAir ,
                            edo:LinearWeightFilledSubmerged ,
                            edo:MaxPressure ,
                            edo:TestPressure .


###  https://w3id.org/energy-domain/edo#TubingCoupling
edo:TubingCoupling rdf:type owl:Class ;
                   rdfs:subClassOf edo:Coupling ;
                   dcterms:identifier "TubingCoupling" ;
                   skos:definition "Acoplamentos para linhas de condução de fluidos (i.e. hidráulicos ou pneumáticos)."@pt-br ,
                                   "Couplings for fluid conveyance lines (i.e. hydraulic or pneumatic)."@en ;
                   skos:prefLabel "Acoplamento de Tubulação"@pt-br ,
                                  "Tubing Coupling"@en ;
                   edo:hasAttribute edo:Length ,
                                    edo:MaxPressure .


###  https://w3id.org/energy-domain/edo#TubingHanger
edo:TubingHanger rdf:type owl:Class ;
                 rdfs:subClassOf edo:PressureComponent ;
                 dcterms:identifier "TubingHanger" ;
                 skos:definition "Componente de topo que oferece suporte mecânico e interfaces (hidráulicas, elétricas, óticas, etc.) aos demais componentes da coluna de poço"@pt-br ,
                                 "Top component providing mechanical support and interfaces (hydraulic, electrical, optical, etc.) to other well tubing components"@en ;
                 skos:prefLabel "Suspensor de coluna"@pt-br ,
                                "Tubing hanger"@en .


###  https://w3id.org/energy-domain/edo#TubingHangerRunningTool
edo:TubingHangerRunningTool rdf:type owl:Class ;
                            rdfs:subClassOf edo:RunningTool ;
                            dcterms:identifier "TubingHangerRunningTool" ;
                            skos:prefLabel "Ferramenta de instalação de TH"@pt-br ,
                                           "Tubing hanger running tool"@en .


###  https://w3id.org/energy-domain/edo#TypeLevelAttribute
edo:TypeLevelAttribute rdf:type owl:Class ;
                       rdfs:subClassOf edo:AttributeScope ;
                       rdfs:comment "Attribute common to all items of the same type."@en ;
                       rdfs:label "Atributo de Tipo"@pt-br ,
                                  "Type-Level Attribute"@en ;
                       skos:definition "Atributo comum a todos os itens do mesmo tipo"@pt-br ,
                                       "Attribute common to all items of the same type"@en .


###  https://w3id.org/energy-domain/edo#UNSBoltSet
edo:UNSBoltSet rdf:type owl:Class ;
               rdfs:subClassOf edo:BoltSet ,
                               edo:IfcInstanciableElement ;
               dcterms:identifier "UNSBoltSet" ;
               skos:definition "A set of bolts conforming to the Unified Numbering System (UNS) standard, ensuring material consistency and reliability in subsea applications."@en ;
               skos:prefLabel "Conjunto de Parafusos UNS"@pt-br ,
                              "UNS Bolt Set"@en ;
               edo:hasAttribute edo:NominalDiameter ,
                                edo:PitchToleranceClass ,
                                edo:ThreadStandard ,
                                edo:ThreadsPerInch ;
               edo:hasDiscipline edo:SubseaFlexiblePipesEngineering ,
                                 edo:SubseaUmbilicalsEngineering ;
               edo:ifc_equivalentClass "IfcMechanicalFastener" ;
               edo:ifc_objectType "UNSBoltSet" ;
               edo:ifc_predefinedType "USERDEFINED" .


###  https://w3id.org/energy-domain/edo#UNSStudSet
edo:UNSStudSet rdf:type owl:Class ;
               rdfs:subClassOf edo:IfcInstanciableElement ,
                               edo:StudSet ;
               dcterms:identifier "UNSStudSet" ;
               skos:definition "UNS stud sets are essential fastening components for subsea oil and gas components, tailored to securely join equipment parts. Each set comprises bolts, nuts, and washers, all in UNS sizing and crafted from high-strength, corrosion-resistant materials to endure the challenging subsea environment. These components provide robust fastening, ensuring structural integrity and leak prevention in end fittings. UNS stud sets are engineered to withstand high pressure and extreme temperatures, playing a vital role in the safety and longevity of subsea interconnections."@en ;
               skos:prefLabel "Conjunto de Estojos UNS"@pt-br ,
                              "UNS Stud Set"@en ;
               edo:hasAttribute edo:PitchToleranceClass ,
                                edo:ThreadStandard ,
                                edo:ThreadsPerInch ;
               edo:hasDiscipline edo:SubseaFlexiblePipesEngineering ,
                                 edo:SubseaUmbilicalsEngineering ;
               edo:ifc_equivalentClass "IfcMechanicalFastener" ;
               edo:ifc_objectType "UNSStudSet" ;
               edo:ifc_predefinedType "USERDEFINED" .


###  https://w3id.org/energy-domain/edo#UTA
edo:UTA rdf:type owl:Class ;
        rdfs:subClassOf edo:SubseaEquipment ;
        dcterms:identifier "UTA" ;
        skos:definition "Equipamento para terminação e ancoragem de um umbilical"@pt-br ,
                        "Equipment for umbilical termination and anchoring"@en ;
        skos:prefLabel "Conjunto de terminação de umbilical"@pt-br ,
                       "Umbilical termination assembly"@en ;
        edo:hasDiscipline edo:SubseaUmbilicalsEngineering .


###  https://w3id.org/energy-domain/edo#UTM
edo:UTM rdf:type owl:Class ;
        rdfs:subClassOf edo:LineTerminationModule ;
        dcterms:identifier "UTM" ;
        skos:prefLabel "Módulo de terminação de umbilical"@pt-br ,
                       "Umbilical termination module"@en ;
        edo:hasDiscipline edo:WetChristmasTreesEngineering .


###  https://w3id.org/energy-domain/edo#UltTensStrAlongFibers
edo:UltTensStrAlongFibers rdf:type owl:Class ;
                          rdfs:subClassOf edo:DomainAttribute ;
                          dcterms:accessRights "PUBLIC" ;
                          dcterms:identifier "UltTensStrAlongFibers" ;
                          skos:definition "Indicates the maximum tensile stress a material can withstand along the direction of its fibers before breaking. This property is crucial for assessing the strength of fiber-reinforced materials, ensuring they can handle tensile loads effectively in the direction of fiber alignment."@en ;
                          skos:prefLabel "Tensão máxima de tração longitudinalmente às fibras"@pt-br ,
                                         "Ultimate Tensile Strength Along Fibers"@en ;
                          edo:hasAttributeScope edo:TypeLevelAttribute ;
                          edo:hasLifecycleCreationPhase edo:DetailedDesign ;
                          edo:hasTypedValue edo:FloatValue ;
                          edo:hasUnit unit:PA ;
                          edo:hasValueCardinality edo:SingleValue .


###  https://w3id.org/energy-domain/edo#UltTensStrPerpendFibers
edo:UltTensStrPerpendFibers rdf:type owl:Class ;
                            rdfs:subClassOf edo:DomainAttribute ;
                            dcterms:accessRights "PUBLIC" ;
                            dcterms:identifier "UltTensStrPerpendFibers" ;
                            skos:definition "Indicates the maximum tensile stress a material can withstand when applied perpendicular to the direction of its fibers before breaking. This property is important for evaluating the strength and durability of fiber-reinforced materials under tensile loads that are not aligned with the fibers, providing insights into their performance in various loading conditions."@en ;
                            skos:prefLabel "Tensão máxima de tração perpendicularmente às fibras"@pt-br ,
                                           "Ultimate Tensile Strength Perpendicular To Fibers"@en ;
                            edo:hasAttributeScope edo:TypeLevelAttribute ;
                            edo:hasLifecycleCreationPhase edo:DetailedDesign ;
                            edo:hasTypedValue edo:FloatValue ;
                            edo:hasUnit unit:PA ;
                            edo:hasValueCardinality edo:SingleValue .


###  https://w3id.org/energy-domain/edo#UltimateTensileStress
edo:UltimateTensileStress rdf:type owl:Class ;
                          rdfs:subClassOf edo:DomainAttribute ;
                          dcterms:accessRights "PUBLIC" ;
                          dcterms:identifier "UltimateTensileStress" ;
                          skos:definition "Indicates the maximum stress a material can withstand while being stretched or pulled before breaking. This property is essential for evaluating the material's strength and determining its ability to perform under tensile loads without failure."@en ,
                                          "Tensão máxima de tração (Específica para Materiais Metálicos)"@pt-br ;
                          skos:prefLabel "Tensão Máxima de Tração"@pt-br ,
                                         "Ultimate Tensile Stress"@en ;
                          edo:hasAttributeScope edo:TypeLevelAttribute ;
                          edo:hasLifecycleCreationPhase edo:DetailedDesign ;
                          edo:hasTypedValue edo:FloatValue ;
                          edo:hasUnit unit:PA ;
                          edo:hasValueCardinality edo:SingleValue .


###  https://w3id.org/energy-domain/edo#UmbilicalBundle
edo:UmbilicalBundle rdf:type owl:Class ;
                    rdfs:subClassOf edo:IfcInstanciableElement ,
                                    edo:Specification ;
                    dcterms:identifier "UmbilicalBundle" ;
                    skos:definition "O Conjunto de Umbilical é o agrupamento integrado dos elementos funcionais que compõem um umbilical submarino, projetado para transmitir potência hidráulica, energia elétrica e sinais de dados entre os sistemas de superfície e submarinos. Normalmente é formado por vários tubos, cabos e fibras reunidos em um único feixe, protegidos por camadas externas de revestimento e armadura. Projetado para garantir confiabilidade e eficiência em condições de águas profundas, o conjunto de umbilical fornece os canais essenciais de controle e comunicação que permitem a operação segura e contínua dos equipamentos submarinos de produção."@pt-br ,
                                    "The Umbilical Bundle is the integrated assembly of functional elements within a subsea umbilical, designed to transmit hydraulic power, electrical energy, and data signals between surface and subsea systems. It typically consists of multiple tubes, cables, and fibers bundled together and protected by external sheathing and armoring. Engineered to ensure reliability and efficiency under deepwater conditions, the umbilical bundle provides essential control and communication pathways that enable the safe and continuous operation of subsea production equipment."@en ;
                    skos:prefLabel "Conjunto de Umbilical"@pt-br ,
                                   "Umbilical Bundle"@en ;
                    edo:hasAttribute edo:LayAngle ,
                                     edo:LayDirection ,
                                     edo:OuterDiameter ;
                    edo:hasDiscipline edo:SubseaUmbilicalsEngineering ;
                    edo:ifc_equivalentClass "IfcPipeSegmentType" ;
                    edo:ifc_objectType "UmbilicalBundle" ;
                    edo:ifc_predefinedType "USERDEFINED" .


###  https://w3id.org/energy-domain/edo#UmbilicalComponent
edo:UmbilicalComponent rdf:type owl:Class ;
                       rdfs:subClassOf edo:FabricationComponent ;
                       dcterms:identifier "UmbilicalComponent" ;
                       skos:definition "Representa um componente de um sistema umbilical, tipicamente parte de instalações submarinas ou industriais, servindo de base para linhas funcionais e camadas estruturais."@pt-br ,
                                       "Represents a component of an umbilical system, typically part of subsea or industrial installations, forming the basis for functional lines and structural layers."@en ;
                       skos:prefLabel "Componente Umbilical"@pt-br ,
                                      "Componente de umbilical"@pt-br ,
                                      "Umbilical Component"@en ,
                                      "Umbilical component"@en ;
                       edo:hasAttribute edo:LinearWeight ,
                                        edo:OuterDiameter .


###  https://w3id.org/energy-domain/edo#UmbilicalLocation
edo:UmbilicalLocation rdf:type owl:Class ;
                      rdfs:subClassOf edo:IfcInstanciableElement ,
                                      edo:Interconnection ;
                      dcterms:identifier "UmbilicalLocation" ;
                      skos:prefLabel "Local de umbilical"@pt-br ,
                                     "Umbilical location"@en ;
                      edo:hasDiscipline edo:SubseaUmbilicalsEngineering .


###  https://w3id.org/energy-domain/edo#UmbilicalPullingHead
edo:UmbilicalPullingHead rdf:type owl:Class ;
                         rdfs:subClassOf edo:PullingHead ;
                         dcterms:identifier "UmbilicalPullingHead" ;
                         skos:altLabel "Cabeça de Manuseio para Umbilical"@pt-br ;
                         skos:definition "Cabeça de tração tubular (com espaço para pigtails), usada para umbilicais."@pt-br ,
                                         "Tubular pulling head (with space for pigtails), used for umbilicals."@en ;
                         skos:prefLabel "Cabeça de Tração para Umbilical"@pt-br ,
                                        "Umbilical Pulling Head"@en ;
                         edo:hasAttribute edo:FlangeType ,
                                          edo:InternalDiameter ,
                                          edo:InternalLength ;
                         edo:hasDiscipline edo:SubseaUmbilicalsEngineering ;
                         edo:ifc_equivalentClass "IfcPipeFitting" ;
                         edo:ifc_objectType "UmbilicalPullingHead" .


###  https://w3id.org/energy-domain/edo#UmbilicalSegment
edo:UmbilicalSegment rdf:type owl:Class ;
                     rdfs:subClassOf edo:IfcInstanciableElement ,
                                     edo:TransportLineSegment ;
                     dcterms:identifier "UmbilicalSegment" ;
                     skos:prefLabel "Tramo de Umbilical"@pt-br ,
                                    "Umbilical Segment"@en ;
                     edo:hasAttribute edo:AssemblyShouldObeyModelPolarity ,
                                      edo:FlexibleSegmentStatus ,
                                      edo:IdInUnifilarDiagram ,
                                      edo:MainDesignNorm ,
                                      edo:ManufacturingDate ,
                                      edo:ManufacturingNonConformities ,
                                      edo:MaxLengthTolerance ,
                                      edo:SpecialRequirements ,
                                      edo:StdUmbilicalType ,
                                      edo:StructureApplication ;
                     edo:hasDiscipline edo:SubseaUmbilicalsEngineering ;
                     edo:ifc_equivalentClass "UmbilicalSegment" ;
                     edo:ifc_objectType "IfcPipeSegment" ;
                     edo:ifc_predefinedType "USERDEFINED" .


###  https://w3id.org/energy-domain/edo#UmbilicalSpan
edo:UmbilicalSpan rdf:type owl:Class ;
                  rdfs:subClassOf edo:LineSpan ;
                  dcterms:identifier "UmbilicalSpan" ;
                  skos:prefLabel "Trecho de umbilical"@pt-br ,
                                 "Umbilical span"@en .


###  https://w3id.org/energy-domain/edo#UmbilicalStructure
edo:UmbilicalStructure rdf:type owl:Class ;
                       rdfs:subClassOf edo:FlexibleStructure ,
                                       edo:IfcInstanciableElement ;
                       dcterms:identifier "UmbilicalStructure" ;
                       skos:definition "A Estrutura do Umbilical é a configuração em camadas, a especificação, de um umbilical submarino, projetada para fornecer proteção mecânica, flexibilidade e estabilidade em ambientes subaquáticos. Ela é composta por múltiplas camadas e componentes, como tubos, cabos, materiais de enchimento e armaduras, cada um desempenhando uma função específica, incluindo transmissão de energia, comunicação de sinais ou reforço estrutural. Essa estrutura é projetada para suportar as condições de águas profundas, como alta pressão externa e cargas dinâmicas, garantindo a integridade e o desempenho confiável do umbilical ao longo de sua vida útil."@pt-br ,
                                       "The Umbilical Structure is the layered configuration, the specification, of a subsea umbilical, designed to provide mechanical protection, flexibility, and stability in underwater environments. It consists of multiple layers and components, such as tubes, cables, fillers, and armoring, each serving a specific function, including power transmission, signal communication, or structural reinforcement. This structure is engineered to withstand deepwater conditions, such as high external pressure and dynamic loads, ensuring the umbilical’s integrity and reliable performance throughout its service life.."@en ;
                       skos:prefLabel "Estrutura do Umbilical"@pt-br ,
                                      "Umbilical Structure"@en ;
                       edo:hasAttribute edo:AxialStiffness ,
                                        edo:BendingStiffnessStorage ,
                                        edo:BreakingTension ,
                                        edo:CrushingLoad ,
                                        edo:DamagingTension ,
                                        edo:FrictionCoeffSheathArmor ,
                                        edo:FrictionCoeffSheathTensioner ,
                                        edo:LinearWeight ,
                                        edo:LinearWeightFilled ,
                                        edo:LinearWeightFilledSubmerged ,
                                        edo:LinearWeightFilledSubmergedFlooded ,
                                        edo:LinearWeightSubmerged ,
                                        edo:MaxDragCoeff ,
                                        edo:MbrDynamicOperation ,
                                        edo:MbrStaticOperation ,
                                        edo:MinDragoeff ,
                                        edo:MinimumBendingRadius ,
                                        edo:MinimumBendingRadiusForStorage ,
                                        edo:OuterArea ,
                                        edo:SpecificMass ,
                                        edo:SpoolingTension ,
                                        edo:TorsionalStiffnessHigherStorage ,
                                        edo:TorsionalStiffnessLowerStorage ,
                                        edo:WorkingTension ;
                       edo:hasDiscipline edo:SubseaUmbilicalsEngineering ;
                       edo:ifc_equivalentClass "IfcPipeSegmentType" ;
                       edo:ifc_objectType "UmbilicalStructure" ;
                       edo:ifc_predefinedType "USERDEFINED" .


###  https://w3id.org/energy-domain/edo#UnifilarDiagram
edo:UnifilarDiagram rdf:type owl:Class ;
                    rdfs:subClassOf edo:DomainAttribute ;
                    dcterms:accessRights "PUBLIC" ;
                    dcterms:identifier "UnifilarDiagram" ;
                    skos:definition "A simplified schematic illustrates the arrangement of flexible pipeline sections and their associated accessories, such as end fittings and clamps. This diagram shows how these sections and accessories are connected, providing a clear overview of the pipeline configuration without detailing internal structures. It is used to aid in planning, installation, and understanding of the flexible pipeline system by visualizing the main components and their positions."@en ;
                    skos:prefLabel "Código do Diagrama Unifilar"@pt-br ,
                                   "Unifilar Diagram"@en ;
                    edo:hasAttributeScope edo:InstanceLevelAttribute ;
                    edo:hasLifecycleCreationPhase edo:DetailedDesign ;
                    edo:hasTypedValue edo:StringValue ;
                    edo:hasValueCardinality edo:SingleValue .


###  https://w3id.org/energy-domain/edo#UnifilarDiagramRev
edo:UnifilarDiagramRev rdf:type owl:Class ;
                       rdfs:subClassOf edo:DomainAttribute ;
                       dcterms:accessRights "PUBLIC" ;
                       dcterms:identifier "UnifilarDiagramRev" ;
                       skos:definition "Indicates the revision number of the unifilar diagram, reflecting updates or changes made to the arrangement of pipeline sections and their accessories. Each revision ensures that the latest configuration is accurately documented for installation and planning purposes."@en ;
                       skos:prefLabel "Número da Revisão do Diagrama Unifilar"@pt-br ,
                                      "Unifilar Diagram Revision"@en ;
                       edo:hasAttributeScope edo:InstanceLevelAttribute ;
                       edo:hasLifecycleCreationPhase edo:DetailedDesign ;
                       edo:hasTypedValue edo:StringValue ;
                       edo:hasValueCardinality edo:SingleValue .


###  https://w3id.org/energy-domain/edo#UpperItubeDiameter
edo:UpperItubeDiameter rdf:type owl:Class ;
                       rdfs:subClassOf edo:DomainAttribute ;
                       dcterms:accessRights "PUBLIC" ;
                       dcterms:identifier "UpperItubeDiameter" ;
                       skos:definition "Diameter of the upper section of the tube or pipe. This measurement is important for ensuring proper fit and compatibility with other components or connections. The diameter of the upper section affects the alignment and sealing capabilities of the assembly, and ensures that the tube or pipe meets the design and operational requirements for the installation or application."@en ;
                       skos:prefLabel "Diâmetro do I-TUBE superior"@pt-br ,
                                      "Upper I-tube Diameter"@en ;
                       edo:hasAttributeScope edo:TypeLevelAttribute ;
                       edo:hasLifecycleCreationPhase edo:DetailedDesign ;
                       edo:hasTypedValue edo:FloatValue ;
                       edo:hasUnit unit:M ;
                       edo:hasValueCardinality edo:SingleValue .


###  https://w3id.org/energy-domain/edo#Upstream
edo:Upstream rdf:type owl:Class ;
             rdfs:subClassOf edo:OilAndGas ;
             rdfs:label "Upstream"@en ,
                        "Upstream"@pt-br ;
             skos:definition "Oil & Gas sector covering exploration, drilling, and production of hydrocarbon resources."@en ,
                             "Setor de Petróleo & Gás que abrange exploração, perfuração e produção de recursos de hidrocarbonetos."@pt-br .


###  https://w3id.org/energy-domain/edo#UtilityPipingEngineering
edo:UtilityPipingEngineering rdf:type owl:Class ;
                             rdfs:subClassOf edo:TechnicalDiscipline ;
                             rdfs:label "Engenharia de Tubulação de Utilidades"@pt-br ,
                                        "Utility Piping Engineering"@en ;
                             skos:definition "Disciplina de engenharia focada no projeto de sistemas de tubulação para serviços de utilidades."@pt-br ,
                                             "Engineering discipline focused on the design of piping systems for utility services."@en .


###  https://w3id.org/energy-domain/edo#UtilizationFactor
edo:UtilizationFactor rdf:type owl:Class ;
                      rdfs:subClassOf edo:CrushingFrictionCoefficientTighteningAttribute ,
                                      edo:CrushingMaximumAllowableTensionAttribute ,
                                      edo:CrushingMaximumAllowableTighteningAttribute ;
                      dcterms:accessRights "PUBLIC" ;
                      dcterms:identifier "UtilizationFactor" ;
                      skos:definition "Represents the ratio used to determine the level of utilisation, indicating how much of the system’s capacity is being used under given conditions. This factor is crucial for assessing whether the structure operates within safe limits or approaching its maximum capacity."@en ;
                      skos:prefLabel "Fator de Utilização"@pt-br ,
                                     "Utilization Factor"@en ;
                      edo:hasAttributeScope edo:TypeLevelAttribute ;
                      edo:hasLifecycleCreationPhase edo:DetailedDesign ;
                      edo:hasTypedValue edo:FloatValue ;
                      edo:hasValueCardinality edo:SingleValue .


###  https://w3id.org/energy-domain/edo#VCM
edo:VCM rdf:type owl:Class ;
        rdfs:subClassOf edo:ConnectionModule ;
        dcterms:identifier "VCM" ;
        skos:prefLabel "Módulo de conexão vertical"@pt-br ,
                       "Vertical connection module"@en ;
        edo:hasDiscipline edo:WetChristmasTreesEngineering .


###  https://w3id.org/energy-domain/edo#ValueNature
edo:ValueNature rdf:type owl:Class ;
                rdfs:subClassOf edo:AttributeClassification .


###  https://w3id.org/energy-domain/edo#ValueOrigin
edo:ValueOrigin rdf:type owl:Class ;
                rdfs:subClassOf edo:AttributeNature ;
                rdfs:comment "Indicates how the value is obtained."@en ;
                rdfs:label "Origem do Valor"@pt-br ,
                           "Value Origin"@en ;
                skos:definition "Indica como o valor é obtido"@pt-br ,
                                "Indicates how the value is obtained"@en .


###  https://w3id.org/energy-domain/edo#Valve
edo:Valve rdf:type owl:Class ;
          rdfs:subClassOf edo:PressureComponent ;
          dcterms:identifier "Valve" ;
          skos:prefLabel "Valve"@en ,
                         "Válvula"@pt-br .


###  https://w3id.org/energy-domain/edo#Version
edo:Version rdf:type owl:Class ;
            rdfs:subClassOf edo:ContentManagementAttribute .


###  https://w3id.org/energy-domain/edo#Vessel
edo:Vessel rdf:type owl:Class ;
           rdfs:subClassOf edo:PressureComponent ;
           dcterms:identifier "Vessel" ;
           skos:prefLabel "Vaso"@pt-br ,
                          "Vessel"@en .


###  https://w3id.org/energy-domain/edo#VoltageRatingTableAttribute
edo:VoltageRatingTableAttribute rdf:type owl:Class ;
                                rdfs:subClassOf edo:DomainAttribute ;
                                rdfs:label "Voltage Rating Table" .


###  https://w3id.org/energy-domain/edo#VoltageRatingTableColumn
edo:VoltageRatingTableColumn rdf:type owl:Class ;
                             rdfs:subClassOf edo:VoltageRatingTableAttribute .


###  https://w3id.org/energy-domain/edo#VoltageRating_MaximumLineVoltage
edo:VoltageRating_MaximumLineVoltage rdf:type owl:Class ;
                                     rdfs:subClassOf edo:VoltageRatingTableColumn ;
                                     dcterms:accessRights "PUBLIC" ;
                                     dcterms:identifier "VoltageRating_MaximumLineVoltage" ;
                                     rdfs:comment "Tensão máxima tolerada, na frequência de alimentação, entre qualquer par de condutores de fase"@pt-br ;
                                     skos:definition "Maximum tolerated voltage at power frequency between any pair of phase conductors"@en ;
                                     skos:prefLabel "Maximum line voltage (U)"@en ,
                                                    "Tensão de linha máxima (U)"@pt-br ;
                                     edo:hasAttributeScope edo:TypeLevelAttribute ;
                                     edo:hasLifecycleCreationPhase edo:DetailedDesign ;
                                     edo:hasTypedValue edo:FloatValue ;
                                     edo:hasUnit unit:KiloV ;
                                     edo:hasValueCardinality edo:SingleValue .


###  https://w3id.org/energy-domain/edo#VoltageRating_MaximumPhaseVoltage
edo:VoltageRating_MaximumPhaseVoltage rdf:type owl:Class ;
                                      rdfs:subClassOf edo:VoltageRatingTableColumn ;
                                      dcterms:accessRights "PUBLIC" ;
                                      dcterms:identifier "VoltageRating_MaximumPhaseVoltage" ;
                                      rdfs:comment "Tensão máxima tolerada, na frequência de alimentação, entre qualquer condutor de fase e a Terra"@pt-br ;
                                      skos:definition "Maximum tolerated voltage at power frequency between any phase conductor and the Earth"@en ;
                                      skos:prefLabel "Maximum phase voltage (Uo)"@en ,
                                                     "Tensão de fase máxima (Uo)"@pt-br ;
                                      edo:hasAttributeScope edo:TypeLevelAttribute ;
                                      edo:hasLifecycleCreationPhase edo:DetailedDesign ;
                                      edo:hasTypedValue edo:FloatValue ;
                                      edo:hasUnit unit:KiloV ;
                                      edo:hasValueCardinality edo:SingleValue .


###  https://w3id.org/energy-domain/edo#VoltageRating_MaximumSystemVoltage
edo:VoltageRating_MaximumSystemVoltage rdf:type owl:Class ;
                                       rdfs:subClassOf edo:VoltageRatingTableColumn ;
                                       dcterms:accessRights "PUBLIC" ;
                                       dcterms:identifier "VoltageRating_MaximumSystemVoltage" ;
                                       rdfs:comment "Maior tensão do sistema conforme IEC 60038"@pt-br ;
                                       skos:definition "Highest system voltage as per IEC 60038"@en ;
                                       skos:prefLabel "Maior tensão do sistema (Um)"@pt-br ,
                                                      "Maximum system voltage (Um)"@en ;
                                       edo:hasAttributeScope edo:TypeLevelAttribute ;
                                       edo:hasLifecycleCreationPhase edo:DetailedDesign ;
                                       edo:hasTypedValue edo:FloatValue ;
                                       edo:hasUnit unit:KiloV ;
                                       edo:hasValueCardinality edo:SingleValue .


###  https://w3id.org/energy-domain/edo#WasteToEnergy
edo:WasteToEnergy rdf:type owl:Class ;
                  rdfs:subClassOf edo:Biomass ;
                  dcterms:identifier "WasteToEnergy" ;
                  skos:definition "Energia a partir de resíduos de biomassa refere-se à conversão da fração orgânica de resíduos urbanos e industriais em energia útil por meio de processos como combustão, gaseificação ou digestão anaeróbica."@pt-br ,
                                  "Waste-to-energy from biomass refers to the conversion of the organic fraction of municipal and industrial waste into useful energy through processes such as combustion, gasification, or anaerobic digestion."@en ;
                  skos:prefLabel "Energia a partir de Resíduos"@pt-br ,
                                 "Waste to Energy"@en .


###  https://w3id.org/energy-domain/edo#WaterIntake
edo:WaterIntake rdf:type owl:Class ;
                rdfs:subClassOf edo:SubseaEquipment ;
                dcterms:identifier "WaterIntake" ;
                skos:prefLabel "Captador de Água"@pt-br ,
                               "Water Intake"@en .


###  https://w3id.org/energy-domain/edo#Wave
edo:Wave rdf:type owl:Class ;
         rdfs:subClassOf edo:Marine ;
         dcterms:identifier "Wave" ;
         skos:definition "Energia das ondas captura a energia cinética e potencial das ondas de superfície do oceano usando dispositivos flutuantes ou submersos. É considerada uma tecnologia promissora, porém ainda emergente, capaz de fornecer eletricidade renovável de forma consistente em regiões costeiras."@pt-br ,
                         "Wave energy captures the kinetic and potential energy of surface ocean waves using floating or submerged devices. It is considered a promising but still emerging technology, capable of providing consistent renewable electricity near coastal regions."@en ;
         skos:prefLabel "Energia das Ondas"@pt-br ,
                        "Wave Energy"@en .


###  https://w3id.org/energy-domain/edo#WearBushing
edo:WearBushing rdf:type owl:Class ;
                rdfs:subClassOf edo:Accessory ;
                dcterms:identifier "WearBushing" ;
                skos:definition "Accessory for protecting delicate surfaces in the flowbase during downhole interventions"@en ,
                                "Acessório para proteção de superfícies delicadas na BAP durante intervenções no poço"@pt-br ;
                skos:prefLabel "Bucha de Desgaste"@pt-br ,
                               "Wear Bushing"@en .


###  https://w3id.org/energy-domain/edo#WearBushingRunningTool
edo:WearBushingRunningTool rdf:type owl:Class ;
                           rdfs:subClassOf edo:RunningTool ;
                           dcterms:identifier "WearBushingRunningTool" ;
                           skos:prefLabel "Ferramenta de instalação de BD"@pt-br ,
                                          "Wear bushing running tool"@en .


###  https://w3id.org/energy-domain/edo#WeightInWater
edo:WeightInWater rdf:type owl:Class ;
                  rdfs:subClassOf edo:DomainAttribute ;
                  dcterms:accessRights "PUBLIC" ;
                  dcterms:identifier "WeightInWater" ;
                  rdfs:comment "Peso efetivo quando submerso, descontando-se o empuxo"@pt-br ;
                  skos:definition "Effective weight when submerged, subtracting upthrust"@en ;
                  skos:prefLabel "Peso na água"@pt-br ,
                                 "Weight in water"@en ;
                  edo:hasAttributeScope edo:TypeLevelAttribute ;
                  edo:hasLifecycleCreationPhase edo:DetailedDesign ;
                  edo:hasTypedValue edo:FloatValue ;
                  edo:hasUnit unit:KiloGM_F ;
                  edo:hasValueCardinality edo:SingleValue .


###  https://w3id.org/energy-domain/edo#WeldedConnection
edo:WeldedConnection rdf:type owl:Class ;
                     rdfs:subClassOf edo:FluidPort ;
                     dcterms:identifier "WeldedConnection" ;
                     skos:definition "Representa uma conexão de porta de fluido realizada por soldagem, formando uma junta permanente. Também define a localização lógica em um modelo onde os componentes de distribuição de fluido são unidos, garantindo o alinhamento e a funcionalidade corretos durante a montagem e a operação. Essa conexão lógica é essencial para definir a interface entre elementos de distribuição de fluido em sistemas submarinos ou outros sistemas de manuseio de fluido."@pt-br ,
                                     "Represents a fluid port connection achieved by welding, forming a permanent joint. It also defines the logical location within a model where fluid distribution components are joined, ensuring proper alignment and functionality during assembly and operation. This logical connection is essential for defining the interface between fluid distribution elements in subsea systems or other fluid handling applications."@en ;
                     skos:prefLabel "Conexão Soldada"@pt-br ,
                                    "Welded Connection"@en ;
                     edo:ifc_equivalentClass "IfcDistributionPort" ;
                     edo:ifc_objectType "WeldedConnection" ;
                     edo:ifc_predefinedType "USERDEFINED" .


###  https://w3id.org/energy-domain/edo#Wellhead
edo:Wellhead rdf:type owl:Class ;
             rdfs:subClassOf edo:Structure ;
             dcterms:identifier "Wellhead" ;
             skos:prefLabel "Cabeça de poço"@pt-br ,
                            "Wellhead"@en .


###  https://w3id.org/energy-domain/edo#WetChristmasTree
edo:WetChristmasTree rdf:type owl:Class ;
                     rdfs:subClassOf edo:FlowControlEquipment ;
                     dcterms:identifier "WetChristmasTree" ;
                     skos:definition "Equipamento composto por válvulas e instrumentos que permite controlar diretamente os fluidos de/para um poço"@pt-br ,
                                     "Piece of equipment containing valves and instrumentation allowing direct control of flow from/to a well"@en ;
                     skos:prefLabel "Wet Christmas tree"@en ,
                                    "Árvore de Natal molhada"@pt-br ;
                     edo:hasDiscipline edo:WetChristmasTreesEngineering ;
                     edo:ifc_objectType "WetChristmasTree" ;
                     edo:ifc_predefinedType "USERDEFINED" .


###  https://w3id.org/energy-domain/edo#WetChristmasTreesEngineering
edo:WetChristmasTreesEngineering rdf:type owl:Class ;
                                 rdfs:subClassOf edo:SubseaEngineering .


###  https://w3id.org/energy-domain/edo#Wind
edo:Wind rdf:type owl:Class ;
         rdfs:subClassOf edo:Renewable ;
         rdfs:label "Energia Eólica"@pt-br ,
                    "Wind Energy"@en ;
         skos:definition "Energia gerada a partir do vento usando turbinas e tecnologias relacionadas."@pt-br ,
                         "Energy generated from wind using turbines and related technologies."@en .


###  https://w3id.org/energy-domain/edo#WireLayer
edo:WireLayer rdf:type owl:Class ;
              rdfs:subClassOf edo:ArmourLayer ;
              dcterms:identifier "WireLayer" ;
              skos:definition "Basis for all wired layers."@en ;
              skos:prefLabel "Camada de Arame"@pt-br ,
                             "Wire Layer"@en .


###  https://w3id.org/energy-domain/edo#WireRopeQuantity
edo:WireRopeQuantity rdf:type owl:Class ;
                     rdfs:subClassOf edo:DomainAttribute ;
                     dcterms:accessRights "PUBLIC" ;
                     dcterms:identifier "WireRopeQuantity" ;
                     skos:definition "Indicates the number of wire ropes required or used for installation or operation"@en ;
                     skos:prefLabel "Quantidade de cordas de Aço"@pt-br ,
                                    "Wire Rope Quantity"@en ;
                     edo:hasAttributeScope edo:TypeLevelAttribute ;
                     edo:hasLifecycleCreationPhase edo:DetailedDesign ;
                     edo:hasTypedValue edo:IntValue ;
                     edo:hasValueCardinality edo:SingleValue .


###  https://w3id.org/energy-domain/edo#WireRopeSegment
edo:WireRopeSegment rdf:type owl:Class ;
                    rdfs:subClassOf edo:RopeSegment ;
                    dcterms:identifier "WireRopeSegment" ;
                    skos:prefLabel "Tramo de cabo de aço"@pt-br ,
                                   "Wire rope segment"@en .


###  https://w3id.org/energy-domain/edo#WireRopeSlingDiameter
edo:WireRopeSlingDiameter rdf:type owl:Class ;
                          rdfs:subClassOf edo:DomainAttribute ;
                          dcterms:accessRights "PUBLIC" ;
                          dcterms:identifier "WireRopeSlingDiameter" ;
                          skos:definition "Diâmetro do Estrobo de Corda de Aço"@pt-br ,
                                          "Specifies the diameter of the wire rope sling. This property provides the measurement of the thickness of the wire rope, which is important for determining its strength and load-bearing capacity."@en ;
                          skos:prefLabel "Diâmetro da eslinga da corda de aço"@pt-br ,
                                         "Wire Rope Sling Diameter"@en ;
                          edo:hasAttributeScope edo:TypeLevelAttribute ;
                          edo:hasLifecycleCreationPhase edo:DetailedDesign ;
                          edo:hasTypedValue edo:FloatValue ;
                          edo:hasUnit unit:M ;
                          edo:hasValueCardinality edo:SingleValue .


###  https://w3id.org/energy-domain/edo#WireRopeSlingLength
edo:WireRopeSlingLength rdf:type owl:Class ;
                        rdfs:subClassOf edo:DomainAttribute ;
                        dcterms:accessRights "PUBLIC" ;
                        dcterms:identifier "WireRopeSlingLength" ;
                        skos:definition "Specifies the length of the wire rope sling used in the installation or operation. This property provides the measurement of the sling’s length, which is essential for ensuring proper fit and functionality during use."@en ;
                        skos:prefLabel "Comprimento da eslinga da corda de aço"@pt-br ,
                                       "Wire Rope Sling Length"@en ;
                        edo:hasAttributeScope edo:TypeLevelAttribute ;
                        edo:hasLifecycleCreationPhase edo:DetailedDesign ;
                        edo:hasTypedValue edo:FloatValue ;
                        edo:hasUnit unit:M ;
                        edo:hasValueCardinality edo:SingleValue .


###  https://w3id.org/energy-domain/edo#WorkingLoadLimit
edo:WorkingLoadLimit rdf:type owl:Class ;
                     rdfs:subClassOf edo:DomainAttribute ;
                     dcterms:accessRights "PUBLIC" ;
                     dcterms:identifier "WorkingLoadLimit" ;
                     skos:definition "The Working Load Limit (WLL) refers to the maximum load that a component, such as a shackle, lifting device, or anchor, is designed to safely support under normal operating conditions."@en ;
                     skos:prefLabel "Limite de Carga de Trabalho"@pt-br ,
                                    "Working Load Limit (WLL)"@en ;
                     edo:hasAttributeScope edo:InstanceLevelAttribute ;
                     edo:hasLifecycleCreationPhase edo:DetailedDesign ;
                     edo:hasTypedValue edo:FloatValue ;
                     edo:hasUnit unit:KiloGM ;
                     edo:hasValueCardinality edo:SingleValue .


###  https://w3id.org/energy-domain/edo#WorkingTension
edo:WorkingTension rdf:type owl:Class ;
                   rdfs:subClassOf edo:DomainAttribute ;
                   dcterms:accessRights "PUBLIC" ;
                   dcterms:identifier "WorkingTension" ;
                   skos:definition "Working tension"@en ;
                   skos:prefLabel "Tensão de trabalho"@pt-br ,
                                  "Working tension"@en ;
                   edo:hasUnit unit:KiloN .


###  https://w3id.org/energy-domain/edo#WoundLayer
edo:WoundLayer rdf:type owl:Class ;
               rdfs:subClassOf edo:FlexibleStructureLayer ;
               dcterms:identifier "WoundLayer" ;
               skos:definition "Base para todas as camadas construídas pelo enrolamento helicoidal de um ou mais elementos"@pt-br ,
                               "Basis for all layers constructed by helical winding of one or more elements."@en ;
               skos:prefLabel "Camada Espiralada"@pt-br ,
                              "Wound Layer"@en .


#################################################################
#    Individuals
#################################################################

###  http://qudt.org/vocab/unit/A
unit:A rdf:type owl:NamedIndividual ,
                qudt:Unit ,
                edo:DomainUnit ;
       dcterms:source "QUDT Units Vocabulary"@en ;
       qudt:conversionMultiplier 1.0 ;
       qudt:definedUnitOfSystem sou:SI ;
       qudt:hasQuantityKind qudt:ElectricCurrent ;
       qudt:symbol "A" ;
       qudt:ucumCode "A" ;
       rdfs:comment "Unit of electric current"@en ;
       rdfs:isDefinedBy unit:A ;
       rdfs:label "Ampere"@en .


###  http://qudt.org/vocab/unit/BAR
unit:BAR rdf:type owl:NamedIndividual ,
                  qudt:Unit ,
                  edo:DomainUnit ;
         dcterms:source "QUDT Units Vocabulary"@en ;
         qudt:conversionMultiplier "100000.0"^^xsd:double ;
         qudt:definedUnitOfSystem sou:NonSI ;
         qudt:hasQuantityKind qudt:Pressure ;
         qudt:symbol "bar" ;
         qudt:ucumCode "bar" ;
         rdfs:comment "Non-SI unit of pressure equal to 100,000 pascals."@en ;
         rdfs:isDefinedBy unit:BAR ;
         rdfs:label "Bar"@en .


###  http://qudt.org/vocab/unit/DB-PER-KM
unit:DB-PER-KM rdf:type owl:NamedIndividual ,
                        qudt:Unit ,
                        edo:DomainUnit ;
               dcterms:source "QUDT Units Vocabulary"@en ;
               qudt:conversionMultiplier 1.0 ;
               qudt:definedUnitOfSystem sou:SI ;
               qudt:hasQuantityKind qudt:LogarithmicRatioPerLength ;
               qudt:symbol "dB/km" ;
               qudt:ucumCode "dB.KM-1" ;
               rdfs:comment "Unit of signal attenuation per distance, commonly used in telecommunications."@en ;
               rdfs:isDefinedBy unit:DB-PER-KM ;
               rdfs:label "Decibel per Kilometer"@en .


###  http://qudt.org/vocab/unit/DEG
unit:DEG rdf:type owl:NamedIndividual ,
                  qudt:Unit ,
                  edo:DomainUnit ;
         dcterms:source "QUDT Units Vocabulary"@en ;
         qudt:conversionMultiplier 0.017453292519943295 ;
         qudt:definedUnitOfSystem sou:SI ;
         qudt:hasQuantityKind qudt:PlaneAngle ;
         qudt:symbol "°" ;
         qudt:ucumCode "DEG" ;
         rdfs:comment "Unit of plane angle measurement"@en ;
         rdfs:isDefinedBy unit:DEG ;
         rdfs:label "Degree"@en .


###  http://qudt.org/vocab/unit/DEG_C
unit:DEG_C rdf:type owl:NamedIndividual ,
                    qudt:Unit ,
                    edo:DomainUnit ;
           dcterms:source "QUDT Units Vocabulary"@en ;
           qudt:conversionMultiplier 1.0 ;
           qudt:definedUnitOfSystem sou:SI ;
           qudt:hasQuantityKind qudt:ThermodynamicTemperature ;
           qudt:symbol "°C" ;
           qudt:ucumCode "degC" ;
           rdfs:comment "Unit of temperature equal to one kelvin difference but offset by 273.15 from absolute zero."@en ;
           rdfs:isDefinedBy unit:DEG-C ;
           rdfs:label "Degree Celsius"@en .


###  http://qudt.org/vocab/unit/DM2
unit:DM2 rdf:type owl:NamedIndividual ,
                  qudt:Unit ,
                  edo:DomainUnit ;
         dcterms:source "QUDT Units Vocabulary"@en ;
         qudt:conversionMultiplier 0.01 ;
         qudt:definedUnitOfSystem sou:SI ;
         qudt:hasQuantityKind qudt:Area ;
         qudt:symbol "dm²" ;
         qudt:ucumCode "DM2" ;
         rdfs:comment "Unit of area equal to 0.01 square meters."@en ;
         rdfs:isDefinedBy unit:DM2 ;
         rdfs:label "Square Decimeter"@en .


###  http://qudt.org/vocab/unit/IN
unit:IN rdf:type owl:NamedIndividual ,
                 qudt:Unit ,
                 edo:DomainUnit ;
        dcterms:source "QUDT Units Vocabulary"@en ;
        qudt:conversionMultiplier 0.0254 ;
        qudt:definedUnitOfSystem sou:Imperial ;
        qudt:hasQuantityKind qudt:Length ;
        qudt:symbol "in" ;
        qudt:ucumCode "IN" ;
        rdfs:comment "Imperial unit of length equal to 1/12 of a foot."@en ;
        rdfs:isDefinedBy unit:IN ;
        rdfs:label "Inch"@en .


###  http://qudt.org/vocab/unit/J-PER-KiloGM-K
unit:J-PER-KiloGM-K rdf:type owl:NamedIndividual ,
                             qudt:Unit ,
                             edo:DomainUnit ;
                    dcterms:source "QUDT Units Vocabulary"@en ;
                    qudt:conversionMultiplier 1.0 ;
                    qudt:definedUnitOfSystem sou:SI ;
                    qudt:hasQuantityKind qudt:SpecificHeatCapacity ;
                    qudt:symbol "J/(kg·K)" ;
                    qudt:ucumCode "J.KG-1.K-1" ;
                    rdfs:comment "Represents energy (in joules) per unit mass (kilogram) per unit temperature (Kelvin)."@en ;
                    rdfs:isDefinedBy unit:J-PER-KG-K ;
                    rdfs:label "Joule per Kilogram-Kelvin"@en .


###  http://qudt.org/vocab/unit/K
unit:K rdf:type owl:NamedIndividual ,
                qudt:Unit ,
                edo:DomainUnit ;
       dcterms:source "QUDT Units Vocabulary"@en ;
       qudt:conversionMultiplier 1.0 ;
       qudt:definedUnitOfSystem sou:SI ;
       qudt:hasQuantityKind qudt:ThermodynamicTemperature ;
       qudt:symbol "K" ;
       qudt:ucumCode "K" ;
       rdfs:comment "Unit of thermodynamic temperature"@en ;
       rdfs:isDefinedBy unit:K ;
       rdfs:label "Kelvin"@en .


###  http://qudt.org/vocab/unit/KiloGM
unit:KiloGM rdf:type owl:NamedIndividual ,
                     qudt:Unit ,
                     edo:DomainUnit ;
            dcterms:source "QUDT Units Vocabulary"@en ;
            qudt:conversionMultiplier 1.0 ;
            qudt:definedUnitOfSystem sou:SI ;
            qudt:hasQuantityKind qudt:Mass ;
            qudt:symbol "kg" ;
            qudt:ucumCode "KG" ;
            rdfs:comment "Unit of mass in the metric system"@en ;
            rdfs:isDefinedBy unit:KG ;
            rdfs:label "Kilogram"@en .


###  http://qudt.org/vocab/unit/KiloGM-PER-M
unit:KiloGM-PER-M rdf:type owl:NamedIndividual ,
                           qudt:Unit ,
                           edo:DomainUnit ;
                  dcterms:source "QUDT Units Vocabulary"@en ;
                  qudt:conversionMultiplier 1.0 ;
                  qudt:definedUnitOfSystem sou:SI ;
                  qudt:hasQuantityKind qudt:LinearMassDensity ;
                  qudt:symbol "kg/m" ;
                  qudt:ucumCode "KG.M-1" ;
                  rdfs:comment "Unit of linear mass density"@en ;
                  rdfs:isDefinedBy unit:KG-PER-M ;
                  rdfs:label "Kilogram per meter"@en .


###  http://qudt.org/vocab/unit/KiloGM-PER-M3
unit:KiloGM-PER-M3 rdf:type owl:NamedIndividual ,
                            qudt:Unit ,
                            edo:DomainUnit ;
                   dcterms:source "QUDT Units Vocabulary"@en ;
                   qudt:conversionMultiplier 1.0 ;
                   qudt:definedUnitOfSystem sou:SI ;
                   qudt:hasQuantityKind qudt:MassDensity ;
                   qudt:symbol "kg/m³" ;
                   qudt:ucumCode "KG.M-3" ;
                   rdfs:comment "Unit of mass density"@en ;
                   rdfs:isDefinedBy unit:KG-PER-M3 ;
                   rdfs:label "Kilogram per cubic meter"@en .


###  http://qudt.org/vocab/unit/KiloGM_F
unit:KiloGM_F rdf:type owl:NamedIndividual ,
                       qudt:Unit ,
                       edo:DomainUnit ;
              dcterms:source "QUDT Units Vocabulary"@en ;
              qudt:conversionMultiplier 9.80665 ;
              qudt:definedUnitOfSystem sou:SI ;
              qudt:hasQuantityKind qudt:Force ;
              qudt:symbol "kgf" ;
              qudt:ucumCode "KGM" ;
              rdfs:comment "Unit of force equal to the force exerted by one kilogram of mass under standard gravity (9.80665 m/s²)."@en ;
              rdfs:isDefinedBy unit:KGF ;
              rdfs:label "Kilogram-force"@en .


###  http://qudt.org/vocab/unit/KiloGM_F-PER-M
unit:KiloGM_F-PER-M rdf:type owl:NamedIndividual ,
                             qudt:Unit ,
                             edo:DomainUnit ;
                    dcterms:source "QUDT Units Vocabulary"@en ;
                    qudt:conversionMultiplier 9.80665 ;
                    qudt:definedUnitOfSystem sou:SI ;
                    qudt:hasQuantityKind qudt:LinearForceDensity ;
                    qudt:symbol "kgf/m" ;
                    qudt:ucumCode "KGF.M-1" ;
                    rdfs:comment "Unit of linear force density, representing one kilogram-force per meter length."@en ;
                    rdfs:isDefinedBy unit:KGF-PER-M ;
                    rdfs:label "Kilogram-force per Meter"@en .


###  http://qudt.org/vocab/unit/KiloN
unit:KiloN rdf:type owl:NamedIndividual ,
                    qudt:Unit ,
                    edo:DomainUnit ;
           dcterms:source "QUDT Units Vocabulary"@en ;
           qudt:conversionMultiplier 1000.0 ;
           qudt:definedUnitOfSystem sou:SI ;
           qudt:hasQuantityKind qudt:Force ;
           qudt:symbol "kN" ;
           qudt:ucumCode "kN" ;
           rdfs:comment "Unit of force equal to 1,000 newtons."@en ;
           rdfs:isDefinedBy unit:KiloN ;
           rdfs:label "Kilonewton"@en .


###  http://qudt.org/vocab/unit/KiloN-M
unit:KiloN-M rdf:type owl:NamedIndividual ,
                      qudt:Unit ,
                      edo:DomainUnit ;
             dcterms:source "QUDT Units Vocabulary"@en ;
             qudt:conversionMultiplier 1000.0 ;
             qudt:definedUnitOfSystem sou:SI ;
             qudt:hasQuantityKind qudt:Torque ;
             qudt:symbol "kN·m" ;
             qudt:ucumCode "kN.M" ;
             rdfs:comment "Unit of moment or torque equal to one kilonewton multiplied by one meter."@en ;
             rdfs:isDefinedBy unit:KiloN-M ;
             rdfs:label "Kilonewton Meter"@en .


###  http://qudt.org/vocab/unit/KiloN-M2
unit:KiloN-M2 rdf:type owl:NamedIndividual ,
                       qudt:Unit ,
                       edo:DomainUnit ;
              dcterms:source "QUDT Units Vocabulary"@en ;
              qudt:conversionMultiplier 1000.0 ;
              qudt:definedUnitOfSystem sou:SI ;
              qudt:hasQuantityKind qudt:MomentOfArea ;
              qudt:symbol "kN·m²" ;
              qudt:ucumCode "kN.M2" ;
              rdfs:comment "Derived unit representing kilonewton times square meter, used in moment of inertia or flexural stiffness."@en ;
              rdfs:isDefinedBy unit:KiloN-M2 ;
              rdfs:label "Kilonewton Square Meter"@en .


###  http://qudt.org/vocab/unit/KiloN-PER-M
unit:KiloN-PER-M rdf:type owl:NamedIndividual ,
                          qudt:Unit ,
                          edo:DomainUnit ;
                 dcterms:source "QUDT Units Vocabulary"@en ;
                 qudt:conversionMultiplier 1000.0 ;
                 qudt:definedUnitOfSystem sou:SI ;
                 qudt:hasQuantityKind qudt:LinearForceDensity ;
                 qudt:symbol "kN/m" ;
                 qudt:ucumCode "kN.M-1" ;
                 rdfs:comment "Unit of linear load or distributed force equal to 1,000 newtons per meter."@en ;
                 rdfs:isDefinedBy unit:KiloN-PER-M ;
                 rdfs:label "Kilonewton per Meter"@en .


###  http://qudt.org/vocab/unit/KiloV
unit:KiloV rdf:type owl:NamedIndividual ,
                    qudt:Unit ,
                    edo:DomainUnit ;
           dcterms:source "QUDT Units Vocabulary"@en ;
           qudt:conversionMultiplier 1000.0 ;
           qudt:definedUnitOfSystem sou:SI ;
           qudt:hasQuantityKind qudt:ElectricPotential ;
           qudt:symbol "kV" ;
           qudt:ucumCode "kV" ;
           rdfs:comment "Unit of electric potential equal to one thousand volts."@en ;
           rdfs:isDefinedBy unit:KiloV ;
           rdfs:label "Kilovolt"@en .


###  http://qudt.org/vocab/unit/M
unit:M rdf:type owl:NamedIndividual ,
                qudt:Unit ,
                edo:DomainUnit ;
       dcterms:source "QUDT Units Vocabulary"@en ;
       qudt:conversionMultiplier 1.0 ;
       qudt:definedUnitOfSystem sou:SI ;
       qudt:hasQuantityKind qudt:Length ;
       qudt:symbol "m" ;
       qudt:ucumCode "M" ;
       rdfs:comment "Unit of length in the metric system"@en ;
       rdfs:isDefinedBy unit:M ;
       rdfs:label "Meter"@en .


###  http://qudt.org/vocab/unit/M2
unit:M2 rdf:type owl:NamedIndividual ,
                 qudt:Unit ,
                 edo:DomainUnit ;
        dcterms:source "QUDT Units Vocabulary"@en ;
        qudt:conversionMultiplier 1.0 ;
        qudt:definedUnitOfSystem sou:SI ;
        qudt:hasQuantityKind qudt:Area ;
        qudt:symbol "m²" ;
        qudt:ucumCode "M2" ;
        rdfs:comment "Unit of area in the metric system"@en ;
        rdfs:isDefinedBy unit:M2 ;
        rdfs:label "Square meter"@en .


###  http://qudt.org/vocab/unit/M2-PER-SEC
unit:M2-PER-SEC rdf:type owl:NamedIndividual ,
                         qudt:Unit ,
                         edo:DomainUnit ;
                dcterms:source "QUDT Units Vocabulary"@en ;
                qudt:conversionMultiplier 1.0 ;
                qudt:definedUnitOfSystem sou:SI ;
                qudt:hasFactorUnit [ qudt:exponent -1 ;
                                     qudt:hasUnit unit:S
                                   ] ,
                                   [ qudt:exponent 2 ;
                                     qudt:hasUnit unit:M
                                   ] ;
                qudt:hasQuantityKind qudt:AreaFlux ;
                qudt:symbol "m²/s" ;
                qudt:ucumCode "M2.S-1" ;
                rdfs:comment "Unit of area flux or similar rates per unit time"@en ;
                rdfs:isDefinedBy unit:M2-PER-SEC ;
                rdfs:label "Square meter per second"@en .


###  http://qudt.org/vocab/unit/M3
unit:M3 rdf:type owl:NamedIndividual ,
                 qudt:Unit ,
                 edo:DomainUnit ;
        dcterms:source "QUDT Units Vocabulary"@en ;
        qudt:conversionMultiplier 1.0 ;
        qudt:definedUnitOfSystem sou:SI ;
        qudt:hasQuantityKind qudt:Volume ;
        qudt:symbol "m³" ;
        qudt:ucumCode "M3" ;
        rdfs:comment "Unit of volume in the metric system"@en ;
        rdfs:isDefinedBy unit:M3 ;
        rdfs:label "Cubic meter"@en .


###  http://qudt.org/vocab/unit/M4
unit:M4 rdf:type owl:NamedIndividual ,
                 qudt:Unit ,
                 edo:DomainUnit ;
        dcterms:source "QUDT Units Vocabulary"@en ;
        qudt:conversionMultiplier 1.0 ;
        qudt:definedUnitOfSystem sou:SI ;
        qudt:hasQuantityKind qudt:AreaMoment ;
        qudt:symbol "m⁴" ;
        qudt:ucumCode "M4" ;
        rdfs:comment "Derived unit for moments of area (e.g., beam bending calculations)"@en ;
        rdfs:isDefinedBy unit:M4 ;
        rdfs:label "Meter to the fourth power"@en .


###  http://qudt.org/vocab/unit/MM2
unit:MM2 rdf:type owl:NamedIndividual ,
                  qudt:Unit ,
                  edo:DomainUnit ;
         dcterms:source "QUDT Units Vocabulary"@en ;
         qudt:conversionMultiplier "1.0E-6"^^xsd:double ;
         qudt:definedUnitOfSystem sou:SI ;
         qudt:hasQuantityKind qudt:Area ;
         qudt:symbol "mm²" ;
         qudt:ucumCode "MM2" ;
         rdfs:comment "Unit of area equal to one millionth of a square meter."@en ;
         rdfs:isDefinedBy unit:MM2 ;
         rdfs:label "Square Millimeter"@en .


###  http://qudt.org/vocab/unit/MOL-PER-M3-PA
unit:MOL-PER-M3-PA rdf:type owl:NamedIndividual ,
                            qudt:Unit ,
                            edo:DomainUnit ;
                   dcterms:source "QUDT Units Vocabulary"@en ;
                   qudt:conversionMultiplier 1.0 ;
                   qudt:definedUnitOfSystem sou:SI ;
                   qudt:hasQuantityKind qudt:MolarDensityPerPressure ;
                   qudt:symbol "mol/(m³·Pa)" ;
                   qudt:ucumCode "MOL.M-3.PA-1" ;
                   rdfs:comment "Represents the amount of substance (in moles) per cubic meter per Pascal of pressure."@en ;
                   rdfs:isDefinedBy unit:MOL-PER-M3-PA ;
                   rdfs:label "Mole per cubic meter per Pascal"@en .


###  http://qudt.org/vocab/unit/MPa
unit:MPa rdf:type owl:NamedIndividual ,
                  qudt:Unit ,
                  edo:DomainUnit ;
         dcterms:source "QUDT Units Vocabulary"@en ;
         qudt:conversionMultiplier "1000000.0"^^xsd:double ;
         qudt:definedUnitOfSystem sou:SI ;
         qudt:hasQuantityKind qudt:Pressure ;
         qudt:symbol "MPa" ;
         qudt:ucumCode "MPa" ;
         rdfs:comment "Unit of pressure equal to one million pascals."@en ;
         rdfs:isDefinedBy unit:MPa ;
         rdfs:label "Megapascal"@en .


###  http://qudt.org/vocab/unit/MicroM
unit:MicroM rdf:type owl:NamedIndividual ,
                     qudt:Unit ,
                     edo:DomainUnit ;
            dcterms:source "QUDT Units Vocabulary"@en ;
            qudt:conversionMultiplier "1.0E-6"^^xsd:double ;
            qudt:definedUnitOfSystem sou:SI ;
            qudt:hasQuantityKind qudt:Length ;
            qudt:symbol "µm" ;
            qudt:ucumCode "UM" ;
            rdfs:comment "Unit of length equal to one millionth of a meter."@en ;
            rdfs:isDefinedBy unit:MicroM ;
            rdfs:label "Micrometer"@en .


###  http://qudt.org/vocab/unit/MicroM3-PER-M3
unit:MicroM3-PER-M3 rdf:type owl:NamedIndividual ,
                             qudt:Unit ,
                             edo:DomainUnit ;
                    dcterms:source "QUDT Units Vocabulary"@en ;
                    qudt:conversionMultiplier "1.0E-18"^^xsd:double ;
                    qudt:definedUnitOfSystem sou:SI ;
                    qudt:hasQuantityKind qudt:Dimensionless ;
                    qudt:symbol "µm³/m³" ;
                    qudt:ucumCode "UM3.M-3" ;
                    rdfs:comment "Custom unit representing volume fraction"@en ;
                    rdfs:isDefinedBy unit:MICRO-M3-PER-M3 ;
                    rdfs:label "Micrometre cubic per cubic meter"@en .


###  http://qudt.org/vocab/unit/MilliM
unit:MilliM rdf:type owl:NamedIndividual ,
                     qudt:Unit ,
                     edo:DomainUnit ;
            dcterms:source "QUDT Units Vocabulary"@en ;
            qudt:conversionMultiplier 0.001 ;
            qudt:definedUnitOfSystem sou:SI ;
            qudt:hasFactorUnit [ qudt:exponent 1 ;
                                 qudt:hasUnit unit:M
                               ] ;
            qudt:hasQuantityKind qudt:Length ;
            qudt:symbol "mm" ;
            qudt:ucumCode "MM" ;
            rdfs:comment "Unit of length equal to one thousandth of a meter"@en ;
            rdfs:isDefinedBy unit:MilliM ;
            rdfs:label "Millimeter"@en .


###  http://qudt.org/vocab/unit/N
unit:N rdf:type owl:NamedIndividual ,
                qudt:Unit ,
                edo:DomainUnit ;
       dcterms:source "QUDT Units Vocabulary"@en ;
       qudt:conversionMultiplier 1.0 ;
       qudt:definedUnitOfSystem sou:SI ;
       qudt:hasFactorUnit [ qudt:exponent -2 ;
                            qudt:hasUnit unit:S
                          ] ,
                          [ qudt:exponent 1 ;
                            qudt:hasUnit unit:KG
                          ] ,
                          [ qudt:exponent 1 ;
                            qudt:hasUnit unit:M
                          ] ;
       qudt:hasQuantityKind qudt:Force ;
       qudt:symbol "N" ;
       qudt:ucumCode "N" ;
       rdfs:comment "Unit of force, equal to the force required to accelerate one kilogram of mass at one meter per second squared"@en ;
       rdfs:isDefinedBy unit:N ;
       rdfs:label "Newton"@en .


###  http://qudt.org/vocab/unit/N-M
unit:N-M rdf:type owl:NamedIndividual ,
                  qudt:Unit ,
                  edo:DomainUnit ;
         dcterms:source "QUDT Units Vocabulary"@en ;
         qudt:conversionMultiplier 1.0 ;
         qudt:definedUnitOfSystem sou:SI ;
         qudt:hasFactorUnit [ qudt:exponent 1 ;
                              qudt:hasUnit unit:N
                            ] ,
                            [ qudt:exponent 1 ;
                              qudt:hasUnit unit:M
                            ] ;
         qudt:hasQuantityKind qudt:Torque ;
         qudt:symbol "N·m" ;
         qudt:ucumCode "N.M" ;
         rdfs:comment "Unit of torque or moment, equal to one newton acting at a perpendicular distance of one meter"@en ;
         rdfs:isDefinedBy unit:N-M ;
         rdfs:label "Newton meter"@en .


###  http://qudt.org/vocab/unit/N-M2
unit:N-M2 rdf:type owl:NamedIndividual ,
                   qudt:Unit ,
                   edo:DomainUnit ;
          dcterms:source "QUDT Units Vocabulary"@en ;
          qudt:conversionMultiplier 1.0 ;
          qudt:definedUnitOfSystem sou:SI ;
          qudt:hasQuantityKind qudt:Pressure ;
          qudt:symbol "N/m²" ;
          qudt:ucumCode "N.M-2" ;
          rdfs:comment "Unit of pressure or stress"@en ;
          rdfs:isDefinedBy unit:N-M2 ;
          rdfs:label "Newton per square meter"@en .


###  http://qudt.org/vocab/unit/N-PER-M
unit:N-PER-M rdf:type owl:NamedIndividual ,
                      qudt:Unit ,
                      edo:DomainUnit ;
             dcterms:source "QUDT Units Vocabulary"@en ;
             qudt:conversionMultiplier 1.0 ;
             qudt:definedUnitOfSystem sou:SI ;
             qudt:hasQuantityKind qudt:ForcePerLength ,
                                  qudt:LinearForceDensity ;
             qudt:symbol "N/m" ;
             qudt:ucumCode "N.M-1" ;
             rdfs:comment "SI unit of linear force density or stiffness, representing one newton per meter."@en ,
                          "Unit of force per unit length"@en ;
             rdfs:isDefinedBy unit:N-PER-M ;
             rdfs:label "Newton per Meter"@en ,
                        "Newton per meter"@en .


###  http://qudt.org/vocab/unit/N-PER-M3
unit:N-PER-M3 rdf:type owl:NamedIndividual ,
                       qudt:Unit ,
                       edo:DomainUnit ;
              dcterms:source "QUDT Units Vocabulary"@en ;
              qudt:conversionMultiplier 1.0 ;
              qudt:definedUnitOfSystem sou:SI ;
              qudt:hasQuantityKind qudt:ForcePerVolume ;
              qudt:symbol "N/m³" ;
              qudt:ucumCode "N.M-3" ;
              rdfs:comment "Newton per cubic meter (N/m³) is a unit used to express the amount of force applied within a given volume."@en ;
              rdfs:isDefinedBy unit:N-PER-M3 ;
              rdfs:label "Newton per Cubic Meter"@en .


###  http://qudt.org/vocab/unit/PA
unit:PA rdf:type owl:NamedIndividual ,
                 qudt:Unit ,
                 edo:DomainUnit ;
        dcterms:source "QUDT Units Vocabulary"@en ;
        qudt:conversionMultiplier 1.0 ;
        qudt:definedUnitOfSystem sou:SI ;
        qudt:hasFactorUnit [ qudt:exponent -2 ;
                             qudt:hasUnit unit:M
                           ] ,
                           [ qudt:exponent 1 ;
                             qudt:hasUnit unit:N
                           ] ;
        qudt:hasQuantityKind qudt:Pressure ;
        qudt:symbol "Pa" ;
        qudt:ucumCode "PA" ;
        rdfs:comment "Unit of pressure. The SI unit of pressure, equal to one newton per square meter."@en ;
        rdfs:isDefinedBy unit:PA ;
        rdfs:label "Pascal"@en .


###  http://qudt.org/vocab/unit/PA-M0dot5
unit:PA-M0dot5 rdf:type owl:NamedIndividual ,
                        qudt:Unit ,
                        edo:DomainUnit ;
               dcterms:source "QUDT Units Vocabulary"@en ;
               qudt:conversionMultiplier 1.0 ;
               qudt:definedUnitOfSystem sou:SI ;
               qudt:hasQuantityKind qudt:StressIntensityFactor ;
               qudt:symbol "Pa·m⁰·⁵" ;
               qudt:ucumCode "PA.M0.5" ;
               rdfs:comment "Unit used in fracture mechanics to express stress intensity factor (Pa√m)."@en ;
               rdfs:isDefinedBy unit:PA-M0dot5 ;
               rdfs:label "Pascal times Square Root Meter"@en .


###  http://qudt.org/vocab/unit/PER-M
unit:PER-M rdf:type owl:NamedIndividual ,
                    qudt:Unit ,
                    edo:DomainUnit ;
           dcterms:source "QUDT Units Vocabulary"@en ;
           qudt:conversionMultiplier 1.0 ;
           qudt:definedUnitOfSystem sou:SI ;
           qudt:hasFactorUnit [ qudt:exponent -1 ;
                                qudt:hasUnit unit:M
                              ] ;
           qudt:hasQuantityKind qudt:ReciprocalLength ;
           qudt:symbol "1/m" ;
           qudt:ucumCode "1/M" ;
           rdfs:comment "Reciprocal of meter, used for quantities per unit length"@en ;
           rdfs:isDefinedBy unit:PER-M ;
           rdfs:label "Per meter"@en .


###  http://qudt.org/vocab/unit/PERCENT
unit:PERCENT rdf:type owl:NamedIndividual ,
                      qudt:Unit ,
                      edo:DomainUnit ;
             dcterms:source "QUDT Units Vocabulary"@en ;
             qudt:conversionMultiplier 0.01 ;
             qudt:definedUnitOfSystem sou:SI ;
             qudt:hasQuantityKind qudt:Dimensionless ;
             qudt:symbol "%" ;
             qudt:ucumCode "%" ;
             rdfs:comment "Unit representing a fraction of 100"@en ;
             rdfs:isDefinedBy unit:PERCENT ;
             rdfs:label "Percent"@en .


###  http://qudt.org/vocab/unit/PSI
unit:PSI rdf:type owl:NamedIndividual ,
                  qudt:Unit ,
                  edo:DomainUnit ;
         dcterms:source "QUDT Units Vocabulary"@en ;
         qudt:conversionMultiplier 6894.75729 ;
         qudt:definedUnitOfSystem sou:Imperial ;
         qudt:hasQuantityKind qudt:Pressure ;
         qudt:symbol "psi" ;
         qudt:ucumCode "psi" ;
         rdfs:comment "Imperial unit of pressure equal to one pound-force per square inch."@en ;
         rdfs:isDefinedBy unit:PSI ;
         rdfs:label "Pound-force per Square Inch"@en .


###  http://qudt.org/vocab/unit/TONNE_F
unit:TONNE_F rdf:type owl:NamedIndividual ,
                      qudt:Unit ,
                      edo:DomainUnit ;
             dcterms:source "QUDT Units Vocabulary"@en ;
             qudt:conversionMultiplier 9806.65 ;
             qudt:definedUnitOfSystem sou:SI ;
             qudt:hasQuantityKind qudt:Force ;
             qudt:symbol "tf" ;
             qudt:ucumCode "TF" ;
             rdfs:comment "Unit of force equal to the weight of one metric tonne under standard gravity."@en ;
             rdfs:isDefinedBy unit:TONNE_F ;
             rdfs:label "Tonne-force"@en .


###  http://qudt.org/vocab/unit/V
unit:V rdf:type owl:NamedIndividual ,
                qudt:Unit ,
                edo:DomainUnit ;
       dcterms:source "QUDT Units Vocabulary"@en ;
       qudt:conversionMultiplier 1.0 ;
       qudt:definedUnitOfSystem sou:SI ;
       qudt:hasQuantityKind qudt:ElectricPotential ;
       qudt:symbol "V" ;
       qudt:ucumCode "V" ;
       rdfs:comment "SI unit of electric potential or electromotive force."@en ;
       rdfs:isDefinedBy unit:V ;
       rdfs:label "Volt"@en .


###  http://qudt.org/vocab/unit/W-PER-M-K
unit:W-PER-M-K rdf:type owl:NamedIndividual ,
                        qudt:Unit ,
                        edo:DomainUnit ;
               dcterms:source "QUDT Units Vocabulary"@en ;
               qudt:conversionMultiplier 1.0 ;
               qudt:definedUnitOfSystem sou:SI ;
               qudt:hasQuantityKind qudt:ThermalConductivity ;
               qudt:symbol "W/(m·K)" ;
               qudt:ucumCode "W.M-1.K-1" ;
               rdfs:comment "Unit of thermal conductivity"@en ;
               rdfs:isDefinedBy unit:W-PER-M-K ;
               rdfs:label "Watt per meter kelvin"@en .


###  http://qudt.org/vocab/unit/YR_Common
unit:YR_Common rdf:type owl:NamedIndividual ,
                        qudt:Unit ,
                        edo:DomainUnit ;
               dcterms:source "QUDT Units Vocabulary"@en ;
               qudt:conversionMultiplier 31536000.0 ;
               qudt:definedUnitOfSystem sou:SI ;
               qudt:hasQuantityKind qudt:Time ;
               qudt:symbol "yr" ;
               qudt:ucumCode "a" ;
               rdfs:comment "Unit of time equal to 365 or 366 days."@en ;
               rdfs:isDefinedBy unit:YR ;
               rdfs:label "Year"@en .


###  https://w3id.org/energy-domain/edo#M3-PER-M
edo:M3-PER-M rdf:type owl:NamedIndividual ,
                      edo:DomainUnit ;
             qudt:conversionMultiplier 1.0 ;
             qudt:definedUnitOfSystem sou:SI ;
             qudt:hasFactorUnit [ qudt:exponent 3 ;
                                  qudt:hasUnit unit:M
                                ] ,
                                [ qudt:exponent -1 ;
                                  qudt:hasUnit unit:M
                                ] ;
             qudt:hasQuantityKind qudt:VolumePerLength ;
             qudt:symbol "m³/m" ;
             qudt:ucumCode "M3.M-1" ;
             rdfs:comment "Extended from QUDT model for custom Subsea domain units"@en ;
             rdfs:isDefinedBy <https://w3id.org/energy-domain/edo> ;
             rdfs:label "Cubic meter per meter"@en .


###  https://w3id.org/energy-domain/edo#MOL-PER-M-SEC-PA
edo:MOL-PER-M-SEC-PA rdf:type owl:NamedIndividual ,
                              edo:DomainUnit ;
                     qudt:conversionMultiplier 1.0 ;
                     qudt:definedUnitOfSystem sou:SI ;
                     qudt:hasFactorUnit [ qudt:exponent -1 ;
                                          qudt:hasUnit unit:PA
                                        ] ,
                                        [ qudt:exponent -1 ;
                                          qudt:hasUnit unit:M
                                        ] ,
                                        [ qudt:exponent -1 ;
                                          qudt:hasUnit unit:S
                                        ] ,
                                        [ qudt:exponent 1 ;
                                          qudt:hasUnit unit:MOL
                                        ] ;
                     qudt:hasQuantityKind qudt:MolarFluxPerPressure ;
                     qudt:symbol "mol/(m·s·Pa)" ;
                     qudt:ucumCode "MOL.M-1.S-1.PA-1" ;
                     rdfs:comment "Extended from QUDT model for custom Subsea domain units"@en ;
                     rdfs:isDefinedBy <https://w3id.org/energy-domain/edo> ;
                     rdfs:label "Mole per meter per second per Pascal"@en .


###  https://w3id.org/energy-domain/edo#N-M2-PER-RAD
edo:N-M2-PER-RAD rdf:type owl:NamedIndividual ,
                          edo:DomainUnit ;
                 qudt:conversionMultiplier 1.0 ;
                 qudt:definedUnitOfSystem sou:SI ;
                 qudt:hasFactorUnit [ qudt:exponent -2 ;
                                      qudt:hasUnit unit:M
                                    ] ,
                                    [ qudt:exponent -1 ;
                                      qudt:hasUnit unit:RAD
                                    ] ,
                                    [ qudt:exponent 1 ;
                                      qudt:hasUnit unit:N
                                    ] ;
                 qudt:hasQuantityKind qudt:StressPerAngle ;
                 qudt:symbol "N/m²·rad" ;
                 qudt:ucumCode "N.M-2.RAD-1" ;
                 rdfs:comment "Extended from QUDT model for custom Subsea domain units"@en ;
                 rdfs:isDefinedBy <https://w3id.org/energy-domain/edo> ;
                 rdfs:label "Newton per square meter per radian"@en .


#################################################################
#    Annotations
#################################################################

edo:AbandonmentLife edo:hasUnit unit:YR_Common .


edo:AllowableBendingMoment edo:hasUnit unit:N-M .


edo:Angle edo:hasUnit unit:DEG .


edo:AngleLayingYarnAramid edo:hasUnit unit:DEG ,
                                      unit:W-PER-M-K .


edo:AssyTorquesDry edo:hasUnit unit:N-M .


edo:BendRestrictorForMaxUmbilical edo:hasUnit unit:MilliM .


edo:BodyDiameter edo:hasUnit unit:MilliM .


edo:BrStraightLengthCompressed edo:hasUnit unit:M .


edo:BrStraightLengthExtended edo:hasUnit unit:M .


edo:CrossSectionTable_OuterDiameter edo:hasUnit unit:M .


edo:CrossSectionTable_WeightComponent edo:hasUnit unit:KiloGM .


edo:DesignPressure edo:hasUnit unit:PSI .


edo:Design_Ulor edo:hasUnit unit:M .


edo:EOFWeight_BuoyancyModule edo:hasUnit unit:V .


edo:EquivalentMBR edo:hasUnit unit:M .


edo:FilletRadius edo:hasUnit unit:MilliM .


edo:FinalBuoyancy_EOF edo:hasUnit unit:KiloGM_F .


edo:Flange1_BoreDiameter edo:hasUnit unit:IN .


edo:Flange2_BoreDiameter edo:hasUnit unit:IN .


edo:Height edo:hasUnit unit:MilliM .


edo:HosePressure edo:hasUnit unit:PSI .


edo:InitialBuoyancy_SOL edo:hasUnit unit:KiloGM_F .


edo:LifeSpan edo:hasUnit unit:YR_Common .


edo:LinearWeightDryEmptyAir edo:hasUnit unit:KiloGM_F-PER-M .


edo:LinearWeightDryEmptySubmerged edo:hasUnit unit:KiloGM_F-PER-M .


edo:LinearWeightDryFullAir edo:hasUnit unit:KiloGM_F-PER-M .


edo:LinearWeightDryFullSubmerged edo:hasUnit unit:KiloGM_F-PER-M .


edo:LinearWeightFloodedEmptyAir edo:hasUnit unit:KiloGM_F-PER-M .


edo:LinearWeightFloodedEmptySubmerged edo:hasUnit unit:KiloGM_F-PER-M .


edo:LinearWeightFloodedFullAir edo:hasUnit unit:KiloGM_F-PER-M .


edo:LinearWeightFloodedFullSubmerged edo:hasUnit unit:KiloGM_F-PER-M .


edo:LinearWeightSeawater edo:hasUnit unit:KiloGM_F-PER-M .


edo:LowestLength edo:hasUnit unit:M .


edo:MaxChangeLengthUnderWp edo:hasUnit unit:PERCENT .


edo:MaxInnerTemperature edo:hasUnit unit:DEG_C .


edo:MaxWaterDepth edo:hasUnit unit:M .


edo:MaxWorkingPressure edo:hasUnit unit:BAR .


edo:MaximumVolumetricExpansion edo:hasUnit unit:BAR .


edo:Maximum_Water_Depth edo:hasUnit unit:M .


edo:MbrStorage edo:hasUnit unit:M .


edo:MinBendingRadiusOperation edo:hasUnit unit:MilliM .


edo:MinBendingRadiusStorage edo:hasUnit unit:MilliM .


edo:MinBurstPressureLiner edo:hasUnit unit:BAR .


edo:MinCollapsePressureInMbr edo:hasUnit unit:BAR .


edo:MinCollapsePressureInStraight edo:hasUnit unit:BAR .


edo:MinInnerTemperature edo:hasUnit unit:DEG_C .


edo:MinWaterTemp edo:hasUnit unit:DEG .


edo:MinimumSupportArea edo:hasUnit unit:DM2 .


edo:NominalWeightInAir edo:hasUnit unit:KiloGM_F-PER-M .


edo:RatioWeightODWaterSubmergedUnflooded edo:hasUnit unit:KiloGM_F-PER-M .


edo:RecommendedTorques edo:hasUnit unit:N-PER-M .


edo:SOLWeight_BuoyancyModule edo:hasUnit unit:KiloGM .


edo:SeaWaterDensity edo:hasUnit unit:KiloGM-PER-M3 .


edo:SecuringStrapLength edo:hasUnit unit:MilliM .


edo:ServiceLife edo:hasUnit unit:YR_Common .


edo:SleeveExternalDiameterConnection edo:hasUnit unit:MilliM .


edo:SleeveInnerDiameterConnection edo:hasUnit unit:MilliM .


edo:SleeveInstalationLength edo:hasUnit unit:M .


edo:StorageMinBendingRadius edo:hasUnit unit:MilliM .


edo:StructuralCapacityUnderAxialLoad edo:hasUnit unit:TONNE_F .


edo:Tension edo:hasUnit unit:KiloN-M .


edo:ThermalExchangeCoefficientAt20C edo:hasUnit unit:W-PER-M-K .


edo:TotalAnodeMass edo:hasUnit unit:KiloGM .


edo:UmbilicalCableMBRInstallation edo:hasUnit unit:MilliM .


edo:UmbilicalCableMBROperation edo:hasUnit unit:MilliM .


edo:UmbilicalCableOuterDiameter edo:hasUnit unit:MilliM .


edo:UmbilicalPressure edo:hasUnit unit:BAR .


edo:UtilizationFactorSuperDuplexTube edo:hasUnit unit:PERCENT .


edo:VolumetricExpansion edo:hasUnit unit:BAR .


edo:WaterDepth edo:hasUnit unit:M .


edo:Weight edo:hasUnit unit:KiloGM .


edo:WeightWithoutEndTerminationIn_Air edo:hasUnit unit:KiloGM .


###  Generated by the OWL API (version 4.5.29.2024-05-13T12:11:03Z) https://github.com/owlcs/owlapi
