@prefix : <https://w3id.org/energy-domain/FlexiblePipesDetailedDesign#> .
@prefix edo: <https://w3id.org/energy-domain/edo#> .
@prefix owl: <http://www.w3.org/2002/07/owl#> .
@prefix rdf: <http://www.w3.org/1999/02/22-rdf-syntax-ns#> .
@prefix xml: <http://www.w3.org/XML/1998/namespace> .
@prefix xsd: <http://www.w3.org/2001/XMLSchema#> .
@prefix qudt: <http://qudt.org/schema/qudt/> .
@prefix rdfs: <http://www.w3.org/2000/01/rdf-schema#> .
@prefix skos: <http://www.w3.org/2004/02/skos/core#> .
@prefix unit: <http://qudt.org/vocab/unit/> .
@prefix dcterms: <http://purl.org/dc/terms/> .
@prefix dimension: <http://qudt.org/schema/dimension/> .
@prefix quantitykind: <http://qudt.org/vocab/quantitykind/> .
@base <https://w3id.org/energy-domain/FlexiblePipesDetailedDesign#> .

<https://w3id.org/energy-domain/FlexiblePipesDetailedDesign> rdf:type owl:Ontology ;
                                                              owl:versionIRI <https://w3id.org/energy-domain/FlexiblePipesDetailedDesign/v0.0.1> ;
                                                              dcterms:description "An ontology designed to represent the Detailed Design phase of the engineering discipline of Subsea Flexible Pipes." ;
                                                              dcterms:title "Flexible Pipes Detailed Design" ;
                                                              rdfs:label "Flexible Pipes Detailed Design" ;
                                                              owl:versionInfo "v0.0.1" .

#################################################################
#    Annotation properties
#################################################################

###  http://purl.org/dc/terms/accessRights
dcterms:accessRights rdf:type owl:AnnotationProperty .


###  http://purl.org/dc/terms/description
dcterms:description rdf:type owl:AnnotationProperty .


###  http://purl.org/dc/terms/identifier
dcterms:identifier rdf:type owl:AnnotationProperty .


###  http://purl.org/dc/terms/title
dcterms:title rdf:type owl:AnnotationProperty .


###  http://www.w3.org/2000/01/rdf-schema#subClassOf
rdfs:subClassOf rdf:type owl:AnnotationProperty .


###  http://www.w3.org/2002/07/owl#maxCardinality
owl:maxCardinality rdf:type owl:AnnotationProperty .


###  http://www.w3.org/2002/07/owl#minCardinality
owl:minCardinality rdf:type owl:AnnotationProperty .


###  http://www.w3.org/2004/02/skos/core#altLabel
skos:altLabel rdf:type owl:AnnotationProperty .


###  http://www.w3.org/2004/02/skos/core#definition
skos:definition rdf:type owl:AnnotationProperty .


###  http://www.w3.org/2004/02/skos/core#prefLabel
skos:prefLabel rdf:type owl:AnnotationProperty .


###  https://w3id.org/energy-domain/edo#DomainAnnotation
edo:DomainAnnotation rdf:type owl:AnnotationProperty .


###  https://w3id.org/energy-domain/edo#DomainAuxiliarAnnotation
edo:DomainAuxiliarAnnotation rdf:type owl:AnnotationProperty ;
                             rdfs:subPropertyOf edo:DomainAnnotation .


###  https://w3id.org/energy-domain/edo#DomainEngineeringAnnotation
edo:DomainEngineeringAnnotation rdf:type owl:AnnotationProperty ;
                                rdfs:subPropertyOf edo:DomainAnnotation .


###  https://w3id.org/energy-domain/edo#DomainRelationship
:DomainRelationship rdf:type owl:AnnotationProperty ;
                    rdfs:subPropertyOf :DomainAnnotation .


###  https://w3id.org/energy-domain/edo#appliesTo
edo:appliesTo rdf:type owl:AnnotationProperty ;
              rdfs:label "Applies to"@en ,
                         "Se aplica a"@pt-br ;
              skos:definition "Indica que o sujeito se aplica ao predicado"@pt-br ,
                              "Indicates that the subject applies to the object"@en ;
              rdfs:subPropertyOf edo:DomainAuxiliarAnnotation .


###  https://w3id.org/energy-domain/edo#createdAtLifecyclePhase
edo:createdAtLifecyclePhase rdf:type owl:AnnotationProperty ;
                            rdfs:label "Created at lifecycle phase"@en ,
                                       "Criado na fase do ciclo de vida"@pt-br ;
                            skos:definition "Em que fase do ciclo de vida a informação foi criada"@pt-br ,
                                            "In which lifecycle phase the information was created"@en ;
                            rdfs:subPropertyOf edo:DomainEngineeringAnnotation .


###  https://w3id.org/energy-domain/edo#hasAttribute
edo:hasAttribute rdf:type owl:AnnotationProperty ;
                 rdfs:label "Has attribute"@en ,
                            "Possui atributo"@pt-br ;
                 skos:definition "Indica atributo(s) que a entidade possui"@pt-br ,
                                 "Indicates attribute(s) that the entity has"@en ;
                 rdfs:subPropertyOf edo:DomainAuxiliarAnnotation .


###  https://w3id.org/energy-domain/edo#hasDiscipline
edo:hasDiscipline rdf:type owl:AnnotationProperty ;
                  rdfs:label "Has Discipline"@en ,
                             "Pertence a uma disciplina técnica"@pt-br ;
                  skos:definition "Associa a entidade a uma disciplina técnica"@pt-br ,
                                  "Belongs to a technical discipline"@en ;
                  rdfs:subPropertyOf edo:DomainEngineeringAnnotation .


###  https://w3id.org/energy-domain/edo#hasDomain
edo:hasDomain rdf:type owl:AnnotationProperty ;
              rdfs:label "Has Domain"@en ,
                         "Pertence a um domínio"@pt-br ;
              skos:definition "Associa a entidade a um ou mais domínios"@pt-br ,
                              "Belongs to one or more domains"@en ;
              rdfs:subPropertyOf edo:DomainEngineeringAnnotation .


###  https://w3id.org/energy-domain/edo#hasLocationType
edo:hasLocationType rdf:type owl:AnnotationProperty ;
                    rdfs:label "Has Location Type"@en ,
                               "Pertence a um tipo de locação"@pt-br ;
                    skos:definition "Associa a entidade a um tipo de locação"@pt-br ,
                                    "Belongs to one or more Location Types"@en ;
                    rdfs:subPropertyOf edo:DomainEngineeringAnnotation .


###  https://w3id.org/energy-domain/edo#hasSubDomain
edo:hasSubDomain rdf:type owl:AnnotationProperty ;
                 rdfs:label "Has SubDomain"@en ,
                            "Pertence a um subdomínio"@pt-br ;
                 skos:definition "Associa a entidade a um ou mais subdomínios"@pt-br ,
                                 "Belongs to one or more subdomains"@en ;
                 rdfs:subPropertyOf edo:DomainEngineeringAnnotation .


###  https://w3id.org/energy-domain/edo#hasTypedValue
edo:hasTypedValue rdf:type owl:AnnotationProperty ;
                  rdfs:label "Has Typed Value"@en ,
                             "Possui tipo de valor"@pt-br ;
                  skos:definition "Indica que a entidade tem um valor como número real, inteiro, texto, booleano e etc."@pt-br ,
                                  "Indicates that the entity has a typed value, lik float, string, boolean, integer, etc."@en ;
                  rdfs:subPropertyOf edo:DomainAuxiliarAnnotation .


###  https://w3id.org/energy-domain/edo#hasValueCardinality
edo:hasValueCardinality rdf:type owl:AnnotationProperty ;
                        rdfs:label "Has Value Cardinality"@en ,
                                   "Possui cardinalidade de valor"@pt-br ;
                        skos:definition "Indica a quantidade de valores que a entidade possui"@pt-br ,
                                        "Indicates the quantity of values the entity support"@en ;
                        rdfs:subPropertyOf edo:DomainAuxiliarAnnotation .


###  https://w3id.org/energy-domain/edo#ifc_equivalentClass
edo:ifc_equivalentClass rdf:type owl:AnnotationProperty ;
                        rdfs:label "Classe IFC equivalente"@pt-br ,
                                   "IFC equivalent Class"@en ;
                        skos:definition "Classe IFC equivalente"@pt-br ,
                                        "IFC equivalent class"@en ;
                        rdfs:subPropertyOf edo:DomainEngineeringAnnotation .


###  https://w3id.org/energy-domain/edo#ifc_objectType
edo:ifc_objectType rdf:type owl:AnnotationProperty ;
                   rdfs:label "IFC ObjectType"@en ,
                              "ObjectType IFC"@pt-br ;
                   skos:definition "Object Type for IFC class customization"@en ,
                                   "Object Type para a customização de classes IFC"@pt-br ;
                   rdfs:subPropertyOf edo:DomainEngineeringAnnotation .


###  https://w3id.org/energy-domain/edo#ifc_predefinedType
edo:ifc_predefinedType rdf:type owl:AnnotationProperty ;
                       rdfs:label "IFC PredefinedType"@en ,
                                  "PredefinedType IFC"@pt-br ;
                       skos:definition "Predefined Type for IFC class customization"@en ,
                                       "Predefined Type para a customização de classes IFC"@pt-br ;
                       rdfs:subPropertyOf edo:DomainEngineeringAnnotation .


###  https://w3id.org/energy-domain/edo#validValues
edo:validValues rdf:type owl:AnnotationProperty ;
                rdfs:label "Valid Values"@en ,
                           "Valores Válidos"@pt-br ;
                skos:definition "List of Valid Values for the Attribute"@en ,
                                "Lista de valores válidos para o atributo"@pt-br ;
                rdfs:subPropertyOf edo:DomainAuxiliarAnnotation .


#################################################################
#    Datatypes
#################################################################

###  http://www.w3.org/2001/XMLSchema#date
xsd:date rdf:type rdfs:Datatype .


###  http://www.w3.org/2001/XMLSchema#time
xsd:time rdf:type rdfs:Datatype .


#################################################################
#    Object Properties
#################################################################

###  https://w3id.org/energy-domain/edo#DomainAuxiliarProperty
edo:DomainAuxiliarProperty rdf:type owl:ObjectProperty .


#################################################################
#    Data properties
#################################################################

###  http://www.w3.org/1999/02/22-rdf-syntax-ns#value
rdf:value rdf:type owl:DatatypeProperty .


#################################################################
#    Classes
#################################################################

###  https://w3id.org/energy-domain/edo#AbsoluteInsidePressure
edo:AbsoluteInsidePressure rdf:type owl:Class ;
                           rdfs:subClassOf edo:DomainAttribute ;
                           dcterms:accessRights "PUBLIC" ;
                           dcterms:identifier "AbsoluteInsidePressure" ;
                           skos:definition "Represents the absolute internal pressure exerted within a component or system. This property is crucial for evaluating the structural integrity and performance, ensuring that the system can withstand the specified pressure without failure, particularly in subsea environments where pressure management is critical."@en ;
                           skos:prefLabel "Absolute Inside Pressure"@en ,
                                          "Pressão Absoluta Interna"@pt-br ;
                           edo:hasTypedValue edo:floatValue ;
                           edo:hasValueCardinality edo:singleValue .


###  https://w3id.org/energy-domain/edo#AbsoluteOutsidePressure
edo:AbsoluteOutsidePressure rdf:type owl:Class ;
                            rdfs:subClassOf edo:DomainAttribute ;
                            dcterms:accessRights "PUBLIC" ;
                            dcterms:identifier "AbsoluteOutsidePressure" ;
                            skos:definition "Represents the absolute external pressure exerted on a component or system. This property is essential for evaluating how the system withstands pressure from its surrounding environment, particularly in subsea applications where external pressure can be significantly higher and impact the structural integrity of the system."@en ;
                            skos:prefLabel "Absolute Outside Pressure"@en ,
                                           "Pressão Absoluta Externa"@pt-br ;
                            edo:hasTypedValue edo:floatValue ;
                            edo:hasValueCardinality edo:singleValue .


###  https://w3id.org/energy-domain/edo#AnchoringCollar
edo:AnchoringCollar rdf:type owl:Class ;
                    rdfs:subClassOf edo:SplitCollar ;
                    dcterms:identifier "AnchoringCollar" ;
                    skos:altLabel "Anchor Clamp"@en ,
                                  "Anchoring Device"@en ,
                                  "Fixation Collar"@en ,
                                  "Securing Collar"@en ;
                    skos:definition "A mechanical device used to stabilize and secure flexible pipes, risers, or umbilical systems to fixed structures in subsea applications. By clamping onto the outer layers of the pipe, it prevents unwanted movement during installation and operation, helping to maintain alignment and integrity under tension or compression."@en ,
                                    "Um dispositivo mecânico usado para estabilizar e fixar dutos flexíveis ou risers a estruturas fixas em aplicações submarinas, além de dar suporte aos sistemas umbilicais. Ao se prender às camadas externas do tubo, evita movimentos indesejados durante a instalação e operação, ajudando a manter o alinhamento e a integridade sob tensão ou compressão."@pt-br ;
                    skos:prefLabel "Anchoring Collar"@en ,
                                   "Colar de Ancoragem"@pt-br ;
                    edo:hasAttribute edo:AnodeCollarsAxialSpacing ,
                                     edo:AnodeCollarsQuantity ,
                                     edo:ClampInternalDiameter ,
                                     edo:ExternalDiameter ,
                                     edo:GalvanicMaterial ,
                                     edo:IndividualAnodeMass ,
                                     edo:MetallicStrandLength ,
                                     edo:MetallicStrandSpareQuantity ,
                                     edo:SafeWorkingLoad ;
                    edo:ifc_equivalentClass "IfcPipeFitting" ;
                    edo:ifc_objectType "AnchoringCollar" ;
                    edo:ifc_predefinedType "USERDEFINED" .


###  https://w3id.org/energy-domain/edo#AnodeCollarSet
edo:AnodeCollarSet rdf:type owl:Class ;
                   rdfs:subClassOf edo:SplitCollar ;
                   dcterms:identifier "AnodeCollarSet" ;
                   skos:altLabel "Anode Bracket"@en ,
                                 "Anode Clamp"@en ,
                                 "Cathodic Protection Collar"@en ;
                   skos:definition "Colar de anodo sacrifical usado para proteção contra corrosão em ambientes submarinos. É projetado para ser acoplado ao redor de tubos ou risers e sofrer corrosão controlada, protegendo assim as estruturas metálicas contra ferrugem e degradação. Geralmente fabricado de zinco ou alumínio, garante a longevidade dos equipamentos submarinos ao se sacrificar para evitar a corrosão em infraestruturas críticas."@pt-br ,
                                   "Sacrificial anode collar set used for corrosion protection in subsea environments. It is designed to attach around pipes or risers and undergo controlled corrosion, thus protecting the metallic structures from rust and degradation. Typically made from zinc or aluminum, it ensures the longevity of subsea equipment by sacrificing itself to prevent corrosion on critical infrastructure."@en ;
                   skos:prefLabel "Anode Collar Set"@en ,
                                  "Conjunto de Colares de Anodo"@pt-br ;
                   edo:ifc_equivalentClass "IfcPipeFitting" ;
                   edo:ifc_objectType "AnodeCollarSet" ;
                   edo:ifc_predefinedType "USERDEFINED" .


###  https://w3id.org/energy-domain/edo#AnodeCollarsAxialSpacing
edo:AnodeCollarsAxialSpacing rdf:type owl:Class ;
                             rdfs:subClassOf edo:DomainAttribute ;
                             dcterms:accessRights "PUBLIC" ;
                             dcterms:identifier "AnodeCollarsAxialSpacing" ;
                             skos:definition "Axial distance between each individual collar."@en ;
                             skos:prefLabel "Anode Collars Axial Spacing"@en ,
                                            "Espaçamento Axial entre os Colares de Anodo"@pt-br ;
                             edo:hasTypedValue edo:floatValue ;
                             edo:hasValueCardinality edo:singleValue .


###  https://w3id.org/energy-domain/edo#AnodeCollarsQuantity
edo:AnodeCollarsQuantity rdf:type owl:Class ;
                         rdfs:subClassOf edo:DomainAttribute ;
                         dcterms:accessRights "PUBLIC" ;
                         dcterms:identifier "AnodeCollarsQuantity" ;
                         skos:definition "The total number of anode collars to provide cathodic protection against corrosion."@en ;
                         skos:prefLabel "Anode Collars Quantity"@en ,
                                        "Quantidade de Colares de Anodo"@pt-br ;
                         edo:hasTypedValue edo:intValue ;
                         edo:hasValueCardinality edo:singleValue .


###  https://w3id.org/energy-domain/edo#AntiCollapseSheath
edo:AntiCollapseSheath rdf:type owl:Class ;
                       rdfs:subClassOf edo:SolidLayer ;
                       dcterms:identifier "AntiCollapseSheath" ;
                       skos:definition "Camada de reforço em dutos flexíveis submarinos usados na exploração de petróleo e gás, projetada para evitar o colapso do duto sob altas pressões externas, como as encontradas em ambientes de águas profundas. Sua função principal é fornecer suporte estrutural contra forças externas que poderiam comprimir ou deformar o duto, especialmente durante situações em que a pressão interna é reduzida ou ausente, como quando o duto está vazio. Normalmente feita de materiais metálicos ou poliméricos de alta resistência, a Capa Anti-Colapso garante a integridade do duto flexível em condições extremas."@pt-br ,
                                       "Reinforcement layer in subsea flexible pipes used in oil and gas exploration, designed to prevent the collapse of the pipe under high external pressure conditions, such as those encountered in deepwater environments. Its primary role is to provide structural support against external forces that could compress or deform the pipe, particularly during situations where the internal pressure is reduced or absent, like when the pipe is emptied. Typically made from high-strength metallic or polymeric materials, the Anti Collapse Sheath ensures the integrity of the flexible pipe under extreme conditions."@en ;
                       skos:prefLabel "Anti Collapse Sheath"@en ,
                                      "Capa Anti-Colapso"@pt-br ;
                       edo:ifc_equivalentClass "IfcPipeSegment" ;
                       edo:ifc_objectType "AntiCollapseSheath" ;
                       edo:ifc_predefinedType "USERDEFINED" .


###  https://w3id.org/energy-domain/edo#AntiWearSheath
edo:AntiWearSheath rdf:type owl:Class ;
                   rdfs:subClassOf edo:SolidLayer ;
                   dcterms:identifier "AntiWearSheath" ;
                   skos:definition "Camada de reforço em dutos flexíveis usados na exploração de petróleo e gás, projetada para proteger o duto do desgaste externo e da abrasão causados pelo contato com o fundo marinho, equipamentos ou outros elementos submarinos. Seu papel principal é fornecer uma barreira protetora durável que protege as camadas subjacentes contra danos mecânicos, aumentando a vida útil do tubo flexível. Geralmente feita de materiais poliméricos resistentes ao desgaste, a Capa Anti-Atrito garante a integridade do duto ao reduzir o risco de danos na superfície em condições operacionais adversas."@pt-br ,
                                   "Reinforcement layer in subsea flexible pipes used in oil and gas exploration, designed to protect the pipe from external wear and abrasion caused by contact with the seabed, equipment, or other subsea elements. Its primary role is to provide a durable protective barrier that shields the underlying layers from mechanical damage, extending the lifespan of the flexible pipe. Typically made from wear-resistant polymeric materials, the Anti Wear Sheath ensures the pipe's integrity by reducing the risk of surface damage under harsh operating conditions."@en ;
                   skos:prefLabel "Anti Wear Sheath"@en ,
                                  "Capa Anti-Atrito"@pt-br ;
                   edo:hasAttribute edo:TapesQuantity ;
                   edo:ifc_equivalentClass "IfcPipeSegment" ;
                   edo:ifc_objectType "AntiWearSheath" ;
                   edo:ifc_predefinedType "USERDEFINED" .


###  https://w3id.org/energy-domain/edo#ArchitecturalEngineering
edo:ArchitecturalEngineering rdf:type owl:Class ;
                             rdfs:subClassOf edo:TechnicalDiscipline ;
                             rdfs:label "Architectural Engineering"@en ,
                                        "Engenharia Arquitetônica"@pt-br ;
                             skos:definition "Disciplina de engenharia focada no projeto de edifícios, construção e integração de sistemas."@pt-br ,
                                             "Engineering discipline focused on building design, construction and systems integration."@en .


###  https://w3id.org/energy-domain/edo#ArmourLayer
edo:ArmourLayer rdf:type owl:Class ;
                rdfs:subClassOf edo:WoundLayer ;
                dcterms:identifier "ArmourLayer" ;
                skos:definition "A reinforcement layer in subsea flexible pipes used in oil and gas exploration, designed to provide mechanical strength and protection against external forces, such as pressure and movement. It ensures structural integrity by preventing deformation and failure during operation. Typically made from high-strength metal wires, like carbon steel or stainless steel, the Armor Layer enhances the pipe's durability in harsh underwater conditions."@en ;
                skos:prefLabel "Armour Layer"@en ,
                               "Camada de Armadura"@pt-br .


###  https://w3id.org/energy-domain/edo#AssemblyShouldObeyModelPolarity
edo:AssemblyShouldObeyModelPolarity rdf:type owl:Class ;
                                    rdfs:subClassOf edo:DomainAttribute ;
                                    dcterms:accessRights "PUBLIC" ;
                                    dcterms:identifier "AssemblyShouldObeyModelPolarity" ;
                                    skos:definition "If true, the pipe section must be assembled according to the polarity in the model. If false, it can be mounted in any polarity."@en ;
                                    skos:prefLabel "A Montagem Deve Obedecer à Polaridade do Modelo"@pt-br ,
                                                   "Assembly Should Obey Model Polarity"@en ;
                                    edo:hasTypedValue edo:booleanValue ;
                                    edo:hasValueCardinality edo:singleValue .


###  https://w3id.org/energy-domain/edo#AssemblyTorque
edo:AssemblyTorque rdf:type owl:Class ;
                   rdfs:subClassOf edo:DomainAttribute ;
                   dcterms:accessRights "PUBLIC" ;
                   dcterms:identifier "AssemblyTorque" ;
                   skos:definition "Specifies the torque applied during assembly, ensuring proper tightening for secure connections. This value is critical for maintaining the structural integrity and reliability of the connection under operational loads."@en ;
                   skos:prefLabel "Assembly Torque"@en ,
                                  "Torque de montagem"@pt-br ;
                   edo:hasTypedValue edo:floatValue ;
                   edo:hasValueCardinality edo:singleValue .


###  https://w3id.org/energy-domain/edo#Asset
edo:Asset rdf:type owl:Class ;
          rdfs:subClassOf edo:DomainElement ;
          dcterms:identifier "Asset" ;
          skos:definition "An asset refers to valuable resources such as platforms, equipment, pipelines, and processing facilities crucial for production and transportation. These assets are managed to optimize performance, ensure safety, and maximize operational efficiency throughout their lifecycle."@en ;
          skos:prefLabel "Asset"@en ,
                         "Ativo"@pt-br ;
          edo:hasAttribute edo:IsSpare ,
                           edo:SerialNumber .


###  https://w3id.org/energy-domain/edo#AutomationControlEngineering
edo:AutomationControlEngineering rdf:type owl:Class ;
                                 rdfs:subClassOf edo:TechnicalDiscipline ;
                                 rdfs:label "Automation & Control Engineering"@en ,
                                            "Engenharia de Automação e Controle"@pt-br ;
                                 skos:definition "Disciplina de engenharia focada em sistemas de controle automatizado e automação de processos."@pt-br ,
                                                 "Engineering discipline focused on automated control systems and process automation."@en .


###  https://w3id.org/energy-domain/edo#AxialStiffnessUnderCompressionAtSeaLevel
edo:AxialStiffnessUnderCompressionAtSeaLevel rdf:type owl:Class ;
                                             rdfs:subClassOf edo:DomainAttribute ;
                                             dcterms:accessRights "PUBLIC" ;
                                             dcterms:identifier "AxialStiffnessUnderCompressionAtSeaLevel" ;
                                             skos:definition "Represents the resistance of a component or system to axial deformation under compression when measured at sea level. This property is essential for understanding how the structure behaves under compressive loads, ensuring that it can maintain stability and structural integrity."@en ,
                                                             "Rigidez axial (EA) duto comprimido, 20°C e pressão atmosferica (dentro e fora)"@pt-br ;
                                             skos:prefLabel "Axial Stiffness Under Compression At Sea Level"@en ,
                                                            "Rigidez Axial sob Compressão ao Nível do Mar"@pt-br ;
                                             edo:hasTypedValue edo:floatValue ;
                                             edo:hasValueCardinality edo:singleValue .


###  https://w3id.org/energy-domain/edo#AxialStiffnessUnderTensionAtSeaLevel
edo:AxialStiffnessUnderTensionAtSeaLevel rdf:type owl:Class ;
                                         rdfs:subClassOf edo:DomainAttribute ;
                                         dcterms:accessRights "PUBLIC" ;
                                         dcterms:identifier "AxialStiffnessUnderTensionAtSeaLevel" ;
                                         skos:definition "Represents the resistance of a component or system to axial deformation under tension when measured at sea level. This property is crucial for evaluating how the structure performs under tensile loads, ensuring it can withstand stretching forces while maintaining its integrity."@en ,
                                                         "Rigidez axial (EA) duto tracionado, 20°C e pressão atmosferica (dentro e fora)"@pt-br ;
                                         skos:prefLabel "Axial Stiffness Under Tension At Sea Level"@en ,
                                                        "Rigidez Axial sob Tração ao Nível do Mar"@pt-br ;
                                         edo:hasTypedValue edo:floatValue ;
                                         edo:hasValueCardinality edo:singleValue .


###  https://w3id.org/energy-domain/edo#BasicDesign
edo:BasicDesign rdf:type owl:Class ;
                rdfs:subClassOf edo:LifecyclePhase ;
                rdfs:label "Basic Design"@en ,
                           "Projeto Básico"@pt-br ;
                skos:definition "Fase onde são desenvolvidas especificações gerais de engenharia, layouts e listas de equipamentos principais."@pt-br ,
                                "Phase where general engineering specifications, layouts, and main equipment lists are developed."@en .


###  https://w3id.org/energy-domain/edo#BasicProjectRevision
edo:BasicProjectRevision rdf:type owl:Class ;
                         rdfs:subClassOf edo:DomainAttribute ;
                         dcterms:accessRights "PUBLIC" ;
                         dcterms:identifier "BasicProjectRevision" ;
                         skos:definition "Numeric value incremented with each new submission of the project (e.g., 0000, 0001, 0002, etc.), recorded as text. This value tracks revisions and ensures clarity in version control throughout the project lifecycle, allowing stakeholders to reference the most current or previous versions as needed."@en ,
                                         "Valor numérico incrementado a cada novo envio (0000, 0001, 0002 e etc.) como texto"@pt-br ;
                         skos:prefLabel "Basic Project Revision"@en ,
                                        "Revisão do Projeto Básico"@pt-br ;
                         edo:hasTypedValue edo:stringValue ;
                         edo:hasValueCardinality edo:singleValue .


###  https://w3id.org/energy-domain/edo#BendMomentVsShearForceTable
edo:BendMomentVsShearForceTable rdf:type owl:Class ;
                                rdfs:subClassOf edo:DomainAttribute ;
                                dcterms:accessRights "PUBLIC" ;
                                dcterms:identifier "BendMomentVsShearForceTable" ;
                                skos:definition "Provides data on the relationship between bending moment and shear force, used to evaluate how the structure behaves under combined loading conditions. This information is critical for determining the structural integrity and performance under different operational stresses."@en ;
                                skos:prefLabel "Bending moment vs Shear Force Table"@en ,
                                               "Tabela de Momento de Curvatura em Função da Força Cisalhante"@pt-br .


###  https://w3id.org/energy-domain/edo#BendMomentVsShearForceTable_BendingMoment
edo:BendMomentVsShearForceTable_BendingMoment rdf:type owl:Class ;
                                              rdfs:subClassOf edo:DomainAttribute ;
                                              dcterms:accessRights "PUBLIC" ;
                                              dcterms:identifier "BendMomentVsShearForceTable_BendingMoment" ;
                                              skos:definition "Represents the moment generated by a force causing the component or system to bend around an axis. This property is critical for assessing the structure's ability to resist bending under operational loads, ensuring it maintains its shape and structural integrity."@en ;
                                              skos:prefLabel "Bending Moment"@en ,
                                                             "Momento de flexão"@pt-br ;
                                              edo:hasTypedValue edo:floatValue ;
                                              edo:hasValueCardinality edo:multiValue .


###  https://w3id.org/energy-domain/edo#BendMomentVsShearForceTable_Condition
edo:BendMomentVsShearForceTable_Condition rdf:type owl:Class ;
                                          rdfs:subClassOf edo:DomainAttribute ;
                                          dcterms:accessRights "PUBLIC" ;
                                          dcterms:identifier "BendMomentVsShearForceTable_Condition" ;
                                          skos:definition "Curve data flexible pipe condition."@en ;
                                          skos:prefLabel "Condition"@en ,
                                                         "Condição do flexível para os dados da curva"@pt-br ;
                                          edo:hasTypedValue edo:stringValue ;
                                          edo:hasValueCardinality edo:multiValue .


###  https://w3id.org/energy-domain/edo#BendMomentVsShearForceTable_ShearForce
edo:BendMomentVsShearForceTable_ShearForce rdf:type owl:Class ;
                                           rdfs:subClassOf edo:DomainAttribute ;
                                           dcterms:accessRights "PUBLIC" ;
                                           dcterms:identifier "BendMomentVsShearForceTable_ShearForce" ;
                                           skos:definition "Força de cisalhamento (Obrigatório incluir o valor para força = 0)"@pt-br ,
                                                           "Represents the force applied parallel to the surface of a material or component, causing it to experience shear stress. This property is essential for evaluating the material's ability to resist sliding or deformation when subjected to external forces."@en ;
                                           skos:prefLabel "Força de Cisalhamento"@pt-br ,
                                                          "Shear Force"@en ;
                                           edo:hasTypedValue edo:floatValue ;
                                           edo:hasValueCardinality edo:multiValue .


###  https://w3id.org/energy-domain/edo#BendRestrictor
edo:BendRestrictor rdf:type owl:Class ;
                   rdfs:subClassOf edo:LineAncillary ;
                   dcterms:identifier "BendRestrictor" ;
                   skos:altLabel "Bend Limiter"@en ,
                                 "Bending Restrictor"@en ,
                                 "Curvature Limiter"@en ;
                   skos:definition "Device used in subsea flexible pipes to limit the bending radius and prevent over-bending that could damage the pipe. Typically installed near critical areas such as connectors or end fittings, where excessive bending could compromise the structural integrity of the pipe. The Bend Restrictor consists of multiple interlocking segments that allow flexibility up to a certain radius, beyond which the segments lock to prevent further bending, protecting the pipe from deformation or failure in harsh subsea environments."@en ,
                                   "Dispositivo usado em dutos flexíveis para limitar o raio de curvatura e evitar curvaturas excessivas que poderiam danificar o duto. Normalmente instalado perto de áreas críticas, como conectores ou acessórios finais, onde curvaturas excessivas poderiam comprometer a integridade estrutural do duto. O Restritor de Curvatura consiste em múltiplos segmentos interligados que permitem flexibilidade até um certo raio, além do qual os segmentos se bloqueiam para impedir mais curvaturas, protegendo o duto contra deformações ou falhas em ambientes submarinos adversos."@pt-br ;
                   skos:prefLabel "Bend Restrictor"@en ,
                                  "Restritor de Curvatura"@pt-br ;
                   edo:hasAttribute edo:BendMomentVsShearForceTable ,
                                    edo:BendMomentVsShearForceTable_BendingMoment ,
                                    edo:BendMomentVsShearForceTable_Condition ,
                                    edo:BendMomentVsShearForceTable_ShearForce ;
                   edo:ifc_equivalentClass "IfcPipeFitting" ;
                   edo:ifc_objectType "BendRestrictor" .


###  https://w3id.org/energy-domain/edo#BendStiffener
edo:BendStiffener rdf:type owl:Class ;
                  rdfs:subClassOf edo:LineAncillary ;
                  dcterms:identifier "BendStiffener" ;
                  skos:definition "Device used in subsea flexible pipes to provide gradual stiffness transition between the flexible pipe and a fixed structure, preventing excessive bending at critical areas such as terminations or connectors. The Bend Stiffener is designed to manage stress concentration by stiffening the pipe over a defined length, reducing the risk of damage due to repeated bending, fatigue, or over-flexing. Typically made from high-strength materials, it ensures the long-term structural integrity of the pipe in dynamic subsea environments."@en ;
                  skos:prefLabel "Bend Stiffener"@en ,
                                 "Enrijecedor de Curvatura"@pt-br .


###  https://w3id.org/energy-domain/edo#BendingMomentTable
edo:BendingMomentTable rdf:type owl:Class ;
                       rdfs:subClassOf edo:DomainAttribute ;
                       dcterms:accessRights "PUBLIC" ;
                       dcterms:identifier "BendingMomentTable" ;
                       skos:definition "Provides data on bending moments under different loading conditions, used to evaluate how the structure responds to bending forces. This information is essential for determining the structure's strength, flexibility, and ability to withstand operational stresses."@en ;
                       skos:prefLabel "Bending Moment Table"@en ,
                                      "Tabela de Curvatura x Momento Flexor"@pt-br .


###  https://w3id.org/energy-domain/edo#BendingMomentTable_BendingMoment
edo:BendingMomentTable_BendingMoment rdf:type owl:Class ;
                                     rdfs:subClassOf edo:DomainAttribute ;
                                     dcterms:accessRights "PUBLIC" ;
                                     dcterms:identifier "BendingMomentTable_BendingMoment" ;
                                     skos:definition "Represents the moment generated by a force causing the component or system to bend around an axis. This property is critical for assessing the structure's ability to resist bending under operational loads, ensuring it maintains its shape and structural integrity."@en ;
                                     skos:prefLabel "Bending Moment"@en ,
                                                    "Momento de Flexão"@pt-br ;
                                     edo:hasTypedValue edo:floatValue ;
                                     edo:hasValueCardinality edo:multiValue .


###  https://w3id.org/energy-domain/edo#BendingMomentTable_Curvature
edo:BendingMomentTable_Curvature rdf:type owl:Class ;
                                 rdfs:subClassOf edo:DomainAttribute ;
                                 dcterms:accessRights "PUBLIC" ;
                                 dcterms:identifier "BendingMomentTable_Curvature" ;
                                 skos:definition "Represents the degree to which a component or structure bends or curves along its length. This property is important for understanding the flexibility and bending behavior, ensuring that the structure can perform as required under operational conditions without exceeding its design limits."@en ;
                                 skos:prefLabel "Curvatura"@pt-br ,
                                                "Curvature"@en ;
                                 edo:hasTypedValue edo:floatValue ;
                                 edo:hasValueCardinality edo:multiValue .


###  https://w3id.org/energy-domain/edo#Biomass
edo:Biomass rdf:type owl:Class ;
            rdfs:subClassOf edo:Renewable ;
            rdfs:label "Biomass Energy"@en ,
                       "Energia de Biomassa"@pt-br ;
            skos:definition "Energia produzida a partir de materiais orgânicos como madeira, resíduos agrícolas ou lixo."@pt-br ,
                            "Energy produced from organic materials such as wood, agricultural residues, or waste."@en .


###  https://w3id.org/energy-domain/edo#BoltSet
edo:BoltSet rdf:type owl:Class ;
            rdfs:subClassOf edo:PhysicalConnection ;
            dcterms:identifier "BoltSet" ;
            skos:definition "A collection of bolts and nuts, and washers designed for fastening components in subsea systems. Bolt sets are critical for ensuring structural integrity and are selected based on size, material, and application requirements."@en ;
            skos:prefLabel "Bolt Set"@en ,
                           "Conjunto de Parafusos"@pt-br ;
            edo:hasAttribute edo:AssemblyTorque ,
                             edo:FullyThreaded ,
                             edo:Lubricant ,
                             edo:LubricantFrictionFactor ,
                             edo:NominalLength ,
                             edo:Quantity ,
                             edo:SpareQuantity .


###  https://w3id.org/energy-domain/edo#BoreDiameter
edo:BoreDiameter rdf:type owl:Class ;
                 rdfs:subClassOf edo:DomainAttribute ;
                 dcterms:accessRights "PUBLIC" ;
                 dcterms:identifier "BoreDiameter" ;
                 skos:definition "Internal diameter that defines the size of the passage through which fluids or gases can flow. This dimension is essential in industrial piping, as it determines flow capacity and impacts pressure and velocity within the system."@en ;
                 skos:prefLabel "Bore Diameter"@en ,
                                "Diâmetro do Furo"@pt-br ;
                 edo:hasTypedValue edo:floatValue ;
                 edo:hasValueCardinality edo:singleValue .


###  https://w3id.org/energy-domain/edo#BuoyancyModule
edo:BuoyancyModule rdf:type owl:Class ;
                   rdfs:subClassOf edo:LineAncillary ;
                   dcterms:identifier "BuoyancyModule" ;
                   skos:altLabel "Buoyancy Element"@en ,
                                 "Buoyancy Unit"@en ,
                                 "Floatation Module"@en ,
                                 "Subsea Buoyancy Module"@en ;
                   skos:definition "Device used in subsea systems to provide controlled buoyancy to flexible pipes, risers, or umbilicals, reducing the load on the structure and managing the configuration of the line in the water column. The Buoyancy Module is typically composed of syntactic foam or other materials with low density, designed to withstand high external pressures while maintaining its buoyant properties over time. It plays a key role in optimizing the performance and positioning of subsea lines, ensuring they maintain the required shape and depth in dynamic ocean conditions."@en ,
                                   "Dispositivo utilizado em sistemas submarinos para fornecer flutuabilidade controlada a dutos flexíveis, risers ou umbilicais, reduzindo a carga na estrutura e gerenciando a configuração da linha na coluna d'água. O Módulo de Flutuação é tipicamente composto por espuma sintática ou outros materiais de baixa densidade, projetados para suportar altas pressões externas enquanto mantêm suas propriedades de flutuabilidade ao longo do tempo. Ele desempenha um papel fundamental na otimização do desempenho e do posicionamento das linhas subsea, garantindo que mantenham a forma e a profundidade necessárias em condições oceânicas dinâmicas."@pt-br ;
                   skos:prefLabel "Buoyancy Module"@en ,
                                  "Módulo de Flutuação"@pt-br ;
                   edo:hasAttribute edo:LongTermFloatDensity ,
                                    edo:LongTermFloatVolume ,
                                    edo:NominalFloatDensity ,
                                    edo:NominalFloatVolume ,
                                    edo:PipeMountPosition ,
                                    edo:ShortTermFloatDensity ,
                                    edo:ShortTermFloatVolume ;
                   edo:ifc_equivalentClass "IfcPipeFitting" ;
                   edo:ifc_objectType "BuoyancyModule" ;
                   edo:ifc_predefinedType "USERDEFINED" .


###  https://w3id.org/energy-domain/edo#CO2VolumePercentage
edo:CO2VolumePercentage rdf:type owl:Class ;
                        rdfs:subClassOf edo:DomainAttribute ;
                        dcterms:accessRights "PUBLIC" ;
                        dcterms:identifier "CO2VolumePercentage" ;
                        skos:definition "Represents the percentage of carbon dioxide (CO2) in the total volume of the fluid or gas mixture within the pipeline. This value is essential for determining the material selection and design considerations for the flexible subsea pipeline, as CO2 can influence corrosion rates and impact the overall integrity and lifespan of the pipeline."@en ;
                        skos:prefLabel "Carbon Dioxide (CO2) Volume Percentage"@en ,
                                       "Porcentagem de Volume de Dióxido de Carbono (CO2)"@pt-br ;
                        edo:hasTypedValue edo:floatValue ;
                        edo:hasValueCardinality edo:singleValue .


###  https://w3id.org/energy-domain/edo#CalculatedAbsoluteBurstPressure
edo:CalculatedAbsoluteBurstPressure rdf:type owl:Class ;
                                    rdfs:subClassOf edo:DomainAttribute ;
                                    dcterms:accessRights "PUBLIC" ;
                                    dcterms:identifier "CalculatedAbsoluteBurstPressure" ;
                                    skos:definition "Represents the estimated absolute pressure at which a component or system is expected to fail or rupture. This property is crucial for determining the maximum safe operating pressure, ensuring that the component can withstand internal forces without bursting."@en ;
                                    skos:prefLabel "Calculated Absolute Burst Pressure"@en ,
                                                   "Pressão Absoluta de Ruptura Calculada"@pt-br ;
                                    edo:hasTypedValue edo:floatValue ;
                                    edo:hasValueCardinality edo:singleValue .


###  https://w3id.org/energy-domain/edo#CarcassLayer
edo:CarcassLayer rdf:type owl:Class ;
                 rdfs:subClassOf edo:ArmourLayer ;
                 dcterms:identifier "CarcassLayer" ;
                 skos:definition "A reinforcement layer in subsea flexible pipes that provides structural strength and stability. It helps maintain the shape and integrity of the pipe under operational pressure, ensuring the flexibility of the pipe while protecting the internal components. Typically made from metal or polymer materials, it acts as a foundation for the other protective layers."@en ;
                 skos:prefLabel "Camada de Carcaça"@pt-br ,
                                "Carcass Layer"@en ;
                 edo:hasAttribute edo:MetallicLayerPitch ,
                                  edo:StressAtDesignPressure .


###  https://w3id.org/energy-domain/edo#ChainSegment
edo:ChainSegment rdf:type owl:Class ;
                 rdfs:subClassOf edo:LinearObject ;
                 dcterms:identifier "ChainSegment" .


###  https://w3id.org/energy-domain/edo#CivilEngineering
edo:CivilEngineering rdf:type owl:Class ;
                     rdfs:subClassOf edo:TechnicalDiscipline ;
                     rdfs:label "Civil Engineering"@en ,
                                "Engenharia Civil"@pt-br ;
                     skos:definition "Disciplina de engenharia focada no projeto e construção de infraestrutura."@pt-br ,
                                     "Engineering discipline focused on the design and construction of infrastructure."@en .


###  https://w3id.org/energy-domain/edo#ClampInternalDiameter
edo:ClampInternalDiameter rdf:type owl:Class ;
                          rdfs:subClassOf edo:DomainAttribute ;
                          dcterms:accessRights "PUBLIC" ;
                          dcterms:identifier "ClampInternalDiameter" ;
                          skos:definition "Is the clamp internal diameter"@en ;
                          skos:prefLabel "Clamp Internal Diameter"@en ,
                                         "Diâmetro interno do clamp"@pt-br ;
                          edo:hasTypedValue edo:floatValue ;
                          edo:hasValueCardinality edo:singleValue .


###  https://w3id.org/energy-domain/edo#CollarInternalDiameter
edo:CollarInternalDiameter rdf:type owl:Class ;
                           rdfs:subClassOf edo:DomainAttribute ;
                           dcterms:accessRights "PUBLIC" ;
                           dcterms:identifier "CollarInternalDiameter" ;
                           skos:definition "Inner dimension of the collar, to ensure proper fitting and secure attachment."@en ;
                           skos:prefLabel "Collar Internal Diameter"@en ,
                                          "Diâmetro Interno do Colar"@pt-br ;
                           edo:hasTypedValue edo:floatValue ;
                           edo:hasValueCardinality edo:singleValue .


###  https://w3id.org/energy-domain/edo#Commissioning
edo:Commissioning rdf:type owl:Class ;
                  rdfs:subClassOf edo:LifecyclePhase ;
                  rdfs:label "Comissionamento"@pt-br ,
                             "Commissioning"@en ;
                  skos:definition "Final testing and handover of the system into operational status."@en ,
                                  "Testes finais e entrega do sistema para status operacional."@pt-br .


###  https://w3id.org/energy-domain/edo#CompactObject
edo:CompactObject rdf:type owl:Class ;
                  rdfs:subClassOf edo:Asset ;
                  dcterms:identifier "CompactObject" ;
                  rdfs:label "Compact Object"@en ;
                  skos:definition "A mobile physical object, usually manufactured in a standardized manner."@en ;
                  skos:prefLabel "Compact Object"@en ,
                                 "Objeto Compacto"@pt-br .


###  https://w3id.org/energy-domain/edo#Component
edo:Component rdf:type owl:Class ;
              rdfs:subClassOf edo:CompactObject ;
              dcterms:identifier "Component" ;
              skos:definition "Items always found as part of larger objects, with varying levels of complexity."@en ;
              skos:prefLabel "Component"@en ,
                             "Componente"@pt-br .


###  https://w3id.org/energy-domain/edo#CompositeLayerMaterialType
edo:CompositeLayerMaterialType rdf:type owl:Class ;
                               rdfs:subClassOf edo:DomainAttribute ;
                               dcterms:accessRights "PUBLIC" ;
                               dcterms:identifier "CompositeLayerMaterialType" ;
                               skos:definition "Type of material from which an object is made, allowing for precise documentation and categorisation."@en ;
                               skos:prefLabel "Composite Layer Material Type"@en ,
                                              "Tipo de Material da Camada de Compósito"@pt-br ;
                               edo:hasTypedValue edo:stringValue ;
                               edo:hasValueCardinality edo:singleValue .


###  https://w3id.org/energy-domain/edo#CompositeMaterial
edo:CompositeMaterial rdf:type owl:Class ;
                      rdfs:subClassOf edo:FlexibleStructureLayerMaterial ;
                      dcterms:identifier "CompositeMaterial" ;
                      skos:definition "Material composto por dois ou mais componentes distintos, geralmente fibras de reforço e uma matriz, usado na construção de camadas em dutos flexíveis para aplicações subsea. O Material Compósito oferece uma combinação de alta resistência, resistência à corrosão e flexibilidade, tornando-o adequado para suportar as condições severas de ambientes de águas profundas. Seu uso nas camadas do duto flexível melhora a integridade estrutural do duto, resistência à pressão externa e durabilidade sob carregamento cíclico, ao mesmo tempo em que reduz o peso em comparação com materiais metálicos tradicionais."@pt-br ,
                                      "Material made from two or more distinct components, typically reinforcing fibers and a matrix, used in the construction of layers in flexible pipes for subsea applications. The Composite Material offers a combination of high strength, corrosion resistance, and flexibility, making it suitable for withstanding the harsh conditions of deepwater environments. Its use in flexible pipe layers enhances the pipe's structural integrity, resistance to external pressure, and durability under cyclical loading, while also reducing weight compared to traditional metallic materials."@en ;
                      skos:prefLabel "Composite Material"@en ,
                                     "Material Compósito"@pt-br ;
                      edo:hasAttribute edo:CompositeLayerMaterialType ,
                                       edo:RuptDefAlongFibers ,
                                       edo:RuptDefPerpendFibers ,
                                       edo:UltTensStrAlongFibers ,
                                       edo:UltTensStrPerpendFibers ;
                      edo:ifc_equivalentClass "IfcMaterial" ;
                      edo:ifc_objectType "CompositeMaterial" .


###  https://w3id.org/energy-domain/edo#ConceptualDesign
edo:ConceptualDesign rdf:type owl:Class ;
                     rdfs:subClassOf edo:LifecyclePhase ;
                     rdfs:label "Conceptual Design"@en ,
                                "Projeto Conceitual"@pt-br ;
                     skos:definition "Fase inicial de projeto focada em viabilidade, definição de escopo e seleção de tecnologia."@pt-br ,
                                     "Initial design phase focused on feasibility, scope definition, and technology selection."@en .


###  https://w3id.org/energy-domain/edo#Connection
edo:Connection rdf:type owl:Class ;
               rdfs:subClassOf edo:DomainElement ;
               dcterms:identifier "Connection" ;
               skos:definition "The joining point between two components, enabling fluid, gas, or structural continuity. Connections are designed to ensure secure, leak-free operation in harsh subsea environments."@en ;
               skos:prefLabel "Conexão"@pt-br ,
                              "Connection"@en .


###  https://w3id.org/energy-domain/edo#CriticalCurvatureOfSlipping
edo:CriticalCurvatureOfSlipping rdf:type owl:Class ;
                                rdfs:subClassOf edo:DomainAttribute ;
                                dcterms:accessRights "PUBLIC" ;
                                dcterms:identifier "CriticalCurvatureOfSlipping" ;
                                skos:definition "Represents the minimum curvature at which slipping or movement between layers or components begins to occur. This property is essential for assessing the flexibility and mechanical behavior of the structure, ensuring that it can maintain stability and performance under bending without experiencing slippage."@en ;
                                skos:prefLabel "Critical Curvature Of Slipping"@en ,
                                               "Curvatura crítica de escorregamento"@pt-br ;
                                edo:hasTypedValue edo:floatValue ;
                                edo:hasValueCardinality edo:singleValue .


###  https://w3id.org/energy-domain/edo#DamagingPullInStraightLine
edo:DamagingPullInStraightLine rdf:type owl:Class ;
                               rdfs:subClassOf edo:DomainAttribute ;
                               dcterms:accessRights "PUBLIC" ;
                               dcterms:identifier "DamagingPullInStraightLine" ;
                               skos:definition "Represents the force applied during a straight-line pull-in operation that could cause damage to a component or system. This property is critical for determining safe operational limits during installation, ensuring that the component can withstand the pulling force without suffering structural damage."@en ;
                               skos:prefLabel "Damaging Pull In Straight Line"@en ,
                                              "Tração Crítica em Linha Reta"@pt-br ;
                               edo:hasTypedValue edo:floatValue ;
                               edo:hasValueCardinality edo:singleValue .


###  https://w3id.org/energy-domain/edo#DeadweightCollar
edo:DeadweightCollar rdf:type owl:Class ;
                     rdfs:subClassOf edo:SplitCollar ;
                     dcterms:identifier "DeadweightCollar" ;
                     skos:altLabel "Ballast Collar"@en ,
                                   "Dead Weight Clamp"@en ,
                                   "Sinking Collar"@en ,
                                   "Weight Collar"@en ;
                     skos:definition "Component used in subsea systems to provide additional weight to flexible pipes, risers, or umbilicals, ensuring proper stability and positioning on the seabed. The Deadweight Collar is designed to counteract buoyant forces, preventing unwanted movement of the pipe due to ocean currents or other environmental factors. Typically made from dense materials, it plays a crucial role in maintaining the alignment and stability of lines in dynamic environments, ensuring that the system remains securely anchored."@en ,
                                     "Componente utilizado em sistemas submersos para fornecer peso adicional a dutos flexíveis, risers ou umbilicais, garantindo a estabilidade e o posicionamento adequados no fundo marinho. O Colar de Peso Morto é projetado para contrabalançar as forças de flutuabilidade, prevenindo o movimento indesejado do duto devido a correntes oceânicas ou outros fatores ambientais. Geralmente feito de materiais densos, ele desempenha um papel crucial na manutenção do alinhamento e da estabilidade das linhas submersas em ambientes dinâmicos, garantindo que o sistema permaneça firmemente ancorado."@pt-br ;
                     skos:prefLabel "Colar de Peso Morto"@pt-br ,
                                    "Deadweight Collar"@en ;
                     edo:ifc_equivalentClass "IfcPipeFitting" ;
                     edo:ifc_objectType "DeadweightCollar" ;
                     edo:ifc_predefinedType "USERDEFINED" .


###  https://w3id.org/energy-domain/edo#Decommissioning
edo:Decommissioning rdf:type owl:Class ;
                    rdfs:subClassOf edo:LifecyclePhase ;
                    rdfs:label "Decommissioning"@en ,
                               "Descomissionamento"@pt-br ;
                    skos:definition "Permanent removal of the asset from service, including dismantling and disposal."@en ,
                                    "Remoção permanente do ativo do serviço, incluindo desmontagem e descarte."@pt-br .


###  https://w3id.org/energy-domain/edo#DetailedDesign
edo:DetailedDesign rdf:type owl:Class ;
                   rdfs:subClassOf edo:LifecyclePhase ;
                   rdfs:label "Detailed Design"@en ,
                              "Projeto Detalhado"@pt-br ;
                   skos:definition "Comprehensive engineering phase producing detailed drawings, material specifications, and construction plans."@en ,
                                   "Fase abrangente de engenharia que produz desenhos detalhados, especificações de materiais e planos de construção."@pt-br .


###  https://w3id.org/energy-domain/edo#DiffusionTable
edo:DiffusionTable rdf:type owl:Class ;
                   rdfs:subClassOf edo:DomainAttribute ;
                   dcterms:accessRights "PUBLIC" ;
                   dcterms:identifier "DiffusionTable" ;
                   skos:definition "Difusão (Específica para Materiais Poliméricos)"@pt-br ,
                                   "Provides data on the diffusion rates of substances through materials, used to assess how different fluids or gases permeate the structure over time. This information is crucial for evaluating material suitability and predicting long-term performance under specific environmental conditions."@en ;
                   skos:prefLabel "Diffusion Table"@en ,
                                  "Tabela de Difusão"@pt-br .


###  https://w3id.org/energy-domain/edo#DiffusionTable_DiffusionCoefficient
edo:DiffusionTable_DiffusionCoefficient rdf:type owl:Class ;
                                        rdfs:subClassOf edo:DomainAttribute ;
                                        dcterms:accessRights "PUBLIC" ;
                                        dcterms:identifier "DiffusionTable_DiffusionCoefficient" ;
                                        skos:definition "Represents the rate at which particles, molecules, or substances diffuse through a material. This property is important for evaluating how gases or liquids move within or through a material, helping to understand the behavior of the component, where diffusion can affect performance and integrity."@en ;
                                        skos:prefLabel "Coeficiente de difusão"@pt-br ,
                                                       "Diffusion Coefficient"@en ;
                                        edo:hasTypedValue edo:floatValue ;
                                        edo:hasValueCardinality edo:multiValue .


###  https://w3id.org/energy-domain/edo#DiffusionTable_MoleculeIdentifier
edo:DiffusionTable_MoleculeIdentifier rdf:type owl:Class ;
                                      rdfs:subClassOf edo:DomainAttribute ;
                                      dcterms:accessRights "PUBLIC" ;
                                      dcterms:identifier "DiffusionTable_MoleculeIdentifier" ;
                                      skos:definition "Specifies the type of molecule. This property identifies the particular molecule involved, which is crucial for understanding the material's interaction with or response to different chemical substances."@en ,
                                                      "Tipo de Molécula (co2, h2s, ch4, h2o,…)"@pt-br ;
                                      skos:prefLabel "Identificador de Molécula"@pt-br ,
                                                     "Molecule Identifier"@en ;
                                      edo:hasTypedValue edo:stringValue ;
                                      edo:hasValueCardinality edo:multiValue .


###  https://w3id.org/energy-domain/edo#DiffusionTable_PolymerState
edo:DiffusionTable_PolymerState rdf:type owl:Class ;
                                rdfs:subClassOf edo:DomainAttribute ;
                                dcterms:accessRights "PUBLIC" ;
                                dcterms:identifier "DiffusionTable_PolymerState" ;
                                skos:definition "The state of the polymeric material is specified.. This property is crucial for understanding how the material behaves under different conditions and its suitability for various applications."@en ,
                                                "estado do polímero (plastificado, não plastificado,…)"@pt-br ;
                                skos:prefLabel "Estado do Polímero"@pt-br ,
                                               "Polymer State"@en ;
                                edo:hasTypedValue edo:stringValue ;
                                edo:hasValueCardinality edo:multiValue .


###  https://w3id.org/energy-domain/edo#DiffusionTable_Temperature
edo:DiffusionTable_Temperature rdf:type owl:Class ;
                               rdfs:subClassOf edo:DomainAttribute ;
                               dcterms:accessRights "PUBLIC" ;
                               dcterms:identifier "DiffusionTable_Temperature" ;
                               skos:definition "Represents the thermal condition or measurement of heat for a component or system. This property is important for assessing how the component performs or operates under specific thermal conditions, ensuring it remains within safe and effective operating limits."@en ;
                               skos:prefLabel "Temperatura"@pt-br ,
                                              "Temperature"@en ;
                               edo:hasTypedValue edo:floatValue ;
                               edo:hasValueCardinality edo:multiValue .


###  https://w3id.org/energy-domain/edo#DimensioningCriteria
edo:DimensioningCriteria rdf:type owl:Class ;
                         rdfs:subClassOf edo:DomainAttribute ;
                         dcterms:accessRights "PUBLIC" ;
                         dcterms:identifier "DimensioningCriteria" ;
                         skos:definition "Critério de dimensionamento de raio mínimo de lançamento. Lista pré definida:Linear interpolation (curvature)Most restrictive value between the neighbouring values"@pt-br ,
                                         "Specifies the criteria used to determine the dimensions, providing guidelines and standards for accurate sizing and ensuring that the structure meets required performance and safety specifications."@en ;
                         skos:prefLabel "Critério de Dimensionamento"@pt-br ,
                                        "Dimensioning Criteria"@en ;
                         edo:hasTypedValue edo:stringValue ;
                         edo:hasValueCardinality edo:singleValue .


###  https://w3id.org/energy-domain/edo#DimensionsDrawing
edo:DimensionsDrawing rdf:type owl:Class ;
                      rdfs:subClassOf edo:ReferenceDrawing ;
                      dcterms:identifier "DimensionsDrawing" ;
                      skos:definition "Desenho técnico que fornece medições detalhadas, especificações geométricas e dados angulares dos componentes utilizados. O Desenho de Cotas inclui informações críticas como comprimento, diâmetro, espessura e ângulos, garantindo a fabricação, montagem e instalação precisas das peças. Esse desenho é essencial para atender aos requisitos de projeto e garantir que todos os componentes se encaixem corretamente no sistema como um todo, apoiando a fabricação eficiente e o controle de qualidade."@pt-br ,
                                      "Technical drawing providing detailed measurements, geometric specifications, and angular data of components. The Dimensions Drawing includes critical information such as length, diameter, thickness, and angles, ensuring the precise fabrication, assembly, and installation of the parts. This drawing is essential for meeting design requirements and ensuring that all components fit accurately within the overall system, supporting efficient manufacturing and quality control."@en ;
                      skos:prefLabel "Desenho de Cotas"@pt-br ,
                                     "Dimensions Drawing"@en ;
                      edo:ifc_equivalentClass "IfcDocumentInformation" ;
                      edo:ifc_objectType "DimensionsDrawing" .


###  https://w3id.org/energy-domain/edo#DisplacedVolume
edo:DisplacedVolume rdf:type owl:Class ;
                    rdfs:subClassOf edo:DomainAttribute ;
                    dcterms:accessRights "PUBLIC" ;
                    dcterms:identifier "DisplacedVolume" ;
                    skos:definition "Refers to the total volume of an object that is submerged or immersed in a fluid. This volume is used to calculate the buoyant force acting on the object and is crucial for understanding its buoyancy and stability in the fluid."@en ;
                    skos:prefLabel "Displaced Volume"@en ,
                                   "Volume Deslocado"@pt-br ;
                    edo:hasTypedValue edo:floatValue ;
                    edo:hasValueCardinality edo:singleValue .


###  https://w3id.org/energy-domain/edo#DistributionConnectionPoint
edo:DistributionConnectionPoint rdf:type owl:Class ;
                                rdfs:subClassOf edo:LogicalConnection ;
                                dcterms:identifier "DistributionConnectionPoint" ;
                                skos:definition "Localização em um modelo que indica o ponto específico onde os componentes de distribuição de fluido são conectados. O Ponto de Conexão de Distribuição fornece informações precisas para a montagem e instalação desses componentes, garantindo o alinhamento adequado e a funcionalidade dentro do sistema. Este ponto é crucial para definir a interface entre os elementos de distribuição de fluido em sistemas submarinos ou outros sistemas de manuseio de fluido."@pt-br ,
                                                "Location in a model that indicates the specific point where fluid distribution components are connected. The Distribution Connection Point provides precise information for the assembly and installation of these components, ensuring proper alignment and functionality within the system. This point is critical for defining the interface between fluid distribution elements in subsea or other fluid-handling systems."@en ;
                                skos:prefLabel "Distribution Connection Point"@en ,
                                               "Ponto de Conexão de Distribuição"@pt-br ;
                                edo:ifc_equivalentClass "IfcDistributionPort" ;
                                edo:ifc_objectType "DistributionConnectionPoint" ;
                                edo:ifc_predefinedType "USERDEFINED" .


###  https://w3id.org/energy-domain/edo#Domain
edo:Domain rdf:type owl:Class ;
           rdfs:subClassOf edo:DomainClassification ;
           rdfs:comment "Represents a high-level industrial domain, such as Oil & Gas, Nuclear, or Renewable Energy."@en ;
           rdfs:label "Domínio Industrial"@pt-br ,
                      "Industrial Domain"@en ;
           skos:definition "A high-level industrial sector or application area."@en ,
                           "Um setor industrial ou área de aplicação de alto nível."@pt-br .


###  https://w3id.org/energy-domain/edo#DomainAttribute
edo:DomainAttribute rdf:type owl:Class .


###  https://w3id.org/energy-domain/edo#DomainAuxiliarClass
edo:DomainAuxiliarClass rdf:type owl:Class .


###  https://w3id.org/energy-domain/edo#DomainClassification
edo:DomainClassification rdf:type owl:Class .


###  https://w3id.org/energy-domain/edo#DomainElement
edo:DomainElement rdf:type owl:Class .


###  https://w3id.org/energy-domain/edo#Downstream
edo:Downstream rdf:type owl:Class ;
               rdfs:subClassOf edo:OilAndGas ;
               rdfs:label "Downstream"@en ,
                          "Downstream"@pt-br ;
               skos:definition "Oil & Gas sector covering refining, processing, distribution, and retail of petroleum products."@en ,
                               "Setor de Petróleo & Gás que abrange refino, processamento, distribuição e varejo de produtos petrolíferos."@pt-br .


###  https://w3id.org/energy-domain/edo#DrawingDimensionsTable
edo:DrawingDimensionsTable rdf:type owl:Class ;
                           rdfs:subClassOf edo:DomainAttribute ;
                           dcterms:accessRights "PUBLIC" ;
                           dcterms:identifier "DrawingDimensionsTable" ;
                           skos:definition "Provides dimensional data required for the design and fabrication, ensuring that all measurements are accurately represented for proper construction and assembly. This information is essential for maintaining consistency and precision in the manufacturing process."@en ;
                           skos:prefLabel "Drawing Dimensions Table"@en ,
                                          "Tabela de Dimensões do Desenho"@pt-br .


###  https://w3id.org/energy-domain/edo#DrawingDimensionsTable_DimensionDescription
edo:DrawingDimensionsTable_DimensionDescription rdf:type owl:Class ;
                                                rdfs:subClassOf edo:DomainAttribute ;
                                                dcterms:accessRights "PUBLIC" ;
                                                dcterms:identifier "DrawingDimensionsTable_DimensionDescription" ;
                                                skos:definition "Descrição (Exemplo: Cota do ponto A ao ponto B)"@pt-br ,
                                                                "Provides a detailed description of the dimension. This property explains what the dimension represents, including its relevance and how it relates to other features or components."@en ;
                                                skos:prefLabel "Descrição da Dimensão"@pt-br ,
                                                               "Dimension Description"@en ;
                                                edo:hasTypedValue edo:stringValue ;
                                                edo:hasValueCardinality edo:multiValue .


###  https://w3id.org/energy-domain/edo#DrawingDimensionsTable_DimensionName
edo:DrawingDimensionsTable_DimensionName rdf:type owl:Class ;
                                         rdfs:subClassOf edo:DomainAttribute ;
                                         dcterms:accessRights "PUBLIC" ;
                                         dcterms:identifier "DrawingDimensionsTable_DimensionName" ;
                                         skos:definition "Indicates the name or label assigned to the dimension. This property identifies the specific dimension, which helps in referencing and distinguishing it from other dimensions."@en ;
                                         skos:prefLabel "Dimension Name"@en ,
                                                        "Nome da dimensão"@pt-br ;
                                         edo:hasTypedValue edo:stringValue ;
                                         edo:hasValueCardinality edo:multiValue .


###  https://w3id.org/energy-domain/edo#DrawingDimensionsTable_DimensionUnit
edo:DrawingDimensionsTable_DimensionUnit rdf:type owl:Class ;
                                         rdfs:subClassOf edo:DomainAttribute ;
                                         dcterms:accessRights "PUBLIC" ;
                                         dcterms:identifier "DrawingDimensionsTable_DimensionUnit" ;
                                         skos:definition "A unidade pode qualquer uma do SI (Sistema Internacional de Unidades), por exemplo mm, °, etc."@pt-br ,
                                                         "Specifies the unit of measurement for the dimension value, expressed in SI units. For linear dimensions, this would be meters or millimeters, while for angles, it would be degrees. This property ensures that all measurements are clear, consistent, and standardized."@en ;
                                         skos:prefLabel "Dimension Unit"@en ,
                                                        "Unidade de Dimensão"@pt-br ;
                                         edo:hasTypedValue edo:stringValue ;
                                         edo:hasValueCardinality edo:multiValue .


###  https://w3id.org/energy-domain/edo#DrawingDimensionsTable_DimensionValue
edo:DrawingDimensionsTable_DimensionValue rdf:type owl:Class ;
                                          rdfs:subClassOf edo:DomainAttribute ;
                                          dcterms:accessRights "PUBLIC" ;
                                          dcterms:identifier "DrawingDimensionsTable_DimensionValue" ;
                                          skos:definition "Specifies the actual measurement value of the dimension. This property provides the numerical value for the dimension, which is critical for understanding the size and placement of components or features."@en ;
                                          skos:prefLabel "Dimension Value"@en ,
                                                         "Valor da dimensão"@pt-br ;
                                          edo:hasTypedValue edo:floatValue ;
                                          edo:hasValueCardinality edo:multiValue .


###  https://w3id.org/energy-domain/edo#EModVsTempTable_ElasticityModulus
edo:EModVsTempTable_ElasticityModulus rdf:type owl:Class ;
                                      rdfs:subClassOf edo:DomainAttribute ;
                                      dcterms:accessRights "PUBLIC" ;
                                      dcterms:identifier "EModVsTempTable_ElasticityModulus" ;
                                      skos:definition "Módulo de elasticidade em função da temperatura (Específica para Materiais Poliméricos)"@pt-br ,
                                                      "Represents the modulus of elasticity values corresponding to specific temperatures. This property provides the stiffness or resistance to deformation of the material at each listed temperature, ensuring that the material's mechanical response is understood under varying thermal conditions."@en ;
                                      skos:prefLabel "Elasticity Modulus Versus Temperature Table - Elasticity Modulus"@en ,
                                                     "Tabela do Módulo de Elasticidade em Função da Temperatura - Módulo de Elasticidade"@pt-br ;
                                      edo:hasTypedValue edo:floatValue ;
                                      edo:hasValueCardinality edo:multiValue .


###  https://w3id.org/energy-domain/edo#EarlyLeakMaxPressTable_Press
edo:EarlyLeakMaxPressTable_Press rdf:type owl:Class ;
                                 rdfs:subClassOf edo:DomainAttribute ;
                                 dcterms:accessRights "PUBLIC" ;
                                 dcterms:identifier "EarlyLeakMaxPressTable_Press" ;
                                 skos:definition "Condições de teste dos tramos para Pressão - Máxima - Teste de vazamento hidrostático precoce"@pt-br ,
                                                 "The maximum pressure applied during the Early Leak Test, verifying resistance under extreme pressure conditions."@en ;
                                 skos:prefLabel "Early Leak Maximum Pressure Table - Pressure"@en ,
                                                "Tabela de Pressão Máxima de Vazamento Precoce - Pressão"@pt-br ;
                                 edo:hasTypedValue edo:floatValue ;
                                 edo:hasValueCardinality edo:multiValue .


###  https://w3id.org/energy-domain/edo#EarlyLeakMaxPressTable_PressIntValStrat
edo:EarlyLeakMaxPressTable_PressIntValStrat rdf:type owl:Class ;
                                            rdfs:subClassOf edo:DomainAttribute ;
                                            dcterms:accessRights "PUBLIC" ;
                                            dcterms:identifier "EarlyLeakMaxPressTable_PressIntValStrat" ;
                                            skos:definition "Condições de teste dos tramos para Estratégia de valores intermediários - Máximo - Teste de vazamento hidrostático precoce"@pt-br ,
                                                            "Strategy used to calculate intermediate values between maximum conditions during the Early Leak Test."@en ;
                                            skos:prefLabel "Early Leak Maximum Pressure Table - Pressure Intermediate Values Strategy"@en ,
                                                           "Tabela de Pressão Máxima de Vazamento Precoce - Estratégia de Valores Intermediários de Pressão"@pt-br ;
                                            edo:hasTypedValue edo:stringValue ;
                                            edo:hasValueCardinality edo:singleValue .


###  https://w3id.org/energy-domain/edo#EarlyLeakMaxPressTable_PressValRef
edo:EarlyLeakMaxPressTable_PressValRef rdf:type owl:Class ;
                                       rdfs:subClassOf edo:DomainAttribute ;
                                       dcterms:accessRights "PUBLIC" ;
                                       dcterms:identifier "EarlyLeakMaxPressTable_PressValRef" ;
                                       skos:definition "Comentários Condições de teste dos tramos para - Máximo - Teste de vazamento hidrostático precoce"@pt-br ,
                                                       "Specifies the reference pressure used to determine the Early Leak Maximum Pressure value."@en ;
                                       skos:prefLabel "Early Leak Maximum Pressure Table - Pressure Value Reference"@en ,
                                                      "Tabela de Pressão Máxima de Vazamento Precoce - Referência de Valor de Pressão"@pt-br ;
                                       edo:hasTypedValue edo:stringValue ;
                                       edo:hasValueCardinality edo:multiValue .


###  https://w3id.org/energy-domain/edo#EarlyLeakMaxPressTable_PressValRefMult
edo:EarlyLeakMaxPressTable_PressValRefMult rdf:type owl:Class ;
                                           rdfs:subClassOf edo:DomainAttribute ;
                                           dcterms:accessRights "PUBLIC" ;
                                           dcterms:identifier "EarlyLeakMaxPressTable_PressValRefMult" ;
                                           skos:definition "Early Leak Maximum Pressure Table - Pressure Value Reference Multiplier"@pt-br ,
                                                           "The multiplier applied to the reference pressure to determine the Early Leak Maximum Pressure value."@en ;
                                           skos:prefLabel "Early Leak Maximum Pressure Table - Pressure Value Reference Multiplier"@en ,
                                                          "Tabela de Pressão Máxima de Vazamento Precoce - Multiplicador de Referência de Valor de Pressão"@pt-br ;
                                           edo:hasTypedValue edo:floatValue ;
                                           edo:hasValueCardinality edo:multiValue .


###  https://w3id.org/energy-domain/edo#EarlyLeakMaxPressTable_TensLimit
edo:EarlyLeakMaxPressTable_TensLimit rdf:type owl:Class ;
                                     rdfs:subClassOf edo:DomainAttribute ;
                                     dcterms:accessRights "PUBLIC" ;
                                     dcterms:identifier "EarlyLeakMaxPressTable_TensLimit" ;
                                     skos:definition "Condições de teste dos tramos para Tensão - Máxima - Teste de vazamento hidrostático precoce"@pt-br ,
                                                     "Tensile limit condition that must be respected to avoid damaging the tested product."@en ;
                                     skos:prefLabel "Early Leak Maximum Pressure Table - Tensile Limit"@en ,
                                                    "Tabela de Pressão Máxima de Vazamento Precoce - Limite de Tração"@pt-br ;
                                     edo:hasTypedValue edo:floatValue ;
                                     edo:hasValueCardinality edo:multiValue .


###  https://w3id.org/energy-domain/edo#EarlyLeakMaxPressTable_TensLimitValRef
edo:EarlyLeakMaxPressTable_TensLimitValRef rdf:type owl:Class ;
                                           rdfs:subClassOf edo:DomainAttribute ;
                                           dcterms:accessRights "PUBLIC" ;
                                           dcterms:identifier "EarlyLeakMaxPressTable_TensLimitValRef" ;
                                           skos:definition "Indicates the basis used to establish the tensile limit value during the Early Leak Maximum Pressure Test, ensuring the product's tensile strength is respected to avoid damage."@en ;
                                           skos:prefLabel "Early Leak Maximum Pressure Table - Tensile Limit Value Reference"@en ,
                                                          "Tabela de Pressão Máxima de Vazamento Precoce - Referência do Limite de Tração"@pt-br ;
                                           edo:hasTypedValue edo:stringValue ;
                                           edo:hasValueCardinality edo:multiValue .


###  https://w3id.org/energy-domain/edo#EarlyLeakNomPressTable_Press
edo:EarlyLeakNomPressTable_Press rdf:type owl:Class ;
                                 rdfs:subClassOf edo:DomainAttribute ;
                                 dcterms:accessRights "PUBLIC" ;
                                 dcterms:identifier "EarlyLeakNomPressTable_Press" ;
                                 skos:definition "Condições de teste dos tramos para Pressão - Nominal - Teste de vazamento hidrostático precoce"@pt-br ,
                                                 "The nominal pressure applied during the Early Leak Test, verifying standard operational conditions for leakage detection."@en ;
                                 skos:prefLabel "Early Leak Nominal Pressure Table - Pressure"@en ,
                                                "Tabela de Pressão Nominal de Vazamento Precoce - Pressão"@pt-br ;
                                 edo:hasTypedValue edo:floatValue ;
                                 edo:hasValueCardinality edo:multiValue .


###  https://w3id.org/energy-domain/edo#EarlyLeakNomPressTable_PressIntValStrat
edo:EarlyLeakNomPressTable_PressIntValStrat rdf:type owl:Class ;
                                            rdfs:subClassOf edo:DomainAttribute ;
                                            dcterms:accessRights "PUBLIC" ;
                                            dcterms:identifier "EarlyLeakNomPressTable_PressIntValStrat" ;
                                            skos:definition "Condições de teste dos tramos para Estratégia de valores intermediários - Nominal - Teste de vazamento hidrostático precoce"@pt-br ,
                                                            "Strategy used to calculate intermediate Pressure values between nominal conditions during the Early Leak Test."@en ;
                                            skos:prefLabel "Early Leak Nominal Pressure Table - Pressure Intermediate Values Strategy"@en ,
                                                           "Tabela de Pressão Nominal de Vazamento Precoce - Estratégia de Valores Intermediários de Pressão"@pt-br ;
                                            edo:hasTypedValue edo:stringValue ;
                                            edo:hasValueCardinality edo:multiValue .


###  https://w3id.org/energy-domain/edo#EarlyLeakNomPressTable_PressValRef
edo:EarlyLeakNomPressTable_PressValRef rdf:type owl:Class ;
                                       rdfs:subClassOf edo:DomainAttribute ;
                                       dcterms:accessRights "PUBLIC" ;
                                       dcterms:identifier "EarlyLeakNomPressTable_PressValRef" ;
                                       skos:definition "Comentários Condições de teste dos tramos para - Nominal - Teste de vazamento hidrostático precoce"@pt-br ,
                                                       "Specifies the reference pressure used to determine the Early Leak Nominal Pressure value."@en ;
                                       skos:prefLabel "Early Leak Nominal Pressure Table - Pressure Value Reference"@en ,
                                                      "Tabela de Pressão Nominal de Vazamento Precoce - Referência de Valor de Pressão"@pt-br ;
                                       edo:hasTypedValue edo:stringValue ;
                                       edo:hasValueCardinality edo:multiValue .


###  https://w3id.org/energy-domain/edo#EarlyLeakNomPressTable_PressValRefMult
edo:EarlyLeakNomPressTable_PressValRefMult rdf:type owl:Class ;
                                           rdfs:subClassOf edo:DomainAttribute ;
                                           dcterms:accessRights "PUBLIC" ;
                                           dcterms:identifier "EarlyLeakNomPressTable_PressValRefMult" ;
                                           skos:definition "The multiplier applied to the reference pressure to determine the Early Leak Nominal Pressure value."@en ;
                                           skos:prefLabel "Early Leak Nominal Pressure Table - Pressure Value Reference Multiplier"@en ,
                                                          "Tabela de Pressão Nominal de Vazamento Precoce - Multiplicador de Referência de Valor de Pressão"@pt-br ;
                                           edo:hasTypedValue edo:floatValue ;
                                           edo:hasValueCardinality edo:multiValue .


###  https://w3id.org/energy-domain/edo#EarlyLeakNomPressTable_TensLimit
edo:EarlyLeakNomPressTable_TensLimit rdf:type owl:Class ;
                                     rdfs:subClassOf edo:DomainAttribute ;
                                     dcterms:accessRights "PUBLIC" ;
                                     dcterms:identifier "EarlyLeakNomPressTable_TensLimit" ;
                                     skos:definition "Condições de teste dos tramos para Tensão - Nominal - Teste de vazamento hidrostático precoce"@pt-br ,
                                                     "Tensile limit condition that must be respected to avoid damaging the tested product."@en ;
                                     skos:prefLabel "Early Leak Nominal Pressure Table - Tensile Limit"@en ,
                                                    "Tabela de Pressão Nominal de Vazamento Precoce - Limite de Tração"@pt-br ;
                                     edo:hasTypedValue edo:floatValue ;
                                     edo:hasValueCardinality edo:multiValue .


###  https://w3id.org/energy-domain/edo#EarlyLeakNomPressTable_TensLimitValRef
edo:EarlyLeakNomPressTable_TensLimitValRef rdf:type owl:Class ;
                                           rdfs:subClassOf edo:DomainAttribute ;
                                           dcterms:accessRights "PUBLIC" ;
                                           dcterms:identifier "EarlyLeakNomPressTable_TensLimitValRef" ;
                                           skos:definition "Indicates the basis used to establish the tensile limit value during the Early Leak Nominal Pressure Test, ensuring the product's tensile strength is respected to avoid damage."@en ;
                                           skos:prefLabel "Early Leak Nominal Pressure Table - Tensile Limit Value Reference"@en ,
                                                          "Tabela de Pressão Nominal de Vazamento Precoce - Referência do Limite de Tração"@pt-br ;
                                           edo:hasTypedValue edo:stringValue ;
                                           edo:hasValueCardinality edo:multiValue .


###  https://w3id.org/energy-domain/edo#ElasticityModulusAt23Degrees
edo:ElasticityModulusAt23Degrees rdf:type owl:Class ;
                                 rdfs:subClassOf edo:DomainAttribute ;
                                 dcterms:accessRights "PUBLIC" ;
                                 dcterms:identifier "ElasticityModulusAt23Degrees" ;
                                 skos:definition "Módulo de elasticidade a 23 graus Celsius (Específica para Materiais Metálicos e Poliméricos)"@pt-br ,
                                                 "Specifies the modulus of elasticity of the material at 23 degrees Celsius, indicating its stiffness or resistance to deformation under stress at this temperature. This property is crucial for determining how the flexible structure responds to mechanical loads, ensuring that it maintains structural integrity."@en ;
                                 skos:prefLabel "Elasticity Modulus At 23 Degrees"@en ,
                                                "Módulo de Elasticidade a 23 Graus Celsius"@pt-br ;
                                 edo:hasTypedValue edo:floatValue ;
                                 edo:hasValueCardinality edo:singleValue .


###  https://w3id.org/energy-domain/edo#ElectricalEngineering
edo:ElectricalEngineering rdf:type owl:Class ;
                          rdfs:subClassOf edo:TechnicalDiscipline ;
                          rdfs:label "Electrical Engineering"@en ,
                                     "Engenharia Elétrica"@pt-br ;
                          skos:definition "Disciplina de engenharia focada em sistemas elétricos, distribuição e geração de energia."@pt-br ,
                                          "Engineering discipline focused on electrical systems, power distribution and generation."@en .


###  https://w3id.org/energy-domain/edo#EndFitting
edo:EndFitting rdf:type owl:Class ;
               rdfs:subClassOf edo:PipeTermination ;
               dcterms:identifier "EndFitting" ;
               skos:altLabel "Connector Fitting"@en ,
                             "End Termination"@en ,
                             "Termination Assembly"@en ,
                             "Termination Fitting"@en ;
               skos:definition "Component used in subsea flexible pipes to provide a secure transition between the flexible pipe and rigid structures, such as subsea equipment or topside facilities, as well as to connect two sections of flexible pipe. The End Fitting ensures the structural integrity and sealing of the pipe, allowing for the connection of the flexible line to other equipment or sections while withstanding internal pressures and environmental forces. It is a critical interface that accommodates the pipe's mechanical, hydraulic, and thermal loads, ensuring long-term reliable performance in harsh subsea conditions."@en ,
                               "Componente utilizado em dutos flexíveis para fornecer uma transição segura entre o duto flexível e estruturas rígidas, como equipamentos submersos ou instalações no topo, bem como para conectar duas seções de duto flexível. O Terminador garante a integridade estrutural e o vedamento do duto, permitindo a conexão da linha flexível a outros equipamentos ou seções, resistindo a pressões internas e forças ambientais. É uma interface crítica que acomoda as cargas mecânicas, hidráulicas e térmicas do duto, garantindo desempenho confiável a longo prazo em condições submarinas adversas."@pt-br ;
               skos:prefLabel "Conector de Extremidade"@pt-br ,
                              "End fitting"@en ;
               edo:hasAttribute edo:BoreDiameter ,
                                edo:FlangeFaceType ,
                                edo:FlangeType ,
                                edo:HasFaceORing ,
                                edo:HasModaSensor ,
                                edo:HasN2InjectionPort ,
                                edo:RingGasketInnerDIameter ,
                                edo:RingGasketOuterDiameter ,
                                edo:RingGasketPressureRating ,
                                edo:RingGasketSpecification ,
                                edo:RingGasketStandard ,
                                edo:RingGasketType ;
               edo:ifc_equivalentClass "IfcPipeFitting" ;
               edo:ifc_objectType "EndFitting" ;
               edo:ifc_predefinedType "USERDEFINED" .


###  https://w3id.org/energy-domain/edo#EnergyStorage
edo:EnergyStorage rdf:type owl:Class ;
                  rdfs:subClassOf edo:Domain ;
                  rdfs:label "Armazenamento de Energia"@pt-br ,
                             "Energy Storage"@en ;
                  skos:definition "Technologies for storing energy, such as batteries, pumped hydro, or compressed air."@en ,
                                  "Tecnologias para armazenamento de energia, como baterias, hidroelétricas reversíveis ou ar comprimido."@pt-br .


###  https://w3id.org/energy-domain/edo#EquipmentEngineering
edo:EquipmentEngineering rdf:type owl:Class ;
                         rdfs:subClassOf edo:TechnicalDiscipline ;
                         rdfs:label "Engenharia de Equipamentos"@pt-br ,
                                    "Equipment Engineering"@en ;
                         skos:definition "Disciplina de engenharia focada no projeto e especificação de equipamentos industriais."@pt-br ,
                                         "Engineering discipline focused on the design and specification of industrial equipment."@en .


###  https://w3id.org/energy-domain/edo#EquipmentLocation
edo:EquipmentLocation rdf:type owl:Class ;
                      rdfs:subClassOf edo:PointLocation ;
                      dcterms:identifier "EquipmentLocation" ;
                      skos:definition "Base for installation sites for large underwater equipment."@en ;
                      skos:prefLabel "Equipment Location"@en ,
                                     "Localização de Equipamento"@pt-br .


###  https://w3id.org/energy-domain/edo#ErosionalVelocity
edo:ErosionalVelocity rdf:type owl:Class ;
                      rdfs:subClassOf edo:DomainAttribute ;
                      dcterms:accessRights "PUBLIC" ;
                      dcterms:identifier "ErosionalVelocity" ;
                      skos:definition "Represents the maximum velocity of a fluid at which erosion of the material begins to occur. This property is crucial for determining the operational limits of the system, ensuring that the material can withstand fluid flow without suffering erosive damage."@en ;
                      skos:prefLabel "Erosional Velocity"@en ,
                                     "Velocidade erosional"@pt-br ;
                      edo:hasTypedValue edo:stringValue ;
                      edo:hasValueCardinality edo:singleValue .


###  https://w3id.org/energy-domain/edo#ExecutiveProjectRevision
edo:ExecutiveProjectRevision rdf:type owl:Class ;
                             rdfs:subClassOf edo:DomainAttribute ;
                             dcterms:accessRights "PUBLIC" ;
                             dcterms:identifier "ExecutiveProjectRevision" ;
                             skos:definition "Indicates the revision number of the executive project, represented as a numeric value that is incremented with each new submission (e.g., 0000, 0001, 0002), stored as text for consistency in formatting."@en ,
                                             "Revisão do projeto executivo  Valor numérico incrementado a cada novo envio (0000, 0001, 0002 e etc.) como texto"@pt-br ;
                             skos:prefLabel "Executive Project Revision"@en ,
                                            "Revisão do Projeto Executivo"@pt-br ;
                             edo:hasTypedValue edo:stringValue ;
                             edo:hasValueCardinality edo:singleValue .


###  https://w3id.org/energy-domain/edo#ExternalDiameter
edo:ExternalDiameter rdf:type owl:Class ;
                     rdfs:subClassOf edo:DomainAttribute ;
                     dcterms:accessRights "PUBLIC" ;
                     dcterms:identifier "ExternalDiameter" ;
                     skos:definition "Distance measured across the outermost points, passing through the center."@en ;
                     skos:prefLabel "Diâmetro externo"@pt-br ,
                                    "External Diameter"@en ;
                     edo:hasTypedValue edo:floatValue ;
                     edo:hasValueCardinality edo:singleValue .


###  https://w3id.org/energy-domain/edo#FEED
edo:FEED rdf:type owl:Class ;
         rdfs:subClassOf edo:LifecyclePhase ;
         rdfs:label "FEED (Front-End Engineering Design)"@en ,
                    "FEED (Projeto Básico de Engenharia)"@pt-br ;
         skos:definition "Fase intermediária entre o projeto conceitual e detalhado, refinando detalhes técnicos e de custo."@pt-br ,
                         "Intermediate phase between conceptual and detailed design, refining technical and cost details."@en .


###  https://w3id.org/energy-domain/edo#FabricTape
edo:FabricTape rdf:type owl:Class ;
               rdfs:subClassOf edo:TapeLayer ;
               dcterms:identifier "FabricTape" ;
               skos:definition "Material used in subsea flexible pipe construction, typically applied as a wrapping layer to provide protection and containment for internal components. Fabric Tape is designed to secure and hold various layers of the pipe in place during manufacturing and operation, preventing displacement or damage to the underlying layers. It also adds a layer of abrasion resistance, contributing to the overall durability of the pipe in dynamic subsea environments. Made from high-strength, flexible materials, Fabric Tape plays a key role in maintaining the integrity of the flexible pipe structure."@en ,
                               "Material utilizado na construção de dutos flexíveis, geralmente aplicado como uma camada de envolvimento para fornecer proteção e contenção para os componentes internos. A Fita Construtiva é projetada para segurar e manter as várias camadas do duto no lugar durante a fabricação e operação, evitando o deslocamento ou danos às camadas subjacentes. Ela também adiciona uma camada de resistência à abrasão, contribuindo para a durabilidade geral do duto em ambientes dinâmicos. Feita de materiais flexíveis e de alta resistência, a Fita Construtiva desempenha um papel crucial na manutenção da integridade da estrutura do duto flexível."@pt-br ;
               skos:prefLabel "Fabric Tape"@en ,
                              "Fita Construtiva"@pt-br ;
               edo:ifc_equivalentClass "IfcPipeSegment" ;
               edo:ifc_objectType "FabricTape" ;
               edo:ifc_predefinedType "USERDEFINED" .


###  https://w3id.org/energy-domain/edo#Fabrication
edo:Fabrication rdf:type owl:Class ;
                rdfs:subClassOf edo:LifecyclePhase ;
                rdfs:label "Fabrication"@en ,
                           "Fabricação"@pt-br ;
                skos:definition "Fabricação e montagem de componentes, módulos ou estruturas em oficinas ou estaleiros."@pt-br ,
                                "Manufacturing and assembly of components, modules, or structures in workshops or yards."@en .


###  https://w3id.org/energy-domain/edo#FatMaxPress
edo:FatMaxPress rdf:type owl:Class ;
                rdfs:subClassOf edo:DomainAttribute ;
                dcterms:accessRights "PUBLIC" ;
                dcterms:identifier "FatMaxPress" ;
                skos:definition "Condições de teste dos tramos para Pressão - Máxima - FAT hidrostática"@pt-br ,
                                "The maximum pressure applied during the Factory Acceptance Test (FAT) to ensure the equipment can withstand extreme conditions."@en ;
                skos:prefLabel "Factory Acceptance Test Maximum Pressure"@en ,
                               "Pressão Máxima para o Teste de Aceitação na Fábrica"@pt-br ;
                edo:hasTypedValue edo:floatValue ;
                edo:hasValueCardinality edo:singleValue .


###  https://w3id.org/energy-domain/edo#FatMaxPressValRef
edo:FatMaxPressValRef rdf:type owl:Class ;
                      rdfs:subClassOf edo:DomainAttribute ;
                      dcterms:accessRights "PUBLIC" ;
                      dcterms:identifier "FatMaxPressValRef" ;
                      skos:definition "Comentários Condições de teste dos tramos para - Máximo - FAT hidrostático"@pt-br ,
                                      "Specifies the reference pressure used to determine the FAT maximum pressure value."@en ;
                      skos:prefLabel "Factory Acceptance Test Maximum Pressure Value Reference"@en ,
                                     "Referência de Valor de Pressão Máxima para o Teste de Aceitação na Fábrica"@pt-br ;
                      edo:hasTypedValue edo:stringValue ;
                      edo:hasValueCardinality edo:singleValue .


###  https://w3id.org/energy-domain/edo#FatMaxPressValRefMult
edo:FatMaxPressValRefMult rdf:type owl:Class ;
                          rdfs:subClassOf edo:DomainAttribute ;
                          dcterms:accessRights "PUBLIC" ;
                          dcterms:identifier "FatMaxPressValRefMult" ;
                          skos:definition "The multiplier applied to the reference pressure to determine the FAT maximum pressure value."@en ;
                          skos:prefLabel "Factory Acceptance Test Maximum Pressure Value Reference Multiplier"@en ,
                                         "Multiplicador de Referência de Valor de Pressão Máxima para Teste de Aceitação na Fábrica"@pt-br ;
                          edo:hasTypedValue edo:floatValue ;
                          edo:hasValueCardinality edo:singleValue .


###  https://w3id.org/energy-domain/edo#FatNomPress
edo:FatNomPress rdf:type owl:Class ;
                rdfs:subClassOf edo:DomainAttribute ;
                dcterms:accessRights "PUBLIC" ;
                dcterms:identifier "FatNomPress" ;
                skos:definition "Condições de teste dos tramos para Pressão - Nominal - FAT hidrostático"@pt-br ,
                                "The nominal pressure applied during the Factory Acceptance Test (FAT), simulating typical operating conditions to verify equipment performance."@en ;
                skos:prefLabel "Factory Acceptance Test Nominal Pressure"@en ,
                               "Pressão Nominal para o Teste de Aceitação na Fábrica"@pt-br ;
                edo:hasTypedValue edo:floatValue ;
                edo:hasValueCardinality edo:singleValue .


###  https://w3id.org/energy-domain/edo#FatNomPressValRef
edo:FatNomPressValRef rdf:type owl:Class ;
                      rdfs:subClassOf edo:DomainAttribute ;
                      dcterms:accessRights "PUBLIC" ;
                      dcterms:identifier "FatNomPressValRef" ;
                      skos:definition "Comentários Condições de teste dos tramos para - Nominal - FAT hidrostático"@pt-br ,
                                      "Specifies the reference pressure used to determine the FAT nominal pressure value."@en ;
                      skos:prefLabel "Factory Acceptance Test Nominal Pressure Value Reference"@en ,
                                     "Referência de Valor de Pressão Nominal para o Teste de Aceitação na Fábrica"@pt-br ;
                      edo:hasTypedValue edo:stringValue ;
                      edo:hasValueCardinality edo:singleValue .


###  https://w3id.org/energy-domain/edo#FatNomPressValRefMult
edo:FatNomPressValRefMult rdf:type owl:Class ;
                          rdfs:subClassOf edo:DomainAttribute ;
                          dcterms:accessRights "PUBLIC" ;
                          dcterms:identifier "FatNomPressValRefMult" ;
                          skos:definition "The multiplier applied to the reference pressure to determine the FAT nominal pressure value."@en ;
                          skos:prefLabel "Factory Acceptance Test Nominal Pressure Value Reference Multiplier"@en ,
                                         "Multiplicador de Referência de Valor de Pressão Nominal para Teste de Aceitação na Fábrica"@pt-br ;
                          edo:hasTypedValue edo:floatValue ;
                          edo:hasValueCardinality edo:singleValue .


###  https://w3id.org/energy-domain/edo#FiberOpticJumper
edo:FiberOpticJumper rdf:type owl:Class ;
                     rdfs:subClassOf edo:LinearObject ;
                     dcterms:identifier "FiberOpticJumper" .


###  https://w3id.org/energy-domain/edo#FlangeFaceType
edo:FlangeFaceType rdf:type owl:Class ;
                   rdfs:subClassOf edo:DomainAttribute ;
                   dcterms:accessRights "PUBLIC" ;
                   dcterms:identifier "FlangeFaceType" ;
                   skos:definition "Specific design of the sealing surface used to ensure a secure, leak-tight connection. The face type plays a crucial role in maintaining the integrity of the seal under the extreme pressures and temperatures. It is engineered to prevent leaks, withstand high mechanical loads, and provide long-term durability. The appropriate face type is chosen based on factors such as pressure rating, sealing requirements, and environmental conditions."@en ;
                   skos:prefLabel "Flange Face Type"@en ,
                                  "Tipo da Face do Flange"@pt-br ;
                   edo:hasTypedValue edo:stringValue ;
                   edo:hasValueCardinality edo:singleValue .


###  https://w3id.org/energy-domain/edo#FlangeType
edo:FlangeType rdf:type owl:Class ;
               rdfs:subClassOf edo:DomainAttribute ;
               dcterms:accessRights "PUBLIC" ;
               dcterms:identifier "FlangeType" ;
               skos:definition "Specifies the type of flange within the Standard, which defines certain characteristics, like the Standard itself, Type or Class, Diameter and Operating Pressure."@en ;
               skos:prefLabel "Flange Type"@en ,
                              "Tipo de Flange"@pt-br ;
               edo:hasTypedValue edo:stringValue ;
               edo:hasValueCardinality edo:singleValue .


###  https://w3id.org/energy-domain/edo#FlexiblePipeSegment
edo:FlexiblePipeSegment rdf:type owl:Class ;
                        rdfs:subClassOf edo:PipeSegment ;
                        dcterms:identifier "FlexiblePipeSegment" ;
                        skos:altLabel "Flexible Line Section"@en ,
                                      "Flexible Pipe Section"@en ,
                                      "Flexible Pipe Segment"@en ,
                                      "Subsea Pipe Segment"@en ;
                        skos:definition "A segment of a flexible pipe that forms part of the overall pipeline system. The Flexible Pipe Segment is designed to transport fluids or gases over varying distances and conditions on the seafloor. Each section is engineered to handle specific environmental and operational requirements, contributing to the flexibility, durability, and performance of the subsea pipeline system."@en ,
                                        "Um segmento de duto flexível que faz parte do sistema de pipeline geral. O Tramo Flexível é projetado para transportar fluidos ou gases por distâncias e condições variadas no fundo do mar. Cada seção é projetada para atender a requisitos ambientais e operacionais específicos, contribuindo para a flexibilidade, durabilidade e desempenho do sistema de dutos submarinos."@pt-br ;
                        skos:prefLabel "Flexible Pipe Segment"@en ,
                                       "Tramo de Duto Flexível"@pt-br ;
                        edo:hasAttribute edo:AssemblyShouldObeyModelPolarity ,
                                         edo:EarlyLeakMaxPressTable_Press ,
                                         edo:EarlyLeakMaxPressTable_PressIntValStrat ,
                                         edo:EarlyLeakMaxPressTable_PressValRef ,
                                         edo:EarlyLeakMaxPressTable_PressValRefMult ,
                                         edo:EarlyLeakMaxPressTable_TensLimit ,
                                         edo:EarlyLeakMaxPressTable_TensLimitValRef ,
                                         edo:EarlyLeakNomPressTable_Press ,
                                         edo:EarlyLeakNomPressTable_PressIntValStrat ,
                                         edo:EarlyLeakNomPressTable_PressValRef ,
                                         edo:EarlyLeakNomPressTable_PressValRefMult ,
                                         edo:EarlyLeakNomPressTable_TensLimit ,
                                         edo:EarlyLeakNomPressTable_TensLimitValRef ,
                                         edo:FatMaxPress ,
                                         edo:FatMaxPressValRef ,
                                         edo:FatMaxPressValRefMult ,
                                         edo:FatNomPress ,
                                         edo:FatNomPressValRef ,
                                         edo:FatNomPressValRefMult ,
                                         edo:IdInUnifilarDiagram ,
                                         edo:ManufacturingDate ,
                                         edo:ManufacturingNonConformities ,
                                         edo:MaxLengthTolerance ,
                                         edo:NominalLength ,
                                         edo:OffLeakPLevMaxPress ,
                                         edo:OffLeakPLevMaxPressValRef ,
                                         edo:OffLeakPLevMaxPressValRefMult ,
                                         edo:OffLeakPLevNomPress ,
                                         edo:OffLeakPLevNomPressValRef ,
                                         edo:OffLeakPLevNomPressValRefMult ,
                                         edo:PipeSectionApplication ,
                                         edo:SpecialRequirements ,
                                         edo:StrIntOffPLevMaxPress ,
                                         edo:StrIntOffPLevMaxPressValRef ,
                                         edo:StrIntOffPLevMaxPressValRefMult ,
                                         edo:StrIntOffPLevNomPress ,
                                         edo:StrIntOffPLevNomPressValRef ,
                                         edo:StrIntOffPLevNomPressValRefMult ,
                                         edo:StrIntOnNoTensMaxPress ,
                                         edo:StrIntOnNoTensMaxPressValRef ,
                                         edo:StrIntOnNoTensMaxPressValRefMult ,
                                         edo:StrIntOnNoTensNomPress ,
                                         edo:StrIntOnNoTensNomPressValRef ,
                                         edo:StrIntOnNoTensNomPressValRefMult ;
                        edo:ifc_equivalentClass "IfcPipeSegment" ;
                        edo:ifc_objectType "FlexiblePipeSegment" ;
                        edo:ifc_predefinedType "USERDEFINED" .


###  https://w3id.org/energy-domain/edo#FlexiblePipeStructure
edo:FlexiblePipeStructure rdf:type owl:Class ;
                          rdfs:subClassOf edo:DomainElement ;
                          dcterms:identifier "FlexiblePipeStructure" ;
                          skos:altLabel "Flexible Structure"@en ,
                                        "Subsea Flexible Configuration"@en ,
                                        "Subsea Flexible Design"@en ;
                          skos:definition "A estrutura do duto flexível é a configuração em camadas de um duto flexível, projetada para fornecer flexibilidade e resistência em ambientes subsea. Ela consiste em múltiplas camadas, cada uma servindo a uma função específica, como contenção de pressão, proteção ou reforço. Essa estrutura é projetada para atender às exigências das condições de águas profundas, incluindo alta pressão e movimentos dinâmicos, garantindo a integridade e o desempenho do duto."@pt-br ,
                                          "The Flexible Pipe Structure is the layered configuration of a flexible pipe, designed to provide flexibility and strength in subsea environments. It consists of multiple layers, each serving a specific function, such as pressure containment, protection, or reinforcement. This structure is engineered to handle the demands of deepwater conditions, including high pressure and dynamic movements, ensuring the pipe's integrity and performance."@en ;
                          skos:prefLabel "Estrutura de Duto Flexível"@pt-br ,
                                         "Flexible Pipe Structure"@en ;
                          edo:hasAttribute edo:AbsoluteInsidePressure ,
                                           edo:AbsoluteOutsidePressure ,
                                           edo:AxialStiffnessUnderCompressionAtSeaLevel ,
                                           edo:AxialStiffnessUnderTensionAtSeaLevel ,
                                           edo:BendingMomentTable ,
                                           edo:BendingMomentTable_BendingMoment ,
                                           edo:BendingMomentTable_Curvature ,
                                           edo:CalculatedAbsoluteBurstPressure ,
                                           edo:CriticalCurvatureOfSlipping ,
                                           edo:DamagingPullInStraightLine ,
                                           edo:DimensioningCriteria ,
                                           edo:ErosionalVelocity ,
                                           edo:FlexibleStructureServicesList ,
                                           edo:FrictionCoefBetweenPipeAndTensioner ,
                                           edo:FrictionCoefficientTighteningTable ,
                                           edo:FrictionCoefficientTighteningTable_CoefficientOfFriction ,
                                           edo:FrictionCoefficientTighteningTable_TighteningPerTrack ,
                                           edo:HydrostaticCollapseAbsPressDry ,
                                           edo:InsideTemperature ,
                                           edo:IntermediateValuesStrategy ,
                                           edo:InternalDiameter ,
                                           edo:LayingMinimumRadiusTable ,
                                           edo:LayingMinimumRadiusTable_AbsoluteExternalPressure ,
                                           edo:LayingMinimumRadiusTable_AbsoluteInternalPressure ,
                                           edo:LayingMinimumRadiusTable_Compression ,
                                           edo:LayingMinimumRadiusTable_MinimumAllowableBendingRadius ,
                                           edo:LayingMinimumRadiusTable_SectionSupportedByRigidSupport ,
                                           edo:LayingMinimumRadiusTable_TensileArmourAnnulusCondition ,
                                           edo:LimpTorsionalStiffnessAtSeaLevel ,
                                           edo:LinearMass ,
                                           edo:MaxDesignPressure ,
                                           edo:MaximumAllowableTensileForStraightLine ,
                                           edo:MaximumAllowableTensionTable ,
                                           edo:MaximumAllowableTensionTable_MaximumAllowableTensile ,
                                           edo:MaximumAllowableTensionTable_PulleyRadius ,
                                           edo:MaximumAllowableTensionTable_PulleyVAngle ,
                                           edo:MaximumAllowableTighteningTable ,
                                           edo:MaximumAllowableTighteningTable_AxialLoad ,
                                           edo:MaximumAllowableTighteningTable_TighteningPerTrack ,
                                           edo:MaximumAmbientTemperature ,
                                           edo:MinimumBendingRadiusForStorage ,
                                           edo:OuterDiameter ,
                                           edo:OutsideTemperature ,
                                           edo:PostSlippingBendingStiffness ,
                                           edo:PreSlippingBendingStiffness ,
                                           edo:SpoolingTension ,
                                           edo:StiffTorsionalStiffnessAtSeaLevel ,
                                           edo:StructureApplicationsList ,
                                           edo:StructureCode ,
                                           edo:TensileArmourAnnulusCondition ,
                                           edo:TensileArmourFreeAnnulusVolume ,
                                           edo:TensionerPadsMaterial ,
                                           edo:TensionerPadsOpeningAngle ,
                                           edo:TensionerPadsShape ,
                                           edo:TensionerTracksQuantity ,
                                           edo:TestConditions ,
                                           edo:ThermalExchangeCoefficientFlooded ,
                                           edo:UtilizationFactor ;
                          edo:ifc_equivalentClass "IfcPipeSegmentType" ;
                          edo:ifc_objectType "FlexiblePipeStructure" ;
                          edo:ifc_predefinedType "USERDEFINED" .


###  https://w3id.org/energy-domain/edo#FlexibleStructureLayer
edo:FlexibleStructureLayer rdf:type owl:Class ;
                           rdfs:subClassOf edo:DomainElement ;
                           dcterms:identifier "FlexibleStructureLayer" ;
                           skos:definition "A specific layer within the structure of a subsea flexible pipe, each designed to fulfill a distinct function. These layers work together to provide essential properties such as pressure containment, reinforcement, and environmental protection. Engineered to withstand harsh underwater conditions, each layer contributes to the overall flexibility, durability, and performance of the subsea flexible pipe system."@en ;
                           skos:prefLabel "Camadas de Estruturas Flexíveis"@pt-br ,
                                          "Flexible Structure Layer"@en ;
                           edo:hasAttribute edo:InternalDiameter ,
                                            edo:LayerAnnular ,
                                            edo:LayerAnnularType ,
                                            edo:LayerContinuity ,
                                            edo:LayerGeometryCrossSection ,
                                            edo:LayerGeometryInertiaX ,
                                            edo:LayerGeometryInertiaY ,
                                            edo:LayerGeometryManufacturer ,
                                            edo:LayerGeometryName ,
                                            edo:LayerGeometryProfileThickness ,
                                            edo:LayerGeometryProfileWidth ,
                                            edo:LayerGeometryThickness ,
                                            edo:LayerThickness ,
                                            edo:LayerWatertight ,
                                            edo:LayerWatertightLowerLayerInternalFreeVolume ,
                                            edo:LinearMass .


###  https://w3id.org/energy-domain/edo#FlexibleStructureLayerMaterial
edo:FlexibleStructureLayerMaterial rdf:type owl:Class ;
                                   rdfs:subClassOf edo:DomainElement ;
                                   dcterms:identifier "FlexibleStructureLayerMaterial" ;
                                   skos:definition "Material used to fabricate the individual layers of a subsea flexible structure, each layer serving a distinct function such as pressure containment, tensile reinforcement, or external protection. The Flexible Structure Layer Material is selected based on its specific properties, such as strength, flexibility, corrosion resistance, or thermal insulation, to ensure the overall performance and durability of the flexible pipe in harsh subsea conditions. These materials may include polymers, metals, composites, or other high-performance substances tailored to the pipe's operational demands."@en ;
                                   skos:prefLabel "Flexible Structure Layer Material"@en ,
                                                  "Materiais de Camadas de Estruturas Flexíveis Submarinas"@pt-br ;
                                   edo:hasAttribute edo:ElasticityModulusAt23Degrees ,
                                                    edo:MaterialComposition ,
                                                    edo:PoissonRatioAt23Degrees ,
                                                    edo:SpecificHeatCapacity ,
                                                    edo:SpecificWeight ,
                                                    edo:TechnicalNotes ,
                                                    edo:ThermalConductivityCoefficient .


###  https://w3id.org/energy-domain/edo#FlexibleStructureServicesList
edo:FlexibleStructureServicesList rdf:type owl:Class ;
                                  rdfs:subClassOf edo:DomainAttribute ;
                                  dcterms:accessRights "PUBLIC" ;
                                  dcterms:identifier "FlexibleStructureServicesList" ;
                                  skos:definition "Indicates the list of services that the flexible structure is capable of performing as part of a flexible pipeline. Multiple values can be selected, defining the operational roles the structure is designed to execute."@en ;
                                  skos:prefLabel "Flexible Structure Services List"@en ,
                                                 "Lista de Serviços da Estrutura Flexível"@pt-br ;
                                  edo:hasTypedValue edo:stringValue ;
                                  edo:hasValueCardinality edo:multiValue .


###  https://w3id.org/energy-domain/edo#FloatingProductionUnit
edo:FloatingProductionUnit rdf:type owl:Class ;
                           rdfs:subClassOf edo:Location ;
                           dcterms:identifier "FloatingProductionUnit" ;
                           skos:altLabel "FLNG"@en ,
                                         "FPSO"@en ,
                                         "FPU"@en ,
                                         "Floating Platform"@en ,
                                         "Floating Production Facility"@en ;
                           skos:definition "Offshore platform used in oil and gas exploration and production, designed to extract, process, and store hydrocarbons. The Floating Production Unit (FPU) is anchored or moored to the seabed and can operate in deep waters, often connected to subsea wells via flexible pipes and umbilicals. It accommodates processing equipment for separating oil, gas, and water, as well as facilities for temporary storage or transfer of processed hydrocarbons to tankers or pipelines. FPUs are essential for the efficient and safe production of oil and gas in challenging offshore environments."@en ,
                                           "Plataforma offshore usada na exploração e produção de petróleo e gás, projetada para extrair, processar e armazenar hidrocarbonetos. A Unidade de Produção Flutuante (FPU) é ancorada ou amarrada ao leito marinho e pode operar em águas profundas, frequentemente conectada a poços submarinos por meio de dutos flexíveis e umbilicais. Ela acomoda equipamentos de processamento para separação de petróleo, gás e água, bem como instalações para armazenamento temporário ou transferência de hidrocarbonetos processados para navios-tanque ou dutos. As FPUs são essenciais para a produção eficiente e segura de petróleo e gás em ambientes offshore desafiadores."@pt-br ;
                           skos:prefLabel "Floating Production Unit"@en ,
                                          "Unidade de Produção Flutuante (UEP)"@pt-br ;
                           edo:ifc_equivalentClass "IfcBuilding" ;
                           edo:ifc_objectType "FloatingProductionUnit" ;
                           edo:ifc_predefinedType "USERDEFINED" .


###  https://w3id.org/energy-domain/edo#FlowlineSpan
edo:FlowlineSpan rdf:type owl:Class ;
                 rdfs:subClassOf edo:PipelineSpan ;
                 dcterms:identifier "FlowlineSpan" .


###  https://w3id.org/energy-domain/edo#FractureToughness
edo:FractureToughness rdf:type owl:Class ;
                      rdfs:subClassOf edo:DomainAttribute ;
                      dcterms:accessRights "PUBLIC" ;
                      dcterms:identifier "FractureToughness" ;
                      skos:definition "Represents the material's ability to resist fracture when subjected to stress, particularly in the presence of flaws or cracks. This property is essential for assessing the material's capacity to withstand cracking or failure under load conditions."@en ,
                                      "Tenacidade à fratura (Específica para Materiais Metálicos)"@pt-br ;
                      skos:prefLabel "Fracture Toughness"@en ,
                                     "Tenacidade à Fratura"@pt-br ;
                      edo:hasTypedValue edo:floatValue ;
                      edo:hasValueCardinality edo:singleValue .


###  https://w3id.org/energy-domain/edo#FrictionCoefBetweenPipeAndTensioner
edo:FrictionCoefBetweenPipeAndTensioner rdf:type owl:Class ;
                                        rdfs:subClassOf edo:DomainAttribute ;
                                        dcterms:accessRights "PUBLIC" ;
                                        dcterms:identifier "FrictionCoefBetweenPipeAndTensioner" ;
                                        skos:definition "Coeficiente de atrito entre a sapata e a capa externa (passagem tensionador)"@pt-br ,
                                                        "Represents the coefficient of friction between the pipe and the tensioner during installation or operation. This property is critical for determining the resistance to sliding between the two surfaces, influencing the tension control and handling of the pipe."@en ;
                                        skos:prefLabel "Coeficiente de Atrito entre o Duto e o Tensionador"@pt-br ,
                                                       "Friction Coefficient Between Pipe And Tensioner"@en ;
                                        edo:hasTypedValue edo:floatValue ;
                                        edo:hasValueCardinality edo:singleValue .


###  https://w3id.org/energy-domain/edo#FrictionCoefficientTighteningTable
edo:FrictionCoefficientTighteningTable rdf:type owl:Class ;
                                       rdfs:subClassOf edo:DomainAttribute ;
                                       dcterms:accessRights "PUBLIC" ;
                                       dcterms:identifier "FrictionCoefficientTighteningTable" ;
                                       skos:definition "Esmagamento Coeficiente de atrito Aperto x Tabela CoF"@pt-br ,
                                                       "Provides data on the friction coefficients used during the tightening process, helping to assess the impact of friction on the applied torque and ensuring the correct tension is achieved in fasteners. This information is essential for maintaining mechanical integrity and preventing over- or under-tightening."@en ;
                                       skos:prefLabel "Friction Coefficient Tightening Table"@en ,
                                                      "Tabela de Coeficiente de Atrito x Aperto"@pt-br .


###  https://w3id.org/energy-domain/edo#FrictionCoefficientTighteningTable_CoefficientOfFriction
edo:FrictionCoefficientTighteningTable_CoefficientOfFriction rdf:type owl:Class ;
                                                             rdfs:subClassOf edo:DomainAttribute ;
                                                             dcterms:accessRights "PUBLIC" ;
                                                             dcterms:identifier "FrictionCoefficientTighteningTable_CoefficientOfFriction" ;
                                                             skos:definition "Represents the ratio that describes the force of friction between two surfaces in contact, relative to the normal force pressing them together. This property is important for evaluating the resistance to sliding or movement, ensuring proper performance of components under operational conditions."@en ;
                                                             skos:prefLabel "Coefficient Of Friction"@en ,
                                                                            "Coeficiente de Atrito"@pt-br ;
                                                             edo:hasTypedValue edo:floatValue ;
                                                             edo:hasValueCardinality edo:multiValue .


###  https://w3id.org/energy-domain/edo#FrictionCoefficientTighteningTable_TighteningPerTrack
edo:FrictionCoefficientTighteningTable_TighteningPerTrack rdf:type owl:Class ;
                                                          rdfs:subClassOf edo:DomainAttribute ;
                                                          dcterms:accessRights "PUBLIC" ;
                                                          dcterms:identifier "FrictionCoefficientTighteningTable_TighteningPerTrack" ;
                                                          skos:definition "Indicates the amount of tightening applied per track during an operation. This property is important for ensuring consistent force distribution across multiple tracks, helping to maintain proper alignment and secure attachment during the tightening process."@en ;
                                                          skos:prefLabel "Aperto por lagarta"@pt-br ,
                                                                         "Tightening Per Track"@en ;
                                                          edo:hasTypedValue edo:floatValue ;
                                                          edo:hasValueCardinality edo:multiValue .


###  https://w3id.org/energy-domain/edo#FullyThreaded
edo:FullyThreaded rdf:type owl:Class ;
                  rdfs:subClassOf edo:DomainAttribute ;
                  dcterms:accessRights "PUBLIC" ;
                  dcterms:identifier "FullyThreaded" ;
                  skos:definition "Indicates whether the component will be used fully threaded (TRUE) or not (FALSE)."@en ;
                  skos:prefLabel "Completamente Rosqueado"@pt-br ,
                                 "Fully Threaded"@en ;
                  edo:hasTypedValue edo:booleanValue ;
                  edo:hasValueCardinality edo:singleValue .


###  https://w3id.org/energy-domain/edo#GalvanicMaterial
edo:GalvanicMaterial rdf:type owl:Class ;
                     rdfs:subClassOf edo:DomainAttribute ;
                     dcterms:accessRights "PUBLIC" ;
                     dcterms:identifier "GalvanicMaterial" ;
                     skos:definition "Refers to the material used in galvanic protection systems, which is typically a metal or alloy designed to corrode in place of the protected structure. This material is selected for its ability to act as a sacrificial anode in a galvanic cell, thereby preventing corrosion of the primary structure, such as a subsea flexible pipeline. The choice of galvanic material is critical for the long-term protection and integrity of the pipeline system."@en ;
                     skos:prefLabel "Galvanic Material"@en ,
                                    "Material Galvânico"@pt-br ;
                     edo:hasTypedValue edo:stringValue ;
                     edo:hasValueCardinality edo:singleValue .


###  https://w3id.org/energy-domain/edo#Geothermal
edo:Geothermal rdf:type owl:Class ;
               rdfs:subClassOf edo:Renewable ;
               rdfs:label "Energia Geotérmica"@pt-br ,
                          "Geothermal Energy"@en ;
               skos:definition "Energia derivada do calor armazenado abaixo da superfície da Terra."@pt-br ,
                               "Energy derived from heat stored beneath the Earth's surface."@en .


###  https://w3id.org/energy-domain/edo#GrooveDiameter
edo:GrooveDiameter rdf:type owl:Class ;
                   rdfs:subClassOf edo:DomainAttribute ;
                   dcterms:accessRights "PUBLIC" ;
                   dcterms:identifier "GrooveDiameter" ;
                   skos:definition "Specifies the diameter of the end fitting at the location where the groove is machined. This measurement is crucial for ensuring that the groove correctly accommodates the end fitting during installation on a vessel. The part diameter at the groove location ensures proper alignment and secure attachment of the end fitting to the installation equipment or support system."@en ;
                   skos:prefLabel "Diâmetro do Groove"@pt-br ,
                                  "Groove Diameter"@en ;
                   edo:hasTypedValue edo:floatValue ;
                   edo:hasValueCardinality edo:singleValue .


###  https://w3id.org/energy-domain/edo#GrooveHeight
edo:GrooveHeight rdf:type owl:Class ;
                 rdfs:subClassOf edo:DomainAttribute ;
                 dcterms:accessRights "PUBLIC" ;
                 dcterms:identifier "GrooveHeight" ;
                 skos:definition "Specifies the vertical dimension of the groove from its base to the top edge. This measurement is crucial for ensuring that the groove can accommodate the intended components or fittings properly, allowing for a secure and precise fit. The groove height helps to determine the correct depth and functionality of the groove in relation to the end fitting and the overall installation process."@en ;
                 skos:prefLabel "Altura do Groove"@pt-br ,
                                "Groove Height"@en ;
                 edo:hasTypedValue edo:floatValue ;
                 edo:hasValueCardinality edo:singleValue .


###  https://w3id.org/energy-domain/edo#GrooveMinimumSupportArea
edo:GrooveMinimumSupportArea rdf:type owl:Class ;
                             rdfs:subClassOf edo:DomainAttribute ;
                             dcterms:accessRights "PUBLIC" ;
                             dcterms:identifier "GrooveMinimumSupportArea" ;
                             skos:definition "Specifies the minimum required area of the support surface within the groove. This measurement is crucial for ensuring that the groove provides adequate support and stability for the components or fittings it interfaces with. A sufficient support area helps prevent misalignment and ensures that the components are securely held in place during operation and installation."@en ;
                             skos:prefLabel "Groove Minimum Support Area"@en ,
                                            "Área Mínima de Apoio no Groove"@pt-br ;
                             edo:hasTypedValue edo:floatValue ;
                             edo:hasValueCardinality edo:singleValue .


###  https://w3id.org/energy-domain/edo#GroovePoint
edo:GroovePoint rdf:type owl:Class ;
                rdfs:subClassOf edo:ModelLocationPoint ;
                dcterms:identifier "GroovePoint" ;
                skos:definition "Ponto na linha de centro do End Fitting para indicar a posição do Groove"@pt-br ,
                                "The Groove Point is a designated point on the center line of the End Fitting, used to indicate the exact position of a groove. The groove itself is a recessed area designed specifically to lock the End Fitting during onboard installation, ensuring that it remains securely in place during the process. The Groove Support Point provides a reference for locating the groove, facilitating the precise alignment and positioning required for a smooth installation."@en ;
                skos:prefLabel "Groove Point"@en ,
                               "Ponto de Groove"@pt-br ;
                edo:hasAttribute edo:GrooveDiameter ,
                                 edo:GrooveHeight ,
                                 edo:GrooveMinimumSupportArea ,
                                 edo:GrooveSupportSurfaceDiameter ,
                                 edo:GrooveSupportSurfaceFilletRadius ,
                                 edo:GrvCntrPntDstnceFrmTermFlange ,
                                 edo:SafeWorkingLoad ,
                                 edo:TechnicalNotes ,
                                 edo:TestProp ,
                                 edo:TestProp2 ;
                edo:ifc_equivalentClass "IfcDistributionPort" ;
                edo:ifc_objectType "GroovePoint" ;
                edo:ifc_predefinedType "USERDEFINED" .


###  https://w3id.org/energy-domain/edo#GrooveSupportSurfaceDiameter
edo:GrooveSupportSurfaceDiameter rdf:type owl:Class ;
                                 rdfs:subClassOf edo:DomainAttribute ;
                                 dcterms:accessRights "PUBLIC" ;
                                 dcterms:identifier "GrooveSupportSurfaceDiameter" ;
                                 skos:definition "Indicates the diameter of the support surface within the groove. This measurement is critical for ensuring that the groove provides sufficient contact area for the components it interfaces with, contributing to a stable and secure fit."@en ;
                                 skos:prefLabel "Diâmetro da superfície de apoio do acessório"@pt-br ,
                                                "Groove Support Surface Diameter"@en ;
                                 edo:hasTypedValue edo:floatValue ;
                                 edo:hasValueCardinality edo:singleValue .


###  https://w3id.org/energy-domain/edo#GrooveSupportSurfaceFilletRadius
edo:GrooveSupportSurfaceFilletRadius rdf:type owl:Class ;
                                     rdfs:subClassOf edo:DomainAttribute ;
                                     dcterms:accessRights "PUBLIC" ;
                                     dcterms:identifier "GrooveSupportSurfaceFilletRadius" ;
                                     skos:definition "Adoçamento (Superfície de apoio) do acessório"@pt-br ,
                                                     "Indicates the radius of the fillet on the support surface of the end fitting. This fillet is a rounded corner or edge designed to reduce stress concentrations and enhance the structural integrity of the connection. The radius measurement is crucial for ensuring that the end fitting aligns properly with other components and provides a smooth, stable interface."@en ;
                                     skos:prefLabel "Groove Support Surface Fillet Radius"@en ,
                                                    "Raio de Chanframento (Superfície de Apoio) do Acessório"@pt-br ;
                                     edo:hasTypedValue edo:floatValue ;
                                     edo:hasValueCardinality edo:singleValue .


###  https://w3id.org/energy-domain/edo#GrvCntrPntDstnceFrmTermFlange
edo:GrvCntrPntDstnceFrmTermFlange rdf:type owl:Class ;
                                  rdfs:subClassOf edo:DomainAttribute ;
                                  dcterms:accessRights "PUBLIC" ;
                                  dcterms:identifier "GrvCntrPntDstnceFrmTermFlange" ;
                                  skos:definition "Distance from the center of the groove to the outer edge of the termination flange, the flange where the other end fitting is connected. This measurement provides the position of the groove relative to the termination flange for precise identification of a specific groove within the end fitting"@en ,
                                                  "Distância do centro do groove até a borda externa do flange de terminação, o flange onde o outro end fitting é conectado. Esta medição fornece a posição do groove em relação ao flange para a identificação precisa de um groove específico dentro do end fitting."@pt-br ;
                                  skos:prefLabel "Distância do Ponto Central do Groove até o Flange de Terminação"@pt-br ,
                                                 "Groove Center Point Distance From Termination Flange"@en ;
                                  edo:hasTypedValue edo:floatValue ;
                                  edo:hasValueCardinality edo:singleValue .


###  https://w3id.org/energy-domain/edo#H2SVolumeConcentration
edo:H2SVolumeConcentration rdf:type owl:Class ;
                           rdfs:subClassOf edo:DomainAttribute ;
                           dcterms:accessRights "PUBLIC" ;
                           dcterms:identifier "H2SVolumeConcentration" ;
                           skos:definition "Represents the concentration of hydrogen sulfide (H2S) in the total volume of the gas mixture, expressed in parts per million by volume (ppmv). This value is crucial for assessing material compatibility and corrosion risks in subsea flexible pipelines, as H2S is highly corrosive and can significantly impact the integrity and lifespan of the pipeline. Accurate measurement of H2S concentration is essential for ensuring the safe and reliable operation of the pipeline in harsh environments."@en ;
                           skos:prefLabel "Concentração Volumétrica de Sulfeto de Hidrogênio (H2S)"@pt-br ,
                                          "Hydrogen Sulfide (H2S) Volume Concentration"@en ;
                           edo:hasTypedValue edo:floatValue ;
                           edo:hasValueCardinality edo:singleValue .


###  https://w3id.org/energy-domain/edo#HVACEngineering
edo:HVACEngineering rdf:type owl:Class ;
                    rdfs:subClassOf edo:TechnicalDiscipline ;
                    rdfs:label "Engenharia de HVAC"@pt-br ,
                               "HVAC Engineering"@en ;
                    skos:definition "Disciplina de engenharia focada em sistemas de aquecimento, ventilação e ar condicionado."@pt-br ,
                                    "Engineering discipline focused on heating, ventilation and air conditioning systems."@en .


###  https://w3id.org/energy-domain/edo#HandlingCollar
edo:HandlingCollar rdf:type owl:Class ;
                   rdfs:subClassOf edo:SplitCollar ;
                   dcterms:identifier "HandlingCollar" ;
                   skos:altLabel "Handling Clamp"@en ,
                                 "Installation Collar"@en ,
                                 "Lifting Collar"@en ,
                                 "Support Collar"@en ;
                   skos:definition "Device used in subsea operations to facilitate the safe handling, lifting, and maneuvering of flexible pipes or heavy components during installation or retrieval. Typically attached around the pipe or component, it provides secure lifting points for cranes or other lifting equipment. Designed to distribute the load evenly, it prevents damage to the pipe or equipment while ensuring efficient and controlled movements in subsea environments."@en ;
                   skos:prefLabel "Colar de Manuseio"@pt-br ,
                                  "Handling Collar"@en ;
                   edo:ifc_equivalentClass "IfcPipeFitting" ;
                   edo:ifc_objectType "HandlingCollar" ;
                   edo:ifc_predefinedType "USERDEFINED" .


###  https://w3id.org/energy-domain/edo#HangOffCollar
edo:HangOffCollar rdf:type owl:Class ;
                  rdfs:subClassOf edo:LineAncillary ;
                  dcterms:identifier "HangOffCollar" ;
                  skos:altLabel "Hang-Off Clamp"@en ,
                                "Hang-Off Device"@en ,
                                "Support Collar"@en ,
                                "Termination Collar"@en ;
                  skos:definition "Device used to secure and support flexible pipes or risers during installation, particularly when they are suspended from a platform or vessel. It provides a stable attachment point, distributing the load and preventing excessive movement or strain on the pipe. The Hang Off Collar is crucial for maintaining the integrity of the pipe while it is held in place before final connection or during temporary suspension in subsea operations."@en ;
                  skos:prefLabel "Hang Off Collar"@en ,
                                 "Sistema de Suspensão"@pt-br ;
                  edo:hasAttribute edo:CollarInternalDiameter ,
                                   edo:FlangeType ,
                                   edo:MaxDynamicLoad ,
                                   edo:SafeWorkingLoad ,
                                   edo:UpperItubeDiameter ;
                  edo:ifc_equivalentClass "IfcPipeFitting" ;
                  edo:ifc_objectType "HangOffCollar" ;
                  edo:ifc_predefinedType "USERDEFINED" .


###  https://w3id.org/energy-domain/edo#HardwareItem
edo:HardwareItem rdf:type owl:Class ;
              rdfs:subClassOf edo:Component ;
              dcterms:identifier "HardwareItem" ;
              skos:definition "Simple mechanical items such as pipe components, etc."@en ;
              skos:prefLabel "Hardware Item"@en ,
                             "Item de Hardware"@pt-br ;
               :hasAttribute :DisplacedVolume ,
                             :DrawingDimensionsTable ,
                             :DrawingDimensionsTable_DimensionDescription ,
                             :DrawingDimensionsTable_DimensionName ,
                             :DrawingDimensionsTable_DimensionUnit ,
                             :DrawingDimensionsTable_DimensionValue ,
                             :IdInUnifilarDiagram ,
                             :InternalVolume ,
                             :ManufacturerDefinedMaterialName ,
                             :Mass ,
                             :MaterialSupplierName ,
                             :PartNumber ,
                             :ProjectDrawingCode ,
                             :ProjectDrawingRevision ,
                             :SupplierProvidedMaterialName .


###  https://w3id.org/energy-domain/edo#HasFaceORing
edo:HasFaceORing rdf:type owl:Class ;
                 rdfs:subClassOf edo:DomainAttribute ;
                 dcterms:accessRights "PUBLIC" ;
                 dcterms:identifier "HasFaceORing" ;
                 skos:definition "Indicates whether the item has a face oring (TRUE) or not (FALSE)."@en ;
                 skos:prefLabel "Has Face ORing"@en ,
                                "Possui ORing na Face"@pt-br ;
                 edo:hasTypedValue edo:booleanValue ;
                 edo:hasValueCardinality edo:singleValue .


###  https://w3id.org/energy-domain/edo#HasModaSensor
edo:HasModaSensor rdf:type owl:Class ;
                  rdfs:subClassOf edo:DomainAttribute ;
                  dcterms:accessRights "PUBLIC" ;
                  dcterms:identifier "HasModaSensor" ;
                  skos:definition "Indicates whether the item includes a MODA sensor (TRUE) or Not (FALSE)."@en ;
                  skos:prefLabel "Has Moda Sensor"@en ,
                                 "Possui Sensor MODA"@pt-br ;
                  edo:hasTypedValue edo:booleanValue ;
                  edo:hasValueCardinality edo:singleValue .


###  https://w3id.org/energy-domain/edo#HasN2InjectionPort
edo:HasN2InjectionPort rdf:type owl:Class ;
                       rdfs:subClassOf edo:DomainAttribute ;
                       dcterms:accessRights "PUBLIC" ;
                       dcterms:identifier "HasN2InjectionPort" ;
                       skos:definition "Indicates whether the item includes a nitrogen (N2) injection port (TRUE) or Not (FALSE)."@en ;
                       skos:prefLabel "Has N2 Injection Port"@en ,
                                      "Possui Porta de Injeção de Nitrogênio"@pt-br ;
                       edo:hasTypedValue edo:booleanValue ;
                       edo:hasValueCardinality edo:singleValue .


###  https://w3id.org/energy-domain/edo#HasThermalInsulation
edo:HasThermalInsulation rdf:type owl:Class ;
                         rdfs:subClassOf edo:DomainAttribute ;
                         dcterms:accessRights "PUBLIC" ;
                         dcterms:identifier "HasThermalInsulation" ;
                         skos:prefLabel "Has Thermal Insulation"@en ,
                                        "Possui isolamento térmico"@pt-br ;
                         edo:hasTypedValue edo:booleanValue ;
                         edo:hasValueCardinality edo:singleValue .


###  https://w3id.org/energy-domain/edo#HighStrengthTape
edo:HighStrengthTape rdf:type owl:Class ;
                     rdfs:subClassOf edo:TapeLayer ;
                     dcterms:identifier "HighStrengthTape" ;
                     skos:definition "Material used in subsea flexible pipes, typically applied as a reinforcing layer to provide additional strength and resistance to external forces. High Strength Tape is designed to improve the tensile properties of the flexible pipe, enhancing its ability to withstand high internal pressures, tension, and dynamic loads in harsh subsea environments. It is typically made from advanced fibers or composite materials, ensuring durability and long-term performance in demanding conditions."@en ;
                     skos:prefLabel "Fita de Alta Resistência"@pt-br ,
                                    "High Strength Tape"@en ;
                     edo:ifc_equivalentClass "IfcPipeSegment" ;
                     edo:ifc_objectType "HighStrengthTape" ;
                     edo:ifc_predefinedType "USERDEFINED" .


###  https://w3id.org/energy-domain/edo#HoldingBandage
edo:HoldingBandage rdf:type owl:Class ;
                   rdfs:subClassOf edo:TapeLayer ;
                   dcterms:identifier "HoldingBandage" ;
                   skos:definition "Reinforcement layer used in subsea flexible pipes to secure and hold internal components in place during manufacturing and operation. The Holding Bandage helps maintain the alignment and stability of the various layers of the pipe, preventing displacement or movement under dynamic conditions. Typically made from high-strength, flexible materials, it contributes to the overall durability and structural integrity of the pipe, ensuring reliable performance in harsh subsea environments."@en ;
                   skos:prefLabel "Bandagem de Reforço"@pt-br ,
                                  "Holding Bandage"@en ;
                   edo:hasAttribute edo:ModulusOfElasticity ,
                                    edo:StressAtDesignPressure ,
                                    edo:TapesQuantity ;
                   edo:ifc_equivalentClass "IfcPipeSegment" ;
                   edo:ifc_objectType "HoldingBandage" ;
                   edo:ifc_predefinedType "USERDEFINED" .


###  https://w3id.org/energy-domain/edo#HydrogenEnergy
edo:HydrogenEnergy rdf:type owl:Class ;
                   rdfs:subClassOf edo:Domain ;
                   rdfs:label "Energia de Hidrogênio"@pt-br ,
                              "Hydrogen Energy"@en ;
                   skos:definition "Production, storage, and utilization of hydrogen as an energy carrier."@en ,
                                   "Produção, armazenamento e utilização de hidrogênio como vetor energético."@pt-br .


###  https://w3id.org/energy-domain/edo#Hydropower
edo:Hydropower rdf:type owl:Class ;
               rdfs:subClassOf edo:Renewable ;
               rdfs:label "Energia Hidrelétrica"@pt-br ,
                          "Hydropower"@en ;
               skos:definition "Energia gerada a partir da água em movimento, incluindo barragens e energia das marés."@pt-br ,
                               "Energy generated from moving water, including dams and tidal power."@en .


###  https://w3id.org/energy-domain/edo#HydrostaticCollapseAbsPressDry
edo:HydrostaticCollapseAbsPressDry rdf:type owl:Class ;
                                   rdfs:subClassOf edo:DomainAttribute ;
                                   dcterms:accessRights "PUBLIC" ;
                                   dcterms:identifier "HydrostaticCollapseAbsPressDry" ;
                                   skos:definition "Pressão Absoluta de colapso hidrostático, anular seco, linha reta"@pt-br ,
                                                   "Represents the absolute pressure at which a component or material will collapse under hydrostatic forces when in a dry state. This property is important for evaluating the material's ability to withstand external pressure without deformation or failure."@en ;
                                   skos:prefLabel "Hydrostatic Collapse Absolute Pressure Dry"@en ,
                                                  "Pressão Absoluta de Colapso Hidrostático a Seco"@pt-br ;
                                   edo:hasTypedValue edo:floatValue ;
                                   edo:hasValueCardinality edo:singleValue .


###  https://w3id.org/energy-domain/edo#ITube
edo:ITube rdf:type owl:Class ;
          rdfs:subClassOf edo:RiserSupport ;
          dcterms:identifier "ITube" .


###  https://w3id.org/energy-domain/edo#IdInUnifilarDiagram
edo:IdInUnifilarDiagram rdf:type owl:Class ;
                        rdfs:subClassOf edo:DomainAttribute ;
                        dcterms:accessRights "PUBLIC" ;
                        dcterms:identifier "IdInUnifilarDiagram" ;
                        skos:definition "Identificador do item no diagrama unifilar (unifilar \"classico\", pre-existente) conforme a coluna \"item\" do unifilar."@pt-br ,
                                        "Numeric identifier used to represent the component in a unifilar diagram, ensuring clear reference and traceability within the diagram. This identifier allows for easy identification of the component's position and connection points in the simplified representation of the system."@en ;
                        skos:prefLabel "Id In Unifilar Diagram"@en ,
                                       "Identificador no Diagrama Unifilar"@pt-br ;
                        edo:hasTypedValue edo:intValue ;
                        edo:hasValueCardinality edo:singleValue .


###  https://w3id.org/energy-domain/edo#IndividualAnodeMass
edo:IndividualAnodeMass rdf:type owl:Class ;
                        rdfs:subClassOf edo:DomainAttribute ;
                        dcterms:accessRights "PUBLIC" ;
                        dcterms:identifier "IndividualAnodeMass" ;
                        skos:definition "Total mass of the sacrificial anode material within each individual anode."@en ;
                        skos:prefLabel "Individual Anode Mass"@en ,
                                       "Massa Individual do Anodo"@pt-br ;
                        edo:hasTypedValue edo:floatValue ;
                        edo:hasValueCardinality edo:singleValue .


###  https://w3id.org/energy-domain/edo#InnerTube
edo:InnerTube rdf:type owl:Class ;
              rdfs:subClassOf edo:SolidLayer ;
              dcterms:identifier "InnerTube" ;
              skos:definition "The Inner Tube is the innermost layer of a subsea flexible pipe, responsible for containing and transporting the fluid, such as oil or gas. It is designed to withstand internal pressures and prevent fluid leakage while offering resistance to the corrosive and abrasive nature of the transported substances. The Inner Tube is typically made from high-performance polymeric materials that ensure durability, flexibility, and chemical resistance, making it a critical component in maintaining the integrity of the flexible pipe in subsea operations."@en ;
              skos:prefLabel "Inner Tube"@en ,
                             "Tubo Interno"@pt-br ;
              edo:ifc_equivalentClass "IfcPipeSegment" ;
              edo:ifc_objectType "InnerTube" ;
              edo:ifc_predefinedType "USERDEFINED" .


###  https://w3id.org/energy-domain/edo#InsideTemperature
edo:InsideTemperature rdf:type owl:Class ;
                      rdfs:subClassOf edo:DomainAttribute ;
                      dcterms:accessRights "PUBLIC" ;
                      dcterms:identifier "InsideTemperature" ;
                      skos:definition "Represents the internal temperature within a component or system. This property is important for assessing the thermal conditions inside the system, ensuring that it operates within safe temperature limits, particularly in subsea environments where temperature control is essential for maintaining performance and integrity."@en ;
                      skos:prefLabel "Inside Temperature"@en ,
                                     "Temperatura Interna"@pt-br ;
                      edo:hasTypedValue edo:floatValue ;
                      edo:hasValueCardinality edo:singleValue .


###  https://w3id.org/energy-domain/edo#Installation
edo:Installation rdf:type owl:Class ;
                 rdfs:subClassOf edo:LifecyclePhase ;
                 rdfs:label "Instalação"@pt-br ,
                            "Installation"@en ;
                 skos:definition "Placement and integration of equipment, piping, and structures at the site."@en ,
                                 "Posicionamento e integração de equipamentos, tubulações e estruturas no local."@pt-br .


###  https://w3id.org/energy-domain/edo#InstrumentationEngineering
edo:InstrumentationEngineering rdf:type owl:Class ;
                               rdfs:subClassOf edo:TechnicalDiscipline ;
                               rdfs:label "Engenharia de Instrumentação"@pt-br ,
                                          "Instrumentation Engineering"@en ;
                               skos:definition "Disciplina de engenharia focada em sistemas de instrumentação de medição e controle."@pt-br ,
                                               "Engineering discipline focused on measurement and control instrumentation systems."@en .


###  https://w3id.org/energy-domain/edo#InsulationTape
edo:InsulationTape rdf:type owl:Class ;
                   rdfs:subClassOf edo:TapeLayer ;
                   dcterms:identifier "InsulationTape" ;
                   skos:definition "Material used in subsea flexible pipes to provide thermal insulation, ensuring that the temperature of the transported fluids remains stable during flow. Insulation Tape is applied in layers around the pipe to minimize heat loss or gain, which is critical for maintaining the fluid's properties, such as viscosity, in deepwater environments. It is typically made from materials with low thermal conductivity, such as polymers or composites, and is essential for enhancing the efficiency and performance of subsea pipelines in harsh temperature conditions."@en ;
                   skos:prefLabel "Fita de Isolamento"@pt-br ,
                                  "Insulation Tape"@en ;
                   edo:ifc_equivalentClass "IfcPipeSegment" ;
                   edo:ifc_objectType "InsulationTape" ;
                   edo:ifc_predefinedType "USERDEFINED" .


###  https://w3id.org/energy-domain/edo#Interconnection
edo:Interconnection rdf:type owl:Class ;
                    rdfs:subClassOf edo:LinearLocation ;
                    dcterms:identifier "Interconnection" ;
                    skos:definition "Location that contains the entire length of an interconnection, with its various sections, terminations, inline equipment, etc."@en ;
                    skos:prefLabel "Interconnection"@en ,
                                   "Interligação"@pt-br .


###  https://w3id.org/energy-domain/edo#InterlockedCarcass
edo:InterlockedCarcass rdf:type owl:Class ;
                       rdfs:subClassOf edo:CarcassLayer ;
                       dcterms:identifier "InterlockedCarcass" ;
                       skos:definition "The Interlocked Carcass is a metallic layer used in certain subsea flexible pipes to provide internal pressure resistance and prevent collapse. It is designed with interlocking metal strips that offer high strength while maintaining flexibility. This layer enhances the structural integrity of the flexible pipe, protecting it from external pressures and harsh subsea conditions. The Interlocked Carcass allows the pipe to bend without losing its shape or collapsing under deepwater pressure."@en ;
                       skos:prefLabel "Carcaça"@pt-br ,
                                      "Interlocked Carcass"@en ;
                       edo:ifc_equivalentClass "IfcPipeSegment" ;
                       edo:ifc_objectType "InterlockedCarcass" ;
                       edo:ifc_predefinedType "USERDEFINED" .


###  https://w3id.org/energy-domain/edo#IntermediateBendStiffener
edo:IntermediateBendStiffener rdf:type owl:Class ;
                              rdfs:subClassOf edo:BendStiffener ;
                              dcterms:identifier "IntermediateBendStiffener" ;
                              skos:altLabel "Curvature Stiffener"@en ,
                                            "Intermediate Bending Stiffener"@en ,
                                            "Stiffener"@en ;
                              skos:definition "A device used in subsea flexible pipes to provide localized stiffness at specific points along the length of the pipe, preventing excessive bending and reducing stress concentration. The Intermediate Bend Stiffener is typically installed between critical areas to ensure that the pipe maintains a controlled bending radius, protecting it from over-flexing or fatigue. Made from durable materials, it helps prolong the service life of the flexible pipe by distributing loads more evenly and reducing the risk of damage in dynamic subsea environments."@en ,
                                              "Dispositivo usado em tubos flexíveis submarinos para fornecer rigidez localizada em pontos específicos ao longo do comprimento do tubo, evitando dobras excessivas e reduzindo a concentração de tensões. O Enrijecedor de Curvatura Intermediário é tipicamente instalado entre áreas críticas para garantir que o tubo mantenha um raio de curvatura controlado, protegendo-o contra flexões excessivas ou fadiga. Feito de materiais duráveis, ajuda a prolongar a vida útil do tubo flexível, distribuindo as cargas de forma mais uniforme e reduzindo o risco de danos em ambientes submarinos dinâmicos."@pt-br ;
                              skos:prefLabel "Enrijecedor de Curvatura Intermediário"@pt-br ,
                                             "Intermediate Bend Stiffener"@en ;
                              edo:ifc_equivalentClass "IfcPipeFitting" ;
                              edo:ifc_objectType "IntermediateBendStiffener" .


###  https://w3id.org/energy-domain/edo#IntermediateSheath
edo:IntermediateSheath rdf:type owl:Class ;
                       rdfs:subClassOf edo:SolidLayer ;
                       dcterms:identifier "IntermediateSheath" ;
                       skos:definition "A protective layer within a subsea flexible pipe, positioned between other structural layers to provide additional protection and separation. The Intermediate Sheath serves to isolate different layers, preventing abrasion, wear, or interaction that could compromise the integrity of the pipe. Typically made from polymeric materials, this sheath also contributes to the overall durability and flexibility of the pipe, ensuring it can withstand the dynamic conditions of subsea environments while maintaining the performance of the internal and external layers."@en ;
                       skos:prefLabel "Barreira Intermediária de Vedação"@pt-br ,
                                      "Intermediate Sheath"@en ;
                       edo:ifc_equivalentClass "IfcPipeSegment" ;
                       edo:ifc_objectType "IntermediateSheath" ;
                       edo:ifc_predefinedType "USERDEFINED" .


###  https://w3id.org/energy-domain/edo#IntermediateValuesStrategy
edo:IntermediateValuesStrategy rdf:type owl:Class ;
                               rdfs:subClassOf edo:DomainAttribute ;
                               dcterms:accessRights "PUBLIC" ;
                               dcterms:identifier "IntermediateValuesStrategy" ;
                               skos:definition "Defines the approach used to handle or calculate intermediate values between specified data points. This property is important for ensuring accuracy in analysis or simulations, particularly when determining values that fall between measured or specified conditions."@en ;
                               skos:prefLabel "Estratégia para Valores Intermediários"@pt-br ,
                                              "Intermediate Values Strategy"@en ;
                               edo:hasTypedValue edo:stringValue ;
                               edo:hasValueCardinality edo:singleValue .


###  https://w3id.org/energy-domain/edo#InternalDiameter
edo:InternalDiameter rdf:type owl:Class ;
                     rdfs:subClassOf edo:DomainAttribute ;
                     dcterms:accessRights "PUBLIC" ;
                     dcterms:identifier "InternalDiameter" ;
                     skos:definition "Distance measured across the innermost points, passing through the center."@en ;
                     skos:prefLabel "Diâmetro interno"@pt-br ,
                                    "Internal Diameter"@en ;
                     edo:hasTypedValue edo:floatValue ;
                     edo:hasValueCardinality edo:singleValue .


###  https://w3id.org/energy-domain/edo#InternalIncidentalPressureTable
edo:InternalIncidentalPressureTable rdf:type owl:Class ;
                                    rdfs:subClassOf edo:DomainAttribute ;
                                    dcterms:accessRights "PUBLIC" ;
                                    dcterms:identifier "InternalIncidentalPressureTable" ;
                                    skos:definition "Provides data on internal incidental pressures, which are temporary or unexpected pressure spikes within the structure. This information is crucial for understanding the pressure limits the structure may face and ensuring it can withstand short-term variations without compromising its integrity."@en ;
                                    skos:prefLabel "Internal Incidental Pressure Table"@en ,
                                                   "Tabela de Pressão Incidental Interna"@pt-br .


###  https://w3id.org/energy-domain/edo#InternalIncidentalPressureTable_PositionReference
edo:InternalIncidentalPressureTable_PositionReference rdf:type owl:Class ;
                                                      rdfs:subClassOf edo:DomainAttribute ;
                                                      dcterms:accessRights "PUBLIC" ;
                                                      dcterms:identifier "InternalIncidentalPressureTable_PositionReference" ;
                                                      skos:definition "Identifies the specific point along the pipeline. This serves as the reference for vertical position and pressure values."@en ,
                                                                      "Valores válidos:Top (Para a conexão topside - E.g. Conector superior)TDPSubSeaConnection (Ex. ANM)"@pt-br ;
                                                      skos:prefLabel "Position Reference"@en ,
                                                                     "Referência de Posição"@pt-br ;
                                                      edo:hasTypedValue edo:stringValue ;
                                                      edo:hasValueCardinality edo:multiValue .


###  https://w3id.org/energy-domain/edo#InternalIncidentalPressureTable_Pressure
edo:InternalIncidentalPressureTable_Pressure rdf:type owl:Class ;
                                             rdfs:subClassOf edo:DomainAttribute ;
                                             dcterms:accessRights "PUBLIC" ;
                                             dcterms:identifier "InternalIncidentalPressureTable_Pressure" ;
                                             skos:definition "Indicates the force exerted per unit area on the surface of a material or component. This property is critical for evaluating how the component responds to external or internal forces, ensuring it can withstand operational pressure conditions."@en ;
                                             skos:prefLabel "Pressure"@en ,
                                                            "Pressão"@pt-br ;
                                             edo:hasTypedValue edo:floatValue ;
                                             edo:hasValueCardinality edo:multiValue .


###  https://w3id.org/energy-domain/edo#InternalIncidentalPressureTable_VPosWRTWaterline
edo:InternalIncidentalPressureTable_VPosWRTWaterline rdf:type owl:Class ;
                                                     rdfs:subClassOf edo:DomainAttribute ;
                                                     dcterms:accessRights "PUBLIC" ;
                                                     dcterms:identifier "InternalIncidentalPressureTable_VPosWRTWaterline" ;
                                                     skos:definition "Valores negativos para pontos submersos, e valores positivos para pontos acima da água. Considerando calado máximo da plataforma, quando aplicável."@pt-br ,
                                                                     "Vertical position with respect to the waterline, where positive values indicate points above the water and negative values indicate points below. The platform's maximum draft is considered when applicable."@en ;
                                                     skos:prefLabel "Posição Vertical em Relação à Linha D'Água"@pt-br ,
                                                                    "Vertical Position With Respect To Waterline"@en ;
                                                     edo:hasTypedValue edo:intValue ;
                                                     edo:hasValueCardinality edo:multiValue .


###  https://w3id.org/energy-domain/edo#InternalPressureSheath
edo:InternalPressureSheath rdf:type owl:Class ;
                           rdfs:subClassOf edo:SolidLayer ;
                           dcterms:identifier "InternalPressureSheath" ;
                           skos:definition "A layer within a subsea flexible pipe designed to contain the internal fluid and withstand the internal pressure exerted by the transported medium, such as oil, gas, or water. The Internal Pressure Sheath plays a crucial role in preventing fluid leakage and maintaining pressure integrity within the pipe. Typically made from high-performance polymeric materials, it ensures the safe transport of fluids under high-pressure conditions, contributing to the pipe's overall structural stability and long-term reliability in harsh subsea environments."@en ;
                           skos:prefLabel "Barreira Interna de Pressão"@pt-br ,
                                          "Internal Pressure Sheath"@en ;
                           edo:ifc_equivalentClass "IfcPipeSegment" ;
                           edo:ifc_objectType "InternalPressureSheath" ;
                           edo:ifc_predefinedType "USERDEFINED" .


###  https://w3id.org/energy-domain/edo#InternalVolume
edo:InternalVolume rdf:type owl:Class ;
                   rdfs:subClassOf edo:DomainAttribute ;
                   dcterms:accessRights "PUBLIC" ;
                   dcterms:identifier "InternalVolume" ;
                   skos:definition "Refers to the volume of space within an object that can be occupied by a fluid when the object is fully filled or immersed. This property is essential for understanding the capacity and fluid-holding capabilities of the accessory."@en ;
                   skos:prefLabel "Internal Volume"@en ,
                                  "Volume interno"@pt-br ;
                   edo:hasTypedValue edo:floatValue ;
                   edo:hasValueCardinality edo:singleValue .


###  https://w3id.org/energy-domain/edo#IsSpare
edo:IsSpare rdf:type owl:Class ;
            rdfs:subClassOf edo:DomainAttribute ;
            dcterms:accessRights "PUBLIC" ;
            dcterms:identifier "IsSpare" ;
            skos:definition "Indicates whether the item is spare (TRUE) or not (FALSE)."@en ;
            skos:prefLabel "Is Spare"@en ,
                           "É um sobressalente"@pt-br ;
            edo:hasTypedValue edo:booleanValue ;
            edo:hasValueCardinality edo:singleValue .


###  https://w3id.org/energy-domain/edo#LayerAnnular
edo:LayerAnnular rdf:type owl:Class ;
                 rdfs:subClassOf edo:DomainAttribute ;
                 dcterms:accessRights "PUBLIC" ;
                 dcterms:identifier "LayerAnnular" ;
                 skos:definition "Indicates whether the layer is part of the annular structure of the tensile armours. If true, it confirms that the layer contributes to the annular arrangement, which is important for understanding its role in the structural integrity and load distribution."@en ,
                                 "True se a camada faz parte do anular das armaduras de tração"@pt-br ;
                 skos:prefLabel "Camada Anular"@pt-br ,
                                "Layer Annular"@en ;
                 edo:hasTypedValue edo:booleanValue ;
                 edo:hasValueCardinality edo:singleValue .


###  https://w3id.org/energy-domain/edo#LayerAnnularType
edo:LayerAnnularType rdf:type owl:Class ;
                     rdfs:subClassOf edo:DomainAttribute ;
                     dcterms:accessRights "PUBLIC" ;
                     dcterms:identifier "LayerAnnularType" ;
                     skos:definition "Specifies the type of annular layer based on the condition it is designed for. This information is crucial for understanding the intended role of the layer in the overall structural configuration and how it is expected to perform under the projected operational conditions."@en ,
                                     "Tipo de anular conforme o estado do anular: Não pertence ao anular; Anular nunca alagado; Anular sempre alagado; Anular possivelmente alagado"@pt-br ;
                     skos:prefLabel "Layer Annular Type"@en ,
                                    "Tipo de Anular"@pt-br ;
                     edo:hasTypedValue edo:stringValue ;
                     edo:hasValueCardinality edo:singleValue .


###  https://w3id.org/energy-domain/edo#LayerContinuity
edo:LayerContinuity rdf:type owl:Class ;
                    rdfs:subClassOf edo:DomainAttribute ;
                    dcterms:accessRights "PUBLIC" ;
                    dcterms:identifier "LayerContinuity" ;
                    skos:definition "Indicates whether the layer is continuous, such as when it is extruded. If true, it confirms that the layer has no interruptions or joints, which is important for ensuring uniformity and strength in the structure."@en ,
                                    "True se a camada é contínua (extrudada)"@pt-br ;
                    skos:prefLabel "Continuidade da Camada"@pt-br ,
                                   "Layer Continuity"@en ;
                    edo:hasTypedValue edo:booleanValue ;
                    edo:hasValueCardinality edo:singleValue .


###  https://w3id.org/energy-domain/edo#LayerGeometryCrossSection
edo:LayerGeometryCrossSection rdf:type owl:Class ;
                              rdfs:subClassOf edo:DomainAttribute ;
                              dcterms:accessRights "PUBLIC" ;
                              dcterms:identifier "LayerGeometryCrossSection" ;
                              skos:definition "Indicates the geometry of the layer's cross-section. This property provides detailed information about the shape and dimensions of the layer when viewed in cross-section, which is important for understanding how the layer contributes to the overall structure's performance and integrity."@en ;
                              skos:prefLabel "Layer Geometry Cross Section"@en ,
                                             "Seção Transversal da Geometria da Camada"@pt-br ;
                              edo:hasTypedValue edo:floatValue ;
                              edo:hasValueCardinality edo:singleValue .


###  https://w3id.org/energy-domain/edo#LayerGeometryInertiaX
edo:LayerGeometryInertiaX rdf:type owl:Class ;
                          rdfs:subClassOf edo:DomainAttribute ;
                          dcterms:accessRights "PUBLIC" ;
                          dcterms:identifier "LayerGeometryInertiaX" ;
                          skos:definition "Indicates the moment of inertia of the layer's geometry around the X-axis. This property is crucial for understanding the layer's resistance to bending or deformation when subjected to forces along the X-axis, contributing to the structural stability and performance of the component."@en ;
                          skos:prefLabel "Inércia X da Geometria da Camada"@pt-br ,
                                         "Layer Geometry Inertia X"@en ;
                          edo:hasTypedValue edo:floatValue ;
                          edo:hasValueCardinality edo:singleValue .


###  https://w3id.org/energy-domain/edo#LayerGeometryInertiaY
edo:LayerGeometryInertiaY rdf:type owl:Class ;
                          rdfs:subClassOf edo:DomainAttribute ;
                          dcterms:accessRights "PUBLIC" ;
                          dcterms:identifier "LayerGeometryInertiaY" ;
                          skos:definition "Indicates the moment of inertia of the layer's geometry around the Y-axis. This property is important for evaluating the layer's resistance to bending or deformation when subjected to forces along the Y-axis, helping to ensure the structural stability and performance of the component."@en ;
                          skos:prefLabel "Inércia  Y da Geometria da Camada"@pt-br ,
                                         "Layer Geometry Inertia Y"@en ;
                          edo:hasTypedValue edo:floatValue ;
                          edo:hasValueCardinality edo:singleValue .


###  https://w3id.org/energy-domain/edo#LayerGeometryManufacturer
edo:LayerGeometryManufacturer rdf:type owl:Class ;
                              rdfs:subClassOf edo:DomainAttribute ;
                              dcterms:accessRights "PUBLIC" ;
                              dcterms:identifier "LayerGeometryManufacturer" ;
                              skos:definition "Indicates the manufacturer responsible for producing the layer's geometry. This property is important for tracking the origin and quality of the layer, providing key information about the source of the material or component used in the structure."@en ;
                              skos:prefLabel "Fabricante da Geometria da Camada"@pt-br ,
                                             "Layer Geometry Manufacturer"@en ;
                              edo:hasTypedValue edo:stringValue ;
                              edo:hasValueCardinality edo:singleValue .


###  https://w3id.org/energy-domain/edo#LayerGeometryName
edo:LayerGeometryName rdf:type owl:Class ;
                      rdfs:subClassOf edo:DomainAttribute ;
                      dcterms:accessRights "PUBLIC" ;
                      dcterms:identifier "LayerGeometryName" ;
                      skos:definition "Indicates the name assigned to the layer's geometry. This property is used to identify and distinguish the specific geometry of the layer, helping with organization, tracking, and reference within the overall structure or design."@en ;
                      skos:prefLabel "Layer Geometry Name"@en ,
                                     "Nome da Geometria da Camada"@pt-br ;
                      edo:hasTypedValue edo:stringValue ;
                      edo:hasValueCardinality edo:singleValue .


###  https://w3id.org/energy-domain/edo#LayerGeometryProfileThickness
edo:LayerGeometryProfileThickness rdf:type owl:Class ;
                                  rdfs:subClassOf edo:DomainAttribute ;
                                  dcterms:accessRights "PUBLIC" ;
                                  dcterms:identifier "LayerGeometryProfileThickness" ;
                                  skos:definition "Indicates the thickness of the layer's geometric profile. This property is important for understanding the contribution of the layer to the overall structure, particularly in terms of strength, flexibility, and resistance to external forces."@en ;
                                  skos:prefLabel "Espessura do Perfil da Geometria da Camada"@pt-br ,
                                                 "Layer Geometry Profile Thickness"@en ;
                                  edo:hasTypedValue edo:floatValue ;
                                  edo:hasValueCardinality edo:singleValue .


###  https://w3id.org/energy-domain/edo#LayerGeometryProfileWidth
edo:LayerGeometryProfileWidth rdf:type owl:Class ;
                              rdfs:subClassOf edo:DomainAttribute ;
                              dcterms:accessRights "PUBLIC" ;
                              dcterms:identifier "LayerGeometryProfileWidth" ;
                              skos:definition "Indicates the width of the layer's geometric profile. This property is important for understanding the dimensions of the layer, contributing to the overall structural design, and influencing factors such as load distribution and mechanical performance."@en ;
                              skos:prefLabel "Largura do Perfil da Geometria da Camada"@pt-br ,
                                             "Layer Geometry Profile Width"@en ;
                              edo:hasTypedValue edo:floatValue ;
                              edo:hasValueCardinality edo:singleValue .


###  https://w3id.org/energy-domain/edo#LayerGeometryThickness
edo:LayerGeometryThickness rdf:type owl:Class ;
                           rdfs:subClassOf edo:DomainAttribute ;
                           dcterms:accessRights "PUBLIC" ;
                           dcterms:identifier "LayerGeometryThickness" ;
                           skos:definition "Indicates the overall thickness of the layer's geometry. This property is critical for evaluating the structural contribution of the layer, including its strength, flexibility, and resistance to external forces."@en ;
                           skos:prefLabel "Espessura da Geometria da Camada"@pt-br ,
                                          "Layer Geometry Thickness"@en ;
                           edo:hasTypedValue edo:floatValue ;
                           edo:hasValueCardinality edo:singleValue .


###  https://w3id.org/energy-domain/edo#LayerThickness
edo:LayerThickness rdf:type owl:Class ;
                   rdfs:subClassOf edo:DomainAttribute ;
                   dcterms:accessRights "PUBLIC" ;
                   dcterms:identifier "LayerThickness" ;
                   skos:definition "Indicates the thickness of the layer, providing a key dimension that affects the overall strength, flexibility, and performance of the structure. This value is critical for ensuring that the layer meets design requirements and operational conditions."@en ;
                   skos:prefLabel "Espessura da camada"@pt-br ,
                                  "Layer Thickness"@en ;
                   edo:hasTypedValue edo:floatValue ;
                   edo:hasValueCardinality edo:singleValue .


###  https://w3id.org/energy-domain/edo#LayerWatertight
edo:LayerWatertight rdf:type owl:Class ;
                    rdfs:subClassOf edo:DomainAttribute ;
                    dcterms:accessRights "PUBLIC" ;
                    dcterms:identifier "LayerWatertight" ;
                    skos:definition "Indicates whether the layer is designed to be watertight. This property is critical for assessing the layer's ability to prevent water ingress, ensuring protection and maintaining the integrity of the structure in environments where exposure to water or fluids is expected."@en ;
                    skos:prefLabel "Camada Estanque"@pt-br ,
                                   "Layer Watertight"@en ;
                    edo:hasTypedValue edo:booleanValue ;
                    edo:hasValueCardinality edo:singleValue .


###  https://w3id.org/energy-domain/edo#LayerWatertightLowerLayerInternalFreeVolume
edo:LayerWatertightLowerLayerInternalFreeVolume rdf:type owl:Class ;
                                                rdfs:subClassOf edo:DomainAttribute ;
                                                dcterms:accessRights "PUBLIC" ;
                                                dcterms:identifier "LayerWatertightLowerLayerInternalFreeVolume" ;
                                                skos:definition "Indicates the free volume between this layer and the previous continuous or watertight lower layer. If this layer is not watertight, or if there is no previous watertight lower layer, the value should be indicated as zero. This property is important for assessing the space that may affect pressure distribution or fluid movement within the structure."@en ,
                                                                "Volume livre interno entre essa camada e a camada inferior estanque. Se essa camada não for estanque ou caso não tenha camada inferior estanque, indicar zero."@pt-br ;
                                                skos:prefLabel "Layer Watertight Lower Layer Internal Free Volume"@en ,
                                                               "Volume Livre Interno da Camada Inferior Estanque"@pt-br ;
                                                edo:hasTypedValue edo:floatValue ;
                                                edo:hasValueCardinality edo:singleValue .


###  https://w3id.org/energy-domain/edo#LayingMinimumRadiusTable
edo:LayingMinimumRadiusTable rdf:type owl:Class ;
                             rdfs:subClassOf edo:DomainAttribute ;
                             dcterms:accessRights "PUBLIC" ;
                             dcterms:identifier "LayingMinimumRadiusTable" ;
                             skos:definition "Provides data on the minimum allowable radius for laying operations, ensuring that the structure can be safely deployed without exceeding its bending limits. This information is crucial for preventing damage during installation and ensuring operational integrity."@en ;
                             skos:prefLabel "Laying Minimum Radius Table"@en ,
                                            "Tabela de raio mínimo de lançamento"@pt-br .


###  https://w3id.org/energy-domain/edo#LayingMinimumRadiusTable_AbsoluteExternalPressure
edo:LayingMinimumRadiusTable_AbsoluteExternalPressure rdf:type owl:Class ;
                                                      rdfs:subClassOf edo:DomainAttribute ;
                                                      dcterms:accessRights "PUBLIC" ;
                                                      dcterms:identifier "LayingMinimumRadiusTable_AbsoluteExternalPressure" ;
                                                      skos:definition "Represents the total pressure exerted on a component or system from the external environment, including both atmospheric and hydrostatic pressures. This property is critical for assessing the ability of the system to withstand the full pressure load, ensuring that it maintains structural integrity under extreme conditions."@en ;
                                                      skos:prefLabel "Absolute External Pressure"@en ,
                                                                     "Pressão Externa absoluta"@pt-br ;
                                                      edo:hasTypedValue edo:floatValue ;
                                                      edo:hasValueCardinality edo:multiValue .


###  https://w3id.org/energy-domain/edo#LayingMinimumRadiusTable_AbsoluteInternalPressure
edo:LayingMinimumRadiusTable_AbsoluteInternalPressure rdf:type owl:Class ;
                                                      rdfs:subClassOf edo:DomainAttribute ;
                                                      dcterms:accessRights "PUBLIC" ;
                                                      dcterms:identifier "LayingMinimumRadiusTable_AbsoluteInternalPressure" ;
                                                      skos:definition "Represents the total pressure exerted inside a component or system, accounting for both the atmospheric pressure and any additional internal pressure. This property is crucial for determining the system's ability to handle internal forces, ensuring safe operation under the expected pressure conditions."@en ;
                                                      skos:prefLabel "Absolute Internal Pressure"@en ,
                                                                     "Pressão interna absoluta"@pt-br ;
                                                      edo:hasTypedValue edo:floatValue ;
                                                      edo:hasValueCardinality edo:multiValue .


###  https://w3id.org/energy-domain/edo#LayingMinimumRadiusTable_Compression
edo:LayingMinimumRadiusTable_Compression rdf:type owl:Class ;
                                         rdfs:subClassOf edo:DomainAttribute ;
                                         dcterms:accessRights "PUBLIC" ;
                                         dcterms:identifier "LayingMinimumRadiusTable_Compression" ;
                                         skos:definition "Nota: Devem ser informados valores negativos. Por exemplo, para uma compressão de 10kN, deve ser informado -10."@pt-br ,
                                                         "Represents the force or stress applied to a material or component that causes it to decrease in size along a particular axis. This property is important for evaluating the material's ability to withstand compressive loads without failure."@en ;
                                         skos:prefLabel "Compression"@en ,
                                                        "Compressão"@pt-br ;
                                         edo:hasTypedValue edo:floatValue ;
                                         edo:hasValueCardinality edo:multiValue .


###  https://w3id.org/energy-domain/edo#LayingMinimumRadiusTable_MinimumAllowableBendingRadius
edo:LayingMinimumRadiusTable_MinimumAllowableBendingRadius rdf:type owl:Class ;
                                                           rdfs:subClassOf edo:DomainAttribute ;
                                                           dcterms:accessRights "PUBLIC" ;
                                                           dcterms:identifier "LayingMinimumRadiusTable_MinimumAllowableBendingRadius" ;
                                                           skos:definition "Represents the smallest radius to which a component, such as a pipe or cable, can be bent without causing damage or compromising its structural integrity. This property is essential for determining handling and installation limits to avoid deformation or failure."@en ;
                                                           skos:prefLabel "Minimum Allowable Bending Radius"@en ,
                                                                          "Raio Mínimo de Curvatura Permitido"@pt-br ;
                                                           edo:hasTypedValue edo:stringValue ;
                                                           edo:hasValueCardinality edo:multiValue .


###  https://w3id.org/energy-domain/edo#LayingMinimumRadiusTable_SectionSupportedByRigidSupport
edo:LayingMinimumRadiusTable_SectionSupportedByRigidSupport rdf:type owl:Class ;
                                                            rdfs:subClassOf edo:DomainAttribute ;
                                                            dcterms:accessRights "PUBLIC" ;
                                                            dcterms:identifier "LayingMinimumRadiusTable_SectionSupportedByRigidSupport" ;
                                                            skos:definition "Indicates whether the section is supported by a rigid support (TRUE) or not (FALSE)."@en ;
                                                            skos:prefLabel "Section Supported By Rigid Support"@en ,
                                                                           "Seção Suportada por um Suporte Rígido"@pt-br ;
                                                            edo:hasTypedValue edo:booleanValue ;
                                                            edo:hasValueCardinality edo:multiValue .


###  https://w3id.org/energy-domain/edo#LayingMinimumRadiusTable_TensileArmourAnnulusCondition
edo:LayingMinimumRadiusTable_TensileArmourAnnulusCondition rdf:type owl:Class ;
                                                           rdfs:subClassOf edo:DomainAttribute ;
                                                           dcterms:accessRights "PUBLIC" ;
                                                           dcterms:identifier "LayingMinimumRadiusTable_TensileArmourAnnulusCondition" ;
                                                           skos:definition "Condição do anular das armaduras de tração, Alagado ou Seco"@pt-br ,
                                                                           "Indicates the condition of the annulus in the tensile armour layer, which refers to the space between the tensile armour and other layers."@en ;
                                                           skos:prefLabel "Condição do Anular das Armaduras de Tração"@pt-br ,
                                                                          "Tensile Armour Annulus Condition"@en ;
                                                           edo:hasTypedValue edo:stringValue ;
                                                           edo:hasValueCardinality edo:multiValue .


###  https://w3id.org/energy-domain/edo#LifecyclePhase
edo:LifecyclePhase rdf:type owl:Class ;
                   rdfs:subClassOf edo:DomainClassification ;
                   rdfs:comment "Represents a stage in the lifecycle of an industrial asset."@en ;
                   rdfs:label "Fase do Ciclo de Vida"@pt-br ,
                              "Lifecycle Phase"@en ;
                   skos:definition "A stage in the lifecycle of an industrial asset, from conception to decommissioning."@en ,
                                   "Uma etapa no ciclo de vida de um ativo industrial, desde a concepção até a desativação."@pt-br .


###  https://w3id.org/energy-domain/edo#LimpTorsionalStiffnessAtSeaLevel
edo:LimpTorsionalStiffnessAtSeaLevel rdf:type owl:Class ;
                                     rdfs:subClassOf edo:DomainAttribute ;
                                     dcterms:accessRights "PUBLIC" ;
                                     dcterms:identifier "LimpTorsionalStiffnessAtSeaLevel" ;
                                     skos:definition "Indicates the torsional stiffness of the structure when in a limp or flexible state at sea level conditions. This value is important for assessing how the structure resists twisting forces while maintaining flexibility during operations at sea level."@en ,
                                                     "Rigidez a torção (GJ) (menor valor) a 20°C e pressão atmosferica (dentro e fora)"@pt-br ;
                                     skos:prefLabel "Limp Torsional Stiffness At Sea Level"@en ,
                                                    "Rigidez à Torção em Estado Flexível ao Nível do Mar"@pt-br ;
                                     edo:hasTypedValue edo:floatValue ;
                                     edo:hasValueCardinality edo:singleValue .


###  https://w3id.org/energy-domain/edo#LineAncillary
edo:LineAncillary rdf:type owl:Class ;
                  rdfs:subClassOf edo:HardwareItem ;
                  dcterms:identifier "LineAncillary" ;
                  skos:definition "A component designed to complement and enhance the functionality of subsea flexible pipes. Line Ancillaries include a variety of parts such as connectors, clamps, or collars that facilitate the installation, operation, and maintenance of flexible pipes used in subsea systems. These ancillaries ensure proper alignment, secure connections, and protection against environmental factors, contributing to the reliable performance and integrity of the flexible pipe system in harsh underwater conditions."@en ;
                  skos:prefLabel "Acessório de Linha"@pt-br ,
                                 "Line Ancillary"@en .


###  https://w3id.org/energy-domain/edo#LineSpan
edo:LineSpan rdf:type owl:Class ;
             rdfs:subClassOf edo:Location ;
             dcterms:identifier "LineSpan" .


###  https://w3id.org/energy-domain/edo#LineTermination
edo:LineTermination rdf:type owl:Class ;
                    rdfs:subClassOf edo:HardwareItem ;
                    dcterms:identifier "LineTermination" ;
                    skos:definition "The Line Termination includes components at the endpoints of flexible and rigid pipelines, as well as umbilical systems. These terminations provide secure connections to other equipment, enabling the transfer of fluids, gases, or control signals. Designed for stability and integrity, Line Termination components ensure durable and reliable performance across various pipeline types."@en ;
                    skos:prefLabel "Line Termination"@en ,
                                   "Terminador de Linha"@pt-br .


###  https://w3id.org/energy-domain/edo#LinearLocation
edo:LinearLocation rdf:type owl:Class ;
                   rdfs:subClassOf edo:Location ;
                   dcterms:identifier "LinearLocation" ;
                   skos:definition "Base for locations that extend along a geographically significant route."@en ;
                   skos:prefLabel "Linear Location"@en ,
                                  "Localização Linear"@pt-br .


###  https://w3id.org/energy-domain/edo#LinearMass
edo:LinearMass rdf:type owl:Class ;
               rdfs:subClassOf edo:DomainAttribute ;
               dcterms:accessRights "PUBLIC" ;
               dcterms:identifier "LinearMass" ;
               skos:definition "Indicates the mass per unit length, providing essential information for weight distribution and load calculations. This value is critical for evaluating how the structure will perform under various operational conditions, including installation and transport."@en ;
               skos:prefLabel "Linear Mass"@en ,
                              "Massa Linear"@pt-br ;
               edo:hasTypedValue edo:floatValue ;
               edo:hasValueCardinality edo:singleValue .


###  https://w3id.org/energy-domain/edo#LinearObject
edo:LinearObject rdf:type owl:Class ;
                 rdfs:subClassOf edo:Asset ;
                 dcterms:identifier "LinearObject" ;
                 skos:definition "Base for any type of interconnecting element with linear geometry."@en ;
                 skos:prefLabel "Linear Object"@en ,
                                "Objeto Linear"@pt-br .


###  https://w3id.org/energy-domain/edo#Location
edo:Location rdf:type owl:Class ;
             rdfs:subClassOf edo:DomainElement ;
             dcterms:identifier "Location" ;
             skos:definition "Basis for all model installation locations."@en ;
             skos:prefLabel "Localização"@pt-br ,
                            "Location"@en .


###  https://w3id.org/energy-domain/edo#LocationType
edo:LocationType rdf:type owl:Class ;
                 rdfs:subClassOf edo:DomainClassification ;
                 rdfs:label "Location Type"@en ,
                            "Tipo de Localização"@pt-br ;
                 skos:definition "Classification of industrial activities based on their geographical location."@en ,
                                 "Classificação de atividades industriais baseada em sua localização geográfica."@pt-br .


###  https://w3id.org/energy-domain/edo#LogicalConnection
edo:LogicalConnection rdf:type owl:Class ;
                      rdfs:subClassOf edo:Connection ;
                      dcterms:identifier "LogicalConnection" ;
                      skos:definition "Represents a logical/functional connection between two installation locations."@en ;
                      skos:prefLabel "Conexão Lógica"@pt-br ,
                                     "Logical Connection"@en .


###  https://w3id.org/energy-domain/edo#LongTermFloatDensity
edo:LongTermFloatDensity rdf:type owl:Class ;
                         rdfs:subClassOf edo:DomainAttribute ;
                         dcterms:accessRights "PUBLIC" ;
                         dcterms:identifier "LongTermFloatDensity" ;
                         skos:definition "A densidade do flutuador ao longo do tempo, considerando o acúmulo de água no material ou mudanças na estrutura interna devido à degradação. Isso aumenta a densidade e, portanto, reduz a flutuabilidade"@pt-br ,
                                         "The density of the float material over time, considering factors like water absorption and material degradation, which increase the density and reduce the buoyancy."@en ;
                         skos:prefLabel "Densidade do Flutuador a Longo Prazo"@pt-br ,
                                        "Long Term Float Density"@en ;
                         edo:hasTypedValue edo:floatValue ;
                         edo:hasValueCardinality edo:singleValue .


###  https://w3id.org/energy-domain/edo#LongTermFloatVolume
edo:LongTermFloatVolume rdf:type owl:Class ;
                        rdfs:subClassOf edo:DomainAttribute ;
                        dcterms:accessRights "PUBLIC" ;
                        dcterms:identifier "LongTermFloatVolume" ;
                        skos:definition "O volume esperado ao longo do tempo, após fatores como absorção de água e possíveis deformações. Este volume representa as condições do flutuador em sua fase de vida útil, quando a flutuabilidade tende a ser menor."@pt-br ,
                                        "The expected submerged volume of the float over time, taking into account factors like water absorption and structural deformations that may occur throughout its lifecycle."@en ;
                        skos:prefLabel "Long Term Float Volume"@en ,
                                       "Volume do Flutuador a Longo Prazo"@pt-br ;
                        edo:hasTypedValue edo:floatValue ;
                        edo:hasValueCardinality edo:singleValue .


###  https://w3id.org/energy-domain/edo#LowResistanceTape
edo:LowResistanceTape rdf:type owl:Class ;
                      rdfs:subClassOf edo:TapeLayer ;
                      dcterms:identifier "LowResistanceTape" ;
                      skos:definition "A layer used in subsea flexible pipes to reduce friction between different components or layers, enhancing the overall flexibility and durability of the pipe. The Low Resistance Tape minimizes wear and abrasion caused by the movement of adjacent layers during operation, particularly in dynamic subsea conditions. Made from materials with low friction properties, it helps extend the lifespan of the pipe by reducing internal stresses and preventing damage to critical layers, ensuring smooth and efficient operation under harsh underwater conditions."@en ;
                      skos:prefLabel "Fita de Baixa Resistência"@pt-br ,
                                     "Low Resistance Tape"@en ;
                      edo:ifc_equivalentClass "IfcPipeSegment" ;
                      edo:ifc_objectType "LowResistanceTape" ;
                      edo:ifc_predefinedType "USERDEFINED" .


###  https://w3id.org/energy-domain/edo#Lubricant
edo:Lubricant rdf:type owl:Class ;
              rdfs:subClassOf edo:DomainAttribute ;
              dcterms:accessRights "PUBLIC" ;
              dcterms:identifier "Lubricant" ;
              skos:definition "Specifies the type of lubricant applied to reduce friction during tightening and ensure consistent torque application. The use of the correct lubricant is critical in preventing galling and corrosion, and helps to maintain the long-term integrity."@en ;
              skos:prefLabel "Lubricant"@en ,
                             "Nome do Lubrificante"@pt-br ;
              edo:hasTypedValue edo:stringValue ;
              edo:hasValueCardinality edo:singleValue .


###  https://w3id.org/energy-domain/edo#LubricantFrictionFactor
edo:LubricantFrictionFactor rdf:type owl:Class ;
                            rdfs:subClassOf edo:DomainAttribute ;
                            dcterms:accessRights "PUBLIC" ;
                            dcterms:identifier "LubricantFrictionFactor" ;
                            skos:definition "Indicates the friction factor of the lubricant applied, which affects the torque required to achieve proper tightening. This value is crucial for ensuring that the correct amount of torque is applied, accounting for the reduction in friction caused by the lubricant."@en ;
                            skos:prefLabel "Fator de atrito do lubrificante"@pt-br ,
                                           "Lubricant Friction Factor"@en ;
                            edo:hasTypedValue edo:floatValue ;
                            edo:hasValueCardinality edo:singleValue .


###  https://w3id.org/energy-domain/edo#Maintenance
edo:Maintenance rdf:type owl:Class ;
                rdfs:subClassOf edo:LifecyclePhase ;
                rdfs:label "Maintenance"@en ,
                           "Manutenção"@pt-br ;
                skos:definition "Intervenções planejadas ou corretivas para preservar a funcionalidade e segurança do ativo."@pt-br ,
                                "Planned or corrective interventions to preserve asset functionality and safety."@en .


###  https://w3id.org/energy-domain/edo#ManufacturerDefinedMaterialName
edo:ManufacturerDefinedMaterialName rdf:type owl:Class ;
                                    rdfs:subClassOf edo:DomainAttribute ;
                                    dcterms:accessRights "PUBLIC" ;
                                    dcterms:identifier "ManufacturerDefinedMaterialName" ;
                                    skos:definition "Name of the material as designated by the manufacturer of the final item. This property identifies the specific material name used by the manufacturer, providing clarity on the material specifications for the finished accessory."@en ;
                                    skos:prefLabel "Manufacturer Defined Material Name"@en ,
                                                   "Nome do material conforme designado pelo fabricante do item final"@pt-br ;
                                    edo:hasTypedValue edo:stringValue ;
                                    edo:hasValueCardinality edo:multiValue .


###  https://w3id.org/energy-domain/edo#ManufacturingDate
edo:ManufacturingDate rdf:type owl:Class ;
                      rdfs:subClassOf edo:DomainAttribute ;
                      dcterms:accessRights "PUBLIC" ;
                      dcterms:identifier "ManufacturingDate" ;
                      skos:definition "Manufacturing date refers to the specific date when an object or product was produced or fabricated. This information is essential for tracking production batches, ensuring quality control, and determining the product’s shelf life or warranty period."@en ;
                      skos:prefLabel "Data de Fabricação"@pt-br ,
                                     "Manufacturing Date"@en ;
                      edo:hasTypedValue edo:stringValue ;
                      edo:hasValueCardinality edo:singleValue .


###  https://w3id.org/energy-domain/edo#ManufacturingNonConformities
edo:ManufacturingNonConformities rdf:type owl:Class ;
                                 rdfs:subClassOf edo:DomainAttribute ;
                                 dcterms:accessRights "PUBLIC" ;
                                 dcterms:identifier "ManufacturingNonConformities" ;
                                 skos:definition "Indicates whether the item has manufacturing non-conformities (TRUE) or not (FALSE)."@en ;
                                 skos:prefLabel "Manufacturing Non Conformities"@en ,
                                                "Não Conformidades de Fabricação"@pt-br ;
                                 edo:hasTypedValue edo:booleanValue ;
                                 edo:hasValueCardinality edo:singleValue .


###  https://w3id.org/energy-domain/edo#Mass
edo:Mass rdf:type owl:Class ;
         rdfs:subClassOf edo:DomainAttribute ;
         dcterms:accessRights "PUBLIC" ;
         dcterms:identifier "Mass" ;
         skos:definition "Amount of matter that makes up an object."@en ;
         skos:prefLabel "Mass"@en ,
                        "Massa"@pt-br ;
         edo:hasTypedValue edo:floatValue ;
         edo:hasValueCardinality edo:singleValue .


###  https://w3id.org/energy-domain/edo#MaterialComposition
edo:MaterialComposition rdf:type owl:Class ;
                        rdfs:subClassOf edo:DomainAttribute ;
                        dcterms:accessRights "PUBLIC" ;
                        dcterms:identifier "MaterialComposition" ;
                        skos:definition "Indicates the composition of the fabrication material used. This property provides details about the specific material, helping to assess its mechanical, thermal, and chemical properties. It is crucial for evaluating the material's suitability for various operational conditions and services."@en ,
                                        "Tipo do material."@pt-br ;
                        skos:prefLabel "Composição do Material"@pt-br ,
                                       "Material Composition"@en ;
                        edo:hasTypedValue edo:stringValue ;
                        edo:hasValueCardinality edo:singleValue .


###  https://w3id.org/energy-domain/edo#MaterialRequest
edo:MaterialRequest rdf:type owl:Class ;
                    rdfs:subClassOf edo:DomainAttribute ;
                    dcterms:accessRights "PUBLIC" ;
                    dcterms:identifier "MaterialRequest" ;
                    skos:definition "Code used to identify the document that specifies the materials required for the project, serving as the basis for generating the purchase order. It ensures accurate tracking and procurement of necessary items for project execution."@en ;
                    skos:prefLabel "Código da Requisição de Material (RM)"@pt-br ,
                                   "Material Request"@en ;
                    edo:hasTypedValue edo:stringValue ;
                    edo:hasValueCardinality edo:singleValue .


###  https://w3id.org/energy-domain/edo#MaterialRequestRev
edo:MaterialRequestRev rdf:type owl:Class ;
                       rdfs:subClassOf edo:DomainAttribute ;
                       dcterms:accessRights "PUBLIC" ;
                       dcterms:identifier "MaterialRequestRev" ;
                       skos:definition "Indicates the revision number of the Material Request document, ensuring that the most up-to-date version is referenced during procurement and project execution."@en ;
                       skos:prefLabel "Material Request Revision"@en ,
                                      "Revisão da Requisição de Material (RM)"@pt-br ;
                       edo:hasTypedValue edo:stringValue ;
                       edo:hasValueCardinality edo:singleValue .


###  https://w3id.org/energy-domain/edo#MaterialSupplierName
edo:MaterialSupplierName rdf:type owl:Class ;
                         rdfs:subClassOf edo:DomainAttribute ;
                         dcterms:accessRights "PUBLIC" ;
                         dcterms:identifier "MaterialSupplierName" ;
                         skos:definition "Name of the company responsible for supplying the material. This property identifies the supplier of the material used in the accessory, ensuring traceability and accountability."@en ;
                         skos:prefLabel "Material Supplier Name"@en ,
                                        "Nome da empresa responsável por fornecer o material"@pt-br ;
                         edo:hasTypedValue edo:stringValue ;
                         edo:hasValueCardinality edo:singleValue .


###  https://w3id.org/energy-domain/edo#MaxDesignAbsIntPresTable
edo:MaxDesignAbsIntPresTable rdf:type owl:Class ;
                             rdfs:subClassOf edo:DomainAttribute ;
                             dcterms:accessRights "PUBLIC" ;
                             dcterms:identifier "MaxDesignAbsIntPresTable" ;
                             skos:definition "Provides data on the maximum design absolute internal pressure, used to evaluate the highest internal pressure the structure is designed to withstand. This information is critical for ensuring the structure's integrity and safety under the most demanding operational conditions."@en ;
                             skos:prefLabel "Maximum Design Absolute Internal Pressure Table"@en ,
                                            "Tabela da Máxima Pressão Interna Absoluta de Projeto"@pt-br .


###  https://w3id.org/energy-domain/edo#MaxDesignAbsIntPresTable_PositionReference
edo:MaxDesignAbsIntPresTable_PositionReference rdf:type owl:Class ;
                                               rdfs:subClassOf edo:DomainAttribute ;
                                               dcterms:accessRights "PUBLIC" ;
                                               dcterms:identifier "MaxDesignAbsIntPresTable_PositionReference" ;
                                               skos:definition "Identifies the specific point along the pipeline, such as the topside connection, TDP (Touchdown Point), or subsea connection point. This serves as the reference for vertical position and pressure values."@en ,
                                                               "Ponto. Valores válidos:Top (Para a conexão topside - E.g. Conector superior)TDPSubSeaConnection (Ex. ANM)"@pt-br ;
                                               skos:prefLabel "Position Reference"@en ,
                                                              "Referência de Posição"@pt-br ;
                                               edo:hasTypedValue edo:stringValue ;
                                               edo:hasValueCardinality edo:multiValue .


###  https://w3id.org/energy-domain/edo#MaxDesignAbsIntPresTable_Pressure
edo:MaxDesignAbsIntPresTable_Pressure rdf:type owl:Class ;
                                      rdfs:subClassOf edo:DomainAttribute ;
                                      dcterms:accessRights "PUBLIC" ;
                                      dcterms:identifier "MaxDesignAbsIntPresTable_Pressure" ;
                                      skos:definition "Indicates the force exerted per unit area on the surface of a material or component. This property is critical for evaluating how the component responds to external or internal forces, ensuring it can withstand operational pressure conditions."@en ;
                                      skos:prefLabel "Maximum Design Absolute Internal Pressure"@en ,
                                                     "Máxima Pressão Interna Absoluta de Projeto"@pt-br ;
                                      edo:hasTypedValue edo:floatValue ;
                                      edo:hasValueCardinality edo:multiValue .


###  https://w3id.org/energy-domain/edo#MaxDesignAbsIntPresTable_VPosWRTWaterline
edo:MaxDesignAbsIntPresTable_VPosWRTWaterline rdf:type owl:Class ;
                                              rdfs:subClassOf edo:DomainAttribute ;
                                              dcterms:accessRights "PUBLIC" ;
                                              dcterms:identifier "MaxDesignAbsIntPresTable_VPosWRTWaterline" ;
                                              skos:definition "Valores negativos para pontos submersos, e valores positivos para pontos acima da água. Considerando calado máximo da plataforma, quando aplicável."@pt-br ,
                                                              "Vertical position with respect to the waterline, where positive values indicate points above the water and negative values indicate points below. The platform's maximum draft is considered when applicable."@en ;
                                              skos:prefLabel "Posição Vertical em Relação à Linha D'Água"@pt-br ,
                                                             "Vertical Position With Respect To Waterline"@en ;
                                              edo:hasTypedValue edo:intValue ;
                                              edo:hasValueCardinality edo:multiValue .


###  https://w3id.org/energy-domain/edo#MaxDesignPressure
edo:MaxDesignPressure rdf:type owl:Class ;
                      rdfs:subClassOf edo:DomainAttribute ;
                      dcterms:accessRights "PUBLIC" ;
                      dcterms:identifier "MaxDesignPressure" ;
                      skos:definition "The highest internal or external pressure that the component or system is designed to withstand under operational conditions, ensuring safety and reliability."@en ;
                      skos:prefLabel "Maximum Design Pressure"@en ,
                                     "Pressão Máxima de Projeto"@pt-br ;
                      edo:hasTypedValue edo:floatValue ;
                      edo:hasValueCardinality edo:singleValue .


###  https://w3id.org/energy-domain/edo#MaxDynamicLoad
edo:MaxDynamicLoad rdf:type owl:Class ;
                   rdfs:subClassOf edo:DomainAttribute ;
                   dcterms:accessRights "PUBLIC" ;
                   dcterms:identifier "MaxDynamicLoad" ;
                   skos:definition "Maximum Dynamic Load (MDL) that the component can endure during operation. This value indicates the highest load the component can support while experiencing varying forces or impacts. Understanding this limit is essential for ensuring the component’s safety, reliability, and structural integrity in dynamic environments."@en ;
                   skos:prefLabel "Carga Dinâmica Máxima (MDL)"@pt-br ,
                                  "Maximum Dynamic Load (MDL)"@en ;
                   edo:hasTypedValue edo:floatValue ;
                   edo:hasValueCardinality edo:singleValue .


###  https://w3id.org/energy-domain/edo#MaxLengthTolerance
edo:MaxLengthTolerance rdf:type owl:Class ;
                       rdfs:subClassOf edo:DomainAttribute ;
                       dcterms:accessRights "PUBLIC" ;
                       dcterms:identifier "MaxLengthTolerance" ;
                       skos:definition "Max length tolerance refers to the maximum allowable deviation from the specified or nominal length of an object. It defines the upper limit of acceptable variance during manufacturing or inspection, ensuring that the length stays within the defined range for quality control and compliance with design specifications."@en ;
                       skos:prefLabel "Maximum Length Tolerance"@en ,
                                      "Tolerância Máxima de Comprimento"@pt-br ;
                       edo:hasTypedValue edo:floatValue ;
                       edo:hasValueCardinality edo:singleValue .


###  https://w3id.org/energy-domain/edo#MaxPermissibleDeformationDynamic
edo:MaxPermissibleDeformationDynamic rdf:type owl:Class ;
                                     rdfs:subClassOf edo:DomainAttribute ;
                                     dcterms:accessRights "PUBLIC" ;
                                     dcterms:identifier "MaxPermissibleDeformationDynamic" ;
                                     skos:definition "Maximum deformation that the material can undergo under dynamic loading conditions is specified. This property is crucial for assessing how the material will behave when subjected to varying forces or impacts, ensuring it maintains functionality and structural integrity without excessive deformation or failure."@en ,
                                                     "Máxima Deformação Admissível (Aplicações Dinâmicas) (Específica para Materiais Poliméricos)"@pt-br ;
                                     skos:prefLabel "Maximum Permissible Deformation Dynamic"@en ,
                                                    "Máxima Deformação Admissível"@pt-br ;
                                     edo:hasTypedValue edo:floatValue ;
                                     edo:hasValueCardinality edo:singleValue .


###  https://w3id.org/energy-domain/edo#MaxPermissibleDeformationStatic
edo:MaxPermissibleDeformationStatic rdf:type owl:Class ;
                                    rdfs:subClassOf edo:DomainAttribute ;
                                    dcterms:accessRights "PUBLIC" ;
                                    dcterms:identifier "MaxPermissibleDeformationStatic" ;
                                    skos:definition "Indicates the maximum deformation the material can tolerate under static loading conditions. This property defines the extent to which the material can be deformed without failure or significant structural compromise when subjected to constant, non-varying forces or loads."@en ,
                                                    "Máxima Deformação Admissível (Aplicações Estáticas) (Específica para Materiais Poliméricos)"@pt-br ;
                                    skos:prefLabel "Maximum Permissible Deformation Static"@en ,
                                                   "Máxima Deformação Admissível em Aplicações Estáticas"@pt-br ;
                                    edo:hasTypedValue edo:floatValue ;
                                    edo:hasValueCardinality edo:singleValue .


###  https://w3id.org/energy-domain/edo#MaximumAllowableTensileForStraightLine
edo:MaximumAllowableTensileForStraightLine rdf:type owl:Class ;
                                           rdfs:subClassOf edo:DomainAttribute ;
                                           dcterms:accessRights "PUBLIC" ;
                                           dcterms:identifier "MaximumAllowableTensileForStraightLine" ;
                                           skos:definition "MaximumAllowableTensileForStraightLine refers to the highest tensile force that can be applied to the flexible pipe in a straight-line configuration without risking damage or compromising the structural integrity of the pipe. This property is critical during installation and operation, ensuring that the pipe can withstand axial loads without overstressing or damaging its internal layers, such as the tensile armour, while maintaining safe handling limits."@en ;
                                           skos:prefLabel "Maximum Allowable Tensile For Straight Line"@en ,
                                                          "Tração Máxima Permitida para Linha Reta"@pt-br ;
                                           edo:hasTypedValue edo:floatValue ;
                                           edo:hasValueCardinality edo:singleValue .


###  https://w3id.org/energy-domain/edo#MaximumAllowableTensionTable
edo:MaximumAllowableTensionTable rdf:type owl:Class ;
                                 rdfs:subClassOf edo:DomainAttribute ;
                                 dcterms:accessRights "PUBLIC" ;
                                 dcterms:identifier "MaximumAllowableTensionTable" ;
                                 skos:definition "Provides data on the maximum allowable tension that the structure can withstand under various conditions. This information is critical for ensuring the structure's safe operation, preventing overstressing, and maintaining structural integrity during use."@en ;
                                 skos:prefLabel "Maximum Allowable Tension Table"@en ,
                                                "Tabela de Tensão Máxima Admissível"@pt-br .


###  https://w3id.org/energy-domain/edo#MaximumAllowableTensionTable_MaximumAllowableTensile
edo:MaximumAllowableTensionTable_MaximumAllowableTensile rdf:type owl:Class ;
                                                         rdfs:subClassOf edo:DomainAttribute ;
                                                         dcterms:accessRights "PUBLIC" ;
                                                         dcterms:identifier "MaximumAllowableTensionTable_MaximumAllowableTensile" ;
                                                         skos:definition "Indicates the highest tensile force a component can safely withstand without compromising its integrity."@en ;
                                                         skos:prefLabel "Maximum Allowable Tensile"@en ,
                                                                        "Tração Máxima Permitida"@pt-br ;
                                                         edo:hasTypedValue edo:floatValue ;
                                                         edo:hasValueCardinality edo:multiValue .


###  https://w3id.org/energy-domain/edo#MaximumAllowableTensionTable_PulleyRadius
edo:MaximumAllowableTensionTable_PulleyRadius rdf:type owl:Class ;
                                              rdfs:subClassOf edo:DomainAttribute ;
                                              dcterms:accessRights "PUBLIC" ;
                                              dcterms:identifier "MaximumAllowableTensionTable_PulleyRadius" ;
                                              skos:definition "The distance measured from the center of the pulley to the bottom of the \"V\" shape."@en ;
                                              skos:prefLabel "Pulley Radius"@en ,
                                                             "Raio da Polia"@pt-br ;
                                              edo:hasTypedValue edo:floatValue ;
                                              edo:hasValueCardinality edo:multiValue .


###  https://w3id.org/energy-domain/edo#MaximumAllowableTensionTable_PulleyVAngle
edo:MaximumAllowableTensionTable_PulleyVAngle rdf:type owl:Class ;
                                              rdfs:subClassOf edo:DomainAttribute ;
                                              dcterms:accessRights "PUBLIC" ;
                                              dcterms:identifier "MaximumAllowableTensionTable_PulleyVAngle" ;
                                              skos:definition "The angle formed by the opening of the \"V\" Groove in the pulley, measured in degrees."@en ;
                                              skos:prefLabel "Pulley V Groove Angle"@en ,
                                                             "Ângulo do Sulco em V da Polia"@pt-br ;
                                              edo:hasTypedValue edo:floatValue ;
                                              edo:hasValueCardinality edo:multiValue .


###  https://w3id.org/energy-domain/edo#MaximumAllowableTighteningTable
edo:MaximumAllowableTighteningTable rdf:type owl:Class ;
                                    rdfs:subClassOf edo:DomainAttribute ;
                                    dcterms:accessRights "PUBLIC" ;
                                    dcterms:identifier "MaximumAllowableTighteningTable" ;
                                    skos:definition "Esmagamento Máximo permitido Aperto x Tabela de carga axial"@pt-br ,
                                                    "Provides data on the maximum allowable tightening parameters for fasteners, ensuring that the correct torque is applied without exceeding limits that could compromise the integrity of the components. This information is crucial for maintaining mechanical reliability and preventing damage during assembly."@en ;
                                    skos:prefLabel "Maximum Allowable Tightening Table"@en ,
                                                   "Tabela de Aperto Máximo Permitido"@pt-br .


###  https://w3id.org/energy-domain/edo#MaximumAllowableTighteningTable_AxialLoad
edo:MaximumAllowableTighteningTable_AxialLoad rdf:type owl:Class ;
                                              rdfs:subClassOf edo:DomainAttribute ;
                                              dcterms:accessRights "PUBLIC" ;
                                              dcterms:identifier "MaximumAllowableTighteningTable_AxialLoad" ;
                                              skos:definition "Represents the force applied along the longitudinal axis of a component or system. This property is important for evaluating the ability of the structure to resist stretching or compression, ensuring it maintains integrity under operational loads."@en ;
                                              skos:prefLabel "Axial Load"@en ,
                                                             "Tabela de Aperto Máximo Permitido - Carga Axial"@pt-br ;
                                              edo:hasTypedValue edo:floatValue ;
                                              edo:hasValueCardinality edo:multiValue .


###  https://w3id.org/energy-domain/edo#MaximumAllowableTighteningTable_TighteningPerTrack
edo:MaximumAllowableTighteningTable_TighteningPerTrack rdf:type owl:Class ;
                                                       rdfs:subClassOf edo:DomainAttribute ;
                                                       dcterms:accessRights "PUBLIC" ;
                                                       dcterms:identifier "MaximumAllowableTighteningTable_TighteningPerTrack" ;
                                                       skos:definition "Indicates the amount of tightening applied per track during an operation. This property is important for ensuring consistent force distribution across multiple tracks, helping to maintain proper alignment and secure attachment during the tightening process."@en ;
                                                       skos:prefLabel "Tabela de Aperto Máximo Permitido - Aperto por Lagarta"@pt-br ,
                                                                      "Tightening Per Track"@en ;
                                                       edo:hasTypedValue edo:floatValue ;
                                                       edo:hasValueCardinality edo:multiValue .


###  https://w3id.org/energy-domain/edo#MaximumAmbientTemperature
edo:MaximumAmbientTemperature rdf:type owl:Class ;
                              rdfs:subClassOf edo:DomainAttribute ;
                              dcterms:accessRights "PUBLIC" ;
                              dcterms:identifier "MaximumAmbientTemperature" ;
                              skos:definition "Represents the highest ambient temperature at which a component or material can operate effectively without risk of degradation or failure. This property is crucial for ensuring the material's performance and longevity under elevated temperature conditions."@en ;
                              skos:prefLabel "Maximum Ambient Temperature"@en ,
                                             "Temperatura ambiente máxima"@pt-br ;
                              edo:hasTypedValue edo:floatValue ;
                              edo:hasValueCardinality edo:singleValue .


###  https://w3id.org/energy-domain/edo#MaximumTemperature
edo:MaximumTemperature rdf:type owl:Class ;
                       rdfs:subClassOf edo:DomainAttribute ;
                       dcterms:accessRights "PUBLIC" ;
                       dcterms:identifier "MaximumTemperature" ;
                       skos:definition "Represents the highest temperature at which the structure or component can safely operate without compromising its integrity or performance. This value is critical for ensuring that materials and components maintain their mechanical properties and do not experience degradation, deformation, or failure under extreme thermal conditions."@en ;
                       skos:prefLabel "Maximum Temperature"@en ,
                                      "Temperatura Máxima"@pt-br ;
                       edo:hasTypedValue edo:floatValue ;
                       edo:hasValueCardinality edo:singleValue .


###  https://w3id.org/energy-domain/edo#MaximumThermalExchangeCoefficient
edo:MaximumThermalExchangeCoefficient rdf:type owl:Class ;
                                      rdfs:subClassOf edo:DomainAttribute ;
                                      dcterms:accessRights "PUBLIC" ;
                                      dcterms:identifier "MaximumThermalExchangeCoefficient" ;
                                      skos:definition "Indicates the maximum allowable value for the Thermal Exchange Coefficient (TEC), specifying the upper limit for heat transfer in the design. This value ensures that the flexible pipeline meets thermal performance requirements without exceeding the permissible heat transfer rate, which could affect its integrity and operational efficiency."@en ;
                                      skos:prefLabel "Coeficiente Máximo de Troca Térmica (TEC)"@pt-br ,
                                                     "Maximum Thermal Exchange Coefficient (TEC)"@en ;
                                      edo:hasTypedValue edo:floatValue ;
                                      edo:hasValueCardinality edo:singleValue .


###  https://w3id.org/energy-domain/edo#MetallicLayerMaterialType
edo:MetallicLayerMaterialType rdf:type owl:Class ;
                              rdfs:subClassOf edo:DomainAttribute ;
                              dcterms:accessRights "PUBLIC" ;
                              dcterms:identifier "MetallicLayerMaterialType" ;
                              skos:definition "Type of material from which an object is made, allowing for precise documentation and categorisation."@en ;
                              skos:prefLabel "Metallic Layer Material Type"@en ,
                                             "Tipo de Material da Camada Metálica"@pt-br ;
                              edo:hasTypedValue edo:stringValue ;
                              edo:hasValueCardinality edo:singleValue .


###  https://w3id.org/energy-domain/edo#MetallicLayerPitch
edo:MetallicLayerPitch rdf:type owl:Class ;
                       rdfs:subClassOf edo:DomainAttribute ;
                       dcterms:accessRights "PUBLIC" ;
                       dcterms:identifier "MetallicLayerPitch" ;
                       skos:definition "Indicates the distance between adjacent metallic elements in the layer, typically arranged helicoidally. This value is critical for determining the mechanical properties of the metallic layer, such as its flexibility, strength, and performance under load."@en ;
                       skos:prefLabel "Metallic Layer Pitch"@en ,
                                      "Passo da Camada Metálica"@pt-br ;
                       edo:hasTypedValue edo:floatValue ;
                       edo:hasValueCardinality edo:singleValue .


###  https://w3id.org/energy-domain/edo#MetallicMaterial
edo:MetallicMaterial rdf:type owl:Class ;
                     rdfs:subClassOf edo:FlexibleStructureLayerMaterial ;
                     dcterms:identifier "MetallicMaterial" ;
                     skos:definition "Material used in the fabrication of metallic layers in subsea flexible pipes, chosen for its strength, durability, and resistance to harsh environmental conditions. The Metallic Material provides structural reinforcement, enhances pressure resistance, and supports the pipe's overall integrity. Commonly used materials include stainless steel, carbon steel, or other corrosion-resistant alloys, which are selected based on their ability to withstand the operational demands of deepwater environments, such as high pressure, tension, and dynamic loading."@en ;
                     skos:prefLabel "Material Metálico"@pt-br ,
                                    "Metallic Material"@en ;
                     edo:hasAttribute edo:FractureToughness ,
                                      edo:MetallicLayerMaterialType ,
                                      edo:UltimateTensileStress ;
                     edo:ifc_equivalentClass "IfcMaterial" ;
                     edo:ifc_objectType "MetallicMaterial" .


###  https://w3id.org/energy-domain/edo#MetallicStrandLength
edo:MetallicStrandLength rdf:type owl:Class ;
                         rdfs:subClassOf edo:DomainAttribute ;
                         dcterms:accessRights "PUBLIC" ;
                         dcterms:identifier "MetallicStrandLength" ;
                         skos:definition "The total length of the metallic strand used in the anode to endfittings connection"@en ;
                         skos:prefLabel "Comprimento da Cordoalha Metálica"@pt-br ,
                                        "Metallic Strand Length"@en ;
                         edo:hasTypedValue edo:floatValue ;
                         edo:hasValueCardinality edo:singleValue .


###  https://w3id.org/energy-domain/edo#MetallicStrandSet
edo:MetallicStrandSet rdf:type owl:Class ;
                      rdfs:subClassOf edo:PhysicalConnection ;
                      dcterms:identifier "MetallicStrandSet" ;
                      skos:definition "Galvanic connection cables set providing reliable electrical link between anodes and metal infrastructure for effective corrosion mitigation."@en ;
                      skos:prefLabel "Conjunto de Cordoalhas de Continuidade"@pt-br ,
                                     "Metallic Strand Set"@en ;
                      edo:hasAttribute edo:StrandsTable ,
                                       edo:StrandsTable_SpareQuantity ,
                                       edo:StrandsTable_StrandsLength ,
                                       edo:StrandsTable_StrandsQuantity ;
                      edo:ifc_equivalentClass "IfcCableSegment" ;
                      edo:ifc_objectType "MetallicStrandSet" ;
                      edo:ifc_predefinedType "USERDEFINED" .


###  https://w3id.org/energy-domain/edo#MetallicStrandSpareQuantity
edo:MetallicStrandSpareQuantity rdf:type owl:Class ;
                                rdfs:subClassOf edo:DomainAttribute ;
                                dcterms:accessRights "PUBLIC" ;
                                dcterms:identifier "MetallicStrandSpareQuantity" ;
                                skos:definition "The additional quantity of metallic strands provided as spare material for contingency or repair purposes."@en ;
                                skos:prefLabel "Metallic Strand Spare Quantity"@en ,
                                               "Quantidade de Cordoalhas Metálicas Sobressalentes"@pt-br ;
                                edo:hasTypedValue edo:intValue ;
                                edo:hasValueCardinality edo:singleValue .


###  https://w3id.org/energy-domain/edo#MetricBoltSet
edo:MetricBoltSet rdf:type owl:Class ;
                  rdfs:subClassOf edo:BoltSet ;
                  dcterms:identifier "MetricBoltSet" ;
                  skos:definition "A set of bolts and accompanying hardware sized using the metric measurement system, commonly used in subsea applications for international compatibility and standardization."@en ;
                  skos:prefLabel "Conjunto de Parafusos Métrico"@pt-br ,
                                 "Metric Bolt Set"@en ;
                  edo:hasAttribute edo:NominalDiameter ,
                                   edo:PitchToleranceClass ,
                                   edo:ThreadPitch ,
                                   edo:ThreadStandard ;
                  edo:ifc_equivalentClass "IfcMechanicalFastener" ;
                  edo:ifc_objectType "MetricBoltSet" ;
                  edo:ifc_predefinedType "USERDEFINED" .


###  https://w3id.org/energy-domain/edo#MetricStudSet
edo:MetricStudSet rdf:type owl:Class ;
                  rdfs:subClassOf edo:StudSet ;
                  dcterms:identifier "MetricStudSet" ;
                  skos:altLabel "Metric Stud"@en ,
                                "Metric Threaded Rod"@en ;
                  skos:definition "Metric studs are crucial fastening components for subsea oil and gas components, designed specifically to secure equipment parts. Each set includes bolts, nuts, and washers in metric sizing, made from high-strength, corrosion-resistant materials to withstand the demanding subsea environment. These components offer dependable fastening, ensuring structural integrity and leak prevention in end fittings. Metric stud sets are engineered to endure high pressure and extreme temperatures, making them essential for the safety and durability of subsea interconnections."@en ;
                  skos:prefLabel "Conjunto de Estojos Métrico"@pt-br ,
                                 "Metric Stud Set"@en ;
                  edo:hasAttribute edo:PitchToleranceClass ,
                                   edo:ThreadPitch ,
                                   edo:ThreadStandard ;
                  edo:ifc_equivalentClass "IfcMechanicalFastener" ;
                  edo:ifc_objectType "MetricStudSet" ;
                  edo:ifc_predefinedType "USERDEFINED" .


###  https://w3id.org/energy-domain/edo#Midstream
edo:Midstream rdf:type owl:Class ;
              rdfs:subClassOf edo:OilAndGas ;
              rdfs:label "Midstream"@en ,
                         "Midstream"@pt-br ;
              skos:definition "Oil & Gas sector covering transportation, storage, and wholesale marketing of crude or refined petroleum products."@en ,
                              "Setor de Petróleo & Gás que abrange transporte, armazenamento e comercialização atacadista de produtos petrolíferos brutos ou refinados."@pt-br .


###  https://w3id.org/energy-domain/edo#MinimumBendingRadiusForStorage
edo:MinimumBendingRadiusForStorage rdf:type owl:Class ;
                                   rdfs:subClassOf edo:DomainAttribute ;
                                   dcterms:accessRights "PUBLIC" ;
                                   dcterms:identifier "MinimumBendingRadiusForStorage" ;
                                   skos:definition "Represents the smallest radius to which a component can be bent during storage without causing damage or affecting its performance. This property is important for ensuring that the component maintains its integrity while in storage, preventing deformation or weakening."@en ;
                                   skos:prefLabel "Minimum Bending Radius For Storage"@en ,
                                                  "Raio Mínimo de Curvatura para Armazenamento"@pt-br ;
                                   edo:hasTypedValue edo:floatValue ;
                                   edo:hasValueCardinality edo:singleValue .


###  https://w3id.org/energy-domain/edo#MinimumTemperature
edo:MinimumTemperature rdf:type owl:Class ;
                       rdfs:subClassOf edo:DomainAttribute ;
                       dcterms:accessRights "PUBLIC" ;
                       dcterms:identifier "MinimumTemperature" ;
                       skos:definition "Represents the lowest temperature at which the structure or component can safely operate without experiencing performance degradation or failure. This value is important for ensuring that the materials maintain their properties and structural integrity when exposed to extremely low temperatures"@en ;
                       skos:prefLabel "Minimum Temperature"@en ,
                                      "Temperatura Mínima"@pt-br ;
                       edo:hasTypedValue edo:floatValue ;
                       edo:hasValueCardinality edo:singleValue .


###  https://w3id.org/energy-domain/edo#MinimumThermalExchangeCoefficient
edo:MinimumThermalExchangeCoefficient rdf:type owl:Class ;
                                      rdfs:subClassOf edo:DomainAttribute ;
                                      dcterms:accessRights "PUBLIC" ;
                                      dcterms:identifier "MinimumThermalExchangeCoefficient" ;
                                      skos:definition "Indicates the minimum allowable value for the Thermal Exchange Coefficient (TEC), specifying the lower limit for heat transfer in the design. This value ensures that the flexible pipeline maintains sufficient heat transfer capability to meet operational performance requirements."@en ;
                                      skos:prefLabel "Coeficiente Mínimo de Troca Térmica (TEC)"@pt-br ,
                                                     "Minimum Thermal Exchange Coefficient (TEC)"@en ;
                                      edo:hasTypedValue edo:floatValue ;
                                      edo:hasValueCardinality edo:singleValue .


###  https://w3id.org/energy-domain/edo#ModelLocationPoint
edo:ModelLocationPoint rdf:type owl:Class ;
                       rdfs:subClassOf edo:DomainElement ;
                       dcterms:identifier "ModelLocationPoint" ;
                       skos:definition "A specific reference point or coordinate used to define the precise location of equipment, infrastructure, or components within a 3D model."@en ;
                       skos:prefLabel "Model Location Point"@en ,
                                      "Ponto de Localização no Modelo"@pt-br .


###  https://w3id.org/energy-domain/edo#ModulusOfElasticity
edo:ModulusOfElasticity rdf:type owl:Class ;
                        rdfs:subClassOf edo:DomainAttribute ;
                        dcterms:accessRights "PUBLIC" ;
                        dcterms:identifier "ModulusOfElasticity" ;
                        skos:definition "The modulus of elasticity represents the material's ability to resist deformation under stress. It quantifies the ratio of stress to strain within the elastic range of the material. This property is crucial for understanding how the material will behave under various loads and conditions."@en ;
                        skos:prefLabel "Modulus Of Elasticity"@en ,
                                       "Módulo de elasticidade"@pt-br ;
                        edo:hasTypedValue edo:floatValue ;
                        edo:hasValueCardinality edo:singleValue .


###  https://w3id.org/energy-domain/edo#MooringAccessory
edo:MooringAccessory rdf:type owl:Class ;
                     rdfs:subClassOf edo:HardwareItem ;
                     dcterms:identifier "MooringAccessory" ;
                     skos:definition "A Mooring Accessory includes components like anchors, chains, and connectors used to secure offshore platforms or vessels to the seabed, ensuring stability and safety in harsh marine conditions."@en ;
                     skos:prefLabel "Acessório de Amarração"@pt-br ,
                                    "Mooring Accessory"@en .


###  https://w3id.org/energy-domain/edo#NominalDiameter
edo:NominalDiameter rdf:type owl:Class ;
                    rdfs:subClassOf edo:DomainAttribute ;
                    dcterms:accessRights "PUBLIC" ;
                    dcterms:identifier "NominalDiameter" ;
                    skos:definition "The standard diameter of the component or pipe, typically used for classification and specification purposes."@en ;
                    skos:prefLabel "Diâmetro Nominal"@pt-br ,
                                   "Nominal Diameter"@en ;
                    edo:hasTypedValue edo:stringValue ;
                    edo:hasValueCardinality edo:singleValue .


###  https://w3id.org/energy-domain/edo#NominalFloatDensity
edo:NominalFloatDensity rdf:type owl:Class ;
                        rdfs:subClassOf edo:DomainAttribute ;
                        dcterms:accessRights "PUBLIC" ;
                        dcterms:identifier "NominalFloatDensity" ;
                        skos:definition "A densidade ideal do flutuador antes de qualquer absorção de água ou degradação. Usada para calcular a flutuabilidade inicial máxima, idealmente no ponto de fabricação."@pt-br ,
                                        "The ideal density of the float material before any water absorption or degradation occurs. This is used to calculate the float's maximum buoyancy at the beginning of its use."@en ;
                        skos:prefLabel "Densidade Nominal do Flutuador"@pt-br ,
                                       "Nominal Float Density"@en ;
                        edo:hasTypedValue edo:floatValue ;
                        edo:hasValueCardinality edo:singleValue .


###  https://w3id.org/energy-domain/edo#NominalFloatVolume
edo:NominalFloatVolume rdf:type owl:Class ;
                       rdfs:subClassOf edo:DomainAttribute ;
                       dcterms:accessRights "PUBLIC" ;
                       dcterms:identifier "NominalFloatVolume" ;
                       skos:definition "O volume ideal, ou \"de fábrica\", sem considerar a absorção de água ou deformações. É usado para calcular a flutuabilidade máxima possível, antes de qualquer degradação."@pt-br ,
                                       "The ideal or factory-specified volume of the float before any external effects like water absorption or deformation occur. This value is used to calculate the maximum buoyancy under perfect conditions."@en ;
                       skos:prefLabel "Nominal Float Volume"@en ,
                                      "Volume Nominal do Flutuador"@pt-br ;
                       edo:hasTypedValue edo:floatValue ;
                       edo:hasValueCardinality edo:singleValue .


###  https://w3id.org/energy-domain/edo#NominalLength
edo:NominalLength rdf:type owl:Class ;
                  rdfs:subClassOf edo:DomainAttribute ;
                  dcterms:accessRights "PUBLIC" ;
                  dcterms:identifier "NominalLength" ;
                  skos:definition "Nominal length refers to the length of an object as designed, typically used as a reference value. It may not represent the exact physical measurement but serves as the standard or intended length for manufacturing, design, or specification purposes."@en ;
                  skos:prefLabel "Comprimento Nominal"@pt-br ,
                                 "Nominal Length"@en ;
                  edo:hasTypedValue edo:floatValue ;
                  edo:hasValueCardinality edo:singleValue .


###  https://w3id.org/energy-domain/edo#Nuclear
edo:Nuclear rdf:type owl:Class ;
            rdfs:subClassOf edo:Domain ;
            rdfs:label "Energia Nuclear"@pt-br ,
                       "Nuclear Energy"@en ;
            skos:definition "Domínio industrial que abrange a geração de energia a partir de reações nucleares, incluindo fissão e fusão."@pt-br ,
                            "Industrial domain covering the generation of energy from nuclear reactions, including fission and fusion."@en .


###  https://w3id.org/energy-domain/edo#NuclearFuelCycle
edo:NuclearFuelCycle rdf:type owl:Class ;
                     rdfs:subClassOf edo:Nuclear ;
                     rdfs:label "Ciclo do Combustível Nuclear"@pt-br ,
                                "Nuclear Fuel Cycle"@en ;
                     skos:definition "Processes involved in mining, processing, enrichment, and disposal of nuclear fuel."@en ,
                                     "Processos envolvidos na mineração, processamento, enriquecimento e descarte de combustível nuclear."@pt-br .


###  https://w3id.org/energy-domain/edo#NuclearPowerGeneration
edo:NuclearPowerGeneration rdf:type owl:Class ;
                           rdfs:subClassOf edo:Nuclear ;
                           rdfs:label "Geração de Energia Nuclear"@pt-br ,
                                      "Nuclear Power Generation"@en ;
                           skos:definition "Operation and maintenance of nuclear power plants for electricity production."@en ,
                                           "Operação e manutenção de usinas nucleares para produção de eletricidade."@pt-br .


###  https://w3id.org/energy-domain/edo#NumberOfChokeValves
edo:NumberOfChokeValves rdf:type owl:Class ;
                        rdfs:subClassOf edo:DomainAttribute ;
                        dcterms:accessRights "PUBLIC" ;
                        dcterms:identifier "NumberOfChokeValves" ;
                        skos:definition "Number of process choke valves"@en ,
                                        "Número de válvulas choke"@pt-br ;
                        skos:prefLabel "Number Of Choke Valves"@en ,
                                       "Número de válvulas de estrangulamento"@pt-br ;
                        edo:hasTypedValue edo:intValue ;
                        edo:hasValueCardinality edo:singleValue .


###  https://w3id.org/energy-domain/edo#NumberOfRemoteProcessIsolationValves
edo:NumberOfRemoteProcessIsolationValves rdf:type owl:Class ;
                                         rdfs:subClassOf edo:DomainAttribute ;
                                         dcterms:accessRights "PUBLIC" ;
                                         dcterms:identifier "NumberOfRemoteProcessIsolationValves" ;
                                         skos:definition "Number of remotely-actuated process isolation valves"@en ,
                                                         "Número de válvulas de isolamento de processo com atuação remota"@pt-br ;
                                         skos:prefLabel "Number Of Remote Process Isolation Valves"@en ,
                                                        "Número de válvulas de isolamento de processo remoto"@pt-br ;
                                         edo:hasTypedValue edo:intValue ;
                                         edo:hasValueCardinality edo:singleValue .


###  https://w3id.org/energy-domain/edo#OffLeakPLevMaxPress
edo:OffLeakPLevMaxPress rdf:type owl:Class ;
                        rdfs:subClassOf edo:DomainAttribute ;
                        dcterms:accessRights "PUBLIC" ;
                        dcterms:identifier "OffLeakPLevMaxPress" ;
                        skos:definition "Condições de teste dos tramos para Pressão - Máxima - Teste de vazamento hidrostático offshore (no nível da plataforma)"@pt-br ,
                                        "The maximum pressure applied during the Offshore Leak Test (at platform level), ensuring no leaks occur under extreme pressure."@en ;
                        skos:prefLabel "Offshore Leak Test At Platform Level Maximum Pressure"@en ,
                                       "Teste de Vazamento Offshore na Pressão Máxima no Nível da Plataforma"@pt-br ;
                        edo:hasTypedValue edo:floatValue ;
                        edo:hasValueCardinality edo:singleValue .


###  https://w3id.org/energy-domain/edo#OffLeakPLevMaxPressValRef
edo:OffLeakPLevMaxPressValRef rdf:type owl:Class ;
                              rdfs:subClassOf edo:DomainAttribute ;
                              dcterms:accessRights "PUBLIC" ;
                              dcterms:identifier "OffLeakPLevMaxPressValRef" ;
                              skos:definition "Comentários Condições de teste dos tramos para - Máximo - Teste de vazamento hidrostático offshore (no nível da plataforma)"@pt-br ,
                                              "Specifies the reference pressure used to determine the Offshore Leak Test maximum pressure value."@en ;
                              skos:prefLabel "Offshore Leak Test At Platform Level Maximum Pressure Value Reference"@en ,
                                             "Referência de Valor de Pressão Máxima para Teste de Vazamento Offshore no Nível da Plataforma"@pt-br ;
                              edo:hasTypedValue edo:stringValue ;
                              edo:hasValueCardinality edo:singleValue .


###  https://w3id.org/energy-domain/edo#OffLeakPLevMaxPressValRefMult
edo:OffLeakPLevMaxPressValRefMult rdf:type owl:Class ;
                                  rdfs:subClassOf edo:DomainAttribute ;
                                  dcterms:accessRights "PUBLIC" ;
                                  dcterms:identifier "OffLeakPLevMaxPressValRefMult" ;
                                  skos:definition "The multiplier applied to the reference pressure to determine the Offshore Leak Test maximum pressure value."@en ;
                                  skos:prefLabel "Multiplicador de Referência de Valor de Pressão Máxima para Teste de Vazamento Offshore no Nível da Plataforma"@pt-br ,
                                                 "Offshore Leak Test At Platform Level Maximum Pressure Value Reference Multiplier"@en ;
                                  edo:hasTypedValue edo:floatValue ;
                                  edo:hasValueCardinality edo:singleValue .


###  https://w3id.org/energy-domain/edo#OffLeakPLevNomPress
edo:OffLeakPLevNomPress rdf:type owl:Class ;
                        rdfs:subClassOf edo:DomainAttribute ;
                        dcterms:accessRights "PUBLIC" ;
                        dcterms:identifier "OffLeakPLevNomPress" ;
                        skos:definition "Condições de teste dos tramos para Pressão - Nominal - Teste de vazamento hidrostático offshore (no nível da plataforma)"@pt-br ,
                                        "The nominal pressure applied during the Offshore Leak Test (at platform level), simulating typical operating conditions to assess for leaks."@en ;
                        skos:prefLabel "Offshore Leak Test At Platform Level Nominal Pressure"@en ,
                                       "Pressão Nominal para Teste de Vazamento Offshore no Nível da Plataforma"@pt-br ;
                        edo:hasTypedValue edo:floatValue ;
                        edo:hasValueCardinality edo:singleValue .


###  https://w3id.org/energy-domain/edo#OffLeakPLevNomPressValRef
edo:OffLeakPLevNomPressValRef rdf:type owl:Class ;
                              rdfs:subClassOf edo:DomainAttribute ;
                              dcterms:accessRights "PUBLIC" ;
                              dcterms:identifier "OffLeakPLevNomPressValRef" ;
                              skos:definition "Comentários Condições de teste dos tramos para - Nominal - Teste de vazamento hidrostático offshore (no nível da plataforma)"@pt-br ,
                                              "Specifies the reference pressure used to determine the Offshore Leak Test nominal pressure value."@en ;
                              skos:prefLabel "Offshore Leak Test At Platform Level Nominal Pressure Value Reference"@en ,
                                             "Referência de Valor de Pressão Nominal para Teste de Vazamento Offshore no Nível da Plataforma"@pt-br ;
                              edo:hasTypedValue edo:stringValue ;
                              edo:hasValueCardinality edo:singleValue .


###  https://w3id.org/energy-domain/edo#OffLeakPLevNomPressValRefMult
edo:OffLeakPLevNomPressValRefMult rdf:type owl:Class ;
                                  rdfs:subClassOf edo:DomainAttribute ;
                                  dcterms:accessRights "PUBLIC" ;
                                  dcterms:identifier "OffLeakPLevNomPressValRefMult" ;
                                  skos:definition "The multiplier applied to the reference pressure to determine the Offshore Leak Test nominal pressure value."@en ;
                                  skos:prefLabel "Multiplicador de Referência de Valor de Pressão Nominal para Teste de Vazamento Offshore no Nível da Plataforma"@pt-br ,
                                                 "Offshore Leak Test At Platform Level Nominal Pressure Value Reference Multiplier"@en ;
                                  edo:hasTypedValue edo:floatValue ;
                                  edo:hasValueCardinality edo:singleValue .


###  https://w3id.org/energy-domain/edo#Offshore
edo:Offshore rdf:type owl:Class ;
             rdfs:subClassOf edo:LocationType ;
             rdfs:label "Offshore"@en ,
                        "Offshore"@pt-br ;
             skos:definition "Atividades industriais realizadas no mar, tipicamente para produção de petróleo & gás ou energia eólica."@pt-br ,
                             "Industrial activities conducted at sea, typically for oil & gas or wind energy production."@en .


###  https://w3id.org/energy-domain/edo#OilAndGas
edo:OilAndGas rdf:type owl:Class ;
              rdfs:subClassOf edo:Domain ;
              rdfs:label "Oil & Gas"@en ,
                         "Petróleo & Gás"@pt-br ;
              skos:definition "Domínio industrial que abrange todas as atividades relacionadas à exploração, produção, refino e distribuição de petróleo e gás."@pt-br ,
                              "Industrial domain covering all activities related to the exploration, production, refining, and distribution of oil and gas."@en .


###  https://w3id.org/energy-domain/edo#Onshore
edo:Onshore rdf:type owl:Class ;
            rdfs:subClassOf edo:LocationType ;
            rdfs:label "Onshore"@en ,
                       "Onshore"@pt-br ;
            skos:definition "Atividades industriais realizadas em terra."@pt-br ,
                            "Industrial activities conducted on land."@en .


###  https://w3id.org/energy-domain/edo#OpenReceptacle
edo:OpenReceptacle rdf:type owl:Class ;
                   rdfs:subClassOf edo:RiserSupport ;
                   dcterms:identifier "OpenReceptacle" .


###  https://w3id.org/energy-domain/edo#Operation
edo:Operation rdf:type owl:Class ;
              rdfs:subClassOf edo:LifecyclePhase ;
              rdfs:label "Operation"@en ,
                         "Operação"@pt-br ;
              skos:definition "Normal use of the asset for its intended purpose, including monitoring and control."@en ,
                              "Uso normal do ativo para seu propósito pretendido, incluindo monitoramento e controle."@pt-br .


###  https://w3id.org/energy-domain/edo#OuterDiameter
edo:OuterDiameter rdf:type owl:Class ;
                  rdfs:subClassOf edo:DomainAttribute ;
                  dcterms:accessRights "PUBLIC" ;
                  dcterms:identifier "OuterDiameter" ;
                  skos:definition "Represents the external diameter of a component, typically measured from one outer edge to the opposite outer edge. This property is important for ensuring proper fit, compatibility, and performance within a system or assembly."@en ;
                  skos:prefLabel "Diâmetro externo"@pt-br ,
                                 "Outer Diameter"@en ;
                  edo:hasTypedValue edo:floatValue ;
                  edo:hasValueCardinality edo:singleValue .


###  https://w3id.org/energy-domain/edo#OutsideTemperature
edo:OutsideTemperature rdf:type owl:Class ;
                       rdfs:subClassOf edo:DomainAttribute ;
                       dcterms:accessRights "PUBLIC" ;
                       dcterms:identifier "OutsideTemperature" ;
                       skos:definition "Represents the external temperature surrounding a component or system. This property is important for assessing the thermal conditions that the component is exposed to, ensuring it operates within safe temperature limits."@en ;
                       skos:prefLabel "Outside Temperature"@en ,
                                      "Temperatura Externa"@pt-br ;
                       edo:hasTypedValue edo:floatValue ;
                       edo:hasValueCardinality edo:singleValue .


###  https://w3id.org/energy-domain/edo#PackageEquipmentEngineering
edo:PackageEquipmentEngineering rdf:type owl:Class ;
                                rdfs:subClassOf edo:EquipmentEngineering ;
                                rdfs:label "Engenharia de Equipamentos Modulares"@pt-br ,
                                           "Package Equipment Engineering"@en ;
                                skos:definition "Engenharia de sistemas de equipamentos modulares ou montados em skids."@pt-br ,
                                                "Engineering of skid-mounted or modular equipment systems."@en .


###  https://w3id.org/energy-domain/edo#PartNumber
edo:PartNumber rdf:type owl:Class ;
               rdfs:subClassOf edo:DomainAttribute ;
               dcterms:accessRights "PUBLIC" ;
               dcterms:identifier "PartNumber" ;
               skos:definition "The Part Number is a unique identifier assigned to each type of element, ensuring consistency and ease of reference. This identifier helps in categorizing, ordering, and tracking the accessory within the system. When the drawing code is used consistently across all projects for a specific type of accessory, it can also serve as the Part Number, facilitating uniformity in documentation and usage."@en ;
               skos:prefLabel "Número da peça do acessório"@pt-br ,
                              "Part Number"@en ;
               edo:hasTypedValue edo:stringValue ;
               edo:hasValueCardinality edo:singleValue .


###  https://w3id.org/energy-domain/edo#PermeabilityTable
edo:PermeabilityTable rdf:type owl:Class ;
                      rdfs:subClassOf edo:DomainAttribute ;
                      dcterms:accessRights "PUBLIC" ;
                      dcterms:identifier "PermeabilityTable" ;
                      skos:definition "Permeabilidade (Específica para Materiais Poliméricos)"@pt-br ,
                                      "Provides data on the permeability of various substances through materials, helping to assess the rate at which fluids or gases can pass through the structure. This information is crucial for evaluating material performance, ensuring compatibility, and predicting long-term behavior under operational conditions."@en ;
                      skos:prefLabel "Permeability Table"@en ,
                                     "Tabela de Permeabilidade"@pt-br .


###  https://w3id.org/energy-domain/edo#PermeabilityTable_MoleculeIdentifier
edo:PermeabilityTable_MoleculeIdentifier rdf:type owl:Class ;
                                         rdfs:subClassOf edo:DomainAttribute ;
                                         dcterms:accessRights "PUBLIC" ;
                                         dcterms:identifier "PermeabilityTable_MoleculeIdentifier" ;
                                         skos:definition "Specifies the type of molecule. This property identifies the particular molecule involved, which is crucial for understanding the material's interaction with or response to different chemical substances."@en ,
                                                         "tipo de molécula (co2, h2s, ch4, h2o,…)"@pt-br ;
                                         skos:prefLabel "Identificador de Molécula"@pt-br ,
                                                        "Molecule Identifier"@en ;
                                         edo:hasTypedValue edo:stringValue ;
                                         edo:hasValueCardinality edo:multiValue .


###  https://w3id.org/energy-domain/edo#PermeabilityTable_PermeabilityCoefficient
edo:PermeabilityTable_PermeabilityCoefficient rdf:type owl:Class ;
                                              rdfs:subClassOf edo:DomainAttribute ;
                                              dcterms:accessRights "PUBLIC" ;
                                              dcterms:identifier "PermeabilityTable_PermeabilityCoefficient" ;
                                              skos:definition "Represents the rate at which a substance, such as a gas or liquid, can pass through a material. This property is crucial for understanding the material's resistance to permeation, helping to assess its suitability for containing or isolating specific substances."@en ;
                                              skos:prefLabel "Coeficiente de Permeabilidade"@pt-br ,
                                                             "Permeability Coefficient"@en ;
                                              edo:hasTypedValue edo:floatValue ;
                                              edo:hasValueCardinality edo:multiValue .


###  https://w3id.org/energy-domain/edo#PermeabilityTable_PolymerState
edo:PermeabilityTable_PolymerState rdf:type owl:Class ;
                                   rdfs:subClassOf edo:DomainAttribute ;
                                   dcterms:accessRights "PUBLIC" ;
                                   dcterms:identifier "PermeabilityTable_PolymerState" ;
                                   skos:definition "(plastificado, não plastificado,…)"@pt-br ,
                                                   "The state of the polymeric material is specified.. This property is crucial for understanding how the material behaves under different conditions and its suitability for various applications."@en ;
                                   skos:prefLabel "Estado do Polímero"@pt-br ,
                                                  "Polymer State"@en ;
                                   edo:hasTypedValue edo:stringValue ;
                                   edo:hasValueCardinality edo:multiValue .


###  https://w3id.org/energy-domain/edo#PermeabilityTable_Temperature
edo:PermeabilityTable_Temperature rdf:type owl:Class ;
                                  rdfs:subClassOf edo:DomainAttribute ;
                                  dcterms:accessRights "PUBLIC" ;
                                  dcterms:identifier "PermeabilityTable_Temperature" ;
                                  skos:definition "Represents the thermal condition or measurement of heat for a component or system. This property is important for assessing how the component performs or operates under specific thermal conditions, ensuring it remains within safe and effective operating limits."@en ;
                                  skos:prefLabel "Temperatura"@pt-br ,
                                                 "Temperature"@en ;
                                  edo:hasTypedValue edo:floatValue ;
                                  edo:hasValueCardinality edo:multiValue .


###  https://w3id.org/energy-domain/edo#PhysicalConnection
edo:PhysicalConnection rdf:type owl:Class ;
                       rdfs:subClassOf edo:Connection ;
                       dcterms:identifier "PhysicalConnection" ;
                       skos:definition "A Physical Connection refers to the actual link or interface between two or more components, such as pipes, equipment, or systems, that allows for the transfer of fluids, energy, or data."@en ;
                       skos:prefLabel "Conexão Física"@pt-br ,
                                      "Physical Connection"@en .


###  https://w3id.org/energy-domain/edo#Piggable
edo:Piggable rdf:type owl:Class ;
             rdfs:subClassOf edo:DomainAttribute ;
             dcterms:accessRights "PUBLIC" ;
             dcterms:identifier "Piggable" ;
             skos:definition "Especifica se o equipamento possui pelo menos um circuito interno de escoamento que permita passagem de pig"@pt-br ,
                             "Whether equipment has at least one internal flow circuit allowing pig runs"@en ;
             skos:prefLabel "Piggable"@en ,
                            "Pigável"@pt-br ;
             edo:hasTypedValue edo:booleanValue ;
             edo:hasValueCardinality edo:singleValue .


###  https://w3id.org/energy-domain/edo#PipeMountPosition
edo:PipeMountPosition rdf:type owl:Class ;
                      rdfs:subClassOf edo:DomainAttribute ;
                      dcterms:accessRights "PUBLIC" ;
                      dcterms:identifier "PipeMountPosition" ;
                      skos:definition "Cota em metros da posição em que o item é montado no tramo no sentido do fluxo do fluido."@pt-br ,
                                      "Indicates the distance from the end fitting to the position of the accessory along the direction of fluid flow within the pipe body. This property specifies the precise location of the accessory relative to the end fitting, which is essential for accurate installation and alignment within the tubular body."@en ;
                      skos:prefLabel "Pipe Mount Position"@en ,
                                     "Posição de Montagem no Duto"@pt-br ;
                      edo:hasTypedValue edo:floatValue ;
                      edo:hasValueCardinality edo:singleValue .


###  https://w3id.org/energy-domain/edo#PipePullingHead
edo:PipePullingHead rdf:type owl:Class ;
                    rdfs:subClassOf edo:PullingHead ;
                    dcterms:identifier "PipePullingHead" ;
                    skos:altLabel "Cable Head"@en ,
                                  "Installation Head"@en ,
                                  "Pull Head"@en ,
                                  "Pulling Grip"@en ,
                                  "Pulling Tool"@en ;
                    skos:definition "A component used in subsea flexible pipe installations to provide a secure attachment point for pulling the pipe into position during installation or retrieval operations. The Pulling Head is fitted to the end of the flexible pipe, allowing connection to pulling equipment such as winches or cranes. It is designed to withstand high loads, ensuring that the pipe can be pulled safely without causing damage. The Pulling Head is essential for handling, testing, and securing the pipe in place during subsea installation."@en ;
                    skos:prefLabel "Cabeça de Tração do Duto"@pt-br ,
                                   "Pipe Pulling Head"@en ;
                    edo:hasAttribute edo:FlangeType ,
                                     edo:PullingHeadType ,
                                     edo:RingGasketInnerDIameter ,
                                     edo:RingGasketMaterial ,
                                     edo:RingGasketOuterDiameter ,
                                     edo:RingGasketPressureRating ,
                                     edo:RingGasketSpecification ,
                                     edo:RingGasketStandard ,
                                     edo:RingGasketType ,
                                     edo:SafeWorkingLoad ;
                    edo:ifc_equivalentClass "IfcPipeFitting" ;
                    edo:ifc_objectType "PipePullingHead" ;
                    edo:ifc_predefinedType "USERDEFINED" .


###  https://w3id.org/energy-domain/edo#PipeSectionApplication
edo:PipeSectionApplication rdf:type owl:Class ;
                           rdfs:subClassOf edo:DomainAttribute ;
                           dcterms:accessRights "PUBLIC" ;
                           dcterms:identifier "PipeSectionApplication" ;
                           skos:definition "Aplicação do tramo, de acordo com as seguintes nomenclaturas: R (Riser); RT (seção de topo do riser); RI (seção intermediaria do riser); RF (seção de fundo do riser); F (Flowline)"@pt-br ,
                                           "Indicates the specific application of the flexible pipe section in the interconnection system, categorizing it based on its role or position within the riser or flowline."@en ;
                           skos:prefLabel "Aplicação do Tramo"@pt-br ,
                                          "Pipe Section Application"@en ;
                           edo:hasTypedValue edo:stringValue ;
                           edo:hasValueCardinality edo:singleValue .


###  https://w3id.org/energy-domain/edo#PipeSegment
edo:PipeSegment rdf:type owl:Class ;
                rdfs:subClassOf edo:TransportLineSegment ;
                dcterms:identifier "PipeSegment" ;
                skos:definition "Pipeline segment for movement/flow of fluids."@en ,
                                "Segmento de Duto"@pt-br ;
                skos:prefLabel "Pipe Segment"@en ,
                               "Segmento de Duto"@pt-br .


###  https://w3id.org/energy-domain/edo#PipeTermination
edo:PipeTermination rdf:type owl:Class ;
                    rdfs:subClassOf edo:LineTermination ;
                    dcterms:identifier "PipeTermination" ;
                    skos:definition "The Pipe Termination refers to the components at the end of a pipeline that provide the final connection to other equipment or systems. These terminations are crucial for ensuring a secure and reliable interface between the pipeline and surrounding infrastructure, allowing for the proper transfer of fluids or gases and maintaining the integrity of the overall system."@en ;
                    skos:prefLabel "Pipe Termination"@en ,
                                   "Terminador de Duto"@pt-br .


###  https://w3id.org/energy-domain/edo#PipelineSpan
edo:PipelineSpan rdf:type owl:Class ;
                 rdfs:subClassOf edo:LineSpan ;
                 dcterms:identifier "PipelineSpan" .


###  https://w3id.org/energy-domain/edo#PitchToleranceClass
edo:PitchToleranceClass rdf:type owl:Class ;
                        rdfs:subClassOf edo:DomainAttribute ;
                        dcterms:accessRights "PUBLIC" ;
                        dcterms:identifier "PitchToleranceClass" ;
                        skos:definition "A classification defining the acceptable deviation range for the pitch measurement, ensuring consistency in the helical arrangement of wires or threads."@en ;
                        skos:prefLabel "Classe de Tolerância de Passo"@pt-br ,
                                       "Pitch Tolerance Class"@en ;
                        edo:hasTypedValue edo:stringValue ;
                        edo:hasValueCardinality edo:singleValue .


###  https://w3id.org/energy-domain/edo#Planned_Start_Timestamp
edo:Planned_Start_Timestamp rdf:type owl:Class ;
                            rdfs:subClassOf edo:DomainAttribute ;
                            dcterms:accessRights "PUBLIC" ;
                            dcterms:identifier "Planned_Start_Timestamp" ;
                            skos:prefLabel "Planned Start Timestamp"@en ;
                            edo:hasTypedValue edo:dateTimeValue ;
                            edo:hasValueCardinality edo:singleValue .


###  https://w3id.org/energy-domain/edo#PointLocation
edo:PointLocation rdf:type owl:Class ;
                  rdfs:subClassOf edo:Location ;
                  dcterms:identifier "PointLocation" ;
                  skos:definition "Basis for all locations that can conventionally be situated at a single geographic point."@en ;
                  skos:prefLabel "Localização de Ponto"@pt-br ,
                                 "Point Location"@en .


###  https://w3id.org/energy-domain/edo#PoissonRatioAt23Degrees
edo:PoissonRatioAt23Degrees rdf:type owl:Class ;
                            rdfs:subClassOf edo:DomainAttribute ;
                            dcterms:accessRights "PUBLIC" ;
                            dcterms:identifier "PoissonRatioAt23Degrees" ;
                            skos:definition "Coeficiente de Poisson a 23 graus Celsius (Específica para Materiais Metálicos e Poliméricos)"@pt-br ,
                                            "Indicates Poisson's ratio of the material at 23 degrees Celsius, representing the ratio of transverse strain to axial strain when the material is subjected to stress. This property is essential for understanding the material's deformation behavior under load and its response to mechanical forces in subsea environments."@en ;
                            skos:prefLabel "Coeficiente de Poisson a 23 Graus Celsius"@pt-br ,
                                           "Poisson Ratio At 23 Degrees"@en ;
                            edo:hasTypedValue edo:floatValue ;
                            edo:hasValueCardinality edo:singleValue .


###  https://w3id.org/energy-domain/edo#PolymericLayerMaterialType
edo:PolymericLayerMaterialType rdf:type owl:Class ;
                               rdfs:subClassOf edo:DomainAttribute ;
                               dcterms:accessRights "PUBLIC" ;
                               dcterms:identifier "PolymericLayerMaterialType" ;
                               skos:definition "Type of material from which an object is made, allowing for precise documentation and categorisation."@en ;
                               skos:prefLabel "Polymeric Layer Material Type"@en ,
                                              "Tipo de Material da Camada Polimérica"@pt-br ;
                               edo:hasTypedValue edo:stringValue ;
                               edo:hasValueCardinality edo:singleValue .


###  https://w3id.org/energy-domain/edo#PolymericMaterial
edo:PolymericMaterial rdf:type owl:Class ;
                      rdfs:subClassOf edo:FlexibleStructureLayerMaterial ;
                      dcterms:identifier "PolymericMaterial" ;
                      skos:definition "Material made from polymers, used to fabricate flexible layers in subsea flexible pipes. Polymeric Material is selected for its properties such as flexibility, chemical resistance, and durability, making it suitable for withstanding the harsh conditions of subsea environments. These materials are commonly used in layers that provide insulation, protection, or pressure containment, ensuring the overall performance and integrity of the flexible pipe under dynamic loads and extreme underwater conditions."@en ;
                      skos:prefLabel "Material Polimérico"@pt-br ,
                                     "Polymeric Material"@en ;
                      edo:hasAttribute edo:DiffusionTable ,
                                       edo:DiffusionTable_DiffusionCoefficient ,
                                       edo:DiffusionTable_MoleculeIdentifier ,
                                       edo:DiffusionTable_PolymerState ,
                                       edo:DiffusionTable_Temperature ,
                                       edo:EModVsTempTable_ElasticityModulus ,
                                       edo:MaxPermissibleDeformationDynamic ,
                                       edo:MaxPermissibleDeformationStatic ,
                                       edo:MinimumTemperature ,
                                       edo:PermeabilityTable ,
                                       edo:PermeabilityTable_MoleculeIdentifier ,
                                       edo:PermeabilityTable_PermeabilityCoefficient ,
                                       edo:PermeabilityTable_PolymerState ,
                                       edo:PermeabilityTable_Temperature ,
                                       edo:PolymericLayerMaterialType ,
                                       edo:SolubilityTable ,
                                       edo:SolubilityTable_MoleculeIdentifier ,
                                       edo:SolubilityTable_PolymerState ,
                                       edo:SolubilityTable_SolubilityCoefficient ,
                                       edo:SolubilityTable_Temperature ;
                      edo:ifc_equivalentClass "IfcMaterial" ;
                      edo:ifc_objectType "PolymericMaterial" .


###  https://w3id.org/energy-domain/edo#PostSlippingBendingStiffness
edo:PostSlippingBendingStiffness rdf:type owl:Class ;
                                 rdfs:subClassOf edo:DomainAttribute ;
                                 dcterms:accessRights "PUBLIC" ;
                                 dcterms:identifier "PostSlippingBendingStiffness" ;
                                 skos:definition "Represents the stiffness of a component after slipping occurs during bending. This property is important for evaluating the structural response and stability of the component once it has experienced slippage, ensuring that it can still withstand bending loads without significant deformation."@en ;
                                 skos:prefLabel "Post Slipping Bending Stiffness"@en ,
                                                "Rigidez de Flexão Pós-Escorregamento"@pt-br ;
                                 edo:hasTypedValue edo:floatValue ;
                                 edo:hasValueCardinality edo:singleValue .


###  https://w3id.org/energy-domain/edo#PreCommissioning
edo:PreCommissioning rdf:type owl:Class ;
                     rdfs:subClassOf edo:LifecyclePhase ;
                     rdfs:label "Pre-Commissioning"@en ,
                                "Pré-Comissionamento"@pt-br ;
                     skos:definition "Verification and functional testing before introducing operational fluids or energy."@en ,
                                     "Verificação e testes funcionais antes da introdução de fluidos ou energia operacionais."@pt-br .


###  https://w3id.org/energy-domain/edo#PreSlippingBendingStiffness
edo:PreSlippingBendingStiffness rdf:type owl:Class ;
                                rdfs:subClassOf edo:DomainAttribute ;
                                dcterms:accessRights "PUBLIC" ;
                                dcterms:identifier "PreSlippingBendingStiffness" ;
                                skos:definition "Represents the stiffness of a component before any slipping occurs during bending. This property is important for assessing how the component resists bending forces prior to slippage, ensuring that it maintains its shape and performance under load."@en ;
                                skos:prefLabel "Pre Slipping Bending Stiffness"@en ,
                                               "Rigidez de Flexão Pré-Escorregamento"@pt-br ;
                                edo:hasTypedValue edo:floatValue ;
                                edo:hasValueCardinality edo:singleValue .


###  https://w3id.org/energy-domain/edo#PressureArmour
edo:PressureArmour rdf:type owl:Class ;
                   rdfs:subClassOf edo:CarcassLayer ;
                   dcterms:identifier "PressureArmour" ;
                   skos:definition "A high-strength, metallic layer used in subsea flexible pipes to provide resistance against both internal and external pressure. The Pressure Armour prevents the pipe from expanding under high internal pressures and protects against collapse due to external pressure. Typically made from helically wound steel or other strong materials, it supports the pipe's structural integrity and ensures reliable operation in harsh subsea environments."@en ;
                   skos:prefLabel "Armadura de Pressão"@pt-br ,
                                  "Pressure Armour"@en ;
                   edo:ifc_equivalentClass "IfcPipeSegment" ;
                   edo:ifc_objectType "PressureArmour" ;
                   edo:ifc_predefinedType "USERDEFINED" .


###  https://w3id.org/energy-domain/edo#ProcessEngineering
edo:ProcessEngineering rdf:type owl:Class ;
                       rdfs:subClassOf edo:TechnicalDiscipline ;
                       rdfs:label "Engenharia de Processos"@pt-br ,
                                  "Process Engineering"@en ;
                       skos:definition "Disciplina de engenharia focada no projeto e otimização de processos industriais."@pt-br ,
                                       "Engineering discipline focused on the design and optimization of industrial processes."@en .


###  https://w3id.org/energy-domain/edo#ProcessPipingEngineering
edo:ProcessPipingEngineering rdf:type owl:Class ;
                             rdfs:subClassOf edo:TechnicalDiscipline ;
                             rdfs:label "Engenharia de Tubulação de Processo"@pt-br ,
                                        "Process Piping Engineering"@en ;
                             skos:definition "Disciplina de engenharia focada no projeto de sistemas de tubulação para fluidos de processo."@pt-br ,
                                             "Engineering discipline focused on the design of piping systems for process fluids."@en .


###  https://w3id.org/energy-domain/edo#Procurement
edo:Procurement rdf:type owl:Class ;
                rdfs:subClassOf edo:LifecyclePhase ;
                rdfs:label "Aquisição"@pt-br ,
                           "Procurement"@en ;
                skos:definition "Acquisition of materials, equipment, and services required for project execution."@en ,
                                "Aquisição de materiais, equipamentos e serviços necessários para execução do projeto."@pt-br .


###  https://w3id.org/energy-domain/edo#Project
edo:Project rdf:type owl:Class ;
            rdfs:subClassOf edo:DomainElement ;
            dcterms:identifier "Project" ;
            skos:definition "A broad concept that encompasses the design, development, and planning of various components or systems."@en ;
            skos:prefLabel "Project"@en ,
                           "Projeto"@pt-br ;
            edo:ifc_equivalentClass "IfcProject" .


###  https://w3id.org/energy-domain/edo#ProjectAcronym
edo:ProjectAcronym rdf:type owl:Class ;
                   rdfs:subClassOf edo:DomainAttribute ;
                   dcterms:accessRights "PUBLIC" ;
                   dcterms:identifier "ProjectAcronym" ;
                   skos:definition "Abreviação do nome do projeto da Interligação Submarina. Ex., 'SEP' para o \"FPSO Carioca do campo de Sépia\""@pt-br ,
                                   "Indicates the unique identification code assigned to the operator's project. This property is used for tracking, managing, and referencing the project throughout all phases of its lifecycle, ensuring proper identification and organization."@en ;
                   skos:prefLabel "Abreviação do Nome do Projeto da Interligação Submarina"@pt-br ,
                                  "Project Acronym"@en ;
                   edo:hasTypedValue edo:stringValue ;
                   edo:hasValueCardinality edo:singleValue .


###  https://w3id.org/energy-domain/edo#ProjectCode
edo:ProjectCode rdf:type owl:Class ;
                rdfs:subClassOf edo:DomainAttribute ;
                dcterms:accessRights "PUBLIC" ;
                dcterms:identifier "ProjectCode" ;
                skos:definition "Unique identification code assigned to the operator's project, used for tracking, managing, and referencing the project across all phases of its lifecycle."@en ;
                skos:prefLabel "Código Identificador único do projeto da operadora da Interligação Submarina"@pt-br ,
                               "Project Code"@en ;
                edo:hasTypedValue edo:stringValue ;
                edo:hasValueCardinality edo:singleValue .


###  https://w3id.org/energy-domain/edo#ProjectDrawingCode
edo:ProjectDrawingCode rdf:type owl:Class ;
                       rdfs:subClassOf edo:DomainAttribute ;
                       dcterms:accessRights "PUBLIC" ;
                       dcterms:identifier "ProjectDrawingCode" ;
                       skos:definition "Indicates the unique alphanumeric code assigned to the project drawing. This property is used to reference and locate the specific drawing associated with the item, providing a clear and organized method for tracking and accessing drawing documents."@en ,
                                       "Número do desenho do projeto do acessório"@pt-br ;
                       skos:prefLabel "Número do Desenho do Projeto"@pt-br ,
                                      "Project Drawing Code"@en ;
                       edo:hasTypedValue edo:stringValue ;
                       edo:hasValueCardinality edo:singleValue .


###  https://w3id.org/energy-domain/edo#ProjectDrawingRevision
edo:ProjectDrawingRevision rdf:type owl:Class ;
                           rdfs:subClassOf edo:DomainAttribute ;
                           dcterms:accessRights "PUBLIC" ;
                           dcterms:identifier "ProjectDrawingRevision" ;
                           skos:definition "Indicates the revision number or identifier of the project drawing. This property tracks the version of the drawing, providing essential information for identifying updates, changes, and the most current version of the drawing related to the item."@en ;
                           skos:prefLabel "Project Drawing Revision"@en ,
                                          "Revisão do Desenho do Projeto"@pt-br ;
                           edo:hasTypedValue edo:stringValue ;
                           edo:hasValueCardinality edo:singleValue .


###  https://w3id.org/energy-domain/edo#ProtectiveSheath
edo:ProtectiveSheath rdf:type owl:Class ;
                     rdfs:subClassOf edo:SolidLayer ;
                     dcterms:identifier "ProtectiveSheath" ;
                     skos:definition "A layer in subsea flexible pipes designed to shield internal components from external environmental factors such as abrasion, mechanical damage, or chemical exposure. The Protective Sheath serves as the outermost barrier, providing defense against harsh subsea conditions while preserving the integrity of the underlying layers. Typically made from durable polymeric materials, it plays a critical role in extending the lifespan of the flexible pipe by protecting it from physical and chemical wear."@en ;
                     skos:prefLabel "Capa de Proteção"@pt-br ,
                                    "Protective Sheath"@en ;
                     edo:ifc_equivalentClass "IfcPipeSegment" ;
                     edo:ifc_objectType "ProtectiveSheath" ;
                     edo:ifc_predefinedType "USERDEFINED" .


###  https://w3id.org/energy-domain/edo#PullInCollar
edo:PullInCollar rdf:type owl:Class ;
                 rdfs:subClassOf edo:SplitCollar ;
                 dcterms:identifier "PullInCollar" ;
                 skos:altLabel "Installation Collar"@en ,
                               "Pull-In Clamp"@en ,
                               "Pulling Collar"@en ,
                               "Tension Collar"@en ;
                 skos:definition "A device used in subsea operations to assist in the installation of flexible pipes or risers by providing a secure attachment point for pulling the pipe into position. The Pull In Collar is typically installed around the pipe and serves as a handling point for pulling equipment during installation. It ensures a controlled and secure method of pulling the pipe into place, preventing damage to the pipe while facilitating smooth and efficient installation in subsea environments."@en ;
                 skos:prefLabel "Colar de Pull In"@pt-br ,
                                "Pull In Collar"@en ;
                 edo:hasAttribute edo:WireRopeQuantity ,
                                  edo:WireRopeSlingDiameter ,
                                  edo:WireRopeSlingLength ;
                 edo:ifc_equivalentClass "IfcPipeFitting" ;
                 edo:ifc_objectType "PullInCollar" ;
                 edo:ifc_predefinedType "USERDEFINED" .


###  https://w3id.org/energy-domain/edo#PullingHead
edo:PullingHead rdf:type owl:Class ;
                rdfs:subClassOf edo:LineAncillary ;
                dcterms:identifier "PullingHead" ;
                skos:altLabel "Cable Head"@en ,
                              "Installation Head"@en ,
                              "Pulling Grip"@en ,
                              "Pulling Tool"@en ;
                skos:definition "A component used in subsea flexible pipe installations to provide a secure attachment point for pulling the pipe into position during installation or retrieval operations. The Pulling Head is fitted to the end of the flexible pipe, allowing connection to pulling equipment such as winches or cranes. It is designed to withstand high loads, ensuring that the pipe can be pulled safely without causing damage. The Pulling Head is essential for handling, testing, and securing the pipe in place during subsea installation."@en ;
                skos:prefLabel "Cabeça de Tração"@pt-br ,
                               "Pulling Head"@en .


###  https://w3id.org/energy-domain/edo#PullingHeadType
edo:PullingHeadType rdf:type owl:Class ;
                    rdfs:subClassOf edo:DomainAttribute ;
                    dcterms:accessRights "PUBLIC" ;
                    dcterms:identifier "PullingHeadType" ;
                    skos:definition "Specifies the type of pulling head used for the installation or retrieval of subsea flexible structures. It describes the design and functionality of the pulling head, including details such as compatibility with specific installation methods, mechanical connections, and any special features or adaptations for handling loads during pulling operations. This property helps to ensure the correct pulling head is selected based on the requirements of the project and the conditions of the installation site."@en ;
                    skos:prefLabel "Pulling Head Type"@en ,
                                   "Tipo de Cabeça de Tração"@pt-br ;
                    edo:hasTypedValue edo:stringValue ;
                    edo:hasValueCardinality edo:singleValue .


###  https://w3id.org/energy-domain/edo#Quantity
edo:Quantity rdf:type owl:Class ;
             rdfs:subClassOf edo:DomainAttribute ;
             dcterms:accessRights "PUBLIC" ;
             dcterms:identifier "Quantity" ;
             skos:definition "Quantity of items."@en ;
             skos:prefLabel "Quantidade de Itens"@pt-br ,
                            "Quantity"@en ;
             edo:hasTypedValue edo:intValue ;
             edo:hasValueCardinality edo:singleValue .


###  https://w3id.org/energy-domain/edo#Recycling
edo:Recycling rdf:type owl:Class ;
              rdfs:subClassOf edo:LifecyclePhase ;
              rdfs:label "Reciclagem"@pt-br ,
                         "Recycling"@en ;
              skos:definition "Processamento e reutilização de materiais recuperados durante o descomissionamento."@pt-br ,
                              "Processing and reusing materials recovered during decommissioning."@en .


###  https://w3id.org/energy-domain/edo#ReferenceDrawing
edo:ReferenceDrawing rdf:type owl:Class ;
                     rdfs:subClassOf edo:DomainElement ;
                     dcterms:identifier "ReferenceDrawing" ;
                     skos:definition "A technical drawing providing detailed information about a specific component, system, or assembly, used as a guide for manufacturing, installation, or maintenance in subsea projects."@en ;
                     skos:prefLabel "Desenhos de Referência"@pt-br ,
                                    "Reference Drawing"@en .


###  https://w3id.org/energy-domain/edo#Renewable
edo:Renewable rdf:type owl:Class ;
              rdfs:subClassOf edo:Domain ;
              rdfs:label "Energia Renovável"@pt-br ,
                         "Renewable Energy"@en ;
              skos:definition "Domínio industrial que abrange fontes de energia que são naturalmente reabastecidas, como solar, eólica e hidrelétrica."@pt-br ,
                              "Industrial domain covering energy sources that are naturally replenished, such as solar, wind, and hydropower."@en .


###  https://w3id.org/energy-domain/edo#RingGasket
edo:RingGasket rdf:type owl:Class ;
               rdfs:subClassOf edo:PhysicalConnection ;
               dcterms:identifier "RingGasket" ;
               skos:altLabel " Seal Ring"@en ,
                             "Gasket"@en ,
                             "O-Ring"@en ,
                             "Packing Ring"@en ,
                             "Seal Gasket"@en ,
                             "Sealing Ring"@en ;
               skos:definition "The seal ring is a crucial component used in subsea oil and gas interconnection end fittings to ensure a secure and leak-proof connection between pipes or equipment. Typically made from high-performance materials such as elastomers or metals, the seal ring is designed to withstand extreme pressure, temperature, and environmental conditions found in subsea operations. It is installed within the end fitting to create a reliable seal that prevents fluid leakage and maintains the integrity of the interconnection. The seal ring’s precise design and material selection are essential for ensuring long-term durability and performance in harsh subsea environments."@en ;
               skos:prefLabel "Junta de Conexão"@pt-br ,
                              "Ring Gasket"@en ;
               edo:hasAttribute edo:RingGasketInnerDIameter ,
                                edo:RingGasketMaterial ,
                                edo:RingGasketOuterDiameter ,
                                edo:RingGasketPressureRating ,
                                edo:RingGasketSpecification ,
                                edo:RingGasketStandard ,
                                edo:RingGasketType ;
               edo:ifc_equivalentClass "IfcMechanicalFastener" ;
               edo:ifc_objectType "RingGasket" ;
               edo:ifc_predefinedType "USERDEFINED" .


###  https://w3id.org/energy-domain/edo#RingGasketInnerDIameter
edo:RingGasketInnerDIameter rdf:type owl:Class ;
                            rdfs:subClassOf edo:DomainAttribute ;
                            dcterms:accessRights "PUBLIC" ;
                            dcterms:identifier "RingGasketInnerDIameter" ;
                            skos:definition "The internal diameter, which determines the size of the bore it fits into. This dimension is crucial for ensuring a proper fit and effective sealing."@en ;
                            skos:prefLabel "Diâmetro Interno da Junta de Vedação"@pt-br ,
                                           "Ring Gasket Inner Diameter"@en ;
                            edo:hasTypedValue edo:floatValue ;
                            edo:hasValueCardinality edo:singleValue .


###  https://w3id.org/energy-domain/edo#RingGasketMaterial
edo:RingGasketMaterial rdf:type owl:Class ;
                       rdfs:subClassOf edo:DomainAttribute ;
                       dcterms:accessRights "PUBLIC" ;
                       dcterms:identifier "RingGasketMaterial" ;
                       skos:definition "Type of material from which an object is made, allowing for precise documentation and categorisation."@en ;
                       skos:prefLabel "Material da Junta de Vedação"@pt-br ,
                                      "Ring Gasket Material"@en ;
                       edo:hasTypedValue edo:stringValue ;
                       edo:hasValueCardinality edo:singleValue .


###  https://w3id.org/energy-domain/edo#RingGasketOuterDiameter
edo:RingGasketOuterDiameter rdf:type owl:Class ;
                            rdfs:subClassOf edo:DomainAttribute ;
                            dcterms:accessRights "PUBLIC" ;
                            dcterms:identifier "RingGasketOuterDiameter" ;
                            skos:definition "The external diameter, which determines the size of the surface it seals against. This dimension is essential for providing a secure seal and preventing leakage."@en ;
                            skos:prefLabel "Diâmetro Externo da Junta de Vedação"@pt-br ,
                                           "Ring Gasket Outer Diameter"@en ;
                            edo:hasTypedValue edo:floatValue ;
                            edo:hasValueCardinality edo:singleValue .


###  https://w3id.org/energy-domain/edo#RingGasketPressureRating
edo:RingGasketPressureRating rdf:type owl:Class ;
                             rdfs:subClassOf edo:DomainAttribute ;
                             dcterms:accessRights "PUBLIC" ;
                             dcterms:identifier "RingGasketPressureRating" ;
                             skos:definition "The maximum pressure it can withstand without failing. This rating is important for ensuring that the seal ring performs effectively under the operating pressures of the application."@en ;
                             skos:prefLabel "Classificação de Pressão da Junta de Vedação"@pt-br ,
                                            "Ring Gasket Pressure Rating"@en ;
                             edo:hasTypedValue edo:floatValue ;
                             edo:hasValueCardinality edo:singleValue .


###  https://w3id.org/energy-domain/edo#RingGasketSpecification
edo:RingGasketSpecification rdf:type owl:Class ;
                            rdfs:subClassOf edo:DomainAttribute ;
                            dcterms:accessRights "PUBLIC" ;
                            dcterms:identifier "RingGasketSpecification" ;
                            skos:definition "The detailed description of it's design and performance characteristics, including material, size, and pressure rating. This provides comprehensive information about the seal ring's suitability for specific applications."@en ;
                            skos:prefLabel "Especificação da Junta de Vedação"@pt-br ,
                                           "Ring Gasket Specification"@en ;
                            edo:hasTypedValue edo:stringValue ;
                            edo:hasValueCardinality edo:singleValue .


###  https://w3id.org/energy-domain/edo#RingGasketStandard
edo:RingGasketStandard rdf:type owl:Class ;
                       rdfs:subClassOf edo:DomainAttribute ;
                       dcterms:accessRights "PUBLIC" ;
                       dcterms:identifier "RingGasketStandard" ;
                       skos:definition "The standard or specification it conforms to, such as API, ISO, or other industry standards. This indicates the compliance of the seal ring with established guidelines for quality and performance."@en ;
                       skos:prefLabel "Padrão da Junta de Vedação"@pt-br ,
                                      "Ring Gasket Standard"@en ;
                       edo:hasTypedValue edo:stringValue ;
                       edo:hasValueCardinality edo:singleValue .


###  https://w3id.org/energy-domain/edo#RingGasketType
edo:RingGasketType rdf:type owl:Class ;
                   rdfs:subClassOf edo:DomainAttribute ;
                   dcterms:accessRights "PUBLIC" ;
                   dcterms:identifier "RingGasketType" ;
                   skos:definition "The specific type or design. This classification helps identify the appropriate seal ring based on its design and application requirements, ensuring it meets the sealing needs under various conditions."@en ;
                   skos:prefLabel "Ring Gasket Type"@en ,
                                  "Tipo de Junta de Vedação"@pt-br ;
                   edo:hasTypedValue edo:stringValue ;
                   edo:hasValueCardinality edo:singleValue .


###  https://w3id.org/energy-domain/edo#RiserBalcony
edo:RiserBalcony rdf:type owl:Class ;
                 rdfs:subClassOf edo:Location ;
                 dcterms:identifier "RiserBalcony" ;
                 skos:definition "Installation location for supports and accessories on the riser balcony of the production unit."@en ;
                 skos:prefLabel "Plataforma do Riser"@pt-br ,
                                "Riser Balcony"@en .


###  https://w3id.org/energy-domain/edo#RiserConfiguration
edo:RiserConfiguration rdf:type owl:Class ;
                       rdfs:subClassOf edo:DomainAttribute ;
                       dcterms:accessRights "PUBLIC" ;
                       dcterms:identifier "RiserConfiguration" ;
                       skos:definition "This property specifies the configuration type for the riser section of the pipeline. It provides key information on the structural design, indicating the arrangement and dynamic behaviour of the riser system. The chosen configuration affects how the structure responds to environmental forces, such as currents and pressure, and plays a critical role in determining the overall performance and durability of the system."@en ;
                       skos:prefLabel "Configuração do Riser"@pt-br ,
                                      "Riser Configuration"@en ;
                       edo:hasTypedValue edo:stringValue ;
                       edo:hasValueCardinality edo:singleValue .


###  https://w3id.org/energy-domain/edo#RiserSpan
edo:RiserSpan rdf:type owl:Class ;
              rdfs:subClassOf edo:PipelineSpan ;
              dcterms:identifier "RiserSpan" .


###  https://w3id.org/energy-domain/edo#RiserSupport
edo:RiserSupport rdf:type owl:Class ;
                 rdfs:subClassOf edo:Component ;
                 dcterms:identifier "RiserSupport" .


###  https://w3id.org/energy-domain/edo#RotatingEquipmentEngineering
edo:RotatingEquipmentEngineering rdf:type owl:Class ;
                                 rdfs:subClassOf edo:EquipmentEngineering ;
                                 rdfs:label "Engenharia de Equipamentos Rotativos"@pt-br ,
                                            "Rotating Equipment Engineering"@en ;
                                 skos:definition "Engenharia de equipamentos mecânicos com componentes rotativos como bombas, compressores e turbinas."@pt-br ,
                                                 "Engineering of mechanical equipment with rotating components such as pumps, compressors, and turbines."@en .


###  https://w3id.org/energy-domain/edo#RuptDefAlongFibers
edo:RuptDefAlongFibers rdf:type owl:Class ;
                       rdfs:subClassOf edo:DomainAttribute ;
                       dcterms:accessRights "PUBLIC" ;
                       dcterms:identifier "RuptDefAlongFibers" ;
                       skos:definition "Describes the deformation that occurs when the composite material ruptures in a direction parallel to its fibers. This property is essential for assessing the material's behavior under stress aligned with the fiber orientation, providing insights into its performance and durability in subsea structures where axial forces are present."@en ;
                       skos:prefLabel "Deformação de Ruptura longitudinalmente às fibras"@pt-br ,
                                      "Rupture Deformation Along Fibers"@en ;
                       edo:hasTypedValue edo:floatValue ;
                       edo:hasValueCardinality edo:singleValue .


###  https://w3id.org/energy-domain/edo#RuptDefPerpendFibers
edo:RuptDefPerpendFibers rdf:type owl:Class ;
                         rdfs:subClassOf edo:DomainAttribute ;
                         dcterms:accessRights "PUBLIC" ;
                         dcterms:identifier "RuptDefPerpendFibers" ;
                         skos:definition "Describes the deformation that occurs when the composite material ruptures in a direction perpendicular to its fibers. This property is crucial for understanding the material's behavior under stress conditions that do not align with the fiber orientation, helping to assess its performance and failure limits in subsea structures."@en ;
                         skos:prefLabel "Deformação de Ruptura perpendicularmente às fibras"@pt-br ,
                                        "Rupture Deformation Perpendicular To Fibers"@en ;
                         edo:hasTypedValue edo:floatValue ;
                         edo:hasValueCardinality edo:singleValue .


###  https://w3id.org/energy-domain/edo#SacrificialSheath
edo:SacrificialSheath rdf:type owl:Class ;
                      rdfs:subClassOf edo:SolidLayer ;
                      dcterms:identifier "SacrificialSheath" ;
                      skos:definition "A protective layer in subsea flexible pipes designed to absorb damage from external environmental factors, such as abrasion or impact, over time. The Sacrificial Sheath is intended to wear out or degrade under harsh conditions, thereby preserving the integrity of the underlying layers and prolonging the overall lifespan of the pipe. Made from durable materials, this sheath acts as the first line of defense, allowing for the controlled degradation of the pipe's outer surface without affecting its core structural or functional performance."@en ;
                      skos:prefLabel "Camada de Sacrifício"@pt-br ,
                                     "Sacrificial Sheath"@en ;
                      edo:ifc_equivalentClass "IfcPipeSegment" ;
                      edo:ifc_objectType "SacrificialSheath" ;
                      edo:ifc_predefinedType "USERDEFINED" .


###  https://w3id.org/energy-domain/edo#SafeWorkingLoad
edo:SafeWorkingLoad rdf:type owl:Class ;
                    rdfs:subClassOf edo:DomainAttribute ;
                    dcterms:accessRights "PUBLIC" ;
                    dcterms:identifier "SafeWorkingLoad" ;
                    skos:definition "Safe Working Load (SWL) refers to the maximum load that can be safely handled under normal operating conditions. This value ensures the equipment operates within its designed capacity, preventing overloading and potential failure."@en ;
                    skos:prefLabel "Carga Máxima Segura de Trabalho"@pt-br ,
                                   "Safe Working Load"@en ;
                    edo:hasTypedValue edo:floatValue ;
                    edo:hasValueCardinality edo:singleValue .


###  https://w3id.org/energy-domain/edo#SafetyLossPreventionEngineering
edo:SafetyLossPreventionEngineering rdf:type owl:Class ;
                                    rdfs:subClassOf edo:TechnicalDiscipline ;
                                    rdfs:label "Engenharia de Segurança e Prevenção de Perdas"@pt-br ,
                                               "Safety & Loss Prevention Engineering"@en ;
                                    skos:definition "Disciplina de engenharia focada em avaliação de riscos, sistemas de segurança e prevenção de perdas."@pt-br ,
                                                    "Engineering discipline focused on risk assessment, safety systems and loss prevention."@en .


###  https://w3id.org/energy-domain/edo#SerialNumber
edo:SerialNumber rdf:type owl:Class ;
                 rdfs:subClassOf edo:DomainAttribute ;
                 dcterms:accessRights "PUBLIC" ;
                 dcterms:identifier "SerialNumber" ;
                 skos:definition "A unique identifier assigned to each individual item, distinguishing it from all other units of the same type. The Serial Number is critical for traceability, maintenance, and warranty purposes, ensuring that the history, performance, and lifecycle of the equipment can be tracked. It is often used in conjunction with a Part Number, which identifies the type or model of the component."@en ;
                 skos:prefLabel "Número de Série"@pt-br ,
                                "Serial Number"@en ;
                 edo:hasTypedValue edo:stringValue ;
                 edo:hasValueCardinality edo:singleValue .


###  https://w3id.org/energy-domain/edo#Service
edo:Service rdf:type owl:Class ;
            rdfs:subClassOf edo:DomainAttribute ;
            dcterms:accessRights "PUBLIC" ;
            dcterms:identifier "Service" ;
            skos:definition "Escolha um da lista: IA (Injeção de água); IG (Injeção de Gás); LPO (Linha de Produção de Óleo); PG (Produtor de Gás); SE (Serviço); GAS (Gasoduto); UEH (Umbilical Eletro Hidráulico); CEP (Cabo Elétrico de Potência)"@pt-br ,
                            "Indicates the type of service the pipeline is designated for, specifying its operational purpose within the project. This classification is used to ensure proper management, installation, and use of the pipeline according to its intended function."@en ;
            skos:prefLabel "Indica o Tipo de Serviço"@pt-br ,
                           "Indicates the Type of Service"@en ;
            edo:hasTypedValue edo:stringValue ;
            edo:hasValueCardinality edo:singleValue .


###  https://w3id.org/energy-domain/edo#Shackle
edo:Shackle rdf:type owl:Class ;
            rdfs:subClassOf edo:MooringAccessory ;
            dcterms:identifier "Shackle" ;
            skos:altLabel "Anchor Shackle"@en ,
                          "Bow Shackle"@en ,
                          "Clevis"@en ,
                          "D-Shackle"@en ,
                          "U-Bolt"@en ;
            skos:definition "A device used to connect and secure components in subsea systems, particularly during lifting, handling, or mooring operations. The Shackle typically consists of a U-shaped metal piece with a removable pin or bolt, allowing it to link components such as chains, slings, or cables. It provides a strong and reliable connection point, ensuring that loads can be safely transferred or lifted without risk of detachment or failure. Shackles are essential for securing flexible lines and other equipment during installation and maintenance in subsea environments."@en ;
            skos:prefLabel "Manilha"@pt-br ,
                           "Shackle"@en ;
            edo:hasAttribute edo:ShackleInnerDiameter ,
                             edo:ShackleOpeningWidth ,
                             edo:ShackleOuterDiameter ,
                             edo:ShackleThickness ,
                             edo:WorkingLoadLimit ;
            edo:ifc_equivalentClass "IfcMechanicalFastener" ;
            edo:ifc_objectType "Shackle" ;
            edo:ifc_predefinedType "USERDEFINED" .


###  https://w3id.org/energy-domain/edo#ShackleInnerDiameter
edo:ShackleInnerDiameter rdf:type owl:Class ;
                         rdfs:subClassOf edo:DomainAttribute ;
                         dcterms:accessRights "PUBLIC" ;
                         dcterms:identifier "ShackleInnerDiameter" ;
                         skos:definition "Indicates the inner diameter of the shackle. This property measures the width of the space inside the shackle, which is important for ensuring compatibility with other components and for determining the appropriate fit and load distribution."@en ;
                         skos:prefLabel "Diâmetro interno da furação do olhal"@pt-br ,
                                        "Shackle Inner Diameter"@en ;
                         edo:hasTypedValue edo:floatValue ;
                         edo:hasValueCardinality edo:singleValue .


###  https://w3id.org/energy-domain/edo#ShackleOpeningWidth
edo:ShackleOpeningWidth rdf:type owl:Class ;
                        rdfs:subClassOf edo:DomainAttribute ;
                        dcterms:accessRights "PUBLIC" ;
                        dcterms:identifier "ShackleOpeningWidth" ;
                        skos:definition "Measures the width of the opening in the shackle where components, such as pins or cables, are inserted. This property is crucial for ensuring that the shackle can properly accommodate and secure the intended connecting elements."@en ;
                        skos:prefLabel "Largura da Abertura"@pt-br ,
                                       "Shackle Opening Width"@en ;
                        edo:hasTypedValue edo:floatValue ;
                        edo:hasValueCardinality edo:singleValue .


###  https://w3id.org/energy-domain/edo#ShackleOuterDiameter
edo:ShackleOuterDiameter rdf:type owl:Class ;
                         rdfs:subClassOf edo:DomainAttribute ;
                         dcterms:accessRights "PUBLIC" ;
                         dcterms:identifier "ShackleOuterDiameter" ;
                         skos:definition "Indicates the outer diameter of the shackle. This property provides the measurement of the overall width of the shackle, which is crucial for ensuring it fits properly with other components and meets the design specifications for load-bearing and connection requirements."@en ;
                         skos:prefLabel "Diâmetro externo do olhal"@pt-br ,
                                        "Shackle Outer Diameter"@en ;
                         edo:hasTypedValue edo:floatValue ;
                         edo:hasValueCardinality edo:singleValue .


###  https://w3id.org/energy-domain/edo#ShackleThickness
edo:ShackleThickness rdf:type owl:Class ;
                     rdfs:subClassOf edo:DomainAttribute ;
                     dcterms:accessRights "PUBLIC" ;
                     dcterms:identifier "ShackleThickness" ;
                     skos:definition "Specifies the thickness of the shackle material. This property measures the distance between the inner and outer surfaces of the shackle, which is essential for understanding its strength, durability, and ability to handle load stresses."@en ;
                     skos:prefLabel "Espessura do olhal"@pt-br ,
                                    "Shackle Thickness"@en ;
                     edo:hasTypedValue edo:floatValue ;
                     edo:hasValueCardinality edo:singleValue .


###  https://w3id.org/energy-domain/edo#ShortTermFloatDensity
edo:ShortTermFloatDensity rdf:type owl:Class ;
                          rdfs:subClassOf edo:DomainAttribute ;
                          dcterms:accessRights "PUBLIC" ;
                          dcterms:identifier "ShortTermFloatDensity" ;
                          skos:definition "Representa a densidade do flutuador logo após o início da operação, considerando um aumento de densidade devido à absorção de água em pequena quantidade ou outras alterações superficiais."@pt-br ,
                                          "The density of the float material in the early stages of operation, accounting for slight water absorption or other surface-level changes."@en ;
                          skos:prefLabel "Densidade do Flutuador a Curto Prazo"@pt-br ,
                                         "Short Term Float Density"@en ;
                          edo:hasTypedValue edo:floatValue ;
                          edo:hasValueCardinality edo:singleValue .


###  https://w3id.org/energy-domain/edo#ShortTermFloatVolume
edo:ShortTermFloatVolume rdf:type owl:Class ;
                         rdfs:subClassOf edo:DomainAttribute ;
                         dcterms:accessRights "PUBLIC" ;
                         dcterms:identifier "ShortTermFloatVolume" ;
                         skos:definition "O volume submerso esperado logo após o início da operação, levando em consideração pequenas variações iniciais, como a absorção mínima de água ou pequenas deformações. Serve para calcular a flutuabilidade em condições reais no curto prazo."@pt-br ,
                                         "The expected submerged volume of the float during the initial phase of operation, considering minor factors like slight water absorption or small deformations."@en ;
                         skos:prefLabel "Short Term Float Volume"@en ,
                                        "Volume do Flutuador a Curto Prazo"@pt-br ;
                         edo:hasTypedValue edo:floatValue ;
                         edo:hasValueCardinality edo:singleValue .


###  https://w3id.org/energy-domain/edo#Solar
edo:Solar rdf:type owl:Class ;
          rdfs:subClassOf edo:Renewable ;
          rdfs:label "Energia Solar"@pt-br ,
                     "Solar Energy"@en ;
          skos:definition "Energia obtida da luz solar, incluindo sistemas fotovoltaicos e térmicos."@pt-br ,
                          "Energy harnessed from sunlight, including photovoltaic and thermal systems."@en .


###  https://w3id.org/energy-domain/edo#SolidLayer
edo:SolidLayer rdf:type owl:Class ;
               rdfs:subClassOf edo:FlexibleStructureLayer ;
               dcterms:identifier "SolidLayer" ;
               skos:definition "Camada maciça formada por extrusão contínua de um material"@pt-br ,
                               "Continuous layer used in subsea flexible pipes or similar structures, typically fabricated through extrusion. It provides structural reinforcement, pressure containment, or environmental protection, ensuring the integrity and performance of the pipe by offering consistent support or shielding."@en ;
               skos:prefLabel "Camada Sólida"@pt-br ,
                              "Solid Layer"@en .


###  https://w3id.org/energy-domain/edo#SolubilityTable
edo:SolubilityTable rdf:type owl:Class ;
                    rdfs:subClassOf edo:DomainAttribute ;
                    dcterms:accessRights "PUBLIC" ;
                    dcterms:identifier "SolubilityTable" ;
                    skos:definition "Provides data on the solubility of various substances in a material, used to evaluate how different fluids or gases dissolve into the structure. This information is essential for assessing material compatibility and predicting the effects of prolonged exposure to specific substances under operational conditions."@en ;
                    skos:prefLabel "Solubility Table (Specific for Polymeric Materials)"@en ,
                                   "Tabela de Solubilidade (Específica para Materiais Poliméricos)"@pt-br .


###  https://w3id.org/energy-domain/edo#SolubilityTable_MoleculeIdentifier
edo:SolubilityTable_MoleculeIdentifier rdf:type owl:Class ;
                                       rdfs:subClassOf edo:DomainAttribute ;
                                       dcterms:accessRights "PUBLIC" ;
                                       dcterms:identifier "SolubilityTable_MoleculeIdentifier" ;
                                       skos:definition "Specifies the type of molecule. This property identifies the particular molecule involved, which is crucial for understanding the material's interaction with or response to different chemical substances."@en ,
                                                       "Tipo de Molécula (co2, h2s, ch4, h2o,…)"@pt-br ;
                                       skos:prefLabel "Identificador de Molécula"@pt-br ,
                                                      "Molecule Identifier"@en ;
                                       edo:hasTypedValue edo:stringValue ;
                                       edo:hasValueCardinality edo:multiValue .


###  https://w3id.org/energy-domain/edo#SolubilityTable_PolymerState
edo:SolubilityTable_PolymerState rdf:type owl:Class ;
                                 rdfs:subClassOf edo:DomainAttribute ;
                                 dcterms:accessRights "PUBLIC" ;
                                 dcterms:identifier "SolubilityTable_PolymerState" ;
                                 skos:definition "The state of the polymeric material is specified.. This property is crucial for understanding how the material behaves under different conditions and its suitability for various applications."@en ;
                                 skos:prefLabel "Estado do Polímero"@pt-br ,
                                                "Polymer State"@en ;
                                 edo:hasTypedValue edo:stringValue ;
                                 edo:hasValueCardinality edo:multiValue .


###  https://w3id.org/energy-domain/edo#SolubilityTable_SolubilityCoefficient
edo:SolubilityTable_SolubilityCoefficient rdf:type owl:Class ;
                                          rdfs:subClassOf edo:DomainAttribute ;
                                          dcterms:accessRights "PUBLIC" ;
                                          dcterms:identifier "SolubilityTable_SolubilityCoefficient" ;
                                          skos:definition "Represents the rate at which a substance dissolves in a specific material, indicating how much of the substance can be absorbed by the material. This property is important for understanding the material's chemical compatibility and behavior when exposed to various substances."@en ;
                                          skos:prefLabel "Coeficiente de solubilidade"@pt-br ,
                                                         "Solubility Coefficient"@en ;
                                          edo:hasTypedValue edo:floatValue ;
                                          edo:hasValueCardinality edo:multiValue .


###  https://w3id.org/energy-domain/edo#SolubilityTable_Temperature
edo:SolubilityTable_Temperature rdf:type owl:Class ;
                                rdfs:subClassOf edo:DomainAttribute ;
                                dcterms:accessRights "PUBLIC" ;
                                dcterms:identifier "SolubilityTable_Temperature" ;
                                skos:definition "Represents the thermal condition or measurement of heat for a component or system. This property is important for assessing how the component performs or operates under specific thermal conditions, ensuring it remains within safe and effective operating limits."@en ;
                                skos:prefLabel "Temperatura"@pt-br ,
                                               "Temperature"@en ;
                                edo:hasTypedValue edo:floatValue ;
                                edo:hasValueCardinality edo:multiValue .


###  https://w3id.org/energy-domain/edo#SpareQuantity
edo:SpareQuantity rdf:type owl:Class ;
                  rdfs:subClassOf edo:DomainAttribute ;
                  dcterms:accessRights "PUBLIC" ;
                  dcterms:identifier "SpareQuantity" ;
                  skos:definition "Specifies the number of spare units available, ensuring adequate backup components are on hand for maintenance or replacement. This quantity helps in planning and minimizing downtime during operations."@en ;
                  skos:prefLabel "Quantidade de Sobressalentes"@pt-br ,
                                 "Spare Quantity"@en ;
                  edo:hasTypedValue edo:intValue ;
                  edo:hasValueCardinality edo:singleValue .


###  https://w3id.org/energy-domain/edo#SpecialRequirements
edo:SpecialRequirements rdf:type owl:Class ;
                        rdfs:subClassOf edo:DomainAttribute ;
                        dcterms:accessRights "PUBLIC" ;
                        dcterms:identifier "SpecialRequirements" ;
                        skos:definition "Requisitos especiais, Observações ou Documentos especiais para o tramo"@pt-br ,
                                        "Special requirements refer to specific conditions, standards, or instructions that must be met during the design, manufacturing, installation, or operation of an object or system. These can include unique technical specifications, safety measures, regulatory compliance, or client-specific requests that go beyond standard procedures."@en ;
                        skos:prefLabel "Requisitos Especiais"@pt-br ,
                                       "Special Requirements"@en ;
                        edo:hasTypedValue edo:stringValue ;
                        edo:hasValueCardinality edo:singleValue .


###  https://w3id.org/energy-domain/edo#SpecificHeatCapacity
edo:SpecificHeatCapacity rdf:type owl:Class ;
                         rdfs:subClassOf edo:DomainAttribute ;
                         dcterms:accessRights "PUBLIC" ;
                         dcterms:identifier "SpecificHeatCapacity" ;
                         skos:definition "Calor Específico do material"@pt-br ,
                                         "Indicates the amount of heat required to raise the temperature of the material by a specific amount, typically measured per unit mass. This property is important for understanding the thermal behavior of the material.."@en ;
                         skos:prefLabel "Calor Específico"@pt-br ,
                                        "Specific Heat Capacity"@en ;
                         edo:hasTypedValue edo:floatValue ;
                         edo:hasValueCardinality edo:singleValue .


###  https://w3id.org/energy-domain/edo#SpecificWeight
edo:SpecificWeight rdf:type owl:Class ;
                   rdfs:subClassOf edo:DomainAttribute ;
                   dcterms:accessRights "PUBLIC" ;
                   dcterms:identifier "SpecificWeight" ;
                   skos:definition "Indicates the weight of the material per unit volume. This property is crucial for understanding the material's density and its impact on the overall weight."@en ,
                                   "Peso específico do material"@pt-br ;
                   skos:prefLabel "Peso Específico"@pt-br ,
                                  "Specific Weight"@en ;
                   edo:hasTypedValue edo:floatValue ;
                   edo:hasValueCardinality edo:singleValue .


###  https://w3id.org/energy-domain/edo#SplitCollar
edo:SplitCollar rdf:type owl:Class ;
                rdfs:subClassOf edo:LineAncillary ;
                dcterms:identifier "SplitCollar" ;
                skos:definition "A component used to encircle and secure parts of subsea systems, such as flexible pipes, risers, or accessories. The Split Collar is designed with a split or gap, allowing it to be clamped around the pipe or component and then fastened together. This design facilitates easy installation and removal, making it useful for applications where adjustments or maintenance are required. The Split Collar provides structural support, alignment, and stability, ensuring that the connected components remain securely in place."@en ;
                skos:prefLabel "Colar Bipartido"@pt-br ,
                               "Split Collar"@en ;
                edo:hasAttribute edo:PipeMountPosition .


###  https://w3id.org/energy-domain/edo#SpoolingTension
edo:SpoolingTension rdf:type owl:Class ;
                    rdfs:subClassOf edo:DomainAttribute ;
                    dcterms:accessRights "PUBLIC" ;
                    dcterms:identifier "SpoolingTension" ;
                    skos:definition "Represents the tension applied to a flexible component during the spooling process. This property is crucial for ensuring that the material is wound onto the reel or spool without exceeding its mechanical limits, preventing damage or deformation during handling and storage."@en ;
                    skos:prefLabel "Spooling Tension"@en ,
                                   "Tração de Desenrolamento"@pt-br ;
                    edo:hasTypedValue edo:floatValue ;
                    edo:hasValueCardinality edo:singleValue .


###  https://w3id.org/energy-domain/edo#StaticEquipmentEngineering
edo:StaticEquipmentEngineering rdf:type owl:Class ;
                               rdfs:subClassOf edo:EquipmentEngineering ;
                               rdfs:label "Engenharia de Equipamentos Estáticos"@pt-br ,
                                          "Static Equipment Engineering"@en ;
                               skos:definition "Engenharia de equipamentos industriais sem partes móveis como vasos de pressão, tanques e trocadores de calor."@pt-br ,
                                               "Engineering of non-moving industrial equipment such as pressure vessels, tanks, and heat exchangers."@en .


###  https://w3id.org/energy-domain/edo#StiffTorsionalStiffnessAtSeaLevel
edo:StiffTorsionalStiffnessAtSeaLevel rdf:type owl:Class ;
                                      rdfs:subClassOf edo:DomainAttribute ;
                                      dcterms:accessRights "PUBLIC" ;
                                      dcterms:identifier "StiffTorsionalStiffnessAtSeaLevel" ;
                                      skos:definition "Represents the torsional stiffness of a component when measured at sea level, indicating its resistance to twisting under applied torque. This property is important for ensuring that the component maintains its structural integrity and performance under rotational forces."@en ,
                                                      "Rigidez a torção (GJ) (maior valor) a 20°C e pressão atmosferica (dentro e fora)"@pt-br ;
                                      skos:prefLabel "Rigidez a Torção Rígida ao Nível do Mar"@pt-br ,
                                                     "Stiff Torsional Stiffness At Sea Level"@en ;
                                      edo:hasTypedValue edo:floatValue ;
                                      edo:hasValueCardinality edo:singleValue .


###  https://w3id.org/energy-domain/edo#StopperCollar
edo:StopperCollar rdf:type owl:Class ;
                  rdfs:subClassOf edo:SplitCollar ;
                  dcterms:identifier "StopperCollar" ;
                  skos:altLabel "Locking Collar"@en ,
                                "Positioning Collar"@en ,
                                "Retention Collar"@en ,
                                "Stopper Clamp"@en ;
                  skos:definition "A component used to prevent the movement or displacement of other parts in subsea systems. The Stopper Collar is installed around the pipe or component and acts as a physical barrier to stop or limit movement, ensuring components stay in their intended positions. It is crucial for maintaining alignment and stability during installation, operation, or maintenance, providing secure positioning and preventing unwanted shifts or displacements."@en ;
                  skos:prefLabel "Colar Batente"@pt-br ,
                                 "Stopper Collar"@en ;
                  edo:ifc_equivalentClass "IfcPipeFitting" ;
                  edo:ifc_objectType "StopperCollar" ;
                  edo:ifc_predefinedType "USERDEFINED" .


###  https://w3id.org/energy-domain/edo#StrIntOffPLevMaxPress
edo:StrIntOffPLevMaxPress rdf:type owl:Class ;
                          rdfs:subClassOf edo:DomainAttribute ;
                          dcterms:accessRights "PUBLIC" ;
                          dcterms:identifier "StrIntOffPLevMaxPress" ;
                          skos:definition "Condições de teste dos tramos para Pressão - Máxima - Teste de integridade estrutural hidrostática (off-shore, no nível da plataforma)"@pt-br ,
                                          "The maximum pressure applied during the Structural Integrity Test (offshore, at platform level), ensuring structural integrity under extreme conditions."@en ;
                          skos:prefLabel "Integridade Estrutural Offshore com Pressão Máxima no Nível da Plataforma"@pt-br ,
                                         "Structural Integrity Offshore Leak Test At Platform Level Maximum Pressure"@en ;
                          edo:hasTypedValue edo:floatValue ;
                          edo:hasValueCardinality edo:singleValue .


###  https://w3id.org/energy-domain/edo#StrIntOffPLevMaxPressValRef
edo:StrIntOffPLevMaxPressValRef rdf:type owl:Class ;
                                rdfs:subClassOf edo:DomainAttribute ;
                                dcterms:accessRights "PUBLIC" ;
                                dcterms:identifier "StrIntOffPLevMaxPressValRef" ;
                                skos:definition "Comentários Condições de teste dos tramos para - Máximo - Teste de integridade estrutural hidrostática (off-shore, no nível da plataforma)"@pt-br ,
                                                "Specifies the reference pressure used to determine the Structural Offshore Maximum Pressure value."@en ;
                                skos:prefLabel "Referência de Valor de Pressão Máxima para Teste de Integridade Estrutural Offshore e de Vazamento no Nível da Plataforma"@pt-br ,
                                               "Structural Integrity Offshore Leak Test At Platform Level Maximum Pressure Value Reference"@en ;
                                edo:hasTypedValue edo:stringValue ;
                                edo:hasValueCardinality edo:singleValue .


###  https://w3id.org/energy-domain/edo#StrIntOffPLevMaxPressValRefMult
edo:StrIntOffPLevMaxPressValRefMult rdf:type owl:Class ;
                                    rdfs:subClassOf edo:DomainAttribute ;
                                    dcterms:accessRights "PUBLIC" ;
                                    dcterms:identifier "StrIntOffPLevMaxPressValRefMult" ;
                                    skos:definition "The multiplier applied to the reference pressure to determine the Structural Offshore Maximum Pressure value."@en ;
                                    skos:prefLabel "Multiplicador de Referência de Valor de Pressão Máxima para Teste de Integridade Estrutural Offshore no Nível da Plataforma"@pt-br ,
                                                   "Structural Integrity Offshore Leak Test At Platform Level Maximum Pressure Value Reference Multiplier"@en ;
                                    edo:hasTypedValue edo:floatValue ;
                                    edo:hasValueCardinality edo:singleValue .


###  https://w3id.org/energy-domain/edo#StrIntOffPLevNomPress
edo:StrIntOffPLevNomPress rdf:type owl:Class ;
                          rdfs:subClassOf edo:DomainAttribute ;
                          dcterms:accessRights "PUBLIC" ;
                          dcterms:identifier "StrIntOffPLevNomPress" ;
                          skos:definition "Condições de teste dos tramos para Pressão - Nominal - Teste de integridade estrutural hidrostática (off-shore, no nível da plataforma)"@pt-br ,
                                          "The nominal pressure applied during the Structural Integrity Test (offshore, at platform level), simulating typical conditions to verify structural integrity."@en ;
                          skos:prefLabel "Integridade Estrutural Offshore com Pressão Nominal no Nível da Plataforma"@pt-br ,
                                         "Structural Integrity Offshore Leak Test At Platform Level Nominal Pressure"@en ;
                          edo:hasTypedValue edo:floatValue ;
                          edo:hasValueCardinality edo:singleValue .


###  https://w3id.org/energy-domain/edo#StrIntOffPLevNomPressValRef
edo:StrIntOffPLevNomPressValRef rdf:type owl:Class ;
                                rdfs:subClassOf edo:DomainAttribute ;
                                dcterms:accessRights "PUBLIC" ;
                                dcterms:identifier "StrIntOffPLevNomPressValRef" ;
                                skos:definition "Comentários Condições de teste dos tramos para - Nominal - Teste de integridade estrutural hidrostática (off-shore, no nível da plataforma)"@pt-br ,
                                                "Specifies the reference pressure used to determine the Structural Offshore Leak Test Nominal Pressure value."@en ;
                                skos:prefLabel "Referência de Valor de Pressão Nominal para Teste de Integridade Estrutural Offshore no Nível da Plataforma"@pt-br ,
                                               "Structural Integrity Offshore Leak Test At Platform Level Nominal Pressure Value Reference"@en ;
                                edo:hasTypedValue edo:stringValue ;
                                edo:hasValueCardinality edo:singleValue .


###  https://w3id.org/energy-domain/edo#StrIntOffPLevNomPressValRefMult
edo:StrIntOffPLevNomPressValRefMult rdf:type owl:Class ;
                                    rdfs:subClassOf edo:DomainAttribute ;
                                    dcterms:accessRights "PUBLIC" ;
                                    dcterms:identifier "StrIntOffPLevNomPressValRefMult" ;
                                    skos:definition "The multiplier applied to the reference pressure to determine the Structural Offshore Nominal Pressure value."@en ;
                                    skos:prefLabel "Multiplicador de Referência de Valor de Pressão Nominal para Teste de Integridade Estrutural Offshore no Nível da Plataforma"@pt-br ,
                                                   "Structural Integrity Offshore Leak Test At Platform Level Nominal Pressure Value Reference Multiplier"@en ;
                                    edo:hasTypedValue edo:floatValue ;
                                    edo:hasValueCardinality edo:singleValue .


###  https://w3id.org/energy-domain/edo#StrIntOnNoTensMaxPress
edo:StrIntOnNoTensMaxPress rdf:type owl:Class ;
                           rdfs:subClassOf edo:DomainAttribute ;
                           dcterms:accessRights "PUBLIC" ;
                           dcterms:identifier "StrIntOnNoTensMaxPress" ;
                           skos:definition "Condições de teste dos tramos para Pressão - Máxima - Teste de integridade estrutural hidrostática (a bordo, sem tensão)"@pt-br ,
                                           "The maximum pressure applied during the Structural Integrity Test (onboard, without tension), verifying performance under extreme conditions."@en ;
                           skos:prefLabel "Integridade Estrutural a Bordo sem Pressão Máxima de Tensão"@pt-br ,
                                          "Structural Integrity Onboard With No Tension Maximum Pressure"@en ;
                           edo:hasTypedValue edo:floatValue ;
                           edo:hasValueCardinality edo:singleValue .


###  https://w3id.org/energy-domain/edo#StrIntOnNoTensMaxPressValRef
edo:StrIntOnNoTensMaxPressValRef rdf:type owl:Class ;
                                 rdfs:subClassOf edo:DomainAttribute ;
                                 dcterms:accessRights "PUBLIC" ;
                                 dcterms:identifier "StrIntOnNoTensMaxPressValRef" ;
                                 skos:definition "Comentários Condições de teste dos tramos para - Máximo - Teste de integridade estrutural hidrostática (a bordo, sem tensão)"@pt-br ,
                                                 "Specifies the reference pressure used to determine the Structural Onboard Maximum Pressure value."@en ;
                                 skos:prefLabel "Referência de Valor de Pressão Máxima para Integridade Estrutural a Bordo sem Tensão"@pt-br ,
                                                "Structural Integrity Onboard With No Tension Maximum Pressure Value Reference"@en ;
                                 edo:hasTypedValue edo:stringValue ;
                                 edo:hasValueCardinality edo:singleValue .


###  https://w3id.org/energy-domain/edo#StrIntOnNoTensMaxPressValRefMult
edo:StrIntOnNoTensMaxPressValRefMult rdf:type owl:Class ;
                                     rdfs:subClassOf edo:DomainAttribute ;
                                     dcterms:accessRights "PUBLIC" ;
                                     dcterms:identifier "StrIntOnNoTensMaxPressValRefMult" ;
                                     skos:definition "The multiplier applied to the reference pressure to determine the Structural Onboard Maximum Pressure value."@en ;
                                     skos:prefLabel "Multiplicador de Referência de Valor de Pressão Máxima para Integridade Estrutural a Bordo sem Tensão"@pt-br ,
                                                    "Structural Integrity Onboard With No Tension Maximum Pressure Value Reference Multiplier"@en ;
                                     edo:hasTypedValue edo:floatValue ;
                                     edo:hasValueCardinality edo:singleValue .


###  https://w3id.org/energy-domain/edo#StrIntOnNoTensNomPress
edo:StrIntOnNoTensNomPress rdf:type owl:Class ;
                           rdfs:subClassOf edo:DomainAttribute ;
                           dcterms:accessRights "PUBLIC" ;
                           dcterms:identifier "StrIntOnNoTensNomPress" ;
                           skos:definition "Condições de teste dos tramos para Pressão - Nominal - Teste de integridade estrutural hidrostática (on-board, sem tensão)"@pt-br ,
                                           "The nominal pressure applied during the Structural Integrity Test (onboard, without tension), simulating typical conditions to verify structural integrity."@en ;
                           skos:prefLabel "Integridade Estrutural a Bordo sem Pressão Nominal de Tensão"@pt-br ,
                                          "Structural Integrity Onboard With No Tension Nominal Pressure"@en ;
                           edo:hasTypedValue edo:floatValue ;
                           edo:hasValueCardinality edo:singleValue .


###  https://w3id.org/energy-domain/edo#StrIntOnNoTensNomPressValRef
edo:StrIntOnNoTensNomPressValRef rdf:type owl:Class ;
                                 rdfs:subClassOf edo:DomainAttribute ;
                                 dcterms:accessRights "PUBLIC" ;
                                 dcterms:identifier "StrIntOnNoTensNomPressValRef" ;
                                 skos:definition "Comentários Condições de teste dos tramos para - Nominal - Teste de integridade estrutural hidrostática (on-board, sem tensão)"@pt-br ,
                                                 "Specifies the reference pressure used to determine the Structural Onboard Nominal Pressure value."@en ;
                                 skos:prefLabel "Integridade Estrutural a Bordo sem Referência de Valor de Pressão Nominal de Tensão"@pt-br ,
                                                "Structural Integrity Onboard With No Tension Nominal Pressure Value Reference"@en ;
                                 edo:hasTypedValue edo:stringValue ;
                                 edo:hasValueCardinality edo:singleValue .


###  https://w3id.org/energy-domain/edo#StrIntOnNoTensNomPressValRefMult
edo:StrIntOnNoTensNomPressValRefMult rdf:type owl:Class ;
                                     rdfs:subClassOf edo:DomainAttribute ;
                                     dcterms:accessRights "PUBLIC" ;
                                     dcterms:identifier "StrIntOnNoTensNomPressValRefMult" ;
                                     skos:definition "The multiplier applied to the reference pressure to determine the Structural Onboard Nominal Pressure value."@en ;
                                     skos:prefLabel "Multiplicador de Referência de Valor de Pressão Nominal para Integridade Estrutural a Bordo sem Tensão"@pt-br ,
                                                    "Structural Integrity Onboard With No Tension Nominal Pressure Value Reference Multiplier"@en ;
                                     edo:hasTypedValue edo:floatValue ;
                                     edo:hasValueCardinality edo:singleValue .


###  https://w3id.org/energy-domain/edo#StrandsTable
edo:StrandsTable rdf:type owl:Class ;
                 rdfs:subClassOf edo:DomainAttribute ;
                 dcterms:accessRights "PUBLIC" ;
                 dcterms:identifier "StrandsTable" ;
                 skos:definition "Provides detailed information about the mechanical and geometrical properties, including dimensions and material characteristics, necessary for understanding and evaluating the component's performance and suitability for its intended application."@en ;
                 skos:prefLabel "Strands Table"@en ,
                                "Tabela de Propriedades das Cordoalhas"@pt-br .


###  https://w3id.org/energy-domain/edo#StrandsTable_SpareQuantity
edo:StrandsTable_SpareQuantity rdf:type owl:Class ;
                               rdfs:subClassOf edo:DomainAttribute ;
                               dcterms:accessRights "PUBLIC" ;
                               dcterms:identifier "StrandsTable_SpareQuantity" ;
                               skos:definition "Specifies the number of spare units available, ensuring adequate backup components are on hand for maintenance or replacement. This quantity helps in planning and minimizing downtime during operations in subsea environments."@en ;
                               skos:prefLabel "Quantidade de Sobressalentes"@pt-br ,
                                              "Spare Quantity"@en ;
                               edo:hasTypedValue edo:intValue ;
                               edo:hasValueCardinality edo:multiValue .


###  https://w3id.org/energy-domain/edo#StrandsTable_StrandsLength
edo:StrandsTable_StrandsLength rdf:type owl:Class ;
                               rdfs:subClassOf edo:DomainAttribute ;
                               dcterms:accessRights "PUBLIC" ;
                               dcterms:identifier "StrandsTable_StrandsLength" ;
                               skos:definition "Length of the individual strands."@en ;
                               skos:prefLabel "Comprimento das Cordoalhas"@pt-br ,
                                              "Strands Length"@en ;
                               edo:hasTypedValue edo:floatValue ;
                               edo:hasValueCardinality edo:multiValue .


###  https://w3id.org/energy-domain/edo#StrandsTable_StrandsQuantity
edo:StrandsTable_StrandsQuantity rdf:type owl:Class ;
                                 rdfs:subClassOf edo:DomainAttribute ;
                                 dcterms:accessRights "PUBLIC" ;
                                 dcterms:identifier "StrandsTable_StrandsQuantity" ;
                                 skos:definition "Number of individual strands used, determining the overall reinforcement and strength of the component."@en ;
                                 skos:prefLabel "Quantidade de Cordoalhas"@pt-br ,
                                                "Strands Quantity"@en ;
                                 edo:hasTypedValue edo:intValue ;
                                 edo:hasValueCardinality edo:multiValue .


###  https://w3id.org/energy-domain/edo#StressAtDesignPressure
edo:StressAtDesignPressure rdf:type owl:Class ;
                           rdfs:subClassOf edo:DomainAttribute ;
                           dcterms:accessRights "PUBLIC" ;
                           dcterms:identifier "StressAtDesignPressure" ;
                           skos:definition "Maximum stress that the material can withstand when subjected to design pressure is specified. This parameter is critical for ensuring that the material maintains its structural integrity and performs reliably under the operational pressure conditions specified in the design."@en ;
                           skos:prefLabel "Stress At Design Pressure"@en ,
                                          "Tensão na pressão de projeto"@pt-br ;
                           edo:hasTypedValue edo:floatValue ;
                           edo:hasValueCardinality edo:singleValue .


###  https://w3id.org/energy-domain/edo#StructuralEngineering
edo:StructuralEngineering rdf:type owl:Class ;
                          rdfs:subClassOf edo:CivilEngineering ;
                          rdfs:label "Engenharia Estrutural"@pt-br ,
                                     "Structural Engineering"@en ;
                          skos:definition "Disciplina de engenharia focada na integridade estrutural e projeto de edifícios e infraestrutura."@pt-br ,
                                          "Engineering discipline focused on the structural integrity and design of buildings and infrastructure."@en .


###  https://w3id.org/energy-domain/edo#StructureApplicationsList
edo:StructureApplicationsList rdf:type owl:Class ;
                              rdfs:subClassOf edo:DomainAttribute ;
                              dcterms:accessRights "PUBLIC" ;
                              dcterms:identifier "StructureApplicationsList" ;
                              skos:definition "Indicates the possible positions where the structure can be applied along the pipeline system. Multiple values can be selected to show in which sections, such as different parts of a riser or flowline, the structure is suitable for use."@en ,
                                              "Lista de todas as possíveis aplicações para a estrutura Valores aplicáveis (Mais de um valor pode ser escolhido): R (Riser) RT (Para seção de topo do riser) RI (Para seção intermediaria do riser) RF (Para seção de fundo do riser) F (Para Flowline)"@pt-br ;
                              skos:prefLabel "Lista de Aplicações da Estrutura"@pt-br ,
                                             "Structure Applications List"@en ;
                              edo:hasTypedValue edo:stringValue ;
                              edo:hasValueCardinality edo:multiValue .


###  https://w3id.org/energy-domain/edo#StructureCode
edo:StructureCode rdf:type owl:Class ;
                  rdfs:subClassOf edo:DomainAttribute ;
                  dcterms:accessRights "PUBLIC" ;
                  dcterms:identifier "StructureCode" ;
                  skos:definition "Indicates the code or identifier assigned to the structure. This property is used to uniquely identify and reference the structure within a system, ensuring proper tracking, documentation, and management."@en ;
                  skos:prefLabel "Código da estrutura"@pt-br ,
                                 "Structure Code"@en ;
                  edo:hasTypedValue edo:stringValue ;
                  edo:hasValueCardinality edo:singleValue .


###  https://w3id.org/energy-domain/edo#StudSet
edo:StudSet rdf:type owl:Class ;
            rdfs:subClassOf edo:PhysicalConnection ;
            dcterms:identifier "StudSet" ;
            skos:altLabel "Stud"@en ,
                          "Threaded Rod"@en ;
            skos:definition "Stud sets are essential fastening components used in subsea oil and gas interconnection end fittings to securely assemble and connect various parts of the equipment. Each set typically includes bolts, nuts, and washers, all made from high-strength, corrosion-resistant materials to endure the harsh subsea environment. These components are designed to provide reliable mechanical fastening, ensuring the structural integrity and leak-proof performance of the end fittings. The stud sets are carefully engineered to withstand high pressure and extreme temperatures, making them critical for maintaining the operational safety and longevity of subsea interconnections."@en ;
            skos:prefLabel "Estojos"@pt-br ,
                           "Stud Set"@en ;
            edo:hasAttribute edo:AssemblyTorque ,
                             edo:FullyThreaded ,
                             edo:Lubricant ,
                             edo:LubricantFrictionFactor ,
                             edo:NominalDiameter ,
                             edo:Quantity ,
                             edo:SpareQuantity .


###  https://w3id.org/energy-domain/edo#SubProjectId
edo:SubProjectId rdf:type owl:Class ;
                 rdfs:subClassOf edo:DomainAttribute ;
                 dcterms:accessRights "PUBLIC" ;
                 dcterms:identifier "SubProjectId" ;
                 skos:definition "Refers to the identification code assigned to the well or piece of equipment for which the interconnection is being designed. This code is often provisional, used during the initial stages of development, such as during the fabrication or installation of flexible pipelines, before a final approval or designation is granted. It serves as a reference point for all equipment and documentation until the well or equipment receives its definitive identification from the relevant regulatory authority. Examples include codes like LL-S.P6, LL-S.MSIAG1, or simpler identifiers such as P6 or MSIAG1."@en ;
                 skos:prefLabel "Id do Subprojeto"@pt-br ,
                                "Sub Project Id"@en ;
                 edo:hasTypedValue edo:stringValue ;
                 edo:hasValueCardinality edo:singleValue .


###  https://w3id.org/energy-domain/edo#SubseaConnectionPoint
edo:SubseaConnectionPoint rdf:type owl:Class ;
                          rdfs:subClassOf edo:LogicalConnection ;
                          dcterms:identifier "SubseaConnectionPoint" ;
                          skos:definition "The Subsea Connection Point is the interface on subsea equipment where a flexible pipe connects. It serves as the critical link between the flexible pipe and subsea systems, enabling the transfer of fluids or gases. Designed to withstand high pressures and harsh underwater conditions, the Subsea External Point ensures a secure and reliable connection, facilitating efficient operation of various subsea systems."@en ;
                          skos:prefLabel "Ponto de Conexão Submarino"@pt-br ,
                                         "Subsea Connection Point"@en ;
                          edo:ifc_equivalentClass "IfcPipeFitting" ;
                          edo:ifc_objectType "SubseaConnectionPoint" ;
                          edo:ifc_predefinedType "USERDEFINED" .


###  https://w3id.org/energy-domain/edo#SubseaEngineering
edo:SubseaEngineering rdf:type owl:Class ;
                      rdfs:subClassOf edo:TechnicalDiscipline ;
                      rdfs:label "Engenharia Submarina"@pt-br ,
                                 "Subsea Engineering"@en ;
                      skos:definition "Disciplina de engenharia focada em sistemas e equipamentos subaquáticos para operações offshore."@pt-br ,
                                      "Engineering discipline focused on underwater systems and equipment for offshore operations."@en .


###  https://w3id.org/energy-domain/edo#SubseaFlexiblePipesBsddDictionary
edo:SubseaFlexiblePipesBsddDictionary rdf:type owl:Class ;
                                      rdfs:subClassOf edo:DomainElement ;
                                      dcterms:identifier "SubseaFlexiblePipesBsddDictionary" ;
                                      skos:definition "Bsdd Dictionary of Subsea Flexible Pipelines."@en ;
                                      skos:prefLabel "Dicionário Bsdd de Dutos Flexíveis Submarinos"@pt-br ,
                                                     "Subsea Flexible Pipes Bsdd Dictionary"@en ;
                                      edo:ifc_equivalentClass "IfcClassification" ;
                                      edo:ifc_objectType "SubseaFlexiblePipesBsddDictionary" ;
                                      edo:ifc_predefinedType "USERDEFINED" .


###  https://w3id.org/energy-domain/edo#SubseaFlexiblePipesEngineering
edo:SubseaFlexiblePipesEngineering rdf:type owl:Class ;
                                   rdfs:subClassOf edo:SubseaEngineering ;
                                   rdfs:label "Engenharia de Tubos Flexíveis Submarinos"@pt-br ,
                                              "Subsea Flexible Pipes Engineering"@en ;
                                   skos:definition "Engenharia de sistemas de tubos flexíveis utilizados em aplicações submarinas."@pt-br ,
                                                   "Engineering of flexible pipe systems used in subsea applications."@en .


###  https://w3id.org/energy-domain/edo#SubseaLayout
edo:SubseaLayout rdf:type owl:Class ;
                 rdfs:subClassOf edo:Location ;
                 dcterms:identifier "SubseaLayout" ;
                 skos:definition "The arrangement or map of components and systems within a subsea environment, including pipelines, risers, manifolds, and other infrastructure."@en ;
                 skos:prefLabel "Arranjo Submarino"@pt-br ,
                                "Subsea Layout"@en .


###  https://w3id.org/energy-domain/edo#SubseaOilField
edo:SubseaOilField rdf:type owl:Class ;
                   rdfs:subClassOf edo:SubseaLayout ;
                   dcterms:identifier "SubseaOilField" ;
                   skos:altLabel "Subsea Hydrocarbon Field"@en ,
                                 "Subsea Oil Reservoir"@en ,
                                 "Subsea Oil Site"@en ,
                                 "Subsea Petroleum Field"@en ;
                   skos:definition "A subsea oil field refers to an underwater reservoir of hydrocarbons located beneath the seabed. It involves the extraction of oil and gas from deposits situated in deepwater or shallow marine environments. The subsea oil field includes a range of equipment and infrastructure, such as subsea wells, pipelines, and production systems, all designed to safely and efficiently extract and transport hydrocarbons to processing facilities on the surface or shore. The development and operation of subsea oil fields require specialized technology and expertise to manage the challenges of deepwater environments and ensure the successful production and handling of resources."@en ;
                   skos:prefLabel "Campo de Petróleo Submarino"@pt-br ,
                                  "Subsea Oil Field"@en ;
                   edo:ifc_equivalentClass "IfcSite" ;
                   edo:ifc_objectType "SubseaOilField" .


###  https://w3id.org/energy-domain/edo#SubseaPipeline
edo:SubseaPipeline rdf:type owl:Class ;
                   rdfs:subClassOf edo:Interconnection ;
                   dcterms:identifier "SubseaPipeline" ;
                   skos:definition "A Subsea Pipeline is a conduit installed on the seafloor designed to transport oil, gas, or other fluids from underwater production facilities to processing or storage locations on the surface or shore. Engineered to withstand harsh underwater conditions, including high pressures, corrosive environments, and dynamic movements, the Subsea Pipeline is constructed with durable materials and advanced technologies to ensure reliable and efficient fluid transfer."@en ;
                   skos:prefLabel "Linha Submarina"@pt-br ,
                                  "Subsea Pipeline"@en ;
                   edo:hasAttribute edo:BasicProjectRevision ,
                                    edo:CO2VolumePercentage ,
                                    edo:ExecutiveProjectRevision ,
                                    edo:H2SVolumeConcentration ,
                                    edo:InternalDiameter ,
                                    edo:InternalIncidentalPressureTable ,
                                    edo:InternalIncidentalPressureTable_PositionReference ,
                                    edo:InternalIncidentalPressureTable_Pressure ,
                                    edo:InternalIncidentalPressureTable_VPosWRTWaterline ,
                                    edo:MaterialRequest ,
                                    edo:MaterialRequestRev ,
                                    edo:MaxDesignAbsIntPresTable ,
                                    edo:MaxDesignAbsIntPresTable_PositionReference ,
                                    edo:MaxDesignAbsIntPresTable_Pressure ,
                                    edo:MaxDesignAbsIntPresTable_VPosWRTWaterline ,
                                    edo:MaximumTemperature ,
                                    edo:MaximumThermalExchangeCoefficient ,
                                    edo:MinimumThermalExchangeCoefficient ,
                                    edo:NominalLength ,
                                    edo:ProjectAcronym ,
                                    edo:ProjectCode ,
                                    edo:RiserConfiguration ,
                                    edo:Service ,
                                    edo:SubProjectId ,
                                    edo:UnifilarDiagram ,
                                    edo:UnifilarDiagramRev ;
                   edo:ifc_equivalentClass "IfcBuilding" ;
                   edo:ifc_objectType "SubseaPipeline" ;
                   edo:ifc_predefinedType "USERDEFINED" .


###  https://w3id.org/energy-domain/edo#SubseaRigidPipesEngineering
edo:SubseaRigidPipesEngineering rdf:type owl:Class ;
                                rdfs:subClassOf edo:SubseaEngineering ;
                                rdfs:label "Engenharia de Tubos Rígidos Submarinos"@pt-br ,
                                           "Subsea Rigid Pipes Engineering"@en ;
                                skos:definition "Engenharia de sistemas de tubulações rígidas utilizadas em aplicações submarinas."@pt-br ,
                                                "Engineering of rigid pipeline systems used in subsea applications."@en .


###  https://w3id.org/energy-domain/edo#SubseaStructuresEngineering
edo:SubseaStructuresEngineering rdf:type owl:Class ;
                                rdfs:subClassOf edo:SubseaEngineering ;
                                rdfs:label "Engenharia de Estruturas Submarinas"@pt-br ,
                                           "Subsea Structures Engineering"@en ;
                                skos:definition "Engenharia de manifolds submarinos, árvores de natal e outros componentes estruturais."@pt-br ,
                                                "Engineering of subsea manifolds, christmas trees, and other structural components."@en .


###  https://w3id.org/energy-domain/edo#SubseaUmbilicalsEngineering
edo:SubseaUmbilicalsEngineering rdf:type owl:Class ;
                                rdfs:subClassOf edo:SubseaEngineering ;
                                rdfs:label "Engenharia de Umbilicais Submarinos"@pt-br ,
                                           "Subsea Umbilicals Engineering"@en ;
                                skos:definition "Engenharia de sistemas de umbilicais submarinos fornecendo controle, energia e injeção química."@pt-br ,
                                                "Engineering of subsea umbilical systems providing control, power and chemical injection."@en .


###  https://w3id.org/energy-domain/edo#SubseaWell
edo:SubseaWell rdf:type owl:Class ;
               rdfs:subClassOf edo:EquipmentLocation ;
               dcterms:identifier "SubseaWell" ;
               skos:definition "A Subsea Well is a well located on the seafloor from which hydrocarbons such as oil and gas are extracted. Positioned underwater, it typically involves a wellhead assembly that includes valves, controls, and monitoring equipment to manage the extraction process. The Subsea Well is connected to surface facilities via pipelines and umbilicals, which facilitate the transport of extracted resources and the provision of necessary services like power and communication. Designed to operate under high pressure and harsh marine conditions, the subsea well is a critical component of offshore oil and gas production systems."@en ;
               skos:prefLabel "Poço"@pt-br ,
                              "Subsea Well"@en ;
               edo:ifc_equivalentClass "IfcBuilding" ;
               edo:ifc_objectType "SubseaWell" ;
               edo:ifc_predefinedType "USERDEFINED" .


###  https://w3id.org/energy-domain/edo#SupplierProvidedMaterialName
edo:SupplierProvidedMaterialName rdf:type owl:Class ;
                                 rdfs:subClassOf edo:DomainAttribute ;
                                 dcterms:accessRights "PUBLIC" ;
                                 dcterms:identifier "SupplierProvidedMaterialName" ;
                                 skos:definition "Name of the material as specified by the original supplier. This property identifies the exact material provided, ensuring it aligns with the required specifications for the accessory."@en ;
                                 skos:prefLabel "Nome do material conforme designado pelo fornecedor original do material"@pt-br ,
                                                "Supplier Provided Material Name"@en ;
                                 edo:hasTypedValue edo:stringValue ;
                                 edo:hasValueCardinality edo:singleValue .


###  https://w3id.org/energy-domain/edo#TapeLayer
edo:TapeLayer rdf:type owl:Class ;
              rdfs:subClassOf edo:WoundLayer ;
              dcterms:identifier "TapeLayer" ;
              skos:definition "A layer within the structure of a subsea flexible pipe composed of tape-like materials. This layer is designed to provide additional reinforcement and protection. Typically made from high-strength polymers or other durable materials, the tape layer contributes to the pipe’s overall flexibility, structural integrity, and resistance to external environmental factors. Engineered for harsh underwater conditions, it helps maintain the performance and durability of the flexible pipe system."@en ;
              skos:prefLabel "Camada de Fita"@pt-br ,
                             "Tape Layer"@en .


###  https://w3id.org/energy-domain/edo#TapesQuantity
edo:TapesQuantity rdf:type owl:Class ;
                  rdfs:subClassOf edo:DomainAttribute ;
                  dcterms:accessRights "PUBLIC" ;
                  dcterms:identifier "TapesQuantity" ;
                  skos:definition "Number of tapes applied within the structure, influencing factors such as insulation, protection, and reinforcement. "@en ;
                  skos:prefLabel "Quantidade de fitas"@pt-br ,
                                 "Tapes Quantity"@en ;
                  edo:hasTypedValue edo:intValue ;
                  edo:hasValueCardinality edo:singleValue .


###  https://w3id.org/energy-domain/edo#TechnicalDiscipline
edo:TechnicalDiscipline rdf:type owl:Class ;
                        rdfs:subClassOf edo:DomainClassification ;
                        rdfs:comment "Superclass for all technical engineering disciplines."@en ;
                        rdfs:label "Disciplina Técnica"@pt-br ,
                                   "Technical Discipline"@en ;
                        skos:definition "A specialized field of engineering or technical expertise within industrial projects."@en ,
                                        "Um campo especializado de engenharia ou expertise técnica dentro de projetos industriais."@pt-br .


###  https://w3id.org/energy-domain/edo#TechnicalNotes
edo:TechnicalNotes rdf:type owl:Class ;
                   rdfs:subClassOf edo:DomainAttribute ;
                   dcterms:accessRights "PUBLIC" ;
                   dcterms:identifier "TechnicalNotes" ;
                   skos:definition "A field used to provide additional technical information or clarifications that may not be covered by other specific properties, to support a comprehensive understanding of the material’s behavior and suitability."@en ;
                   skos:prefLabel "Notas Técnicas"@pt-br ,
                                  "Technical Notes"@en ;
                   edo:hasTypedValue edo:stringValue ;
                   edo:hasValueCardinality edo:singleValue .


###  https://w3id.org/energy-domain/edo#TensileArmour
edo:TensileArmour rdf:type owl:Class ;
                  rdfs:subClassOf edo:WireLayer ;
                  dcterms:identifier "TensileArmour" ;
                  skos:definition "Protective layer designed to withstand high tensile stresses and mechanical loads, Tensile Armour is composed of high-strength steel wires or reinforced materials arranged in a helical configuration around the riser. It provides essential resistance to tension and shields the inner layers from mechanical damage and wear, ensuring the riser's integrity and durability during installation and operation in extreme underwater conditions."@en ;
                  skos:prefLabel "Armadura de Tração"@pt-br ,
                                 "Tensile Armour"@en ;
                  edo:hasAttribute edo:TensileWireLayAngle ,
                                   edo:TensileWiresCount ;
                  edo:ifc_equivalentClass "IfcPipeSegment" ;
                  edo:ifc_objectType "TensileArmour" ;
                  edo:ifc_predefinedType "USERDEFINED" .


###  https://w3id.org/energy-domain/edo#TensileArmourAnnulusCondition
edo:TensileArmourAnnulusCondition rdf:type owl:Class ;
                                  rdfs:subClassOf edo:DomainAttribute ;
                                  dcterms:accessRights "PUBLIC" ;
                                  dcterms:identifier "TensileArmourAnnulusCondition" ;
                                  skos:definition "Condição do anular das amarduras de tração, Alagado ou Seco"@pt-br ,
                                                  "Indicates the condition of the annulus in the tensile armour layer, which refers to the space between the tensile armour and other layers."@en ;
                                  skos:prefLabel "Condição do Anular das Armaduras de Tração"@pt-br ,
                                                 "Tensile Armour Annulus Condition"@en ;
                                  edo:hasTypedValue edo:stringValue ;
                                  edo:hasValueCardinality edo:singleValue .


###  https://w3id.org/energy-domain/edo#TensileArmourFreeAnnulusVolume
edo:TensileArmourFreeAnnulusVolume rdf:type owl:Class ;
                                   rdfs:subClassOf edo:DomainAttribute ;
                                   dcterms:accessRights "PUBLIC" ;
                                   dcterms:identifier "TensileArmourFreeAnnulusVolume" ;
                                   skos:definition "Indicates the available volume within the annulus of the tensile armour layer that is not occupied by material."@en ;
                                   skos:prefLabel "Tensile Armour Free Annulus Volume"@en ,
                                                  "Volume livre do anular das armaduras de tração"@pt-br ;
                                   edo:hasTypedValue edo:floatValue ;
                                   edo:hasValueCardinality edo:singleValue .


###  https://w3id.org/energy-domain/edo#TensileWireLayAngle
edo:TensileWireLayAngle rdf:type owl:Class ;
                        rdfs:subClassOf edo:DomainAttribute ;
                        dcterms:accessRights "PUBLIC" ;
                        dcterms:identifier "TensileWireLayAngle" ;
                        skos:definition "Refers to the angle formed between the individual tensile wires and the longitudinal axis of the flexible pipe. This angle determines how the wires are arranged around the pipe, influencing its mechanical properties and performance under load."@en ;
                        skos:prefLabel "Tensile Wire Lay Angle"@en ,
                                       "Ângulo de Enrolamento dos Arames sob Tração"@pt-br ;
                        edo:hasTypedValue edo:floatValue ;
                        edo:hasValueCardinality edo:singleValue .


###  https://w3id.org/energy-domain/edo#TensileWiresCount
edo:TensileWiresCount rdf:type owl:Class ;
                      rdfs:subClassOf edo:DomainAttribute ;
                      dcterms:accessRights "PUBLIC" ;
                      dcterms:identifier "TensileWiresCount" ;
                      skos:definition "Indicates the total number of tensile wires in the layer, which contributes to the mechanical strength and load-bearing capacity of the flexible pipe."@en ;
                      skos:prefLabel "Quantidade de Arames de Tração"@pt-br ,
                                     "Tensile Wires Count"@en ;
                      edo:hasTypedValue edo:intValue ;
                      edo:hasValueCardinality edo:singleValue .


###  https://w3id.org/energy-domain/edo#TensionerPadsMaterial
edo:TensionerPadsMaterial rdf:type owl:Class ;
                          rdfs:subClassOf edo:DomainAttribute ;
                          dcterms:accessRights "PUBLIC" ;
                          dcterms:identifier "TensionerPadsMaterial" ;
                          skos:definition "Indicates the fabrication material used for the tensioner pads. This property is important for assessing the durability, friction, and wear resistance of the pads, ensuring they perform effectively under operational conditions."@en ,
                                          "Nome do material da sapata do tensionador (Por exemplo, Carbon Steel)"@pt-br ;
                          skos:prefLabel "Material das Sapatas do Tensionador"@pt-br ,
                                         "Tensioner Pads Material"@en ;
                          edo:hasTypedValue edo:stringValue ;
                          edo:hasValueCardinality edo:singleValue .


###  https://w3id.org/energy-domain/edo#TensionerPadsOpeningAngle
edo:TensionerPadsOpeningAngle rdf:type owl:Class ;
                              rdfs:subClassOf edo:DomainAttribute ;
                              dcterms:accessRights "PUBLIC" ;
                              dcterms:identifier "TensionerPadsOpeningAngle" ;
                              skos:definition "Defines the opening angle of the tensioner pads. This angle is crucial for determining how the pads make contact with the surface, affecting the distribution of force and the overall efficiency of the tightening process. Proper control of this angle ensures effective load application and surface protection during operation."@en ;
                              skos:prefLabel "Tensioner Pads Opening Angle"@en ,
                                             "Ângulo de Abertura das Sapatas do Tensionador"@pt-br ;
                              edo:hasTypedValue edo:intValue ;
                              edo:hasValueCardinality edo:singleValue .


###  https://w3id.org/energy-domain/edo#TensionerPadsShape
edo:TensionerPadsShape rdf:type owl:Class ;
                       rdfs:subClassOf edo:DomainAttribute ;
                       dcterms:accessRights "PUBLIC" ;
                       dcterms:identifier "TensionerPadsShape" ;
                       skos:definition "Disposição geométrica da sapata (Por exemplo \"V\")"@pt-br ,
                                       "Specifies the geometric shape of the tensioner pads. The shape affects the contact area, frictional performance, and overall effectiveness of the tightening process, influencing how forces are applied and distributed."@en ;
                       skos:prefLabel "Forma das Sapatas do Tensionador"@pt-br ,
                                      "Tensioner Pads Shape"@en ;
                       edo:hasTypedValue edo:stringValue ;
                       edo:hasValueCardinality edo:singleValue .


###  https://w3id.org/energy-domain/edo#TensionerTracksQuantity
edo:TensionerTracksQuantity rdf:type owl:Class ;
                            rdfs:subClassOf edo:DomainAttribute ;
                            dcterms:accessRights "PUBLIC" ;
                            dcterms:identifier "TensionerTracksQuantity" ;
                            skos:definition "Indicates the quantity of tensioner tracks. This value is important for understanding the distribution of tightening forces and how evenly the load is applied across the structure during the tightening process."@en ,
                                            "Quantidade de lagartas do tensionador (Por exemplo, 4)"@pt-br ;
                            skos:prefLabel "Quantidade de Lagartas do Tensionador"@pt-br ,
                                           "Tensioner Tracks Quantity"@en ;
                            edo:hasTypedValue edo:intValue ;
                            edo:hasValueCardinality edo:singleValue .


###  https://w3id.org/energy-domain/edo#TestConditions
edo:TestConditions rdf:type owl:Class ;
                   rdfs:subClassOf edo:DomainAttribute ;
                   dcterms:accessRights "PUBLIC" ;
                   dcterms:identifier "TestConditions" ;
                   skos:definition "Descrição completa das condições para a execução do ensaio"@pt-br ,
                                   "Specifies unstructured complementary information regarding the conditions under which a test is performed. This property may include additional details such as temperature, pressure, load, or other factors that could influence the test results, providing context for accurate interpretation of performance assessments."@en ;
                   skos:prefLabel "Condições de Teste"@pt-br ,
                                  "Test Conditions"@en ;
                   edo:hasTypedValue edo:stringValue ;
                   edo:hasValueCardinality edo:singleValue .


###  https://w3id.org/energy-domain/edo#TestProp
edo:TestProp rdf:type owl:Class ;
             rdfs:subClassOf edo:DomainAttribute ;
             dcterms:accessRights "PUBLIC" ;
             dcterms:identifier "TestProp" ;
             rdfs:subClassOf "IfscPropertySingleValue" ;
             skos:definition "Test Property"@en ,
                             "Test Property"@pt-br ;
             skos:prefLabel "Test Property"@en ,
                            "Test Property"@pt-br ;
             edo:hasTypedValue edo:stringValue .


###  https://w3id.org/energy-domain/edo#TestProp2
edo:TestProp2 rdf:type owl:Class ;
              rdfs:subClassOf edo:DomainAttribute ;
              dcterms:accessRights "PUBLIC" ;
              dcterms:identifier "TestProp2" ;
              rdfs:subClassOf "IfscPropertySingleValue" ;
              skos:definition "Test Property2"@en ,
                              "Test Property2"@pt-br ;
              skos:prefLabel "Test Property2"@en ,
                             "Test Property2"@pt-br ;
              edo:hasTypedValue edo:floatValue .


###  https://w3id.org/energy-domain/edo#ThermalConductivityCoefficient
edo:ThermalConductivityCoefficient rdf:type owl:Class ;
                                   rdfs:subClassOf edo:DomainAttribute ;
                                   dcterms:accessRights "PUBLIC" ;
                                   dcterms:identifier "ThermalConductivityCoefficient" ;
                                   skos:definition "Coeficiente de Condutividade Térmica do material (Obs. Para materiais compósitos, indicar o coefitiente no sentido longitudinal das fibras)"@pt-br ,
                                                   "Indicates the material's ability to conduct heat, measured as the rate at which heat passes through the material under a temperature gradient. This property is important for assessing how the material handles heat transfer in subsea environments, ensuring it can maintain performance under varying thermal conditions."@en ;
                                   skos:prefLabel "Coeficiente de Condutividade Térmica"@pt-br ,
                                                  "Thermal Conductivity Coefficient"@en ;
                                   edo:hasTypedValue edo:floatValue ;
                                   edo:hasValueCardinality edo:singleValue .


###  https://w3id.org/energy-domain/edo#ThermalExchangeCoefficientFlooded
edo:ThermalExchangeCoefficientFlooded rdf:type owl:Class ;
                                      rdfs:subClassOf edo:DomainAttribute ;
                                      dcterms:accessRights "PUBLIC" ;
                                      dcterms:identifier "ThermalExchangeCoefficientFlooded" ;
                                      skos:definition "Coeficiente de troca térmica na temperatura máxima de projeto no interior, na temperatura da profundidade máxima especificada da água no exterior, com os anulares de isolamento e das armadura de tração alagados, no final da vida útil."@pt-br ,
                                                      "Indicates the rate at which heat is transferred through a material or component in flooded conditions. This property is essential for assessing the material's thermal performance, influencing its ability to manage heat effectively in operational scenarios where it is exposed to fluid filling."@en ;
                                      skos:prefLabel "Coeficiente de Troca Térmica em Condição Alagada"@pt-br ,
                                                     "Thermal Exchange Coefficient Flooded"@en ;
                                      edo:hasTypedValue edo:floatValue ;
                                      edo:hasValueCardinality edo:singleValue .


###  https://w3id.org/energy-domain/edo#ThermalPower
edo:ThermalPower rdf:type owl:Class ;
                 rdfs:subClassOf edo:Domain ;
                 rdfs:label "Energia Térmica"@pt-br ,
                            "Thermal Power"@en ;
                 skos:definition "Energy production from fossil fuels (coal, natural gas) through thermal conversion."@en ,
                                 "Produção de energia a partir de combustíveis fósseis (carvão, gás natural) através de conversão térmica."@pt-br .


###  https://w3id.org/energy-domain/edo#ThreadPitch
edo:ThreadPitch rdf:type owl:Class ;
                rdfs:subClassOf edo:DomainAttribute ;
                dcterms:accessRights "PUBLIC" ;
                dcterms:identifier "ThreadPitch" ;
                skos:definition "The distance between adjacent thread crests, measured along the thread's axis, determining the threading's fineness or coarseness."@en ;
                skos:prefLabel "Passo da Rosca"@pt-br ,
                               "Thread Pitch"@en ;
                edo:hasTypedValue edo:floatValue ;
                edo:hasValueCardinality edo:singleValue .


###  https://w3id.org/energy-domain/edo#ThreadStandard
edo:ThreadStandard rdf:type owl:Class ;
                   rdfs:subClassOf edo:DomainAttribute ;
                   dcterms:accessRights "PUBLIC" ;
                   dcterms:identifier "ThreadStandard" ;
                   skos:definition "The standard specification governing the design and dimensions of threads used in the component, ensuring compatibility and interchangeability."@en ;
                   skos:prefLabel "Padrão de Rosca"@pt-br ,
                                  "Thread Standard"@en ;
                   edo:hasTypedValue edo:stringValue ;
                   edo:hasValueCardinality edo:singleValue .


###  https://w3id.org/energy-domain/edo#ThreadsPerInch
edo:ThreadsPerInch rdf:type owl:Class ;
                   rdfs:subClassOf edo:DomainAttribute ;
                   dcterms:accessRights "PUBLIC" ;
                   dcterms:identifier "ThreadsPerInch" ;
                   skos:definition "Threads per Inch. Indicates the number of threads present in one inch of the bolt"@en ;
                   skos:prefLabel "Fios por Polegada"@pt-br ,
                                  "Threads Per Inch"@en ;
                   edo:hasTypedValue edo:floatValue ;
                   edo:hasValueCardinality edo:singleValue .


###  https://w3id.org/energy-domain/edo#Timestamp
edo:Timestamp rdf:type owl:Class ;
              rdfs:subClassOf edo:DomainAttribute ;
              dcterms:accessRights "PUBLIC" ;
              dcterms:identifier "Timestamp" ;
              skos:definition "Exact date and time, providing a precise reference for tracking when an event or action occurred within the system."@en ;
              skos:prefLabel "Timestamp"@en ;
              edo:hasTypedValue edo:dateTimeValue ;
              edo:hasValueCardinality edo:singleValue .


###  https://w3id.org/energy-domain/edo#TopBendStiffener
edo:TopBendStiffener rdf:type owl:Class ;
                     rdfs:subClassOf edo:BendStiffener ;
                     dcterms:identifier "TopBendStiffener" ;
                     skos:altLabel "Curvature Stiffener"@en ,
                                   "Stiffener"@en ,
                                   "Top Bending Stiffener"@en ;
                     skos:definition "Designed to support and stabilize the riser where it transitions from the seabed to the floating platform or vessel, the Top Bend Stiffener is composed of high-strength materials such as steel or composites. It helps prevent excessive bending, distributes mechanical loads, and enhances flexibility management, ensuring the riser's structural integrity and performance during installation and operation in dynamic offshore conditions."@en ;
                     skos:prefLabel "Enrijecedor de Curvatura de Topo"@pt-br ,
                                    "Top Bend Stiffener"@en ;
                     edo:ifc_equivalentClass "IfcPipeFitting" ;
                     edo:ifc_objectType "TopBendStiffener" .


###  https://w3id.org/energy-domain/edo#TopsideConnectionPoint
edo:TopsideConnectionPoint rdf:type owl:Class ;
                           rdfs:subClassOf edo:LogicalConnection ;
                           dcterms:identifier "TopsideConnectionPoint" ;
                           skos:definition "Designed to connect the riser to the floating platform or vessel, the Topside Connection Point is a crucial component that ensures a secure and reliable interface between the riser and the topside facilities. Composed of high-strength materials, this connector is engineered to handle the mechanical loads and dynamic conditions of offshore environments. It facilitates the transfer of fluids and provides structural stability, playing a key role in maintaining the overall integrity and functionality of the riser system."@en ;
                           skos:prefLabel "Ponto de Conexão de Topo"@pt-br ,
                                          "Topside Connection Point"@en ;
                           edo:ifc_equivalentClass "IfcPipeFitting" ;
                           edo:ifc_objectType "TopsideConnectionPoint" ;
                           edo:ifc_predefinedType "USERDEFINED" .


###  https://w3id.org/energy-domain/edo#TransportLineSegment
edo:TransportLineSegment rdf:type owl:Class ;
                         rdfs:subClassOf edo:LinearObject ;
                         dcterms:identifier "TransportLineSegment" ;
                         skos:definition "Line for conducting some type of flow."@en ;
                         skos:prefLabel "Segmento de Linha de Transporte"@pt-br ,
                                        "Transport Line Segment"@en .


###  https://w3id.org/energy-domain/edo#Transportation
edo:Transportation rdf:type owl:Class ;
                   rdfs:subClassOf edo:LifecyclePhase ;
                   rdfs:label "Transportation"@en ,
                              "Transporte"@pt-br ;
                   skos:definition "Logistics and transport of materials and equipment to the construction or installation site."@en ,
                                   "Logística e transporte de materiais e equipamentos para o local de construção ou instalação."@pt-br .


###  https://w3id.org/energy-domain/edo#TypedValue
edo:TypedValue rdf:type owl:Class ;
               rdfs:subClassOf edo:DomainAuxiliarClass ;
               rdfs:comment "Superclass for values constrained to a specific XSD datatype."@en ;
               rdfs:label "Typed Value"@en .


###  https://w3id.org/energy-domain/edo#UNSBoltSet
edo:UNSBoltSet rdf:type owl:Class ;
               rdfs:subClassOf edo:BoltSet ;
               dcterms:identifier "UNSBoltSet" ;
               skos:definition "A set of bolts conforming to the Unified Numbering System (UNS) standard, ensuring material consistency and reliability in subsea applications."@en ;
               skos:prefLabel "Conjunto de Parafusos UNS"@pt-br ,
                              "UNS Bolt Set"@en ;
               edo:hasAttribute edo:NominalDiameter ,
                                edo:PitchToleranceClass ,
                                edo:ThreadStandard ,
                                edo:ThreadsPerInch ;
               edo:ifc_equivalentClass "IfcMechanicalFastener" ;
               edo:ifc_objectType "UNSBoltSet" ;
               edo:ifc_predefinedType "USERDEFINED" .


###  https://w3id.org/energy-domain/edo#UNSStudSet
edo:UNSStudSet rdf:type owl:Class ;
               rdfs:subClassOf edo:StudSet ;
               dcterms:identifier "UNSStudSet" ;
               skos:definition "UNS stud sets are essential fastening components for subsea oil and gas components, tailored to securely join equipment parts. Each set comprises bolts, nuts, and washers, all in UNS sizing and crafted from high-strength, corrosion-resistant materials to endure the challenging subsea environment. These components provide robust fastening, ensuring structural integrity and leak prevention in end fittings. UNS stud sets are engineered to withstand high pressure and extreme temperatures, playing a vital role in the safety and longevity of subsea interconnections."@en ;
               skos:prefLabel "Conjunto de Estojos UNS"@pt-br ,
                              "UNS Stud Set"@en ;
               edo:hasAttribute edo:PitchToleranceClass ,
                                edo:ThreadStandard ,
                                edo:ThreadsPerInch ;
               edo:ifc_equivalentClass "IfcMechanicalFastener" ;
               edo:ifc_objectType "UNSStudSet" ;
               edo:ifc_predefinedType "USERDEFINED" .


###  https://w3id.org/energy-domain/edo#UltTensStrAlongFibers
edo:UltTensStrAlongFibers rdf:type owl:Class ;
                          rdfs:subClassOf edo:DomainAttribute ;
                          dcterms:accessRights "PUBLIC" ;
                          dcterms:identifier "UltTensStrAlongFibers" ;
                          skos:definition "Indicates the maximum tensile stress a material can withstand along the direction of its fibers before breaking. This property is crucial for assessing the strength of fiber-reinforced materials, ensuring they can handle tensile loads effectively in the direction of fiber alignment."@en ;
                          skos:prefLabel "Tensão máxima de tração longitudinalmente às fibras"@pt-br ,
                                         "Ultimate Tensile Strength Along Fibers"@en ;
                          edo:hasTypedValue edo:floatValue ;
                          edo:hasValueCardinality edo:singleValue .


###  https://w3id.org/energy-domain/edo#UltTensStrPerpendFibers
edo:UltTensStrPerpendFibers rdf:type owl:Class ;
                            rdfs:subClassOf edo:DomainAttribute ;
                            dcterms:accessRights "PUBLIC" ;
                            dcterms:identifier "UltTensStrPerpendFibers" ;
                            skos:definition "Indicates the maximum tensile stress a material can withstand when applied perpendicular to the direction of its fibers before breaking. This property is important for evaluating the strength and durability of fiber-reinforced materials under tensile loads that are not aligned with the fibers, providing insights into their performance in various loading conditions."@en ;
                            skos:prefLabel "Tensão máxima de tração perpendicularmente às fibras"@pt-br ,
                                           "Ultimate Tensile Strength Perpendicular To Fibers"@en ;
                            edo:hasTypedValue edo:floatValue ;
                            edo:hasValueCardinality edo:singleValue .


###  https://w3id.org/energy-domain/edo#UltimateTensileStress
edo:UltimateTensileStress rdf:type owl:Class ;
                          rdfs:subClassOf edo:DomainAttribute ;
                          dcterms:accessRights "PUBLIC" ;
                          dcterms:identifier "UltimateTensileStress" ;
                          skos:definition "Indicates the maximum stress a material can withstand while being stretched or pulled before breaking. This property is essential for evaluating the material's strength and determining its ability to perform under tensile loads without failure."@en ,
                                          "Tensão máxima de tração (Específica para Materiais Metálicos)"@pt-br ;
                          skos:prefLabel "Tensão Máxima de Tração"@pt-br ,
                                         "Ultimate Tensile Stress"@en ;
                          edo:hasTypedValue edo:floatValue ;
                          edo:hasValueCardinality edo:singleValue .


###  https://w3id.org/energy-domain/edo#UnifilarDiagram
edo:UnifilarDiagram rdf:type owl:Class ;
                    rdfs:subClassOf edo:DomainAttribute ;
                    dcterms:accessRights "PUBLIC" ;
                    dcterms:identifier "UnifilarDiagram" ;
                    skos:definition "A simplified schematic illustrates the arrangement of flexible pipeline sections and their associated accessories, such as end fittings and clamps. This diagram shows how these sections and accessories are connected, providing a clear overview of the pipeline configuration without detailing internal structures. It is used to aid in planning, installation, and understanding of the flexible pipeline system by visualizing the main components and their positions."@en ;
                    skos:prefLabel "Código do Diagrama Unifilar"@pt-br ,
                                   "Unifilar Diagram"@en ;
                    edo:hasTypedValue edo:stringValue ;
                    edo:hasValueCardinality edo:singleValue .


###  https://w3id.org/energy-domain/edo#UnifilarDiagramRev
edo:UnifilarDiagramRev rdf:type owl:Class ;
                       rdfs:subClassOf edo:DomainAttribute ;
                       dcterms:accessRights "PUBLIC" ;
                       dcterms:identifier "UnifilarDiagramRev" ;
                       skos:definition "Indicates the revision number of the unifilar diagram, reflecting updates or changes made to the arrangement of pipeline sections and their accessories. Each revision ensures that the latest configuration is accurately documented for installation and planning purposes."@en ;
                       skos:prefLabel "Número da Revisão do Diagrama Unifilar"@pt-br ,
                                      "Unifilar Diagram Revision"@en ;
                       edo:hasTypedValue edo:stringValue ;
                       edo:hasValueCardinality edo:singleValue .


###  https://w3id.org/energy-domain/edo#UpperItubeDiameter
edo:UpperItubeDiameter rdf:type owl:Class ;
                       rdfs:subClassOf edo:DomainAttribute ;
                       dcterms:accessRights "PUBLIC" ;
                       dcterms:identifier "UpperItubeDiameter" ;
                       skos:definition "Diameter of the upper section of the tube or pipe. This measurement is important for ensuring proper fit and compatibility with other components or connections. The diameter of the upper section affects the alignment and sealing capabilities of the assembly, and ensures that the tube or pipe meets the design and operational requirements for the installation or application."@en ;
                       skos:prefLabel "Diâmetro do I-TUBE superior"@pt-br ,
                                      "Upper I-tube Diameter"@en ;
                       edo:hasTypedValue edo:floatValue ;
                       edo:hasValueCardinality edo:singleValue .


###  https://w3id.org/energy-domain/edo#Upstream
edo:Upstream rdf:type owl:Class ;
             rdfs:subClassOf edo:OilAndGas ;
             rdfs:label "Upstream"@en ,
                        "Upstream"@pt-br ;
             skos:definition "Oil & Gas sector covering exploration, drilling, and production of hydrocarbon resources."@en ,
                             "Setor de Petróleo & Gás que abrange exploração, perfuração e produção de recursos de hidrocarbonetos."@pt-br .


###  https://w3id.org/energy-domain/edo#UtilityPipingEngineering
edo:UtilityPipingEngineering rdf:type owl:Class ;
                             rdfs:subClassOf edo:TechnicalDiscipline ;
                             rdfs:label "Engenharia de Tubulação de Utilidades"@pt-br ,
                                        "Utility Piping Engineering"@en ;
                             skos:definition "Disciplina de engenharia focada no projeto de sistemas de tubulação para serviços de utilidades."@pt-br ,
                                             "Engineering discipline focused on the design of piping systems for utility services."@en .


###  https://w3id.org/energy-domain/edo#UtilizationFactor
edo:UtilizationFactor rdf:type owl:Class ;
                      rdfs:subClassOf edo:DomainAttribute ;
                      dcterms:accessRights "PUBLIC" ;
                      dcterms:identifier "UtilizationFactor" ;
                      skos:definition "Represents the ratio used to determine the level of utilisation, indicating how much of the system’s capacity is being used under given conditions. This factor is crucial for assessing whether the structure operates within safe limits or approaching its maximum capacity."@en ;
                      skos:prefLabel "Fator de Utilização"@pt-br ,
                                     "Utilization Factor"@en ;
                      edo:hasTypedValue edo:floatValue ;
                      edo:hasValueCardinality edo:singleValue .


###  https://w3id.org/energy-domain/edo#ValueCardinality
edo:ValueCardinality rdf:type owl:Class ;
                     rdfs:subClassOf edo:DomainAuxiliarClass ;
                     rdfs:comment "Superclass for constraints on the cardinality of values (single or multiple)."@en ;
                     rdfs:label "Value Cardinality"@en .


###  https://w3id.org/energy-domain/edo#Wind
edo:Wind rdf:type owl:Class ;
         rdfs:subClassOf edo:Renewable ;
         rdfs:label "Energia Eólica"@pt-br ,
                    "Wind Energy"@en ;
         skos:definition "Energia gerada a partir do vento usando turbinas e tecnologias relacionadas."@pt-br ,
                         "Energy generated from wind using turbines and related technologies."@en .


###  https://w3id.org/energy-domain/edo#WireLayer
edo:WireLayer rdf:type owl:Class ;
              rdfs:subClassOf edo:ArmourLayer ;
              dcterms:identifier "WireLayer" ;
              skos:definition "Basis for all wired layers."@en ;
              skos:prefLabel "Camada de Arame"@pt-br ,
                             "Wire Layer"@en .


###  https://w3id.org/energy-domain/edo#WireRopeQuantity
edo:WireRopeQuantity rdf:type owl:Class ;
                     rdfs:subClassOf edo:DomainAttribute ;
                     dcterms:accessRights "PUBLIC" ;
                     dcterms:identifier "WireRopeQuantity" ;
                     skos:definition "Indicates the number of wire ropes required or used for installation or operation"@en ;
                     skos:prefLabel "Quantidade de cordas de Aço"@pt-br ,
                                    "Wire Rope Quantity"@en ;
                     edo:hasTypedValue edo:intValue ;
                     edo:hasValueCardinality edo:singleValue .


###  https://w3id.org/energy-domain/edo#WireRopeSlingDiameter
edo:WireRopeSlingDiameter rdf:type owl:Class ;
                          rdfs:subClassOf edo:DomainAttribute ;
                          dcterms:accessRights "PUBLIC" ;
                          dcterms:identifier "WireRopeSlingDiameter" ;
                          skos:definition "Diâmetro do Estrobo de Corda de Aço"@pt-br ,
                                          "Specifies the diameter of the wire rope sling. This property provides the measurement of the thickness of the wire rope, which is important for determining its strength and load-bearing capacity."@en ;
                          skos:prefLabel "Diâmetro do Estrobo de Corda de Aço"@pt-br ,
                                         "Wire Rope Sling Diameter"@en ;
                          edo:hasTypedValue edo:floatValue ;
                          edo:hasValueCardinality edo:singleValue .


###  https://w3id.org/energy-domain/edo#WireRopeSlingLength
edo:WireRopeSlingLength rdf:type owl:Class ;
                        rdfs:subClassOf edo:DomainAttribute ;
                        dcterms:accessRights "PUBLIC" ;
                        dcterms:identifier "WireRopeSlingLength" ;
                        skos:definition "Specifies the length of the wire rope sling used in the installation or operation. This property provides the measurement of the sling’s length, which is essential for ensuring proper fit and functionality during use."@en ;
                        skos:prefLabel "Comprimento do Estrobo da Corda de Aço"@pt-br ,
                                       "Wire Rope Sling Length"@en ;
                        edo:hasTypedValue edo:floatValue ;
                        edo:hasValueCardinality edo:singleValue .


###  https://w3id.org/energy-domain/edo#WorkingLoadLimit
edo:WorkingLoadLimit rdf:type owl:Class ;
                     rdfs:subClassOf edo:DomainAttribute ;
                     dcterms:accessRights "PUBLIC" ;
                     dcterms:identifier "WorkingLoadLimit" ;
                     skos:definition "The Working Load Limit (WLL) refers to the maximum load that a component, such as a shackle, lifting device, or anchor, is designed to safely support under normal operating conditions."@en ;
                     skos:prefLabel "Limite de Carga de Trabalho"@pt-br ,
                                    "Working Load Limit (WLL)"@en ;
                     edo:hasTypedValue edo:floatValue ;
                     edo:hasValueCardinality edo:singleValue .


###  https://w3id.org/energy-domain/edo#WoundLayer
edo:WoundLayer rdf:type owl:Class ;
               rdfs:subClassOf edo:FlexibleStructureLayer ;
               dcterms:identifier "WoundLayer" ;
               skos:definition "Basis for all layers constructed by helical winding of one or more elements."@en ;
               skos:prefLabel "Camada Espiralada"@pt-br ,
                              "Wound Layer"@en .


###  https://w3id.org/energy-domain/edo#anyURIType
edo:anyURIType rdf:type owl:Class ;
               owl:equivalentClass [ rdf:type owl:Restriction ;
                                     owl:onProperty rdf:value ;
                                     owl:allValuesFrom xsd:anyURI
                                   ] ;
               rdfs:subClassOf edo:TypedValue ;
               rdfs:comment "Constraint for xsd:anyURI (URIs/IRIs)"@en ;
               rdfs:label "URI Value"@en .


###  https://w3id.org/energy-domain/edo#base64BinaryType
edo:base64BinaryType rdf:type owl:Class ;
                     owl:equivalentClass [ rdf:type owl:Restriction ;
                                           owl:onProperty rdf:value ;
                                           owl:allValuesFrom xsd:base64Binary
                                         ] ;
                     rdfs:subClassOf edo:TypedValue ;
                     rdfs:comment "Constraint for xsd:base64Binary (binary data)"@en ;
                     rdfs:label "Base64 Binary"@en .


###  https://w3id.org/energy-domain/edo#booleanValue
edo:booleanValue rdf:type owl:Class ;
                 owl:equivalentClass [ rdf:type owl:Restriction ;
                                       owl:onProperty rdf:value ;
                                       owl:allValuesFrom xsd:boolean
                                     ] ;
                 rdfs:subClassOf edo:TypedValue ;
                 rdfs:comment "Constraint for xsd:boolean (true/false)"@en ;
                 rdfs:label "Boolean Value"@en .


###  https://w3id.org/energy-domain/edo#dateTimeValue
edo:dateTimeValue rdf:type owl:Class ;
                  owl:equivalentClass [ rdf:type owl:Restriction ;
                                        owl:onProperty rdf:value ;
                                        owl:allValuesFrom xsd:dateTime
                                      ] ;
                  rdfs:subClassOf edo:TypedValue ;
                  rdfs:comment "Constraint for xsd:dateTime (timestamps)"@en ;
                  rdfs:label "DateTime Value"@en .


###  https://w3id.org/energy-domain/edo#dateValue
edo:dateValue rdf:type owl:Class ;
              owl:equivalentClass [ rdf:type owl:Restriction ;
                                    owl:onProperty rdf:value ;
                                    owl:allValuesFrom xsd:date
                                  ] ;
              rdfs:subClassOf edo:TypedValue ;
              rdfs:comment "Constraint for xsd:date (calendar dates)"@en ;
              rdfs:label "Date Value"@en .


###  https://w3id.org/energy-domain/edo#decimalValue
edo:decimalValue rdf:type owl:Class ;
                 owl:equivalentClass [ rdf:type owl:Restriction ;
                                       owl:onProperty rdf:value ;
                                       owl:allValuesFrom xsd:decimal
                                     ] ;
                 rdfs:subClassOf edo:TypedValue ;
                 rdfs:comment "Constraint for xsd:decimal (arbitrary precision numbers)"@en ;
                 rdfs:label "Decimal Value"@en .


###  https://w3id.org/energy-domain/edo#doubleValue
edo:doubleValue rdf:type owl:Class ;
                owl:equivalentClass [ rdf:type owl:Restriction ;
                                      owl:onProperty rdf:value ;
                                      owl:allValuesFrom xsd:double
                                    ] ;
                rdfs:subClassOf edo:TypedValue ;
                rdfs:comment "Constraint for xsd:double (64-bit floating point)"@en ;
                rdfs:label "Double Value"@en .


###  https://w3id.org/energy-domain/edo#floatValue
edo:floatValue rdf:type owl:Class ;
               owl:equivalentClass [ rdf:type owl:Restriction ;
                                     owl:onProperty rdf:value ;
                                     owl:allValuesFrom xsd:float
                                   ] ;
               rdfs:subClassOf edo:TypedValue ;
               rdfs:comment "Constraint for xsd:float (32-bit floating point)"@en ;
               rdfs:label "Float Value"@en .


###  https://w3id.org/energy-domain/edo#intValue
edo:intValue rdf:type owl:Class ;
             owl:equivalentClass [ rdf:type owl:Restriction ;
                                   owl:onProperty rdf:value ;
                                   owl:allValuesFrom xsd:int
                                 ] ;
             rdfs:subClassOf edo:TypedValue ;
             rdfs:comment "Constraint for xsd:int (32-bit integer)"@en ;
             rdfs:label "Integer Value"@en .


###  https://w3id.org/energy-domain/edo#longValue
edo:longValue rdf:type owl:Class ;
              owl:equivalentClass [ rdf:type owl:Restriction ;
                                    owl:onProperty rdf:value ;
                                    owl:allValuesFrom xsd:long
                                  ] ;
              rdfs:subClassOf edo:TypedValue ;
              rdfs:comment "Constraint for xsd:long (64-bit integer)"@en ;
              rdfs:label "Long Value"@en .


###  https://w3id.org/energy-domain/edo#multiValue
edo:multiValue rdf:type owl:Class ;
               rdfs:subClassOf edo:ValueCardinality ;
               rdfs:comment "Constraint allowing multiple values (RDF list)"@en ;
               rdfs:label "Multiple Values"@en .


###  https://w3id.org/energy-domain/edo#singleValue
edo:singleValue rdf:type owl:Class ;
                rdfs:subClassOf edo:ValueCardinality ;
                rdfs:comment "Constraint ensuring only one value (not a list)"@en ;
                rdfs:label "Single Value"@en .


###  https://w3id.org/energy-domain/edo#stringValue
edo:stringValue rdf:type owl:Class ;
                owl:equivalentClass [ rdf:type owl:Restriction ;
                                      owl:onProperty rdf:value ;
                                      owl:allValuesFrom xsd:string
                                    ] ;
                rdfs:subClassOf edo:TypedValue ;
                rdfs:comment "Constraint for xsd:string (character strings)"@en ;
                rdfs:label "String Value"@en .


###  https://w3id.org/energy-domain/edo#timeValue
edo:timeValue rdf:type owl:Class ;
              owl:equivalentClass [ rdf:type owl:Restriction ;
                                    owl:onProperty rdf:value ;
                                    owl:allValuesFrom xsd:time
                                  ] ;
              rdfs:subClassOf edo:TypedValue ;
              rdfs:comment "Constraint for xsd:time (time of day)"@en ;
              rdfs:label "Time Value"@en .


###  Generated by the OWL API (version 4.5.29.2024-05-13T12:11:03Z) https://github.com/owlcs/owlapi
